<?xml version="1.0"?>
<rdf:RDF xmlns="https://w3id.org/italia/social-security/onto/core/"
     xml:base="https://w3id.org/italia/social-security/onto/core/"
     xmlns:L0="https://w3id.org/italia/onto/l0/"
     xmlns:owl="http://www.w3.org/2002/07/owl#"
     xmlns:swrlb="http://www.w3.org/2003/11/swrlb#"
     xmlns:CPV="https://w3id.org/italia/onto/CPV/"
     xmlns:swrl="http://www.w3.org/2003/11/swrl#"
     xmlns:xsd="http://www.w3.org/2001/XMLSchema#"
     xmlns:skos="http://www.w3.org/2004/02/skos/core#"
     xmlns:rdfs="http://www.w3.org/2000/01/rdf-schema#"
     xmlns:COV="https://w3id.org/italia/onto/COV/"
     xmlns:CLV="https://w3id.org/italia/onto/CLV/"
     xmlns:rdf="http://www.w3.org/1999/02/22-rdf-syntax-ns#"
	 xmlns:dct="http://purl.org/dc/terms/"
	 xmlns:dcatapit="http://dati.gov.it/onto/dcatapit#"
	 xmlns:foaf="http://xmlns.com/foaf/0.1/"
	 xmlns:dcat="http://www.w3.org/ns/dcat#"
	 xmlns:adms="https://w3id.org/italia/onto/ADMS/"
	 xmlns:vcard="http://www.w3.org/2006/vcard/ns#"
     xmlns:TI="https://w3id.org/italia/onto/TI/"
     xmlns:INPSCore="https://w3id.org/italia/social-security/onto/core/"
     xmlns:xml="http://www.w3.org/XML/1998/namespace"
     xmlns:time="http://www.w3.org/2006/time#"
     xmlns:RO="https://w3id.org/italia/onto/RO/">
    <owl:Ontology rdf:about="https://w3id.org/italia/social-security/onto/core/">
    <owl:versionIRI rdf:resource="https://w3id.org/italia/social-security/onto/core/1.0"/>
    <owl:imports rdf:resource="https://w3id.org/italia/onto/CLV/"/>
    <owl:imports rdf:resource="https://w3id.org/italia/onto/COV/"/>
    <owl:imports rdf:resource="https://w3id.org/italia/onto/CPV/"/>
    <owl:imports rdf:resource="https://w3id.org/italia/onto/l0/"/>
    <owl:imports rdf:resource="https://w3id.org/italia/onto/RO/"/>
    <dct:title xml:lang="it">Ontologia Core di INPS </dct:title>
    <dct:title xml:lang="en">Core INPS Ontology</dct:title>
    <adms:last rdf:resource="https://w3id.org/italia/social-security/onto/core/1.0"/>
    <dcat:keyword xml:lang="it">Persona</dcat:keyword>
    <dcat:keyword xml:lang="it">Agente</dcat:keyword>
    <dcat:keyword xml:lang="it">Sede INPS</dcat:keyword>
    <dcat:keyword xml:lang="it">Organizzazione</dcat:keyword>
    <dcat:keyword xml:lang="en">Person</dcat:keyword>
    <dcat:keyword xml:lang="en">Agent</dcat:keyword>
    <dcat:keyword xml:lang="en">INPS Office</dcat:keyword>
    <dcat:keyword xml:lang="en">Organization</dcat:keyword>
	<rdfs:comment xml:lang="it">Ontologia INPS relativa alle componenti del dominio funzionale dell'istituto comuni a procedure e servizi svolti dall'ente stesso. Tra di essi troviamo, ad esempio, le dislocazioni territoriali, come le sedi, e le entità astratte, come i ruoli.</rdfs:comment>
	<rdfs:comment xml:lang="en">This is the ontology of the INPS Organization about components of the institution's functional domain common to procedures and services performed by the institution itself. These include, for example, territorial dislocations, such as locations, and abstract entities, such as roles.</rdfs:comment>
    <adms:target xml:lang="it">Cittadini</adms:target>
    <adms:target xml:lang="it">Imprese</adms:target>
    <adms:target xml:lang="it">Pubbliche Amministrazioni</adms:target>
    <dcat:contactPoint rdf:resource="https://w3id.org/italia/social-security/data/organization/DirezioneCentraleTII"/>
    <dct:creator rdf:resource="https://w3id.org/italia/social-security/data/organization/inps"/>
    <dct:issued rdf:datatype="http://www.w3.org/2001/XMLSchema#dateTime">2024-01-16T00:00:00Z</dct:issued>
    <adms:type rdf:resource="https://w3id.org/italia/onto/ADMS/ServiceOnytology"/>
    <adms:hasSemanticAssetDistribution rdf:resource="https://w3id.org/italia/social-security/data/core/distribution/CORE-RDF-TURTLE"/>
    <adms:hasSemanticAssetDistribution rdf:resource="https://w3id.org/italia/social-security/data/core/distribution/CORE-RDF-XML"/>
    <adms:hasSemanticAssetDistribution rdf:resource="https://w3id.org/italia/social-security/data/core/distribution/CORE-N-TRIPLES"/>
    <rdfs:isDefinedBy rdf:resource="https://w3id.org/italia/social-security/onto/core/"/>
    <dct:modified rdf:datatype="http://www.w3.org/2001/XMLSchema#dateTime">2024-01-17T00:00:00Z</dct:modified>
    <rdfs:label xml:lang="it">Ontologia Core di INPS</rdfs:label>
    <rdfs:label xml:lang="en">Core INPS Ontology</rdfs:label>
    <adms:hasKeyClass rdf:resource="https://w3id.org/italia/social-security/onto/core/SedeINPS"/>
    <adms:hasKeyClass rdf:resource="https://w3id.org/italia/social-security/onto/core/RuoloDiAgente"/>
    <adms:hasKeyClass rdf:resource="https://w3id.org/italia/social-security/onto/core/RuoloDiOrganizzazione"/>
    <adms:hasKeyClass rdf:resource="https://w3id.org/italia/social-security/onto/core/RuoloDiPersona"/>
    <adms:semanticAssetInUse rdf:resource="https://w3id.org/italia/data/project/NDC"/>
    <adms:hasTask rdf:resource="https://w3id.org/italia/onto/ADMS/AnnotationTask"/>
    <adms:hasTask rdf:resource="https://w3id.org/italia/onto/ADMS/QueryFormulationTask"/>
    <adms:hasTask rdf:resource="https://w3id.org/italia/onto/ADMS/SearchTask"/>
    <adms:status>catalogued</adms:status>
    <adms:status>published</adms:status>
    <dct:accrualPeriodicity rdf:resource="http://publications.europa.eu/resource/authority/frequency/IRREG"/>
    <dct:rightsHolder rdf:resource="https://w3id.org/italia/social-security/data/organization/DirezioneCentraleTII"/>
    <adms:hasContributor rdf:resource="https://w3id.org/italia/social-security/data/organization/td"/>
    <owl:versionInfo xml:lang="it">Versione 1.0 - Modificata il 17 Gennaio 2024</owl:versionInfo>
    <owl:versionInfo xml:lang="en">Version 1.0 - Modified on 17 January 2024</owl:versionInfo>
    <adms:hasOntologyLanguage rdf:resource="https://w3id.org/italia/onto/ADMS/OWL"/>
    <adms:hasFormalityLevel rdf:resource="https://w3id.org/italia/onto/ADMS/Formal"/>
    <dcat:theme rdf:resource="http://publications.europa.eu/resource/authority/data-theme/SOCI"/>
    <dct:publisher rdf:resource="https://w3id.org/italia/social-security/data/organization/DirezioneCentraleTII"/>
    <adms:officialURI rdf:datatype="http://www.w3.org/2001/XMLSchema#anyURI">https://w3id.org/italia/social-security/onto/core</adms:officialURI>
    <dct:language rdf:resource="http://publications.europa.eu/resource/authority/language/ENG"/>
    <dct:language rdf:resource="http://publications.europa.eu/resource/authority/language/ITA"/>
    <adms:acronym>inps</adms:acronym>
	<dct:description xml:lang="it">Ontologia INPS relativa alle componenti del dominio funzionale dell'istituto comuni a procedure e servizi svolti dall'ente stesso. Tra di essi troviamo, ad esempio, le dislocazioni territoriali, come le sedi, e le entità astratte, come i ruoli.</dct:description>
	<dct:description xml:lang="en">This is the ontology of the INPS Organization about components of the institution's functional domain common to procedures and services performed by the institution itself. These include, for example, territorial dislocations, such as locations, and abstract entities, such as roles.</dct:description>
    <dct:identifier>https://w3id.org/italia/social-security/onto/core</dct:identifier>
    <adms:prefix>inpsc</adms:prefix>
  </owl:Ontology>



    <!--
    ///////////////////////////////////////////////////////////////////////////////////////
    //
    // Datatypes
    //
    ///////////////////////////////////////////////////////////////////////////////////////
     -->




    <!-- http://www.w3.org/2001/XMLSchema#string -->

    <rdfs:Datatype rdf:about="http://www.w3.org/2001/XMLSchema#string"/>



    <!--
    ///////////////////////////////////////////////////////////////////////////////////////
    //
    // Object Properties
    //
    ///////////////////////////////////////////////////////////////////////////////////////
     -->




    <!-- https://w3id.org/italia/onto/CLV/hasAddress -->

    <owl:ObjectProperty rdf:about="https://w3id.org/italia/onto/CLV/hasAddress">
        <rdf:type rdf:resource="http://www.w3.org/2002/07/owl#FunctionalProperty"/>
    </owl:ObjectProperty>



    <!-- https://w3id.org/italia/onto/CLV/hasAddressComponent -->

    <owl:ObjectProperty rdf:about="https://w3id.org/italia/onto/CLV/hasAddressComponent"/>



    <!-- https://w3id.org/italia/onto/CLV/hasPrimaryAddress -->

    <owl:ObjectProperty rdf:about="https://w3id.org/italia/onto/CLV/hasPrimaryAddress"/>



    <!-- https://w3id.org/italia/onto/COV/hasOrganizzation -->

    <owl:ObjectProperty rdf:about="https://w3id.org/italia/onto/COV/hasOrganizzation">
        <rdf:type rdf:resource="http://www.w3.org/2002/07/owl#FunctionalProperty"/>
        <rdfs:domain rdf:resource="https://w3id.org/italia/social-security/onto/core/SedeINPS"/>
        <rdfs:range rdf:resource="https://w3id.org/italia/onto/COV/PublicOrganization"/>
    </owl:ObjectProperty>



    <!-- https://w3id.org/italia/onto/CPV/hasCurrentResidence -->

    <owl:ObjectProperty rdf:about="https://w3id.org/italia/onto/CPV/hasCurrentResidence"/>



    <!-- https://w3id.org/italia/onto/RO/holdsRoleInTime -->

    <owl:ObjectProperty rdf:about="https://w3id.org/italia/onto/RO/holdsRoleInTime"/>



    <!-- https://w3id.org/italia/social-security/onto/core/haSedeINPS -->

    <owl:ObjectProperty rdf:about="https://w3id.org/italia/social-security/onto/core/haSedeINPS">
        <rdf:type rdf:resource="http://www.w3.org/2002/07/owl#FunctionalProperty"/>
        <rdfs:domain>
            <owl:Class>
                <owl:unionOf rdf:parseType="Collection">
                    <rdf:Description rdf:about="https://w3id.org/italia/onto/COV/Organization"/>
                    <rdf:Description rdf:about="https://w3id.org/italia/onto/CPV/Alive"/>
                </owl:unionOf>
            </owl:Class>
        </rdfs:domain>
        <rdfs:range rdf:resource="https://w3id.org/italia/social-security/onto/core/SedeINPS"/>
        <rdfs:comment xml:lang="en">Relationship linking a Living Person or an Organization to an INPS Office. Each Living Person or Organization has a single INPS office.</rdfs:comment>
        <rdfs:comment xml:lang="it">Relazione che collega una Persona in Vita o un&apos;Organizzazione ad una Sede INPS. Ciascuna Persona in Vita o Organizzazione ha un&apos;unica Sede INPS.</rdfs:comment>
        <rdfs:label xml:lang="it">ha sede INPS</rdfs:label>
        <rdfs:label xml:lang="en">has INPS office</rdfs:label>
    </owl:ObjectProperty>



    <!--
    ///////////////////////////////////////////////////////////////////////////////////////
    //
    // Data properties
    //
    ///////////////////////////////////////////////////////////////////////////////////////
     -->




    <!-- https://w3id.org/italia/social-security/onto/core/codiceSedeINPS -->

    <owl:DatatypeProperty rdf:about="https://w3id.org/italia/social-security/onto/core/codiceSedeINPS">
        <rdf:type rdf:resource="http://www.w3.org/2002/07/owl#FunctionalProperty"/>
        <rdfs:domain rdf:resource="https://w3id.org/italia/social-security/onto/core/SedeINPS"/>
        <rdfs:range rdf:resource="http://www.w3.org/2001/XMLSchema#string"/>
        <rdfs:comment xml:lang="en">INPS office identification code</rdfs:comment>
        <rdfs:comment xml:lang="en">This is the identification code of the INPS office.</rdfs:comment>
        <rdfs:comment xml:lang="it">È il codice relativo alla Sede INPS.</rdfs:comment>
        <rdfs:label xml:lang="it">codice sede INPS</rdfs:label>
    </owl:DatatypeProperty>



    <!--
    ///////////////////////////////////////////////////////////////////////////////////////
    //
    // Classes
    //
    ///////////////////////////////////////////////////////////////////////////////////////
     -->




    <!-- https://w3id.org/italia/onto/COV/HomogeneousOrganizationalArea -->

    <owl:Class rdf:about="https://w3id.org/italia/onto/COV/HomogeneousOrganizationalArea"/>



    <!-- https://w3id.org/italia/onto/COV/Organization -->

    <owl:Class rdf:about="https://w3id.org/italia/onto/COV/Organization">
        <rdfs:subClassOf>
            <owl:Restriction>
                <owl:onProperty rdf:resource="https://w3id.org/italia/social-security/onto/core/haSedeINPS"/>
                <owl:someValuesFrom rdf:resource="http://www.w3.org/2002/07/owl#Thing"/>
            </owl:Restriction>
        </rdfs:subClassOf>
        <owl:disjointWith rdf:resource="https://w3id.org/italia/onto/CPV/Person"/>
    </owl:Class>



    <!-- https://w3id.org/italia/onto/COV/PublicOrganization -->

    <owl:Class rdf:about="https://w3id.org/italia/onto/COV/PublicOrganization">
        <owl:equivalentClass>
            <owl:Restriction>
                <owl:onProperty>
                    <rdf:Description>
                        <owl:inverseOf rdf:resource="https://w3id.org/italia/onto/COV/hasOrganizzation"/>
                    </rdf:Description>
                </owl:onProperty>
                <owl:someValuesFrom rdf:resource="http://www.w3.org/2002/07/owl#Thing"/>
            </owl:Restriction>
        </owl:equivalentClass>
    </owl:Class>



    <!-- https://w3id.org/italia/onto/CPV/Alive -->

    <owl:Class rdf:about="https://w3id.org/italia/onto/CPV/Alive">
        <rdfs:subClassOf>
            <owl:Restriction>
                <owl:onProperty rdf:resource="https://w3id.org/italia/social-security/onto/core/haSedeINPS"/>
                <owl:someValuesFrom rdf:resource="http://www.w3.org/2002/07/owl#Thing"/>
            </owl:Restriction>
        </rdfs:subClassOf>
        <owl:disjointWith rdf:resource="https://w3id.org/italia/onto/CPV/Dead"/>
    </owl:Class>



    <!-- https://w3id.org/italia/onto/CPV/Dead -->

    <owl:Class rdf:about="https://w3id.org/italia/onto/CPV/Dead"/>



    <!-- https://w3id.org/italia/onto/CPV/Person -->

    <owl:Class rdf:about="https://w3id.org/italia/onto/CPV/Person"/>



    <!-- https://w3id.org/italia/onto/l0/Agent -->

    <owl:Class rdf:about="https://w3id.org/italia/onto/l0/Agent"/>



    <!-- https://w3id.org/italia/social-security/onto/core/RuoloDiAgente -->

    <owl:Class rdf:about="https://w3id.org/italia/social-security/onto/core/RuoloDiAgente">
        <owl:equivalentClass>
            <owl:Restriction>
                <owl:onProperty>
                    <rdf:Description>
                        <owl:inverseOf rdf:resource="https://w3id.org/italia/onto/RO/holdsRoleInTime"/>
                    </rdf:Description>
                </owl:onProperty>
                <owl:someValuesFrom>
                    <owl:Class>
                        <owl:unionOf rdf:parseType="Collection">
                            <rdf:Description rdf:about="https://w3id.org/italia/onto/COV/Organization"/>
                            <rdf:Description rdf:about="https://w3id.org/italia/onto/CPV/Person"/>
                        </owl:unionOf>
                    </owl:Class>
                </owl:someValuesFrom>
            </owl:Restriction>
        </owl:equivalentClass>
        <rdfs:comment xml:lang="it">Insieme di mansioni, compiti, responsabilità e doveri attribuiti in un intervallo di tempo, anche non ancora terminato, a una persona o a una organizzazione considerando queste ultime specializzazioni di agente. </rdfs:comment>
        <rdfs:comment xml:lang="en">Set of tasks, duties and responsabilities attributed in a certain time interval, possible not yet determined, to a person or organization, considering these as specializations of an agent. </rdfs:comment>
        <rdfs:label xml:lang="en">Agent Role</rdfs:label>
        <rdfs:label xml:lang="it">Ruolo Di Agente</rdfs:label>
    </owl:Class>



    <!-- https://w3id.org/italia/social-security/onto/core/RuoloDiOrganizzazione -->

    <owl:Class rdf:about="https://w3id.org/italia/social-security/onto/core/RuoloDiOrganizzazione">
        <owl:equivalentClass>
            <owl:Restriction>
                <owl:onProperty>
                    <rdf:Description>
                        <owl:inverseOf rdf:resource="https://w3id.org/italia/onto/RO/holdsRoleInTime"/>
                    </rdf:Description>
                </owl:onProperty>
                <owl:someValuesFrom rdf:resource="https://w3id.org/italia/onto/COV/Organization"/>
            </owl:Restriction>
        </owl:equivalentClass>
        <owl:disjointWith rdf:resource="https://w3id.org/italia/social-security/onto/core/RuoloDiPersona"/>
        <rdfs:comment xml:lang="it">Specializzazione della classe Ruolo Di Agente limitata alle sole organizzazioni.</rdfs:comment>
        <rdfs:comment xml:lang="en">Subclass of the Agent Role class, limited to organization.</rdfs:comment>
        <rdfs:label xml:lang="en">Organization Role</rdfs:label>
        <rdfs:label xml:lang="it">Ruolo Di Organizzazione</rdfs:label>
    </owl:Class>



    <!-- https://w3id.org/italia/social-security/onto/core/RuoloDiPersona -->

    <owl:Class rdf:about="https://w3id.org/italia/social-security/onto/core/RuoloDiPersona">
        <owl:equivalentClass>
            <owl:Restriction>
                <owl:onProperty>
                    <rdf:Description>
                        <owl:inverseOf rdf:resource="https://w3id.org/italia/onto/RO/holdsRoleInTime"/>
                    </rdf:Description>
                </owl:onProperty>
                <owl:someValuesFrom rdf:resource="https://w3id.org/italia/onto/CPV/Person"/>
            </owl:Restriction>
        </owl:equivalentClass>
        <rdfs:comment xml:lang="it">Specializzazione della classe Ruolo Di Agente limitata alle sole persone, in vita o decedute.</rdfs:comment>
        <rdfs:comment xml:lang="en">Subclass of the Agent Role class, limited to people, living or deceased.</rdfs:comment>
        <rdfs:label xml:lang="en">Person Role</rdfs:label>
        <rdfs:label xml:lang="it">Ruolo Di Persona</rdfs:label>
    </owl:Class>



    <!-- https://w3id.org/italia/social-security/onto/core/RuoloDiPersonaDeceduta -->

    <owl:Class rdf:about="https://w3id.org/italia/social-security/onto/core/RuoloDiPersonaDeceduta">
        <owl:equivalentClass>
            <owl:Restriction>
                <owl:onProperty>
                    <rdf:Description>
                        <owl:inverseOf rdf:resource="https://w3id.org/italia/onto/RO/holdsRoleInTime"/>
                    </rdf:Description>
                </owl:onProperty>
                <owl:someValuesFrom rdf:resource="https://w3id.org/italia/onto/CPV/Dead"/>
            </owl:Restriction>
        </owl:equivalentClass>
        <owl:disjointWith rdf:resource="https://w3id.org/italia/social-security/onto/core/RuoloDiPersonaViva"/>
        <rdfs:comment xml:lang="it">Specializzazione della classe Ruolo Di Persona limitata alle sole persone decedute.</rdfs:comment>
        <rdfs:comment xml:lang="en">Subclass of the Person Role class, limited to only dead persons.</rdfs:comment>
        <rdfs:label xml:lang="en">Dead Person Role</rdfs:label>
        <rdfs:label xml:lang="it">Ruolo Di Persona Deceduta</rdfs:label>
    </owl:Class>



    <!-- https://w3id.org/italia/social-security/onto/core/RuoloDiPersonaViva -->

    <owl:Class rdf:about="https://w3id.org/italia/social-security/onto/core/RuoloDiPersonaViva">
        <owl:equivalentClass>
            <owl:Restriction>
                <owl:onProperty>
                    <rdf:Description>
                        <owl:inverseOf rdf:resource="https://w3id.org/italia/onto/RO/holdsRoleInTime"/>
                    </rdf:Description>
                </owl:onProperty>
                <owl:someValuesFrom rdf:resource="https://w3id.org/italia/onto/CPV/Alive"/>
            </owl:Restriction>
        </owl:equivalentClass>
        <rdfs:comment xml:lang="it">Specializzazione della classe Ruolo Di Persona limitata alle sole persone in vita.</rdfs:comment>
        <rdfs:comment xml:lang="en">Subclass of the Person Role class, limited to only alive persons.</rdfs:comment>
        <rdfs:label xml:lang="en">Alive Person Role</rdfs:label>
        <rdfs:label xml:lang="it">Ruolo Di Persona Viva</rdfs:label>
    </owl:Class>



    <!-- https://w3id.org/italia/social-security/onto/core/SedeINPS -->

    <owl:Class rdf:about="https://w3id.org/italia/social-security/onto/core/SedeINPS">
        <owl:equivalentClass>
            <owl:Restriction>
                <owl:onProperty rdf:resource="https://w3id.org/italia/onto/COV/hasOrganizzation"/>
                <owl:someValuesFrom rdf:resource="http://www.w3.org/2002/07/owl#Thing"/>
            </owl:Restriction>
        </owl:equivalentClass>
        <owl:equivalentClass>
            <owl:Restriction>
                <owl:onProperty rdf:resource="https://w3id.org/italia/social-security/onto/core/codiceSedeINPS"/>
                <owl:someValuesFrom rdf:resource="http://www.w3.org/2000/01/rdf-schema#Literal"/>
            </owl:Restriction>
        </owl:equivalentClass>
        <rdfs:subClassOf rdf:resource="https://w3id.org/italia/onto/COV/HomogeneousOrganizationalArea"/>
        <rdfs:comment xml:lang="en">INPS is divided into central, regional and metropolitan structures with guidance, monitoring and coordination tasks, and into territorial offices with operational and user contact functions. In particular, the Institute, throughout the Italian national territory, has set up a &quot;service network&quot; organization which, in a &quot;proximity&quot; logic, is divided into: metropolitan coordination structures, provincial level structures, regional structures. Each INPS office is similar to a Homogeneous Organizational Area (AOO), each benefiting from a single entry and/or exit document flow (IT Protocol service) for the provision of services and the receipt of requests. In this sense, each INPS office is assigned, in addition to an office code assigned by the Institute, also a unique AOO identification code within the Index of Public Administrations (IPA) which makes it possible to identify the telematic communication channels legally permitted that is, at least one certified mailbox for each AOO. The competent INPS office for a citizen and/or company is established on the basis of the citizen&apos;s residence and/or the address of the company headquarters.</rdfs:comment>
        <rdfs:comment xml:lang="it">L’INPS è articolato in strutture centrali, regionali e metropolitane con compiti di indirizzo, monitoraggio e coordinamento, e in sedi territoriali con funzioni operative e di contatto con l’utenza. In particolare, l’Istituto, su tutto il territorio nazionale italiano, si è dotato di un’organizzazione “a reti di servizio” che, in logica di “prossimità”, si suddivide in: strutture di coordinamento metropolitano, strutture a livello provinciale, strutture a livello regionale. Ogni sede INPS è assimilabile ad un Area Organizzativa Omogenea (AOO) usufruendo ciascuna per l&apos;erogazione di servizi e il ricevimento delle richieste, di un unico flusso documentale di entrata e/o uscita (servizio di Protocollo Informatico). In tal senso ad ogni Sede INPS è assegnato, oltre ad un codice di sede attribuito dall&apos;Istituto, anche un codice identificativo AOO univoco nell&apos;ambito dell&apos;Indice delle Pubbliche Amministrazioni (IPA) che permette di individuare i canali di comunicazione telematica normativamente pervisti e cioè almeno una casella di posta elettronica certificata per ciascun AOO. La sede INPS competente per un cittadino e/o un&apos;impresa è stabilita in base alla residenza del cittadino e/o all&apos;indirizzo della sede dell&apos;impresa.</rdfs:comment>
        <rdfs:label xml:lang="en">INPS Office</rdfs:label>
        <rdfs:label xml:lang="it">Sede INPS</rdfs:label>
    </owl:Class>



    <!--
    ///////////////////////////////////////////////////////////////////////////////////////
    //
    // Individuals
    //
    ///////////////////////////////////////////////////////////////////////////////////////
     -->

    <!-- https://w3id.org/italia/social-security/data/core/distribution/CORE-N-TRIPLES -->

    <rdf:Description rdf:about="https://w3id.org/italia/social-security/data/core/distribution/CORE-N-TRIPLES">
      <rdf:type rdf:resource="https://w3id.org/italia/onto/ADMS/SemanticAssetDistribution"/>
      <rdf:type rdf:resource="http://www.w3.org/ns/dcat#Distribution"/>
      <rdf:type rdf:resource="http://dati.gov.it/onto/dcatapit#Distribution"/>
      <rdf:type rdf:resource="http://www.w3.org/2002/07/owl#NamedIndividual"/>
      <dcat:accessURL rdf:resource="https://github.com/INPS-it/NDC/tree/main/assets/ontologies/core/latest"/>
      <dcat:downloadURL rdf:resource="https://raw.githubusercontent.com/INPS-it/NDC/main/assets/ontologies/core/latest/core.n3"/>
      <dct:description xml:lang="it">Questa è la distribuzione N-TRIPLES dell'ontologia INPS relativa alle componenti del dominio funzionale dell'istituto comuni a procedure e servizi svolti dall'ente stesso. Tra di essi troviamo, ad esempio, le dislocazioni territoriali, come le sedi, e le entità astratte, come i ruoli.</dct:description>
      <dct:description xml:lang="en">This is the distribution in N-TRIPLES of the INPS Ontology about components of the institution's functional domain common to procedures and services performed by the institution itself. These include, for example, territorial dislocations, such as locations, and abstract entities, such as roles.</dct:description>
      <dct:format rdf:resource="http://publications.europa.eu/resource/authority/file-type/RDF_N_TRIPLES"/>
      <dct:license rdf:resource="http://creativecommons.org/licenses/by/4.0/"/>
      <dct:title xml:lang="it">Distribuzione N-TRIPLES dell'ontologia INPS - Core</dct:title>
      <dct:title xml:lang="en">N-TRIPLES distribution of the INPS ontology - Core</dct:title>
    </rdf:Description>

    <!-- https://w3id.org/italia/social-security/data/core/distribution/CORE-RDF-TURTLE -->

    <rdf:Description rdf:about="https://w3id.org/italia/social-security/data/core/distribution/CORE-RDF-TURTLE">
      <rdf:type rdf:resource="https://w3id.org/italia/onto/ADMS/SemanticAssetDistribution"/>
      <rdf:type rdf:resource="http://www.w3.org/ns/dcat#Distribution"/>
      <rdf:type rdf:resource="http://dati.gov.it/onto/dcatapit#Distribution"/>
      <rdf:type rdf:resource="http://www.w3.org/2002/07/owl#NamedIndividual"/>
      <dcat:accessURL rdf:resource="https://github.com/INPS-it/NDC/tree/main/assets/ontologies/core/latest"/>
      <dcat:downloadURL rdf:resource="https://raw.githubusercontent.com/INPS-it/NDC/main/assets/ontologies/core/latest/core.ttl"/>
      <dct:description xml:lang="it">Questa è la distribuzione RDF/Turtle dell'ontologia INPS relativa alle componenti del dominio funzionale dell'istituto comuni a procedure e servizi svolti dall'ente stesso. Tra di essi troviamo, ad esempio, le dislocazioni territoriali, come le sedi, e le entità astratte, come i ruoli.</dct:description>
      <dct:description xml:lang="en">This is the distribution in RDF/Turtle of the INPS Ontology about components of the institution's functional domain common to procedures and services performed by the institution itself. These include, for example, territorial dislocations, such as locations, and abstract entities, such as roles.</dct:description>
      <dct:format rdf:resource="http://publications.europa.eu/resource/authority/file-type/RDF_TURTLE"/>
      <dct:license rdf:resource="http://creativecommons.org/licenses/by/4.0/"/>
      <dct:title xml:lang="it">Distribuzione RDF/Turtle dell'ontologia INPS - Core</dct:title>
      <dct:title xml:lang="en">RDF/Turtle distribution of the INPS ontology - Core</dct:title>
    </rdf:Description>

    <!-- https://w3id.org/italia/social-security/data/core/distribution/CORE-RDF-XML -->

    <rdf:Description rdf:about="https://w3id.org/italia/social-security/data/core/distribution/CORE-RDF-XML">
      <rdf:type rdf:resource="https://w3id.org/italia/onto/ADMS/SemanticAssetDistribution"/>
      <rdf:type rdf:resource="http://www.w3.org/ns/dcat#Distribution"/>
      <rdf:type rdf:resource="http://dati.gov.it/onto/dcatapit#Distribution"/>
      <rdf:type rdf:resource="http://www.w3.org/2002/07/owl#NamedIndividual"/>
      <dcat:accessURL rdf:resource="https://github.com/INPS-it/NDC/tree/main/assets/ontologies/core/latest"/>
      <dcat:downloadURL rdf:resource="https://raw.githubusercontent.com/INPS-it/NDC/main/assets/ontologies/core/latest/core.owl"/>
      <dct:description xml:lang="it">Questa è la distribuzione RDF/XML dell'ontologia INPS relativa alle componenti del dominio funzionale dell'istituto comuni a procedure e servizi svolti dall'ente stesso. Tra di essi troviamo, ad esempio, le dislocazioni territoriali, come le sedi, e le entità astratte, come i ruoli.</dct:description>
      <dct:description xml:lang="en">This is the distribution in RDF/XML of the INPS Ontology about components of the institution's functional domain common to procedures and services performed by the institution itself. These include, for example, territorial dislocations, such as locations, and abstract entities, such as roles.</dct:description>
      <dct:format rdf:resource="http://publications.europa.eu/resource/authority/file-type/RDF_XML"/>
      <dct:license rdf:resource="http://creativecommons.org/licenses/by/4.0/"/>
      <dct:title xml:lang="it">Distribuzione RDF/XML dell'ontologia INPS - Core</dct:title>
      <dct:title xml:lang="en">RDF/XML distribution of the INPS ontology - Core</dct:title>
    </rdf:Description>

	<!-- https://w3id.org/italia/social-security/data/organization/DirezioneCentraleTII -->

    <rdf:Description rdf:about="https://w3id.org/italia/social-security/data/organization/DirezioneCentraleTII">
      <rdf:type rdf:resource="http://dati.gov.it/onto/dcatapit#Organization"/>
      <rdf:type rdf:resource="http://www.w3.org/2002/07/owl#NamedIndividual"/>
      <rdf:type rdf:resource="http://www.w3.org/2006/vcard/ns#Kind"/>
      <rdf:type rdf:resource="http://www.w3.org/2006/vcard/ns#Organization"/>
      <foaf:name xml:lang="en">Central Management of Information Technology and Innovations</foaf:name>
      <foaf:name xml:lang="it">Direzione Centrale Tecnologia, Informatica e Innovazione</foaf:name>
      <vcard:fn>Direzione Centrale Tecnologia, Informatica e Innovazione</vcard:fn>
      <vcard:hasEmail rdf:resource="mailto:dc.tecnologiainformaticaeinnovazione@postacert.inps.gov.it"/> 
    </rdf:Description>

	  <!-- https://w3id.org/italia/social-security/data/organization/inps -->

      <rdf:Description rdf:about="https://w3id.org/italia/social-security/data/organization/inps">
        <rdf:type rdf:resource="https://w3id.org/italia/onto/COV/PublicOrganization"/>
        <rdf:type rdf:resource="http://dati.gov.it/onto/dcatapit#Agent"/>
        <rdf:type rdf:resource="http://xmlns.com/foaf/0.1/Agent"/>
        <rdf:type rdf:resource="http://www.w3.org/2002/07/owl#NamedIndividual"/>
        <dct:identifier>inps</dct:identifier>
        <foaf:name xml:lang="it">Istituto nazionale della previdenza sociale</foaf:name>
        <foaf:name xml:lang="en">National institute for Social Security</foaf:name>
      </rdf:Description>    

    <!-- https://w3id.org/italia/social-security/data/organization/td -->

    <rdf:Description rdf:about="https://w3id.org/italia/social-security/data/organization/td">
      <rdf:type rdf:resource="http://dati.gov.it/onto/dcatapit#Agent"/>
      <rdf:type rdf:resource="http://xmlns.com/foaf/0.1/Agent"/>
      <rdf:type rdf:resource="http://www.w3.org/2002/07/owl#NamedIndividual"/>
      <dct:identifier>TD</dct:identifier>
      <foaf:name xml:lang="en">Digital Transformation Team</foaf:name>
      <foaf:name xml:lang="it">Team per la Trasformazione Digitale</foaf:name>
    </rdf:Description>

    <!-- https://w3id.org/italia/social-security/onto/core/INPS -->

    <owl:NamedIndividual rdf:about="https://w3id.org/italia/social-security/onto/core/INPS">
        <rdf:type rdf:resource="https://w3id.org/italia/onto/COV/PublicOrganization"/>
        <rdfs:comment xml:lang="it">L'Istituto Nazionale della Previdenza Sociale è l'Ente Pubblico che gestisce la liquidazione e il pagamento delle pensioni e delle indennità di natura previdenziale e assistenziale. Le pensioni sono prestazioni previdenziali, determinate sulla base di rapporti assicurativi e finanziate con i contributi di lavoratori e aziende pubbliche e private. Invece, le prestazioni assistenziali o “a sostegno del reddito” tutelano i lavoratori che si trovano in particolari momenti di difficoltà della loro vita lavorativa e provvedono al pagamento di somme destinate a coloro che hanno redditi modesti e famiglie numerose. Per alcune di queste prestazioni l’INPS è coinvolto solo nella fase di erogazione, mentre per altre svolge tutto il procedimento di assegnazione.</rdfs:comment>
        <rdfs:comment xml:lang="en">The National Institute for Social Security is the Italian Public Organization that supplies pensions and other services of social security to who has the right. It also does contributory activity collecting the contributions. The services are based on a mandatory insurance relationship and are funded with the contributions of employed workers, elaborated as a percentage of the wage. It also manages welfare services or &quot;income support&quot; services that protect workers who find themselves in particular difficult moments in their working life and provide for the payment of sums intended for those with modest incomes and large families.</rdfs:comment>
        <rdfs:label xml:lang="en">INPS</rdfs:label>
        <rdfs:label xml:lang="it">INPS</rdfs:label>
    </owl:NamedIndividual>



    <!--
    ///////////////////////////////////////////////////////////////////////////////////////
    //
    // General axioms
    //
    ///////////////////////////////////////////////////////////////////////////////////////
     -->

    <owl:Class>
        <owl:unionOf rdf:parseType="Collection">
            <rdf:Description rdf:about="https://w3id.org/italia/onto/COV/Organization"/>
            <rdf:Description rdf:about="https://w3id.org/italia/onto/CPV/Person"/>
        </owl:unionOf>
        <rdfs:subClassOf rdf:resource="https://w3id.org/italia/onto/l0/Agent"/>
    </owl:Class>
    <owl:Class>
        <owl:unionOf rdf:parseType="Collection">
            <rdf:Description rdf:about="https://w3id.org/italia/onto/CPV/Alive"/>
            <rdf:Description rdf:about="https://w3id.org/italia/onto/CPV/Dead"/>
        </owl:unionOf>
        <rdfs:subClassOf rdf:resource="https://w3id.org/italia/onto/CPV/Person"/>
    </owl:Class>
    <owl:Class>
        <owl:unionOf rdf:parseType="Collection">
            <rdf:Description rdf:about="https://w3id.org/italia/social-security/onto/core/RuoloDiOrganizzazione"/>
            <rdf:Description rdf:about="https://w3id.org/italia/social-security/onto/core/RuoloDiPersona"/>
        </owl:unionOf>
        <rdfs:subClassOf rdf:resource="https://w3id.org/italia/social-security/onto/core/RuoloDiAgente"/>
    </owl:Class>
    <owl:Class>
        <owl:unionOf rdf:parseType="Collection">
            <rdf:Description rdf:about="https://w3id.org/italia/social-security/onto/core/RuoloDiPersonaDeceduta"/>
            <rdf:Description rdf:about="https://w3id.org/italia/social-security/onto/core/RuoloDiPersonaViva"/>
        </owl:unionOf>
        <rdfs:subClassOf rdf:resource="https://w3id.org/italia/social-security/onto/core/RuoloDiPersona"/>
    </owl:Class>
    <owl:Restriction>
        <owl:onProperty>
            <rdf:Description>
                <owl:inverseOf rdf:resource="https://w3id.org/italia/onto/CLV/hasAddressComponent"/>
            </rdf:Description>
        </owl:onProperty>
        <owl:someValuesFrom>
            <owl:Restriction>
                <owl:onProperty>
                    <rdf:Description>
                        <owl:inverseOf rdf:resource="https://w3id.org/italia/onto/CLV/hasPrimaryAddress"/>
                    </rdf:Description>
                </owl:onProperty>
                <owl:someValuesFrom rdf:resource="https://w3id.org/italia/onto/COV/Organization"/>
            </owl:Restriction>
        </owl:someValuesFrom>
        <rdfs:subClassOf>
            <owl:Restriction>
                <owl:onProperty>
                    <rdf:Description>
                        <owl:inverseOf rdf:resource="https://w3id.org/italia/onto/CLV/hasAddressComponent"/>
                    </rdf:Description>
                </owl:onProperty>
                <owl:someValuesFrom>
                    <owl:Restriction>
                        <owl:onProperty>
                            <rdf:Description>
                                <owl:inverseOf rdf:resource="https://w3id.org/italia/onto/CLV/hasAddress"/>
                            </rdf:Description>
                        </owl:onProperty>
                        <owl:someValuesFrom>
                            <owl:Restriction>
                                <owl:onProperty>
                                    <rdf:Description>
                                        <owl:inverseOf rdf:resource="https://w3id.org/italia/social-security/onto/core/haSedeINPS"/>
                                    </rdf:Description>
                                </owl:onProperty>
                                <owl:someValuesFrom rdf:resource="http://www.w3.org/2002/07/owl#Thing"/>
                            </owl:Restriction>
                        </owl:someValuesFrom>
                    </owl:Restriction>
                </owl:someValuesFrom>
            </owl:Restriction>
        </rdfs:subClassOf>
    </owl:Restriction>
    <owl:Restriction>
        <owl:onProperty>
            <rdf:Description>
                <owl:inverseOf rdf:resource="https://w3id.org/italia/onto/CLV/hasAddressComponent"/>
            </rdf:Description>
        </owl:onProperty>
        <owl:someValuesFrom>
            <owl:Restriction>
                <owl:onProperty>
                    <rdf:Description>
                        <owl:inverseOf rdf:resource="https://w3id.org/italia/onto/CPV/hasCurrentResidence"/>
                    </rdf:Description>
                </owl:onProperty>
                <owl:someValuesFrom rdf:resource="https://w3id.org/italia/onto/CPV/Alive"/>
            </owl:Restriction>
        </owl:someValuesFrom>
        <rdfs:subClassOf>
            <owl:Restriction>
                <owl:onProperty>
                    <rdf:Description>
                        <owl:inverseOf rdf:resource="https://w3id.org/italia/onto/CLV/hasAddressComponent"/>
                    </rdf:Description>
                </owl:onProperty>
                <owl:someValuesFrom>
                    <owl:Restriction>
                        <owl:onProperty>
                            <rdf:Description>
                                <owl:inverseOf rdf:resource="https://w3id.org/italia/onto/CLV/hasAddress"/>
                            </rdf:Description>
                        </owl:onProperty>
                        <owl:someValuesFrom>
                            <owl:Restriction>
                                <owl:onProperty>
                                    <rdf:Description>
                                        <owl:inverseOf rdf:resource="https://w3id.org/italia/social-security/onto/core/haSedeINPS"/>
                                    </rdf:Description>
                                </owl:onProperty>
                                <owl:someValuesFrom rdf:resource="http://www.w3.org/2002/07/owl#Thing"/>
                            </owl:Restriction>
                        </owl:someValuesFrom>
                    </owl:Restriction>
                </owl:someValuesFrom>
            </owl:Restriction>
        </rdfs:subClassOf>
    </owl:Restriction>
</rdf:RDF>



<!-- Generated by the OWL API (version 2.4) https://github.com/owlcs/owlapi -->

