<?xml version="1.0"?>
<rdf:RDF xmlns="https://w3id.org/italia/social-security/onto/socialSafetyNet/"
     xml:base="https://w3id.org/italia/social-security/onto/socialSafetyNet/"
     xmlns:L0="https://w3id.org/italia/onto/l0/"
     xmlns:RO="https://w3id.org/italia/onto/RO/"
     xmlns:TI="https://w3id.org/italia/onto/TI/"
     xmlns:CLV="https://w3id.org/italia/onto/CLV/"
     xmlns:COV="https://w3id.org/italia/onto/COV/"
     xmlns:CPV="https://w3id.org/italia/onto/CPV/"
     xmlns:dct="http://purl.org/dc/terms/"
     xmlns:owl="http://www.w3.org/2002/07/owl#"
     xmlns:rdf="http://www.w3.org/1999/02/22-rdf-syntax-ns#"
     xmlns:xml="http://www.w3.org/XML/1998/namespace"
     xmlns:xsd="http://www.w3.org/2001/XMLSchema#"
     xmlns:adms="https://w3id.org/italia/onto/ADMS/"
     xmlns:dcat="http://www.w3.org/ns/dcat#"
     xmlns:foaf="http://xmlns.com/foaf/0.1/"
     xmlns:rdfs="http://www.w3.org/2000/01/rdf-schema#"
     xmlns:vcard="http://www.w3.org/2006/vcard/ns#"
     xmlns:smapit="https://w3id.org/italia/onto/SM/"
     xmlns:INPSCore="https://w3id.org/italia/social-security/onto/core/"
     xmlns:dcatapit="http://dati.gov.it/onto/dcatapit#"
     xmlns:INPSSafety="https://w3id.org/italia/social-security/onto/socialSafetyNet/"
     xmlns:ateco-2007="https://w3id.org/italia/controlled-vocabulary/classifications-for-organizations/ateco-2007/"
     xmlns:INPSPensions="https://w3id.org/italia/social-security/onto/pensions/"
     xmlns:INPSContributions="https://w3id.org/italia/social-security/onto/contributions/">
    <owl:Ontology rdf:about="https://w3id.org/italia/social-security/onto/socialSafetyNet/">
        <owl:versionIRI rdf:resource="https://w3id.org/italia/social-security/onto/socialSafetyNet/1.0.0"/>
        <owl:imports rdf:resource="https://w3id.org/italia/onto/COV/"/>
        <owl:imports rdf:resource="https://w3id.org/italia/onto/TI/"/>
        <owl:imports rdf:resource="https://w3id.org/italia/onto/l0/"/>
        <owl:imports rdf:resource="https://w3id.org/italia/social-security/onto/contributions/"/>
        <owl:imports rdf:resource="https://w3id.org/italia/social-security/onto/core/"/>
        <dct:accrualPeriodicity rdf:resource="http://publications.europa.eu/resource/authority/frequency/IRREG"/>
        <dct:creator rdf:resource="https://w3id.org/italia/social-security/data/organization/inps"/>
        <dct:description xml:lang="it">L&apos;ontologia INPS relativa alla NASpI rappresenta un insieme strutturato di concetti e relazioni che descrivono in modo dettagliato il sistema di indennità di disoccupazione NASpI erogato dall&apos;Istituto Nazionale della Previdenza Sociale (INPS).</dct:description>
        <dct:description xml:lang="en">The INPS ontology related to NASpI represents a structured set of concepts and relationships that provide a detailed description of the NASpI unemployment benefit system administered by the Italian National Institute of Social Security (INPS).</dct:description>
        <dct:identifier>https://w3id.org/italia/social-security/onto/socialSafetyNet</dct:identifier>
        <dct:issued rdf:datatype="http://www.w3.org/2001/XMLSchema#dateTime">2024-06-06T00:00:00+00:00</dct:issued>
        <dct:language rdf:resource="http://publications.europa.eu/resource/authority/language/ENG"/>
        <dct:language rdf:resource="http://publications.europa.eu/resource/authority/language/ITA"/>
        <dct:modified rdf:datatype="http://www.w3.org/2001/XMLSchema#dateTime">2024-01-17T00:00:00+00:00</dct:modified>
        <dct:publisher rdf:resource="https://w3id.org/italia/social-security/data/organization/inps"/>
        <dct:rightsHolder rdf:resource="https://w3id.org/italia/social-security/data/organization/inps"/>
        <dct:title xml:lang="en">INPS Ontology related to NASpI (New Social Insurance for Employment)</dct:title>
        <dct:title xml:lang="it">Ontologia INPS relativa a NASpI (Nuova Assicurazione Sociale per l&apos;Impiego) </dct:title>
        <rdfs:comment xml:lang="it">L&apos;ontologia INPS relativa alla NASpI rappresenta un insieme strutturato di concetti e relazioni che descrivono in modo dettagliato il sistema di indennità di disoccupazione NASpI erogato dall&apos;Istituto Nazionale della Previdenza Sociale (INPS).</rdfs:comment>
        <rdfs:comment xml:lang="en">The INPS ontology related to NASpI represents a structured set of concepts and relationships that provide a detailed description of the NASpI unemployment benefit system administered by the Italian National Institute of Social Security (INPS).</rdfs:comment>
        <rdfs:isDefinedBy rdf:resource="https://w3id.org/italia/social-security/onto/socialSafetyNet/"/>
        <rdfs:label xml:lang="en">INPS Ontology related to NASpI (New Social Insurance for Employment)</rdfs:label>
        <rdfs:label xml:lang="it">Ontologia INPS relativa a NASpI (Nuova Assicurazione Sociale per l&apos;Impiego) </rdfs:label>
        <owl:versionInfo xml:lang="en">Version 1.0 - Modified on 06 June 2024</owl:versionInfo>
        <owl:versionInfo xml:lang="it">Versione 1.0 - Modificata il 26 Giugno 2024</owl:versionInfo>
        <dcat:contactPoint rdf:resource="https://w3id.org/italia/social-security/data/organization/DirezioneCentraleTII"/>
        <dcat:keyword xml:lang="it">domanda NASpI</dcat:keyword>
        <dcat:keyword xml:lang="it">fascicolo di lavoro</dcat:keyword>
        <dcat:keyword xml:lang="it">inoccupato</dcat:keyword>
        <dcat:keyword xml:lang="it">lavoratore</dcat:keyword>
        <dcat:keyword xml:lang="it">richiedente NASpI</dcat:keyword>
        <dcat:keyword xml:lang="en">worker</dcat:keyword>
        <dcat:theme rdf:resource="http://publications.europa.eu/resource/authority/data-theme/SOCI"/>
        <adms:acronym>inps</adms:acronym>
        <adms:hasContributor rdf:resource="https://w3id.org/italia/social-security/data/organization/td"/>
        <adms:hasFormalityLevel rdf:resource="https://w3id.org/italia/onto/ADMS/Formal"/>
        <adms:hasKeyClass rdf:resource="https://w3id.org/italia/social-security/onto/socialSafetyNet/Disoccupato"/>
        <adms:hasKeyClass rdf:resource="https://w3id.org/italia/social-security/onto/socialSafetyNet/DomandaNASpI"/>
        <adms:hasKeyClass rdf:resource="https://w3id.org/italia/social-security/onto/socialSafetyNet/FascicoloDiLavoro"/>
        <adms:hasKeyClass rdf:resource="https://w3id.org/italia/social-security/onto/socialSafetyNet/Inoccupato"/>
        <adms:hasKeyClass rdf:resource="https://w3id.org/italia/social-security/onto/socialSafetyNet/RichiedenteNASpI"/>
        <adms:hasOntologyLanguage rdf:resource="https://w3id.org/italia/onto/ADMS/OWL"/>
        <adms:hasSemanticAssetDistribution rdf:resource="https://w3id.org/italia/social-security/data/socialSafetyNet/distribution/SAFETY-N-TRIPLES"/>
        <adms:hasSemanticAssetDistribution rdf:resource="https://w3id.org/italia/social-security/data/socialSafetyNet/distribution/SAFETY-RDF-TURTLE"/>
        <adms:hasSemanticAssetDistribution rdf:resource="https://w3id.org/italia/social-security/data/socialSafetyNet/distribution/SAFETY-RDF-XML"/>
        <adms:hasTask rdf:resource="https://w3id.org/italia/onto/ADMS/AnnotationTask"/>
        <adms:hasTask rdf:resource="https://w3id.org/italia/onto/ADMS/QueryFormulationTask"/>
        <adms:hasTask rdf:resource="https://w3id.org/italia/onto/ADMS/SearchTask"/>
        <adms:last rdf:resource="https://w3id.org/italia/social-security/onto/socialSafetyNet/1.0"/>
        <adms:officialURI rdf:datatype="http://www.w3.org/2001/XMLSchema#anyURI">https://w3id.org/italia/social-security/onto/socialSafetyNet</adms:officialURI>
        <adms:prefix>INPSSafety</adms:prefix>
        <adms:semanticAssetInUse rdf:resource="https://w3id.org/italia/data/project/NDC"/>
        <adms:status>catalogued</adms:status>
        <adms:status>published</adms:status>
        <adms:target xml:lang="it">Cittadini</adms:target>
        <adms:target xml:lang="it">Imprese</adms:target>
        <adms:target xml:lang="it">Pubbliche Amministrazioni</adms:target>
        <adms:type rdf:resource="https://w3id.org/italia/onto/ADMS/ServiceOnytology"/>
    </owl:Ontology>



    <!--
    ///////////////////////////////////////////////////////////////////////////////////////
    //
    // Annotation properties
    //
    ///////////////////////////////////////////////////////////////////////////////////////
     -->




    <!-- http://purl.org/dc/terms/accrualPeriodicity -->

    <owl:AnnotationProperty rdf:about="http://purl.org/dc/terms/accrualPeriodicity"/>



    <!-- http://purl.org/dc/terms/creator -->

    <owl:AnnotationProperty rdf:about="http://purl.org/dc/terms/creator"/>



    <!-- http://purl.org/dc/terms/description -->

    <owl:AnnotationProperty rdf:about="http://purl.org/dc/terms/description"/>



    <!-- http://purl.org/dc/terms/format -->

    <owl:AnnotationProperty rdf:about="http://purl.org/dc/terms/format"/>



    <!-- http://purl.org/dc/terms/identifier -->

    <owl:AnnotationProperty rdf:about="http://purl.org/dc/terms/identifier"/>



    <!-- http://purl.org/dc/terms/issued -->

    <owl:AnnotationProperty rdf:about="http://purl.org/dc/terms/issued"/>



    <!-- http://purl.org/dc/terms/language -->

    <owl:AnnotationProperty rdf:about="http://purl.org/dc/terms/language"/>



    <!-- http://purl.org/dc/terms/license -->

    <owl:AnnotationProperty rdf:about="http://purl.org/dc/terms/license"/>



    <!-- http://purl.org/dc/terms/modified -->

    <owl:AnnotationProperty rdf:about="http://purl.org/dc/terms/modified"/>



    <!-- http://purl.org/dc/terms/publisher -->

    <owl:AnnotationProperty rdf:about="http://purl.org/dc/terms/publisher"/>



    <!-- http://purl.org/dc/terms/rightsHolder -->

    <owl:AnnotationProperty rdf:about="http://purl.org/dc/terms/rightsHolder"/>



    <!-- http://purl.org/dc/terms/title -->

    <owl:AnnotationProperty rdf:about="http://purl.org/dc/terms/title"/>



    <!-- http://www.w3.org/2006/vcard/ns#fn -->

    <owl:AnnotationProperty rdf:about="http://www.w3.org/2006/vcard/ns#fn"/>



    <!-- http://www.w3.org/2006/vcard/ns#hasEmail -->

    <owl:AnnotationProperty rdf:about="http://www.w3.org/2006/vcard/ns#hasEmail"/>



    <!-- http://www.w3.org/ns/dcat#accessURL -->

    <owl:AnnotationProperty rdf:about="http://www.w3.org/ns/dcat#accessURL"/>



    <!-- http://www.w3.org/ns/dcat#contactPoint -->

    <owl:AnnotationProperty rdf:about="http://www.w3.org/ns/dcat#contactPoint"/>



    <!-- http://www.w3.org/ns/dcat#downloadURL -->

    <owl:AnnotationProperty rdf:about="http://www.w3.org/ns/dcat#downloadURL"/>



    <!-- http://www.w3.org/ns/dcat#keyword -->

    <owl:AnnotationProperty rdf:about="http://www.w3.org/ns/dcat#keyword"/>



    <!-- http://www.w3.org/ns/dcat#theme -->

    <owl:AnnotationProperty rdf:about="http://www.w3.org/ns/dcat#theme"/>



    <!-- http://xmlns.com/foaf/0.1/name -->

    <owl:AnnotationProperty rdf:about="http://xmlns.com/foaf/0.1/name"/>



    <!-- https://w3id.org/italia/onto/ADMS/acronym -->

    <owl:AnnotationProperty rdf:about="https://w3id.org/italia/onto/ADMS/acronym"/>



    <!-- https://w3id.org/italia/onto/ADMS/hasContributor -->

    <owl:AnnotationProperty rdf:about="https://w3id.org/italia/onto/ADMS/hasContributor"/>



    <!-- https://w3id.org/italia/onto/ADMS/hasFormalityLevel -->

    <owl:AnnotationProperty rdf:about="https://w3id.org/italia/onto/ADMS/hasFormalityLevel"/>



    <!-- https://w3id.org/italia/onto/ADMS/hasKeyClass -->

    <owl:AnnotationProperty rdf:about="https://w3id.org/italia/onto/ADMS/hasKeyClass"/>



    <!-- https://w3id.org/italia/onto/ADMS/hasOntologyLanguage -->

    <owl:AnnotationProperty rdf:about="https://w3id.org/italia/onto/ADMS/hasOntologyLanguage"/>



    <!-- https://w3id.org/italia/onto/ADMS/hasSemanticAssetDistribution -->

    <owl:AnnotationProperty rdf:about="https://w3id.org/italia/onto/ADMS/hasSemanticAssetDistribution"/>



    <!-- https://w3id.org/italia/onto/ADMS/hasTask -->

    <owl:AnnotationProperty rdf:about="https://w3id.org/italia/onto/ADMS/hasTask"/>



    <!-- https://w3id.org/italia/onto/ADMS/last -->

    <owl:AnnotationProperty rdf:about="https://w3id.org/italia/onto/ADMS/last"/>



    <!-- https://w3id.org/italia/onto/ADMS/officialURI -->

    <owl:AnnotationProperty rdf:about="https://w3id.org/italia/onto/ADMS/officialURI"/>



    <!-- https://w3id.org/italia/onto/ADMS/prefix -->

    <owl:AnnotationProperty rdf:about="https://w3id.org/italia/onto/ADMS/prefix"/>



    <!-- https://w3id.org/italia/onto/ADMS/semanticAssetInUse -->

    <owl:AnnotationProperty rdf:about="https://w3id.org/italia/onto/ADMS/semanticAssetInUse"/>



    <!-- https://w3id.org/italia/onto/ADMS/status -->

    <owl:AnnotationProperty rdf:about="https://w3id.org/italia/onto/ADMS/status"/>



    <!-- https://w3id.org/italia/onto/ADMS/target -->

    <owl:AnnotationProperty rdf:about="https://w3id.org/italia/onto/ADMS/target"/>



    <!-- https://w3id.org/italia/onto/ADMS/type -->

    <owl:AnnotationProperty rdf:about="https://w3id.org/italia/onto/ADMS/type"/>



    <!--
    ///////////////////////////////////////////////////////////////////////////////////////
    //
    // Datatypes
    //
    ///////////////////////////////////////////////////////////////////////////////////////
     -->




    <!-- http://www.w3.org/2001/XMLSchema#boolean -->

    <rdfs:Datatype rdf:about="http://www.w3.org/2001/XMLSchema#boolean"/>



    <!-- http://www.w3.org/2001/XMLSchema#dateTime -->

    <rdfs:Datatype rdf:about="http://www.w3.org/2001/XMLSchema#dateTime"/>



    <!-- http://www.w3.org/2001/XMLSchema#decimal -->

    <rdfs:Datatype rdf:about="http://www.w3.org/2001/XMLSchema#decimal"/>



    <!-- http://www.w3.org/2001/XMLSchema#string -->

    <rdfs:Datatype rdf:about="http://www.w3.org/2001/XMLSchema#string"/>



    <!--
    ///////////////////////////////////////////////////////////////////////////////////////
    //
    // Object Properties
    //
    ///////////////////////////////////////////////////////////////////////////////////////
     -->




    <!-- https://w3id.org/italia/onto/CLV/hasAddress -->

    <owl:ObjectProperty rdf:about="https://w3id.org/italia/onto/CLV/hasAddress"/>



    <!-- https://w3id.org/italia/onto/CLV/hasAdressinTime -->

    <owl:ObjectProperty rdf:about="https://w3id.org/italia/onto/CLV/hasAdressinTime"/>



    <!-- https://w3id.org/italia/onto/CLV/hasCountry -->

    <owl:ObjectProperty rdf:about="https://w3id.org/italia/onto/CLV/hasCountry"/>



    <!-- https://w3id.org/italia/onto/CLV/withAddress -->

    <owl:ObjectProperty rdf:about="https://w3id.org/italia/onto/CLV/withAddress"/>



    <!-- https://w3id.org/italia/onto/COV/hasActivityType -->

    <owl:ObjectProperty rdf:about="https://w3id.org/italia/onto/COV/hasActivityType"/>



    <!-- https://w3id.org/italia/onto/CPV/residentIn -->

    <owl:ObjectProperty rdf:about="https://w3id.org/italia/onto/CPV/residentIn"/>



    <!-- https://w3id.org/italia/onto/RO/holdsRoleInTime -->

    <owl:ObjectProperty rdf:about="https://w3id.org/italia/onto/RO/holdsRoleInTime"/>



    <!-- https://w3id.org/italia/onto/SM/hasOnlineContactPoint -->

    <owl:ObjectProperty rdf:about="https://w3id.org/italia/onto/SM/hasOnlineContactPoint"/>



    <!-- https://w3id.org/italia/onto/TI/atTime -->

    <owl:ObjectProperty rdf:about="https://w3id.org/italia/onto/TI/atTime"/>



    <!-- https://w3id.org/italia/onto/TI/hasTemporalEntity -->

    <owl:ObjectProperty rdf:about="https://w3id.org/italia/onto/TI/hasTemporalEntity"/>



    <!-- https://w3id.org/italia/onto/l0/hasFirstMember -->

    <owl:ObjectProperty rdf:about="https://w3id.org/italia/onto/l0/hasFirstMember"/>



    <!-- https://w3id.org/italia/onto/l0/hasMember -->

    <owl:ObjectProperty rdf:about="https://w3id.org/italia/onto/l0/hasMember"/>



    <!-- https://w3id.org/italia/social-security/onto/socialSafetyNet/accettaContrattoDiLavoro -->

    <owl:ObjectProperty rdf:about="https://w3id.org/italia/social-security/onto/socialSafetyNet/accettaContrattoDiLavoro">
        <rdfs:domain rdf:resource="https://w3id.org/italia/social-security/onto/socialSafetyNet/Lavoratore"/>
        <rdfs:range rdf:resource="https://w3id.org/italia/social-security/onto/socialSafetyNet/ContrattoDiLavoro"/>
        <owl:propertyChainAxiom rdf:parseType="Collection">
            <rdf:Description rdf:about="https://w3id.org/italia/social-security/onto/socialSafetyNet/forniscePrestazioneLavorativa"/>
            <rdf:Description rdf:about="https://w3id.org/italia/social-security/onto/socialSafetyNet/èRegolatoDaContratto"/>
        </owl:propertyChainAxiom>
        <rdfs:comment xml:lang="en">Property that links a Worker to a Work contract</rdfs:comment>
        <rdfs:comment xml:lang="it">Proprietà che lega un Lavoratore a un Contratto di lavoro.</rdfs:comment>
        <rdfs:label xml:lang="en">accepts work contract</rdfs:label>
        <rdfs:label xml:lang="it">accetta contratto di lavoro</rdfs:label>
    </owl:ObjectProperty>



    <!-- https://w3id.org/italia/social-security/onto/socialSafetyNet/comunicaDomandaDiPensionamento -->

    <owl:ObjectProperty rdf:about="https://w3id.org/italia/social-security/onto/socialSafetyNet/comunicaDomandaDiPensionamento">
        <rdf:type rdf:resource="http://www.w3.org/2002/07/owl#FunctionalProperty"/>
        <rdf:type rdf:resource="http://www.w3.org/2002/07/owl#InverseFunctionalProperty"/>
        <rdfs:domain rdf:resource="https://w3id.org/italia/social-security/onto/socialSafetyNet/ComunicazioneEventoNASpI"/>
        <rdfs:range rdf:resource="https://w3id.org/italia/social-security/onto/socialSafetyNet/DomandaDiPensionamento"/>
        <rdfs:comment xml:lang="en">Property that links a NASpI event communication to one and only one Retirement claim.</rdfs:comment>
        <rdfs:comment xml:lang="it">Proprietà che lega una Comunicazione evento NASpI a una e una sola Domanda di pensionamento.</rdfs:comment>
        <rdfs:label xml:lang="it">comunica domanda di pensionamento</rdfs:label>
        <rdfs:label xml:lang="en">notifies retirement claim</rdfs:label>
    </owl:ObjectProperty>



    <!-- https://w3id.org/italia/social-security/onto/socialSafetyNet/comunicaIscrizioneUfficioDelLavoro -->

    <owl:ObjectProperty rdf:about="https://w3id.org/italia/social-security/onto/socialSafetyNet/comunicaIscrizioneUfficioDelLavoro">
        <rdf:type rdf:resource="http://www.w3.org/2002/07/owl#FunctionalProperty"/>
        <rdf:type rdf:resource="http://www.w3.org/2002/07/owl#InverseFunctionalProperty"/>
        <rdfs:domain rdf:resource="https://w3id.org/italia/social-security/onto/socialSafetyNet/ComunicazioneEventoNASpI"/>
        <rdfs:range rdf:resource="https://w3id.org/italia/social-security/onto/socialSafetyNet/IscrizioneUfficioDelLavoro"/>
        <rdfs:comment xml:lang="en">Property that links a NASpI Event Communication to one and only one Labour office registration. Registration can be related to a Foreign labour office and, in the case of a Frontier worker, it is mandatory.</rdfs:comment>
        <rdfs:comment xml:lang="it">Proprietà che lega una Comunicazione evento NASpI a una e una sola Iscrizione ufficio del lavoro. L&apos;iscrizione può essere relativa ad un Ufficio del lavoro estero e, nel caso di un Lavoratore frontaliero, è obbligatoria.</rdfs:comment>
        <rdfs:label xml:lang="it">comunica iscrizione ufficio del Lavoro</rdfs:label>
        <rdfs:label xml:lang="en">notifies labour office registration</rdfs:label>
    </owl:ObjectProperty>



    <!-- https://w3id.org/italia/social-security/onto/socialSafetyNet/comunicaNuovaAttivitàLavorativaAutonoma -->

    <owl:ObjectProperty rdf:about="https://w3id.org/italia/social-security/onto/socialSafetyNet/comunicaNuovaAttivitàLavorativaAutonoma">
        <rdf:type rdf:resource="http://www.w3.org/2002/07/owl#FunctionalProperty"/>
        <rdf:type rdf:resource="http://www.w3.org/2002/07/owl#InverseFunctionalProperty"/>
        <rdfs:domain rdf:resource="https://w3id.org/italia/social-security/onto/socialSafetyNet/ComunicazioneEventoNASpI"/>
        <rdfs:range>
            <owl:Class>
                <owl:unionOf rdf:parseType="Collection">
                    <rdf:Description rdf:about="https://w3id.org/italia/social-security/onto/socialSafetyNet/CollaborazioneCoordinataEContinuativa"/>
                    <rdf:Description rdf:about="https://w3id.org/italia/social-security/onto/socialSafetyNet/ContrattoDOpera"/>
                    <rdf:Description rdf:about="https://w3id.org/italia/social-security/onto/socialSafetyNet/ContrattoDOperaProfessionale"/>
                </owl:unionOf>
            </owl:Class>
        </rdfs:range>
        <rdfs:comment xml:lang="en">Property that links a NASpI event communication to one and only one new self-employment or parasubordinate employment contract. The contract linked to the communication falls within the time period of the NASpI Service to which the communication is in turn linked. If the income generated by the new contract is less than the limit provided, the benefit is maintained and the amount of the compensation is recalculated, otherwise the benefit lapses.</rdfs:comment>
        <rdfs:comment xml:lang="it">Proprietà che lega un Comunicazione evento NASpI a uno e un solo nuovo contratto di lavoro autonomo o parasubordinato. Il contratto legato alla comunicazione cade nel periodo temporale della Prestazione NASpI a cui la comunicazione è a sua volta legata. Se il reddito prodotto dal nuovo contratto è inferiore al limite previsto, la prestazione viene mantenuta e l&apos;importo dell&apos;indennità ricalcolato, altrimenti la prestazione decade.</rdfs:comment>
        <rdfs:label xml:lang="it">comunica nuova attività lavorativa autonoma</rdfs:label>
        <rdfs:label xml:lang="en">notifies new self-employment activity</rdfs:label>
    </owl:ObjectProperty>



    <!-- https://w3id.org/italia/social-security/onto/socialSafetyNet/comunicaNuovaAttivitàLavorativaSubordinata -->

    <owl:ObjectProperty rdf:about="https://w3id.org/italia/social-security/onto/socialSafetyNet/comunicaNuovaAttivitàLavorativaSubordinata">
        <rdf:type rdf:resource="http://www.w3.org/2002/07/owl#FunctionalProperty"/>
        <rdf:type rdf:resource="http://www.w3.org/2002/07/owl#InverseFunctionalProperty"/>
        <rdfs:domain rdf:resource="https://w3id.org/italia/social-security/onto/socialSafetyNet/ComunicazioneEventoNASpI"/>
        <rdfs:range rdf:resource="https://w3id.org/italia/social-security/onto/socialSafetyNet/ContrattoDiLavoroSubordinato"/>
        <rdfs:comment xml:lang="en">Property that links a NASpI event communication to one and only one Salaried employment contract. The contract linked to the communication falls within the time period of the NASpI Service to which the communication is in turn linked. If the income produced by the new contract is less than the limit provided, the benefit is maintained and the amount of the indemnity is recalculated, otherwise if the duration of the new contract is less than 6 months, the benefit is suspended, if higher it causes it to lapse.</rdfs:comment>
        <rdfs:comment xml:lang="it">Proprietà che lega un Comunicazione evento NASpI a uno e un solo Contratto di lavoro subordinato. Il contratto legato alla comunicazione cade nel periodo temporale della Prestazione NASpI a cui la comunicazione è a sua volta legata. Se il reddito prodotto dal nuovo contratto è inferiore al limite previsto, la prestazione viene mantenuta e l&apos;importo dell&apos;indennità ricalcolato, altrimenti se la durata del nuovo contratto è inferiore a 6 mesi, la prestazione viene sospesa, se superiore la fa decadere.</rdfs:comment>
        <rdfs:label xml:lang="it">comunica nuova attività lavorativa subordinata</rdfs:label>
        <rdfs:label xml:lang="en">notifies new salaried employment activity</rdfs:label>
    </owl:ObjectProperty>



    <!-- https://w3id.org/italia/social-security/onto/socialSafetyNet/comunicaPeriodoDiIndisponibilità -->

    <owl:ObjectProperty rdf:about="https://w3id.org/italia/social-security/onto/socialSafetyNet/comunicaPeriodoDiIndisponibilità">
        <rdf:type rdf:resource="http://www.w3.org/2002/07/owl#FunctionalProperty"/>
        <rdf:type rdf:resource="http://www.w3.org/2002/07/owl#InverseFunctionalProperty"/>
        <rdfs:domain rdf:resource="https://w3id.org/italia/social-security/onto/socialSafetyNet/ComunicazioneEventoNASpI"/>
        <rdfs:range rdf:resource="https://w3id.org/italia/social-security/onto/socialSafetyNet/IndisponibilitàPerNASpI"/>
        <rdfs:comment xml:lang="en">Property that links a NASpI event communication to one and only one NASpI unavailability period.</rdfs:comment>
        <rdfs:comment xml:lang="it">Proprietà che lega una Comunicazione evento NASpI a uno e un solo Periodo di indisponibilità per NASpI.</rdfs:comment>
        <rdfs:label xml:lang="it">comunica periodo di indisponibilità</rdfs:label>
        <rdfs:label xml:lang="en">notifies unavailability period</rdfs:label>
    </owl:ObjectProperty>



    <!-- https://w3id.org/italia/social-security/onto/socialSafetyNet/comunicaPeriodoEspatrio -->

    <owl:ObjectProperty rdf:about="https://w3id.org/italia/social-security/onto/socialSafetyNet/comunicaPeriodoEspatrio">
        <rdf:type rdf:resource="http://www.w3.org/2002/07/owl#FunctionalProperty"/>
        <rdf:type rdf:resource="http://www.w3.org/2002/07/owl#InverseFunctionalProperty"/>
        <rdfs:domain rdf:resource="https://w3id.org/italia/social-security/onto/socialSafetyNet/ComunicazioneEventoNASpI"/>
        <rdfs:range rdf:resource="https://w3id.org/italia/social-security/onto/socialSafetyNet/EspatrioInNASpI"/>
        <rdfs:comment xml:lang="en">Property that links a NASpI event communication to one and only one NASpI expatriation period. The event of expatriation, depending on its motivation, may give rise to the suspension or forfeiture of the NASpI Benefit.</rdfs:comment>
        <rdfs:comment xml:lang="it">Proprietà che lega una Comunicazione evento NASpI a uno e un solo Espatrio in NASpI. L&apos;evento di espatrio, in base alla sua motivazione, può dar luogo alla sospensione o al decadimento della Prestazione NASpI.</rdfs:comment>
        <rdfs:label xml:lang="it">comunica periodo espatrio</rdfs:label>
        <rdfs:label xml:lang="en">notifies expatriation period</rdfs:label>
    </owl:ObjectProperty>



    <!-- https://w3id.org/italia/social-security/onto/socialSafetyNet/comunicaRinunciaNASpI -->

    <owl:ObjectProperty rdf:about="https://w3id.org/italia/social-security/onto/socialSafetyNet/comunicaRinunciaNASpI">
        <rdf:type rdf:resource="http://www.w3.org/2002/07/owl#FunctionalProperty"/>
        <rdf:type rdf:resource="http://www.w3.org/2002/07/owl#InverseFunctionalProperty"/>
        <rdfs:domain rdf:resource="https://w3id.org/italia/social-security/onto/socialSafetyNet/ComunicazioneEventoNASpI"/>
        <rdfs:range rdf:resource="https://w3id.org/italia/social-security/onto/socialSafetyNet/AttoDiRinunciaAllaNASpI"/>
        <rdfs:comment xml:lang="en">Property that links a NASpI event communication to one and only one NASpI waiver deed.</rdfs:comment>
        <rdfs:comment xml:lang="it">Proprietà che lega una Comunicazione evento NASpI a uno e un solo Atto di rinuncia alla NASpI.</rdfs:comment>
        <rdfs:label xml:lang="it">comunica rinuncia NASpI</rdfs:label>
        <rdfs:label xml:lang="en">notifies NASpI waiver</rdfs:label>
    </owl:ObjectProperty>



    <!-- https://w3id.org/italia/social-security/onto/socialSafetyNet/emetteAttoDiDecadenzaDisoccupazione -->

    <owl:ObjectProperty rdf:about="https://w3id.org/italia/social-security/onto/socialSafetyNet/emetteAttoDiDecadenzaDisoccupazione">
        <rdfs:domain rdf:resource="https://w3id.org/italia/social-security/onto/socialSafetyNet/CentroPerLImpiego"/>
        <rdfs:range rdf:resource="https://w3id.org/italia/social-security/onto/socialSafetyNet/AttoDiDecadenzaStatoDiDisoccupazione"/>
        <rdfs:comment xml:lang="en">Property that links a Employment Centre to a Unemployment status forfeiture deed issued by it.</rdfs:comment>
        <rdfs:comment xml:lang="it">Proprietà che lega un Centro per l&apos;Impiego a un Atto di decadenza stato di disoccupazione dallo stesso emesso.</rdfs:comment>
        <rdfs:label xml:lang="it">emette atto di decadenza disoccupazione</rdfs:label>
        <rdfs:label xml:lang="en">issues unemployment forfeiture deed</rdfs:label>
    </owl:ObjectProperty>



    <!-- https://w3id.org/italia/social-security/onto/socialSafetyNet/emetteAttoDiNotificaViolazione -->

    <owl:ObjectProperty rdf:about="https://w3id.org/italia/social-security/onto/socialSafetyNet/emetteAttoDiNotificaViolazione">
        <rdf:type rdf:resource="http://www.w3.org/2002/07/owl#InverseFunctionalProperty"/>
        <rdfs:domain rdf:resource="https://w3id.org/italia/social-security/onto/socialSafetyNet/UfficioDelLavoro"/>
        <rdfs:range rdf:resource="https://w3id.org/italia/social-security/onto/socialSafetyNet/AttoDiNotificaViolazioneObblighiAttivazione"/>
        <rdfs:comment xml:lang="en">Property that links a Labour office to a Activations obligations breach notification deed issued by it. The deed can only be linked to one Employment centre.</rdfs:comment>
        <rdfs:comment xml:lang="it">Proprietà che lega un Ufficio del lavoro a un Atto di notifica violazione obblighi attivazione dallo stesso emesso. L&apos;atto può essere legato ad un solo Ufficio del lavoro.</rdfs:comment>
        <rdfs:label xml:lang="it">emette atto di notifica violazione</rdfs:label>
        <rdfs:label xml:lang="en">issues breach notification deed</rdfs:label>
    </owl:ObjectProperty>



    <!-- https://w3id.org/italia/social-security/onto/socialSafetyNet/forniscePrestazioneLavorativa -->

    <owl:ObjectProperty rdf:about="https://w3id.org/italia/social-security/onto/socialSafetyNet/forniscePrestazioneLavorativa">
        <rdf:type rdf:resource="http://www.w3.org/2002/07/owl#InverseFunctionalProperty"/>
        <rdfs:domain rdf:resource="https://w3id.org/italia/social-security/onto/socialSafetyNet/Lavoratore"/>
        <rdfs:range rdf:resource="https://w3id.org/italia/social-security/onto/socialSafetyNet/RapportoDiLavoro"/>
        <rdfs:comment xml:lang="en">Property that links a Worker to a Work Relationship. Each Work Relationship instance is linked to a single Worker instance.</rdfs:comment>
        <rdfs:comment xml:lang="it">Proprietà che lega un Lavoratore a un Rapporto di lavoro. Ciascuna istanza di Rapporto di lavoro è legata ad una unica istanza di Lavoratore.</rdfs:comment>
        <rdfs:label xml:lang="it">fornisce prestazione lavorativa</rdfs:label>
        <rdfs:label xml:lang="en">provides work</rdfs:label>
    </owl:ObjectProperty>



    <!-- https://w3id.org/italia/social-security/onto/socialSafetyNet/generaDecadenzaNASpI -->

    <owl:ObjectProperty rdf:about="https://w3id.org/italia/social-security/onto/socialSafetyNet/generaDecadenzaNASpI">
        <rdf:type rdf:resource="http://www.w3.org/2002/07/owl#FunctionalProperty"/>
        <rdf:type rdf:resource="http://www.w3.org/2002/07/owl#InverseFunctionalProperty"/>
        <rdfs:domain rdf:resource="https://w3id.org/italia/social-security/onto/socialSafetyNet/AttoDiDecadenzaNASpI"/>
        <rdfs:range rdf:resource="https://w3id.org/italia/social-security/onto/socialSafetyNet/StatoDiDecadutoDiNASpI"/>
        <rdfs:comment xml:lang="en">Property that links a NASpI forfeiture deed to one and only one NASpI forfeiture status.</rdfs:comment>
        <rdfs:comment xml:lang="it">Proprietà che lega un Atto di decadenza NASpI a uno e un solo Stato di decaduto di NASpI.</rdfs:comment>
        <rdfs:label xml:lang="it">genera decadenza NASpI</rdfs:label>
        <rdfs:label xml:lang="en">generates NASpI forfeiture</rdfs:label>
    </owl:ObjectProperty>



    <!-- https://w3id.org/italia/social-security/onto/socialSafetyNet/generaSospensioneNASpI -->

    <owl:ObjectProperty rdf:about="https://w3id.org/italia/social-security/onto/socialSafetyNet/generaSospensioneNASpI">
        <rdf:type rdf:resource="http://www.w3.org/2002/07/owl#FunctionalProperty"/>
        <rdf:type rdf:resource="http://www.w3.org/2002/07/owl#InverseFunctionalProperty"/>
        <rdfs:domain rdf:resource="https://w3id.org/italia/social-security/onto/socialSafetyNet/ComunicazioneEventoNASpI"/>
        <rdfs:range rdf:resource="https://w3id.org/italia/social-security/onto/socialSafetyNet/StatoDiSospesoDiNASpI"/>
        <rdfs:comment xml:lang="en">Property that links a NASpI event communication to one and only one NASpI suspended status.</rdfs:comment>
        <rdfs:comment xml:lang="it">Proprietà che lega una Comunicazione evento NASpI a uno e un solo Stato di sospeso di NASpI.</rdfs:comment>
        <rdfs:label xml:lang="it">genera sospensione NASpI</rdfs:label>
        <rdfs:label xml:lang="en">generates NASpI suspension</rdfs:label>
    </owl:ObjectProperty>



    <!-- https://w3id.org/italia/social-security/onto/socialSafetyNet/generaStatoDiDisoccupazione -->

    <owl:ObjectProperty rdf:about="https://w3id.org/italia/social-security/onto/socialSafetyNet/generaStatoDiDisoccupazione">
        <rdf:type rdf:resource="http://www.w3.org/2002/07/owl#FunctionalProperty"/>
        <rdfs:domain rdf:resource="https://w3id.org/italia/social-security/onto/socialSafetyNet/AttoDiCessazioneRapportoDiLavoro"/>
        <rdfs:range rdf:resource="https://w3id.org/italia/social-security/onto/socialSafetyNet/StatoDiDisoccupazione"/>
        <rdfs:comment xml:lang="en">Property that links a Employment termination deed to a Unemployment status. Each Employment termination deed instance is linked to a single Unemployment status instance.</rdfs:comment>
        <rdfs:comment xml:lang="it">Proprietà che lega un Atto di cessazione rapporto di lavoro a un Stato di disoccupazione. Ciascuna istanza di Atto di cessazione rapporto di lavoro è legata ad una unica istanza di Stato di disoccupazione.</rdfs:comment>
        <rdfs:label xml:lang="it">genera stato di disoccupazione</rdfs:label>
        <rdfs:label xml:lang="en">generates unemployment status</rdfs:label>
    </owl:ObjectProperty>



    <!-- https://w3id.org/italia/social-security/onto/socialSafetyNet/haAlboProfessionale -->

    <owl:ObjectProperty rdf:about="https://w3id.org/italia/social-security/onto/socialSafetyNet/haAlboProfessionale">
        <rdf:type rdf:resource="http://www.w3.org/2002/07/owl#InverseFunctionalProperty"/>
        <rdfs:domain rdf:resource="https://w3id.org/italia/social-security/onto/socialSafetyNet/OrdineProfessionale"/>
        <rdfs:range rdf:resource="https://w3id.org/italia/social-security/onto/socialSafetyNet/AlboProfessionale"/>
        <rdfs:comment xml:lang="en">Property that links a Professional association to a Professional Register. Each Professional Register instance is linked to a single Professional association instance.</rdfs:comment>
        <rdfs:comment xml:lang="it">Proprietà che lega un Ordine professionale a un Albo professionale. Ciascuna istanza di Albo professionale è legata ad una unica istanza di Ordine professionale.</rdfs:comment>
        <rdfs:label xml:lang="it">ha albo professionale</rdfs:label>
        <rdfs:label xml:lang="en">has professional register</rdfs:label>
    </owl:ObjectProperty>



    <!-- https://w3id.org/italia/social-security/onto/socialSafetyNet/haAlboProfessionaleLocalizzatoIn -->

    <owl:ObjectProperty rdf:about="https://w3id.org/italia/social-security/onto/socialSafetyNet/haAlboProfessionaleLocalizzatoIn">
        <rdf:type rdf:resource="http://www.w3.org/2002/07/owl#FunctionalProperty"/>
        <rdfs:domain rdf:resource="https://w3id.org/italia/social-security/onto/socialSafetyNet/AlboProfessionale"/>
        <rdfs:range rdf:resource="https://w3id.org/italia/onto/CLV/Province"/>
        <rdfs:comment xml:lang="en">Property that links a Professional register to the Province or to the territory of relevance. Each instance of the Professional register is linked to a single Province.</rdfs:comment>
        <rdfs:comment xml:lang="it">Proprietà che lega un Albo professionale alla Provincia ovvero al territorio di pertinenza. Ciascuna istanza di Albo professionale è legata ad una unica Provincia.</rdfs:comment>
        <rdfs:label xml:lang="it">ha albo professionale localizzato in</rdfs:label>
        <rdfs:label xml:lang="en">has professional register located in</rdfs:label>
    </owl:ObjectProperty>



    <!-- https://w3id.org/italia/social-security/onto/socialSafetyNet/haAllegatoPerNASPI -->

    <owl:ObjectProperty rdf:about="https://w3id.org/italia/social-security/onto/socialSafetyNet/haAllegatoPerNASPI">
        <rdf:type rdf:resource="http://www.w3.org/2002/07/owl#InverseFunctionalProperty"/>
        <rdfs:domain>
            <owl:Class>
                <owl:unionOf rdf:parseType="Collection">
                    <rdf:Description rdf:about="https://w3id.org/italia/social-security/onto/socialSafetyNet/ComunicazioneNASpI"/>
                    <rdf:Description rdf:about="https://w3id.org/italia/social-security/onto/socialSafetyNet/DomandaNASpI"/>
                </owl:unionOf>
            </owl:Class>
        </rdfs:domain>
        <rdfs:range rdf:resource="https://w3id.org/italia/social-security/onto/pensions/DocumentoAllegato"/>
        <rdfs:comment xml:lang="en">Property that links a NASpI claim or NASpI Communication to an attached document. Each document is linked to a single NASpI application or communication.</rdfs:comment>
        <rdfs:comment xml:lang="it">Proprietà che lega una Domanda NASpI o una Comunicazione NASpI a un documento allegato. Ciascun documento è legato ad una unica domanda o comunicazione NASpI.</rdfs:comment>
        <rdfs:label xml:lang="it">ha allegato per NASPI</rdfs:label>
        <rdfs:label xml:lang="en">has attached for NASPI</rdfs:label>
    </owl:ObjectProperty>



    <!-- https://w3id.org/italia/social-security/onto/socialSafetyNet/haAttivitàCorrente -->

    <owl:ObjectProperty rdf:about="https://w3id.org/italia/social-security/onto/socialSafetyNet/haAttivitàCorrente">
        <rdf:type rdf:resource="http://www.w3.org/2002/07/owl#InverseFunctionalProperty"/>
        <rdfs:domain rdf:resource="https://w3id.org/italia/social-security/onto/socialSafetyNet/DomandaNASpI"/>
        <rdfs:range rdf:resource="https://w3id.org/italia/social-security/onto/socialSafetyNet/AttivitàCorrente"/>
        <rdfs:comment xml:lang="en">Property that links a NASpI claim to a Current activity. Each Current activity instance is linked to a single NASpI claim instance.</rdfs:comment>
        <rdfs:comment xml:lang="it">Proprietà che lega una Domanda NASpI a una Attività corrente. Ciascuna istanza di Attività corrente è legata ad una unica istanza di Domanda NASpI.</rdfs:comment>
        <rdfs:label xml:lang="it">ha attività corrente</rdfs:label>
        <rdfs:label xml:lang="en">has current activity</rdfs:label>
    </owl:ObjectProperty>



    <!-- https://w3id.org/italia/social-security/onto/socialSafetyNet/haAttoDiCessazioneRapportoDiLavoro -->

    <owl:ObjectProperty rdf:about="https://w3id.org/italia/social-security/onto/socialSafetyNet/haAttoDiCessazioneRapportoDiLavoro">
        <rdfs:domain rdf:resource="https://w3id.org/italia/social-security/onto/socialSafetyNet/RapportoDiLavoro"/>
        <rdfs:range rdf:resource="https://w3id.org/italia/social-security/onto/socialSafetyNet/AttoDiCessazioneRapportoDiLavoro"/>
        <rdfs:comment xml:lang="en">Property that links a Work Relationship to a Employment termination deed.</rdfs:comment>
        <rdfs:comment xml:lang="it">Proprietà che lega un Rapporto di lavoro a un Atto di cessazione rapporto di lavoro.</rdfs:comment>
        <rdfs:label xml:lang="it">ha atto di cessazione rapporto di lavoro</rdfs:label>
        <rdfs:label xml:lang="en">has dismissal deed</rdfs:label>
    </owl:ObjectProperty>



    <!-- https://w3id.org/italia/social-security/onto/socialSafetyNet/haAttoDiNotificaViolazione -->

    <owl:ObjectProperty rdf:about="https://w3id.org/italia/social-security/onto/socialSafetyNet/haAttoDiNotificaViolazione">
        <rdf:type rdf:resource="http://www.w3.org/2002/07/owl#InverseFunctionalProperty"/>
        <rdfs:domain rdf:resource="https://w3id.org/italia/social-security/onto/socialSafetyNet/SanzionePerViolazioneObblighiNASpI"/>
        <rdfs:range rdf:resource="https://w3id.org/italia/social-security/onto/socialSafetyNet/AttoDiNotificaViolazioneObblighiAttivazione"/>
        <rdfs:comment xml:lang="en">Property that links a NASpI Breach Penalty Fee to an Activations obligations breach notification deed. Each application for an Activations obligations breach notification deed is linked to a single NASpI Breach Penalty Fee.</rdfs:comment>
        <rdfs:comment xml:lang="it">Proprietà che lega una Sanzione per violazione obblighi NASpI ha un Atto di notifica violazione obblighi attivazione . Ciascuna istanza di Atto di notifica violazione obblighi attivazione è legata ad una unica istanza di Sanzione per violazione obblighi NASpI.</rdfs:comment>
        <rdfs:label xml:lang="it">ha atto di notifica violazione</rdfs:label>
        <rdfs:label xml:lang="en">has breach notification deed</rdfs:label>
    </owl:ObjectProperty>



    <!-- https://w3id.org/italia/social-security/onto/socialSafetyNet/haAttoDiRicorsoDomandaNASpI -->

    <owl:ObjectProperty rdf:about="https://w3id.org/italia/social-security/onto/socialSafetyNet/haAttoDiRicorsoDomandaNASpI">
        <rdf:type rdf:resource="http://www.w3.org/2002/07/owl#FunctionalProperty"/>
        <rdf:type rdf:resource="http://www.w3.org/2002/07/owl#InverseFunctionalProperty"/>
        <rdfs:domain rdf:resource="https://w3id.org/italia/social-security/onto/socialSafetyNet/StatoDiRicorsoDiDomandaNASpI"/>
        <rdfs:range rdf:resource="https://w3id.org/italia/social-security/onto/socialSafetyNet/AttoDiRicorsoDomandaNASpI"/>
        <rdfs:comment xml:lang="en">Property that links a NASpI claim appeal deed to one and only one NASpI claim appeal status.</rdfs:comment>
        <rdfs:comment xml:lang="it">Proprietà che lega un Atto di ricorso domanda NASpI a uno e un solo Stato di ricorso domanda di NASpI.</rdfs:comment>
        <rdfs:label xml:lang="it">ha atto di ricorso domanda NASpI</rdfs:label>
        <rdfs:label xml:lang="en">has NASpI claim appeal deed</rdfs:label>
    </owl:ObjectProperty>



    <!-- https://w3id.org/italia/social-security/onto/socialSafetyNet/haAttoDiRiesameDomandaNASpI -->

    <owl:ObjectProperty rdf:about="https://w3id.org/italia/social-security/onto/socialSafetyNet/haAttoDiRiesameDomandaNASpI">
        <rdf:type rdf:resource="http://www.w3.org/2002/07/owl#FunctionalProperty"/>
        <rdf:type rdf:resource="http://www.w3.org/2002/07/owl#InverseFunctionalProperty"/>
        <rdfs:domain rdf:resource="https://w3id.org/italia/social-security/onto/socialSafetyNet/StatoDiRiesameDiDomandaNASpI"/>
        <rdfs:range rdf:resource="https://w3id.org/italia/social-security/onto/socialSafetyNet/AttoDiRiesameDomandaNASpI"/>
        <rdfs:comment xml:lang="en">Property that links a NASpI claim review deed to one and only one NASpI claim review status.</rdfs:comment>
        <rdfs:comment xml:lang="it">Proprietà che lega un Atto di riesame domanda NASpI a uno e un solo Stato di riesame domanda di NASpI.</rdfs:comment>
        <rdfs:label xml:lang="it">ha atto di riesame domanda NASpI</rdfs:label>
        <rdfs:label xml:lang="en">has NASpI claim review deed</rdfs:label>
    </owl:ObjectProperty>



    <!-- https://w3id.org/italia/social-security/onto/socialSafetyNet/haBeneficiarioPrestazioneDiSostegnoAlReddito -->

    <owl:ObjectProperty rdf:about="https://w3id.org/italia/social-security/onto/socialSafetyNet/haBeneficiarioPrestazioneDiSostegnoAlReddito">
        <rdf:type rdf:resource="http://www.w3.org/2002/07/owl#FunctionalProperty"/>
        <rdfs:domain rdf:resource="https://w3id.org/italia/social-security/onto/socialSafetyNet/PrestazioneDiSostegnoAlReddito"/>
        <rdfs:range rdf:resource="https://w3id.org/italia/social-security/onto/socialSafetyNet/BeneficiarioPrestazioneDiSostegnoAlReddito"/>
        <rdfs:comment xml:lang="en">Property that links a Income support benefit to a Income support subsidy beneficiary. Each Income support benefit instance is linked to a single Income support subsidy beneficiary instance.</rdfs:comment>
        <rdfs:comment xml:lang="it">Proprietà che lega una Prestazione di sostegno al reddito a un Beneficiario prestazione di sostegno al reddito. Ciascuna istanza di Prestazione di sostegno al reddito è legata ad una unica istanza di Beneficiario prestazione di sostegno al reddito.</rdfs:comment>
        <rdfs:label xml:lang="it">ha beneficiario prestazione di sostegno al reddito</rdfs:label>
        <rdfs:label xml:lang="en">has income support beneficiary</rdfs:label>
    </owl:ObjectProperty>



    <!-- https://w3id.org/italia/social-security/onto/socialSafetyNet/haCPI -->

    <owl:ObjectProperty rdf:about="https://w3id.org/italia/social-security/onto/socialSafetyNet/haCPI">
        <rdf:type rdf:resource="http://www.w3.org/2002/07/owl#FunctionalProperty"/>
        <rdfs:domain rdf:resource="https://w3id.org/italia/social-security/onto/socialSafetyNet/DichiarazioneDiImmediataDisponibilità"/>
        <rdfs:range rdf:resource="https://w3id.org/italia/social-security/onto/socialSafetyNet/CentroPerLImpiego"/>
        <rdfs:comment xml:lang="en">Property that links a Declaration of immediate availability to an Employment centre, the one with which the Worker who signed the declaration has entered into the Personalized Service Agreement and which follows the worker&apos;s re-integration process. Each Declaration of immediate availability instance is linked to a single Employment centre instance.</rdfs:comment>
        <rdfs:comment xml:lang="it">Proprietà che lega una Dichiarazione di immediata disponibilità a un Centro per l&apos;impiego, quello con cui il Lavoratore che ha sottoscritto la dichiarazione ha stipulato il Patto di Servizio Personalizzato e che segue il percorso di re-inserimento del lavoratore . Ciascuna istanza di Dichiarazione di immediata disponibilità è legata ad una unica istanza di Centro per l&apos;impiego.</rdfs:comment>
        <rdfs:label xml:lang="it">ha CPI</rdfs:label>
        <rdfs:label xml:lang="en">has CPI</rdfs:label>
    </owl:ObjectProperty>



    <!-- https://w3id.org/italia/social-security/onto/socialSafetyNet/haComunicazioneEventiInEspatrio -->

    <owl:ObjectProperty rdf:about="https://w3id.org/italia/social-security/onto/socialSafetyNet/haComunicazioneEventiInEspatrio">
        <rdf:type rdf:resource="http://www.w3.org/2002/07/owl#InverseFunctionalProperty"/>
        <rdfs:domain rdf:resource="https://w3id.org/italia/social-security/onto/socialSafetyNet/StatoDiErogatoInEspatrioDiNASpI"/>
        <rdfs:range rdf:resource="https://w3id.org/italia/social-security/onto/socialSafetyNet/AttoDiNotificaEventoInEspatrio"/>
        <rdfs:comment xml:lang="en">Property that links a NASpI expatriate disbursed status to a Expatriation event notification deed. Each application for a Expatriation event notification deed is linked to a single application for the NASpI expatriate disbursed status.</rdfs:comment>
        <rdfs:comment xml:lang="it">Proprietà che lega una Stato di erogato in espatrio di NASpI a un Atto di notifica evento in espatrio. Ciascuna istanza di Atto di notifica evento in espatrio è legata ad una unica istanza di Stato di erogato in espatrio di NASpI.</rdfs:comment>
        <rdfs:label xml:lang="it">ha comunicazione eventi in espatrio</rdfs:label>
        <rdfs:label xml:lang="en">has communication events in expatriation</rdfs:label>
    </owl:ObjectProperty>



    <!-- https://w3id.org/italia/social-security/onto/socialSafetyNet/haComunicazioneNASpI -->

    <owl:ObjectProperty rdf:about="https://w3id.org/italia/social-security/onto/socialSafetyNet/haComunicazioneNASpI">
        <rdf:type rdf:resource="http://www.w3.org/2002/07/owl#InverseFunctionalProperty"/>
        <rdfs:domain rdf:resource="https://w3id.org/italia/social-security/onto/socialSafetyNet/PrestazioneNASpI"/>
        <rdfs:domain>
            <owl:Restriction>
                <owl:onProperty rdf:resource="https://w3id.org/italia/social-security/onto/socialSafetyNet/haStatoDiPrestazioneNASpI"/>
                <owl:allValuesFrom>
                    <owl:Class>
                        <owl:unionOf rdf:parseType="Collection">
                            <rdf:Description rdf:about="https://w3id.org/italia/social-security/onto/socialSafetyNet/StatoDiErogatoDiNASpI"/>
                            <rdf:Description rdf:about="https://w3id.org/italia/social-security/onto/socialSafetyNet/StatoDiSospesoDiNASpI"/>
                        </owl:unionOf>
                    </owl:Class>
                </owl:allValuesFrom>
            </owl:Restriction>
        </rdfs:domain>
        <rdfs:range rdf:resource="https://w3id.org/italia/social-security/onto/socialSafetyNet/ComunicazioneNASpI"/>
        <rdfs:comment xml:lang="en">Property that links a NASpI benefit to a NASpI communication. Each NASpI communication instance is linked to a single NASpI benefit instance.</rdfs:comment>
        <rdfs:comment xml:lang="it">Proprietà che lega una Prestazione NASpI a una Comunicazione NASpI. Ciascuna istanza di Comunicazione NASpI è legata ad una unica istanza di Prestazione NASpI.</rdfs:comment>
        <rdfs:label xml:lang="it">ha comunicazione NASpI</rdfs:label>
        <rdfs:label xml:lang="en">has NASpI communication</rdfs:label>
    </owl:ObjectProperty>



    <!-- https://w3id.org/italia/social-security/onto/socialSafetyNet/haContributoObbligatorio -->

    <owl:ObjectProperty rdf:about="https://w3id.org/italia/social-security/onto/socialSafetyNet/haContributoObbligatorio">
        <rdf:type rdf:resource="http://www.w3.org/2002/07/owl#InverseFunctionalProperty"/>
        <rdfs:domain rdf:resource="https://w3id.org/italia/social-security/onto/socialSafetyNet/ContrattoDiLavoro"/>
        <rdfs:range rdf:resource="https://w3id.org/italia/social-security/onto/socialSafetyNet/ContributoObbligatorio"/>
        <rdfs:comment xml:lang="en">Property that links a Work contract to a Mandatory contribution. Each Mandatory contribution instance is linked to a single Work contract instance.</rdfs:comment>
        <rdfs:comment xml:lang="it">Proprietà che lega un Contratto di lavoro a un Contributo obbligatorio. Ciascuna istanza di Contributo obbligatorio è legata ad una unica istanza di Contratto di lavoro.</rdfs:comment>
        <rdfs:label xml:lang="it">ha contributo obbligatorio</rdfs:label>
        <rdfs:label xml:lang="en">has mandatory contribution</rdfs:label>
    </owl:ObjectProperty>



    <!-- https://w3id.org/italia/social-security/onto/socialSafetyNet/haContributoPrevidenziale -->

    <owl:ObjectProperty rdf:about="https://w3id.org/italia/social-security/onto/socialSafetyNet/haContributoPrevidenziale">
        <rdf:type rdf:resource="http://www.w3.org/2002/07/owl#InverseFunctionalProperty"/>
        <rdfs:domain rdf:resource="https://w3id.org/italia/social-security/onto/socialSafetyNet/Lavoratore"/>
        <rdfs:range rdf:resource="https://w3id.org/italia/social-security/onto/socialSafetyNet/ContributoPrevidenziale"/>
        <rdfs:comment xml:lang="en">Property that links a Worker to a Social security contribution. Each Social security contribution instance is linked to a single Worker instance.</rdfs:comment>
        <rdfs:comment xml:lang="it">Proprietà che lega un Lavoratore a un Contributo previdenziale. Ciascuna istanza di Contributo previdenziale è legata ad una unica istanza di Lavoratore.</rdfs:comment>
        <rdfs:label xml:lang="it">ha contributo previdenziale</rdfs:label>
        <rdfs:label xml:lang="en">has social security contribution</rdfs:label>
    </owl:ObjectProperty>



    <!-- https://w3id.org/italia/social-security/onto/socialSafetyNet/haContributoUtilePerNASpI -->

    <owl:ObjectProperty rdf:about="https://w3id.org/italia/social-security/onto/socialSafetyNet/haContributoUtilePerNASpI">
        <rdfs:domain rdf:resource="https://w3id.org/italia/social-security/onto/socialSafetyNet/DomandaNASpI"/>
        <rdfs:range rdf:resource="https://w3id.org/italia/social-security/onto/socialSafetyNet/ContributoObbligatorio"/>
        <rdfs:comment xml:lang="en">Property that links a NASpI claim to a Mandatory contribution</rdfs:comment>
        <rdfs:comment xml:lang="it">Proprietà che lega un Domanda NASpI a un Contributo obbligatorio.</rdfs:comment>
        <rdfs:label xml:lang="it">ha contributo utile per NASpI</rdfs:label>
        <rdfs:label xml:lang="en">has NASpI useful contribution</rdfs:label>
    </owl:ObjectProperty>



    <!-- https://w3id.org/italia/social-security/onto/socialSafetyNet/haDID -->

    <owl:ObjectProperty rdf:about="https://w3id.org/italia/social-security/onto/socialSafetyNet/haDID">
        <rdf:type rdf:resource="http://www.w3.org/2002/07/owl#FunctionalProperty"/>
        <rdf:type rdf:resource="http://www.w3.org/2002/07/owl#InverseFunctionalProperty"/>
        <rdfs:domain>
            <owl:Restriction>
                <owl:onProperty rdf:resource="https://w3id.org/italia/social-security/onto/socialSafetyNet/haStatoDiLavoro"/>
                <owl:someValuesFrom>
                    <owl:Class>
                        <owl:unionOf rdf:parseType="Collection">
                            <rdf:Description rdf:about="https://w3id.org/italia/social-security/onto/socialSafetyNet/StatoDiDisoccupazione"/>
                            <rdf:Description rdf:about="https://w3id.org/italia/social-security/onto/socialSafetyNet/StatoDiInoccupazione"/>
                        </owl:unionOf>
                    </owl:Class>
                </owl:someValuesFrom>
            </owl:Restriction>
        </rdfs:domain>
        <rdfs:range rdf:resource="https://w3id.org/italia/social-security/onto/socialSafetyNet/DichiarazioneDiImmediataDisponibilità"/>
        <rdfs:comment xml:lang="en">Property that obligatorily and unequivocally links an Unemployed or a First-time jobseeker to his or her Declaration of Immediate Availability (DID).</rdfs:comment>
        <rdfs:comment xml:lang="it">Proprietà che lega obbligatoriamente e univocamente un Disoccupato o un Inoccupato alla propria Dichiarazione di Immediata Disponibilità (DID).</rdfs:comment>
        <rdfs:label xml:lang="it">ha DID</rdfs:label>
        <rdfs:label xml:lang="en">has DID</rdfs:label>
    </owl:ObjectProperty>



    <!-- https://w3id.org/italia/social-security/onto/socialSafetyNet/haDelegaRiscossionePer -->

    <owl:ObjectProperty rdf:about="https://w3id.org/italia/social-security/onto/socialSafetyNet/haDelegaRiscossionePer">
        <rdf:type rdf:resource="http://www.w3.org/2002/07/owl#FunctionalProperty"/>
        <rdfs:domain rdf:resource="https://w3id.org/italia/social-security/onto/socialSafetyNet/VariazioneDelegaRiscossioneContributiSindacaliNASpI"/>
        <rdfs:range rdf:resource="https://w3id.org/italia/social-security/onto/socialSafetyNet/AssociazioneSindacale"/>
        <rdfs:comment xml:lang="en">Property that links a NASpI union contributions collection proxy change to a Trade union association. Each NASpI union contributions collection proxy change instance is linked to a single Trade union association instance.</rdfs:comment>
        <rdfs:comment xml:lang="it">Proprietà che lega una Variazione delega riscossione contributi sindacali NASpI a una Associazione sindacale. Ciascuna istanza di Variazione delega riscossione contributi sindacali NASpI è legata ad una unica istanza di Associazione sindacale.</rdfs:comment>
        <rdfs:label xml:lang="it">ha delega riscossione per</rdfs:label>
        <rdfs:label xml:lang="en">has delegated collection for</rdfs:label>
    </owl:ObjectProperty>



    <!-- https://w3id.org/italia/social-security/onto/socialSafetyNet/haDelegatoDomandaNASpI -->

    <owl:ObjectProperty rdf:about="https://w3id.org/italia/social-security/onto/socialSafetyNet/haDelegatoDomandaNASpI">
        <rdf:type rdf:resource="http://www.w3.org/2002/07/owl#FunctionalProperty"/>
        <rdfs:domain rdf:resource="https://w3id.org/italia/social-security/onto/socialSafetyNet/DomandaNASpI"/>
        <rdfs:range rdf:resource="https://w3id.org/italia/social-security/onto/socialSafetyNet/DelegatoDomandaNASpI"/>
        <rdfs:comment xml:lang="en">Property that links a NASpI claim to a NASpI claim delegate. Each NASpI claim instance is linked to a single NASpI claim delegate instance.</rdfs:comment>
        <rdfs:comment xml:lang="it">Proprietà che lega una Domanda NASpI a un Delegato domanda NASpI. Ciascuna istanza di Domanda NASpI è legata ad una unica istanza di Delegato domanda NASpI.</rdfs:comment>
        <rdfs:label xml:lang="it">ha delegato domanda NASpI</rdfs:label>
        <rdfs:label xml:lang="en">has NASpI claim delegate</rdfs:label>
    </owl:ObjectProperty>



    <!-- https://w3id.org/italia/social-security/onto/socialSafetyNet/haDestinatarioDomandaNASpI -->

    <owl:ObjectProperty rdf:about="https://w3id.org/italia/social-security/onto/socialSafetyNet/haDestinatarioDomandaNASpI">
        <rdf:type rdf:resource="http://www.w3.org/2002/07/owl#FunctionalProperty"/>
        <rdfs:domain rdf:resource="https://w3id.org/italia/social-security/onto/socialSafetyNet/DomandaNASpI"/>
        <rdfs:range rdf:resource="https://w3id.org/italia/social-security/onto/core/SedeINPS"/>
        <rdfs:comment xml:lang="en">Property that links a NASpI Application to the recipient INPS office on the basis of territorial jurisdiction. Each NASpI application is linked to a single INPS office of destination.</rdfs:comment>
        <rdfs:comment xml:lang="it">Proprietà che lega una Domanda NASpI alla Sede INPS destinataria sulla base della competenza territoriale. Ciascuna istanza di Domanda NASpI è legata ad una unica Sede INPS di destinazione.</rdfs:comment>
        <rdfs:label xml:lang="it">ha destinatario domanda NASpI</rdfs:label>
        <rdfs:label xml:lang="en">has NASpI claim recipient</rdfs:label>
    </owl:ObjectProperty>



    <!-- https://w3id.org/italia/social-security/onto/socialSafetyNet/haDichiarazionePerNASpI -->

    <owl:ObjectProperty rdf:about="https://w3id.org/italia/social-security/onto/socialSafetyNet/haDichiarazionePerNASpI">
        <rdf:type rdf:resource="http://www.w3.org/2002/07/owl#InverseFunctionalProperty"/>
        <rdfs:domain rdf:resource="https://w3id.org/italia/social-security/onto/socialSafetyNet/DomandaNASpI"/>
        <rdfs:range rdf:resource="https://w3id.org/italia/social-security/onto/pensions/Dichiarazione"/>
        <rdfs:comment xml:lang="en">Property that links a NASpI claim to a Declaration signed by the applicant submitting it. Each Declaration application is linked to a single NASpI claim.</rdfs:comment>
        <rdfs:comment xml:lang="it">Proprietà che lega una Domanda NASpI ad una Dichiarazione sottoscritta dal richiedente che la presenta. Ciascuna istanza di Dichiarazione è legata ad una unica Domanda NASpI.</rdfs:comment>
        <rdfs:label xml:lang="it">ha dichiarazione per NASpI</rdfs:label>
        <rdfs:label xml:lang="en">has statement for NASpI</rdfs:label>
    </owl:ObjectProperty>



    <!-- https://w3id.org/italia/social-security/onto/socialSafetyNet/haDomandaNASpI -->

    <owl:ObjectProperty rdf:about="https://w3id.org/italia/social-security/onto/socialSafetyNet/haDomandaNASpI">
        <rdf:type rdf:resource="http://www.w3.org/2002/07/owl#FunctionalProperty"/>
        <rdf:type rdf:resource="http://www.w3.org/2002/07/owl#InverseFunctionalProperty"/>
        <rdfs:domain rdf:resource="https://w3id.org/italia/social-security/onto/socialSafetyNet/PrestazioneNASpI"/>
        <rdfs:range rdf:resource="https://w3id.org/italia/social-security/onto/socialSafetyNet/DomandaNASpI"/>
        <rdfs:comment xml:lang="en">A property that uniquely links a NASpI benefit to its NASpI claim.</rdfs:comment>
        <rdfs:comment xml:lang="it">Proprietà che lega univocamente una Prestazione NASpI alla sua Domanda NASpI.</rdfs:comment>
        <rdfs:label xml:lang="it">ha domanda NASpI</rdfs:label>
        <rdfs:label xml:lang="en">has NASpI claim</rdfs:label>
    </owl:ObjectProperty>



    <!-- https://w3id.org/italia/social-security/onto/socialSafetyNet/haDomicilioPerNASpI -->

    <owl:ObjectProperty rdf:about="https://w3id.org/italia/social-security/onto/socialSafetyNet/haDomicilioPerNASpI">
        <rdfs:subPropertyOf rdf:resource="https://w3id.org/italia/onto/CLV/hasAddress"/>
        <rdfs:domain rdf:resource="https://w3id.org/italia/social-security/onto/socialSafetyNet/DomandaNASpI"/>
        <rdfs:comment xml:lang="en">Property that links a NASpI claim to the applicant&apos;s home address.</rdfs:comment>
        <rdfs:comment xml:lang="it">Proprietà che lega una Domanda NASpI all&apos;indirizzo di domicilio del richiedente</rdfs:comment>
        <rdfs:label xml:lang="it">ha domicilio per NASpI</rdfs:label>
        <rdfs:label xml:lang="en">has NASpI domicile</rdfs:label>
    </owl:ObjectProperty>



    <!-- https://w3id.org/italia/social-security/onto/socialSafetyNet/haElencoDiAlboProfessionale -->

    <owl:ObjectProperty rdf:about="https://w3id.org/italia/social-security/onto/socialSafetyNet/haElencoDiAlboProfessionale">
        <rdf:type rdf:resource="http://www.w3.org/2002/07/owl#InverseFunctionalProperty"/>
        <rdfs:domain rdf:resource="https://w3id.org/italia/social-security/onto/socialSafetyNet/AlboProfessionale"/>
        <rdfs:range rdf:resource="https://w3id.org/italia/social-security/onto/socialSafetyNet/ElencodiAlboProfessionale"/>
        <rdfs:comment xml:lang="en">Property that links a Professional Register to a Professional register directory. Each Professional register directory instance is linked to a single Professional Register instance.</rdfs:comment>
        <rdfs:comment xml:lang="it">Proprietà che lega un Albo professionale a un Elenco di albo professionale. Ciascuna istanza di Elenco di albo professionale è legata ad una unica istanza di Albo professionale.</rdfs:comment>
        <rdfs:label xml:lang="it">ha elenco di albo professionale</rdfs:label>
        <rdfs:label xml:lang="en">has professional register directory</rdfs:label>
    </owl:ObjectProperty>



    <!-- https://w3id.org/italia/social-security/onto/socialSafetyNet/haEstrattoContoContributivo -->

    <owl:ObjectProperty rdf:about="https://w3id.org/italia/social-security/onto/socialSafetyNet/haEstrattoContoContributivo">
        <rdf:type rdf:resource="http://www.w3.org/2002/07/owl#FunctionalProperty"/>
        <rdf:type rdf:resource="http://www.w3.org/2002/07/owl#InverseFunctionalProperty"/>
        <rdfs:domain rdf:resource="https://w3id.org/italia/onto/CPV/Alive"/>
        <rdfs:range rdf:resource="https://w3id.org/italia/social-security/onto/socialSafetyNet/EstrattoContoContributivo"/>
        <rdfs:comment xml:lang="en">Property that links a living person to his or her unique Contribution account statement.</rdfs:comment>
        <rdfs:comment xml:lang="it">Proprietà che lega una Persona viva al suo unico Estratto conto contributivo.</rdfs:comment>
        <rdfs:label xml:lang="it">ha estratto conto contributivo</rdfs:label>
        <rdfs:label xml:lang="en">has contribution account statement</rdfs:label>
    </owl:ObjectProperty>



    <!-- https://w3id.org/italia/social-security/onto/socialSafetyNet/haFascicoloDiLavoro -->

    <owl:ObjectProperty rdf:about="https://w3id.org/italia/social-security/onto/socialSafetyNet/haFascicoloDiLavoro">
        <rdf:type rdf:resource="http://www.w3.org/2002/07/owl#FunctionalProperty"/>
        <rdf:type rdf:resource="http://www.w3.org/2002/07/owl#InverseFunctionalProperty"/>
        <rdfs:domain rdf:resource="https://w3id.org/italia/onto/CPV/Alive"/>
        <rdfs:range rdf:resource="https://w3id.org/italia/social-security/onto/socialSafetyNet/FascicoloDiLavoro"/>
        <rdfs:comment xml:lang="en">Property that links a living person to his or her unique Work folder.</rdfs:comment>
        <rdfs:comment xml:lang="it">Proprietà che lega una Persona viva al suo unico Fascicolo di lavoro.</rdfs:comment>
        <rdfs:label xml:lang="it">ha fascicolo di lavoro</rdfs:label>
        <rdfs:label xml:lang="en">has work folder</rdfs:label>
    </owl:ObjectProperty>



    <!-- https://w3id.org/italia/social-security/onto/socialSafetyNet/haIndirizzoInEspatrio -->

    <owl:ObjectProperty rdf:about="https://w3id.org/italia/social-security/onto/socialSafetyNet/haIndirizzoInEspatrio">
        <rdfs:subPropertyOf rdf:resource="https://w3id.org/italia/onto/CLV/hasAdressinTime"/>
        <rdfs:domain rdf:resource="https://w3id.org/italia/social-security/onto/socialSafetyNet/StatoDiErogatoInEspatrioDiNASpI"/>
        <rdfs:comment xml:lang="en">A sub-property of CLV:hasAddressInTime that indicates the address of an expatriate NASpI Beneficiary.</rdfs:comment>
        <rdfs:comment xml:lang="it">Sotto proprietà di CLV:hasAddressInTime che indica l&apos;indirizzo di un Beneficiario NASpI espatriato.</rdfs:comment>
        <rdfs:label xml:lang="it">ha indirizzo in espatrio</rdfs:label>
        <rdfs:label xml:lang="en">has address in expatriation</rdfs:label>
    </owl:ObjectProperty>



    <!-- https://w3id.org/italia/social-security/onto/socialSafetyNet/haIscrizioneAlboProfessionale -->

    <owl:ObjectProperty rdf:about="https://w3id.org/italia/social-security/onto/socialSafetyNet/haIscrizioneAlboProfessionale">
        <rdf:type rdf:resource="http://www.w3.org/2002/07/owl#InverseFunctionalProperty"/>
        <rdfs:domain rdf:resource="https://w3id.org/italia/social-security/onto/socialSafetyNet/AlboProfessionale"/>
        <rdfs:range rdf:resource="https://w3id.org/italia/social-security/onto/socialSafetyNet/IscrizioneAlboProfessionale"/>
        <rdfs:comment xml:lang="en">Property that links a Professional Register to a Professional register entry. Each Professional register entry instance is linked to a single Professional Register instance.</rdfs:comment>
        <rdfs:comment xml:lang="it">Proprietà che lega un Albo professionale a un Iscrizione albo professionale. Ciascuna istanza di Iscrizione albo professionale è legata ad una unica istanza di Albo professionale.</rdfs:comment>
        <rdfs:label xml:lang="it">ha iscrizione albo professionale</rdfs:label>
        <rdfs:label xml:lang="en">has professional register entry</rdfs:label>
    </owl:ObjectProperty>



    <!-- https://w3id.org/italia/social-security/onto/socialSafetyNet/haIscrizioneUfficioDelLavoro -->

    <owl:ObjectProperty rdf:about="https://w3id.org/italia/social-security/onto/socialSafetyNet/haIscrizioneUfficioDelLavoro">
        <rdfs:domain rdf:resource="https://w3id.org/italia/social-security/onto/socialSafetyNet/PrestazioneNASpI"/>
        <rdfs:range rdf:resource="https://w3id.org/italia/social-security/onto/socialSafetyNet/IscrizioneUfficioDelLavoro"/>
        <rdfs:comment xml:lang="en">Property that links a NASpI Benefit to at least one Labour office registration. A NASpI Beneficiary can, in general, have more than one registration, also considering the Foreign labour offices to which he is registered because he is in expatriate or because he is a Frontier worker.</rdfs:comment>
        <rdfs:comment xml:lang="it">Proprietà che lega una Prestazione NASpI ad almeno una Iscrizione ufficio del lavoro. Un Beneficiario NASpI può, in generale, avere più iscrizioni considerando anche gli Uffici del lavoro esteri a cui è iscritto perché è in espatrio o perché è un Lavoratore frontaliero.</rdfs:comment>
        <rdfs:label xml:lang="it">ha iscrizione ufficio del lavoro</rdfs:label>
        <rdfs:label xml:lang="en">has labour office registration</rdfs:label>
    </owl:ObjectProperty>



    <!-- https://w3id.org/italia/social-security/onto/socialSafetyNet/haModalitàDiPagamentoNASpI -->

    <owl:ObjectProperty rdf:about="https://w3id.org/italia/social-security/onto/socialSafetyNet/haModalitàDiPagamentoNASpI">
        <rdf:type rdf:resource="http://www.w3.org/2002/07/owl#FunctionalProperty"/>
        <rdfs:domain>
            <owl:Class>
                <owl:unionOf rdf:parseType="Collection">
                    <rdf:Description rdf:about="https://w3id.org/italia/social-security/onto/socialSafetyNet/DomandaNASpI"/>
                    <rdf:Description rdf:about="https://w3id.org/italia/social-security/onto/socialSafetyNet/VariazioneModalitàDiPagamentoNASpI"/>
                </owl:unionOf>
            </owl:Class>
        </rdfs:domain>
        <rdfs:range rdf:resource="https://w3id.org/italia/social-security/onto/socialSafetyNet/ModalitàDiPagamentoNASpI"/>
        <rdfs:comment xml:lang="en">Property that links a NASpI claim or NASpI Communication to its unique NASpI payment method.</rdfs:comment>
        <rdfs:comment xml:lang="it">Proprietà che lega una Domanda NASpI o una Comunicazione NASpI alla sua unica Modalità di pagamento NASpI.</rdfs:comment>
        <rdfs:label xml:lang="it">ha modalità di pagamento NASpI</rdfs:label>
        <rdfs:label xml:lang="en">has NASpI payment method</rdfs:label>
    </owl:ObjectProperty>



    <!-- https://w3id.org/italia/social-security/onto/socialSafetyNet/haMotivoCessazioneRapportoDiLavoro -->

    <owl:ObjectProperty rdf:about="https://w3id.org/italia/social-security/onto/socialSafetyNet/haMotivoCessazioneRapportoDiLavoro">
        <rdfs:domain rdf:resource="https://w3id.org/italia/social-security/onto/socialSafetyNet/AttoDiCessazioneRapportoDiLavoro"/>
        <rdfs:range rdf:resource="https://w3id.org/italia/social-security/onto/socialSafetyNet/MotivoCessazioneRapportoDiLavoro"/>
        <rdfs:comment xml:lang="en">Property that links a Employment termination deed to a Work relationship termination cause</rdfs:comment>
        <rdfs:comment xml:lang="it">Proprietà che lega un Atto di cessazione rapporto di lavoro a un Motivo cessazione rapporto di lavoro.</rdfs:comment>
        <rdfs:label xml:lang="it">ha motivo cessazione rapporto di lavoro</rdfs:label>
        <rdfs:label xml:lang="en">has dismissal cause</rdfs:label>
    </owl:ObjectProperty>



    <!-- https://w3id.org/italia/social-security/onto/socialSafetyNet/haMotivoDecadenzaDisoccupazione -->

    <owl:ObjectProperty rdf:about="https://w3id.org/italia/social-security/onto/socialSafetyNet/haMotivoDecadenzaDisoccupazione">
        <rdf:type rdf:resource="http://www.w3.org/2002/07/owl#FunctionalProperty"/>
        <rdfs:domain rdf:resource="https://w3id.org/italia/social-security/onto/socialSafetyNet/AttoDiDecadenzaStatoDiDisoccupazione"/>
        <rdfs:range rdf:resource="https://w3id.org/italia/social-security/onto/socialSafetyNet/MotivoDecadenzaDisoccupazione"/>
        <rdfs:comment xml:lang="en">Property that links a Unemployment status forfeiture deed to a Unemployment forfeiture cause. Each Unemployment status forfeiture deed instance is linked to a single Unemployment forfeiture cause instance.</rdfs:comment>
        <rdfs:comment xml:lang="it">Proprietà che lega un Atto di decadenza stato di disoccupazione a un Motivo decadenza disoccupazione. Ciascuna istanza di Atto di decadenza stato di disoccupazione è legata ad una unica istanza di Motivo decadenza disoccupazione.</rdfs:comment>
        <rdfs:label xml:lang="it">ha motivo decadenza disoccupazione</rdfs:label>
        <rdfs:label xml:lang="en">has unemployment forfeiture cause</rdfs:label>
    </owl:ObjectProperty>



    <!-- https://w3id.org/italia/social-security/onto/socialSafetyNet/haMotivoDecadenzaNASpI -->

    <owl:ObjectProperty rdf:about="https://w3id.org/italia/social-security/onto/socialSafetyNet/haMotivoDecadenzaNASpI">
        <rdf:type rdf:resource="http://www.w3.org/2002/07/owl#FunctionalProperty"/>
        <rdfs:domain rdf:resource="https://w3id.org/italia/social-security/onto/socialSafetyNet/AttoDiDecadenzaNASpI"/>
        <rdfs:range rdf:resource="https://w3id.org/italia/social-security/onto/socialSafetyNet/MotivoDecadenzaNASpI"/>
        <rdfs:comment xml:lang="en">Property that links a NASpI forfeiture deed to a NASpI forfeiture cause. Each NASpI forfeiture deed instance is linked to a single NASpI forfeiture cause instance.</rdfs:comment>
        <rdfs:comment xml:lang="it">Proprietà che lega un Atto di decadenza NASpI a un Motivo decadenza NASpI. Ciascuna istanza di Atto di decadenza NASpI è legata ad una unica istanza di Motivo decadenza NASpI.</rdfs:comment>
        <rdfs:label xml:lang="it">ha motivo decadenza NASpI</rdfs:label>
        <rdfs:label xml:lang="en">has NASpI forfeiture cause</rdfs:label>
    </owl:ObjectProperty>



    <!-- https://w3id.org/italia/social-security/onto/socialSafetyNet/haMotivoDiEspatrio -->

    <owl:ObjectProperty rdf:about="https://w3id.org/italia/social-security/onto/socialSafetyNet/haMotivoDiEspatrio">
        <rdf:type rdf:resource="http://www.w3.org/2002/07/owl#FunctionalProperty"/>
        <rdfs:domain rdf:resource="https://w3id.org/italia/social-security/onto/socialSafetyNet/EspatrioInNASpI"/>
        <rdfs:range rdf:resource="https://w3id.org/italia/social-security/onto/socialSafetyNet/MotivoDiEspatrio"/>
        <rdfs:comment xml:lang="en">Property that links a NASpI expatriation period to a Expatriation cause. Each NASpI expatriation period instance is linked to a single Expatriation cause instance.</rdfs:comment>
        <rdfs:comment xml:lang="it">Proprietà che lega un Espatrio in NASpI a un Motivo di espatrio. Ciascuna istanza di Espatrio in NASpI è legata ad una unica istanza di Motivo di espatrio.</rdfs:comment>
        <rdfs:label xml:lang="it">ha motivo di espatrio</rdfs:label>
        <rdfs:label xml:lang="en">has expatriation cause</rdfs:label>
    </owl:ObjectProperty>



    <!-- https://w3id.org/italia/social-security/onto/socialSafetyNet/haMotivoDiIndisponibilitàOperativa -->

    <owl:ObjectProperty rdf:about="https://w3id.org/italia/social-security/onto/socialSafetyNet/haMotivoDiIndisponibilitàOperativa">
        <rdf:type rdf:resource="http://www.w3.org/2002/07/owl#FunctionalProperty"/>
        <rdfs:domain>
            <owl:Class>
                <owl:unionOf rdf:parseType="Collection">
                    <rdf:Description rdf:about="https://w3id.org/italia/social-security/onto/socialSafetyNet/IndisponibilitàPerNASpI"/>
                    <rdf:Description rdf:about="https://w3id.org/italia/social-security/onto/socialSafetyNet/PrestazioneLavorativaFigurativa"/>
                </owl:unionOf>
            </owl:Class>
        </rdfs:domain>
        <rdfs:range rdf:resource="https://w3id.org/italia/social-security/onto/socialSafetyNet/MotivoDiIndisponibilitàOperativa"/>
        <rdfs:comment xml:lang="en">Property that links a period of operational unavailability to its sole motivation.</rdfs:comment>
        <rdfs:comment xml:lang="it">Proprietà che lega un periodo di indisponibilità operativa alla sua unica motivazione.</rdfs:comment>
        <rdfs:label xml:lang="it">ha motivo di indisponibilità operativa</rdfs:label>
        <rdfs:label xml:lang="en">has operational unavailability cause</rdfs:label>
    </owl:ObjectProperty>



    <!-- https://w3id.org/italia/social-security/onto/socialSafetyNet/haMotivoDiRinunciaNASpI -->

    <owl:ObjectProperty rdf:about="https://w3id.org/italia/social-security/onto/socialSafetyNet/haMotivoDiRinunciaNASpI">
        <rdf:type rdf:resource="http://www.w3.org/2002/07/owl#FunctionalProperty"/>
        <rdfs:domain rdf:resource="https://w3id.org/italia/social-security/onto/socialSafetyNet/AttoDiRinunciaAllaNASpI"/>
        <rdfs:range rdf:resource="https://w3id.org/italia/social-security/onto/socialSafetyNet/MotivoDiRinunciaNASpI"/>
        <rdfs:comment xml:lang="en">Property that links a NASpI waiver deed to a NASpI opt-out cause. Each NASpI waiver deed instance is linked to a single NASpI opt-out cause instance.</rdfs:comment>
        <rdfs:comment xml:lang="it">Proprietà che lega un Atto di rinuncia alla NASpI a un Motivo di rinuncia NASpI. Ciascuna istanza di Atto di rinuncia alla NASpI è legata ad una unica istanza di Motivo di rinuncia NASpI.</rdfs:comment>
        <rdfs:label xml:lang="it">ha motivo di rinuncia NASpI</rdfs:label>
        <rdfs:label xml:lang="en">has NASpI waiver cause</rdfs:label>
    </owl:ObjectProperty>



    <!-- https://w3id.org/italia/social-security/onto/socialSafetyNet/haMotivoSanzioneNASpI -->

    <owl:ObjectProperty rdf:about="https://w3id.org/italia/social-security/onto/socialSafetyNet/haMotivoSanzioneNASpI">
        <rdf:type rdf:resource="http://www.w3.org/2002/07/owl#FunctionalProperty"/>
        <rdfs:domain rdf:resource="https://w3id.org/italia/social-security/onto/socialSafetyNet/SanzionePerViolazioneObblighiNASpI"/>
        <rdfs:range rdf:resource="https://w3id.org/italia/social-security/onto/socialSafetyNet/MotivoSanzioneNASpI"/>
        <rdfs:comment xml:lang="en">Property that links a Sanction deed for NASpI obligations breach to a NASpI sanction cause. Each Sanction deed for NASpI obligations breach instance is linked to a single NASpI sanction cause instance.</rdfs:comment>
        <rdfs:comment xml:lang="it">Proprietà che lega un Atto di sanzione per violazione obblighi NASpI a un Motivo sanzione NASpI. Ciascuna istanza di Atto di sanzione per violazione obblighi NASpI è legata ad una unica istanza di Motivo sanzione NASpI.</rdfs:comment>
        <rdfs:label xml:lang="it">ha motivo sanzione NASpI</rdfs:label>
        <rdfs:label xml:lang="en">has NASpI sanction cause</rdfs:label>
    </owl:ObjectProperty>



    <!-- https://w3id.org/italia/social-security/onto/socialSafetyNet/haOggettoVariazioneDelegaSindacale -->

    <owl:ObjectProperty rdf:about="https://w3id.org/italia/social-security/onto/socialSafetyNet/haOggettoVariazioneDelegaSindacale">
        <rdf:type rdf:resource="http://www.w3.org/2002/07/owl#FunctionalProperty"/>
        <rdfs:domain rdf:resource="https://w3id.org/italia/social-security/onto/socialSafetyNet/VariazioneDelegaRiscossioneContributiSindacaliNASpI"/>
        <rdfs:range rdf:resource="https://w3id.org/italia/social-security/onto/socialSafetyNet/OggettoVariazioneDelegaSindacale"/>
        <rdfs:comment xml:lang="en">Property that links a NASpI union contributions collection proxy change to a Trade union proxy change subject. Each NASpI union contributions collection proxy change instance is linked to a single Trade union proxy change subject instance.</rdfs:comment>
        <rdfs:comment xml:lang="it">Proprietà che lega una Variazione delega riscossione contributi sindacali NASpI a un Oggetto variazione delega sindacale. Ciascuna istanza di Variazione delega riscossione contributi sindacali NASpI è legata ad una unica istanza di Oggetto variazione delega sindacale.</rdfs:comment>
        <rdfs:label xml:lang="it">ha oggetto variazione delega sindacale</rdfs:label>
        <rdfs:label xml:lang="en">has trade union delegation object change</rdfs:label>
    </owl:ObjectProperty>



    <!-- https://w3id.org/italia/social-security/onto/socialSafetyNet/haPeriodoDiLavoroEstero -->

    <owl:ObjectProperty rdf:about="https://w3id.org/italia/social-security/onto/socialSafetyNet/haPeriodoDiLavoroEstero">
        <rdfs:domain rdf:resource="https://w3id.org/italia/social-security/onto/socialSafetyNet/DomandaNASpI"/>
        <rdfs:range rdf:resource="https://w3id.org/italia/social-security/onto/pensions/AttivitàEstera"/>
        <rdfs:comment xml:lang="en">Property that links a NASpI claim to a Foreign activity carried out by the applicant. This activity, if carried out in an EEA State or in Switzerland or in a State with bilateral agreements with Italy, may be recognized as usable in the assessment of the requirements for access to the NASpI Benefit. To demonstrate the truthfulness of what has been declared, the applicant must submit the DP U1, failing which it will be the task of the competent INPS office to request from the foreign state body the information useful for the totalization of the periods worked abroad.</rdfs:comment>
        <rdfs:comment xml:lang="it">Proprietà che lega una Domanda NASpI a una Attività estera svolta del richiedente. Questa attività se svolta in uno Stato SEE o in Svizzera o in uno Stato con accordi bilaterali con l&apos;Italia potrà essere riconosciuta come utilizzabile nella valutazione dei requisiti di accesso alla Prestazione NASpI. A dimostrazione della veridicità di quanto dichiarato il richiedente deve presentare il DP U1 in mancanza del quale sarà compito della sede INPS competente richiedere all&apos;ente dello stato estero le informazioni utili alla totalizzazione dei periodi lavorati all&apos;estero.</rdfs:comment>
        <rdfs:label xml:lang="it">ha periodo di lavoro estero</rdfs:label>
        <rdfs:label xml:lang="en">has foreign work period</rdfs:label>
    </owl:ObjectProperty>



    <!-- https://w3id.org/italia/social-security/onto/socialSafetyNet/haPrestazioneAggiuntiva -->

    <owl:ObjectProperty rdf:about="https://w3id.org/italia/social-security/onto/socialSafetyNet/haPrestazioneAggiuntiva">
        <rdfs:domain rdf:resource="https://w3id.org/italia/social-security/onto/socialSafetyNet/PrestazioneDiSostegnoAlReddito"/>
        <rdfs:range rdf:resource="https://w3id.org/italia/social-security/onto/socialSafetyNet/PrestazioneDiSostegnoAlReddito"/>
        <rdfs:comment xml:lang="en">Property that links two Income support benefit together.</rdfs:comment>
        <rdfs:comment xml:lang="it">Proprietà che lega tra di loro due Prestazione di sostegno al reddito.</rdfs:comment>
        <rdfs:label xml:lang="it">ha prestazione aggiuntiva</rdfs:label>
        <rdfs:label xml:lang="en">has additional benefit</rdfs:label>
    </owl:ObjectProperty>



    <!-- https://w3id.org/italia/social-security/onto/socialSafetyNet/haQualifica -->

    <owl:ObjectProperty rdf:about="https://w3id.org/italia/social-security/onto/socialSafetyNet/haQualifica">
        <rdfs:domain rdf:resource="https://w3id.org/italia/social-security/onto/socialSafetyNet/LavoratoreSubordinato"/>
        <rdfs:range rdf:resource="https://w3id.org/italia/social-security/onto/socialSafetyNet/TipoDiQualifica"/>
        <rdfs:comment xml:lang="en">Property that links an Employee to a qualification valid for a Salaried employment relationship.</rdfs:comment>
        <rdfs:comment xml:lang="it">Proprietà che lega un Lavoratore subordinato ad una qualifica valida per un Rapporto di Lavoro.</rdfs:comment>
        <rdfs:label xml:lang="it">ha qualifica</rdfs:label>
        <rdfs:label xml:lang="en">has qualification</rdfs:label>
    </owl:ObjectProperty>



    <!-- https://w3id.org/italia/social-security/onto/socialSafetyNet/haRegistroDellaPrestazioneLavorativa -->

    <owl:ObjectProperty rdf:about="https://w3id.org/italia/social-security/onto/socialSafetyNet/haRegistroDellaPrestazioneLavorativa">
        <rdf:type rdf:resource="http://www.w3.org/2002/07/owl#FunctionalProperty"/>
        <rdf:type rdf:resource="http://www.w3.org/2002/07/owl#InverseFunctionalProperty"/>
        <rdfs:domain>
            <owl:Class>
                <owl:intersectionOf rdf:parseType="Collection">
                    <rdf:Description rdf:about="https://w3id.org/italia/social-security/onto/socialSafetyNet/ContrattoDiLavoroSubordinato"/>
                    <owl:Restriction>
                        <owl:onProperty>
                            <rdf:Description>
                                <owl:inverseOf rdf:resource="https://w3id.org/italia/social-security/onto/socialSafetyNet/èRegolatoDaContratto"/>
                            </rdf:Description>
                        </owl:onProperty>
                        <owl:someValuesFrom rdf:resource="https://w3id.org/italia/social-security/onto/socialSafetyNet/RapportoDiLavoro"/>
                    </owl:Restriction>
                </owl:intersectionOf>
            </owl:Class>
        </rdfs:domain>
        <rdfs:range rdf:resource="https://w3id.org/italia/social-security/onto/socialSafetyNet/RegistroDellaPrestazioneLavorativa"/>
        <rdfs:comment xml:lang="en">Property that links a Salaried employment contract to one and only one Work provision registry.</rdfs:comment>
        <rdfs:comment xml:lang="it">Proprietà che lega un Contratto di lavoro subordinato a uno e un solo Registro della prestazione lavorativa.</rdfs:comment>
        <rdfs:label xml:lang="it">ha registro della prestazione lavorativa</rdfs:label>
        <rdfs:label xml:lang="en">has work provision registry</rdfs:label>
    </owl:ObjectProperty>



    <!-- https://w3id.org/italia/social-security/onto/socialSafetyNet/haRichiedenteNASpI -->

    <owl:ObjectProperty rdf:about="https://w3id.org/italia/social-security/onto/socialSafetyNet/haRichiedenteNASpI">
        <rdf:type rdf:resource="http://www.w3.org/2002/07/owl#FunctionalProperty"/>
        <rdfs:domain rdf:resource="https://w3id.org/italia/social-security/onto/socialSafetyNet/DomandaNASpI"/>
        <rdfs:range rdf:resource="https://w3id.org/italia/social-security/onto/socialSafetyNet/RichiedenteNASpI"/>
        <rdfs:comment xml:lang="en">Property that links a NASpI claim to a NASpI Applicant. Each NASpI claim instance is linked to a single NASpI Applicant instance.</rdfs:comment>
        <rdfs:comment xml:lang="it">Proprietà che lega una Domanda NASpI a un Richiedente NASpI. Ciascuna istanza di Domanda NASpI è legata ad una unica istanza di Richiedente NASpI.</rdfs:comment>
        <rdfs:label xml:lang="it">ha richiedente NASpI</rdfs:label>
        <rdfs:label xml:lang="en">has NASpI applicant</rdfs:label>
    </owl:ObjectProperty>



    <!-- https://w3id.org/italia/social-security/onto/socialSafetyNet/haSanzioneNASpI -->

    <owl:ObjectProperty rdf:about="https://w3id.org/italia/social-security/onto/socialSafetyNet/haSanzioneNASpI">
        <rdf:type rdf:resource="http://www.w3.org/2002/07/owl#InverseFunctionalProperty"/>
        <rdfs:domain rdf:resource="https://w3id.org/italia/social-security/onto/socialSafetyNet/StatoDiErogatoDiNASpI"/>
        <rdfs:range rdf:resource="https://w3id.org/italia/social-security/onto/socialSafetyNet/SanzionePerViolazioneObblighiNASpI"/>
        <rdfs:comment xml:lang="en">Property that links a NASpI disbursement status to a NASpI Breach Penalty Fee. This sanction can be linked to only one disbursement status, the one that has been generated since the date of validity of the sanction that determines a reduction in the monthly amount disbursed.</rdfs:comment>
        <rdfs:comment xml:lang="it">Proprietà che lega uno Stato di erogato di NASpI a una Sanzione per violazione obblighi NASpI. Tale sanzione può essere legata a un solo stato di erogazione, quello che è stato generato a partire dalla data di validità della sanzione che determina un decurtamento dell&apos;importo mensile erogato.</rdfs:comment>
        <rdfs:label xml:lang="it">ha sanzione NASpI</rdfs:label>
        <rdfs:label xml:lang="en">has NASpI sanction</rdfs:label>
    </owl:ObjectProperty>



    <!-- https://w3id.org/italia/social-security/onto/socialSafetyNet/haSituazioneLavorativa -->

    <owl:ObjectProperty rdf:about="https://w3id.org/italia/social-security/onto/socialSafetyNet/haSituazioneLavorativa">
        <rdf:type rdf:resource="http://www.w3.org/2002/07/owl#FunctionalProperty"/>
        <rdfs:domain rdf:resource="https://w3id.org/italia/social-security/onto/socialSafetyNet/DomandaNASpI"/>
        <rdfs:range rdf:resource="https://w3id.org/italia/social-security/onto/socialSafetyNet/StatoDiLavoro"/>
        <rdfs:comment xml:lang="en">Property that links a NASpI claim to a Working status. Each NASpI claim instance is linked to a single Working status instance. The Working status to which the NASpI claim refers is the one valid for the use of the benefit, i.e. the last Employment status or the current Partial unemployment status.</rdfs:comment>
        <rdfs:comment xml:lang="it">Proprietà che lega una Domanda NASpI a un Stato di lavoro. Ciascuna istanza di Domanda NASpI è legata ad una unica istanza di Stato di lavoro. Lo Stato di lavoro a cui si riferisce la Domanda NASpI è quello valido per la fruizione della prestazione ovvero l&apos;ultimo Stato di occupazione o l&apos;attuale Stato di disoccupazione parziale.</rdfs:comment>
        <rdfs:label xml:lang="it">ha situazione lavorativa</rdfs:label>
        <rdfs:label xml:lang="en">has working situation</rdfs:label>
    </owl:ObjectProperty>



    <!-- https://w3id.org/italia/social-security/onto/socialSafetyNet/haStatoCompetente -->

    <owl:ObjectProperty rdf:about="https://w3id.org/italia/social-security/onto/socialSafetyNet/haStatoCompetente">
        <rdf:type rdf:resource="http://www.w3.org/2002/07/owl#FunctionalProperty"/>
        <rdfs:domain rdf:resource="https://w3id.org/italia/social-security/onto/socialSafetyNet/StatoDiLavoro"/>
        <rdfs:range rdf:resource="https://w3id.org/italia/social-security/onto/socialSafetyNet/StatoCompetente"/>
        <rdfs:comment xml:lang="en">Property that links a Working status to a Competent state. Each Working status instance is linked to a single Competent state instance. For his relationship, it is possible to establish the competence relating to the provision of the NASpI Benefit by INPS which, net of the possession of the requirements, will concern applicants who have Italy as a Competent country or are Frontier workers or other than frontier workers who, despite having a competent State other than Italy, are resident in Italy.</rdfs:comment>
        <rdfs:comment xml:lang="it">Proprietà che lega un Stato di lavoro a un Stato competente. Ciascuna istanza di Stato di lavoro è legata ad una unica istanza di Stato competente. In virtù di questa relazione è possibile stabilire la competenza relativa all&apos;erogazione della Prestazione NASpI da parte dell&apos;INPS che, al netto del possesso dei requisiti previsti, riguarderà i richiedenti che hanno l&apos;Italia come Paese Competente o sono Lavoratori frontalieri o diversi dai frontalieri che, pur avendo uno Stato competete diverso dall&apos;Italia, risultano residenti in Italia.</rdfs:comment>
        <rdfs:label xml:lang="it">ha stato competente</rdfs:label>
        <rdfs:label xml:lang="en">has competent state</rdfs:label>
    </owl:ObjectProperty>



    <!-- https://w3id.org/italia/social-security/onto/socialSafetyNet/haStatoDiDomandaNASpI -->

    <owl:ObjectProperty rdf:about="https://w3id.org/italia/social-security/onto/socialSafetyNet/haStatoDiDomandaNASpI">
        <rdf:type rdf:resource="http://www.w3.org/2002/07/owl#InverseFunctionalProperty"/>
        <rdfs:domain rdf:resource="https://w3id.org/italia/social-security/onto/socialSafetyNet/DomandaNASpI"/>
        <rdfs:range rdf:resource="https://w3id.org/italia/social-security/onto/socialSafetyNet/StatoDiDomandaNASpI"/>
        <rdfs:comment xml:lang="en">Property that links a NASpI claim to a NASpI claim status. Each NASpI claim status instance is linked to a single NASpI claim instance. This property then ties the NASpI claim to the events that characterize its life cycle.</rdfs:comment>
        <rdfs:comment xml:lang="it">Proprietà che lega una Domanda NASpI a uno Stato di domanda NASpI. Ciascuna istanza di Stato di domanda NASpI è legata ad una unica istanza di Domanda NASpI. Questa proprietà lega quindi la Domanda NASpI agli eventi che caratterizzano il suo ciclo di vita.</rdfs:comment>
        <rdfs:label xml:lang="it">ha stato di domanda NASpI</rdfs:label>
        <rdfs:label xml:lang="en">has NASpI claim status</rdfs:label>
    </owl:ObjectProperty>



    <!-- https://w3id.org/italia/social-security/onto/socialSafetyNet/haStatoDiLavoro -->

    <owl:ObjectProperty rdf:about="https://w3id.org/italia/social-security/onto/socialSafetyNet/haStatoDiLavoro">
        <rdf:type rdf:resource="http://www.w3.org/2002/07/owl#InverseFunctionalProperty"/>
        <rdfs:domain rdf:resource="https://w3id.org/italia/social-security/onto/socialSafetyNet/Lavoratore"/>
        <rdfs:range rdf:resource="https://w3id.org/italia/social-security/onto/socialSafetyNet/StatoDiLavoro"/>
        <rdfs:comment xml:lang="en">Property that links a Worker to a Working status. Each Working status instance is linked to a single Worker instance.</rdfs:comment>
        <rdfs:comment xml:lang="it">Proprietà che lega un Lavoratore a un Stato di lavoro. Ciascuna istanza di Stato di lavoro è legata ad una unica istanza di Lavoratore.</rdfs:comment>
        <rdfs:label xml:lang="it">ha stato di lavoro</rdfs:label>
        <rdfs:label xml:lang="en">has working status</rdfs:label>
    </owl:ObjectProperty>



    <!-- https://w3id.org/italia/social-security/onto/socialSafetyNet/haStatoDiOccupazione -->

    <owl:ObjectProperty rdf:about="https://w3id.org/italia/social-security/onto/socialSafetyNet/haStatoDiOccupazione">
        <rdfs:domain rdf:resource="https://w3id.org/italia/social-security/onto/socialSafetyNet/RapportoDiLavoro"/>
        <rdfs:range>
            <owl:Class>
                <owl:unionOf rdf:parseType="Collection">
                    <rdf:Description rdf:about="https://w3id.org/italia/social-security/onto/socialSafetyNet/StatoDiDisoccupazioneParziale"/>
                    <rdf:Description rdf:about="https://w3id.org/italia/social-security/onto/socialSafetyNet/StatoDiOccupazione"/>
                </owl:unionOf>
            </owl:Class>
        </rdfs:range>
        <rdfs:comment xml:lang="en">Property that links a Work relationship to an Employment status or to a Partial unemployment status.</rdfs:comment>
        <rdfs:comment xml:lang="it">Proprietà che lega un Rapporto di lavoro a uno Stato di occupazione o a uno Stato di disoccupazione parziale.</rdfs:comment>
        <rdfs:label xml:lang="it">ha stato di occupazione</rdfs:label>
        <rdfs:label xml:lang="en">has employment status</rdfs:label>
    </owl:ObjectProperty>



    <!-- https://w3id.org/italia/social-security/onto/socialSafetyNet/haStatoDiPrestazioneNASpI -->

    <owl:ObjectProperty rdf:about="https://w3id.org/italia/social-security/onto/socialSafetyNet/haStatoDiPrestazioneNASpI">
        <rdf:type rdf:resource="http://www.w3.org/2002/07/owl#InverseFunctionalProperty"/>
        <rdfs:domain rdf:resource="https://w3id.org/italia/social-security/onto/socialSafetyNet/PrestazioneNASpI"/>
        <rdfs:range rdf:resource="https://w3id.org/italia/social-security/onto/socialSafetyNet/StatoDiPrestazioneNASpI"/>
        <rdfs:comment xml:lang="en">Property that links a NASpI benefit to a NASpI benefit status. Each NASpI benefit status instance is linked to a single NASpI benefit instance. This property therefore links the NASpI Performance to the events that characterize its life cycle.</rdfs:comment>
        <rdfs:comment xml:lang="it">Proprietà che lega una Prestazione NASpI a un Stato di prestazione NASpI. Ciascuna istanza di Stato di prestazione NASpI è legata ad una unica istanza di Prestazione NASpI. Questa proprietà lega quindi la Prestazione NASpI agli eventi che caratterizzano il suo ciclo di vita.</rdfs:comment>
        <rdfs:label xml:lang="it">ha stato di prestazione NASpI</rdfs:label>
        <rdfs:label xml:lang="en">has NASpI benefit status</rdfs:label>
    </owl:ObjectProperty>



    <!-- https://w3id.org/italia/social-security/onto/socialSafetyNet/haTipoAttivitàCorrente -->

    <owl:ObjectProperty rdf:about="https://w3id.org/italia/social-security/onto/socialSafetyNet/haTipoAttivitàCorrente">
        <rdf:type rdf:resource="http://www.w3.org/2002/07/owl#FunctionalProperty"/>
        <rdfs:domain rdf:resource="https://w3id.org/italia/social-security/onto/socialSafetyNet/AttivitàCorrente"/>
        <rdfs:range rdf:resource="https://w3id.org/italia/social-security/onto/socialSafetyNet/TipoDiRapportoDiLavoro"/>
        <rdfs:comment xml:lang="en">Property that links a Current Activity to its unique Type of work relationship, which is used here to characterize the activity performed.</rdfs:comment>
        <rdfs:comment xml:lang="it">Proprietà che lega una Attività corrente al suo unico Tipo di rapporto di lavoro, qui utilizzato per caratterizzare l&apos;attività svolta.</rdfs:comment>
        <rdfs:label xml:lang="it">ha tipo attività corrente</rdfs:label>
        <rdfs:label xml:lang="en">has current activity type</rdfs:label>
    </owl:ObjectProperty>



    <!-- https://w3id.org/italia/social-security/onto/socialSafetyNet/haTipoDiAttivitàAutonoma -->

    <owl:ObjectProperty rdf:about="https://w3id.org/italia/social-security/onto/socialSafetyNet/haTipoDiAttivitàAutonoma">
        <rdfs:domain rdf:resource="https://w3id.org/italia/social-security/onto/socialSafetyNet/LavoratoreAutonomo"/>
        <rdfs:range rdf:resource="https://w3id.org/italia/social-security/onto/socialSafetyNet/TipoDiAttivitàAutonoma"/>
        <rdfs:comment xml:lang="en">Property that links a Self-employed to a Self-employed activity type</rdfs:comment>
        <rdfs:comment xml:lang="it">Proprietà che lega un Lavoratore autonomo a un Tipo di attività autonoma.</rdfs:comment>
        <rdfs:label xml:lang="it">ha tipo di attività autonoma</rdfs:label>
        <rdfs:label xml:lang="en">has activity type</rdfs:label>
    </owl:ObjectProperty>



    <!-- https://w3id.org/italia/social-security/onto/socialSafetyNet/haTipoDiAttivitàEconomica -->

    <owl:ObjectProperty rdf:about="https://w3id.org/italia/social-security/onto/socialSafetyNet/haTipoDiAttivitàEconomica">
        <rdfs:domain rdf:resource="https://w3id.org/italia/social-security/onto/socialSafetyNet/LavoratoreAPartitaIVA"/>
        <rdfs:range rdf:resource="https://w3id.org/italia/social-security/onto/socialSafetyNet/TipoDiAttivitàEconomica"/>
        <rdfs:comment xml:lang="en">Property that links a VAT-registered worker to a Economic activity type</rdfs:comment>
        <rdfs:comment xml:lang="it">Proprietà che lega un Lavoratore a partita IVA a un Tipo di attività economica.</rdfs:comment>
        <rdfs:label xml:lang="it">ha tipo di attività economica</rdfs:label>
        <rdfs:label xml:lang="en">has economic activity type</rdfs:label>
    </owl:ObjectProperty>



    <!-- https://w3id.org/italia/social-security/onto/socialSafetyNet/haTipoDiComunicazioneNASpI -->

    <owl:ObjectProperty rdf:about="https://w3id.org/italia/social-security/onto/socialSafetyNet/haTipoDiComunicazioneNASpI">
        <rdf:type rdf:resource="http://www.w3.org/2002/07/owl#FunctionalProperty"/>
        <rdfs:domain rdf:resource="https://w3id.org/italia/social-security/onto/socialSafetyNet/ComunicazioneNASpI"/>
        <rdfs:range rdf:resource="https://w3id.org/italia/social-security/onto/socialSafetyNet/TipoDiComunicazioneNASpI"/>
        <rdfs:comment xml:lang="en">Property that binds a NASpI communication to its unique NASpI communication type.</rdfs:comment>
        <rdfs:comment xml:lang="it">Proprietà che lega una Comunicazione NASpI al suo unico Tipo di comunicazione NASpI.</rdfs:comment>
        <rdfs:label xml:lang="it">ha tipo di comunicazione NASpI</rdfs:label>
        <rdfs:label xml:lang="en">has NASpI communication type</rdfs:label>
    </owl:ObjectProperty>



    <!-- https://w3id.org/italia/social-security/onto/socialSafetyNet/haTipoDiContribuzione -->

    <owl:ObjectProperty rdf:about="https://w3id.org/italia/social-security/onto/socialSafetyNet/haTipoDiContribuzione">
        <rdf:type rdf:resource="http://www.w3.org/2002/07/owl#FunctionalProperty"/>
        <rdfs:domain rdf:resource="https://w3id.org/italia/social-security/onto/socialSafetyNet/ContributoPrevidenziale"/>
        <rdfs:range rdf:resource="https://w3id.org/italia/social-security/onto/socialSafetyNet/TipoDiContribuzione"/>
        <rdfs:comment xml:lang="en">Property that links a Social security contribution to its unique Contribution type.</rdfs:comment>
        <rdfs:comment xml:lang="it">Proprietà che lega un Contributo previdenziale al suo unico Tipo di contribuzione.</rdfs:comment>
        <rdfs:label xml:lang="it">ha tipo di contribuzione</rdfs:label>
        <rdfs:label xml:lang="en">has contribution type</rdfs:label>
    </owl:ObjectProperty>



    <!-- https://w3id.org/italia/social-security/onto/socialSafetyNet/haTipoDiDelegatoNASpI -->

    <owl:ObjectProperty rdf:about="https://w3id.org/italia/social-security/onto/socialSafetyNet/haTipoDiDelegatoNASpI">
        <rdf:type rdf:resource="http://www.w3.org/2002/07/owl#FunctionalProperty"/>
        <rdfs:domain rdf:resource="https://w3id.org/italia/social-security/onto/socialSafetyNet/DelegatoDomandaNASpI"/>
        <rdfs:range rdf:resource="https://w3id.org/italia/social-security/onto/pensions/TipoDiDelegato"/>
        <rdfs:comment xml:lang="en">A property that links a NASpI claims delegate to a Delegate Type.</rdfs:comment>
        <rdfs:comment xml:lang="it">Proprietà che lega un Delegato domanda NASpI a un Tipo di delegato.</rdfs:comment>
        <rdfs:label xml:lang="it">ha tipo di delegato NASpI</rdfs:label>
        <rdfs:label xml:lang="en">has NASpI delegate type</rdfs:label>
    </owl:ObjectProperty>



    <!-- https://w3id.org/italia/social-security/onto/socialSafetyNet/haTipoDiProfessione -->

    <owl:ObjectProperty rdf:about="https://w3id.org/italia/social-security/onto/socialSafetyNet/haTipoDiProfessione">
        <rdfs:domain rdf:resource="https://w3id.org/italia/social-security/onto/socialSafetyNet/LiberoProfessionista"/>
        <rdfs:range rdf:resource="https://w3id.org/italia/social-security/onto/socialSafetyNet/TipoDiProfessione"/>
        <rdfs:comment xml:lang="en">Property that links a Freelancer to a Profession type.</rdfs:comment>
        <rdfs:comment xml:lang="it">Proprietà che lega un Libero professionista a un Tipo di professione.</rdfs:comment>
        <rdfs:label xml:lang="it">ha tipo di professione</rdfs:label>
        <rdfs:label xml:lang="en">has profession type</rdfs:label>
    </owl:ObjectProperty>



    <!-- https://w3id.org/italia/social-security/onto/socialSafetyNet/haTipoDiQualifica-CategoriaPerNASpI -->

    <owl:ObjectProperty rdf:about="https://w3id.org/italia/social-security/onto/socialSafetyNet/haTipoDiQualifica-CategoriaPerNASpI">
        <rdf:type rdf:resource="http://www.w3.org/2002/07/owl#FunctionalProperty"/>
        <rdfs:domain rdf:resource="https://w3id.org/italia/social-security/onto/socialSafetyNet/RichiedenteNASpI"/>
        <rdfs:range>
            <owl:Class>
                <owl:unionOf rdf:parseType="Collection">
                    <rdf:Description rdf:about="https://w3id.org/italia/social-security/onto/socialSafetyNet/TipoDiCategoria"/>
                    <rdf:Description rdf:about="https://w3id.org/italia/social-security/onto/socialSafetyNet/TipoDiQualifica"/>
                </owl:unionOf>
            </owl:Class>
        </rdfs:range>
        <rdfs:comment xml:lang="en">Property that link a NASpI Applicant to his/her category or qualification.</rdfs:comment>
        <rdfs:comment xml:lang="it">Proprietà che lega un Richiedente NASpI alla sua categoria o qualifica.</rdfs:comment>
        <rdfs:label xml:lang="it">ha tipo di qualifica-categoria per NASpI</rdfs:label>
        <rdfs:label xml:lang="en">has qualification-category type for NASpI</rdfs:label>
    </owl:ObjectProperty>



    <!-- https://w3id.org/italia/social-security/onto/socialSafetyNet/haTipoDiRapportoDiLavoro -->

    <owl:ObjectProperty rdf:about="https://w3id.org/italia/social-security/onto/socialSafetyNet/haTipoDiRapportoDiLavoro">
        <rdf:type rdf:resource="http://www.w3.org/2002/07/owl#FunctionalProperty"/>
        <rdfs:domain rdf:resource="https://w3id.org/italia/social-security/onto/socialSafetyNet/RapportoDiLavoro"/>
        <rdfs:range rdf:resource="https://w3id.org/italia/social-security/onto/socialSafetyNet/TipoDiRapportoDiLavoro"/>
        <rdfs:comment xml:lang="en">Property that links a Work Relationship to a Employment relationship type. Each Work Relationship instance is linked to a single Employment relationship type instance.</rdfs:comment>
        <rdfs:comment xml:lang="it">Proprietà che lega un Rapporto di lavoro a un Tipo di rapporto di lavoro. Ciascuna istanza di Rapporto di lavoro è legata ad una unica istanza di Tipo di rapporto di lavoro.</rdfs:comment>
        <rdfs:label xml:lang="it">ha tipo di rapporto di lavoro</rdfs:label>
        <rdfs:label xml:lang="en">has work relationship type</rdfs:label>
    </owl:ObjectProperty>



    <!-- https://w3id.org/italia/social-security/onto/socialSafetyNet/haTipoModalitàDiPagamentoNASpI -->

    <owl:ObjectProperty rdf:about="https://w3id.org/italia/social-security/onto/socialSafetyNet/haTipoModalitàDiPagamentoNASpI">
        <rdf:type rdf:resource="http://www.w3.org/2002/07/owl#FunctionalProperty"/>
        <rdfs:domain rdf:resource="https://w3id.org/italia/social-security/onto/socialSafetyNet/ModalitàDiPagamentoNASpI"/>
        <rdfs:range rdf:resource="https://w3id.org/italia/social-security/onto/socialSafetyNet/TipoDiModalitàDiPagamentoNASpI"/>
        <rdfs:comment xml:lang="en">Property that links a NASpI payment method to its unique NASpI payment method type.</rdfs:comment>
        <rdfs:comment xml:lang="it">Proprietà che lega una Modalità di pagamento NASpI al suo unico Tipo di modalità di pagamento NASpI.</rdfs:comment>
        <rdfs:label xml:lang="it">ha tipo modalità di pagamento NASpI</rdfs:label>
        <rdfs:label xml:lang="en">has NASpI payment method type</rdfs:label>
    </owl:ObjectProperty>



    <!-- https://w3id.org/italia/social-security/onto/socialSafetyNet/haTitoloDiStudio -->

    <owl:ObjectProperty rdf:about="https://w3id.org/italia/social-security/onto/socialSafetyNet/haTitoloDiStudio">
        <rdf:type rdf:resource="http://www.w3.org/2002/07/owl#FunctionalProperty"/>
        <rdfs:domain rdf:resource="https://w3id.org/italia/social-security/onto/socialSafetyNet/RichiedenteNASpI"/>
        <rdfs:range rdf:resource="https://w3id.org/italia/social-security/onto/socialSafetyNet/TitoloDiStudio"/>
        <rdfs:comment xml:lang="en">Property that links a NASpI Applicant to his/her educational qualification.</rdfs:comment>
        <rdfs:comment xml:lang="it">Proprietà che lega un Richiedente NASpI al suo titolo di studio.</rdfs:comment>
        <rdfs:label xml:lang="it">ha titolo di studio</rdfs:label>
        <rdfs:label xml:lang="en">has educational qualification</rdfs:label>
    </owl:ObjectProperty>



    <!-- https://w3id.org/italia/social-security/onto/socialSafetyNet/haUfficioDelLavoroDiIscrizione -->

    <owl:ObjectProperty rdf:about="https://w3id.org/italia/social-security/onto/socialSafetyNet/haUfficioDelLavoroDiIscrizione">
        <rdf:type rdf:resource="http://www.w3.org/2002/07/owl#FunctionalProperty"/>
        <rdfs:domain rdf:resource="https://w3id.org/italia/social-security/onto/socialSafetyNet/IscrizioneUfficioDelLavoro"/>
        <rdfs:range rdf:resource="https://w3id.org/italia/social-security/onto/socialSafetyNet/UfficioDelLavoro"/>
        <rdfs:comment xml:lang="en">Property that links a Labour office registration to its one and only Labour office.</rdfs:comment>
        <rdfs:comment xml:lang="it">Proprietà che lega una Iscrizione ufficio del lavoro al relativo e unico Ufficio del lavoro.</rdfs:comment>
        <rdfs:label xml:lang="it">ha ufficio del lavoro di iscrizione</rdfs:label>
        <rdfs:label xml:lang="en">has enrolment labour office</rdfs:label>
    </owl:ObjectProperty>



    <!-- https://w3id.org/italia/social-security/onto/socialSafetyNet/proponeContrattoDiLavoro -->

    <owl:ObjectProperty rdf:about="https://w3id.org/italia/social-security/onto/socialSafetyNet/proponeContrattoDiLavoro">
        <rdfs:domain rdf:resource="https://w3id.org/italia/social-security/onto/socialSafetyNet/TitolareDelRapportoDiLavoro"/>
        <rdfs:range rdf:resource="https://w3id.org/italia/social-security/onto/socialSafetyNet/ContrattoDiLavoro"/>
        <owl:propertyChainAxiom rdf:parseType="Collection">
            <rdf:Description rdf:about="https://w3id.org/italia/social-security/onto/socialSafetyNet/retribuiscePrestazioneLavorativa"/>
            <rdf:Description rdf:about="https://w3id.org/italia/social-security/onto/socialSafetyNet/èRegolatoDaContratto"/>
        </owl:propertyChainAxiom>
        <rdfs:comment xml:lang="en">Property that links a Work relationship rightsholder to a Work contract</rdfs:comment>
        <rdfs:comment xml:lang="it">Proprietà che lega un Titolare del rapporto di lavoro a un Contratto di lavoro.</rdfs:comment>
        <rdfs:label xml:lang="it">propone contratto di lavoro</rdfs:label>
        <rdfs:label xml:lang="en">proposes work contract</rdfs:label>
    </owl:ObjectProperty>



    <!-- https://w3id.org/italia/social-security/onto/socialSafetyNet/retribuiscePrestazioneLavorativa -->

    <owl:ObjectProperty rdf:about="https://w3id.org/italia/social-security/onto/socialSafetyNet/retribuiscePrestazioneLavorativa">
        <rdf:type rdf:resource="http://www.w3.org/2002/07/owl#InverseFunctionalProperty"/>
        <rdfs:domain rdf:resource="https://w3id.org/italia/social-security/onto/socialSafetyNet/TitolareDelRapportoDiLavoro"/>
        <rdfs:range rdf:resource="https://w3id.org/italia/social-security/onto/socialSafetyNet/RapportoDiLavoro"/>
        <rdfs:comment xml:lang="en">Property that links a Work relationship rightsholder to a Work Relationship. Each Work Relationship instance is linked to a single Work relationship rightsholder instance.</rdfs:comment>
        <rdfs:comment xml:lang="it">Proprietà che lega un Titolare del rapporto di lavoro a un Rapporto di lavoro. Ciascuna istanza di Rapporto di lavoro è legata ad una unica istanza di Titolare del rapporto di lavoro.</rdfs:comment>
        <rdfs:label xml:lang="en">pays for work</rdfs:label>
        <rdfs:label xml:lang="it">retribuisce prestazione lavorativa</rdfs:label>
    </owl:ObjectProperty>



    <!-- https://w3id.org/italia/social-security/onto/socialSafetyNet/revocaStatoDiDisoccupazione -->

    <owl:ObjectProperty rdf:about="https://w3id.org/italia/social-security/onto/socialSafetyNet/revocaStatoDiDisoccupazione">
        <rdf:type rdf:resource="http://www.w3.org/2002/07/owl#FunctionalProperty"/>
        <rdf:type rdf:resource="http://www.w3.org/2002/07/owl#InverseFunctionalProperty"/>
        <rdfs:domain rdf:resource="https://w3id.org/italia/social-security/onto/socialSafetyNet/AttoDiDecadenzaStatoDiDisoccupazione"/>
        <rdfs:range rdf:resource="https://w3id.org/italia/social-security/onto/socialSafetyNet/StatoDiDisoccupazione"/>
        <rdfs:comment xml:lang="en">Property that links a Unemployment status forfeiture deed to one and only one Unemployment status.</rdfs:comment>
        <rdfs:comment xml:lang="it">Proprietà che lega un Atto di decadenza stato di disoccupazione a uno e un solo Stato di disoccupazione.</rdfs:comment>
        <rdfs:label xml:lang="it">revoca stato di disoccupazione</rdfs:label>
        <rdfs:label xml:lang="en">unemployment status revocation</rdfs:label>
    </owl:ObjectProperty>



    <!-- https://w3id.org/italia/social-security/onto/socialSafetyNet/richiedeCertificazioneNASpI -->

    <owl:ObjectProperty rdf:about="https://w3id.org/italia/social-security/onto/socialSafetyNet/richiedeCertificazioneNASpI">
        <rdfs:domain rdf:resource="https://w3id.org/italia/social-security/onto/socialSafetyNet/EspatrioInNASpI"/>
        <rdfs:range rdf:resource="https://w3id.org/italia/social-security/onto/socialSafetyNet/AttoDiCertificazioneDiBeneficiarioNASpI"/>
        <rdfs:comment xml:lang="en">Property that links a NASpI expatriation period to a NASpI beneficiary certification deed (PD U2). The NASpI Beneficiary who expatriates in search of work must necessarily request this document to prove his or her status as a recipient of unemployment benefits at the employment offices of a foreign country.</rdfs:comment>
        <rdfs:comment xml:lang="it">Proprietà che lega un Espatrio in NASpI a un Atto di certificazione di Beneficiario NASpI (PD U2). Il Beneficiario NASpI che espatria in cerca di lavoro deve necessariamente richiedere tale documento per dimostrare la sua condizione di beneficiario d&apos;indennità di disoccupazione presso gli uffici del lavoro di uno stato estero.</rdfs:comment>
        <rdfs:label xml:lang="en">requires NASpI certification</rdfs:label>
        <rdfs:label xml:lang="it">richiede certificazione NASpI</rdfs:label>
    </owl:ObjectProperty>



    <!-- https://w3id.org/italia/social-security/onto/socialSafetyNet/èIscrittoAlboProfessionale -->

    <owl:ObjectProperty rdf:about="https://w3id.org/italia/social-security/onto/socialSafetyNet/èIscrittoAlboProfessionale">
        <rdf:type rdf:resource="http://www.w3.org/2002/07/owl#InverseFunctionalProperty"/>
        <rdfs:domain>
            <owl:Restriction>
                <owl:onProperty rdf:resource="https://w3id.org/italia/onto/RO/holdsRoleInTime"/>
                <owl:someValuesFrom rdf:resource="https://w3id.org/italia/social-security/onto/socialSafetyNet/LiberoProfessionistaProtetto"/>
            </owl:Restriction>
        </rdfs:domain>
        <rdfs:range rdf:resource="https://w3id.org/italia/social-security/onto/socialSafetyNet/IscrizioneAlboProfessionale"/>
        <rdfs:comment xml:lang="en">Property that links a Person to his/her entry in a Professional register. Each application for registration is linked to a single instance of Person.</rdfs:comment>
        <rdfs:comment xml:lang="it">Proprietà che lega una Persona alla sua Iscrizione in un Albo professionale. Ciascuna istanza di iscrizione è legata ad una unica istanza di Persona.</rdfs:comment>
        <rdfs:label xml:lang="en">is professional register member</rdfs:label>
        <rdfs:label xml:lang="it">è iscritto albo professionale</rdfs:label>
    </owl:ObjectProperty>



    <!-- https://w3id.org/italia/social-security/onto/socialSafetyNet/èIscrittoUfficioDelLavoro -->

    <owl:ObjectProperty rdf:about="https://w3id.org/italia/social-security/onto/socialSafetyNet/èIscrittoUfficioDelLavoro">
        <rdf:type rdf:resource="http://www.w3.org/2002/07/owl#InverseFunctionalProperty"/>
        <rdfs:domain>
            <owl:Restriction>
                <owl:onProperty rdf:resource="https://w3id.org/italia/onto/RO/holdsRoleInTime"/>
                <owl:someValuesFrom rdf:resource="https://w3id.org/italia/social-security/onto/socialSafetyNet/Lavoratore"/>
            </owl:Restriction>
        </rdfs:domain>
        <rdfs:range rdf:resource="https://w3id.org/italia/social-security/onto/socialSafetyNet/IscrizioneUfficioDelLavoro"/>
        <rdfs:comment xml:lang="en">Property that links a Person to his or her Labour office registration. Each application for registration is linked to a single instance of Person. A Person with the role of Unemployed or First-time jobseeker must necessarily be registered with a Labour office or Employment centre referred to by his Declaration of immediate availability.</rdfs:comment>
        <rdfs:comment xml:lang="it">Proprietà che lega una Persona alla sua Iscrizione ufficio del Lavoro. Ciascuna istanza di iscrizione è legata ad una unica istanza di Persona. Una Persona con ruolo di Disoccupato o Inoccupato deve essere necessariamente iscritta ad un Ufficio del lavoro ovvero al Centro Per l&apos;Impiego riferito dalla sua Dichiarazione di Immediata Disponibilità.</rdfs:comment>
        <rdfs:label xml:lang="en">is labour office member</rdfs:label>
        <rdfs:label xml:lang="it">è iscritto ufficio del lavoro</rdfs:label>
    </owl:ObjectProperty>



    <!-- https://w3id.org/italia/social-security/onto/socialSafetyNet/èRegolatoDaContratto -->

    <owl:ObjectProperty rdf:about="https://w3id.org/italia/social-security/onto/socialSafetyNet/èRegolatoDaContratto">
        <rdf:type rdf:resource="http://www.w3.org/2002/07/owl#InverseFunctionalProperty"/>
        <rdfs:domain rdf:resource="https://w3id.org/italia/social-security/onto/socialSafetyNet/RapportoDiLavoro"/>
        <rdfs:range rdf:resource="https://w3id.org/italia/social-security/onto/socialSafetyNet/ContrattoDiLavoro"/>
        <rdfs:comment xml:lang="en">Property that links a Work Relationship to a Work contract. Each Work contract instance is linked to a single Work Relationship instance.</rdfs:comment>
        <rdfs:comment xml:lang="it">Proprietà che lega un Rapporto di lavoro a un Contratto di lavoro. Ciascuna istanza di Contratto di lavoro è legata ad una unica istanza di Rapporto di lavoro.</rdfs:comment>
        <rdfs:label xml:lang="en">is regulated by contract</rdfs:label>
        <rdfs:label xml:lang="it">è regolato da contratto</rdfs:label>
    </owl:ObjectProperty>



    <!--
    ///////////////////////////////////////////////////////////////////////////////////////
    //
    // Data properties
    //
    ///////////////////////////////////////////////////////////////////////////////////////
     -->




    <!-- https://w3id.org/italia/social-security/onto/socialSafetyNet/BIC -->

    <owl:DatatypeProperty rdf:about="https://w3id.org/italia/social-security/onto/socialSafetyNet/BIC">
        <rdf:type rdf:resource="http://www.w3.org/2002/07/owl#FunctionalProperty"/>
        <rdfs:domain rdf:resource="https://w3id.org/italia/social-security/onto/socialSafetyNet/ModalitàDiPagamentoNASpI"/>
        <rdfs:range rdf:resource="http://www.w3.org/2001/XMLSchema#string"/>
        <rdfs:comment xml:lang="it">Bank Identifier Code: codice identificativo di una banca (o di una sua dipendenza) utilizzato dal sistema di messaggistica bancaria internazionale SWIFT.</rdfs:comment>
        <rdfs:comment xml:lang="en">Bank Identifier Code: identification code of a bank (or one of its dependencies) used by SWIFT, the international banking messaging system.</rdfs:comment>
        <rdfs:label xml:lang="en">BIC</rdfs:label>
        <rdfs:label xml:lang="it">BIC</rdfs:label>
    </owl:DatatypeProperty>



    <!-- https://w3id.org/italia/social-security/onto/socialSafetyNet/IBAN -->

    <owl:DatatypeProperty rdf:about="https://w3id.org/italia/social-security/onto/socialSafetyNet/IBAN">
        <rdf:type rdf:resource="http://www.w3.org/2002/07/owl#FunctionalProperty"/>
        <rdfs:domain rdf:resource="https://w3id.org/italia/social-security/onto/socialSafetyNet/ModalitàDiPagamentoNASpI"/>
        <rdfs:range rdf:resource="http://www.w3.org/2001/XMLSchema#string"/>
        <rdfs:comment xml:lang="en">Identification Bank Account Number: code that uniquely identifies, internationally, the bank or postal account of a customer at a financial intermediary.</rdfs:comment>
        <rdfs:comment xml:lang="it">Identification Bank Account Number: codice che identifica in maniera univoca, a livello internazionale, il conto, corrente o postale, di un cliente presso un intermediario finanziario.</rdfs:comment>
        <rdfs:label xml:lang="en">IBAN</rdfs:label>
        <rdfs:label xml:lang="it">IBAN</rdfs:label>
    </owl:DatatypeProperty>



    <!-- https://w3id.org/italia/social-security/onto/socialSafetyNet/contribuzioneAntePrestazioniFruite -->

    <owl:DatatypeProperty rdf:about="https://w3id.org/italia/social-security/onto/socialSafetyNet/contribuzioneAntePrestazioniFruite">
        <rdf:type rdf:resource="http://www.w3.org/2002/07/owl#FunctionalProperty"/>
        <rdfs:domain rdf:resource="https://w3id.org/italia/social-security/onto/socialSafetyNet/StatoDiAccoltaDiDomandaNASpI"/>
        <rdfs:comment xml:lang="en">Number of weeks of contributions in the last four years preceding any unemployment benefits already used. The contribution weeks used for these benefits can no longer be used.</rdfs:comment>
        <rdfs:comment xml:lang="it">Numero di settimane di contribuzione dell&apos;ultimo quadriennio che precedono eventuali prestazioni per disoccupazione già fruite. Le settimane di contribuzione utilizzate per tali prestazioni non possono essere più utilizzate.</rdfs:comment>
        <rdfs:label xml:lang="en">contributions before benefits used</rdfs:label>
        <rdfs:label xml:lang="it">contribuzione ante prestazioni fruite</rdfs:label>
    </owl:DatatypeProperty>



    <!-- https://w3id.org/italia/social-security/onto/socialSafetyNet/contribuzioneIndisponibile -->

    <owl:DatatypeProperty rdf:about="https://w3id.org/italia/social-security/onto/socialSafetyNet/contribuzioneIndisponibile">
        <rdf:type rdf:resource="http://www.w3.org/2002/07/owl#FunctionalProperty"/>
        <rdfs:domain rdf:resource="https://w3id.org/italia/social-security/onto/socialSafetyNet/StatoDiAccoltaDiDomandaNASpI"/>
        <rdfs:comment xml:lang="en">Total number of contribution days in the last four years used for other previous unemployment benefits that can no longer be used.</rdfs:comment>
        <rdfs:comment xml:lang="it">Totale dei giorni di contribuzione nell&apos;ultimo quadriennio utilizzati per altre prestazioni di disoccupazione pregresse e non più utilizzabili.</rdfs:comment>
        <rdfs:label xml:lang="it">contribuzione indisponibile</rdfs:label>
        <rdfs:label xml:lang="en">unavailable contribution</rdfs:label>
    </owl:DatatypeProperty>



    <!-- https://w3id.org/italia/social-security/onto/socialSafetyNet/contribuzionePostPrestazioniFruite -->

    <owl:DatatypeProperty rdf:about="https://w3id.org/italia/social-security/onto/socialSafetyNet/contribuzionePostPrestazioniFruite">
        <rdf:type rdf:resource="http://www.w3.org/2002/07/owl#FunctionalProperty"/>
        <rdfs:domain rdf:resource="https://w3id.org/italia/social-security/onto/socialSafetyNet/StatoDiAccoltaDiDomandaNASpI"/>
        <rdfs:comment xml:lang="en">Number of weeks of contributions in the last four years following the last unemployment benefit, if any.</rdfs:comment>
        <rdfs:comment xml:lang="it">Numero di settimane di contribuzione dell&apos;ultimo quadriennio successive all&apos;ultima prestazione per disoccupazione eventualmente fruita.</rdfs:comment>
        <rdfs:label xml:lang="en">contribution after benefits used</rdfs:label>
        <rdfs:label xml:lang="it">contribuzione post prestazioni fruite</rdfs:label>
    </owl:DatatypeProperty>



    <!-- https://w3id.org/italia/social-security/onto/socialSafetyNet/dataAvvenutaViolazioneAttivazione -->

    <owl:DatatypeProperty rdf:about="https://w3id.org/italia/social-security/onto/socialSafetyNet/dataAvvenutaViolazioneAttivazione">
        <rdfs:domain rdf:resource="https://w3id.org/italia/social-security/onto/socialSafetyNet/AttoDiNotificaViolazioneObblighiAttivazione"/>
        <rdfs:range rdf:resource="http://www.w3.org/2001/XMLSchema#dateTime"/>
        <rdfs:comment xml:lang="it">Data di accadimento di una violazione degli adempimenti conseguenti alla sottoscrizione di un PSP.</rdfs:comment>
        <rdfs:comment xml:lang="en">Date of occurrence of a breach of the obligations resulting from the subscription of a PSP.</rdfs:comment>
        <rdfs:label xml:lang="en">activation obligation violation date</rdfs:label>
        <rdfs:label xml:lang="it">data avvenuta violazione attivazione</rdfs:label>
    </owl:DatatypeProperty>



    <!-- https://w3id.org/italia/social-security/onto/socialSafetyNet/dataCessazioneRapportoDiLavoro -->

    <owl:DatatypeProperty rdf:about="https://w3id.org/italia/social-security/onto/socialSafetyNet/dataCessazioneRapportoDiLavoro">
        <rdf:type rdf:resource="http://www.w3.org/2002/07/owl#FunctionalProperty"/>
        <rdfs:domain rdf:resource="https://w3id.org/italia/social-security/onto/socialSafetyNet/AttoDiCessazioneRapportoDiLavoro"/>
        <rdfs:range rdf:resource="http://www.w3.org/2001/XMLSchema#dateTime"/>
        <rdfs:comment xml:lang="it">Data di compimento di un Atto di cessazione rapporto di lavoro.</rdfs:comment>
        <rdfs:comment xml:lang="en">Date of fulfilment of a Employment termination deed.</rdfs:comment>
        <rdfs:label xml:lang="it">data cessazione rapporto di lavoro</rdfs:label>
        <rdfs:label xml:lang="en">employment relationship end date</rdfs:label>
    </owl:DatatypeProperty>



    <!-- https://w3id.org/italia/social-security/onto/socialSafetyNet/dataDecadenzaDisoccupazione -->

    <owl:DatatypeProperty rdf:about="https://w3id.org/italia/social-security/onto/socialSafetyNet/dataDecadenzaDisoccupazione">
        <rdf:type rdf:resource="http://www.w3.org/2002/07/owl#FunctionalProperty"/>
        <rdfs:domain rdf:resource="https://w3id.org/italia/social-security/onto/socialSafetyNet/AttoDiDecadenzaStatoDiDisoccupazione"/>
        <rdfs:range rdf:resource="http://www.w3.org/2001/XMLSchema#dateTime"/>
        <rdfs:comment xml:lang="it">Data di decadenza da uno Stato di disoccupazione indicata nel relativo atto. A partire da tale data verrà sospeso il sussidio eventualmente legato a tale stato.</rdfs:comment>
        <rdfs:comment xml:lang="en">The date of forfeiture of an Unemployment status indicated in the relevant deed. From that date, any subsidy linked to this status will be suspended.</rdfs:comment>
        <rdfs:label xml:lang="it">data decadenza disoccupazione</rdfs:label>
        <rdfs:label xml:lang="en">unemployment forfeiture date</rdfs:label>
    </owl:DatatypeProperty>



    <!-- https://w3id.org/italia/social-security/onto/socialSafetyNet/dataDecadenzaNASpI -->

    <owl:DatatypeProperty rdf:about="https://w3id.org/italia/social-security/onto/socialSafetyNet/dataDecadenzaNASpI">
        <rdf:type rdf:resource="http://www.w3.org/2002/07/owl#FunctionalProperty"/>
        <rdfs:domain rdf:resource="https://w3id.org/italia/social-security/onto/socialSafetyNet/AttoDiDecadenzaNASpI"/>
        <rdfs:range rdf:resource="http://www.w3.org/2001/XMLSchema#dateTime"/>
        <rdfs:comment xml:lang="it">Data di decadenza da una Prestazione NASpI indicata nel relativo atto. A partire da tale data il sussidio verrà sospeso, con eventuale recupero delle somme già erogate.</rdfs:comment>
        <rdfs:comment xml:lang="en">Date of forfeiture of a NASpI benefit indicated in the relevant deed. From that date, the subsidy will be suspended, with possible recovery of the sums already paid.</rdfs:comment>
        <rdfs:label xml:lang="en">NASpI forfeiture date</rdfs:label>
        <rdfs:label xml:lang="it">data decadenza NASpI</rdfs:label>
    </owl:DatatypeProperty>



    <!-- https://w3id.org/italia/social-security/onto/socialSafetyNet/dataFinePrestazioneNASpI -->

    <owl:DatatypeProperty rdf:about="https://w3id.org/italia/social-security/onto/socialSafetyNet/dataFinePrestazioneNASpI">
        <rdf:type rdf:resource="http://www.w3.org/2002/07/owl#FunctionalProperty"/>
        <rdfs:domain rdf:resource="https://w3id.org/italia/social-security/onto/socialSafetyNet/PrestazioneNASpI"/>
        <rdfs:range rdf:resource="http://www.w3.org/2001/XMLSchema#dateTime"/>
        <rdfs:comment xml:lang="it">Data di termine di una Prestazione NASpI.</rdfs:comment>
        <rdfs:comment xml:lang="en">The date of termination of a NASpI Benefit.</rdfs:comment>
        <rdfs:label xml:lang="en">NASpI benefit end date</rdfs:label>
        <rdfs:label xml:lang="it">data fine prestazione NASpI</rdfs:label>
    </owl:DatatypeProperty>



    <!-- https://w3id.org/italia/social-security/onto/socialSafetyNet/dataInizioAttivitàCorrente -->

    <owl:DatatypeProperty rdf:about="https://w3id.org/italia/social-security/onto/socialSafetyNet/dataInizioAttivitàCorrente">
        <rdf:type rdf:resource="http://www.w3.org/2002/07/owl#FunctionalProperty"/>
        <rdfs:domain rdf:resource="https://w3id.org/italia/social-security/onto/socialSafetyNet/AttivitàCorrente"/>
        <rdfs:range rdf:resource="http://www.w3.org/2001/XMLSchema#dateTime"/>
        <rdfs:comment xml:lang="it">Data di inizio dell&apos;attività svolta dal Richiedente NASpI in concomitanza con la prestazione NASpI richiesta. La data deve cadere nell&apos;anno in cui si presenta la domanda, altrimenti è il primo giorno dell&apos;anno se antecedente.</rdfs:comment>
        <rdfs:comment xml:lang="en">Start date of the activity carried out by the NASpI Applicant in conjunction with the NASpI benefit requested. The date must fall in the year in which the claim is submitted, otherwise it is the first day of the year if earlier.</rdfs:comment>
        <rdfs:label xml:lang="en">current activity start date</rdfs:label>
        <rdfs:label xml:lang="it">data inizio attività corrente</rdfs:label>
    </owl:DatatypeProperty>



    <!-- https://w3id.org/italia/social-security/onto/socialSafetyNet/dataInizioPrestazioneNASpI -->

    <owl:DatatypeProperty rdf:about="https://w3id.org/italia/social-security/onto/socialSafetyNet/dataInizioPrestazioneNASpI">
        <rdf:type rdf:resource="http://www.w3.org/2002/07/owl#FunctionalProperty"/>
        <rdfs:domain rdf:resource="https://w3id.org/italia/social-security/onto/socialSafetyNet/PrestazioneNASpI"/>
        <rdfs:range rdf:resource="http://www.w3.org/2001/XMLSchema#dateTime"/>
        <rdfs:comment xml:lang="it">Data di inizio di una Prestazione NASpI.</rdfs:comment>
        <rdfs:comment xml:lang="en">The start date of a NASpI Benefit.</rdfs:comment>
        <rdfs:label xml:lang="en">NASpI benefit start date</rdfs:label>
        <rdfs:label xml:lang="it">data inizio prestazione NASpI</rdfs:label>
    </owl:DatatypeProperty>



    <!-- https://w3id.org/italia/social-security/onto/socialSafetyNet/dataIscrizioneAlboProfessionale -->

    <owl:DatatypeProperty rdf:about="https://w3id.org/italia/social-security/onto/socialSafetyNet/dataIscrizioneAlboProfessionale">
        <rdf:type rdf:resource="http://www.w3.org/2002/07/owl#FunctionalProperty"/>
        <rdfs:domain rdf:resource="https://w3id.org/italia/social-security/onto/socialSafetyNet/IscrizioneAlboProfessionale"/>
        <rdfs:range rdf:resource="http://www.w3.org/2001/XMLSchema#dateTime"/>
        <rdfs:comment xml:lang="en">The date on which a person has registered in a specific Professional register.</rdfs:comment>
        <rdfs:comment xml:lang="it">È la data in cui una persona si è iscritta in uno specifico Albo professionale.</rdfs:comment>
        <rdfs:label xml:lang="it">data iscrizione albo professionale</rdfs:label>
        <rdfs:label xml:lang="en">professional register entry date</rdfs:label>
    </owl:DatatypeProperty>



    <!-- https://w3id.org/italia/social-security/onto/socialSafetyNet/dataPresentazioneNASpI -->

    <owl:DatatypeProperty rdf:about="https://w3id.org/italia/social-security/onto/socialSafetyNet/dataPresentazioneNASpI">
        <rdf:type rdf:resource="http://www.w3.org/2002/07/owl#FunctionalProperty"/>
        <rdfs:domain rdf:resource="https://w3id.org/italia/social-security/onto/socialSafetyNet/StatoDiDomandaNASpI"/>
        <rdfs:range rdf:resource="http://www.w3.org/2001/XMLSchema#dateTime"/>
        <rdfs:comment xml:lang="it">Data di inoltro di una Domanda NASpI. Per le domande in stato di bozza è la data di ultimo salvataggio. </rdfs:comment>
        <rdfs:comment xml:lang="en">Date of submission of a NASpI claim. For applications in draft status, this is the date they were last saved.</rdfs:comment>
        <rdfs:label xml:lang="en">NASpI sending date</rdfs:label>
        <rdfs:label xml:lang="it">data presentazione NASpI</rdfs:label>
    </owl:DatatypeProperty>



    <!-- https://w3id.org/italia/social-security/onto/socialSafetyNet/dataSospensioneAccordoCPI -->

    <owl:DatatypeProperty rdf:about="https://w3id.org/italia/social-security/onto/socialSafetyNet/dataSospensioneAccordoCPI">
        <rdf:type rdf:resource="http://www.w3.org/2002/07/owl#FunctionalProperty"/>
        <rdfs:domain rdf:resource="https://w3id.org/italia/social-security/onto/socialSafetyNet/AttoDiCertificazioneDiBeneficiarioNASpI"/>
        <rdfs:range rdf:resource="http://www.w3.org/2001/XMLSchema#dateTime"/>
        <rdfs:comment xml:lang="it">Data in cui il Beneficiario NASpI ha cessato di essere a disposizione del CPI competente per espatriare in cerca di lavoro.</rdfs:comment>
        <rdfs:comment xml:lang="en">The date on which the NASpI beneficiary ceased to be available to the competent CPI to expatriate in search of work.</rdfs:comment>
        <rdfs:label xml:lang="en">CPI Agreement Suspension Date</rdfs:label>
        <rdfs:label xml:lang="it">data sospensione accordo CPI</rdfs:label>
    </owl:DatatypeProperty>



    <!-- https://w3id.org/italia/social-security/onto/socialSafetyNet/dataValiditàSanzioneNASpI -->

    <owl:DatatypeProperty rdf:about="https://w3id.org/italia/social-security/onto/socialSafetyNet/dataValiditàSanzioneNASpI">
        <rdf:type rdf:resource="http://www.w3.org/2002/07/owl#FunctionalProperty"/>
        <rdfs:domain rdf:resource="https://w3id.org/italia/social-security/onto/socialSafetyNet/SanzionePerViolazioneObblighiNASpI"/>
        <rdfs:range rdf:resource="http://www.w3.org/2001/XMLSchema#dateTime"/>
        <rdfs:comment xml:lang="it">Data da cui decorre la sanzione.</rdfs:comment>
        <rdfs:comment xml:lang="en">Date from which the sanction takes effect.</rdfs:comment>
        <rdfs:label xml:lang="en">NASpI sanction validity date</rdfs:label>
        <rdfs:label xml:lang="it">data validità sanzione NASpI</rdfs:label>
    </owl:DatatypeProperty>



    <!-- https://w3id.org/italia/social-security/onto/socialSafetyNet/durataEffettivaPrestazioneNASpI -->

    <owl:DatatypeProperty rdf:about="https://w3id.org/italia/social-security/onto/socialSafetyNet/durataEffettivaPrestazioneNASpI">
        <rdf:type rdf:resource="http://www.w3.org/2002/07/owl#FunctionalProperty"/>
        <rdfs:domain rdf:resource="https://w3id.org/italia/social-security/onto/socialSafetyNet/PrestazioneNASpI"/>
        <rdfs:range rdf:resource="http://www.w3.org/2001/XMLSchema#decimal"/>
        <rdfs:comment xml:lang="it">Durata effettiva in giorni della Prestazione NASpI calcolata al momento della terminazione della prestazione.</rdfs:comment>
        <rdfs:comment xml:lang="en">Effective duration in days of the NASpI Benefit calculated at the time of termination of the benefit.</rdfs:comment>
        <rdfs:label xml:lang="it">durata effettiva prestazione NASpI</rdfs:label>
        <rdfs:label xml:lang="en">effective NASpI benefit duration</rdfs:label>
    </owl:DatatypeProperty>



    <!-- https://w3id.org/italia/social-security/onto/socialSafetyNet/durataTeoricaPrestazioneNASpI -->

    <owl:DatatypeProperty rdf:about="https://w3id.org/italia/social-security/onto/socialSafetyNet/durataTeoricaPrestazioneNASpI">
        <rdf:type rdf:resource="http://www.w3.org/2002/07/owl#FunctionalProperty"/>
        <rdfs:domain rdf:resource="https://w3id.org/italia/social-security/onto/socialSafetyNet/PrestazioneNASpI"/>
        <rdfs:range rdf:resource="http://www.w3.org/2001/XMLSchema#decimal"/>
        <rdfs:comment xml:lang="it">Durata stimata in giorni della Prestazione NASpI al momento dell&apos;accoglimento della domanda.</rdfs:comment>
        <rdfs:comment xml:lang="en">Estimated duration in days of the NASpI benefit at the time of acceptance of the application.</rdfs:comment>
        <rdfs:label xml:lang="it">durata teorica prestazione NASpI</rdfs:label>
        <rdfs:label xml:lang="en">theoretical NASpI benefit duration</rdfs:label>
    </owl:DatatypeProperty>



    <!-- https://w3id.org/italia/social-security/onto/socialSafetyNet/imponibileContributivo -->

    <owl:DatatypeProperty rdf:about="https://w3id.org/italia/social-security/onto/socialSafetyNet/imponibileContributivo">
        <rdf:type rdf:resource="http://www.w3.org/2002/07/owl#FunctionalProperty"/>
        <rdfs:domain rdf:resource="https://w3id.org/italia/social-security/onto/socialSafetyNet/ContributoObbligatorio"/>
        <rdfs:range rdf:resource="http://www.w3.org/2001/XMLSchema#decimal"/>
        <rdfs:label xml:lang="it">imponibile contributivo</rdfs:label>
        <rdfs:label xml:lang="en">taxable contribution</rdfs:label>
    </owl:DatatypeProperty>



    <!-- https://w3id.org/italia/social-security/onto/socialSafetyNet/importoLordoMensileIndennitàNASpI -->

    <owl:DatatypeProperty rdf:about="https://w3id.org/italia/social-security/onto/socialSafetyNet/importoLordoMensileIndennitàNASpI">
        <rdf:type rdf:resource="http://www.w3.org/2002/07/owl#FunctionalProperty"/>
        <rdfs:domain rdf:resource="https://w3id.org/italia/social-security/onto/socialSafetyNet/StatoDiErogatoDiNASpI"/>
        <rdfs:range rdf:resource="http://www.w3.org/2001/XMLSchema#decimal"/>
        <rdfs:comment xml:lang="it">Importo mensile dell&apos;indennità NASpI. Tale importo può cambiare nel tempo (dal quarto mese di erogazione l&apos;indennità viene decurtata del 3% al mese) dando luogo nuove istanze di Stato di erogato di NASpI.</rdfs:comment>
        <rdfs:comment xml:lang="en">Monthly amount of NASpI allowance. This amount may change over time (from the fourth month of disbursement, the indemnity is reduced by 3% per month), giving rise to new NASpI disbursement status.</rdfs:comment>
        <rdfs:label xml:lang="en">gross monthly amount NASpI allowance</rdfs:label>
        <rdfs:label xml:lang="it">importo lordo mensile indennità NASpI</rdfs:label>
    </owl:DatatypeProperty>



    <!-- https://w3id.org/italia/social-security/onto/socialSafetyNet/importoMensileIniziale -->

    <owl:DatatypeProperty rdf:about="https://w3id.org/italia/social-security/onto/socialSafetyNet/importoMensileIniziale">
        <rdf:type rdf:resource="http://www.w3.org/2002/07/owl#FunctionalProperty"/>
        <rdfs:domain rdf:resource="https://w3id.org/italia/social-security/onto/socialSafetyNet/StatoDiAccoltaDiDomandaNASpI"/>
        <rdfs:range rdf:resource="http://www.w3.org/2001/XMLSchema#decimal"/>
        <rdfs:comment xml:lang="it">Importo lordo mensile iniziale dell&apos;indennità NASpI.</rdfs:comment>
        <rdfs:comment xml:lang="en">Initial gross monthly amount of NASpI allowance.</rdfs:comment>
        <rdfs:label xml:lang="it">importo mensile iniziale</rdfs:label>
        <rdfs:label xml:lang="en">initial monthly amount</rdfs:label>
    </owl:DatatypeProperty>



    <!-- https://w3id.org/italia/social-security/onto/socialSafetyNet/importoRetribuzioneUtileComplessiva -->

    <owl:DatatypeProperty rdf:about="https://w3id.org/italia/social-security/onto/socialSafetyNet/importoRetribuzioneUtileComplessiva">
        <rdf:type rdf:resource="http://www.w3.org/2002/07/owl#FunctionalProperty"/>
        <rdfs:domain rdf:resource="https://w3id.org/italia/social-security/onto/socialSafetyNet/StatoDiAccoltaDiDomandaNASpI"/>
        <rdfs:range rdf:resource="http://www.w3.org/2001/XMLSchema#decimal"/>
        <rdfs:comment xml:lang="it">Retribuzione lorda totale nell&apos;ultimo quadriennio.</rdfs:comment>
        <rdfs:comment xml:lang="en">Total gross salary over the last four years.</rdfs:comment>
        <rdfs:label xml:lang="it">importo retribuzione utile complessiva</rdfs:label>
        <rdfs:label xml:lang="en">total earnings amount</rdfs:label>
    </owl:DatatypeProperty>



    <!-- https://w3id.org/italia/social-security/onto/socialSafetyNet/importoSanzioneNASpI -->

    <owl:DatatypeProperty rdf:about="https://w3id.org/italia/social-security/onto/socialSafetyNet/importoSanzioneNASpI">
        <rdf:type rdf:resource="http://www.w3.org/2002/07/owl#FunctionalProperty"/>
        <rdfs:domain rdf:resource="https://w3id.org/italia/social-security/onto/socialSafetyNet/SanzionePerViolazioneObblighiNASpI"/>
        <rdfs:range rdf:resource="http://www.w3.org/2001/XMLSchema#decimal"/>
        <rdfs:comment xml:lang="it">Importo della sanzione che verrà defalcato dall&apos;importo lordo mensile indennità NASpI.</rdfs:comment>
        <rdfs:comment xml:lang="en">The amount of the penalty that will be deducted from the gross monthly amount NASpI allowance.</rdfs:comment>
        <rdfs:label xml:lang="en">NASpI sanction amount</rdfs:label>
        <rdfs:label xml:lang="it">importo sanzione NASpI</rdfs:label>
    </owl:DatatypeProperty>



    <!-- https://w3id.org/italia/social-security/onto/socialSafetyNet/matricolaINPS -->

    <owl:DatatypeProperty rdf:about="https://w3id.org/italia/social-security/onto/socialSafetyNet/matricolaINPS">
        <rdf:type rdf:resource="http://www.w3.org/2002/07/owl#FunctionalProperty"/>
        <rdfs:domain rdf:resource="https://w3id.org/italia/social-security/onto/socialSafetyNet/DatoreDiLavoro"/>
        <rdfs:range rdf:resource="http://www.w3.org/2001/XMLSchema#string"/>
        <rdfs:comment xml:lang="en">A 10-digit numeric code that is assigned by INPS to an Employer.</rdfs:comment>
        <rdfs:comment xml:lang="it">Codice numerico composto da 10 cifre che viene assegnato dall&apos;INPS aa un Datore di lavoro.</rdfs:comment>
        <rdfs:label xml:lang="en">INPS matriculation number</rdfs:label>
        <rdfs:label xml:lang="it">matricola INPS</rdfs:label>
    </owl:DatatypeProperty>



    <!-- https://w3id.org/italia/social-security/onto/socialSafetyNet/nomeConfederazioneSindacale -->

    <owl:DatatypeProperty rdf:about="https://w3id.org/italia/social-security/onto/socialSafetyNet/nomeConfederazioneSindacale">
        <rdf:type rdf:resource="http://www.w3.org/2002/07/owl#FunctionalProperty"/>
        <rdfs:domain rdf:resource="https://w3id.org/italia/social-security/onto/socialSafetyNet/AssociazioneSindacale"/>
        <rdfs:range rdf:resource="http://www.w3.org/2001/XMLSchema#string"/>
        <rdfs:comment xml:lang="en">Name of the federation that brings together several trade unions.</rdfs:comment>
        <rdfs:comment xml:lang="it">Nome della federazione che raggruppa diverse sigle sindacali.</rdfs:comment>
        <rdfs:label xml:lang="it">nome confederazione sindacale</rdfs:label>
        <rdfs:label xml:lang="en">trade union confederation name</rdfs:label>
    </owl:DatatypeProperty>



    <!-- https://w3id.org/italia/social-security/onto/socialSafetyNet/notaComunicazioneNASpI -->

    <owl:DatatypeProperty rdf:about="https://w3id.org/italia/social-security/onto/socialSafetyNet/notaComunicazioneNASpI">
        <rdf:type rdf:resource="http://www.w3.org/2002/07/owl#FunctionalProperty"/>
        <rdfs:domain rdf:resource="https://w3id.org/italia/social-security/onto/socialSafetyNet/ComunicazioneNASpI"/>
        <rdfs:range rdf:resource="http://www.w3.org/2001/XMLSchema#string"/>
        <rdfs:comment xml:lang="it">Nota di testo per integrare le informazioni inserite in una Comunicazione NASpI come, ad esempio, il reddito previsto per una nuova attività lavorativa.</rdfs:comment>
        <rdfs:comment xml:lang="en">Text note to supplement the information entered in a NASpI Communication such as, for example, the expected income for a new job.</rdfs:comment>
        <rdfs:label xml:lang="en">NASpI communication note</rdfs:label>
        <rdfs:label xml:lang="it">nota comunicazione NASpI</rdfs:label>
    </owl:DatatypeProperty>



    <!-- https://w3id.org/italia/social-security/onto/socialSafetyNet/notaDomandaNASpI -->

    <owl:DatatypeProperty rdf:about="https://w3id.org/italia/social-security/onto/socialSafetyNet/notaDomandaNASpI">
        <rdf:type rdf:resource="http://www.w3.org/2002/07/owl#FunctionalProperty"/>
        <rdfs:domain rdf:resource="https://w3id.org/italia/social-security/onto/socialSafetyNet/DomandaNASpI"/>
        <rdfs:range rdf:resource="http://www.w3.org/2001/XMLSchema#string"/>
        <rdfs:comment xml:lang="it">Nota di testo per integrare le informazioni inserite in una Domanda NASpI.</rdfs:comment>
        <rdfs:comment xml:lang="en">Text note to supplement the information entered in a NASpI claim.</rdfs:comment>
        <rdfs:label xml:lang="en">NASpI claim note</rdfs:label>
        <rdfs:label xml:lang="it">nota domanda NASpI</rdfs:label>
    </owl:DatatypeProperty>



    <!-- https://w3id.org/italia/social-security/onto/socialSafetyNet/numeroDomusNASpI -->

    <owl:DatatypeProperty rdf:about="https://w3id.org/italia/social-security/onto/socialSafetyNet/numeroDomusNASpI">
        <rdf:type rdf:resource="http://www.w3.org/2002/07/owl#FunctionalProperty"/>
        <rdfs:domain rdf:resource="https://w3id.org/italia/social-security/onto/socialSafetyNet/StatoDiDomandaNASpI"/>
        <rdfs:range rdf:resource="http://www.w3.org/2001/XMLSchema#string"/>
        <rdfs:comment xml:lang="it">Identificativo progressivo emesso al momento della redazione di una Domanda NASpI così come per ogni domanda di prestazione richiesta all&apos;INPS.</rdfs:comment>
        <rdfs:comment xml:lang="en">Progressive identifier issued at the time of drafting a NASpI Application as well as for each application for benefits requested from INPS.</rdfs:comment>
        <rdfs:label xml:lang="en">NASpI Domus number</rdfs:label>
        <rdfs:label xml:lang="it">numero Domus NASpI</rdfs:label>
    </owl:DatatypeProperty>



    <!-- https://w3id.org/italia/social-security/onto/socialSafetyNet/numeroIscrizioneAlboProfessionale -->

    <owl:DatatypeProperty rdf:about="https://w3id.org/italia/social-security/onto/socialSafetyNet/numeroIscrizioneAlboProfessionale">
        <rdf:type rdf:resource="http://www.w3.org/2002/07/owl#FunctionalProperty"/>
        <rdfs:domain rdf:resource="https://w3id.org/italia/social-security/onto/socialSafetyNet/IscrizioneAlboProfessionale"/>
        <rdfs:range rdf:resource="http://www.w3.org/2001/XMLSchema#string"/>
        <rdfs:comment xml:lang="it">Identifica la singola iscrizione nell&apos;ambito di un Albo professionale.</rdfs:comment>
        <rdfs:comment xml:lang="en">Identifies the individual entry in a Professional register.</rdfs:comment>
        <rdfs:label xml:lang="it">numero iscrizione albo professionale</rdfs:label>
        <rdfs:label xml:lang="en">professional register registration number</rdfs:label>
    </owl:DatatypeProperty>



    <!-- https://w3id.org/italia/social-security/onto/socialSafetyNet/numeroOreDiPrestazioneLavorativa -->

    <owl:DatatypeProperty rdf:about="https://w3id.org/italia/social-security/onto/socialSafetyNet/numeroOreDiPrestazioneLavorativa">
        <rdf:type rdf:resource="http://www.w3.org/2002/07/owl#FunctionalProperty"/>
        <rdfs:domain rdf:resource="https://w3id.org/italia/social-security/onto/socialSafetyNet/PrestazioneLavorativaEffettiva"/>
        <rdfs:range rdf:resource="http://www.w3.org/2001/XMLSchema#decimal"/>
        <rdfs:comment xml:lang="it">Indica la durata in ore di una singola Prestazione lavorativa effettiva</rdfs:comment>
        <rdfs:comment xml:lang="en">Indicates the duration in hours of a single Actual work provision</rdfs:comment>
        <rdfs:label xml:lang="it">numero ore di prestazione lavorativa</rdfs:label>
        <rdfs:label xml:lang="en">work hours number</rdfs:label>
    </owl:DatatypeProperty>



    <!-- https://w3id.org/italia/social-security/onto/socialSafetyNet/numeroPraticaNASpIDelDelegato -->

    <owl:DatatypeProperty rdf:about="https://w3id.org/italia/social-security/onto/socialSafetyNet/numeroPraticaNASpIDelDelegato">
        <rdf:type rdf:resource="http://www.w3.org/2002/07/owl#FunctionalProperty"/>
        <rdfs:domain rdf:resource="https://w3id.org/italia/social-security/onto/socialSafetyNet/DomandaNASpI"/>
        <rdfs:range rdf:resource="http://www.w3.org/2001/XMLSchema#string"/>
        <rdfs:comment xml:lang="it">Identificativo assegnato dal delegato, tipicamente un Patronato, alla pratica riguardante la presentazione della domanda di NASpI per conto del cittadino delegante ovvero il Richiedente NASpI.</rdfs:comment>
        <rdfs:comment xml:lang="en">Identifier assigned by the delegate, typically a Patronato, to the file concerning the submission of the NASpI claim on behalf of the delegating citizen or the NASpI Applicant.</rdfs:comment>
        <rdfs:label xml:lang="en">delegate NASpI claim number</rdfs:label>
        <rdfs:label xml:lang="it">numero pratica NASpI del delegato</rdfs:label>
    </owl:DatatypeProperty>



    <!-- https://w3id.org/italia/social-security/onto/socialSafetyNet/numeroProtocolloNASpI -->

    <owl:DatatypeProperty rdf:about="https://w3id.org/italia/social-security/onto/socialSafetyNet/numeroProtocolloNASpI">
        <rdf:type rdf:resource="http://www.w3.org/2002/07/owl#FunctionalProperty"/>
        <rdfs:domain>
            <owl:Class>
                <owl:unionOf rdf:parseType="Collection">
                    <rdf:Description rdf:about="https://w3id.org/italia/social-security/onto/socialSafetyNet/ComunicazioneNASpI"/>
                    <rdf:Description rdf:about="https://w3id.org/italia/social-security/onto/socialSafetyNet/StatoDiDomandaNASpI"/>
                </owl:unionOf>
            </owl:Class>
        </rdfs:domain>
        <rdfs:range rdf:resource="http://www.w3.org/2001/XMLSchema#string"/>
        <rdfs:comment xml:lang="it">Numero di protocollo assegnato ad una Domanda NASpI o ad una Comunicazione NASpI. L&apos;assegnazione potrebbe avvenire anche in un momento successivo alla data di trasmissione.</rdfs:comment>
        <rdfs:comment xml:lang="en">Protocol number assigned to a NASpI claim or NASpI Communication. The assignment may also take place after the date of transmission.</rdfs:comment>
        <rdfs:label xml:lang="en">NASpI protocol number</rdfs:label>
        <rdfs:label xml:lang="it">numero protocollo NASpI</rdfs:label>
    </owl:DatatypeProperty>



    <!-- https://w3id.org/italia/social-security/onto/socialSafetyNet/numeroSettimaneContributiveUtilizzate -->

    <owl:DatatypeProperty rdf:about="https://w3id.org/italia/social-security/onto/socialSafetyNet/numeroSettimaneContributiveUtilizzate">
        <rdf:type rdf:resource="http://www.w3.org/2002/07/owl#FunctionalProperty"/>
        <rdfs:domain rdf:resource="https://w3id.org/italia/social-security/onto/socialSafetyNet/PrestazioneNASpI"/>
        <rdfs:range rdf:resource="http://www.w3.org/2001/XMLSchema#decimal"/>
        <rdfs:comment xml:lang="en">Number of contribution weeks used for the provision of a NASpI Benefit.</rdfs:comment>
        <rdfs:comment xml:lang="it">Numero di settimane contributive utilizzate per l&apos;erogazione di una Prestazione NASpI.</rdfs:comment>
        <rdfs:label xml:lang="en">contribution weeks used number</rdfs:label>
        <rdfs:label xml:lang="it">numero settimane contributive utilizzate</rdfs:label>
    </owl:DatatypeProperty>



    <!-- https://w3id.org/italia/social-security/onto/socialSafetyNet/numeroSettimaneLavorate -->

    <owl:DatatypeProperty rdf:about="https://w3id.org/italia/social-security/onto/socialSafetyNet/numeroSettimaneLavorate">
        <rdf:type rdf:resource="http://www.w3.org/2002/07/owl#FunctionalProperty"/>
        <rdfs:domain rdf:resource="https://w3id.org/italia/social-security/onto/socialSafetyNet/StatoDiAccoltaDiDomandaNASpI"/>
        <rdfs:range rdf:resource="http://www.w3.org/2001/XMLSchema#decimal"/>
        <rdfs:comment xml:lang="en">Number of contribution weeks in the last four years.</rdfs:comment>
        <rdfs:comment xml:lang="it">Numero di settimane lavorate nell&apos;ultimo quadriennio.</rdfs:comment>
        <rdfs:label xml:lang="it">numero settimane lavorate</rdfs:label>
        <rdfs:label xml:lang="en">weeks worked number</rdfs:label>
    </owl:DatatypeProperty>



    <!-- https://w3id.org/italia/social-security/onto/socialSafetyNet/numeroUnitàTemporaliPerDiritto -->

    <owl:DatatypeProperty rdf:about="https://w3id.org/italia/social-security/onto/socialSafetyNet/numeroUnitàTemporaliPerDiritto">
        <rdf:type rdf:resource="http://www.w3.org/2002/07/owl#FunctionalProperty"/>
        <rdfs:domain rdf:resource="https://w3id.org/italia/social-security/onto/socialSafetyNet/ContributoObbligatorio"/>
        <rdfs:range rdf:resource="http://www.w3.org/2001/XMLSchema#decimal"/>
        <rdfs:comment xml:lang="en">Amount of contributions useful in the period for pension entitlement.</rdfs:comment>
        <rdfs:comment xml:lang="it">Quantità di contributi utili nel periodo per il diritto alla pensione.</rdfs:comment>
        <rdfs:label xml:lang="it">numero unità temporali per diritto</rdfs:label>
        <rdfs:label xml:lang="en">time units number per entitlement</rdfs:label>
    </owl:DatatypeProperty>



    <!-- https://w3id.org/italia/social-security/onto/socialSafetyNet/numeroUnitàTemporaliPerMisura -->

    <owl:DatatypeProperty rdf:about="https://w3id.org/italia/social-security/onto/socialSafetyNet/numeroUnitàTemporaliPerMisura">
        <rdf:type rdf:resource="http://www.w3.org/2002/07/owl#FunctionalProperty"/>
        <rdfs:domain rdf:resource="https://w3id.org/italia/social-security/onto/socialSafetyNet/ContributoObbligatorio"/>
        <rdfs:range rdf:resource="http://www.w3.org/2001/XMLSchema#decimal"/>
        <rdfs:comment xml:lang="en">Amount of contributions useful in the period for the pension measure.</rdfs:comment>
        <rdfs:comment xml:lang="it">Quantità di contributi utili nel periodo per la misura della pensione.</rdfs:comment>
        <rdfs:label xml:lang="it">numero unità temporali per misura</rdfs:label>
        <rdfs:label xml:lang="en">time units number per measure</rdfs:label>
    </owl:DatatypeProperty>



    <!-- https://w3id.org/italia/social-security/onto/socialSafetyNet/numeroUnitàTemporaliUtilizzatePerDisoccupazione -->

    <owl:DatatypeProperty rdf:about="https://w3id.org/italia/social-security/onto/socialSafetyNet/numeroUnitàTemporaliUtilizzatePerDisoccupazione">
        <rdf:type rdf:resource="http://www.w3.org/2002/07/owl#FunctionalProperty"/>
        <rdfs:domain rdf:resource="https://w3id.org/italia/social-security/onto/socialSafetyNet/ContributoAssicurazioneGeneraleObbligatoria"/>
        <rdfs:range rdf:resource="http://www.w3.org/2001/XMLSchema#decimal"/>
        <rdfs:comment xml:lang="en">Amount of contributions for the period used towards entitlement to unemployment benefits.</rdfs:comment>
        <rdfs:comment xml:lang="it">Quantità di contributi del periodo utilizzati ai fini del diritto a fruire delle indennità per la disoccupazione.</rdfs:comment>
        <rdfs:label xml:lang="it">numero unità temporali utilizzate per disoccupazione</rdfs:label>
        <rdfs:label xml:lang="en">time units number used for unemployment</rdfs:label>
    </owl:DatatypeProperty>



    <!-- https://w3id.org/italia/social-security/onto/socialSafetyNet/partitaIVA -->

    <owl:DatatypeProperty rdf:about="https://w3id.org/italia/social-security/onto/socialSafetyNet/partitaIVA">
        <rdf:type rdf:resource="http://www.w3.org/2002/07/owl#FunctionalProperty"/>
        <rdfs:domain rdf:resource="https://w3id.org/italia/social-security/onto/socialSafetyNet/LavoratoreAPartitaIVA"/>
        <rdfs:range rdf:resource="http://www.w3.org/2001/XMLSchema#string"/>
        <rdfs:comment xml:lang="en">An 11-digit numeric code that uniquely identifies a person who carries out an activity, business or otherwise, relevant for the purposes of indirect taxation (VAT).</rdfs:comment>
        <rdfs:comment xml:lang="it">Codice numerico di 11 cifre che identifica univocamente un soggetto che esercita un&apos;attività, di impresa e non, rilevante ai fini dell&apos;imposizione fiscale indiretta (IVA).</rdfs:comment>
        <rdfs:label xml:lang="en">VAT</rdfs:label>
        <rdfs:label xml:lang="it">partita IVA</rdfs:label>
    </owl:DatatypeProperty>



    <!-- https://w3id.org/italia/social-security/onto/socialSafetyNet/redditoPrevistoAttivitàCorrente -->

    <owl:DatatypeProperty rdf:about="https://w3id.org/italia/social-security/onto/socialSafetyNet/redditoPrevistoAttivitàCorrente">
        <rdf:type rdf:resource="http://www.w3.org/2002/07/owl#FunctionalProperty"/>
        <rdfs:domain rdf:resource="https://w3id.org/italia/social-security/onto/socialSafetyNet/AttivitàCorrente"/>
        <rdfs:range rdf:resource="http://www.w3.org/2001/XMLSchema#decimal"/>
        <rdfs:comment xml:lang="en">Income generated by a Current activity that the NASpI Applicant expects to receive during the year. In the case of self-employed workers, freelancers and parasubordinates, an expected income must always be indicated, even if it is zero.</rdfs:comment>
        <rdfs:comment xml:lang="it">Reddito generato da una Attività corrente che il Richiedente NASpI prevede di percepire nell&apos;anno. Nel caso di lavoratori autonomi, liberi professionisti e parasubordinati dovrà sempre essere indicato un reddito previsto anche se pari a zero.</rdfs:comment>
        <rdfs:label xml:lang="en">expected income current activity</rdfs:label>
        <rdfs:label xml:lang="it">reddito previsto attività corrente</rdfs:label>
    </owl:DatatypeProperty>



    <!-- https://w3id.org/italia/social-security/onto/socialSafetyNet/seCessazioneSenzaPreavviso -->

    <owl:DatatypeProperty rdf:about="https://w3id.org/italia/social-security/onto/socialSafetyNet/seCessazioneSenzaPreavviso">
        <rdf:type rdf:resource="http://www.w3.org/2002/07/owl#FunctionalProperty"/>
        <rdfs:domain rdf:resource="https://w3id.org/italia/social-security/onto/socialSafetyNet/AttoDiCessazioneRapportoDiLavoro"/>
        <rdfs:range rdf:resource="http://www.w3.org/2001/XMLSchema#boolean"/>
        <rdfs:comment xml:lang="it">Indica se un Atto di cessazione rapporto di lavoro non ha dato luogo al dovuto periodo di preavviso neanche sotto forma di indennizzo.</rdfs:comment>
        <rdfs:comment xml:lang="en">Indicates whether a Employment termination deed has not given rise to the due period of notice or in the form of compensation.</rdfs:comment>
        <rdfs:label xml:lang="en">dismissal without notice flag</rdfs:label>
        <rdfs:label xml:lang="it">se cessazione senza preavviso</rdfs:label>
    </owl:DatatypeProperty>



    <!-- https://w3id.org/italia/social-security/onto/socialSafetyNet/seIndennitàMancatoPreavviso -->

    <owl:DatatypeProperty rdf:about="https://w3id.org/italia/social-security/onto/socialSafetyNet/seIndennitàMancatoPreavviso">
        <rdf:type rdf:resource="http://www.w3.org/2002/07/owl#FunctionalProperty"/>
        <rdfs:domain rdf:resource="https://w3id.org/italia/social-security/onto/socialSafetyNet/DomandaNASpI"/>
        <rdfs:range rdf:resource="http://www.w3.org/2001/XMLSchema#boolean"/>
        <rdfs:comment xml:lang="it">Indica se il Richiedente NASpI percepirà l&apos;indennità di mancato preavviso relativamente al rapporto di lavoro appena cessato. </rdfs:comment>
        <rdfs:comment xml:lang="en">Indicates whether the NASpI Applicant will receive compensation for failure to give notice in respect of the employment relationship that has just ended.</rdfs:comment>
        <rdfs:label xml:lang="it">se indennità mancato preavviso</rdfs:label>
        <rdfs:label xml:lang="en">without notice dismissal allowance flag</rdfs:label>
    </owl:DatatypeProperty>



    <!-- https://w3id.org/italia/social-security/onto/socialSafetyNet/seIscrittoAlbo-CassaProfessionale -->

    <owl:DatatypeProperty rdf:about="https://w3id.org/italia/social-security/onto/socialSafetyNet/seIscrittoAlbo-CassaProfessionale">
        <rdf:type rdf:resource="http://www.w3.org/2002/07/owl#FunctionalProperty"/>
        <rdfs:domain rdf:resource="https://w3id.org/italia/social-security/onto/socialSafetyNet/RichiedenteNASpI"/>
        <rdfs:range rdf:resource="http://www.w3.org/2001/XMLSchema#boolean"/>
        <rdfs:comment xml:lang="it">Indica se il Richiedente NASpI è iscritto a un Albo professionale o una Cassa professionale. In tal caso si dovrà sempre indicare una Attività corrente anche con reddito previsto pari a zero.</rdfs:comment>
        <rdfs:comment xml:lang="en">Indicates whether the NASpI Applicant is registered in a Professional register or a Professional fund. In this case, you will always have to indicate a Current activity even with an expected income of zero.</rdfs:comment>
        <rdfs:label xml:lang="en">professional register-fund registered flag</rdfs:label>
        <rdfs:label xml:lang="it">se iscritto albo-cassa professionale</rdfs:label>
    </owl:DatatypeProperty>



    <!-- https://w3id.org/italia/social-security/onto/socialSafetyNet/seLicenziatoPerSuperamentoPeriodoComporto -->

    <owl:DatatypeProperty rdf:about="https://w3id.org/italia/social-security/onto/socialSafetyNet/seLicenziatoPerSuperamentoPeriodoComporto">
        <rdf:type rdf:resource="http://www.w3.org/2002/07/owl#FunctionalProperty"/>
        <rdfs:domain rdf:resource="https://w3id.org/italia/social-security/onto/socialSafetyNet/RichiedenteNASpI"/>
        <rdfs:range rdf:resource="http://www.w3.org/2001/XMLSchema#boolean"/>
        <rdfs:comment xml:lang="it">Indica se il Richiedente NASpI è stato licenziato per superamento del periodo di comporto ovvero del limite massimo stabilito dalla legge, dai contratti collettivi, o in via residuale, dagli usi, di assenza per malattia.</rdfs:comment>
        <rdfs:comment xml:lang="en">Indicates whether the NASpI Applicant has been dismissed for exceeding the protected period or the maximum limit established by law, collective agreements, or residually, by customs, of absence due to illness.</rdfs:comment>
        <rdfs:label xml:lang="en">dismissed for exceeding illness period protected flag</rdfs:label>
        <rdfs:label xml:lang="it">se licenziato per superamento periodo comporto</rdfs:label>
    </owl:DatatypeProperty>



    <!-- https://w3id.org/italia/social-security/onto/socialSafetyNet/seRichiestaDetrazionePerLavoroDipendente -->

    <owl:DatatypeProperty rdf:about="https://w3id.org/italia/social-security/onto/socialSafetyNet/seRichiestaDetrazionePerLavoroDipendente">
        <rdf:type rdf:resource="http://www.w3.org/2002/07/owl#FunctionalProperty"/>
        <rdfs:domain rdf:resource="https://w3id.org/italia/social-security/onto/socialSafetyNet/StatoDiErogatoDiNASpI"/>
        <rdfs:range rdf:resource="http://www.w3.org/2001/XMLSchema#boolean"/>
        <rdfs:comment xml:lang="it">Indica la richiesta da parte del beneficiario dell&apos;applicazione delle detrazioni per redditi di lavoro dipendente e assimilati.</rdfs:comment>
        <rdfs:comment xml:lang="en">Indicates the beneficiary&apos;s request for the application of deductions for employment income and similar income.</rdfs:comment>
        <rdfs:label xml:lang="en">employment deduction request flag</rdfs:label>
        <rdfs:label xml:lang="it">se richiesta detrazione per lavoro dipendente</rdfs:label>
    </owl:DatatypeProperty>



    <!-- https://w3id.org/italia/social-security/onto/socialSafetyNet/seSocioDiSocietà -->

    <owl:DatatypeProperty rdf:about="https://w3id.org/italia/social-security/onto/socialSafetyNet/seSocioDiSocietà">
        <rdf:type rdf:resource="http://www.w3.org/2002/07/owl#FunctionalProperty"/>
        <rdfs:domain rdf:resource="https://w3id.org/italia/social-security/onto/socialSafetyNet/RichiedenteNASpI"/>
        <rdfs:range rdf:resource="http://www.w3.org/2001/XMLSchema#boolean"/>
        <rdfs:comment xml:lang="it">Indica se il Richiedente NASpI è socio di una società di persone o capitali. In tal caso si dovrà sempre indicare una Attività corrente anche con reddito previsto pari a zero.</rdfs:comment>
        <rdfs:comment xml:lang="en">Indicates whether the NASpI Applicant is a partner in a partnership or corporation. In this case, you will always have to indicate a Current activity even with an expected income of zero.</rdfs:comment>
        <rdfs:label xml:lang="en">company partner flag</rdfs:label>
        <rdfs:label xml:lang="it">se socio di società</rdfs:label>
    </owl:DatatypeProperty>



    <!-- https://w3id.org/italia/social-security/onto/socialSafetyNet/seStatoDiMalattiaInCorso -->

    <owl:DatatypeProperty rdf:about="https://w3id.org/italia/social-security/onto/socialSafetyNet/seStatoDiMalattiaInCorso">
        <rdf:type rdf:resource="http://www.w3.org/2002/07/owl#FunctionalProperty"/>
        <rdfs:domain rdf:resource="https://w3id.org/italia/social-security/onto/socialSafetyNet/RichiedenteNASpI"/>
        <rdfs:range rdf:resource="http://www.w3.org/2001/XMLSchema#boolean"/>
        <rdfs:comment xml:lang="it">Indica se il Richiedente NASpI è attualmente (alla data della Domanda NASpI) in malattia o ricoverato.</rdfs:comment>
        <rdfs:comment xml:lang="en">Indicates whether the NASpI Applicant is currently (as of the date of the NASpI claim) ill or hospitalized.</rdfs:comment>
        <rdfs:label xml:lang="en">current illness status flag</rdfs:label>
        <rdfs:label xml:lang="it">se stato di malattia in corso</rdfs:label>
    </owl:DatatypeProperty>



    <!-- https://w3id.org/italia/social-security/onto/socialSafetyNet/seStatoDiMalattiaPregressa -->

    <owl:DatatypeProperty rdf:about="https://w3id.org/italia/social-security/onto/socialSafetyNet/seStatoDiMalattiaPregressa">
        <rdf:type rdf:resource="http://www.w3.org/2002/07/owl#FunctionalProperty"/>
        <rdfs:domain rdf:resource="https://w3id.org/italia/social-security/onto/socialSafetyNet/RichiedenteNASpI"/>
        <rdfs:range rdf:resource="http://www.w3.org/2001/XMLSchema#boolean"/>
        <rdfs:comment xml:lang="it">Indica se il Richiedente NASpI è stato in malattia o ricoverato. Ciò potrebbe giustificare un eventuale ritardo nella presentazione della Domanda NASpI.</rdfs:comment>
        <rdfs:comment xml:lang="en">Indicates whether the NASpI Applicant has been sick or hospitalized. This may justify a possible delay in the submission of the NASpI claim.</rdfs:comment>
        <rdfs:label xml:lang="en">previous illness status flag</rdfs:label>
        <rdfs:label xml:lang="it">se stato di malattia pregressa</rdfs:label>
    </owl:DatatypeProperty>



    <!-- https://w3id.org/italia/social-security/onto/socialSafetyNet/seSvolgeAttivitàAPartitaIVA -->

    <owl:DatatypeProperty rdf:about="https://w3id.org/italia/social-security/onto/socialSafetyNet/seSvolgeAttivitàAPartitaIVA">
        <rdf:type rdf:resource="http://www.w3.org/2002/07/owl#FunctionalProperty"/>
        <rdfs:domain rdf:resource="https://w3id.org/italia/social-security/onto/socialSafetyNet/RichiedenteNASpI"/>
        <rdfs:range rdf:resource="http://www.w3.org/2001/XMLSchema#boolean"/>
        <rdfs:comment xml:lang="it">Indica se il Richiedente NASpI, titolare di una Partita IVA, svolge un&apos;attività ad essa ricollegabile. In tal caso si dovrà sempre indicare una Attività corrente anche con reddito previsto pari a zero.</rdfs:comment>
        <rdfs:comment xml:lang="en">Indicates whether the NASpI Applicant, holder of a VAT number, carries out an activity related to it. In this case, you will always have to indicate a Current Asset even with an expected income of zero.</rdfs:comment>
        <rdfs:label xml:lang="en">VAT self-employed activity flag</rdfs:label>
        <rdfs:label xml:lang="it">se svolge attività a partita IVA</rdfs:label>
    </owl:DatatypeProperty>



    <!-- https://w3id.org/italia/social-security/onto/socialSafetyNet/seSvolgeAttivitàProfesionale -->

    <owl:DatatypeProperty rdf:about="https://w3id.org/italia/social-security/onto/socialSafetyNet/seSvolgeAttivitàProfesionale">
        <rdf:type rdf:resource="http://www.w3.org/2002/07/owl#FunctionalProperty"/>
        <rdfs:domain rdf:resource="https://w3id.org/italia/social-security/onto/socialSafetyNet/RichiedenteNASpI"/>
        <rdfs:range rdf:resource="http://www.w3.org/2001/XMLSchema#boolean"/>
        <rdfs:label xml:lang="it">se svolge attività profesionale</rdfs:label>
    </owl:DatatypeProperty>



    <!-- https://w3id.org/italia/social-security/onto/socialSafetyNet/seTitolareAssegnoDiInvalidità -->

    <owl:DatatypeProperty rdf:about="https://w3id.org/italia/social-security/onto/socialSafetyNet/seTitolareAssegnoDiInvalidità">
        <rdf:type rdf:resource="http://www.w3.org/2002/07/owl#FunctionalProperty"/>
        <rdfs:domain rdf:resource="https://w3id.org/italia/social-security/onto/socialSafetyNet/RichiedenteNASpI"/>
        <rdfs:range rdf:resource="http://www.w3.org/2001/XMLSchema#boolean"/>
        <rdfs:comment xml:lang="it">Indica se il Richiedente NASpI è titolare di un assegno di invalidità.</rdfs:comment>
        <rdfs:comment xml:lang="en">Indicates whether the NASpI Applicant is in receipt of a disability allowance.</rdfs:comment>
        <rdfs:label xml:lang="en">disability allowance holder flag</rdfs:label>
        <rdfs:label xml:lang="it">se titolare assegno di invalidità</rdfs:label>
    </owl:DatatypeProperty>



    <!-- https://w3id.org/italia/social-security/onto/socialSafetyNet/seTitolarePartitaIVA -->

    <owl:DatatypeProperty rdf:about="https://w3id.org/italia/social-security/onto/socialSafetyNet/seTitolarePartitaIVA">
        <rdf:type rdf:resource="http://www.w3.org/2002/07/owl#FunctionalProperty"/>
        <rdfs:domain rdf:resource="https://w3id.org/italia/social-security/onto/socialSafetyNet/RichiedenteNASpI"/>
        <rdfs:range rdf:resource="http://www.w3.org/2001/XMLSchema#boolean"/>
        <rdfs:comment xml:lang="it">Indica se il Richiedente NASpI possiede una Partita IVA. In tal caso si dovrà sempre indicare una Attività corrente anche con reddito previsto pari a zero.</rdfs:comment>
        <rdfs:comment xml:lang="en">Indicates whether the NASpI Applicant has a VAT number. In this case, you will always have to indicate a Current activity even with an expected income of zero.</rdfs:comment>
        <rdfs:label xml:lang="en">VAT holder flag</rdfs:label>
        <rdfs:label xml:lang="it">se titolare partita IVA</rdfs:label>
    </owl:DatatypeProperty>



    <!-- https://w3id.org/italia/social-security/onto/socialSafetyNet/siglaSindacale -->

    <owl:DatatypeProperty rdf:about="https://w3id.org/italia/social-security/onto/socialSafetyNet/siglaSindacale">
        <rdf:type rdf:resource="http://www.w3.org/2002/07/owl#FunctionalProperty"/>
        <rdfs:domain rdf:resource="https://w3id.org/italia/social-security/onto/socialSafetyNet/AssociazioneSindacale"/>
        <rdfs:range rdf:resource="http://www.w3.org/2001/XMLSchema#string"/>
        <rdfs:comment xml:lang="it">Acronimo di una organizzazione sindacale.</rdfs:comment>
        <rdfs:comment xml:lang="en">Acronym of a trade union organization.</rdfs:comment>
        <rdfs:label xml:lang="en">Trade union acronym</rdfs:label>
        <rdfs:label xml:lang="it">sigla sindacale</rdfs:label>
    </owl:DatatypeProperty>



    <!-- https://w3id.org/italia/social-security/onto/socialSafetyNet/unitàDiMisuraTemporale -->

    <owl:DatatypeProperty rdf:about="https://w3id.org/italia/social-security/onto/socialSafetyNet/unitàDiMisuraTemporale">
        <rdf:type rdf:resource="http://www.w3.org/2002/07/owl#FunctionalProperty"/>
        <rdfs:domain rdf:resource="https://w3id.org/italia/social-security/onto/socialSafetyNet/ContributoObbligatorio"/>
        <rdfs:range rdf:resource="http://www.w3.org/2001/XMLSchema#string"/>
        <rdfs:comment xml:lang="en">A unit of measurement used to indicate the number of useful contributions in the period. It can be days, weeks, or months.</rdfs:comment>
        <rdfs:comment xml:lang="it">Unità di misura con cui sono indiati il numero di contributi utili nel periodo. Possono essere giorni, settimane o mesi.</rdfs:comment>
        <rdfs:label xml:lang="en">measurement time unit</rdfs:label>
        <rdfs:label xml:lang="it">unità di misura temporale</rdfs:label>
    </owl:DatatypeProperty>



    <!--
    ///////////////////////////////////////////////////////////////////////////////////////
    //
    // Classes
    //
    ///////////////////////////////////////////////////////////////////////////////////////
     -->




    <!-- http://dati.gov.it/onto/dcatapit#Agent -->

    <owl:Class rdf:about="http://dati.gov.it/onto/dcatapit#Agent"/>



    <!-- http://dati.gov.it/onto/dcatapit#Distribution -->

    <owl:Class rdf:about="http://dati.gov.it/onto/dcatapit#Distribution"/>



    <!-- http://dati.gov.it/onto/dcatapit#Organization -->

    <owl:Class rdf:about="http://dati.gov.it/onto/dcatapit#Organization"/>



    <!-- http://www.w3.org/2006/vcard/ns#Kind -->

    <owl:Class rdf:about="http://www.w3.org/2006/vcard/ns#Kind"/>



    <!-- http://www.w3.org/2006/vcard/ns#Organization -->

    <owl:Class rdf:about="http://www.w3.org/2006/vcard/ns#Organization"/>



    <!-- http://www.w3.org/ns/dcat#Distribution -->

    <owl:Class rdf:about="http://www.w3.org/ns/dcat#Distribution"/>



    <!-- http://xmlns.com/foaf/0.1/Agent -->

    <owl:Class rdf:about="http://xmlns.com/foaf/0.1/Agent"/>



    <!-- https://w3id.org/italia/onto/ADMS/SemanticAssetDistribution -->

    <owl:Class rdf:about="https://w3id.org/italia/onto/ADMS/SemanticAssetDistribution"/>



    <!-- https://w3id.org/italia/onto/CLV/Country -->

    <owl:Class rdf:about="https://w3id.org/italia/onto/CLV/Country"/>



    <!-- https://w3id.org/italia/onto/CLV/Province -->

    <owl:Class rdf:about="https://w3id.org/italia/onto/CLV/Province"/>



    <!-- https://w3id.org/italia/onto/COV/Employment -->

    <owl:Class rdf:about="https://w3id.org/italia/onto/COV/Employment"/>



    <!-- https://w3id.org/italia/onto/COV/Organization -->

    <owl:Class rdf:about="https://w3id.org/italia/onto/COV/Organization"/>



    <!-- https://w3id.org/italia/onto/COV/PrivateOrganization -->

    <owl:Class rdf:about="https://w3id.org/italia/onto/COV/PrivateOrganization"/>



    <!-- https://w3id.org/italia/onto/COV/PublicOrganization -->

    <owl:Class rdf:about="https://w3id.org/italia/onto/COV/PublicOrganization"/>



    <!-- https://w3id.org/italia/onto/CPV/Alive -->

    <owl:Class rdf:about="https://w3id.org/italia/onto/CPV/Alive"/>



    <!-- https://w3id.org/italia/onto/TI/TimeIndexedEvent -->

    <owl:Class rdf:about="https://w3id.org/italia/onto/TI/TimeIndexedEvent"/>



    <!-- https://w3id.org/italia/onto/l0/Collection -->

    <owl:Class rdf:about="https://w3id.org/italia/onto/l0/Collection"/>



    <!-- https://w3id.org/italia/onto/l0/Sequence -->

    <owl:Class rdf:about="https://w3id.org/italia/onto/l0/Sequence"/>



    <!-- https://w3id.org/italia/social-security/onto/contributions/ContrattoDiLavoroDomestico -->

    <owl:Class rdf:about="https://w3id.org/italia/social-security/onto/contributions/ContrattoDiLavoroDomestico">
        <rdfs:subClassOf rdf:resource="https://w3id.org/italia/social-security/onto/socialSafetyNet/ContrattoATempoIndeterminato"/>
    </owl:Class>



    <!-- https://w3id.org/italia/social-security/onto/contributions/LavoratoreDomestico -->

    <owl:Class rdf:about="https://w3id.org/italia/social-security/onto/contributions/LavoratoreDomestico">
        <rdfs:subClassOf rdf:resource="https://w3id.org/italia/social-security/onto/socialSafetyNet/LavoratoreSubordinato"/>
        <rdfs:subClassOf>
            <owl:Restriction>
                <owl:onProperty rdf:resource="https://w3id.org/italia/social-security/onto/socialSafetyNet/accettaContrattoDiLavoro"/>
                <owl:someValuesFrom rdf:resource="https://w3id.org/italia/social-security/onto/contributions/ContrattoDiLavoroDomestico"/>
            </owl:Restriction>
        </rdfs:subClassOf>
    </owl:Class>



    <!-- https://w3id.org/italia/social-security/onto/core/RuoloDiAgente -->

    <owl:Class rdf:about="https://w3id.org/italia/social-security/onto/core/RuoloDiAgente"/>



    <!-- https://w3id.org/italia/social-security/onto/core/RuoloDiPersonaViva -->

    <owl:Class rdf:about="https://w3id.org/italia/social-security/onto/core/RuoloDiPersonaViva"/>



    <!-- https://w3id.org/italia/social-security/onto/core/SedeINPS -->

    <owl:Class rdf:about="https://w3id.org/italia/social-security/onto/core/SedeINPS"/>



    <!-- https://w3id.org/italia/social-security/onto/pensions/AttivitàEstera -->

    <owl:Class rdf:about="https://w3id.org/italia/social-security/onto/pensions/AttivitàEstera"/>



    <!-- https://w3id.org/italia/social-security/onto/pensions/Dichiarazione -->

    <owl:Class rdf:about="https://w3id.org/italia/social-security/onto/pensions/Dichiarazione">
        <rdfs:subClassOf>
            <owl:Restriction>
                <owl:onProperty>
                    <rdf:Description>
                        <owl:inverseOf rdf:resource="https://w3id.org/italia/social-security/onto/socialSafetyNet/haDichiarazionePerNASpI"/>
                    </rdf:Description>
                </owl:onProperty>
                <owl:someValuesFrom rdf:resource="http://www.w3.org/2002/07/owl#Thing"/>
            </owl:Restriction>
        </rdfs:subClassOf>
    </owl:Class>



    <!-- https://w3id.org/italia/social-security/onto/pensions/DocumentoAllegato -->

    <owl:Class rdf:about="https://w3id.org/italia/social-security/onto/pensions/DocumentoAllegato"/>



    <!-- https://w3id.org/italia/social-security/onto/pensions/TipoDiDelegato -->

    <owl:Class rdf:about="https://w3id.org/italia/social-security/onto/pensions/TipoDiDelegato"/>



    <!-- https://w3id.org/italia/social-security/onto/socialSafetyNet/AlboProfessionale -->

    <owl:Class rdf:about="https://w3id.org/italia/social-security/onto/socialSafetyNet/AlboProfessionale">
        <rdfs:subClassOf>
            <owl:Restriction>
                <owl:onProperty rdf:resource="https://w3id.org/italia/social-security/onto/socialSafetyNet/haAlboProfessionaleLocalizzatoIn"/>
                <owl:someValuesFrom rdf:resource="http://www.w3.org/2002/07/owl#Thing"/>
            </owl:Restriction>
        </rdfs:subClassOf>
        <rdfs:subClassOf>
            <owl:Restriction>
                <owl:onProperty>
                    <rdf:Description>
                        <owl:inverseOf rdf:resource="https://w3id.org/italia/social-security/onto/socialSafetyNet/haAlboProfessionale"/>
                    </rdf:Description>
                </owl:onProperty>
                <owl:someValuesFrom rdf:resource="http://www.w3.org/2002/07/owl#Thing"/>
            </owl:Restriction>
        </rdfs:subClassOf>
        <rdfs:comment xml:lang="en">A register in which the names and data of all persons authorized to practice a profession regulated by law are collected. State laws generally require registration in a specific register in order to carry out certain activities, particularly where the health and safety of citizens come into play. Registration in the register is essential especially for those who intend to work as freelancers, as it allows you to sign projects, appraisals, consultancy, certifications, etc., the lack of which is punishable by law (src.: Wikipedia).</rdfs:comment>
        <rdfs:comment xml:lang="it">Registro in cui sono raccolti i nomi e i dati di tutte le persone abilitate a esercitare una professione regolamentata dalla legge. Le leggi statali generalmente impongono l&apos;obbligo di iscrizione a uno specifico albo, per poter svolgere determinate attività, in particolare là dove entrano in gioco la salute e la sicurezza dei cittadini. L&apos;iscrizione all&apos;albo è fondamentale soprattutto per chi intende svolgere la libera professione, in quanto consente di firmare progetti, perizie, consulenze, certificazioni, ecc., la cui mancanza è punibile penalmente (fnt.: Wikipedia).</rdfs:comment>
        <rdfs:label xml:lang="it">Albo professionale</rdfs:label>
        <rdfs:label xml:lang="en">Professional Register</rdfs:label>
    </owl:Class>



    <!-- https://w3id.org/italia/social-security/onto/socialSafetyNet/Apprendista -->

    <owl:Class rdf:about="https://w3id.org/italia/social-security/onto/socialSafetyNet/Apprendista">
        <rdfs:subClassOf rdf:resource="https://w3id.org/italia/social-security/onto/socialSafetyNet/LavoratoreSubordinato"/>
        <rdfs:subClassOf>
            <owl:Restriction>
                <owl:onProperty rdf:resource="https://w3id.org/italia/social-security/onto/socialSafetyNet/accettaContrattoDiLavoro"/>
                <owl:someValuesFrom rdf:resource="https://w3id.org/italia/social-security/onto/socialSafetyNet/ContrattoDiApprendistato"/>
            </owl:Restriction>
        </rdfs:subClassOf>
        <rdfs:comment xml:lang="en">Employee subclass relating to those who sign an Apprenticeship agreement.</rdfs:comment>
        <rdfs:comment xml:lang="it">Sottoclasse di Lavoratore subordinato relativa a coloro che sottoscrivono un Contratto di apprendistato.</rdfs:comment>
        <rdfs:label xml:lang="it">Apprendista</rdfs:label>
        <rdfs:label xml:lang="en">Apprentice</rdfs:label>
    </owl:Class>



    <!-- https://w3id.org/italia/social-security/onto/socialSafetyNet/AssociazioneSindacale -->

    <owl:Class rdf:about="https://w3id.org/italia/social-security/onto/socialSafetyNet/AssociazioneSindacale">
        <rdfs:subClassOf rdf:resource="https://w3id.org/italia/onto/COV/PrivateOrganization"/>
        <rdfs:subClassOf>
            <owl:Restriction>
                <owl:onProperty rdf:resource="https://w3id.org/italia/social-security/onto/socialSafetyNet/nomeConfederazioneSindacale"/>
                <owl:someValuesFrom rdf:resource="http://www.w3.org/2000/01/rdf-schema#Literal"/>
            </owl:Restriction>
        </rdfs:subClassOf>
        <rdfs:subClassOf>
            <owl:Restriction>
                <owl:onProperty rdf:resource="https://w3id.org/italia/social-security/onto/socialSafetyNet/siglaSindacale"/>
                <owl:someValuesFrom rdf:resource="http://www.w3.org/2000/01/rdf-schema#Literal"/>
            </owl:Restriction>
        </rdfs:subClassOf>
        <rdfs:comment xml:lang="it">Ente che rappresenta una categoria di lavoratori o datori di lavoro in un rapporto di lavoro.</rdfs:comment>
        <rdfs:comment xml:lang="en">Entity that represents a category of workers or employers in an Work relationship.</rdfs:comment>
        <rdfs:label xml:lang="it">Associazione sindacale</rdfs:label>
        <rdfs:label xml:lang="en">Trade union association</rdfs:label>
    </owl:Class>



    <!-- https://w3id.org/italia/social-security/onto/socialSafetyNet/AttivitàAgricola -->

    <owl:Class rdf:about="https://w3id.org/italia/social-security/onto/socialSafetyNet/AttivitàAgricola">
        <rdfs:subClassOf>
            <owl:Class>
                <owl:oneOf rdf:parseType="Collection">
                    <rdf:Description rdf:about="https://w3id.org/italia/controlled-vocabulary/classifications-for-organizations/ateco-2007/A"/>
                </owl:oneOf>
            </owl:Class>
        </rdfs:subClassOf>
        <rdfs:comment xml:lang="it">Insieme di codici ATECO (ATtività ECOnomica) attinenti alle attività agricole ovvero: coltivazione del fondo; selvicoltura (impianto e coltivazione di boschi, foreste o selve); allevamento di animali (non solo da bestiame); attività connesse (ad esempio, manipolazione e commercializzazione di prodotti, agriturismo). </rdfs:comment>
        <rdfs:comment xml:lang="en">Set of ATECO codes (economic activity) pertaining to agricultural activities, namely: cultivation of the land; silviculture (planting and cultivation of woods, forests or woods); animal husbandry (not only livestock); related activities (e.g. handling and marketing of products, agritourism).</rdfs:comment>
        <rdfs:label xml:lang="en">Agricultural activity</rdfs:label>
        <rdfs:label xml:lang="it">Attività agricola</rdfs:label>
    </owl:Class>



    <!-- https://w3id.org/italia/social-security/onto/socialSafetyNet/AttivitàCorrente -->

    <owl:Class rdf:about="https://w3id.org/italia/social-security/onto/socialSafetyNet/AttivitàCorrente">
        <rdfs:subClassOf>
            <owl:Restriction>
                <owl:onProperty rdf:resource="https://w3id.org/italia/social-security/onto/socialSafetyNet/haTipoAttivitàCorrente"/>
                <owl:someValuesFrom rdf:resource="http://www.w3.org/2002/07/owl#Thing"/>
            </owl:Restriction>
        </rdfs:subClassOf>
        <rdfs:subClassOf>
            <owl:Restriction>
                <owl:onProperty>
                    <rdf:Description>
                        <owl:inverseOf rdf:resource="https://w3id.org/italia/social-security/onto/socialSafetyNet/haAttivitàCorrente"/>
                    </rdf:Description>
                </owl:onProperty>
                <owl:someValuesFrom rdf:resource="http://www.w3.org/2002/07/owl#Thing"/>
            </owl:Restriction>
        </rdfs:subClassOf>
        <rdfs:subClassOf>
            <owl:Restriction>
                <owl:onProperty rdf:resource="https://w3id.org/italia/social-security/onto/socialSafetyNet/dataInizioAttivitàCorrente"/>
                <owl:someValuesFrom rdf:resource="http://www.w3.org/2000/01/rdf-schema#Literal"/>
            </owl:Restriction>
        </rdfs:subClassOf>
        <rdfs:subClassOf>
            <owl:Restriction>
                <owl:onProperty rdf:resource="https://w3id.org/italia/social-security/onto/socialSafetyNet/redditoPrevistoAttivitàCorrente"/>
                <owl:someValuesFrom rdf:resource="http://www.w3.org/2000/01/rdf-schema#Literal"/>
            </owl:Restriction>
        </rdfs:subClassOf>
        <rdfs:comment xml:lang="en">Activities that a NASpI Applicant carries out in conjunction with the submission of the NASpI Application. The expected income of this activity in the year must be declared, which may not coincide with that produced by the existing work relationships. </rdfs:comment>
        <rdfs:comment xml:lang="it">Attività che un Richiedente NASpI svolge in concomitanza con la presentazione della Domanda NASpI. Di questa attività deve essere dichiarato il reddito previsto nell&apos;anno che potrebbe non coincidere non quello prodotto dai rapporti di lavoro in essere. </rdfs:comment>
        <rdfs:label xml:lang="it">Attività Corrente</rdfs:label>
        <rdfs:label xml:lang="en">Current Activity</rdfs:label>
    </owl:Class>



    <!-- https://w3id.org/italia/social-security/onto/socialSafetyNet/Atto -->

    <owl:Class rdf:about="https://w3id.org/italia/social-security/onto/socialSafetyNet/Atto">
        <rdfs:comment xml:lang="en">Manifestation of determination of will or judgment capable of producing legal consequences. It has a date of issue and therefore of validity and an identifier assigned by the subject who issued it or who receives. Having legal value, it is typically produced in written form.</rdfs:comment>
        <rdfs:comment xml:lang="it">Manifestazione di una determinazione di volontà o di giudizio in grado di produrre conseguenze giuridiche. Ha una data di emissione e quindi di validità e un identificatore assegnato dal soggetto che lo ha emesso o che lo riceve. Avendo valore giuridico è tipicamente prodotto in forma scritta.</rdfs:comment>
        <rdfs:label xml:lang="it">Atto</rdfs:label>
        <rdfs:label xml:lang="en">Deed</rdfs:label>
    </owl:Class>



    <!-- https://w3id.org/italia/social-security/onto/socialSafetyNet/AttoDiCertificazioneDiBeneficiarioNASpI -->

    <owl:Class rdf:about="https://w3id.org/italia/social-security/onto/socialSafetyNet/AttoDiCertificazioneDiBeneficiarioNASpI">
        <rdfs:subClassOf rdf:resource="https://w3id.org/italia/social-security/onto/socialSafetyNet/Atto"/>
        <rdfs:subClassOf>
            <owl:Restriction>
                <owl:onProperty rdf:resource="https://w3id.org/italia/social-security/onto/socialSafetyNet/dataSospensioneAccordoCPI"/>
                <owl:someValuesFrom rdf:resource="http://www.w3.org/2000/01/rdf-schema#Literal"/>
            </owl:Restriction>
        </rdfs:subClassOf>
        <rdfs:comment xml:lang="en">Deed subclass, called PD U2, which certifies the condition of NASpI Beneficiary.</rdfs:comment>
        <rdfs:comment xml:lang="it">Sottoclasse di Atto, denominato PD U2, che attesta la condizione di Beneficiario NASpI.</rdfs:comment>
        <rdfs:label xml:lang="it">Atto di certificazione di Beneficiario NASpI</rdfs:label>
        <rdfs:label xml:lang="en">NASpI beneficiary certification deed</rdfs:label>
    </owl:Class>



    <!-- https://w3id.org/italia/social-security/onto/socialSafetyNet/AttoDiCertificazioneLavoroEstero -->

    <owl:Class rdf:about="https://w3id.org/italia/social-security/onto/socialSafetyNet/AttoDiCertificazioneLavoroEstero">
        <rdfs:subClassOf rdf:resource="https://w3id.org/italia/social-security/onto/socialSafetyNet/Atto"/>
        <rdfs:comment xml:lang="en">Deed subclass, called PD U1, which concerns the certification of periods of insurance and/or employment issued by the competent institution of the State in which the person has carried out a work activity. In the case of a Worker residing in Italy who submits an application for NASpI having worked in a foreign country (EU or in agreement), this document must be issued by the competent foreign institution (with reversed parties, it must be issued by INPS at the request of the interested party).</rdfs:comment>
        <rdfs:comment xml:lang="it">Sottoclasse di Atto, denominato PD U1, che riguarda l&apos;attestazione dei periodi di assicurazione e/o occupazione rilasciato dall’Istituzione competente dello Stato in cui la persona ha svolto una attività lavorativa. Nel caso del Lavoratore residente in Italia che presenta domanda di NASpI avendo svolto attività lavorativa in un paese estero (comunitario o in accordo), tale atto deve essere rilasciato dalla competente istituzione estera (a parti invertite, dovrà essere rilasciato dall&apos;INPS su richiesta dell&apos;interessato).</rdfs:comment>
        <rdfs:label xml:lang="it">Atto di certificazione lavoro estero</rdfs:label>
        <rdfs:label xml:lang="en">Foreign work certification deed</rdfs:label>
    </owl:Class>



    <!-- https://w3id.org/italia/social-security/onto/socialSafetyNet/AttoDiCessazioneRapportoDiLavoro -->

    <owl:Class rdf:about="https://w3id.org/italia/social-security/onto/socialSafetyNet/AttoDiCessazioneRapportoDiLavoro">
        <rdfs:subClassOf rdf:resource="https://w3id.org/italia/social-security/onto/socialSafetyNet/Atto"/>
        <rdfs:subClassOf>
            <owl:Restriction>
                <owl:onProperty rdf:resource="https://w3id.org/italia/social-security/onto/socialSafetyNet/haMotivoCessazioneRapportoDiLavoro"/>
                <owl:someValuesFrom rdf:resource="http://www.w3.org/2002/07/owl#Thing"/>
            </owl:Restriction>
        </rdfs:subClassOf>
        <rdfs:subClassOf>
            <owl:Restriction>
                <owl:onProperty>
                    <rdf:Description>
                        <owl:inverseOf rdf:resource="https://w3id.org/italia/social-security/onto/socialSafetyNet/haAttoDiCessazioneRapportoDiLavoro"/>
                    </rdf:Description>
                </owl:onProperty>
                <owl:someValuesFrom rdf:resource="http://www.w3.org/2002/07/owl#Thing"/>
            </owl:Restriction>
        </rdfs:subClassOf>
        <rdfs:subClassOf>
            <owl:Restriction>
                <owl:onProperty rdf:resource="https://w3id.org/italia/social-security/onto/socialSafetyNet/dataCessazioneRapportoDiLavoro"/>
                <owl:someValuesFrom rdf:resource="http://www.w3.org/2000/01/rdf-schema#Literal"/>
            </owl:Restriction>
        </rdfs:subClassOf>
        <rdfs:comment xml:lang="en">Deed subclass concerning the termination of a Work relationship. The issuance of the deed is within the power of both parties involved in the relationship.</rdfs:comment>
        <rdfs:comment xml:lang="it">Sottoclasse di Atto riguardante la terminazione di un rapporto di lavoro. L&apos;emissione dell&apos;atto è nella facoltà di entrambe le parti coinvolte nel rapporto.</rdfs:comment>
        <rdfs:label xml:lang="it">Atto di cessazione rapporto di lavoro</rdfs:label>
        <rdfs:label xml:lang="en">Employment termination deed</rdfs:label>
    </owl:Class>



    <!-- https://w3id.org/italia/social-security/onto/socialSafetyNet/AttoDiDecadenzaNASpI -->

    <owl:Class rdf:about="https://w3id.org/italia/social-security/onto/socialSafetyNet/AttoDiDecadenzaNASpI">
        <rdfs:subClassOf rdf:resource="https://w3id.org/italia/social-security/onto/socialSafetyNet/Atto"/>
        <rdfs:subClassOf>
            <owl:Restriction>
                <owl:onProperty rdf:resource="https://w3id.org/italia/social-security/onto/socialSafetyNet/generaDecadenzaNASpI"/>
                <owl:someValuesFrom rdf:resource="http://www.w3.org/2002/07/owl#Thing"/>
            </owl:Restriction>
        </rdfs:subClassOf>
        <rdfs:subClassOf>
            <owl:Restriction>
                <owl:onProperty rdf:resource="https://w3id.org/italia/social-security/onto/socialSafetyNet/haMotivoDecadenzaNASpI"/>
                <owl:someValuesFrom rdf:resource="http://www.w3.org/2002/07/owl#Thing"/>
            </owl:Restriction>
        </rdfs:subClassOf>
        <rdfs:subClassOf>
            <owl:Restriction>
                <owl:onProperty rdf:resource="https://w3id.org/italia/social-security/onto/socialSafetyNet/dataDecadenzaNASpI"/>
                <owl:someValuesFrom rdf:resource="http://www.w3.org/2000/01/rdf-schema#Literal"/>
            </owl:Restriction>
        </rdfs:subClassOf>
        <rdfs:comment xml:lang="en">Deed subclass concerning the forfeiture of the right to the NASpI benefit.</rdfs:comment>
        <rdfs:comment xml:lang="it">Sottoclasse di Atto riguardante la decadenza del diritto alla Prestazione NASpI.</rdfs:comment>
        <rdfs:label xml:lang="it">Atto di decadenza NASpI</rdfs:label>
        <rdfs:label xml:lang="en">NASpI forfeiture deed</rdfs:label>
    </owl:Class>



    <!-- https://w3id.org/italia/social-security/onto/socialSafetyNet/AttoDiDecadenzaStatoDiDisoccupazione -->

    <owl:Class rdf:about="https://w3id.org/italia/social-security/onto/socialSafetyNet/AttoDiDecadenzaStatoDiDisoccupazione">
        <rdfs:subClassOf rdf:resource="https://w3id.org/italia/social-security/onto/socialSafetyNet/Atto"/>
        <rdfs:subClassOf>
            <owl:Restriction>
                <owl:onProperty rdf:resource="https://w3id.org/italia/social-security/onto/socialSafetyNet/haMotivoDecadenzaDisoccupazione"/>
                <owl:someValuesFrom rdf:resource="http://www.w3.org/2002/07/owl#Thing"/>
            </owl:Restriction>
        </rdfs:subClassOf>
        <rdfs:subClassOf>
            <owl:Restriction>
                <owl:onProperty rdf:resource="https://w3id.org/italia/social-security/onto/socialSafetyNet/revocaStatoDiDisoccupazione"/>
                <owl:someValuesFrom rdf:resource="http://www.w3.org/2002/07/owl#Thing"/>
            </owl:Restriction>
        </rdfs:subClassOf>
        <rdfs:subClassOf>
            <owl:Restriction>
                <owl:onProperty>
                    <rdf:Description>
                        <owl:inverseOf rdf:resource="https://w3id.org/italia/social-security/onto/socialSafetyNet/emetteAttoDiDecadenzaDisoccupazione"/>
                    </rdf:Description>
                </owl:onProperty>
                <owl:someValuesFrom rdf:resource="http://www.w3.org/2002/07/owl#Thing"/>
            </owl:Restriction>
        </rdfs:subClassOf>
        <rdfs:subClassOf>
            <owl:Restriction>
                <owl:onProperty rdf:resource="https://w3id.org/italia/social-security/onto/socialSafetyNet/dataDecadenzaDisoccupazione"/>
                <owl:someValuesFrom rdf:resource="http://www.w3.org/2000/01/rdf-schema#Literal"/>
            </owl:Restriction>
        </rdfs:subClassOf>
        <rdfs:comment xml:lang="en">Deed subclass concerning the revocation of a Worker&apos;s Unemployment status. The issuance of such a deed by the CPI has the consequence, among other things, of the interruption of any subsidy linked to it and the recovery of the sums already paid from the date of revocation indicated in the deed.</rdfs:comment>
        <rdfs:comment xml:lang="it">Sottoclasse di Atto riguardante la revoca dello Stato di disoccupazione di un Lavoratore. L&apos;emissione di tale atto da parte del CPI ha come conseguenza, tra le altre, l&apos;interruzione dell&apos;eventuale sussidio ad esso collegato e il recupero delle somme già erogate dalla data di revoca indicata nell&apos;atto.</rdfs:comment>
        <rdfs:label xml:lang="it">Atto di decadenza stato di disoccupazione</rdfs:label>
        <rdfs:label xml:lang="en">Unemployment status forfeiture deed</rdfs:label>
    </owl:Class>



    <!-- https://w3id.org/italia/social-security/onto/socialSafetyNet/AttoDiNotificaEventoInEspatrio -->

    <owl:Class rdf:about="https://w3id.org/italia/social-security/onto/socialSafetyNet/AttoDiNotificaEventoInEspatrio">
        <rdfs:subClassOf rdf:resource="https://w3id.org/italia/social-security/onto/socialSafetyNet/Atto"/>
        <rdfs:subClassOf>
            <owl:Restriction>
                <owl:onProperty>
                    <rdf:Description>
                        <owl:inverseOf rdf:resource="https://w3id.org/italia/social-security/onto/socialSafetyNet/haComunicazioneEventiInEspatrio"/>
                    </rdf:Description>
                </owl:onProperty>
                <owl:someValuesFrom rdf:resource="http://www.w3.org/2002/07/owl#Thing"/>
            </owl:Restriction>
        </rdfs:subClassOf>
        <rdfs:comment xml:lang="en">Deed subclass concerning the notification of facts that occurred during the period of expatriation of a NASpI Beneficiary and that were communicated by the institution of the State to which the beneficiary went (PAPER SED U010). Such facts may change the NASpI benefit status.</rdfs:comment>
        <rdfs:comment xml:lang="it">Sottoclasse di Atto riguardante la notifica di fatti che si sono verificati durante il periodo di espatrio di un Beneficiario NASpI e che sono stati comunicati con il PAPER SED U010 dall’istituzione dello Stato in cui il beneficiario si è recato. Tali fatti possono modificare lo Stato di prestazione NASpI.</rdfs:comment>
        <rdfs:label xml:lang="it">Atto di notifica evento in espatrio</rdfs:label>
        <rdfs:label xml:lang="en">Expatriation event notification deed</rdfs:label>
    </owl:Class>



    <!-- https://w3id.org/italia/social-security/onto/socialSafetyNet/AttoDiNotificaViolazioneObblighiAttivazione -->

    <owl:Class rdf:about="https://w3id.org/italia/social-security/onto/socialSafetyNet/AttoDiNotificaViolazioneObblighiAttivazione">
        <rdfs:subClassOf rdf:resource="https://w3id.org/italia/social-security/onto/socialSafetyNet/Atto"/>
        <rdfs:subClassOf>
            <owl:Restriction>
                <owl:onProperty>
                    <rdf:Description>
                        <owl:inverseOf rdf:resource="https://w3id.org/italia/social-security/onto/socialSafetyNet/emetteAttoDiNotificaViolazione"/>
                    </rdf:Description>
                </owl:onProperty>
                <owl:someValuesFrom rdf:resource="http://www.w3.org/2002/07/owl#Thing"/>
            </owl:Restriction>
        </rdfs:subClassOf>
        <rdfs:subClassOf>
            <owl:Restriction>
                <owl:onProperty rdf:resource="https://w3id.org/italia/social-security/onto/socialSafetyNet/dataAvvenutaViolazioneAttivazione"/>
                <owl:someValuesFrom rdf:resource="http://www.w3.org/2000/01/rdf-schema#Literal"/>
            </owl:Restriction>
        </rdfs:subClassOf>
        <rdfs:label xml:lang="en">Activations obligations breach notification deed</rdfs:label>
        <rdfs:label xml:lang="it">Atto di notifica violazione obblighi attivazione</rdfs:label>
    </owl:Class>



    <!-- https://w3id.org/italia/social-security/onto/socialSafetyNet/AttoDiRicorsoDomandaNASpI -->

    <owl:Class rdf:about="https://w3id.org/italia/social-security/onto/socialSafetyNet/AttoDiRicorsoDomandaNASpI">
        <rdfs:comment xml:lang="en">Deed subclass concerning the request for appeal of a NASpI claim refused due to lack of requirements by the NASpI Applicant. The document must be submitted online through the appropriate submission channels.</rdfs:comment>
        <rdfs:comment xml:lang="it">Sottoclasse di Atto riguardante la richiesta di ricorso di una Domanda NASpI rifiutata per mancanza di requisiti da parte del Richiedente NASpI. L&apos;atto dovrà essere presentato on-line tramite i predisposti canali di inoltro.</rdfs:comment>
        <rdfs:label xml:lang="it">Atto di ricorso domanda NASpI</rdfs:label>
        <rdfs:label xml:lang="en">NASpI claim appeal deed</rdfs:label>
    </owl:Class>



    <!-- https://w3id.org/italia/social-security/onto/socialSafetyNet/AttoDiRiesameDomandaNASpI -->

    <owl:Class rdf:about="https://w3id.org/italia/social-security/onto/socialSafetyNet/AttoDiRiesameDomandaNASpI">
        <rdfs:comment xml:lang="en">Deed subclass concerning the request for review of a NASpI claim refused for lack of mandatory information. The document can be sent via PEC or submitted in person.</rdfs:comment>
        <rdfs:comment xml:lang="it">Sottoclasse di Atto riguardante la richiesta di riesame di una Domanda NASpI rifiutata per mancanza di informazioni obbligatorie. L&apos;atto potrà essere inviato via PEC o presentato di persona.</rdfs:comment>
        <rdfs:label xml:lang="it">Atto di riesame domanda NASpI</rdfs:label>
        <rdfs:label xml:lang="en">NASpI claim review deed</rdfs:label>
    </owl:Class>



    <!-- https://w3id.org/italia/social-security/onto/socialSafetyNet/AttoDiRinunciaAllaNASpI -->

    <owl:Class rdf:about="https://w3id.org/italia/social-security/onto/socialSafetyNet/AttoDiRinunciaAllaNASpI">
        <rdfs:subClassOf rdf:resource="https://w3id.org/italia/social-security/onto/socialSafetyNet/Atto"/>
        <rdfs:subClassOf>
            <owl:Restriction>
                <owl:onProperty rdf:resource="https://w3id.org/italia/social-security/onto/socialSafetyNet/haMotivoDiRinunciaNASpI"/>
                <owl:someValuesFrom rdf:resource="http://www.w3.org/2002/07/owl#Thing"/>
            </owl:Restriction>
        </rdfs:subClassOf>
        <rdfs:comment xml:lang="en">Deed subclass concerning the waiver of the NASpI Benefit by an already beneficiary. Failure to do so will result in the forfeiture of the benefit.</rdfs:comment>
        <rdfs:comment xml:lang="it">Sottoclasse di Atto riguardante la rinuncia della Prestazione NASpI da parte di un già beneficiario. La rinuncia comporta il decadimento della prestazione.</rdfs:comment>
        <rdfs:label xml:lang="it">Atto di rinuncia alla NASpI</rdfs:label>
        <rdfs:label xml:lang="en">NASpI waiver deed</rdfs:label>
    </owl:Class>



    <!-- https://w3id.org/italia/social-security/onto/socialSafetyNet/BeneficiarioDIS-COLL -->

    <owl:Class rdf:about="https://w3id.org/italia/social-security/onto/socialSafetyNet/BeneficiarioDIS-COLL">
        <rdfs:subClassOf rdf:resource="https://w3id.org/italia/social-security/onto/socialSafetyNet/BeneficiarioPrestazioneDiSostegnoAlReddito"/>
        <rdfs:subClassOf>
            <owl:Restriction>
                <owl:onProperty>
                    <rdf:Description>
                        <owl:inverseOf rdf:resource="https://w3id.org/italia/social-security/onto/socialSafetyNet/haBeneficiarioPrestazioneDiSostegnoAlReddito"/>
                    </rdf:Description>
                </owl:onProperty>
                <owl:someValuesFrom rdf:resource="https://w3id.org/italia/social-security/onto/socialSafetyNet/PrestazioneDIS-COLL"/>
            </owl:Restriction>
        </rdfs:subClassOf>
        <rdfs:comment xml:lang="en">Role of Income support subsidy beneficiary concerning beneficiaries of DIS-COLL benefit.</rdfs:comment>
        <rdfs:comment xml:lang="it">Ruolo di Beneficiario prestazione di sostegno al reddito riguardante i beneficiari di Prestazione DIS-COLL.</rdfs:comment>
        <rdfs:label xml:lang="it">Beneficiario DIS-COLL</rdfs:label>
        <rdfs:label xml:lang="en">DIS-COLL Beneficiary</rdfs:label>
    </owl:Class>



    <!-- https://w3id.org/italia/social-security/onto/socialSafetyNet/BeneficiarioDetrazioneFiscalePerCarichiFamiliari -->

    <owl:Class rdf:about="https://w3id.org/italia/social-security/onto/socialSafetyNet/BeneficiarioDetrazioneFiscalePerCarichiFamiliari">
        <rdfs:subClassOf rdf:resource="https://w3id.org/italia/social-security/onto/socialSafetyNet/BeneficiarioPrestazioneDiSostegnoAlReddito"/>
        <rdfs:subClassOf>
            <owl:Restriction>
                <owl:onProperty>
                    <rdf:Description>
                        <owl:inverseOf rdf:resource="https://w3id.org/italia/social-security/onto/socialSafetyNet/haBeneficiarioPrestazioneDiSostegnoAlReddito"/>
                    </rdf:Description>
                </owl:onProperty>
                <owl:someValuesFrom rdf:resource="https://w3id.org/italia/social-security/onto/socialSafetyNet/DetrazioneFiscalePerCarichiFamigliari"/>
            </owl:Restriction>
        </rdfs:subClassOf>
        <rdfs:comment xml:lang="en">Role of Income support subsidy beneficiary concerning beneficiaries of Family expenses tax deduction benefit.</rdfs:comment>
        <rdfs:comment xml:lang="it">Ruolo di Beneficiario prestazione di sostegno al reddito riguardante i beneficiari di Detrazione fiscale per carichi familiari.</rdfs:comment>
        <rdfs:label xml:lang="it">Beneficiario detrazione fiscale per carichi familiari</rdfs:label>
        <rdfs:label xml:lang="en">Family expenses tax deduction beneficiary</rdfs:label>
    </owl:Class>



    <!-- https://w3id.org/italia/social-security/onto/socialSafetyNet/BeneficiarioNASpI -->

    <owl:Class rdf:about="https://w3id.org/italia/social-security/onto/socialSafetyNet/BeneficiarioNASpI">
        <rdfs:subClassOf rdf:resource="https://w3id.org/italia/social-security/onto/socialSafetyNet/BeneficiarioPrestazioneDiSostegnoAlReddito"/>
        <rdfs:subClassOf>
            <owl:Class>
                <owl:unionOf rdf:parseType="Collection">
                    <rdf:Description rdf:about="https://w3id.org/italia/social-security/onto/contributions/LavoratoreDomestico"/>
                    <owl:Class>
                        <owl:intersectionOf rdf:parseType="Collection">
                            <rdf:Description rdf:about="https://w3id.org/italia/social-security/onto/socialSafetyNet/DipendentePrivato"/>
                            <owl:Class>
                                <owl:complementOf rdf:resource="https://w3id.org/italia/social-security/onto/socialSafetyNet/LavoratoreSubordinatoAgricolo"/>
                            </owl:Class>
                        </owl:intersectionOf>
                    </owl:Class>
                    <owl:Class>
                        <owl:intersectionOf rdf:parseType="Collection">
                            <rdf:Description rdf:about="https://w3id.org/italia/social-security/onto/socialSafetyNet/DipendentePubblico"/>
                            <owl:Class>
                                <owl:complementOf rdf:resource="https://w3id.org/italia/social-security/onto/socialSafetyNet/LavoratoreSubordinatoAgricolo"/>
                            </owl:Class>
                            <owl:Restriction>
                                <owl:onProperty rdf:resource="https://w3id.org/italia/social-security/onto/socialSafetyNet/accettaContrattoDiLavoro"/>
                                <owl:someValuesFrom rdf:resource="https://w3id.org/italia/social-security/onto/socialSafetyNet/ContrattoATempoDeterminato"/>
                            </owl:Restriction>
                        </owl:intersectionOf>
                    </owl:Class>
                </owl:unionOf>
            </owl:Class>
        </rdfs:subClassOf>
        <rdfs:subClassOf>
            <owl:Restriction>
                <owl:onProperty rdf:resource="https://w3id.org/italia/social-security/onto/socialSafetyNet/haStatoDiLavoro"/>
                <owl:someValuesFrom rdf:resource="https://w3id.org/italia/social-security/onto/socialSafetyNet/StatoDiDisoccupazioneInvolontaria"/>
            </owl:Restriction>
        </rdfs:subClassOf>
        <rdfs:subClassOf>
            <owl:Restriction>
                <owl:onProperty>
                    <rdf:Description>
                        <owl:inverseOf rdf:resource="https://w3id.org/italia/social-security/onto/socialSafetyNet/haBeneficiarioPrestazioneDiSostegnoAlReddito"/>
                    </rdf:Description>
                </owl:onProperty>
                <owl:someValuesFrom rdf:resource="https://w3id.org/italia/social-security/onto/socialSafetyNet/PrestazioneNASpI"/>
            </owl:Restriction>
        </rdfs:subClassOf>
        <rdfs:comment xml:lang="en">Role of Income support subsidy beneficiary concerning beneficiaries of NASpI benefit.</rdfs:comment>
        <rdfs:comment xml:lang="it">Ruolo di Beneficiario prestazione di sostegno al reddito riguardante i beneficiari di Prestazione NASpI.</rdfs:comment>
        <rdfs:label xml:lang="it">Beneficiario NASpI</rdfs:label>
        <rdfs:label xml:lang="en">NASpI beneficiary</rdfs:label>
    </owl:Class>



    <!-- https://w3id.org/italia/social-security/onto/socialSafetyNet/BeneficiarioPrestazioneANF -->

    <owl:Class rdf:about="https://w3id.org/italia/social-security/onto/socialSafetyNet/BeneficiarioPrestazioneANF">
        <rdfs:subClassOf rdf:resource="https://w3id.org/italia/social-security/onto/socialSafetyNet/BeneficiarioPrestazioneDiSostegnoAlReddito"/>
        <rdfs:subClassOf>
            <owl:Restriction>
                <owl:onProperty>
                    <rdf:Description>
                        <owl:inverseOf rdf:resource="https://w3id.org/italia/social-security/onto/socialSafetyNet/haBeneficiarioPrestazioneDiSostegnoAlReddito"/>
                    </rdf:Description>
                </owl:onProperty>
                <owl:someValuesFrom rdf:resource="https://w3id.org/italia/social-security/onto/socialSafetyNet/PrestazioneANF"/>
            </owl:Restriction>
        </rdfs:subClassOf>
        <rdfs:comment xml:lang="en">Role of Income support subsidy beneficiary concerning beneficiaries of ANF benefit.</rdfs:comment>
        <rdfs:comment xml:lang="it">Ruolo di Beneficiario prestazione di sostegno al reddito riguardante i beneficiari di Prestazione ANF.</rdfs:comment>
        <rdfs:label xml:lang="en">ANF beneficiary</rdfs:label>
        <rdfs:label xml:lang="it">Beneficiario prestazione ANF</rdfs:label>
    </owl:Class>



    <!-- https://w3id.org/italia/social-security/onto/socialSafetyNet/BeneficiarioPrestazioneDiSostegnoAlReddito -->

    <owl:Class rdf:about="https://w3id.org/italia/social-security/onto/socialSafetyNet/BeneficiarioPrestazioneDiSostegnoAlReddito">
        <rdfs:subClassOf rdf:resource="https://w3id.org/italia/social-security/onto/core/RuoloDiPersonaViva"/>
        <rdfs:subClassOf>
            <owl:Restriction>
                <owl:onProperty>
                    <rdf:Description>
                        <owl:inverseOf rdf:resource="https://w3id.org/italia/social-security/onto/socialSafetyNet/haBeneficiarioPrestazioneDiSostegnoAlReddito"/>
                    </rdf:Description>
                </owl:onProperty>
                <owl:someValuesFrom rdf:resource="http://www.w3.org/2002/07/owl#Thing"/>
            </owl:Restriction>
        </rdfs:subClassOf>
        <rdfs:comment xml:lang="en">Role of Living person attributed to those who benefit from an economic subsidy for health, economic or job-related reasons.</rdfs:comment>
        <rdfs:comment xml:lang="it">Ruolo di Persona viva attribuito a chi beneficia di un sussidio economico per motivi di salute, economiche o legate alla perdita dell’occupazione.</rdfs:comment>
        <rdfs:label xml:lang="it">Beneficiario prestazione di sostegno al reddito</rdfs:label>
        <rdfs:label xml:lang="en">Income support subsidy beneficiary</rdfs:label>
    </owl:Class>



    <!-- https://w3id.org/italia/social-security/onto/socialSafetyNet/CentroPerLImpiego -->

    <owl:Class rdf:about="https://w3id.org/italia/social-security/onto/socialSafetyNet/CentroPerLImpiego">
        <rdfs:subClassOf rdf:resource="https://w3id.org/italia/social-security/onto/socialSafetyNet/UfficioDelLavoro"/>
        <owl:disjointWith rdf:resource="https://w3id.org/italia/social-security/onto/socialSafetyNet/UfficioDelLavoroEstero"/>
        <rdfs:comment xml:lang="en">Labour office subclass belonging to the of the Italian Public Administration, of regional and/or provincial competence, which is entrusted with the function of implementing public policies on labour and providing services to facilitate the relocation of workers in Unemployment status or First-time jobseeker status through the stipulation of a Personalized Service Agreement (PSP) or a specific path of accompaniment to job placement that provides for the preparation of the balance of skills and activities aimed at active job search and vocational training or retraining.</rdfs:comment>
        <rdfs:comment xml:lang="it">Sottoclasse di Ufficio del lavoro appartenente alla Pubblica Amministrazione italiana, di competenza regionale e/o provinciale, a cui è demandata la funzione di attuare politiche pubbliche in materia di lavoro ed erogare servizi per favorire la ricollocazione di lavoratori in Stato di disoccupazione o inoccupazione tramite la stipula di un Patto di Servizio Personalizzato (PSP) ovvero di un percorso specifico di accompagnamento all&apos;inserimento lavorativo che prevede la redazione del bilancio delle competenze e attività finalizzate alla ricerca attiva di lavoro e alla formazione o riqualificazione professionale.</rdfs:comment>
        <rdfs:label xml:lang="it">Centro per l&apos;impiego</rdfs:label>
        <rdfs:label xml:lang="en">Employment centre</rdfs:label>
    </owl:Class>



    <!-- https://w3id.org/italia/social-security/onto/socialSafetyNet/CollaborazioneCoordinataEContinuativa -->

    <owl:Class rdf:about="https://w3id.org/italia/social-security/onto/socialSafetyNet/CollaborazioneCoordinataEContinuativa">
        <rdfs:subClassOf rdf:resource="https://w3id.org/italia/social-security/onto/socialSafetyNet/ContrattoDiLavoro"/>
        <rdfs:comment xml:lang="it">Sottoclasse di Contratto di lavoro che prevede l&apos;erogazione della prestazione lavorativa in autonomia da parte del Lavoratore e senza vincolo di subordinazione ma eseguita nell&apos;ambito di un rapporto unitario e continuativo con il Datore di Lavoro, non legato a vincoli di progetto/programma o di risultato o di tempo. È la tipica forma di lavoro parasubordinato.</rdfs:comment>
        <rdfs:comment xml:lang="en">Work contract subclass that provides for the provision of work independently by the Worker and without subordination constraint but carried out within a unitary and continuous relationship with the Employer, not linked to project/program or result or time constraints. It is the typical form of parasubordinate work.</rdfs:comment>
        <rdfs:label xml:lang="it">Collaborazione coordinata e continuativa</rdfs:label>
        <rdfs:label xml:lang="en">Coordinated and continuous collaboration</rdfs:label>
    </owl:Class>



    <!-- https://w3id.org/italia/social-security/onto/socialSafetyNet/CommittenteDOpera -->

    <owl:Class rdf:about="https://w3id.org/italia/social-security/onto/socialSafetyNet/CommittenteDOpera">
        <rdfs:subClassOf rdf:resource="https://w3id.org/italia/social-security/onto/socialSafetyNet/TitolareDelRapportoDiLavoro"/>
        <rdfs:subClassOf>
            <owl:Restriction>
                <owl:onProperty rdf:resource="https://w3id.org/italia/social-security/onto/socialSafetyNet/proponeContrattoDiLavoro"/>
                <owl:someValuesFrom rdf:resource="https://w3id.org/italia/social-security/onto/socialSafetyNet/ContrattoDOpera"/>
            </owl:Restriction>
        </rdfs:subClassOf>
        <owl:disjointWith rdf:resource="https://w3id.org/italia/social-security/onto/socialSafetyNet/DatoreDiLavoro"/>
        <rdfs:comment xml:lang="it">Sottoclasse di Titolare di rapporto di lavoro relativa a chi sottoscrive un Contratto d&apos;opera.</rdfs:comment>
        <rdfs:comment xml:lang="en">Work relationship rightsholder subclass relating to those who sign a Manufacturing service contract.</rdfs:comment>
        <rdfs:label xml:lang="it">Committente d&apos;opera</rdfs:label>
        <rdfs:label xml:lang="en">Project owner</rdfs:label>
    </owl:Class>



    <!-- https://w3id.org/italia/social-security/onto/socialSafetyNet/ComunicazioneEventoNASpI -->

    <owl:Class rdf:about="https://w3id.org/italia/social-security/onto/socialSafetyNet/ComunicazioneEventoNASpI">
        <rdfs:subClassOf rdf:resource="https://w3id.org/italia/social-security/onto/socialSafetyNet/ComunicazioneNASpI"/>
        <rdfs:subClassOf>
            <owl:Restriction>
                <owl:onProperty rdf:resource="https://w3id.org/italia/social-security/onto/socialSafetyNet/numeroProtocolloNASpI"/>
                <owl:someValuesFrom rdf:resource="http://www.w3.org/2000/01/rdf-schema#Literal"/>
            </owl:Restriction>
        </rdfs:subClassOf>
        <rdfs:comment xml:lang="en">NASpI Communication subclass concerning events that affect the payment of the benefit.</rdfs:comment>
        <rdfs:comment xml:lang="it">Sottoclasse di Comunicazione NASpI riguardante gli eventi che influiscono sul pagamento della prestazione.</rdfs:comment>
        <rdfs:label xml:lang="it">Comunicazione evento NASpI</rdfs:label>
        <rdfs:label xml:lang="en">NASpI event communication</rdfs:label>
    </owl:Class>



    <!-- https://w3id.org/italia/social-security/onto/socialSafetyNet/ComunicazioneNASpI -->

    <owl:Class rdf:about="https://w3id.org/italia/social-security/onto/socialSafetyNet/ComunicazioneNASpI">
        <rdfs:subClassOf rdf:resource="https://w3id.org/italia/onto/TI/TimeIndexedEvent"/>
        <rdfs:subClassOf>
            <owl:Restriction>
                <owl:onProperty>
                    <rdf:Description>
                        <owl:inverseOf rdf:resource="https://w3id.org/italia/social-security/onto/socialSafetyNet/haComunicazioneNASpI"/>
                    </rdf:Description>
                </owl:onProperty>
                <owl:someValuesFrom rdf:resource="http://www.w3.org/2002/07/owl#Thing"/>
            </owl:Restriction>
        </rdfs:subClassOf>
        <owl:disjointWith rdf:resource="https://w3id.org/italia/social-security/onto/socialSafetyNet/DomandaNASpI"/>
        <rdfs:comment xml:lang="en">Class of events that vary the situation of the NASpI beneficiary and that occur during the provision of a NASpI benefit and that must be compulsorily communicated to INPS. They only affect NASpI benefit in a disbursed or suspended status.</rdfs:comment>
        <rdfs:comment xml:lang="it">Classe degli eventi che variano la situazione del Beneficiario NASpI e che avvengono nel corso dell&apos;erogazione di una prestazione NASpI e che devono essere obbligatoriamente comunicati all&apos;INPS. Riguardano solo Prestazioni NASpI in stato di erogazione o di sospensione.</rdfs:comment>
        <rdfs:label xml:lang="it">Comunicazione NASpI</rdfs:label>
        <rdfs:label xml:lang="en">NASpI communication</rdfs:label>
    </owl:Class>



    <!-- https://w3id.org/italia/social-security/onto/socialSafetyNet/ComunicazioneVariazioneNASpI -->

    <owl:Class rdf:about="https://w3id.org/italia/social-security/onto/socialSafetyNet/ComunicazioneVariazioneNASpI">
        <rdfs:subClassOf rdf:resource="https://w3id.org/italia/social-security/onto/socialSafetyNet/ComunicazioneNASpI"/>
        <rdfs:subClassOf>
            <owl:Restriction>
                <owl:onProperty rdf:resource="https://w3id.org/italia/social-security/onto/socialSafetyNet/numeroProtocolloNASpI"/>
                <owl:someValuesFrom rdf:resource="http://www.w3.org/2000/01/rdf-schema#Literal"/>
            </owl:Restriction>
        </rdfs:subClassOf>
        <rdfs:comment xml:lang="en">NASpI Communication subclass concerning the updating of the data present in the NASpI claim.</rdfs:comment>
        <rdfs:comment xml:lang="it">Sottoclasse di Comunicazione NASpI riguardante l&apos;aggiornamento dei dati presenti nella Domanda NASpI.</rdfs:comment>
        <rdfs:label xml:lang="it">Comunicazione variazione NASpI</rdfs:label>
        <rdfs:label xml:lang="en">NASpI change communication</rdfs:label>
    </owl:Class>



    <!-- https://w3id.org/italia/social-security/onto/socialSafetyNet/ContrattoAProgetto -->

    <owl:Class rdf:about="https://w3id.org/italia/social-security/onto/socialSafetyNet/ContrattoAProgetto">
        <rdfs:subClassOf rdf:resource="https://w3id.org/italia/social-security/onto/socialSafetyNet/CollaborazioneCoordinataEContinuativa"/>
        <rdfs:comment xml:lang="en">Coordinated and continuous collaboration subclass, legally equivalent to it, but limited to the completion of a specific project or program that defines its duration and expected result.</rdfs:comment>
        <rdfs:comment xml:lang="it">Sottoclasse di Collaborazione coordinata e continuativa giuridicamente ad essa equiparata ma circoscritta al compimento di uno specifico progetto o programma che ne definisce la durata e il risultato atteso.</rdfs:comment>
        <rdfs:label xml:lang="it">Contratto a progetto</rdfs:label>
        <rdfs:label xml:lang="en">Project-based contract</rdfs:label>
    </owl:Class>



    <!-- https://w3id.org/italia/social-security/onto/socialSafetyNet/ContrattoATempoDeterminato -->

    <owl:Class rdf:about="https://w3id.org/italia/social-security/onto/socialSafetyNet/ContrattoATempoDeterminato">
        <rdfs:subClassOf rdf:resource="https://w3id.org/italia/social-security/onto/socialSafetyNet/ContrattoDiLavoroSubordinato"/>
        <owl:disjointWith rdf:resource="https://w3id.org/italia/social-security/onto/socialSafetyNet/ContrattoATempoIndeterminato"/>
        <rdfs:comment xml:lang="en">Salaried employment contract subclass that includes contracts that provide for a predetermined duration, through the affixing of a term. The maximum duration of the contract is currently set at 12 months, with the possibility of extension to 24 months, but only under special conditions.</rdfs:comment>
        <rdfs:comment xml:lang="it">Sottoclasse di Contratto di lavoro subordinato che raccoglie i contratti che prevedono una durata predeterminata, mediante l’apposizione di un termine. La durata massima del contratto è attualmente fissata in 12 mesi, con possibilità di estensione a 24 mesi, ma solo al ricorrere particolari condizioni.</rdfs:comment>
        <rdfs:label xml:lang="it">Contratto a tempo determinato</rdfs:label>
        <rdfs:label xml:lang="en">Fixed-term contract</rdfs:label>
    </owl:Class>



    <!-- https://w3id.org/italia/social-security/onto/socialSafetyNet/ContrattoATempoIndeterminato -->

    <owl:Class rdf:about="https://w3id.org/italia/social-security/onto/socialSafetyNet/ContrattoATempoIndeterminato">
        <rdfs:subClassOf rdf:resource="https://w3id.org/italia/social-security/onto/socialSafetyNet/ContrattoDiLavoroSubordinato"/>
        <rdfs:comment xml:lang="en">Salaried employment contract subclass that includes contracts that do not provide for a duration constraint. This is the typical form of the Salaried employment contract.</rdfs:comment>
        <rdfs:comment xml:lang="it">Sottoclasse di Contratto di lavoro subordinato che raccoglie i contratti che non prevedono un vincolo di durata. È la forma tipica del Contratto di lavoro subordinato.</rdfs:comment>
        <rdfs:label xml:lang="it">Contratto a tempo indeterminato</rdfs:label>
        <rdfs:label xml:lang="en">Open-ended contract</rdfs:label>
    </owl:Class>



    <!-- https://w3id.org/italia/social-security/onto/socialSafetyNet/ContrattoDOpera -->

    <owl:Class rdf:about="https://w3id.org/italia/social-security/onto/socialSafetyNet/ContrattoDOpera">
        <rdfs:subClassOf rdf:resource="https://w3id.org/italia/social-security/onto/socialSafetyNet/ContrattoDiLavoro"/>
        <rdfs:comment xml:lang="it">Sottoclasse di Contratto di lavoro in cui una parte si obbliga, a fronte di un corrispettivo, a compiere un&apos;opera o un servizio in favore di un&apos;altra, detta Committente d&apos;opera, con lavoro prevalentemente proprio e senza vincolo di subordinazione. Solitamente è previsto un termine del contratto legato sia al risultato che al tempo per conseguirlo.</rdfs:comment>
        <rdfs:comment xml:lang="en">Work contract subclass in which one party undertakes, in return for consideration, to perform a work or service in favour of another, called the Project owner, with mainly his own work and without subordination. There is usually a term of the contract linked to both the result and the time to achieve it.</rdfs:comment>
        <rdfs:label xml:lang="it">Contratto d&apos;opera</rdfs:label>
        <rdfs:label xml:lang="en">Manufacturing service contract</rdfs:label>
    </owl:Class>



    <!-- https://w3id.org/italia/social-security/onto/socialSafetyNet/ContrattoDOperaProfessionale -->

    <owl:Class rdf:about="https://w3id.org/italia/social-security/onto/socialSafetyNet/ContrattoDOperaProfessionale">
        <rdfs:subClassOf rdf:resource="https://w3id.org/italia/social-security/onto/socialSafetyNet/ContrattoDiLavoro"/>
        <rdfs:comment xml:lang="it">Sottoclasse di Contratto di lavoro in cui una parte si obbliga, a fronte di un corrispettivo, a svolgere una prestazione professionale non manuale volta ad un fine di rilevanza sociale. Tale prestazione non è solitamente legata al raggiungimento di un risultato quanto all&apos;impiego di capacità utili al perseguimento dello scopo del contratto.</rdfs:comment>
        <rdfs:comment xml:lang="en">Work contract subclass in which a party undertakes, in return for consideration, to perform a non-manual professional service aimed at a purpose of social relevance. Such performance is usually not linked to the achievement of a result but to the use of skills useful for the pursuit of the purpose of the contract.</rdfs:comment>
        <rdfs:label xml:lang="it">Contratto d&apos;opera professionale</rdfs:label>
        <rdfs:label xml:lang="en">Professional service contract</rdfs:label>
    </owl:Class>



    <!-- https://w3id.org/italia/social-security/onto/socialSafetyNet/ContrattoDiApprendistato -->

    <owl:Class rdf:about="https://w3id.org/italia/social-security/onto/socialSafetyNet/ContrattoDiApprendistato">
        <rdfs:subClassOf rdf:resource="https://w3id.org/italia/social-security/onto/socialSafetyNet/ContrattoATempoIndeterminato"/>
        <rdfs:comment xml:lang="en">Open-ended contract subclass aimed at the training and employment of young people. It is therefore a mixed-cause contract, i.e. in which, alongside the cause of exchange (work for remuneration) typical of the Salaried employment contract, the educational purpose is placed.</rdfs:comment>
        <rdfs:comment xml:lang="it">Sottoclasse di Contratto a tempo indeterminato finalizzato alla formazione ed all’occupazione dei giovani. È quindi un contratto a causa mista, nel quale cioè accanto alla causa di scambio (lavoro verso retribuzione) tipica del contratto di lavoro subordinato si pone la finalità formativa.</rdfs:comment>
        <rdfs:label xml:lang="en">Apprenticeship agreement</rdfs:label>
        <rdfs:label xml:lang="it">Contratto di apprendistato</rdfs:label>
    </owl:Class>



    <!-- https://w3id.org/italia/social-security/onto/socialSafetyNet/ContrattoDiLavoro -->

    <owl:Class rdf:about="https://w3id.org/italia/social-security/onto/socialSafetyNet/ContrattoDiLavoro">
        <rdfs:subClassOf rdf:resource="https://w3id.org/italia/onto/TI/TimeIndexedEvent"/>
        <rdfs:subClassOf>
            <owl:Restriction>
                <owl:onProperty>
                    <rdf:Description>
                        <owl:inverseOf rdf:resource="https://w3id.org/italia/social-security/onto/socialSafetyNet/accettaContrattoDiLavoro"/>
                    </rdf:Description>
                </owl:onProperty>
                <owl:someValuesFrom rdf:resource="http://www.w3.org/2002/07/owl#Thing"/>
            </owl:Restriction>
        </rdfs:subClassOf>
        <rdfs:subClassOf>
            <owl:Restriction>
                <owl:onProperty>
                    <rdf:Description>
                        <owl:inverseOf rdf:resource="https://w3id.org/italia/social-security/onto/socialSafetyNet/proponeContrattoDiLavoro"/>
                    </rdf:Description>
                </owl:onProperty>
                <owl:someValuesFrom rdf:resource="http://www.w3.org/2002/07/owl#Thing"/>
            </owl:Restriction>
        </rdfs:subClassOf>
        <rdfs:subClassOf>
            <owl:Restriction>
                <owl:onProperty>
                    <rdf:Description>
                        <owl:inverseOf rdf:resource="https://w3id.org/italia/social-security/onto/socialSafetyNet/èRegolatoDaContratto"/>
                    </rdf:Description>
                </owl:onProperty>
                <owl:someValuesFrom rdf:resource="http://www.w3.org/2002/07/owl#Thing"/>
            </owl:Restriction>
        </rdfs:subClassOf>
        <rdfs:comment xml:lang="en">A legal act that gives rise to a work relationship.</rdfs:comment>
        <rdfs:comment xml:lang="it">Atto giuridico che da origine ad un rapporto di lavoro.</rdfs:comment>
        <rdfs:label xml:lang="it">Contratto di lavoro</rdfs:label>
        <rdfs:label xml:lang="en">Work contract</rdfs:label>
    </owl:Class>



    <!-- https://w3id.org/italia/social-security/onto/socialSafetyNet/ContrattoDiLavoroSubordinato -->

    <owl:Class rdf:about="https://w3id.org/italia/social-security/onto/socialSafetyNet/ContrattoDiLavoroSubordinato">
        <rdfs:subClassOf rdf:resource="https://w3id.org/italia/social-security/onto/socialSafetyNet/ContrattoDiLavoro"/>
        <rdfs:comment xml:lang="it">Sottoclasse di Contratto di lavoro che raccoglie i contratti che prevedono giuridicamente il vincolo della subordinazione del Lavoratore rispetto al Titolare del contratto, qui denominato Datore di lavoro. Tale vincolo di subordinazione si esplica nei principi di eterodirezione, ovvero la facoltà del datore di lavoro di impartire ordini e istruzioni al lavoratore, e la dipendenza, ovvero l&apos;alienità del lavoratore rispetto alla finalità della prestazione e alla proprietà del risultato.</rdfs:comment>
        <rdfs:comment xml:lang="en">Work contract subclass that includes contracts that legally provide for the subordination of the Worker to the Contract Holder, hereinafter referred to as the Employer. This bond of subordination is expressed in the principles of heterodirection, i.e. the employer&apos;s right to give orders and instructions to the worker, and dependence, i.e. the alienation of the worker with respect to the purpose of the service and the ownership of the result.</rdfs:comment>
        <rdfs:label xml:lang="it">Contratto di lavoro subordinato</rdfs:label>
        <rdfs:label xml:lang="en">Salaried employment contract</rdfs:label>
    </owl:Class>



    <!-- https://w3id.org/italia/social-security/onto/socialSafetyNet/ContributoAssicurazioneGeneraleObbligatoria -->

    <owl:Class rdf:about="https://w3id.org/italia/social-security/onto/socialSafetyNet/ContributoAssicurazioneGeneraleObbligatoria">
        <rdfs:subClassOf rdf:resource="https://w3id.org/italia/social-security/onto/socialSafetyNet/ContributoObbligatorio"/>
        <rdfs:subClassOf>
            <owl:Restriction>
                <owl:onProperty>
                    <rdf:Description>
                        <owl:inverseOf rdf:resource="https://w3id.org/italia/social-security/onto/socialSafetyNet/haContributoObbligatorio"/>
                    </rdf:Description>
                </owl:onProperty>
                <owl:someValuesFrom rdf:resource="https://w3id.org/italia/social-security/onto/socialSafetyNet/ContrattoDiLavoroSubordinato"/>
            </owl:Restriction>
        </rdfs:subClassOf>
        <rdfs:comment xml:lang="en">Mandatory contribution subclass relating to payments made by workers with a Salaried employment contract.</rdfs:comment>
        <rdfs:comment xml:lang="it">Sottoclasse di Contributo obbligatorio relativo ai versamenti effettuati dai lavoratori con Contratto di lavoro subordinato.</rdfs:comment>
        <rdfs:label xml:lang="it">Contributo assicurazione generale obbligatoria</rdfs:label>
        <rdfs:label xml:lang="en">Mandatory general insurance contribution</rdfs:label>
    </owl:Class>



    <!-- https://w3id.org/italia/social-security/onto/socialSafetyNet/ContributoDaRiscatto -->

    <owl:Class rdf:about="https://w3id.org/italia/social-security/onto/socialSafetyNet/ContributoDaRiscatto">
        <rdfs:subClassOf rdf:resource="https://w3id.org/italia/social-security/onto/socialSafetyNet/ContributoPrevidenziale"/>
        <rdfs:comment xml:lang="en">Social security contribution subclass refers to the portion of contributions that is paid by the employee (with financial burden to be borne by him, borne by the employer or through the transfer of funds from other social security institutions) to regularize, from an insurance point of view, the periods that have not been covered by contributions (such as, for example,  the duration of legal courses of university study). It is to all intents and purposes equivalent to the mandatory one, both in terms of the right and the size of the pension.</rdfs:comment>
        <rdfs:comment xml:lang="it">Sottoclasse di Contributo previdenziale riferito alla quota di contributi che viene versata dal lavoratore (con onere finanziario a suo carico, a carico del datore di lavoro o attraverso il trasferimento di fondi da altri enti di previdenza) per regolarizzare, dal punto di vista assicurativo, i periodi che non siano stati coperti da contribuzione (come ad esempio, il periodo di durata de corsi legali di studio universitario). È a tutti gli effetti equiparata a quella obbligatoria, sia per il diritto che per la misura della pensione.</rdfs:comment>
        <rdfs:label xml:lang="it">Contributo da riscatto</rdfs:label>
        <rdfs:label xml:lang="en">Redemption contribution</rdfs:label>
    </owl:Class>



    <!-- https://w3id.org/italia/social-security/onto/socialSafetyNet/ContributoFigurativo -->

    <owl:Class rdf:about="https://w3id.org/italia/social-security/onto/socialSafetyNet/ContributoFigurativo">
        <rdfs:subClassOf rdf:resource="https://w3id.org/italia/social-security/onto/socialSafetyNet/ContributoPrevidenziale"/>
        <rdfs:comment xml:lang="en">Social security contribution subclass refers to the portion of contributions relating to periods in which the worker did not perform work for reasons not attributable to his or her will. It constitutes a specific protection that allows the worker to also cover periods that would remain without pension insurance due to the suspension or termination of the work relationship. The law exhaustively identifies the cases in which contributions can be credited ex officio or at the request of the person concerned, without this entailing any burden on the worker, such as, for example, military service, periods of wage integration, compulsory and optional abstention from work.</rdfs:comment>
        <rdfs:comment xml:lang="it">Sottoclasse di Contributo previdenziale riferito alla quota di contributi relativi a periodi in cui il lavoratore non ha eseguito la prestazione lavorativa per cause non imputabili alla sua volontà. Essa costituisce una specifica tutela che permette al lavoratore di coprire anche periodi che rimarrebbero senza assicurazione pensionistica a causa della sospensione o cessazione del rapporto di lavoro. La legge individua tassativamente le ipotesi nelle quali i contributi possono essere accreditati d’ufficio o su domanda dell’interessato, senza che ciò comporti alcun onere a carico del lavoratore come, ad esempio, il servizio militare, i periodi di integrazione salariale, l’astensione obbligatoria e facoltativa dal lavoro.</rdfs:comment>
        <rdfs:label xml:lang="it">Contributo figurativo</rdfs:label>
        <rdfs:label xml:lang="en">Imputed contribution</rdfs:label>
    </owl:Class>



    <!-- https://w3id.org/italia/social-security/onto/socialSafetyNet/ContributoGestioneSeparata -->

    <owl:Class rdf:about="https://w3id.org/italia/social-security/onto/socialSafetyNet/ContributoGestioneSeparata">
        <rdfs:subClassOf rdf:resource="https://w3id.org/italia/social-security/onto/socialSafetyNet/ContributoObbligatorio"/>
        <rdfs:subClassOf>
            <owl:Restriction>
                <owl:onProperty>
                    <rdf:Description>
                        <owl:inverseOf rdf:resource="https://w3id.org/italia/social-security/onto/socialSafetyNet/haContributoObbligatorio"/>
                    </rdf:Description>
                </owl:onProperty>
                <owl:someValuesFrom>
                    <owl:Class>
                        <owl:unionOf rdf:parseType="Collection">
                            <rdf:Description rdf:about="https://w3id.org/italia/social-security/onto/socialSafetyNet/CollaborazioneCoordinataEContinuativa"/>
                            <rdf:Description rdf:about="https://w3id.org/italia/social-security/onto/socialSafetyNet/ContrattoDOpera"/>
                            <rdf:Description rdf:about="https://w3id.org/italia/social-security/onto/socialSafetyNet/ContrattoDOperaProfessionale"/>
                        </owl:unionOf>
                    </owl:Class>
                </owl:someValuesFrom>
            </owl:Restriction>
        </rdfs:subClassOf>
        <rdfs:comment xml:lang="en">Mandatory contribution subclass relating to payments made by workers with parasubordinate or self-employed contracts or freelancers not belonging to a professional order with a social security fund.</rdfs:comment>
        <rdfs:comment xml:lang="it">Sottoclasse di Contributo obbligatorio relativo ai versamenti effettuati dai lavoratori con contratto di lavoro parasubordinato o autonomo o i liberi professionisti non afferenti ad un ordine professionale con cassa previdenziale.</rdfs:comment>
        <rdfs:label xml:lang="it">Contributo gestione separata</rdfs:label>
        <rdfs:label xml:lang="en">Separate pension scheme contribution</rdfs:label>
    </owl:Class>



    <!-- https://w3id.org/italia/social-security/onto/socialSafetyNet/ContributoGestioneSpecialeArtigiani -->

    <owl:Class rdf:about="https://w3id.org/italia/social-security/onto/socialSafetyNet/ContributoGestioneSpecialeArtigiani">
        <rdfs:subClassOf rdf:resource="https://w3id.org/italia/social-security/onto/socialSafetyNet/ContributoObbligatorio"/>
        <rdfs:comment xml:lang="en">Mandatory contribution subclass relating to payments made by workers with economic activity falling within the scope of crafts.</rdfs:comment>
        <rdfs:comment xml:lang="it">Sottoclasse di Contributo obbligatorio relativo ai versamenti effettuati dai lavoratori con attività economica rientrante nell&apos;ambito dell&apos;artigianato.</rdfs:comment>
        <rdfs:label xml:lang="en">Artisans pension scheme contribution</rdfs:label>
        <rdfs:label xml:lang="it">Contributo gestione speciale artigiani</rdfs:label>
    </owl:Class>



    <!-- https://w3id.org/italia/social-security/onto/socialSafetyNet/ContributoGestioneSpecialeCommercianti -->

    <owl:Class rdf:about="https://w3id.org/italia/social-security/onto/socialSafetyNet/ContributoGestioneSpecialeCommercianti">
        <rdfs:subClassOf rdf:resource="https://w3id.org/italia/social-security/onto/socialSafetyNet/ContributoObbligatorio"/>
        <rdfs:comment xml:lang="en">Mandatory contribution subclass relating to payments made by workers with economic activity falling within the scope of commerce.</rdfs:comment>
        <rdfs:comment xml:lang="it">Sottoclasse di Contributo obbligatorio relativo ai versamenti effettuati dai lavoratori con attività economica rientrante nell&apos;ambito del commercio.</rdfs:comment>
        <rdfs:label xml:lang="it">Contributo gestione speciale commercianti</rdfs:label>
        <rdfs:label xml:lang="en">Traders pension scheme contribution</rdfs:label>
    </owl:Class>



    <!-- https://w3id.org/italia/social-security/onto/socialSafetyNet/ContributoGestioneSpecialeLavoratoriAgricoli -->

    <owl:Class rdf:about="https://w3id.org/italia/social-security/onto/socialSafetyNet/ContributoGestioneSpecialeLavoratoriAgricoli">
        <rdfs:subClassOf rdf:resource="https://w3id.org/italia/social-security/onto/socialSafetyNet/ContributoObbligatorio"/>
        <rdfs:subClassOf>
            <owl:Restriction>
                <owl:onProperty>
                    <rdf:Description>
                        <owl:inverseOf rdf:resource="https://w3id.org/italia/social-security/onto/socialSafetyNet/haContributoObbligatorio"/>
                    </rdf:Description>
                </owl:onProperty>
                <owl:someValuesFrom>
                    <owl:Restriction>
                        <owl:onProperty>
                            <rdf:Description>
                                <owl:inverseOf rdf:resource="https://w3id.org/italia/social-security/onto/socialSafetyNet/proponeContrattoDiLavoro"/>
                            </rdf:Description>
                        </owl:onProperty>
                        <owl:someValuesFrom rdf:resource="https://w3id.org/italia/social-security/onto/socialSafetyNet/DatoreDiLavoroAgricolo"/>
                    </owl:Restriction>
                </owl:someValuesFrom>
            </owl:Restriction>
        </rdfs:subClassOf>
        <rdfs:comment xml:lang="en">Mandatory contribution subclass relating to payments made by workers with a salaried employment contract belonging to an Agricultural Employer.</rdfs:comment>
        <rdfs:comment xml:lang="it">Sottoclasse di Contributo obbligatorio relativo ai versamenti effettuati dai lavoratori con contratto di lavoro subordinato facente capo a un Datore di lavoro agricolo.</rdfs:comment>
        <rdfs:label xml:lang="en">Agricultural workers pensions scheme contribution</rdfs:label>
        <rdfs:label xml:lang="it">Contributo gestione speciale lavoratori agricoli</rdfs:label>
    </owl:Class>



    <!-- https://w3id.org/italia/social-security/onto/socialSafetyNet/ContributoLavoroEstero -->

    <owl:Class rdf:about="https://w3id.org/italia/social-security/onto/socialSafetyNet/ContributoLavoroEstero">
        <rdfs:subClassOf rdf:resource="https://w3id.org/italia/social-security/onto/socialSafetyNet/ContributoObbligatorio"/>
        <rdfs:comment xml:lang="en">Mandatory contribution subclass concerning the contributions paid by the Worker on an accrual basis to a social security institution of a foreign country, in particular belonging to the EC or EEA or Switzerland. These contributions, in addition to being valid with regard to the right to a pension, are also valid for obtaining the disoccupation subsidy in the same way as the mandatory contributions paid in Italy. To certify the periods of insurance, the worker can produce the DP U1 issued by the competent foreign social security institution or, failing that, this information can be requested from the foreign institution by INPS using the PAPER SED U001 form to which the foreign institution will respond using the PAPER SED U002 and PAPER SED U017 forms, while the information relating to salaries must be requested with the PAPER SED U003 to which the foreign institution will reply with the PAPER SED U004.</rdfs:comment>
        <rdfs:comment xml:lang="it">Sottoclasse di Contributo obbligatorio riguardante i contributi versati per competenza dal Lavoratore presso un istituto di previdenza di un paese estero, in particolare facente parte della CE o della SEE o la Svizzera. Tali contributi, oltre a valere in ordine al diritto alla pensione sono validi anche per ottenere il sussidio di disoccupazione alla stregua dei contributi obbligatori versati in Italia. Per attestare i periodi di assicurazione il lavoratore può produrre il DP U1 rilasciato dalla competente istituto previdenziale estero o, in mancanza, tali informazioni possono essere richieste all&apos;istituto estero dall&apos;INPS utilizzando il formulario PAPER SED U001 a cui l&apos;istituto estero risponderà utilizzando i formulari PAPER SED U002 e PAPER SED U017, mentre le informazioni relative alle retribuzioni dovranno essere richieste con il PAPER SED U003 a cui l’Istituzione estera risponderà con il PAPER SED U004.</rdfs:comment>
        <rdfs:label xml:lang="it">Contributo lavoro estero</rdfs:label>
        <rdfs:label xml:lang="en">Foreign work contribution</rdfs:label>
    </owl:Class>



    <!-- https://w3id.org/italia/social-security/onto/socialSafetyNet/ContributoObbligatorio -->

    <owl:Class rdf:about="https://w3id.org/italia/social-security/onto/socialSafetyNet/ContributoObbligatorio">
        <rdfs:subClassOf rdf:resource="https://w3id.org/italia/social-security/onto/socialSafetyNet/ContributoPrevidenziale"/>
        <rdfs:subClassOf>
            <owl:Restriction>
                <owl:onProperty>
                    <rdf:Description>
                        <owl:inverseOf rdf:resource="https://w3id.org/italia/social-security/onto/socialSafetyNet/haContributoObbligatorio"/>
                    </rdf:Description>
                </owl:onProperty>
                <owl:someValuesFrom rdf:resource="http://www.w3.org/2002/07/owl#Thing"/>
            </owl:Restriction>
        </rdfs:subClassOf>
        <rdfs:subClassOf>
            <owl:Restriction>
                <owl:onProperty rdf:resource="https://w3id.org/italia/social-security/onto/socialSafetyNet/imponibileContributivo"/>
                <owl:someValuesFrom rdf:resource="http://www.w3.org/2000/01/rdf-schema#Literal"/>
            </owl:Restriction>
        </rdfs:subClassOf>
        <rdfs:subClassOf>
            <owl:Restriction>
                <owl:onProperty rdf:resource="https://w3id.org/italia/social-security/onto/socialSafetyNet/numeroUnitàTemporaliPerDiritto"/>
                <owl:someValuesFrom rdf:resource="http://www.w3.org/2000/01/rdf-schema#Literal"/>
            </owl:Restriction>
        </rdfs:subClassOf>
        <rdfs:subClassOf>
            <owl:Restriction>
                <owl:onProperty rdf:resource="https://w3id.org/italia/social-security/onto/socialSafetyNet/numeroUnitàTemporaliPerMisura"/>
                <owl:someValuesFrom rdf:resource="http://www.w3.org/2000/01/rdf-schema#Literal"/>
            </owl:Restriction>
        </rdfs:subClassOf>
        <rdfs:subClassOf>
            <owl:Restriction>
                <owl:onProperty rdf:resource="https://w3id.org/italia/social-security/onto/socialSafetyNet/unitàDiMisuraTemporale"/>
                <owl:someValuesFrom rdf:resource="http://www.w3.org/2000/01/rdf-schema#Literal"/>
            </owl:Restriction>
        </rdfs:subClassOf>
        <rdfs:comment xml:lang="en">Social security contribution subclass refers to the portion of contributions that each worker must necessarily pay to the social security institution related to his or her activity.The taxable amount, the amount and the methods of payment of the mandatory contribution relate to the periods during which the worker actually performs his activity and therefore receives remuneration. They vary depending on the type of employment relationship, for example, self-employed or salaried.</rdfs:comment>
        <rdfs:comment xml:lang="it">Sottoclasse di Contributo previdenziale riferito alla quota di contributi che ogni lavoratore deve necessariamente versare all’ente previdenziale afferente alla propria attività.La base imponibile, la misura e le modalità di pagamento della contribuzione obbligatoria riguardano i periodi durante i quali il lavoratore presta effettivamente la propria attività e percepisce, pertanto, un compenso. Esse variano a seconda del tipo di rapporto di lavoro, ad esempio, autonomo o subordinato.</rdfs:comment>
        <rdfs:label xml:lang="it">Contributo obbligatorio</rdfs:label>
        <rdfs:label xml:lang="en">Mandatory contribution</rdfs:label>
    </owl:Class>



    <!-- https://w3id.org/italia/social-security/onto/socialSafetyNet/ContributoPrevidenziale -->

    <owl:Class rdf:about="https://w3id.org/italia/social-security/onto/socialSafetyNet/ContributoPrevidenziale">
        <rdfs:subClassOf rdf:resource="https://w3id.org/italia/onto/TI/TimeIndexedEvent"/>
        <rdfs:subClassOf>
            <owl:Restriction>
                <owl:onProperty rdf:resource="https://w3id.org/italia/social-security/onto/socialSafetyNet/haTipoDiContribuzione"/>
                <owl:someValuesFrom rdf:resource="http://www.w3.org/2002/07/owl#Thing"/>
            </owl:Restriction>
        </rdfs:subClassOf>
        <rdfs:subClassOf>
            <owl:Restriction>
                <owl:onProperty>
                    <rdf:Description>
                        <owl:inverseOf rdf:resource="https://w3id.org/italia/onto/l0/hasMember"/>
                    </rdf:Description>
                </owl:onProperty>
                <owl:someValuesFrom rdf:resource="https://w3id.org/italia/social-security/onto/socialSafetyNet/EstrattoContoContributivo"/>
            </owl:Restriction>
        </rdfs:subClassOf>
        <rdfs:subClassOf>
            <owl:Restriction>
                <owl:onProperty>
                    <rdf:Description>
                        <owl:inverseOf rdf:resource="https://w3id.org/italia/social-security/onto/socialSafetyNet/haContributoPrevidenziale"/>
                    </rdf:Description>
                </owl:onProperty>
                <owl:someValuesFrom rdf:resource="http://www.w3.org/2002/07/owl#Thing"/>
            </owl:Restriction>
        </rdfs:subClassOf>
        <rdfs:comment xml:lang="en">Event of payment of a sum of money, valid for a certain period of time, intended for the social security institution, typically INPS, to finance pension benefits or to guarantee workers adequate means for their living needs, in the event of disability, old age or involuntary unemployment. The contribution is normally calculated by applying a percentage rate to the compensation received by the worker in relation to his or her work provision.</rdfs:comment>
        <rdfs:comment xml:lang="it">Evento di versamento di una somma di denaro, valido per un determinato periodo temporale, destinato all’ente previdenziale, tipicamente INPS, per finanziare le prestazioni pensionistiche ovvero garantire ai lavoratori mezzi adeguati alle loro esigenze di vita, in caso di invalidità, vecchiaia o disoccupazione involontaria. Il contributo è normalmente calcolato applicando un’aliquota percentuale sul compenso ricevuto dal lavoratore in relazione alla sua prestazione lavorativa.</rdfs:comment>
        <rdfs:label xml:lang="it">Contributo previdenziale</rdfs:label>
        <rdfs:label xml:lang="en">Social security contribution</rdfs:label>
    </owl:Class>



    <!-- https://w3id.org/italia/social-security/onto/socialSafetyNet/ContributoVolontario -->

    <owl:Class rdf:about="https://w3id.org/italia/social-security/onto/socialSafetyNet/ContributoVolontario">
        <rdfs:subClassOf rdf:resource="https://w3id.org/italia/social-security/onto/socialSafetyNet/ContributoPrevidenziale"/>
        <rdfs:comment xml:lang="en">Social security contribution subclass refers to the portion of contributions paid by the worker, when the work relationship is interrupted or terminated for reasons other than those provided for the imputed contribution, in order to maintain the rights deriving from insurance or to meet the requirements for the provision of the benefit.</rdfs:comment>
        <rdfs:comment xml:lang="it">Sottoclasse di Contributo previdenziale riferito alla quota di contributi versata dal lavoratore, quando il rapporto di lavoro sia interrotto o cessato per cause diverse da quelle previste per la contribuzione figurativa, al fine di conservare i diritti derivanti dalle assicurazioni o per raggiungere i requisiti per l’erogazione della prestazione.</rdfs:comment>
        <rdfs:label xml:lang="it">Contributo volontario</rdfs:label>
        <rdfs:label xml:lang="en">Voluntary contribution</rdfs:label>
    </owl:Class>



    <!-- https://w3id.org/italia/social-security/onto/socialSafetyNet/DatoreDiLavoro -->

    <owl:Class rdf:about="https://w3id.org/italia/social-security/onto/socialSafetyNet/DatoreDiLavoro">
        <rdfs:subClassOf rdf:resource="https://w3id.org/italia/social-security/onto/socialSafetyNet/TitolareDelRapportoDiLavoro"/>
        <rdfs:subClassOf>
            <owl:Restriction>
                <owl:onProperty rdf:resource="https://w3id.org/italia/social-security/onto/socialSafetyNet/proponeContrattoDiLavoro"/>
                <owl:someValuesFrom>
                    <owl:Class>
                        <owl:unionOf rdf:parseType="Collection">
                            <rdf:Description rdf:about="https://w3id.org/italia/social-security/onto/socialSafetyNet/CollaborazioneCoordinataEContinuativa"/>
                            <rdf:Description rdf:about="https://w3id.org/italia/social-security/onto/socialSafetyNet/ContrattoDiLavoroSubordinato"/>
                        </owl:unionOf>
                    </owl:Class>
                </owl:someValuesFrom>
            </owl:Restriction>
        </rdfs:subClassOf>
        <rdfs:comment xml:lang="it">Sottoclasse di Titolare di rapporto di lavora che specializza tale ruolo per i contratti di tipo subordinato e parasubordinato.</rdfs:comment>
        <rdfs:comment xml:lang="en">Work relationship rightsholder subclass who specializes this role for subordinate and parasubordinate contracts.</rdfs:comment>
        <rdfs:label xml:lang="it">Datore di lavoro</rdfs:label>
        <rdfs:label xml:lang="en">Employer</rdfs:label>
    </owl:Class>



    <!-- https://w3id.org/italia/social-security/onto/socialSafetyNet/DatoreDiLavoroAgricolo -->

    <owl:Class rdf:about="https://w3id.org/italia/social-security/onto/socialSafetyNet/DatoreDiLavoroAgricolo">
        <rdfs:subClassOf rdf:resource="https://w3id.org/italia/social-security/onto/socialSafetyNet/DatoreDiLavoro"/>
        <rdfs:comment xml:lang="en">Role of Agent attributed to employers who are also agricultural entrepreneurs.</rdfs:comment>
        <rdfs:comment xml:lang="it">Ruolo di Agente attribuito ai datori di lavoro che sono anche imprenditori agricoli.</rdfs:comment>
        <rdfs:label xml:lang="en">Agricultural Employer</rdfs:label>
        <rdfs:label xml:lang="it">Datore di lavoro agricolo</rdfs:label>
    </owl:Class>



    <!-- https://w3id.org/italia/social-security/onto/socialSafetyNet/DelegatoDomandaNASpI -->

    <owl:Class rdf:about="https://w3id.org/italia/social-security/onto/socialSafetyNet/DelegatoDomandaNASpI">
        <rdfs:subClassOf rdf:resource="https://w3id.org/italia/social-security/onto/core/RuoloDiAgente"/>
        <rdfs:subClassOf>
            <owl:Restriction>
                <owl:onProperty rdf:resource="https://w3id.org/italia/social-security/onto/socialSafetyNet/haTipoDiDelegatoNASpI"/>
                <owl:someValuesFrom rdf:resource="http://www.w3.org/2002/07/owl#Thing"/>
            </owl:Restriction>
        </rdfs:subClassOf>
        <rdfs:comment xml:lang="en">Role of Agent of those who can submit a NASpI claim on behalf of an applicant, usually a Patronato.</rdfs:comment>
        <rdfs:comment xml:lang="it">Ruolo di Agente di chi può presentare una Domanda NASpI su mandato di un richiedente, solitamente un Patronato.</rdfs:comment>
        <rdfs:label xml:lang="it">Delegato domanda NASpI</rdfs:label>
        <rdfs:label xml:lang="en">NASpI claim delegate</rdfs:label>
    </owl:Class>



    <!-- https://w3id.org/italia/social-security/onto/socialSafetyNet/DetrazioneFiscalePerCarichiFamigliari -->

    <owl:Class rdf:about="https://w3id.org/italia/social-security/onto/socialSafetyNet/DetrazioneFiscalePerCarichiFamigliari">
        <rdfs:subClassOf rdf:resource="https://w3id.org/italia/social-security/onto/socialSafetyNet/PrestazioneDiSostegnoAlReddito"/>
        <rdfs:comment xml:lang="it">Beneficio fiscale legato alla condizione familiare del beneficiario che dipende sia dalla composizione del suo nucleo familiare sia dal reddito percepito da ciascun componente.</rdfs:comment>
        <rdfs:comment xml:lang="en">Tax benefit linked to the beneficiary&apos;s family condition that depends both on the composition of his or her household and on the income received by each member.</rdfs:comment>
        <rdfs:label xml:lang="it">Detrazione fiscale per carichi famigliari</rdfs:label>
        <rdfs:label xml:lang="en">Family expenses tax deduction</rdfs:label>
    </owl:Class>



    <!-- https://w3id.org/italia/social-security/onto/socialSafetyNet/DichiarazioneDiImmediataDisponibilità -->

    <owl:Class rdf:about="https://w3id.org/italia/social-security/onto/socialSafetyNet/DichiarazioneDiImmediataDisponibilità">
        <rdfs:subClassOf rdf:resource="https://w3id.org/italia/social-security/onto/socialSafetyNet/Atto"/>
        <rdfs:subClassOf>
            <owl:Restriction>
                <owl:onProperty rdf:resource="https://w3id.org/italia/social-security/onto/socialSafetyNet/haCPI"/>
                <owl:someValuesFrom rdf:resource="http://www.w3.org/2002/07/owl#Thing"/>
            </owl:Restriction>
        </rdfs:subClassOf>
        <rdfs:subClassOf>
            <owl:Restriction>
                <owl:onProperty>
                    <rdf:Description>
                        <owl:inverseOf rdf:resource="https://w3id.org/italia/social-security/onto/socialSafetyNet/haDID"/>
                    </rdf:Description>
                </owl:onProperty>
                <owl:someValuesFrom rdf:resource="http://www.w3.org/2002/07/owl#Thing"/>
            </owl:Restriction>
        </rdfs:subClassOf>
        <rdfs:comment xml:lang="en">Deed subclass by which a worker without job makes himself available to carry out work and to participate in active labour policy measures agreed with the Employment Centre (CPI). The DID can be submitted online to ANPAL (National Agency for Active Labour Policies) or through the CPI and certifies the worker&apos;s Unemployment status, putting him/her in a position to be able to take advantage of the services for integration into the labour market and any subsidies to which he/she is entitled.</rdfs:comment>
        <rdfs:comment xml:lang="it">Sottoclasse di Atto con cui un Lavoratore senza occupazione si rende disponibile allo svolgimento di attività lavorativa e alla partecipazione alle misure di politica attiva del lavoro concordate con il Centro Per l&apos;Impiego (CPI). La DID può essere presentata on-line all&apos;ANPAL (Agenzia Nazionale Politiche Attive del Lavoro) o per il tramite del CPI e certifica lo Stato di disoccupazione del lavoratore ponendolo nella condizione di poter usufruire dei servizi per l’inserimento nel mercato del lavoro e degli eventuali sussidi a cui ha diritto.</rdfs:comment>
        <rdfs:label xml:lang="en">Declaration of immediate availability</rdfs:label>
        <rdfs:label xml:lang="it">Dichiarazione di immediata disponibilità</rdfs:label>
    </owl:Class>



    <!-- https://w3id.org/italia/social-security/onto/socialSafetyNet/DipendentePrivato -->

    <owl:Class rdf:about="https://w3id.org/italia/social-security/onto/socialSafetyNet/DipendentePrivato">
        <rdfs:subClassOf rdf:resource="https://w3id.org/italia/social-security/onto/socialSafetyNet/Lavoratore"/>
        <owl:disjointWith rdf:resource="https://w3id.org/italia/social-security/onto/socialSafetyNet/DipendentePubblico"/>
        <rdfs:comment xml:lang="it">Sottoclasse di Lavoratore che fornisce la sua prestazione lavorativa ad una organizzazione privata. Tipicamente un lavoratore dipendente è un lavoratore subordinato non domestico.</rdfs:comment>
        <rdfs:comment xml:lang="en">Worker subclass who provides his work to a private organization. Typically, he/she is an employee but non-domestic.</rdfs:comment>
        <rdfs:label xml:lang="it">Dipendente privato</rdfs:label>
        <rdfs:label xml:lang="en">Private Employee</rdfs:label>
    </owl:Class>



    <!-- https://w3id.org/italia/social-security/onto/socialSafetyNet/DipendentePubblico -->

    <owl:Class rdf:about="https://w3id.org/italia/social-security/onto/socialSafetyNet/DipendentePubblico">
        <rdfs:subClassOf rdf:resource="https://w3id.org/italia/social-security/onto/socialSafetyNet/Lavoratore"/>
        <rdfs:comment xml:lang="it">Sottoclasse di Lavoratore che, da un punto di vista soggettivo, fornisce la sua prestazione lavorativa ad una Pubblica Amministrazione. Tipicamente un lavoratore dipendente è un lavoratore subordinato non domestico.</rdfs:comment>
        <rdfs:comment xml:lang="en">Worker subclass who, from a subjective point of view, provides his work to a Public Administration. Typically, he/she is an employee but non-domestic.</rdfs:comment>
        <rdfs:label xml:lang="en">Civil servant</rdfs:label>
        <rdfs:label xml:lang="it">Dipendente pubblico</rdfs:label>
    </owl:Class>



    <!-- https://w3id.org/italia/social-security/onto/socialSafetyNet/Disoccupato -->

    <owl:Class rdf:about="https://w3id.org/italia/social-security/onto/socialSafetyNet/Disoccupato">
        <rdfs:subClassOf rdf:resource="https://w3id.org/italia/social-security/onto/socialSafetyNet/Lavoratore"/>
        <rdfs:subClassOf>
            <owl:Restriction>
                <owl:onProperty rdf:resource="https://w3id.org/italia/onto/TI/hasTemporalEntity"/>
                <owl:someValuesFrom>
                    <owl:Restriction>
                        <owl:onProperty>
                            <rdf:Description>
                                <owl:inverseOf rdf:resource="https://w3id.org/italia/onto/TI/atTime"/>
                            </rdf:Description>
                        </owl:onProperty>
                        <owl:someValuesFrom rdf:resource="https://w3id.org/italia/social-security/onto/socialSafetyNet/StatoDiDisoccupazione"/>
                    </owl:Restriction>
                </owl:someValuesFrom>
            </owl:Restriction>
        </rdfs:subClassOf>
        <rdfs:subClassOf>
            <owl:Restriction>
                <owl:onProperty rdf:resource="https://w3id.org/italia/social-security/onto/socialSafetyNet/haFascicoloDiLavoro"/>
                <owl:someValuesFrom>
                    <owl:Restriction>
                        <owl:onProperty rdf:resource="https://w3id.org/italia/onto/l0/hasMember"/>
                        <owl:someValuesFrom rdf:resource="https://w3id.org/italia/social-security/onto/socialSafetyNet/StatoDiDisoccupazione"/>
                    </owl:Restriction>
                </owl:someValuesFrom>
            </owl:Restriction>
        </rdfs:subClassOf>
        <rdfs:subClassOf>
            <owl:Restriction>
                <owl:onProperty rdf:resource="https://w3id.org/italia/social-security/onto/socialSafetyNet/haStatoDiLavoro"/>
                <owl:someValuesFrom rdf:resource="https://w3id.org/italia/social-security/onto/socialSafetyNet/StatoDiDisoccupazione"/>
            </owl:Restriction>
        </rdfs:subClassOf>
        <owl:disjointWith rdf:resource="https://w3id.org/italia/social-security/onto/socialSafetyNet/Inoccupato"/>
        <rdfs:comment xml:lang="en">Role of Worker of those who are in an Unemployed status.</rdfs:comment>
        <rdfs:comment xml:lang="it">Ruolo di Lavoratore di coloro che sono in Stato di disoccupazione.</rdfs:comment>
        <rdfs:label xml:lang="it">Disoccupato</rdfs:label>
        <rdfs:label xml:lang="en">Unemployed</rdfs:label>
    </owl:Class>



    <!-- https://w3id.org/italia/social-security/onto/socialSafetyNet/DomandaDiPensionamento -->

    <owl:Class rdf:about="https://w3id.org/italia/social-security/onto/socialSafetyNet/DomandaDiPensionamento">
        <rdfs:subClassOf rdf:resource="https://w3id.org/italia/onto/TI/TimeIndexedEvent"/>
        <rdfs:comment xml:lang="en">Event of submission of a pension claim by an eligible person. Reaching the requirements for retirement is incompatible with the NASpI Benefit and causes its forfeiture.</rdfs:comment>
        <rdfs:comment xml:lang="it">Evento di presentazione di una domanda di pensionamento da parte di un avente diritto. Il raggiungimento dei requisiti per il pensionamento è incompatibile con la Prestazione NASpI e ne provoca la decadenza.</rdfs:comment>
        <rdfs:label xml:lang="it">Domanda di pensionamento</rdfs:label>
        <rdfs:label xml:lang="en">Retirement claim</rdfs:label>
    </owl:Class>



    <!-- https://w3id.org/italia/social-security/onto/socialSafetyNet/DomandaNASpI -->

    <owl:Class rdf:about="https://w3id.org/italia/social-security/onto/socialSafetyNet/DomandaNASpI">
        <rdfs:subClassOf>
            <owl:Restriction>
                <owl:onProperty rdf:resource="https://w3id.org/italia/social-security/onto/socialSafetyNet/haContributoUtilePerNASpI"/>
                <owl:someValuesFrom rdf:resource="http://www.w3.org/2002/07/owl#Thing"/>
            </owl:Restriction>
        </rdfs:subClassOf>
        <rdfs:subClassOf>
            <owl:Restriction>
                <owl:onProperty rdf:resource="https://w3id.org/italia/social-security/onto/socialSafetyNet/haDelegatoDomandaNASpI"/>
                <owl:someValuesFrom rdf:resource="http://www.w3.org/2002/07/owl#Thing"/>
            </owl:Restriction>
        </rdfs:subClassOf>
        <rdfs:subClassOf>
            <owl:Restriction>
                <owl:onProperty rdf:resource="https://w3id.org/italia/social-security/onto/socialSafetyNet/haDestinatarioDomandaNASpI"/>
                <owl:someValuesFrom rdf:resource="http://www.w3.org/2002/07/owl#Thing"/>
            </owl:Restriction>
        </rdfs:subClassOf>
        <rdfs:subClassOf>
            <owl:Restriction>
                <owl:onProperty rdf:resource="https://w3id.org/italia/social-security/onto/socialSafetyNet/haModalitàDiPagamentoNASpI"/>
                <owl:someValuesFrom rdf:resource="http://www.w3.org/2002/07/owl#Thing"/>
            </owl:Restriction>
        </rdfs:subClassOf>
        <rdfs:subClassOf>
            <owl:Restriction>
                <owl:onProperty rdf:resource="https://w3id.org/italia/social-security/onto/socialSafetyNet/haRichiedenteNASpI"/>
                <owl:someValuesFrom rdf:resource="http://www.w3.org/2002/07/owl#Thing"/>
            </owl:Restriction>
        </rdfs:subClassOf>
        <rdfs:subClassOf>
            <owl:Restriction>
                <owl:onProperty rdf:resource="https://w3id.org/italia/social-security/onto/socialSafetyNet/haSituazioneLavorativa"/>
                <owl:someValuesFrom rdf:resource="http://www.w3.org/2002/07/owl#Thing"/>
            </owl:Restriction>
        </rdfs:subClassOf>
        <rdfs:subClassOf>
            <owl:Restriction>
                <owl:onProperty rdf:resource="https://w3id.org/italia/social-security/onto/socialSafetyNet/haStatoDiDomandaNASpI"/>
                <owl:someValuesFrom rdf:resource="http://www.w3.org/2002/07/owl#Thing"/>
            </owl:Restriction>
        </rdfs:subClassOf>
        <rdfs:subClassOf>
            <owl:Restriction>
                <owl:onProperty rdf:resource="https://w3id.org/italia/social-security/onto/socialSafetyNet/seIndennitàMancatoPreavviso"/>
                <owl:someValuesFrom rdf:resource="http://www.w3.org/2000/01/rdf-schema#Literal"/>
            </owl:Restriction>
        </rdfs:subClassOf>
        <owl:disjointWith rdf:resource="https://w3id.org/italia/social-security/onto/socialSafetyNet/VariazioneModalitàDiPagamentoNASpI"/>
        <rdfs:comment xml:lang="en">Application for access to a NASpI benefit. The application is submitted to INPS exclusively electronically using the applicant&apos;s or delegate&apos;s access credentials (SPID), within 68 days, under penalty of forfeiture, starting from the date of termination of the employment relationship, in relation to the different reasons for termination or any unavailability due to maternity or illness.</rdfs:comment>
        <rdfs:comment xml:lang="it">Istanza di domanda per l&apos;accesso ad una Prestazione NASpI. La domanda viene presentata all&apos;INPS esclusivamente in via telematica utilizzando le credenziali di acceso del richiedente (SPID) o del delegato, entro 68 giorni, a pena di decadenza, che decorrono dalla data di cessazione del rapporto di lavoro, rapportata alla diverse motivazioni di cessazione o eventuali indisponibilità per maternità o malattia.</rdfs:comment>
        <rdfs:label xml:lang="it">Domanda NASpI</rdfs:label>
        <rdfs:label xml:lang="en">NASpI claim</rdfs:label>
    </owl:Class>



    <!-- https://w3id.org/italia/social-security/onto/socialSafetyNet/ElencodiAlboProfessionale -->

    <owl:Class rdf:about="https://w3id.org/italia/social-security/onto/socialSafetyNet/ElencodiAlboProfessionale">
        <rdfs:subClassOf>
            <owl:Restriction>
                <owl:onProperty>
                    <rdf:Description>
                        <owl:inverseOf rdf:resource="https://w3id.org/italia/social-security/onto/socialSafetyNet/haElencoDiAlboProfessionale"/>
                    </rdf:Description>
                </owl:onProperty>
                <owl:someValuesFrom rdf:resource="http://www.w3.org/2002/07/owl#Thing"/>
            </owl:Restriction>
        </rdfs:subClassOf>
        <rdfs:comment xml:lang="it">L&apos;Albo professionale di ciascun Ordine professionale può essere suddiviso in più elenchi (ad esempio quello dei giornalisti in quelli dei professionisti e dei pubblicisti).</rdfs:comment>
        <rdfs:comment xml:lang="en">The Professional register of each Professional association can be divided into several lists (e.g. that of journalists, those of professionals and publicists).</rdfs:comment>
        <rdfs:label xml:lang="it">Elenco di albo professionale</rdfs:label>
        <rdfs:label xml:lang="en">Professional register directory</rdfs:label>
    </owl:Class>



    <!-- https://w3id.org/italia/social-security/onto/socialSafetyNet/EspatrioInNASpI -->

    <owl:Class rdf:about="https://w3id.org/italia/social-security/onto/socialSafetyNet/EspatrioInNASpI">
        <rdfs:subClassOf rdf:resource="https://w3id.org/italia/onto/TI/TimeIndexedEvent"/>
        <rdfs:subClassOf>
            <owl:Restriction>
                <owl:onProperty rdf:resource="https://w3id.org/italia/social-security/onto/socialSafetyNet/haMotivoDiEspatrio"/>
                <owl:someValuesFrom rdf:resource="http://www.w3.org/2002/07/owl#Thing"/>
            </owl:Restriction>
        </rdfs:subClassOf>
        <rdfs:comment xml:lang="it">Evento di espatrio di un Beneficiario NASpI. Se il Beneficiario NASpI si reca in uno Stato SEE o in Svizzera alla ricerca di lavoro, mantiene la Prestazione NASpI per tre mesi e si rende disponibile per tale periodo ad ufficio per l&apos;impiego di tale stato; se alla scadenza dei tre mesi non fa ritorno in Italia, perde la Prestazione NASpI. Se si reca in uno Stato SEE o in Svizzera per altro motivo o in paese extracomunitario la Prestazione NASpI viene mantenuta ma il beneficiario resta disponibile al CPI con cui ha stipulato il PSP.</rdfs:comment>
        <rdfs:comment xml:lang="en">Expatriation event of a NASpI Beneficiary. If the NASpI Beneficiary travels to an EEA State or Switzerland in search of work, he/she maintains the NASpI Benefit for three months and makes his/her availability for that period to the employment office of that State; if at the end of the three months he does not return to Italy, he loses the NASpI Benefit. If he/she travels to an EEA country or Switzerland for another reason or to a non-EU country, the NASpI Benefit is maintained but the beneficiary remains available at the CPI with which he/she has contracted the PSP.</rdfs:comment>
        <rdfs:label xml:lang="it">Espatrio in NASpI</rdfs:label>
        <rdfs:label xml:lang="en">Expatriation in NASpI</rdfs:label>
    </owl:Class>



    <!-- https://w3id.org/italia/social-security/onto/socialSafetyNet/EstrattoContoContributivo -->

    <owl:Class rdf:about="https://w3id.org/italia/social-security/onto/socialSafetyNet/EstrattoContoContributivo">
        <rdfs:subClassOf rdf:resource="https://w3id.org/italia/onto/l0/Collection"/>
        <rdfs:subClassOf>
            <owl:Restriction>
                <owl:onProperty>
                    <rdf:Description>
                        <owl:inverseOf rdf:resource="https://w3id.org/italia/social-security/onto/socialSafetyNet/haEstrattoContoContributivo"/>
                    </rdf:Description>
                </owl:onProperty>
                <owl:someValuesFrom rdf:resource="http://www.w3.org/2002/07/owl#Thing"/>
            </owl:Restriction>
        </rdfs:subClassOf>
        <owl:disjointWith rdf:resource="https://w3id.org/italia/social-security/onto/socialSafetyNet/FascicoloDiLavoro"/>
        <rdfs:comment xml:lang="en">A collection that groups together the instances of Social security contribution linked to a person.</rdfs:comment>
        <rdfs:comment xml:lang="it">Collezione che raggruppa le istanze di Contributo previdenziale collegate ad una persona.</rdfs:comment>
        <rdfs:label xml:lang="en">Contribution account statement</rdfs:label>
        <rdfs:label xml:lang="it">Estratto conto contributivo</rdfs:label>
    </owl:Class>



    <!-- https://w3id.org/italia/social-security/onto/socialSafetyNet/FascicoloDiLavoro -->

    <owl:Class rdf:about="https://w3id.org/italia/social-security/onto/socialSafetyNet/FascicoloDiLavoro">
        <rdfs:subClassOf rdf:resource="https://w3id.org/italia/onto/l0/Collection"/>
        <rdfs:subClassOf>
            <owl:Restriction>
                <owl:onProperty>
                    <rdf:Description>
                        <owl:inverseOf rdf:resource="https://w3id.org/italia/social-security/onto/socialSafetyNet/haFascicoloDiLavoro"/>
                    </rdf:Description>
                </owl:onProperty>
                <owl:someValuesFrom rdf:resource="http://www.w3.org/2002/07/owl#Thing"/>
            </owl:Restriction>
        </rdfs:subClassOf>
        <rdfs:comment xml:lang="en">A collection that groups together Work status instances linked to a person.</rdfs:comment>
        <rdfs:comment xml:lang="it">Collezione che raggruppa le istanze di Stato di lavoro collegate ad una persona.</rdfs:comment>
        <rdfs:label xml:lang="it">Fascicolo di lavoro</rdfs:label>
        <rdfs:label xml:lang="en">Work folder</rdfs:label>
    </owl:Class>



    <!-- https://w3id.org/italia/social-security/onto/socialSafetyNet/ImprenditoreAgricolo -->

    <owl:Class rdf:about="https://w3id.org/italia/social-security/onto/socialSafetyNet/ImprenditoreAgricolo">
        <rdfs:subClassOf rdf:resource="https://w3id.org/italia/social-security/onto/core/RuoloDiAgente"/>
        <rdfs:comment xml:lang="en">Role of Agent attributed to the person who carries out an Agricultural activity.</rdfs:comment>
        <rdfs:comment xml:lang="it">Ruolo di Agente attribuito a colui che esercita una Attività agricola.</rdfs:comment>
        <rdfs:label xml:lang="en">Agricultural Entrepreneur</rdfs:label>
        <rdfs:label xml:lang="it">Imprenditore agricolo</rdfs:label>
    </owl:Class>



    <!-- https://w3id.org/italia/social-security/onto/socialSafetyNet/IndisponibilitàPerNASpI -->

    <owl:Class rdf:about="https://w3id.org/italia/social-security/onto/socialSafetyNet/IndisponibilitàPerNASpI">
        <rdfs:subClassOf rdf:resource="https://w3id.org/italia/onto/TI/TimeIndexedEvent"/>
        <rdfs:subClassOf>
            <owl:Restriction>
                <owl:onProperty rdf:resource="https://w3id.org/italia/social-security/onto/socialSafetyNet/haMotivoDiIndisponibilitàOperativa"/>
                <owl:someValuesFrom rdf:resource="http://www.w3.org/2002/07/owl#Thing"/>
            </owl:Restriction>
        </rdfs:subClassOf>
        <owl:disjointWith rdf:resource="https://w3id.org/italia/social-security/onto/socialSafetyNet/PrestazioneLavorativaFigurativa"/>
        <rdfs:comment xml:lang="en">Event of unavailability of the NASpI Beneficiary due to illness, hospitalization or maternity.</rdfs:comment>
        <rdfs:comment xml:lang="it">Evento di indisponibilità del Beneficiario NASpI per malattia, ricovero o maternità.</rdfs:comment>
        <rdfs:label xml:lang="it">Indisponibilità per NASpI</rdfs:label>
        <rdfs:label xml:lang="en">NASpI unavailability</rdfs:label>
    </owl:Class>



    <!-- https://w3id.org/italia/social-security/onto/socialSafetyNet/Inoccupato -->

    <owl:Class rdf:about="https://w3id.org/italia/social-security/onto/socialSafetyNet/Inoccupato">
        <rdfs:subClassOf rdf:resource="https://w3id.org/italia/social-security/onto/socialSafetyNet/Lavoratore"/>
        <rdfs:comment xml:lang="en">Role of Worker of those who are in a First-time jobseeker status.</rdfs:comment>
        <rdfs:comment xml:lang="it">Ruolo di Lavoratore di coloro che sono in Stato di inoccupazione.</rdfs:comment>
        <rdfs:label xml:lang="en">First-time jobseeker</rdfs:label>
        <rdfs:label xml:lang="it">Inoccupato</rdfs:label>
    </owl:Class>



    <!-- https://w3id.org/italia/social-security/onto/socialSafetyNet/IscrizioneAlboProfessionale -->

    <owl:Class rdf:about="https://w3id.org/italia/social-security/onto/socialSafetyNet/IscrizioneAlboProfessionale">
        <rdfs:subClassOf rdf:resource="https://w3id.org/italia/onto/TI/TimeIndexedEvent"/>
        <rdfs:subClassOf>
            <owl:Restriction>
                <owl:onProperty>
                    <rdf:Description>
                        <owl:inverseOf rdf:resource="https://w3id.org/italia/social-security/onto/socialSafetyNet/haIscrizioneAlboProfessionale"/>
                    </rdf:Description>
                </owl:onProperty>
                <owl:someValuesFrom rdf:resource="http://www.w3.org/2002/07/owl#Thing"/>
            </owl:Restriction>
        </rdfs:subClassOf>
        <rdfs:subClassOf>
            <owl:Restriction>
                <owl:onProperty>
                    <rdf:Description>
                        <owl:inverseOf rdf:resource="https://w3id.org/italia/social-security/onto/socialSafetyNet/èIscrittoAlboProfessionale"/>
                    </rdf:Description>
                </owl:onProperty>
                <owl:someValuesFrom rdf:resource="http://www.w3.org/2002/07/owl#Thing"/>
            </owl:Restriction>
        </rdfs:subClassOf>
        <rdfs:subClassOf>
            <owl:Restriction>
                <owl:onProperty rdf:resource="https://w3id.org/italia/social-security/onto/socialSafetyNet/dataIscrizioneAlboProfessionale"/>
                <owl:someValuesFrom rdf:resource="http://www.w3.org/2000/01/rdf-schema#Literal"/>
            </owl:Restriction>
        </rdfs:subClassOf>
        <rdfs:subClassOf>
            <owl:Restriction>
                <owl:onProperty rdf:resource="https://w3id.org/italia/social-security/onto/socialSafetyNet/numeroIscrizioneAlboProfessionale"/>
                <owl:someValuesFrom rdf:resource="http://www.w3.org/2000/01/rdf-schema#Literal"/>
            </owl:Restriction>
        </rdfs:subClassOf>
        <rdfs:comment xml:lang="en">Class of events for registration of persons with the role of Protected freelancer in the relevant professional registers. In some appropriately regulated cases, enrolment is subject to passing a qualifying examination to practise the profession.</rdfs:comment>
        <rdfs:comment xml:lang="it">Classe degli eventi di iscrizione delle persone con ruolo di Libero professionista protetto nei relativi albi professionali. In alcuni casi opportunamente normati, l&apos;iscrizione è subordinata al superamento di un esame di abilitazione all&apos;esercizio della professione.</rdfs:comment>
        <rdfs:label xml:lang="it">Iscrizione albo professionale</rdfs:label>
        <rdfs:label xml:lang="en">Professional register entry</rdfs:label>
    </owl:Class>



    <!-- https://w3id.org/italia/social-security/onto/socialSafetyNet/IscrizioneUfficioDelLavoro -->

    <owl:Class rdf:about="https://w3id.org/italia/social-security/onto/socialSafetyNet/IscrizioneUfficioDelLavoro">
        <rdfs:subClassOf rdf:resource="https://w3id.org/italia/onto/TI/TimeIndexedEvent"/>
        <rdfs:subClassOf>
            <owl:Restriction>
                <owl:onProperty rdf:resource="https://w3id.org/italia/social-security/onto/socialSafetyNet/haUfficioDelLavoroDiIscrizione"/>
                <owl:someValuesFrom rdf:resource="http://www.w3.org/2002/07/owl#Thing"/>
            </owl:Restriction>
        </rdfs:subClassOf>
        <rdfs:subClassOf>
            <owl:Restriction>
                <owl:onProperty>
                    <rdf:Description>
                        <owl:inverseOf rdf:resource="https://w3id.org/italia/social-security/onto/socialSafetyNet/èIscrittoUfficioDelLavoro"/>
                    </rdf:Description>
                </owl:onProperty>
                <owl:someValuesFrom rdf:resource="http://www.w3.org/2002/07/owl#Thing"/>
            </owl:Restriction>
        </rdfs:subClassOf>
        <rdfs:comment xml:lang="en">Class of registration events of persons with the role of Worker at a Labour office.</rdfs:comment>
        <rdfs:comment xml:lang="it">Classe degli eventi di iscrizione delle persone con ruolo di Lavoratore presso un Ufficio del lavoro.</rdfs:comment>
        <rdfs:label xml:lang="it">Iscrizione ufficio del lavoro</rdfs:label>
        <rdfs:label xml:lang="en">Labour office registration</rdfs:label>
    </owl:Class>



    <!-- https://w3id.org/italia/social-security/onto/socialSafetyNet/Lavoratore -->

    <owl:Class rdf:about="https://w3id.org/italia/social-security/onto/socialSafetyNet/Lavoratore">
        <rdfs:subClassOf rdf:resource="https://w3id.org/italia/social-security/onto/core/RuoloDiPersonaViva"/>
        <rdfs:subClassOf>
            <owl:Restriction>
                <owl:onProperty rdf:resource="https://w3id.org/italia/social-security/onto/socialSafetyNet/haStatoDiLavoro"/>
                <owl:someValuesFrom rdf:resource="http://www.w3.org/2002/07/owl#Thing"/>
            </owl:Restriction>
        </rdfs:subClassOf>
        <rdfs:comment xml:lang="it">Ruolo di Persona viva attribuito a chi fornisce, nell&apos;ambito di un rapporto di lavoro, una prestazione lavorativa manuale o intellettuale tipicamente a titolo oneroso o, in alcuni casi particolari, come il volontariato, a titolo gratuito.  </rdfs:comment>
        <rdfs:comment xml:lang="en">The role of Living Person is attributed to those who provide, in the context of a work relationship, a manual or intellectual work provision, typically for consideration or, in some special cases, such as volunteering, free of charge.</rdfs:comment>
        <rdfs:label xml:lang="it">Lavoratore</rdfs:label>
        <rdfs:label xml:lang="en">Worker</rdfs:label>
    </owl:Class>



    <!-- https://w3id.org/italia/social-security/onto/socialSafetyNet/LavoratoreAPartitaIVA -->

    <owl:Class rdf:about="https://w3id.org/italia/social-security/onto/socialSafetyNet/LavoratoreAPartitaIVA">
        <rdfs:subClassOf>
            <owl:Class>
                <owl:unionOf rdf:parseType="Collection">
                    <rdf:Description rdf:about="https://w3id.org/italia/social-security/onto/socialSafetyNet/LavoratoreAutonomo"/>
                    <rdf:Description rdf:about="https://w3id.org/italia/social-security/onto/socialSafetyNet/LiberoProfessionista"/>
                </owl:unionOf>
            </owl:Class>
        </rdfs:subClassOf>
        <rdfs:subClassOf>
            <owl:Restriction>
                <owl:onProperty rdf:resource="https://w3id.org/italia/social-security/onto/socialSafetyNet/haTipoDiAttivitàEconomica"/>
                <owl:someValuesFrom rdf:resource="http://www.w3.org/2002/07/owl#Thing"/>
            </owl:Restriction>
        </rdfs:subClassOf>
        <rdfs:subClassOf>
            <owl:Restriction>
                <owl:onProperty rdf:resource="https://w3id.org/italia/social-security/onto/socialSafetyNet/partitaIVA"/>
                <owl:someValuesFrom rdf:resource="http://www.w3.org/2000/01/rdf-schema#Literal"/>
            </owl:Restriction>
        </rdfs:subClassOf>
        <rdfs:comment xml:lang="it">Classifica quei lavoratori autonomi o liberi professionisti che, in base alla normativa, per svolgere la propria attività devono dotarsi di una partita IVA, aprendo una posizione IVA presso l&apos;Agenzia delle Entrate e dichiarando al contempo le attività economiche (codice ATECO) interessate dalla sua attività. In generale chiunque svolga una attività in proprio deve dotarsi di una partita IVA.</rdfs:comment>
        <rdfs:comment xml:lang="en">Classifies those self-employed workers or freelancers who, according to the legislation, must have a VAT number in order to carry out their activity, opening a VAT position with the Revenue Agency and at the same time declaring the economic activities (ATECO code) affected by their activity. In general, anyone who carries out their own business must have a VAT number.</rdfs:comment>
        <rdfs:label xml:lang="it">Lavoratore a partita IVA</rdfs:label>
        <rdfs:label xml:lang="en">VAT-registered worker</rdfs:label>
    </owl:Class>



    <!-- https://w3id.org/italia/social-security/onto/socialSafetyNet/LavoratoreAutonomo -->

    <owl:Class rdf:about="https://w3id.org/italia/social-security/onto/socialSafetyNet/LavoratoreAutonomo">
        <rdfs:subClassOf rdf:resource="https://w3id.org/italia/social-security/onto/socialSafetyNet/Lavoratore"/>
        <rdfs:comment xml:lang="it">Sottoclasse di Lavoratore relativa a coloro che sottoscrivono un Contratto d&apos;Opera ovvero che forniscono una prestazione lavorativa dietro compenso operando in totale autonomia organizzativa e operativa.</rdfs:comment>
        <rdfs:comment xml:lang="en">Worker subclass relating to those who sign a Manufacturing service contract or who provide work for a fee by operating in total organizational and operational autonomy.</rdfs:comment>
        <rdfs:label xml:lang="it">Lavoratore autonomo</rdfs:label>
        <rdfs:label xml:lang="en">Self-employed</rdfs:label>
    </owl:Class>



    <!-- https://w3id.org/italia/social-security/onto/socialSafetyNet/LavoratoreAutonomoOccasionale -->

    <owl:Class rdf:about="https://w3id.org/italia/social-security/onto/socialSafetyNet/LavoratoreAutonomoOccasionale">
        <rdfs:subClassOf rdf:resource="https://w3id.org/italia/social-security/onto/socialSafetyNet/Lavoratore"/>
        <rdfs:subClassOf>
            <owl:Restriction>
                <owl:onProperty rdf:resource="https://w3id.org/italia/social-security/onto/socialSafetyNet/accettaContrattoDiLavoro"/>
                <owl:someValuesFrom rdf:resource="https://w3id.org/italia/social-security/onto/socialSafetyNet/ContrattoDOpera"/>
            </owl:Restriction>
        </rdfs:subClassOf>
        <rdfs:comment xml:lang="it">Sottoclasse di Lavoratore relativa a coloro che sottoscrivono in modo episodico e non continuativo un Contratto d&apos;Opera, operando in totale autonomia.</rdfs:comment>
        <rdfs:comment xml:lang="en">Worker subclass relating to those who sign an Manufacturing service contract in an episodic and non-continuous way, operating in total autonomy.</rdfs:comment>
        <rdfs:label xml:lang="it">Lavoratore autonomo occasionale</rdfs:label>
        <rdfs:label xml:lang="en">Occasional self-employed</rdfs:label>
    </owl:Class>



    <!-- https://w3id.org/italia/social-security/onto/socialSafetyNet/LavoratoreDiversoDalFrontaliero -->

    <owl:Class rdf:about="https://w3id.org/italia/social-security/onto/socialSafetyNet/LavoratoreDiversoDalFrontaliero">
        <rdfs:subClassOf rdf:resource="https://w3id.org/italia/social-security/onto/socialSafetyNet/Lavoratore"/>
        <owl:disjointWith rdf:resource="https://w3id.org/italia/social-security/onto/socialSafetyNet/LavoratoreFrontaliero"/>
        <rdfs:comment xml:lang="en">Role of Worker relating to those who, in the course of their last employment or self-employed activity, reside in an EU Member State other than the one to whose legislation they are subject and which is not necessarily the State in which the employed or self-employed activity is carried out. Among the categories of workers who fall into this category are: seafarers, those who normally carry out their activity in the territory of two or more EU Member States, persons who are part of flight and cabin crews engaged in passenger or cargo air transport services, seasonal workers.</rdfs:comment>
        <rdfs:comment xml:lang="it">Ruolo di Lavoratore relativa a coloro che, nel corso della loro ultima attività subordinata o autonoma, risiedono in uno Stato membro UE diverso da quello alla cui legislazione sono soggetti e che non è necessariamente lo Stato in cui è esercitata l’attività subordinata o autonoma. Tra le categorie di lavoratori che rientrano in tale tipologia ci sono: i marittimi, chi normalmente esercita la propria attività nel territorio di due o più Stati membri UE, le persone che fanno parte degli equipaggi di condotta e di cabina addetti a servizi di trasporto aereo passeggeri o merci, i lavoratori stagionali.</rdfs:comment>
        <rdfs:label xml:lang="it">Lavoratore diverso dal frontaliero</rdfs:label>
        <rdfs:label xml:lang="en">Worker other than frontier</rdfs:label>
    </owl:Class>



    <!-- https://w3id.org/italia/social-security/onto/socialSafetyNet/LavoratoreFrontaliero -->

    <owl:Class rdf:about="https://w3id.org/italia/social-security/onto/socialSafetyNet/LavoratoreFrontaliero">
        <rdfs:subClassOf rdf:resource="https://w3id.org/italia/social-security/onto/socialSafetyNet/Lavoratore"/>
        <rdfs:comment xml:lang="en">Role of Worker refers to those who work in an EU Member State (State of employment) and reside in another EU Member State (State of residence) to which they return in principle every day or at least once a week. The holder of residence does not preclude the frontier worker, for practical reasons, from also having a (temporary) domicile in the State of employment.</rdfs:comment>
        <rdfs:comment xml:lang="it">Ruolo di Lavoratore riguardante chi lavora in uno Stato membro UE (Stato di occupazione) e risiede in un altro Stato membro UE (Stato di residenza) nel quale ritorna in linea di massima ogni giorno o almeno una volta la settimana. Il possesso della residenza non esclude che il lavoratore frontaliero, per ragioni pratiche, possegga anche una domicilio (temporaneo) nello Stato di occupazione.</rdfs:comment>
        <rdfs:label xml:lang="en">Frontier worker</rdfs:label>
        <rdfs:label xml:lang="it">Lavoratore frontaliero</rdfs:label>
    </owl:Class>



    <!-- https://w3id.org/italia/social-security/onto/socialSafetyNet/LavoratoreParasubordinato -->

    <owl:Class rdf:about="https://w3id.org/italia/social-security/onto/socialSafetyNet/LavoratoreParasubordinato">
        <rdfs:subClassOf rdf:resource="https://w3id.org/italia/social-security/onto/socialSafetyNet/Lavoratore"/>
        <rdfs:subClassOf>
            <owl:Restriction>
                <owl:onProperty rdf:resource="https://w3id.org/italia/social-security/onto/socialSafetyNet/accettaContrattoDiLavoro"/>
                <owl:someValuesFrom rdf:resource="https://w3id.org/italia/social-security/onto/socialSafetyNet/CollaborazioneCoordinataEContinuativa"/>
            </owl:Restriction>
        </rdfs:subClassOf>
        <rdfs:comment xml:lang="it">Sottoclasse di Lavoratore relativa a coloro che sottoscrivono un contratto di Collaborazione coordinata e continuativa.</rdfs:comment>
        <rdfs:comment xml:lang="en">Worker subclass relating to those who sign a contract of Coordinated and continuous collaboration.</rdfs:comment>
        <rdfs:label xml:lang="it">Lavoratore parasubordinato</rdfs:label>
        <rdfs:label xml:lang="en">Para-subordinate worker</rdfs:label>
    </owl:Class>



    <!-- https://w3id.org/italia/social-security/onto/socialSafetyNet/LavoratoreSubordinato -->

    <owl:Class rdf:about="https://w3id.org/italia/social-security/onto/socialSafetyNet/LavoratoreSubordinato">
        <rdfs:subClassOf rdf:resource="https://w3id.org/italia/social-security/onto/socialSafetyNet/Lavoratore"/>
        <rdfs:subClassOf>
            <owl:Restriction>
                <owl:onProperty rdf:resource="https://w3id.org/italia/social-security/onto/socialSafetyNet/accettaContrattoDiLavoro"/>
                <owl:someValuesFrom rdf:resource="https://w3id.org/italia/social-security/onto/socialSafetyNet/ContrattoDiLavoroSubordinato"/>
            </owl:Restriction>
        </rdfs:subClassOf>
        <rdfs:comment xml:lang="it">Sottoclasse di Lavoratore relativa a coloro che sottoscrivono un Contratto di lavoro subordinato.</rdfs:comment>
        <rdfs:comment xml:lang="en">Worker subclass relating to those who sign a Salaried employment contract.</rdfs:comment>
        <rdfs:label xml:lang="en">Employee</rdfs:label>
        <rdfs:label xml:lang="it">Lavoratore subordinato</rdfs:label>
    </owl:Class>



    <!-- https://w3id.org/italia/social-security/onto/socialSafetyNet/LavoratoreSubordinatoAgricolo -->

    <owl:Class rdf:about="https://w3id.org/italia/social-security/onto/socialSafetyNet/LavoratoreSubordinatoAgricolo">
        <rdfs:subClassOf rdf:resource="https://w3id.org/italia/social-security/onto/socialSafetyNet/LavoratoreSubordinato"/>
        <rdfs:subClassOf>
            <owl:Restriction>
                <owl:onProperty rdf:resource="https://w3id.org/italia/social-security/onto/socialSafetyNet/accettaContrattoDiLavoro"/>
                <owl:someValuesFrom>
                    <owl:Restriction>
                        <owl:onProperty>
                            <rdf:Description>
                                <owl:inverseOf rdf:resource="https://w3id.org/italia/social-security/onto/socialSafetyNet/proponeContrattoDiLavoro"/>
                            </rdf:Description>
                        </owl:onProperty>
                        <owl:someValuesFrom rdf:resource="https://w3id.org/italia/social-security/onto/socialSafetyNet/DatoreDiLavoroAgricolo"/>
                    </owl:Restriction>
                </owl:someValuesFrom>
            </owl:Restriction>
        </rdfs:subClassOf>
        <rdfs:comment xml:lang="en">Employee subclass of those who have an Agricultural employer as a counterparty to the Salaried employment contract.</rdfs:comment>
        <rdfs:comment xml:lang="it">Sottoclasse di Lavoratore subordinato di coloro che hanno come controparte del contratto di lavoro un Datore di lavoro agricolo.</rdfs:comment>
        <rdfs:label xml:lang="en">Agricultural employee</rdfs:label>
        <rdfs:label xml:lang="it">Lavoratore subordinato agricolo</rdfs:label>
    </owl:Class>



    <!-- https://w3id.org/italia/social-security/onto/socialSafetyNet/LiberoProfessionista -->

    <owl:Class rdf:about="https://w3id.org/italia/social-security/onto/socialSafetyNet/LiberoProfessionista">
        <rdfs:subClassOf rdf:resource="https://w3id.org/italia/social-security/onto/socialSafetyNet/Lavoratore"/>
        <rdfs:comment xml:lang="it">Sottoclasse di Lavoratore che raccoglie i lavoratori che svolgono  attività professionale di tipo intellettuale ovvero non manuale. Alcune di tali attività possono essere svolte solo acquisendo opportune abilitazioni regolamentate dalla norma e/o dai relativi ordini professionali. La libera professione può essere svolto sia in forma autonoma sia subordinata.</rdfs:comment>
        <rdfs:comment xml:lang="en">Worker subclass that includes workers who carry out professional activities of an intellectual or non-manual type. Some of these activities can only be carried out by acquiring appropriate qualifications regulated by the law and/or by the relevant professional associations. Independent professional work can be carried out both autonomously and subordinately.</rdfs:comment>
        <rdfs:label xml:lang="en">Freelancer</rdfs:label>
        <rdfs:label xml:lang="it">Libero professionista</rdfs:label>
    </owl:Class>



    <!-- https://w3id.org/italia/social-security/onto/socialSafetyNet/LiberoProfessionistaProtetto -->

    <owl:Class rdf:about="https://w3id.org/italia/social-security/onto/socialSafetyNet/LiberoProfessionistaProtetto">
        <rdfs:subClassOf rdf:resource="https://w3id.org/italia/social-security/onto/socialSafetyNet/LiberoProfessionista"/>
        <rdfs:comment xml:lang="en">Freelancer subclass relating to workers who, in order to exercise their professional activity, need to be registered in specific registers, i.e. in the Professional register established by the relevant Professional association.</rdfs:comment>
        <rdfs:comment xml:lang="it">Sottoclasse di Libero Professionista relativa a lavoratori che per esercitare la loro attività professionale necessitano dell&apos;iscrizione a specifici registri cioè all&apos;Albo professionale istituito dal relativo Ordine professionale.</rdfs:comment>
        <rdfs:label xml:lang="it">Libero professionista protetto</rdfs:label>
        <rdfs:label xml:lang="en">Protected freelancer</rdfs:label>
    </owl:Class>



    <!-- https://w3id.org/italia/social-security/onto/socialSafetyNet/ModalitàDiPagamentoNASpI -->

    <owl:Class rdf:about="https://w3id.org/italia/social-security/onto/socialSafetyNet/ModalitàDiPagamentoNASpI">
        <rdfs:subClassOf>
            <owl:Restriction>
                <owl:onProperty rdf:resource="https://w3id.org/italia/social-security/onto/socialSafetyNet/haTipoModalitàDiPagamentoNASpI"/>
                <owl:someValuesFrom rdf:resource="http://www.w3.org/2002/07/owl#Thing"/>
            </owl:Restriction>
        </rdfs:subClassOf>
        <rdfs:comment xml:lang="en">Application for payment methods related to a NASpI claim. If you have chosen to give a bank credit, in Italy or abroad, your IBAN and BIC must be indicated which must necessarily be in the name of the NASpI beneficiary.</rdfs:comment>
        <rdfs:comment xml:lang="it">Istanza di modalità di pagamento relativa ad una Domanda NASpI. In caso sia stato scelto l&apos;accredito bancario, in Italia o all&apos;estero, dovranno essere indicati IBAN e BIC, che dovranno essere necessariamente intestati al Beneficiario NASpI.</rdfs:comment>
        <rdfs:label xml:lang="it">Modalità di pagamento NASpI</rdfs:label>
        <rdfs:label xml:lang="en">NASpI payment method</rdfs:label>
    </owl:Class>



    <!-- https://w3id.org/italia/social-security/onto/socialSafetyNet/MotivoCessazioneInvolontaria -->

    <owl:Class rdf:about="https://w3id.org/italia/social-security/onto/socialSafetyNet/MotivoCessazioneInvolontaria">
        <rdfs:subClassOf rdf:resource="https://w3id.org/italia/social-security/onto/socialSafetyNet/MotivoCessazioneRapportoDiLavoro"/>
        <owl:disjointWith rdf:resource="https://w3id.org/italia/social-security/onto/socialSafetyNet/MotivoCessazioneVolontaria"/>
        <rdfs:comment xml:lang="it">Sottoclasse di Motivo cessazione rapporto di lavoro riguardante i motivi indipendenti dalla volontà del lavoratore.</rdfs:comment>
        <rdfs:comment xml:lang="en">Work relationship termination cause subclass concerning reasons beyond the employee&apos;s control.</rdfs:comment>
        <rdfs:label xml:lang="en">Involuntary dismissal cause</rdfs:label>
        <rdfs:label xml:lang="it">Motivo cessazione involontaria</rdfs:label>
    </owl:Class>



    <!-- https://w3id.org/italia/social-security/onto/socialSafetyNet/MotivoCessazioneRapportoDiLavoro -->

    <owl:Class rdf:about="https://w3id.org/italia/social-security/onto/socialSafetyNet/MotivoCessazioneRapportoDiLavoro">
        <rdfs:subClassOf>
            <owl:Class>
                <owl:unionOf rdf:parseType="Collection">
                    <rdf:Description rdf:about="https://w3id.org/italia/social-security/onto/socialSafetyNet/MotivoCessazioneInvolontaria"/>
                    <rdf:Description rdf:about="https://w3id.org/italia/social-security/onto/socialSafetyNet/MotivoCessazioneVolontaria"/>
                </owl:unionOf>
            </owl:Class>
        </rdfs:subClassOf>
        <rdfs:comment xml:lang="it">Classifica le motivazioni per la cessazione di un rapporto di lavoro.</rdfs:comment>
        <rdfs:comment xml:lang="en">Classify the reasons for terminating a work relationship.</rdfs:comment>
        <rdfs:label xml:lang="it">Motivo cessazione rapporto di lavoro</rdfs:label>
        <rdfs:label xml:lang="en">Work relationship termination cause</rdfs:label>
    </owl:Class>



    <!-- https://w3id.org/italia/social-security/onto/socialSafetyNet/MotivoCessazioneVolontaria -->

    <owl:Class rdf:about="https://w3id.org/italia/social-security/onto/socialSafetyNet/MotivoCessazioneVolontaria">
        <rdfs:subClassOf rdf:resource="https://w3id.org/italia/social-security/onto/socialSafetyNet/MotivoCessazioneRapportoDiLavoro"/>
        <rdfs:comment xml:lang="it">Sottoclasse di Motivo cessazione rapporto di lavoro riguardante i motivi dipendenti dalla volontà del lavoratore.</rdfs:comment>
        <rdfs:comment xml:lang="en">Work relationship termination cause subclass concerning the reasons dependent on the will of the worker.</rdfs:comment>
        <rdfs:label xml:lang="it">Motivo cessazione volontaria</rdfs:label>
        <rdfs:label xml:lang="en">Voluntary dismissal cause</rdfs:label>
    </owl:Class>



    <!-- https://w3id.org/italia/social-security/onto/socialSafetyNet/MotivoDecadenzaDisoccupazione -->

    <owl:Class rdf:about="https://w3id.org/italia/social-security/onto/socialSafetyNet/MotivoDecadenzaDisoccupazione">
        <rdfs:comment xml:lang="it">Classifica le motivazioni per la decadenza dallo Stato di disoccupazione di un Lavoratore. Tra le motivazioni c&apos;è ovviamente l&apos;aver trovato un nuovo lavoro ma anche il non aver ripetutamente partecipato alle iniziative formative precedentemente concordate con il CPI o l&apos;aver rifiutato, senza giustificato motivo, un&apos;offerta congrua di lavoro.</rdfs:comment>
        <rdfs:comment xml:lang="en">Classifies the reasons for the forfeiture of a Worker&apos;s Unemployment status. Among the reasons there is obviously having found a new job but also not having repeatedly participated in the training initiatives previously agreed with the CPI or having refused, without justified reason, a suitable job offer.</rdfs:comment>
        <rdfs:label xml:lang="it">Motivo decadenza disoccupazione</rdfs:label>
        <rdfs:label xml:lang="en">Unemployment forfeiture cause</rdfs:label>
    </owl:Class>



    <!-- https://w3id.org/italia/social-security/onto/socialSafetyNet/MotivoDecadenzaNASpI -->

    <owl:Class rdf:about="https://w3id.org/italia/social-security/onto/socialSafetyNet/MotivoDecadenzaNASpI">
        <rdfs:comment xml:lang="it">Classifica le motivazioni per la decadenza dal diritto alla Prestazione NASpI. Le motivazioni possono essere legate sia ad eventi evolutivi della condizione del lavoratore  (nuova occupazione, pensionamento, etc.) sia a mancati adempimenti obbligatori da parte del Beneficiario NASpI.</rdfs:comment>
        <rdfs:comment xml:lang="en">Classifies the reasons for the forfeiture of the right to the NASpI Benefit. The reasons may be linked both to evolutionary events in the worker&apos;s condition (new employment, retirement, etc.) and to non-compliance by the NASpI Beneficiary.</rdfs:comment>
        <rdfs:label xml:lang="it">Motivo decadenza NASpI</rdfs:label>
        <rdfs:label xml:lang="en">NASpI forfeiture cause</rdfs:label>
    </owl:Class>



    <!-- https://w3id.org/italia/social-security/onto/socialSafetyNet/MotivoDiEspatrio -->

    <owl:Class rdf:about="https://w3id.org/italia/social-security/onto/socialSafetyNet/MotivoDiEspatrio">
        <rdfs:comment xml:lang="it">Classifica i motivi che inducono un Beneficiario NASpI all&apos;espatrio. I motivi principali sono: la ricerca di un nuovo lavoro, l&apos;inizio di un nuovo lavoro o altro. Il mantenimento della Prestazione NASpI viene stabilito in base alla motivazione e allo stato di destinazione dell&apos;espatrio.</rdfs:comment>
        <rdfs:comment xml:lang="en">Classifies the reasons that induce a NASpI Beneficiary to leave the country. The main reasons are: looking for a new job, starting a new job, or whatever. The maintenance of the NASpI benefit is established on the basis of the motivation and the state of destination of the expatriation.</rdfs:comment>
        <rdfs:label xml:lang="en">Expatriation cause</rdfs:label>
        <rdfs:label xml:lang="it">Motivo di espatrio</rdfs:label>
    </owl:Class>



    <!-- https://w3id.org/italia/social-security/onto/socialSafetyNet/MotivoDiIndisponibilitàOperativa -->

    <owl:Class rdf:about="https://w3id.org/italia/social-security/onto/socialSafetyNet/MotivoDiIndisponibilitàOperativa">
        <rdfs:comment xml:lang="it">Classifica le motivazioni di indisponibilità giustificata.</rdfs:comment>
        <rdfs:comment xml:lang="en">Classify the reasons for justified unavailability.</rdfs:comment>
        <rdfs:label xml:lang="it">Motivo di indisponibilità operativa</rdfs:label>
        <rdfs:label xml:lang="en">Operational unavailability type</rdfs:label>
    </owl:Class>



    <!-- https://w3id.org/italia/social-security/onto/socialSafetyNet/MotivoDiRinunciaNASpI -->

    <owl:Class rdf:about="https://w3id.org/italia/social-security/onto/socialSafetyNet/MotivoDiRinunciaNASpI">
        <rdfs:comment xml:lang="it">Classifica i motivi per cui un beneficiario debba rinunciare alla Prestazione NASpI. Tra di essi ricade anche la scelta tra più prestazioni incompatibili a cui una stessa persona a diritto come, ad esempio, l&apos;assegno di invalidità rispetto alla NASpI.</rdfs:comment>
        <rdfs:comment xml:lang="en">Classifies the reasons why a beneficiary should opt out of the NASpI Benefit. This also includes the choice between several incompatible benefits to which the same person is entitled, such as, for example, the disability allowance compared to the NASpI.</rdfs:comment>
        <rdfs:label xml:lang="it">Motivo di rinuncia NASpI</rdfs:label>
        <rdfs:label xml:lang="en">NASpI opt-out cause</rdfs:label>
    </owl:Class>



    <!-- https://w3id.org/italia/social-security/onto/socialSafetyNet/MotivoSanzioneNASpI -->

    <owl:Class rdf:about="https://w3id.org/italia/social-security/onto/socialSafetyNet/MotivoSanzioneNASpI">
        <rdfs:comment xml:lang="it">Classifica le motivazioni di una sanzione NASpI per mancato adempimento degli obblighi di attivazione sociale e lavorativa. Tra i motivi ci sono la mancata presentazione ad una iniziativa formativa concordata così come la partecipazione a lavori di pubblica utilità, senza giustificato motivo.</rdfs:comment>
        <rdfs:comment xml:lang="en">Classifies the reasons for a NASpI sanction for failure to comply with social and work activation obligations. Among the reasons are the failure to show up for an agreed training initiative as well as participation in public utility work, without justified reason.</rdfs:comment>
        <rdfs:label xml:lang="it">Motivo sanzione NASpI</rdfs:label>
        <rdfs:label xml:lang="en">NASpI sanction cause</rdfs:label>
    </owl:Class>



    <!-- https://w3id.org/italia/social-security/onto/socialSafetyNet/OggettoVariazioneDelegaSindacale -->

    <owl:Class rdf:about="https://w3id.org/italia/social-security/onto/socialSafetyNet/OggettoVariazioneDelegaSindacale">
        <rdfs:comment xml:lang="en">Classification of the types of variation requests concerning the delegation to INPS for the deduction of membership contributions to trade unions.</rdfs:comment>
        <rdfs:comment xml:lang="it">Classificazione dei tipi di richiesta di variazione riguardante la delega all&apos;INPS per la trattenuta dei contributi associativi alle organizzazioni sindacali.</rdfs:comment>
        <rdfs:label xml:lang="it">Oggetto variazione delega sindacale</rdfs:label>
        <rdfs:label xml:lang="en">Trade union proxy change subject</rdfs:label>
    </owl:Class>



    <!-- https://w3id.org/italia/social-security/onto/socialSafetyNet/OrdineProfessionale -->

    <owl:Class rdf:about="https://w3id.org/italia/social-security/onto/socialSafetyNet/OrdineProfessionale">
        <rdfs:comment xml:lang="en">Establishment of self-government of a liberal profession with functions of qualification, control and supervision of the activities carried out by professionals registered with the order or rather registered in a special register called Professional register. The order also performs disciplinary functions. In Italy, they are autonomous non-economic public bodies, which by law are subject to the supervision of the Ministry of Health for the health professions, while for the professions in the legal, technical and economic areas the supervision is the responsibility of the Ministry of Justice (src. Wikipedia).</rdfs:comment>
        <rdfs:comment xml:lang="it">Istituzione di autogoverno di una libera professione con funzioni di abilitazione, controllo e sorveglianza delle attività svolte dai professionisti iscritti all&apos;ordine ovvero censiti in un apposito registro detto Albo professionale. L&apos;ordine svolge anche funzioni disciplinari. In Italia sono enti pubblici non economici autonomi, che per legge soggiacciono alla vigilanza del Ministero della Salute per le professioni sanitarie, mentre per le professioni delle aree giuridiche, tecniche ed economiche la vigilanza spetta al Ministero della Giustizia (fnt. Wikipedia).</rdfs:comment>
        <rdfs:label xml:lang="it">Ordine professionale</rdfs:label>
        <rdfs:label xml:lang="en">Professional association</rdfs:label>
    </owl:Class>



    <!-- https://w3id.org/italia/social-security/onto/socialSafetyNet/PrestazioneANF -->

    <owl:Class rdf:about="https://w3id.org/italia/social-security/onto/socialSafetyNet/PrestazioneANF">
        <rdfs:subClassOf rdf:resource="https://w3id.org/italia/social-security/onto/socialSafetyNet/PrestazioneDiSostegnoAlReddito"/>
        <rdfs:comment xml:lang="it">L’Assegno per il Nucleo Familiare (ANF) è una prestazione economica erogata dall&apos;INPS ai nuclei familiari di alcune categorie di lavoratori, dei titolari delle pensioni e delle prestazioni economiche previdenziali da lavoro dipendente e dei lavoratori assistiti dall’assicurazione contro la tubercolosi.</rdfs:comment>
        <rdfs:comment xml:lang="en">The Family Unit Allowance (ANF) is an economic benefit provided by INPS to the households of certain categories of workers, holders of pensions and social security benefits from employment and workers assisted by tuberculosis insurance.</rdfs:comment>
        <rdfs:label xml:lang="en">ANF benefit</rdfs:label>
        <rdfs:label xml:lang="it">Prestazione ANF</rdfs:label>
    </owl:Class>



    <!-- https://w3id.org/italia/social-security/onto/socialSafetyNet/PrestazioneDIS-COLL -->

    <owl:Class rdf:about="https://w3id.org/italia/social-security/onto/socialSafetyNet/PrestazioneDIS-COLL">
        <rdfs:subClassOf rdf:resource="https://w3id.org/italia/social-security/onto/socialSafetyNet/PrestazioneDiSostegnoAlReddito"/>
        <rdfs:comment xml:lang="en">Economic benefit provided for parasubordinate workers who have lost their jobs. It is due to workers with a coordinated and continuous collaboration contract, including the project-based contract provided that: they are enrolled exclusively in the separate pension scheme, are not retired, do not have a VAT number.</rdfs:comment>
        <rdfs:comment xml:lang="it">Prestazione economica prevista a favore di lavoratori parasubordinati che abbiano perduto la propria occupazione. Essa spetta ai lavoratori con contratto di collaborazione coordinata e continuativa, anche a progetto purché: siano iscritti in via esclusiva alla Gestione separata, non siano pensionati, non abbiano partita IVA.</rdfs:comment>
        <rdfs:label xml:lang="en">DIS-COLL benefit</rdfs:label>
        <rdfs:label xml:lang="it">Prestazione DIS-COLL</rdfs:label>
    </owl:Class>



    <!-- https://w3id.org/italia/social-security/onto/socialSafetyNet/PrestazioneDiSostegnoAlReddito -->

    <owl:Class rdf:about="https://w3id.org/italia/social-security/onto/socialSafetyNet/PrestazioneDiSostegnoAlReddito">
        <rdfs:comment xml:lang="it">Intervento di tutela nell&apos;ambito del mercato del lavoro volto a garantire un reddito al lavoratore in stato di disoccupazione.</rdfs:comment>
        <rdfs:comment xml:lang="en">Protective intervention in the labour market aimed at guaranteeing an income to the worker in a state of unemployment.</rdfs:comment>
        <rdfs:label xml:lang="en">Income support benefit</rdfs:label>
        <rdfs:label xml:lang="it">Prestazione di sostegno al reddito</rdfs:label>
    </owl:Class>



    <!-- https://w3id.org/italia/social-security/onto/socialSafetyNet/PrestazioneLavorativa -->

    <owl:Class rdf:about="https://w3id.org/italia/social-security/onto/socialSafetyNet/PrestazioneLavorativa">
        <rdfs:subClassOf rdf:resource="https://w3id.org/italia/onto/TI/TimeIndexedEvent"/>
        <rdfs:subClassOf>
            <owl:Restriction>
                <owl:onProperty>
                    <rdf:Description>
                        <owl:inverseOf rdf:resource="https://w3id.org/italia/onto/l0/hasMember"/>
                    </rdf:Description>
                </owl:onProperty>
                <owl:someValuesFrom rdf:resource="https://w3id.org/italia/social-security/onto/socialSafetyNet/RegistroDellaPrestazioneLavorativa"/>
            </owl:Restriction>
        </rdfs:subClassOf>
        <rdfs:comment xml:lang="it">Rappresenta l&apos;evento di erogazione di una singola prestazione lavorativa in un periodo di tempo. Nell&apos;ambito di un contratto di lavoro subordinato il periodo di tempo è la giornata lavorativa così come definita dal contratto.</rdfs:comment>
        <rdfs:comment xml:lang="en">Represents the event of the provision of a single work execution over a period of time. In the context of an Salaried employment contract, the time period is the working day as defined by the contract.</rdfs:comment>
        <rdfs:label xml:lang="it">Prestazione lavorativa</rdfs:label>
        <rdfs:label xml:lang="en">Work provision</rdfs:label>
    </owl:Class>



    <!-- https://w3id.org/italia/social-security/onto/socialSafetyNet/PrestazioneLavorativaEffettiva -->

    <owl:Class rdf:about="https://w3id.org/italia/social-security/onto/socialSafetyNet/PrestazioneLavorativaEffettiva">
        <rdfs:subClassOf rdf:resource="https://w3id.org/italia/social-security/onto/socialSafetyNet/PrestazioneLavorativa"/>
        <owl:disjointWith rdf:resource="https://w3id.org/italia/social-security/onto/socialSafetyNet/PrestazioneLavorativaFigurativa"/>
        <rdfs:comment xml:lang="it">Sottoclasse di Prestazione lavorativa inerente alle prestazioni effettivamente svolte dal lavoratore.</rdfs:comment>
        <rdfs:comment xml:lang="en">Work provision subclass inherent to the provision actually executed by the worker.</rdfs:comment>
        <rdfs:label xml:lang="en">Actual work provision</rdfs:label>
        <rdfs:label xml:lang="it">Prestazione lavorativa effettiva</rdfs:label>
    </owl:Class>



    <!-- https://w3id.org/italia/social-security/onto/socialSafetyNet/PrestazioneLavorativaFigurativa -->

    <owl:Class rdf:about="https://w3id.org/italia/social-security/onto/socialSafetyNet/PrestazioneLavorativaFigurativa">
        <rdfs:subClassOf rdf:resource="https://w3id.org/italia/social-security/onto/socialSafetyNet/PrestazioneLavorativa"/>
        <rdfs:subClassOf>
            <owl:Restriction>
                <owl:onProperty rdf:resource="https://w3id.org/italia/social-security/onto/socialSafetyNet/haMotivoDiIndisponibilitàOperativa"/>
                <owl:someValuesFrom rdf:resource="http://www.w3.org/2002/07/owl#Thing"/>
            </owl:Restriction>
        </rdfs:subClassOf>
        <rdfs:comment xml:lang="it">Sottoclasse di Prestazione lavorativa inerente alle assenze retribuite previste dal contratto di lavoro. In questo senso la prestazione è comunque riconosciuta e quindi retribuita anche se non vi è stato un adempimento di lavoro.</rdfs:comment>
        <rdfs:comment xml:lang="en">Work provision subclass relating to paid absences provided for in the Work contract. In this sense, the provision is in any case recognized and therefore paid even if there has been no fulfilment of work.</rdfs:comment>
        <rdfs:label xml:lang="en">Figurative work provision</rdfs:label>
        <rdfs:label xml:lang="it">Prestazione lavorativa figurativa</rdfs:label>
    </owl:Class>



    <!-- https://w3id.org/italia/social-security/onto/socialSafetyNet/PrestazioneNASpI -->

    <owl:Class rdf:about="https://w3id.org/italia/social-security/onto/socialSafetyNet/PrestazioneNASpI">
        <rdfs:subClassOf rdf:resource="https://w3id.org/italia/social-security/onto/socialSafetyNet/PrestazioneDiSostegnoAlReddito"/>
        <rdfs:subClassOf>
            <owl:Restriction>
                <owl:onProperty rdf:resource="https://w3id.org/italia/social-security/onto/socialSafetyNet/haDomandaNASpI"/>
                <owl:someValuesFrom rdf:resource="http://www.w3.org/2002/07/owl#Thing"/>
            </owl:Restriction>
        </rdfs:subClassOf>
        <rdfs:subClassOf>
            <owl:Restriction>
                <owl:onProperty rdf:resource="https://w3id.org/italia/social-security/onto/socialSafetyNet/haIscrizioneUfficioDelLavoro"/>
                <owl:someValuesFrom rdf:resource="http://www.w3.org/2002/07/owl#Thing"/>
            </owl:Restriction>
        </rdfs:subClassOf>
        <rdfs:subClassOf>
            <owl:Restriction>
                <owl:onProperty rdf:resource="https://w3id.org/italia/social-security/onto/socialSafetyNet/haStatoDiPrestazioneNASpI"/>
                <owl:someValuesFrom rdf:resource="http://www.w3.org/2002/07/owl#Thing"/>
            </owl:Restriction>
        </rdfs:subClassOf>
        <rdfs:subClassOf>
            <owl:Restriction>
                <owl:onProperty rdf:resource="https://w3id.org/italia/social-security/onto/socialSafetyNet/haDomandaNASpI"/>
                <owl:allValuesFrom>
                    <owl:Restriction>
                        <owl:onProperty rdf:resource="https://w3id.org/italia/social-security/onto/socialSafetyNet/haStatoDiDomandaNASpI"/>
                        <owl:someValuesFrom rdf:resource="https://w3id.org/italia/social-security/onto/socialSafetyNet/StatoDiAccoltaDiDomandaNASpI"/>
                    </owl:Restriction>
                </owl:allValuesFrom>
            </owl:Restriction>
        </rdfs:subClassOf>
        <rdfs:subClassOf>
            <owl:Restriction>
                <owl:onProperty rdf:resource="https://w3id.org/italia/social-security/onto/socialSafetyNet/dataInizioPrestazioneNASpI"/>
                <owl:someValuesFrom rdf:resource="http://www.w3.org/2000/01/rdf-schema#Literal"/>
            </owl:Restriction>
        </rdfs:subClassOf>
        <rdfs:subClassOf>
            <owl:Restriction>
                <owl:onProperty rdf:resource="https://w3id.org/italia/social-security/onto/socialSafetyNet/durataTeoricaPrestazioneNASpI"/>
                <owl:someValuesFrom rdf:resource="http://www.w3.org/2000/01/rdf-schema#Literal"/>
            </owl:Restriction>
        </rdfs:subClassOf>
        <rdfs:comment xml:lang="en">Economic benefit in favour of a worker who finds himself in an unemployment status for reasons beyond his control. It is intended for: all salaried employees, apprentices, working members of cooperatives with an salaried employment relationship, fixed-term employees of public administrations, open-ended agricultural workers employed by cooperatives and their consortia. In order for these categories of workers to be eligible for the benefit, the following requirements are required: the worker must have paid contributions for at least thirteen weeks in the four years prior to the start of the unemployment period; the worker&apos;s unemployment status must be involuntary, i.e. it must not be the result of a choice by the worker himself.</rdfs:comment>
        <rdfs:comment xml:lang="it">Prestazione economica a favore del lavoratore che venga a trovarsi in stato di disoccupazione per ragioni che non dipendono dalla sua volontà. Essa è destinata: a tutti i lavoratori subordinati, agli apprendisti, ai soci lavoratori di cooperative con rapporto di lavoro subordinato, ai dipendenti delle pubbliche amministrazioni a tempo determinato, operai agricoli a tempo indeterminato dipendenti da cooperative e loro consorzi. Affinché queste categorie di lavoratori possano accedere al sussidio sono richiesti i seguenti requisiti: il lavoratore deve aver versato nei quattro anni precedenti l’inizio del periodo di disoccupazione contributi per almeno tredici settimane; lo stato di disoccupazione in cui versa il lavoratore deve essere involontario non deve, cioè, essere frutto di una scelta del lavoratore stesso.</rdfs:comment>
        <rdfs:label xml:lang="en">NASpI benefit</rdfs:label>
        <rdfs:label xml:lang="it">Prestazione NASpI</rdfs:label>
    </owl:Class>



    <!-- https://w3id.org/italia/social-security/onto/socialSafetyNet/RapportoDiLavoro -->

    <owl:Class rdf:about="https://w3id.org/italia/social-security/onto/socialSafetyNet/RapportoDiLavoro">
        <rdfs:subClassOf rdf:resource="https://w3id.org/italia/onto/COV/Employment"/>
        <rdfs:subClassOf>
            <owl:Restriction>
                <owl:onProperty rdf:resource="https://w3id.org/italia/onto/CLV/hasAdressinTime"/>
                <owl:someValuesFrom rdf:resource="http://www.w3.org/2002/07/owl#Thing"/>
            </owl:Restriction>
        </rdfs:subClassOf>
        <rdfs:subClassOf>
            <owl:Restriction>
                <owl:onProperty rdf:resource="https://w3id.org/italia/social-security/onto/socialSafetyNet/haStatoDiOccupazione"/>
                <owl:someValuesFrom rdf:resource="http://www.w3.org/2002/07/owl#Thing"/>
            </owl:Restriction>
        </rdfs:subClassOf>
        <rdfs:subClassOf>
            <owl:Restriction>
                <owl:onProperty>
                    <rdf:Description>
                        <owl:inverseOf rdf:resource="https://w3id.org/italia/social-security/onto/socialSafetyNet/forniscePrestazioneLavorativa"/>
                    </rdf:Description>
                </owl:onProperty>
                <owl:someValuesFrom rdf:resource="http://www.w3.org/2002/07/owl#Thing"/>
            </owl:Restriction>
        </rdfs:subClassOf>
        <rdfs:subClassOf>
            <owl:Restriction>
                <owl:onProperty>
                    <rdf:Description>
                        <owl:inverseOf rdf:resource="https://w3id.org/italia/social-security/onto/socialSafetyNet/retribuiscePrestazioneLavorativa"/>
                    </rdf:Description>
                </owl:onProperty>
                <owl:someValuesFrom rdf:resource="http://www.w3.org/2002/07/owl#Thing"/>
            </owl:Restriction>
        </rdfs:subClassOf>
        <rdfs:comment xml:lang="en">It is the legal relationship deriving from a work contract and which binds the owner of the relationship and the worker to the observance of each other&apos;s obligations, the main ones being: for the worker, the provision of the work and, for the holder, the recognition of the agreed remuneration for such service. In order to establish the competent legislation, the work relationship must be located in the territory.</rdfs:comment>
        <rdfs:comment xml:lang="it">È il rapporto giuridico derivante da un contratto di lavoro e che vincola il titolare del rapporto e il lavoratore all&apos;osservanza delle reciproche obbligazioni, le cui principali sono: per il lavoratore, l&apos;erogazione della prestazione lavorativa e, per il titolare, il riconoscimento della retribuzione pattuita per tale prestazione. Al fine di stabilire la legislazione competente, il rapporto di lavoro deve essere localizzato sul territorio.</rdfs:comment>
        <rdfs:label xml:lang="it">Rapporto di lavoro</rdfs:label>
        <rdfs:label xml:lang="en">Work Relationship</rdfs:label>
    </owl:Class>



    <!-- https://w3id.org/italia/social-security/onto/socialSafetyNet/RegistroDellaPrestazioneLavorativa -->

    <owl:Class rdf:about="https://w3id.org/italia/social-security/onto/socialSafetyNet/RegistroDellaPrestazioneLavorativa">
        <rdfs:subClassOf rdf:resource="https://w3id.org/italia/onto/l0/Sequence"/>
        <rdfs:subClassOf>
            <owl:Restriction>
                <owl:onProperty>
                    <rdf:Description>
                        <owl:inverseOf rdf:resource="https://w3id.org/italia/social-security/onto/socialSafetyNet/haRegistroDellaPrestazioneLavorativa"/>
                    </rdf:Description>
                </owl:onProperty>
                <owl:someValuesFrom rdf:resource="http://www.w3.org/2002/07/owl#Thing"/>
            </owl:Restriction>
        </rdfs:subClassOf>
        <rdfs:comment xml:lang="en">Collection of Work provision events. Considering a Salaried employment contract, in this register it is possible to find information regarding the actual and figurative attendance of the Worker.</rdfs:comment>
        <rdfs:comment xml:lang="it">Collezione di eventi di prestazione lavorativa. Considerando un contratto di lavoro subordinato, in tale registro è possibile trovare le informazioni riguardanti le presenze, effettive e figurative, del Lavoratore.</rdfs:comment>
        <rdfs:label xml:lang="it">Registro della prestazione lavorativa</rdfs:label>
        <rdfs:label xml:lang="en">Work provision registry</rdfs:label>
    </owl:Class>



    <!-- https://w3id.org/italia/social-security/onto/socialSafetyNet/RichiedenteNASpI -->

    <owl:Class rdf:about="https://w3id.org/italia/social-security/onto/socialSafetyNet/RichiedenteNASpI">
        <rdfs:subClassOf rdf:resource="https://w3id.org/italia/social-security/onto/socialSafetyNet/Lavoratore"/>
        <rdfs:subClassOf>
            <owl:Restriction>
                <owl:onProperty rdf:resource="https://w3id.org/italia/onto/SM/hasOnlineContactPoint"/>
                <owl:someValuesFrom rdf:resource="http://www.w3.org/2002/07/owl#Thing"/>
            </owl:Restriction>
        </rdfs:subClassOf>
        <rdfs:subClassOf>
            <owl:Restriction>
                <owl:onProperty rdf:resource="https://w3id.org/italia/social-security/onto/socialSafetyNet/haTipoDiQualifica-CategoriaPerNASpI"/>
                <owl:someValuesFrom rdf:resource="http://www.w3.org/2002/07/owl#Thing"/>
            </owl:Restriction>
        </rdfs:subClassOf>
        <rdfs:subClassOf>
            <owl:Restriction>
                <owl:onProperty rdf:resource="https://w3id.org/italia/social-security/onto/socialSafetyNet/haTitoloDiStudio"/>
                <owl:someValuesFrom rdf:resource="http://www.w3.org/2002/07/owl#Thing"/>
            </owl:Restriction>
        </rdfs:subClassOf>
        <rdfs:subClassOf>
            <owl:Restriction>
                <owl:onProperty>
                    <rdf:Description>
                        <owl:inverseOf rdf:resource="https://w3id.org/italia/social-security/onto/socialSafetyNet/haRichiedenteNASpI"/>
                    </rdf:Description>
                </owl:onProperty>
                <owl:someValuesFrom rdf:resource="http://www.w3.org/2002/07/owl#Thing"/>
            </owl:Restriction>
        </rdfs:subClassOf>
        <rdfs:subClassOf>
            <owl:Restriction>
                <owl:onProperty rdf:resource="https://w3id.org/italia/social-security/onto/socialSafetyNet/seIscrittoAlbo-CassaProfessionale"/>
                <owl:someValuesFrom rdf:resource="http://www.w3.org/2000/01/rdf-schema#Literal"/>
            </owl:Restriction>
        </rdfs:subClassOf>
        <rdfs:subClassOf>
            <owl:Restriction>
                <owl:onProperty rdf:resource="https://w3id.org/italia/social-security/onto/socialSafetyNet/seLicenziatoPerSuperamentoPeriodoComporto"/>
                <owl:someValuesFrom rdf:resource="http://www.w3.org/2000/01/rdf-schema#Literal"/>
            </owl:Restriction>
        </rdfs:subClassOf>
        <rdfs:subClassOf>
            <owl:Restriction>
                <owl:onProperty rdf:resource="https://w3id.org/italia/social-security/onto/socialSafetyNet/seSocioDiSocietà"/>
                <owl:someValuesFrom rdf:resource="http://www.w3.org/2000/01/rdf-schema#Literal"/>
            </owl:Restriction>
        </rdfs:subClassOf>
        <rdfs:subClassOf>
            <owl:Restriction>
                <owl:onProperty rdf:resource="https://w3id.org/italia/social-security/onto/socialSafetyNet/seStatoDiMalattiaInCorso"/>
                <owl:someValuesFrom rdf:resource="http://www.w3.org/2000/01/rdf-schema#Literal"/>
            </owl:Restriction>
        </rdfs:subClassOf>
        <rdfs:subClassOf>
            <owl:Restriction>
                <owl:onProperty rdf:resource="https://w3id.org/italia/social-security/onto/socialSafetyNet/seStatoDiMalattiaPregressa"/>
                <owl:someValuesFrom rdf:resource="http://www.w3.org/2000/01/rdf-schema#Literal"/>
            </owl:Restriction>
        </rdfs:subClassOf>
        <rdfs:subClassOf>
            <owl:Restriction>
                <owl:onProperty rdf:resource="https://w3id.org/italia/social-security/onto/socialSafetyNet/seSvolgeAttivitàAPartitaIVA"/>
                <owl:someValuesFrom rdf:resource="http://www.w3.org/2000/01/rdf-schema#Literal"/>
            </owl:Restriction>
        </rdfs:subClassOf>
        <rdfs:subClassOf>
            <owl:Restriction>
                <owl:onProperty rdf:resource="https://w3id.org/italia/social-security/onto/socialSafetyNet/seSvolgeAttivitàProfesionale"/>
                <owl:someValuesFrom rdf:resource="http://www.w3.org/2000/01/rdf-schema#Literal"/>
            </owl:Restriction>
        </rdfs:subClassOf>
        <rdfs:subClassOf>
            <owl:Restriction>
                <owl:onProperty rdf:resource="https://w3id.org/italia/social-security/onto/socialSafetyNet/seTitolareAssegnoDiInvalidità"/>
                <owl:someValuesFrom rdf:resource="http://www.w3.org/2000/01/rdf-schema#Literal"/>
            </owl:Restriction>
        </rdfs:subClassOf>
        <rdfs:subClassOf>
            <owl:Restriction>
                <owl:onProperty rdf:resource="https://w3id.org/italia/social-security/onto/socialSafetyNet/seTitolarePartitaIVA"/>
                <owl:someValuesFrom rdf:resource="http://www.w3.org/2000/01/rdf-schema#Literal"/>
            </owl:Restriction>
        </rdfs:subClassOf>
        <rdfs:comment xml:lang="en">Role of Worker for those who apply for the NASpI benefit. For the submission of the application, the applicant can avail himself of the service of a delegate (Patronato) to whom he gives a specific mandate.</rdfs:comment>
        <rdfs:comment xml:lang="it">Ruolo di Lavoratore riguardante coloro che presentano domanda per fruire della Prestazione NASpI. Per la presentazione della domanda, il richiedente può avvalersi del servizio di un delegato (Patronato) a cui conferisce specifico mandato.</rdfs:comment>
        <rdfs:label xml:lang="en">NASpI Applicant</rdfs:label>
        <rdfs:label xml:lang="it">Richiedente NASpI</rdfs:label>
    </owl:Class>



    <!-- https://w3id.org/italia/social-security/onto/socialSafetyNet/SanzionePerViolazioneObblighiNASpI -->

    <owl:Class rdf:about="https://w3id.org/italia/social-security/onto/socialSafetyNet/SanzionePerViolazioneObblighiNASpI">
        <rdfs:subClassOf>
            <owl:Restriction>
                <owl:onProperty rdf:resource="https://w3id.org/italia/social-security/onto/socialSafetyNet/haMotivoSanzioneNASpI"/>
                <owl:someValuesFrom rdf:resource="http://www.w3.org/2002/07/owl#Thing"/>
            </owl:Restriction>
        </rdfs:subClassOf>
        <rdfs:subClassOf>
            <owl:Restriction>
                <owl:onProperty>
                    <rdf:Description>
                        <owl:inverseOf rdf:resource="https://w3id.org/italia/social-security/onto/socialSafetyNet/haSanzioneNASpI"/>
                    </rdf:Description>
                </owl:onProperty>
                <owl:someValuesFrom rdf:resource="http://www.w3.org/2002/07/owl#Thing"/>
            </owl:Restriction>
        </rdfs:subClassOf>
        <rdfs:subClassOf>
            <owl:Restriction>
                <owl:onProperty rdf:resource="https://w3id.org/italia/social-security/onto/socialSafetyNet/dataValiditàSanzioneNASpI"/>
                <owl:someValuesFrom rdf:resource="http://www.w3.org/2000/01/rdf-schema#Literal"/>
            </owl:Restriction>
        </rdfs:subClassOf>
        <rdfs:subClassOf>
            <owl:Restriction>
                <owl:onProperty rdf:resource="https://w3id.org/italia/social-security/onto/socialSafetyNet/importoSanzioneNASpI"/>
                <owl:someValuesFrom rdf:resource="http://www.w3.org/2000/01/rdf-schema#Literal"/>
            </owl:Restriction>
        </rdfs:subClassOf>
        <rdfs:label xml:lang="en">NASpI Breach Penalty Fee</rdfs:label>
        <rdfs:label xml:lang="it">Sanzione per violazione obblighi NASpI</rdfs:label>
    </owl:Class>



    <!-- https://w3id.org/italia/social-security/onto/socialSafetyNet/StatoCompetente -->

    <owl:Class rdf:about="https://w3id.org/italia/social-security/onto/socialSafetyNet/StatoCompetente">
        <rdfs:subClassOf rdf:resource="https://w3id.org/italia/onto/CLV/Country"/>
        <rdfs:comment xml:lang="en">Group of States in which, in order to safeguard the principle of the free movement of workers, they grant equal rights to mobile workers who move for work or to seek work within those States. At the same time, it is ensured that only one legislation applies to the worker in relation to the obligations and rights arising from his or her status as a worker. From this point of view, the Competent state is one of those whose legislation applies to an individual worker. The general rule indicates that the Competent state is the State in which the worker has his place of work, the State of employment (lex loci laboris), but more complex situations may arise that are appropriately regulated. In addition to the EEA states, it also includes Switzerland.</rdfs:comment>
        <rdfs:comment xml:lang="it">Insieme di Stati in cui al fine di salvaguardare il principio della libera circolazione dei lavoratori riconoscono uguali diritti ai lavoratori mobili che si spostano per lavoro o per cercare lavoro nell&apos;ambito di tali stati. Allo stesso tempo viene garantito che al lavoratore venga applicata una sola legislazione relativamente a obblighi e diritti derivanti dalla sua condizione di lavoratore. In tale ottica lo Stato competente è uno fra questi la cui legislazione è applicata ad un singolo lavoratore. La regola generale indica come Stato competente quello in cui il lavoratore ha il centro della sua attività lavorativa, Stato di occupazione (lex loci laboris), ma possono verificarsi situazioni più complesse che sono opportunamente normate. Oltre agli Stati SEE include anche la Svizzera.</rdfs:comment>
        <rdfs:label xml:lang="en">Competent state</rdfs:label>
        <rdfs:label xml:lang="it">Stato competente</rdfs:label>
    </owl:Class>



    <!-- https://w3id.org/italia/social-security/onto/socialSafetyNet/StatoDiAccoltaDiDomandaNASpI -->

    <owl:Class rdf:about="https://w3id.org/italia/social-security/onto/socialSafetyNet/StatoDiAccoltaDiDomandaNASpI">
        <rdfs:subClassOf rdf:resource="https://w3id.org/italia/social-security/onto/socialSafetyNet/StatoDiDomandaNASpI"/>
        <rdfs:subClassOf>
            <owl:Restriction>
                <owl:onProperty rdf:resource="https://w3id.org/italia/social-security/onto/socialSafetyNet/contribuzioneAntePrestazioniFruite"/>
                <owl:someValuesFrom rdf:resource="http://www.w3.org/2000/01/rdf-schema#Literal"/>
            </owl:Restriction>
        </rdfs:subClassOf>
        <rdfs:subClassOf>
            <owl:Restriction>
                <owl:onProperty rdf:resource="https://w3id.org/italia/social-security/onto/socialSafetyNet/contribuzioneIndisponibile"/>
                <owl:someValuesFrom rdf:resource="http://www.w3.org/2000/01/rdf-schema#Literal"/>
            </owl:Restriction>
        </rdfs:subClassOf>
        <rdfs:subClassOf>
            <owl:Restriction>
                <owl:onProperty rdf:resource="https://w3id.org/italia/social-security/onto/socialSafetyNet/contribuzionePostPrestazioniFruite"/>
                <owl:someValuesFrom rdf:resource="http://www.w3.org/2000/01/rdf-schema#Literal"/>
            </owl:Restriction>
        </rdfs:subClassOf>
        <rdfs:subClassOf>
            <owl:Restriction>
                <owl:onProperty rdf:resource="https://w3id.org/italia/social-security/onto/socialSafetyNet/importoMensileIniziale"/>
                <owl:someValuesFrom rdf:resource="http://www.w3.org/2000/01/rdf-schema#Literal"/>
            </owl:Restriction>
        </rdfs:subClassOf>
        <rdfs:subClassOf>
            <owl:Restriction>
                <owl:onProperty rdf:resource="https://w3id.org/italia/social-security/onto/socialSafetyNet/importoRetribuzioneUtileComplessiva"/>
                <owl:someValuesFrom rdf:resource="http://www.w3.org/2000/01/rdf-schema#Literal"/>
            </owl:Restriction>
        </rdfs:subClassOf>
        <rdfs:subClassOf>
            <owl:Restriction>
                <owl:onProperty rdf:resource="https://w3id.org/italia/social-security/onto/socialSafetyNet/numeroSettimaneLavorate"/>
                <owl:someValuesFrom rdf:resource="http://www.w3.org/2000/01/rdf-schema#Literal"/>
            </owl:Restriction>
        </rdfs:subClassOf>
        <rdfs:comment xml:lang="en">NASpI claim status subclass concerning the accepted applications that qualify for the provision of the NASpI Benefit.</rdfs:comment>
        <rdfs:comment xml:lang="it">Sottoclasse di Stato di Domanda NASpI riguardante le domande accolte che abilitano all&apos;erogazione della Prestazione NASpI.</rdfs:comment>
        <rdfs:label xml:lang="en">NASpI claim acceptance status</rdfs:label>
        <rdfs:label xml:lang="it">Stato di accolta di domanda NASpI</rdfs:label>
    </owl:Class>



    <!-- https://w3id.org/italia/social-security/onto/socialSafetyNet/StatoDiBozzaComunicazioneNASpI -->

    <owl:Class rdf:about="https://w3id.org/italia/social-security/onto/socialSafetyNet/StatoDiBozzaComunicazioneNASpI">
        <rdfs:subClassOf rdf:resource="https://w3id.org/italia/social-security/onto/socialSafetyNet/ComunicazioneNASpI"/>
        <rdfs:comment xml:lang="en">NASpI Communication subclass covering incomplete and not yet transmitted communications.</rdfs:comment>
        <rdfs:comment xml:lang="it">Sottoclasse di Comunicazione NASpI riguardante le comunicazioni incomplete e non ancora trasmesse.</rdfs:comment>
        <rdfs:label xml:lang="en">NASpI communication draft status</rdfs:label>
        <rdfs:label xml:lang="it">Stato di bozza comunicazione NASpI</rdfs:label>
    </owl:Class>



    <!-- https://w3id.org/italia/social-security/onto/socialSafetyNet/StatoDiBozzaDiDomandaNASpI -->

    <owl:Class rdf:about="https://w3id.org/italia/social-security/onto/socialSafetyNet/StatoDiBozzaDiDomandaNASpI">
        <rdfs:subClassOf rdf:resource="https://w3id.org/italia/social-security/onto/socialSafetyNet/StatoDiDomandaNASpI"/>
        <rdfs:comment xml:lang="en">NASpI claim status subclass covering incomplete and not yet submitted applications.</rdfs:comment>
        <rdfs:comment xml:lang="it">Sottoclasse di Stato di Domanda NASpI riguardante le domande incomplete e non ancora trasmesse.</rdfs:comment>
        <rdfs:label xml:lang="en">NASpI claim draft status</rdfs:label>
        <rdfs:label xml:lang="it">Stato di bozza di domanda NASpI</rdfs:label>
    </owl:Class>



    <!-- https://w3id.org/italia/social-security/onto/socialSafetyNet/StatoDiCessatoDiNASpI -->

    <owl:Class rdf:about="https://w3id.org/italia/social-security/onto/socialSafetyNet/StatoDiCessatoDiNASpI">
        <rdfs:subClassOf rdf:resource="https://w3id.org/italia/social-security/onto/socialSafetyNet/StatoDiPrestazioneNASpI"/>
        <rdfs:comment xml:lang="en">NASpI benefit status subclass that classifies natural benefit termination events.</rdfs:comment>
        <rdfs:comment xml:lang="it">Sottoclasse di Stato di prestazione NASpI che classifica gli eventi di terminazione naturale della prestazione.</rdfs:comment>
        <rdfs:label xml:lang="en">NASpI ended status</rdfs:label>
        <rdfs:label xml:lang="it">Stato di cessato di NASpI</rdfs:label>
    </owl:Class>



    <!-- https://w3id.org/italia/social-security/onto/socialSafetyNet/StatoDiDecadutoDiNASpI -->

    <owl:Class rdf:about="https://w3id.org/italia/social-security/onto/socialSafetyNet/StatoDiDecadutoDiNASpI">
        <rdfs:subClassOf rdf:resource="https://w3id.org/italia/social-security/onto/socialSafetyNet/StatoDiPrestazioneNASpI"/>
        <rdfs:comment xml:lang="en">NASpI benefit status subclass that classifies benefit decay events in advance of its natural expiry.</rdfs:comment>
        <rdfs:comment xml:lang="it">Sottoclasse di Stato di prestazione NASpI che classifica gli eventi di decadimento della prestazione in modo anticipato rispetto alla sua naturale scadenza.</rdfs:comment>
        <rdfs:label xml:lang="en">NASpI forfeiture status</rdfs:label>
        <rdfs:label xml:lang="it">Stato di decaduto di NASpI</rdfs:label>
    </owl:Class>



    <!-- https://w3id.org/italia/social-security/onto/socialSafetyNet/StatoDiDisoccupazione -->

    <owl:Class rdf:about="https://w3id.org/italia/social-security/onto/socialSafetyNet/StatoDiDisoccupazione">
        <rdfs:subClassOf rdf:resource="https://w3id.org/italia/social-security/onto/socialSafetyNet/StatoDiLavoro"/>
        <rdfs:subClassOf>
            <owl:Class>
                <owl:unionOf rdf:parseType="Collection">
                    <rdf:Description rdf:about="https://w3id.org/italia/social-security/onto/socialSafetyNet/StatoDiDisoccupazioneInvolontaria"/>
                    <rdf:Description rdf:about="https://w3id.org/italia/social-security/onto/socialSafetyNet/StatoDiDisoccupazioneVolontaria"/>
                </owl:unionOf>
            </owl:Class>
        </rdfs:subClassOf>
        <rdfs:subClassOf>
            <owl:Class>
                <owl:unionOf rdf:parseType="Collection">
                    <rdf:Description rdf:about="https://w3id.org/italia/social-security/onto/socialSafetyNet/StatoDiDisoccupazioneParziale"/>
                    <rdf:Description rdf:about="https://w3id.org/italia/social-security/onto/socialSafetyNet/StatoDiDisoccupazioneTotale"/>
                </owl:unionOf>
            </owl:Class>
        </rdfs:subClassOf>
        <rdfs:comment xml:lang="it">Sottoclasse di Stato di lavoro che comprende le istanze riguardanti periodi di tempo in cui un lavoratore che ha interrotto un rapporto di lavoro è alla ricerca di un nuovo rapporto di lavoro.</rdfs:comment>
        <rdfs:comment xml:lang="en">Working status subclass that includes instances concerning periods of time in which a worker who has terminated a work relationship is seeking another one.</rdfs:comment>
        <rdfs:label xml:lang="it">Stato di disoccupazione</rdfs:label>
        <rdfs:label xml:lang="en">Unemployment status</rdfs:label>
    </owl:Class>



    <!-- https://w3id.org/italia/social-security/onto/socialSafetyNet/StatoDiDisoccupazioneInvolontaria -->

    <owl:Class rdf:about="https://w3id.org/italia/social-security/onto/socialSafetyNet/StatoDiDisoccupazioneInvolontaria">
        <rdfs:subClassOf rdf:resource="https://w3id.org/italia/social-security/onto/socialSafetyNet/StatoDiDisoccupazione"/>
        <owl:disjointWith rdf:resource="https://w3id.org/italia/social-security/onto/socialSafetyNet/StatoDiDisoccupazioneVolontaria"/>
        <rdfs:comment xml:lang="it">Sottoclasse di Stato di disoccupazione che comprende i casi in cui il precedente Stato di occupazione si è concluso per motivi indipendenti dalla volontà del lavoratore. Rientra in questa casistica anche la fine di un rapporto di lavoro a tempo determinato.</rdfs:comment>
        <rdfs:comment xml:lang="en">Unemployment status subclass that includes cases in which the previous Employment status ended for reasons beyond the worker&apos;s control. This also includes the termination of a fixed-term employment relationship.</rdfs:comment>
        <rdfs:label xml:lang="en">Involuntary unemployment status</rdfs:label>
        <rdfs:label xml:lang="it">Stato di disoccupazione involontaria</rdfs:label>
    </owl:Class>



    <!-- https://w3id.org/italia/social-security/onto/socialSafetyNet/StatoDiDisoccupazioneParziale -->

    <owl:Class rdf:about="https://w3id.org/italia/social-security/onto/socialSafetyNet/StatoDiDisoccupazioneParziale">
        <rdfs:subClassOf rdf:resource="https://w3id.org/italia/social-security/onto/socialSafetyNet/StatoDiDisoccupazione"/>
        <rdfs:subClassOf>
            <owl:Restriction>
                <owl:onProperty>
                    <rdf:Description>
                        <owl:inverseOf rdf:resource="https://w3id.org/italia/social-security/onto/socialSafetyNet/haStatoDiOccupazione"/>
                    </rdf:Description>
                </owl:onProperty>
                <owl:someValuesFrom rdf:resource="http://www.w3.org/2002/07/owl#Thing"/>
            </owl:Restriction>
        </rdfs:subClassOf>
        <owl:disjointWith rdf:resource="https://w3id.org/italia/social-security/onto/socialSafetyNet/StatoDiDisoccupazioneTotale"/>
        <rdfs:comment xml:lang="it">Sottoclasse di Stato di disoccupazione che comprende i casi in cui il lavoratore, pur avendo un rapporto di lavoro, il suo reddito è inferiore al reddito minimo escluso da tassazione o il tempo effettivo di occupazione è inferiore al limite stabilito dalla legge.</rdfs:comment>
        <rdfs:comment xml:lang="en">Unemployment status subclass that includes cases in which the worker, despite having a work relationship, his income is less than the minimum income excluded from taxation or the actual time of employment is less than the limit established by law.</rdfs:comment>
        <rdfs:label xml:lang="en">Partial unemployment status</rdfs:label>
        <rdfs:label xml:lang="it">Stato di disoccupazione parziale</rdfs:label>
    </owl:Class>



    <!-- https://w3id.org/italia/social-security/onto/socialSafetyNet/StatoDiDisoccupazioneTotale -->

    <owl:Class rdf:about="https://w3id.org/italia/social-security/onto/socialSafetyNet/StatoDiDisoccupazioneTotale">
        <rdfs:subClassOf rdf:resource="https://w3id.org/italia/social-security/onto/socialSafetyNet/StatoDiDisoccupazione"/>
        <rdfs:comment xml:lang="it">Sottoclasse di Stato di disoccupazione che comprende i casi in cui il lavoratore non ha alcun rapporto di lavoro nel periodo di tempo.</rdfs:comment>
        <rdfs:comment xml:lang="en">Unemployment status subclass which includes cases where the worker has no work relationship in the time period.</rdfs:comment>
        <rdfs:label xml:lang="it">Stato di disoccupazione totale</rdfs:label>
        <rdfs:label xml:lang="en">Total unemployment status</rdfs:label>
    </owl:Class>



    <!-- https://w3id.org/italia/social-security/onto/socialSafetyNet/StatoDiDisoccupazioneVolontaria -->

    <owl:Class rdf:about="https://w3id.org/italia/social-security/onto/socialSafetyNet/StatoDiDisoccupazioneVolontaria">
        <rdfs:subClassOf rdf:resource="https://w3id.org/italia/social-security/onto/socialSafetyNet/StatoDiDisoccupazione"/>
        <rdfs:comment xml:lang="it">Sottoclasse di Stato di disoccupazione che comprende i casi in cui il precedente Stato di occupazione si è concluso per volontà del lavoratore, ad esempio, per dimissioni o risoluzione consensuale, al netto di particolari casi indicati dalla normativa.</rdfs:comment>
        <rdfs:comment xml:lang="en">Unemployment status subclass that includes cases in which the previous State of employment ended by the will of the worker, for example, by resignation or consensual termination, net of particular cases indicated by the law.</rdfs:comment>
        <rdfs:label xml:lang="it">Stato di disoccupazione volontaria</rdfs:label>
        <rdfs:label xml:lang="en">Voluntary unemployment status</rdfs:label>
    </owl:Class>



    <!-- https://w3id.org/italia/social-security/onto/socialSafetyNet/StatoDiDomandaNASpI -->

    <owl:Class rdf:about="https://w3id.org/italia/social-security/onto/socialSafetyNet/StatoDiDomandaNASpI">
        <rdfs:subClassOf rdf:resource="https://w3id.org/italia/onto/TI/TimeIndexedEvent"/>
        <rdfs:subClassOf>
            <owl:Restriction>
                <owl:onProperty>
                    <rdf:Description>
                        <owl:inverseOf rdf:resource="https://w3id.org/italia/social-security/onto/socialSafetyNet/haStatoDiDomandaNASpI"/>
                    </rdf:Description>
                </owl:onProperty>
                <owl:someValuesFrom rdf:resource="http://www.w3.org/2002/07/owl#Thing"/>
            </owl:Restriction>
        </rdfs:subClassOf>
        <rdfs:subClassOf>
            <owl:Restriction>
                <owl:onProperty rdf:resource="https://w3id.org/italia/social-security/onto/socialSafetyNet/dataPresentazioneNASpI"/>
                <owl:someValuesFrom rdf:resource="http://www.w3.org/2000/01/rdf-schema#Literal"/>
            </owl:Restriction>
        </rdfs:subClassOf>
        <rdfs:subClassOf>
            <owl:Restriction>
                <owl:onProperty rdf:resource="https://w3id.org/italia/social-security/onto/socialSafetyNet/numeroDomusNASpI"/>
                <owl:someValuesFrom rdf:resource="http://www.w3.org/2000/01/rdf-schema#Literal"/>
            </owl:Restriction>
        </rdfs:subClassOf>
        <rdfs:comment xml:lang="en">A class of events that express the life cycle of a NASpI claim over time.</rdfs:comment>
        <rdfs:comment xml:lang="it">Classe degli eventi che esprimono nel tempo il ciclo di vita di una Domanda NASpI.</rdfs:comment>
        <rdfs:label xml:lang="en">NASpI claim status</rdfs:label>
        <rdfs:label xml:lang="it">Stato di domanda NASpI</rdfs:label>
    </owl:Class>



    <!-- https://w3id.org/italia/social-security/onto/socialSafetyNet/StatoDiErogatoDiNASpI -->

    <owl:Class rdf:about="https://w3id.org/italia/social-security/onto/socialSafetyNet/StatoDiErogatoDiNASpI">
        <rdfs:subClassOf rdf:resource="https://w3id.org/italia/social-security/onto/socialSafetyNet/StatoDiPrestazioneNASpI"/>
        <rdfs:subClassOf>
            <owl:Restriction>
                <owl:onProperty rdf:resource="https://w3id.org/italia/social-security/onto/socialSafetyNet/importoLordoMensileIndennitàNASpI"/>
                <owl:someValuesFrom rdf:resource="http://www.w3.org/2000/01/rdf-schema#Literal"/>
            </owl:Restriction>
        </rdfs:subClassOf>
        <rdfs:comment xml:lang="en">NASpI benefit Status subclass that classifies events that occur during the delivery of a NASpI benefit. The update of the monthly amount of the benefit is considered a new event (from the fourth month of disbursement, the indemnity is reduced by 3% per month).</rdfs:comment>
        <rdfs:comment xml:lang="it">Sottoclasse di Stato di prestazione NASpI che classifica gli eventi che accadono durante l&apos;erogazione di una Prestazione NASpI. L&apos;aggiornamento dell&apos;importo mensile della prestazione è considerato un nuovo evento.</rdfs:comment>
        <rdfs:label xml:lang="en">NASpI disbursement status</rdfs:label>
        <rdfs:label xml:lang="it">Stato di erogato di NASpI</rdfs:label>
    </owl:Class>



    <!-- https://w3id.org/italia/social-security/onto/socialSafetyNet/StatoDiErogatoInEspatrioDiNASpI -->

    <owl:Class rdf:about="https://w3id.org/italia/social-security/onto/socialSafetyNet/StatoDiErogatoInEspatrioDiNASpI">
        <rdfs:subClassOf rdf:resource="https://w3id.org/italia/social-security/onto/socialSafetyNet/StatoDiErogatoDiNASpI"/>
        <rdfs:subClassOf>
            <owl:Restriction>
                <owl:onProperty rdf:resource="https://w3id.org/italia/social-security/onto/socialSafetyNet/haIndirizzoInEspatrio"/>
                <owl:someValuesFrom rdf:resource="http://www.w3.org/2002/07/owl#Thing"/>
            </owl:Restriction>
        </rdfs:subClassOf>
        <rdfs:label xml:lang="it">Stato di erogato in espatrio di NASpI</rdfs:label>
    </owl:Class>



    <!-- https://w3id.org/italia/social-security/onto/socialSafetyNet/StatoDiInoccupazione -->

    <owl:Class rdf:about="https://w3id.org/italia/social-security/onto/socialSafetyNet/StatoDiInoccupazione">
        <rdfs:subClassOf rdf:resource="https://w3id.org/italia/social-security/onto/socialSafetyNet/StatoDiLavoro"/>
        <rdfs:comment xml:lang="en">A subclass of employment status that includes instances concerning periods of time in which a worker is seeking his or her first work relationship.</rdfs:comment>
        <rdfs:comment xml:lang="it">Sottoclasse di Stato di lavoro che comprende le istanze riguardanti periodi di tempo in cui un lavoratore è alla ricerca del suo primo rapporto di lavoro.</rdfs:comment>
        <rdfs:label xml:lang="en">First-time jobseeker status</rdfs:label>
        <rdfs:label xml:lang="it">Stato di inoccupazione</rdfs:label>
    </owl:Class>



    <!-- https://w3id.org/italia/social-security/onto/socialSafetyNet/StatoDiIntegrazioneDiDomandaNASpI -->

    <owl:Class rdf:about="https://w3id.org/italia/social-security/onto/socialSafetyNet/StatoDiIntegrazioneDiDomandaNASpI">
        <rdfs:subClassOf rdf:resource="https://w3id.org/italia/social-security/onto/socialSafetyNet/StatoDiDomandaNASpI"/>
        <rdfs:comment xml:lang="en">NASpI claim status subclass concerning applications submitted but on which a supplement has been requested from the applicant.</rdfs:comment>
        <rdfs:comment xml:lang="it">Sottoclasse di Stato di Domanda NASpI riguardante le domande trasmesse ma sulle quali è stata richiesta una integrazione al richiedente.</rdfs:comment>
        <rdfs:label xml:lang="en">NASpI claim integration status</rdfs:label>
        <rdfs:label xml:lang="it">Stato di integrazione di domanda NASpI</rdfs:label>
    </owl:Class>



    <!-- https://w3id.org/italia/social-security/onto/socialSafetyNet/StatoDiLavoro -->

    <owl:Class rdf:about="https://w3id.org/italia/social-security/onto/socialSafetyNet/StatoDiLavoro">
        <rdfs:subClassOf rdf:resource="https://w3id.org/italia/onto/TI/TimeIndexedEvent"/>
        <rdfs:subClassOf>
            <owl:Restriction>
                <owl:onProperty rdf:resource="https://w3id.org/italia/social-security/onto/socialSafetyNet/haStatoCompetente"/>
                <owl:someValuesFrom rdf:resource="http://www.w3.org/2002/07/owl#Thing"/>
            </owl:Restriction>
        </rdfs:subClassOf>
        <rdfs:subClassOf>
            <owl:Restriction>
                <owl:onProperty>
                    <rdf:Description>
                        <owl:inverseOf rdf:resource="https://w3id.org/italia/onto/l0/hasMember"/>
                    </rdf:Description>
                </owl:onProperty>
                <owl:someValuesFrom rdf:resource="https://w3id.org/italia/social-security/onto/socialSafetyNet/FascicoloDiLavoro"/>
            </owl:Restriction>
        </rdfs:subClassOf>
        <rdfs:subClassOf>
            <owl:Restriction>
                <owl:onProperty>
                    <rdf:Description>
                        <owl:inverseOf rdf:resource="https://w3id.org/italia/social-security/onto/socialSafetyNet/haStatoDiLavoro"/>
                    </rdf:Description>
                </owl:onProperty>
                <owl:someValuesFrom rdf:resource="http://www.w3.org/2002/07/owl#Thing"/>
            </owl:Restriction>
        </rdfs:subClassOf>
        <rdfs:comment xml:lang="en">Class of events that express the employment status of a Worker over time.</rdfs:comment>
        <rdfs:comment xml:lang="it">Classe degli eventi che esprimono nel tempo la condizione occupazionale di un lavoratore. </rdfs:comment>
        <rdfs:label xml:lang="it">Stato di lavoro</rdfs:label>
        <rdfs:label xml:lang="en">Working status</rdfs:label>
    </owl:Class>



    <!-- https://w3id.org/italia/social-security/onto/socialSafetyNet/StatoDiOccupazione -->

    <owl:Class rdf:about="https://w3id.org/italia/social-security/onto/socialSafetyNet/StatoDiOccupazione">
        <rdfs:subClassOf rdf:resource="https://w3id.org/italia/social-security/onto/socialSafetyNet/StatoDiLavoro"/>
        <rdfs:subClassOf>
            <owl:Restriction>
                <owl:onProperty>
                    <rdf:Description>
                        <owl:inverseOf rdf:resource="https://w3id.org/italia/social-security/onto/socialSafetyNet/haStatoDiOccupazione"/>
                    </rdf:Description>
                </owl:onProperty>
                <owl:someValuesFrom rdf:resource="http://www.w3.org/2002/07/owl#Thing"/>
            </owl:Restriction>
        </rdfs:subClassOf>
        <rdfs:comment xml:lang="it">Sottoclasse di Stato di lavoro che comprende le istanze riguardanti periodi di tempo in cui un lavoratore è occupato ovvero ha un rapporto di lavoro assoggettato ad una legislazione competente.</rdfs:comment>
        <rdfs:comment xml:lang="en">Working status subclass that includes instances relating to periods of time in which a worker is engaged or has a work relationship subject to a competent legislation.</rdfs:comment>
        <rdfs:label xml:lang="en">Employments status</rdfs:label>
        <rdfs:label xml:lang="it">Stato di occupazione</rdfs:label>
    </owl:Class>



    <!-- https://w3id.org/italia/social-security/onto/socialSafetyNet/StatoDiPrestazioneNASpI -->

    <owl:Class rdf:about="https://w3id.org/italia/social-security/onto/socialSafetyNet/StatoDiPrestazioneNASpI">
        <rdfs:subClassOf rdf:resource="https://w3id.org/italia/onto/TI/TimeIndexedEvent"/>
        <rdfs:subClassOf>
            <owl:Restriction>
                <owl:onProperty>
                    <rdf:Description>
                        <owl:inverseOf rdf:resource="https://w3id.org/italia/social-security/onto/socialSafetyNet/haStatoDiPrestazioneNASpI"/>
                    </rdf:Description>
                </owl:onProperty>
                <owl:someValuesFrom rdf:resource="http://www.w3.org/2002/07/owl#Thing"/>
            </owl:Restriction>
        </rdfs:subClassOf>
        <rdfs:comment xml:lang="en">Class of events that express the life cycle of a NASpI Performance over time.</rdfs:comment>
        <rdfs:comment xml:lang="it">Classe degli eventi che esprimono nel tempo il ciclo di vita di una Prestazione NASpI.</rdfs:comment>
        <rdfs:label xml:lang="en">NASpI benefit status</rdfs:label>
        <rdfs:label xml:lang="it">Stato di prestazione NASpI</rdfs:label>
    </owl:Class>



    <!-- https://w3id.org/italia/social-security/onto/socialSafetyNet/StatoDiProtocollataDiDomandaNASpI -->

    <owl:Class rdf:about="https://w3id.org/italia/social-security/onto/socialSafetyNet/StatoDiProtocollataDiDomandaNASpI">
        <rdfs:subClassOf rdf:resource="https://w3id.org/italia/social-security/onto/socialSafetyNet/StatoDiDomandaNASpI"/>
        <rdfs:subClassOf>
            <owl:Restriction>
                <owl:onProperty rdf:resource="https://w3id.org/italia/social-security/onto/socialSafetyNet/numeroProtocolloNASpI"/>
                <owl:someValuesFrom rdf:resource="http://www.w3.org/2000/01/rdf-schema#Literal"/>
            </owl:Restriction>
        </rdfs:subClassOf>
        <rdfs:comment xml:lang="en">NASpI claim status subclass concerning submitted applications. A receipt protocol is assigned to the application. In this state, you can print the application and its receipt.</rdfs:comment>
        <rdfs:comment xml:lang="it">Sottoclasse di Stato di Domanda NASpI riguardante le domande trasmesse. Alla domanda viene assegnato un protocollo di avvenuta ricezione. In questo stato è possibile stampare la domanda e la sua ricevuta.</rdfs:comment>
        <rdfs:label xml:lang="en">NASpI claim registered status</rdfs:label>
        <rdfs:label xml:lang="it">Stato di protocollata di domanda NASpI</rdfs:label>
    </owl:Class>



    <!-- https://w3id.org/italia/social-security/onto/socialSafetyNet/StatoDiRicorsoDiDomandaNASpI -->

    <owl:Class rdf:about="https://w3id.org/italia/social-security/onto/socialSafetyNet/StatoDiRicorsoDiDomandaNASpI">
        <rdfs:subClassOf rdf:resource="https://w3id.org/italia/social-security/onto/socialSafetyNet/StatoDiDomandaNASpI"/>
        <rdfs:subClassOf>
            <owl:Restriction>
                <owl:onProperty rdf:resource="https://w3id.org/italia/social-security/onto/socialSafetyNet/haAttoDiRicorsoDomandaNASpI"/>
                <owl:someValuesFrom rdf:resource="http://www.w3.org/2002/07/owl#Thing"/>
            </owl:Restriction>
        </rdfs:subClassOf>
        <rdfs:comment xml:lang="en">NASpI claim status subclass concerning applications rejected for not meeting the requirements and to which the applicant has submitted an appeal application.</rdfs:comment>
        <rdfs:comment xml:lang="it">Sottoclasse di Stato di Domanda NASpI riguardante le domande respinte per non possesso dei requisiti previsti e verso cui il richiedente ha inoltrato domanda di ricorso.</rdfs:comment>
        <rdfs:label xml:lang="en">NASpI claim appeal status</rdfs:label>
        <rdfs:label xml:lang="it">Stato di ricorso di domanda NASpI</rdfs:label>
    </owl:Class>



    <!-- https://w3id.org/italia/social-security/onto/socialSafetyNet/StatoDiRiesameDiDomandaNASpI -->

    <owl:Class rdf:about="https://w3id.org/italia/social-security/onto/socialSafetyNet/StatoDiRiesameDiDomandaNASpI">
        <rdfs:subClassOf rdf:resource="https://w3id.org/italia/social-security/onto/socialSafetyNet/StatoDiDomandaNASpI"/>
        <rdfs:subClassOf>
            <owl:Restriction>
                <owl:onProperty rdf:resource="https://w3id.org/italia/social-security/onto/socialSafetyNet/haAttoDiRiesameDomandaNASpI"/>
                <owl:someValuesFrom rdf:resource="http://www.w3.org/2002/07/owl#Thing"/>
            </owl:Restriction>
        </rdfs:subClassOf>
        <rdfs:comment xml:lang="en">NASpI Application Status subclass covering applications rejected for lack of documentation and to which the applicant has submitted a request for review.</rdfs:comment>
        <rdfs:comment xml:lang="it">Sottoclasse di Stato di Domanda NASpI riguardante le domande respinte per mancanza di documentazione e verso cui il richiedente ha inoltrato domanda di riesame.</rdfs:comment>
        <rdfs:label xml:lang="en">NASpI claim review status</rdfs:label>
        <rdfs:label xml:lang="it">Stato di riesame di domanda NASpI</rdfs:label>
    </owl:Class>



    <!-- https://w3id.org/italia/social-security/onto/socialSafetyNet/StatoDiRifiutataDiDomandaNASpI -->

    <owl:Class rdf:about="https://w3id.org/italia/social-security/onto/socialSafetyNet/StatoDiRifiutataDiDomandaNASpI">
        <rdfs:subClassOf rdf:resource="https://w3id.org/italia/social-security/onto/socialSafetyNet/StatoDiDomandaNASpI"/>
        <rdfs:comment xml:lang="en">NASpI claim status subclass covering unaccepted applications.</rdfs:comment>
        <rdfs:comment xml:lang="it">Sottoclasse di Stato di Domanda NASpI riguardante le domande respinte.</rdfs:comment>
        <rdfs:label xml:lang="en">NASpI claim rejection status</rdfs:label>
        <rdfs:label xml:lang="it">Stato di rifiutata di domanda NASpI</rdfs:label>
    </owl:Class>



    <!-- https://w3id.org/italia/social-security/onto/socialSafetyNet/StatoDiSospesoDiNASpI -->

    <owl:Class rdf:about="https://w3id.org/italia/social-security/onto/socialSafetyNet/StatoDiSospesoDiNASpI">
        <rdfs:subClassOf rdf:resource="https://w3id.org/italia/social-security/onto/socialSafetyNet/StatoDiPrestazioneNASpI"/>
        <rdfs:comment xml:lang="en">A subclass of NASpI Performance Status that classifies the events of suspension of the benefit in terms of the payment of the allowance.</rdfs:comment>
        <rdfs:comment xml:lang="it">Sottoclasse di Stato di prestazione NASpI che classifica gli eventi di sospensione della prestazione in termini di erogazione dell&apos;indennità.</rdfs:comment>
        <rdfs:label xml:lang="en">NASpI suspended status</rdfs:label>
        <rdfs:label xml:lang="it">Stato di sospeso di NASpI</rdfs:label>
    </owl:Class>



    <!-- https://w3id.org/italia/social-security/onto/socialSafetyNet/StatoMembroUE -->

    <owl:Class rdf:about="https://w3id.org/italia/social-security/onto/socialSafetyNet/StatoMembroUE">
        <rdfs:subClassOf rdf:resource="https://w3id.org/italia/social-security/onto/socialSafetyNet/StatoSEE"/>
        <rdfs:comment xml:lang="en">A country that is part of the European Union.</rdfs:comment>
        <rdfs:comment xml:lang="it">Stato che fa parte dell&apos;Unione Europea.</rdfs:comment>
        <rdfs:label xml:lang="en">EU member state</rdfs:label>
        <rdfs:label xml:lang="it">Stato membro UE</rdfs:label>
    </owl:Class>



    <!-- https://w3id.org/italia/social-security/onto/socialSafetyNet/StatoSEE -->

    <owl:Class rdf:about="https://w3id.org/italia/social-security/onto/socialSafetyNet/StatoSEE">
        <rdfs:subClassOf rdf:resource="https://w3id.org/italia/social-security/onto/socialSafetyNet/StatoCompetente"/>
        <rdfs:comment xml:lang="it">Comprende, oltre agli Stati membri UE. gli stati di Islanda, Liechtenstein e Norvegia che hanno un accordo con la UE per partecipare al Mercato Comune Europeo senza far parte della UE.</rdfs:comment>
        <rdfs:comment xml:lang="en">Includes, in addition to the EU Member States. the states of Iceland, Liechtenstein and Norway that have an agreement with the EU to participate in the European Common Market without being part of the EU.</rdfs:comment>
        <rdfs:label xml:lang="en">EEA Status</rdfs:label>
        <rdfs:label xml:lang="it">Stato SEE</rdfs:label>
    </owl:Class>



    <!-- https://w3id.org/italia/social-security/onto/socialSafetyNet/TipoDiAttivitàAutonoma -->

    <owl:Class rdf:about="https://w3id.org/italia/social-security/onto/socialSafetyNet/TipoDiAttivitàAutonoma">
        <rdfs:comment xml:lang="en">Classification of activities carried out by self-employed persons independently of the economic activities concerned.</rdfs:comment>
        <rdfs:comment xml:lang="it">Classificazione delle attività svolte da lavoratori autonomi in modo indipendente rispetto alle attività economiche interessate.</rdfs:comment>
        <rdfs:label xml:lang="en">Self-employed activity type</rdfs:label>
        <rdfs:label xml:lang="it">Tipo di attività autonoma</rdfs:label>
    </owl:Class>



    <!-- https://w3id.org/italia/social-security/onto/socialSafetyNet/TipoDiAttivitàEconomica -->

    <owl:Class rdf:about="https://w3id.org/italia/social-security/onto/socialSafetyNet/TipoDiAttivitàEconomica">
        <rdfs:comment xml:lang="en">Classification of economic activities (ATECO) established by ISTAT for national economic statistical surveys. It is used by the MEF to attribute the type of activity carried out by a Company or a Self-employed worker.</rdfs:comment>
        <rdfs:comment xml:lang="it">Classificazione delle attività economiche (ATECO) stabilita dell&apos;ISTAT per le rilevazioni statistiche nazionali di carattere economico. La stessa viene utilizzata dal MEF per attribuire la tipologia di attività svolta da un&apos;Impresa o da un Lavoratore autonomo.</rdfs:comment>
        <rdfs:label xml:lang="en">Economic activity type</rdfs:label>
        <rdfs:label xml:lang="it">Tipo di attività economica</rdfs:label>
    </owl:Class>



    <!-- https://w3id.org/italia/social-security/onto/socialSafetyNet/TipoDiCategoria -->

    <owl:Class rdf:about="https://w3id.org/italia/social-security/onto/socialSafetyNet/TipoDiCategoria">
        <rdfs:comment xml:lang="en">Classification of the type of work performed by a Worker based on the signed Work contract.</rdfs:comment>
        <rdfs:comment xml:lang="it">Classificazione della tipologia di lavoro svolto da un Lavoratore sulla base del Contratto di lavoro sottoscritto.</rdfs:comment>
        <rdfs:label xml:lang="en">Category type</rdfs:label>
        <rdfs:label xml:lang="it">Tipo di categoria</rdfs:label>
    </owl:Class>



    <!-- https://w3id.org/italia/social-security/onto/socialSafetyNet/TipoDiComunicazioneNASpI -->

    <owl:Class rdf:about="https://w3id.org/italia/social-security/onto/socialSafetyNet/TipoDiComunicazioneNASpI">
        <rdfs:comment xml:lang="it">Classifica le tipologie di comunicazione NASpI.</rdfs:comment>
        <rdfs:comment xml:lang="en">Classifies the types of NASpI communication.</rdfs:comment>
        <rdfs:label xml:lang="en">NASpI Communication Type</rdfs:label>
        <rdfs:label xml:lang="it">Tipo di comunicazione NASpI</rdfs:label>
    </owl:Class>



    <!-- https://w3id.org/italia/social-security/onto/socialSafetyNet/TipoDiContribuzione -->

    <owl:Class rdf:about="https://w3id.org/italia/social-security/onto/socialSafetyNet/TipoDiContribuzione">
        <rdfs:comment xml:lang="it">Classifica le tipologie di contribuzione in base all&apos;attività o la tipo di evento che ha dato luogo al versamento del contributo nel periodo.</rdfs:comment>
        <rdfs:comment xml:lang="en">Classifies the types of contributions according to the activity or the type of event that gave rise to the payment of the contribution in the period.</rdfs:comment>
        <rdfs:label xml:lang="en">Contribution type</rdfs:label>
        <rdfs:label xml:lang="it">Tipo di contribuzione</rdfs:label>
    </owl:Class>



    <!-- https://w3id.org/italia/social-security/onto/socialSafetyNet/TipoDiModalitàDiPagamentoNASpI -->

    <owl:Class rdf:about="https://w3id.org/italia/social-security/onto/socialSafetyNet/TipoDiModalitàDiPagamentoNASpI">
        <rdfs:comment xml:lang="it">Classifica le modalità di pagamento previste.</rdfs:comment>
        <rdfs:comment xml:lang="en">Classify the payment methods provided.</rdfs:comment>
        <rdfs:label xml:lang="en">NASpI payment method type</rdfs:label>
        <rdfs:label xml:lang="it">Tipo di modalità di pagamento NASPI</rdfs:label>
    </owl:Class>



    <!-- https://w3id.org/italia/social-security/onto/socialSafetyNet/TipoDiProfessione -->

    <owl:Class rdf:about="https://w3id.org/italia/social-security/onto/socialSafetyNet/TipoDiProfessione">
        <rdfs:comment xml:lang="en">Classification of occupations independently of economic activities.</rdfs:comment>
        <rdfs:comment xml:lang="it">Classificazione delle professioni in modo indipendente rispetto alle attività economiche.</rdfs:comment>
        <rdfs:label xml:lang="en">Profession type</rdfs:label>
        <rdfs:label xml:lang="it">Tipo di professione</rdfs:label>
    </owl:Class>



    <!-- https://w3id.org/italia/social-security/onto/socialSafetyNet/TipoDiQualifica -->

    <owl:Class rdf:about="https://w3id.org/italia/social-security/onto/socialSafetyNet/TipoDiQualifica">
        <rdfs:comment xml:lang="en">Classification of the task performed by a Worker within the scope of the signed Work contract.</rdfs:comment>
        <rdfs:comment xml:lang="it">Classificazione della mansione svolta da un Lavoratore nell&apos;ambito del Contratto di lavoro sottoscritto.</rdfs:comment>
        <rdfs:label xml:lang="en">Qualification type</rdfs:label>
        <rdfs:label xml:lang="it">Tipo di qualifica</rdfs:label>
    </owl:Class>



    <!-- https://w3id.org/italia/social-security/onto/socialSafetyNet/TipoDiRapportoDiLavoro -->

    <owl:Class rdf:about="https://w3id.org/italia/social-security/onto/socialSafetyNet/TipoDiRapportoDiLavoro">
        <rdfs:comment xml:lang="it">Classifica le tipologie di rapporto di lavoro in base alla modalità contrattuale adottata.</rdfs:comment>
        <rdfs:comment xml:lang="en">Classifies the types of work relationship according to the contractual method adopted.</rdfs:comment>
        <rdfs:label xml:lang="it">Tipo di rapporto di lavoro</rdfs:label>
        <rdfs:label xml:lang="en">Work relationship type</rdfs:label>
    </owl:Class>



    <!-- https://w3id.org/italia/social-security/onto/socialSafetyNet/TitolareDelRapportoDiLavoro -->

    <owl:Class rdf:about="https://w3id.org/italia/social-security/onto/socialSafetyNet/TitolareDelRapportoDiLavoro">
        <rdfs:subClassOf rdf:resource="https://w3id.org/italia/social-security/onto/core/RuoloDiAgente"/>
        <rdfs:comment xml:lang="en">Role of Agent attributed to those who remunerate, in the context of a Work relationship, a work service provided by a worker.</rdfs:comment>
        <rdfs:comment xml:lang="it">Ruolo di Agente attribuito a chi retribuisce, nell&apos;ambito di un rapporto di lavoro, una prestazione lavorativa erogata da un lavoratore. </rdfs:comment>
        <rdfs:label xml:lang="it">Titolare del rapporto di lavoro</rdfs:label>
        <rdfs:label xml:lang="en">Work relationship rightsholder</rdfs:label>
    </owl:Class>



    <!-- https://w3id.org/italia/social-security/onto/socialSafetyNet/TitoloDiStudio -->

    <owl:Class rdf:about="https://w3id.org/italia/social-security/onto/socialSafetyNet/TitoloDiStudio">
        <rdfs:comment xml:lang="en">Classification of qualifications.</rdfs:comment>
        <rdfs:comment xml:lang="it">Classificazione dei titoli di studio.</rdfs:comment>
        <rdfs:label xml:lang="en">Educational qualification</rdfs:label>
        <rdfs:label xml:lang="it">Titolo di studio</rdfs:label>
    </owl:Class>



    <!-- https://w3id.org/italia/social-security/onto/socialSafetyNet/UfficioDelLavoro -->

    <owl:Class rdf:about="https://w3id.org/italia/social-security/onto/socialSafetyNet/UfficioDelLavoro">
        <rdfs:subClassOf rdf:resource="https://w3id.org/italia/onto/COV/Organization"/>
        <rdfs:comment xml:lang="en">Organization dedicated to guiding citizens in the labour market, facilitating the matching of labour supply and demand, and supporting the unemployed in their search for a new job.</rdfs:comment>
        <rdfs:comment xml:lang="it">Organizzazione dedicata all&apos;orientamento dei cittadini nel mercato del lavoro, a facilitare l&apos;incontro tra domanda e offerta di lavoro, a supportare i disoccupati nella ricerca di un nuovo lavoro.</rdfs:comment>
        <rdfs:label xml:lang="en">Labour office</rdfs:label>
        <rdfs:label xml:lang="it">Ufficio del lavoro</rdfs:label>
    </owl:Class>



    <!-- https://w3id.org/italia/social-security/onto/socialSafetyNet/UfficioDelLavoroEstero -->

    <owl:Class rdf:about="https://w3id.org/italia/social-security/onto/socialSafetyNet/UfficioDelLavoroEstero">
        <rdfs:subClassOf rdf:resource="https://w3id.org/italia/social-security/onto/socialSafetyNet/UfficioDelLavoro"/>
        <rdfs:comment xml:lang="en">Labour office subclass not located in Italy.</rdfs:comment>
        <rdfs:comment xml:lang="it">Sottoclasse di Ufficio del lavoro  non localizzata in Italia.</rdfs:comment>
        <rdfs:label xml:lang="en">Foreign labour office</rdfs:label>
        <rdfs:label xml:lang="it">Ufficio del lavoro estero</rdfs:label>
    </owl:Class>



    <!-- https://w3id.org/italia/social-security/onto/socialSafetyNet/VariazioneDelegaRiscossioneContributiSindacaliNASpI -->

    <owl:Class rdf:about="https://w3id.org/italia/social-security/onto/socialSafetyNet/VariazioneDelegaRiscossioneContributiSindacaliNASpI">
        <rdfs:subClassOf rdf:resource="https://w3id.org/italia/social-security/onto/socialSafetyNet/ComunicazioneVariazioneNASpI"/>
        <rdfs:subClassOf>
            <owl:Restriction>
                <owl:onProperty rdf:resource="https://w3id.org/italia/social-security/onto/socialSafetyNet/haDelegaRiscossionePer"/>
                <owl:someValuesFrom rdf:resource="http://www.w3.org/2002/07/owl#Thing"/>
            </owl:Restriction>
        </rdfs:subClassOf>
        <rdfs:subClassOf>
            <owl:Restriction>
                <owl:onProperty rdf:resource="https://w3id.org/italia/social-security/onto/socialSafetyNet/haOggettoVariazioneDelegaSindacale"/>
                <owl:someValuesFrom rdf:resource="http://www.w3.org/2002/07/owl#Thing"/>
            </owl:Restriction>
        </rdfs:subClassOf>
        <rdfs:comment xml:lang="en">NASpI communication change subclass concerning the variation of the delegation to INPS for the processing of membership contributions to trade unions.</rdfs:comment>
        <rdfs:comment xml:lang="it">Sottoclasse di Comunicazione variazione NASpI riguardante la variazione della delega all&apos;INPS per la trattenuta dei contributi associativi alle organizzazioni sindacali.</rdfs:comment>
        <rdfs:label xml:lang="en">NASpI union contributions collection proxy change</rdfs:label>
        <rdfs:label xml:lang="it">Variazione delega riscossione contributi sindacali NASpI</rdfs:label>
    </owl:Class>



    <!-- https://w3id.org/italia/social-security/onto/socialSafetyNet/VariazioneDomicilioNASpI -->

    <owl:Class rdf:about="https://w3id.org/italia/social-security/onto/socialSafetyNet/VariazioneDomicilioNASpI">
        <rdfs:subClassOf rdf:resource="https://w3id.org/italia/social-security/onto/socialSafetyNet/ComunicazioneVariazioneNASpI"/>
        <rdfs:subClassOf>
            <owl:Restriction>
                <owl:onProperty rdf:resource="https://w3id.org/italia/onto/CLV/hasAddress"/>
                <owl:someValuesFrom rdf:resource="http://www.w3.org/2002/07/owl#Thing"/>
            </owl:Restriction>
        </rdfs:subClassOf>
        <rdfs:comment xml:lang="en">NASpI change communication subclass concerning the change of domicile of the NASpI Beneficiary.</rdfs:comment>
        <rdfs:comment xml:lang="it">Sottoclasse di Comunicazione variazione NASpI riguardante la variazione del domicilio del Beneficiario NASpI.</rdfs:comment>
        <rdfs:label xml:lang="en">NASpI domicile change</rdfs:label>
        <rdfs:label xml:lang="it">Variazione domicilio NASpI</rdfs:label>
    </owl:Class>



    <!-- https://w3id.org/italia/social-security/onto/socialSafetyNet/VariazioneModalitàDiPagamentoNASpI -->

    <owl:Class rdf:about="https://w3id.org/italia/social-security/onto/socialSafetyNet/VariazioneModalitàDiPagamentoNASpI">
        <rdfs:subClassOf rdf:resource="https://w3id.org/italia/social-security/onto/socialSafetyNet/ComunicazioneVariazioneNASpI"/>
        <rdfs:subClassOf>
            <owl:Restriction>
                <owl:onProperty rdf:resource="https://w3id.org/italia/social-security/onto/socialSafetyNet/haModalitàDiPagamentoNASpI"/>
                <owl:someValuesFrom rdf:resource="http://www.w3.org/2002/07/owl#Thing"/>
            </owl:Restriction>
        </rdfs:subClassOf>
        <rdfs:comment xml:lang="en">NASpI change notification subclass concerning the change in the payment method chosen by the NASpI Beneficiary, including the change of the IBAN.</rdfs:comment>
        <rdfs:comment xml:lang="it">Sottoclasse di Comunicazione variazione NASpI riguardante la variazione della modalità di pagamento scelta dal Beneficiario NASpI, compresa la variazione dell&apos;IBAN.</rdfs:comment>
        <rdfs:label xml:lang="en">NASpI payment method change</rdfs:label>
        <rdfs:label xml:lang="it">Variazione modalità di pagamento NASpI</rdfs:label>
    </owl:Class>



    <!-- https://w3id.org/italia/social-security/onto/socialSafetyNet/VariazioneRecapitoNASpI -->

    <owl:Class rdf:about="https://w3id.org/italia/social-security/onto/socialSafetyNet/VariazioneRecapitoNASpI">
        <rdfs:subClassOf rdf:resource="https://w3id.org/italia/social-security/onto/socialSafetyNet/ComunicazioneVariazioneNASpI"/>
        <rdfs:subClassOf>
            <owl:Restriction>
                <owl:onProperty rdf:resource="https://w3id.org/italia/onto/SM/hasOnlineContactPoint"/>
                <owl:someValuesFrom rdf:resource="http://www.w3.org/2002/07/owl#Thing"/>
            </owl:Restriction>
        </rdfs:subClassOf>
        <rdfs:comment xml:lang="en">NASpI change communication concerning the change of contact details (email, telephone, etc.) of the NASpI Beneficiary.</rdfs:comment>
        <rdfs:comment xml:lang="it">Sottoclasse di Comunicazione variazione NASpI riguardante la variazione dei recapiti (email, telefono, etc.) del Beneficiario NASpI.</rdfs:comment>
        <rdfs:label xml:lang="en">NASpI contacts change</rdfs:label>
        <rdfs:label xml:lang="it">Variazione recapito NASpI</rdfs:label>
    </owl:Class>



    <!--
    ///////////////////////////////////////////////////////////////////////////////////////
    //
    // Individuals
    //
    ///////////////////////////////////////////////////////////////////////////////////////
     -->




    <!-- http://w3id.org/italia/controlled-vocabulary/territorial-classifications/countries/iceland/IS -->

    <owl:NamedIndividual rdf:about="http://w3id.org/italia/controlled-vocabulary/territorial-classifications/countries/iceland/IS">
        <rdf:type rdf:resource="https://w3id.org/italia/social-security/onto/socialSafetyNet/StatoSEE"/>
    </owl:NamedIndividual>



    <!-- http://w3id.org/italia/controlled-vocabulary/territorial-classifications/countries/italy/ITA -->

    <owl:NamedIndividual rdf:about="http://w3id.org/italia/controlled-vocabulary/territorial-classifications/countries/italy/ITA">
        <rdf:type rdf:resource="https://w3id.org/italia/social-security/onto/socialSafetyNet/StatoMembroUE"/>
    </owl:NamedIndividual>



    <!-- http://w3id.org/italia/controlled-vocabulary/territorial-classifications/countries/liechtenstein/LI -->

    <owl:NamedIndividual rdf:about="http://w3id.org/italia/controlled-vocabulary/territorial-classifications/countries/liechtenstein/LI">
        <rdf:type rdf:resource="https://w3id.org/italia/social-security/onto/socialSafetyNet/StatoSEE"/>
    </owl:NamedIndividual>



    <!-- http://w3id.org/italia/controlled-vocabulary/territorial-classifications/countries/norway/NO -->

    <owl:NamedIndividual rdf:about="http://w3id.org/italia/controlled-vocabulary/territorial-classifications/countries/norway/NO">
        <rdf:type rdf:resource="https://w3id.org/italia/social-security/onto/socialSafetyNet/StatoSEE"/>
    </owl:NamedIndividual>



    <!-- http://w3id.org/italia/controlled-vocabulary/territorial-classifications/countries/swiss/CH -->

    <owl:NamedIndividual rdf:about="http://w3id.org/italia/controlled-vocabulary/territorial-classifications/countries/swiss/CH">
        <rdf:type rdf:resource="https://w3id.org/italia/social-security/onto/socialSafetyNet/StatoCompetente"/>
    </owl:NamedIndividual>



    <!-- https://w3id.org/italia/controlled-vocabulary/classifications-for-organizations/ateco-2007/A -->

    <owl:NamedIndividual rdf:about="https://w3id.org/italia/controlled-vocabulary/classifications-for-organizations/ateco-2007/A"/>



    <!-- https://w3id.org/italia/social-security/data/organization/DirezioneCentraleTII -->

    <owl:NamedIndividual rdf:about="https://w3id.org/italia/social-security/data/organization/DirezioneCentraleTII">
        <rdf:type rdf:resource="http://dati.gov.it/onto/dcatapit#Organization"/>
        <rdf:type rdf:resource="http://www.w3.org/2006/vcard/ns#Kind"/>
        <rdf:type rdf:resource="http://www.w3.org/2006/vcard/ns#Organization"/>
        <dct:identifier>DirezioneCentraleTII</dct:identifier>
        <vcard:fn>INPS - Direzione Centrale Tecnologia, Informatica e Innovazione</vcard:fn>
        <vcard:hasEmail rdf:resource="mailto:dc.tecnologiainformaticaeinnovazione@postacert.inps.gov.it"/>
        <foaf:name xml:lang="en">INPS - Central Management of Information Technology and Innovations</foaf:name>
        <foaf:name xml:lang="it">INPS - Direzione Centrale Tecnologia, Informatica e Innovazione</foaf:name>
    </owl:NamedIndividual>



    <!-- https://w3id.org/italia/social-security/data/organization/inps -->

    <owl:NamedIndividual rdf:about="https://w3id.org/italia/social-security/data/organization/inps">
        <rdf:type rdf:resource="http://dati.gov.it/onto/dcatapit#Agent"/>
        <rdf:type rdf:resource="http://xmlns.com/foaf/0.1/Agent"/>
        <rdf:type rdf:resource="https://w3id.org/italia/onto/COV/PublicOrganization"/>
        <dct:identifier>inps</dct:identifier>
        <foaf:name xml:lang="it">Istituto nazionale della previdenza sociale</foaf:name>
        <foaf:name xml:lang="en">National institute for Social Security</foaf:name>
    </owl:NamedIndividual>



    <!-- https://w3id.org/italia/social-security/data/organization/td -->

    <owl:NamedIndividual rdf:about="https://w3id.org/italia/social-security/data/organization/td">
        <rdf:type rdf:resource="http://dati.gov.it/onto/dcatapit#Agent"/>
        <rdf:type rdf:resource="http://xmlns.com/foaf/0.1/Agent"/>
        <dct:identifier>TD</dct:identifier>
        <foaf:name xml:lang="en">Digital Transformation Team</foaf:name>
        <foaf:name xml:lang="it">Team per la Trasformazione Digitale</foaf:name>
    </owl:NamedIndividual>



    <!-- https://w3id.org/italia/social-security/data/socialSafetyNet/distribution/SAFETY-N-TRIPLES -->

    <owl:NamedIndividual rdf:about="https://w3id.org/italia/social-security/data/socialSafetyNet/distribution/SAFETY-N-TRIPLES">
        <rdf:type rdf:resource="http://dati.gov.it/onto/dcatapit#Distribution"/>
        <rdf:type rdf:resource="http://www.w3.org/ns/dcat#Distribution"/>
        <rdf:type rdf:resource="https://w3id.org/italia/onto/ADMS/SemanticAssetDistribution"/>
        <dct:description xml:lang="it">Questa è la distribuzione N-TRIPLES dell&apos;ontologia INPS relativa alla NASpI che rappresenta un insieme strutturato di concetti e relazioni che descrivono in modo dettagliato il sistema di indennità di disoccupazione NASpI erogato dall&apos;Istituto Nazionale della Previdenza Sociale (INPS).</dct:description>
        <dct:description xml:lang="en">This is the distribution in N-TRIPLES of the INPS Ontology relating to NASpI which represents a structured set of concepts and relationships that describe in detail the NASpI unemployment benefit system provided by the National Institute of Social Security (INPS).</dct:description>
        <dct:format rdf:resource="http://publications.europa.eu/resource/authority/file-type/RDF_N_TRIPLES"/>
        <dct:license rdf:resource="http://creativecommons.org/licenses/by/4.0/"/>
        <dct:title xml:lang="it">Distribuzione N-TRIPLES dell&apos;ontologia INPS - NASpI</dct:title>
        <dct:title xml:lang="en">N-TRIPLES distribution of the INPS ontology - NASpI</dct:title>
        <dcat:accessURL rdf:resource="https://github.com/INPS-it/NDC/tree/main/assets/ontologies/socialSafetyNet/latest"/>
        <dcat:downloadURL rdf:resource="https://raw.githubusercontent.com/INPS-it/NDC/main/assets/ontologies/socialSafetyNet/latest/socialSafetyNet.n3"/>
    </owl:NamedIndividual>



    <!-- https://w3id.org/italia/social-security/data/socialSafetyNet/distribution/SAFETY-RDF-TURTLE -->

    <owl:NamedIndividual rdf:about="https://w3id.org/italia/social-security/data/socialSafetyNet/distribution/SAFETY-RDF-TURTLE">
        <rdf:type rdf:resource="http://dati.gov.it/onto/dcatapit#Distribution"/>
        <rdf:type rdf:resource="http://www.w3.org/ns/dcat#Distribution"/>
        <rdf:type rdf:resource="https://w3id.org/italia/onto/ADMS/SemanticAssetDistribution"/>
        <dct:description xml:lang="it">Questa è la distribuzione RDF/Turtle dell&apos;ontologia INPS relativa alla NASpI che rappresenta un insieme strutturato di concetti e relazioni che descrivono in modo dettagliato il sistema di indennità di disoccupazione NASpI erogato dall&apos;Istituto Nazionale della Previdenza Sociale (INPS).</dct:description>
        <dct:description xml:lang="en">This is the distribution in RDF/Turtle of the INPS Ontology relating to NASpI which represents a structured set of concepts and relationships that describe in detail the NASpI unemployment benefit system provided by the National Institute of Social Security (INPS).</dct:description>
        <dct:format rdf:resource="http://publications.europa.eu/resource/authority/file-type/RDF_TURTLE"/>
        <dct:license rdf:resource="http://creativecommons.org/licenses/by/4.0/"/>
        <dct:title xml:lang="it">Distribuzione RDF/Turtle dell&apos;ontologia INPS - NASpI</dct:title>
        <dct:title xml:lang="en">RDF/Turtle distribution of the INPS ontology - NASpI</dct:title>
        <dcat:accessURL rdf:resource="https://github.com/INPS-it/NDC/tree/main/assets/ontologies/socialSafetyNet/latest"/>
        <dcat:downloadURL rdf:resource="https://raw.githubusercontent.com/INPS-it/NDC/main/assets/ontologies/socialSafetyNet/latest/socialSafetyNet.ttl"/>
    </owl:NamedIndividual>



    <!-- https://w3id.org/italia/social-security/data/socialSafetyNet/distribution/SAFETY-RDF-XML -->

    <owl:NamedIndividual rdf:about="https://w3id.org/italia/social-security/data/socialSafetyNet/distribution/SAFETY-RDF-XML">
        <rdf:type rdf:resource="http://dati.gov.it/onto/dcatapit#Distribution"/>
        <rdf:type rdf:resource="http://www.w3.org/ns/dcat#Distribution"/>
        <rdf:type rdf:resource="https://w3id.org/italia/onto/ADMS/SemanticAssetDistribution"/>
        <dct:description xml:lang="it">Questa è la distribuzione RDF/XML dell&apos;ontologia INPS relativa alla NASpI che rappresenta un insieme strutturato di concetti e relazioni che descrivono in modo dettagliato il sistema di indennità di disoccupazione NASpI erogato dall&apos;Istituto Nazionale della Previdenza Sociale (INPS).</dct:description>
        <dct:description xml:lang="en">This is the distribution in RDF/XML of the INPS Ontology relating to NASpI which represents a structured set of concepts and relationships that describe in detail the NASpI unemployment benefit system provided by the National Institute of Social Security (INPS).</dct:description>
        <dct:format rdf:resource="http://publications.europa.eu/resource/authority/file-type/RDF_XML"/>
        <dct:license rdf:resource="http://creativecommons.org/licenses/by/4.0/"/>
        <dct:title xml:lang="it">Distribuzione RDF/XML dell&apos;ontologia INPS - NASpI</dct:title>
        <dct:title xml:lang="en">RDF/XML distribution of the INPS ontology - NASpI</dct:title>
        <dcat:accessURL rdf:resource="https://github.com/INPS-it/NDC/tree/main/assets/ontologies/socialSafetyNet/latest"/>
        <dcat:downloadURL rdf:resource="https://raw.githubusercontent.com/INPS-it/NDC/main/assets/ontologies/socialSafetyNet/latest/socialSafetyNet.owl"/>
    </owl:NamedIndividual>



    <!--
    ///////////////////////////////////////////////////////////////////////////////////////
    //
    // General axioms
    //
    ///////////////////////////////////////////////////////////////////////////////////////
     -->

    <owl:Class>
        <owl:intersectionOf rdf:parseType="Collection">
            <rdf:Description rdf:about="https://w3id.org/italia/social-security/onto/socialSafetyNet/ContrattoDiLavoroSubordinato"/>
            <owl:Restriction>
                <owl:onProperty>
                    <rdf:Description>
                        <owl:inverseOf rdf:resource="https://w3id.org/italia/social-security/onto/socialSafetyNet/èRegolatoDaContratto"/>
                    </rdf:Description>
                </owl:onProperty>
                <owl:someValuesFrom rdf:resource="https://w3id.org/italia/social-security/onto/socialSafetyNet/RapportoDiLavoro"/>
            </owl:Restriction>
        </owl:intersectionOf>
        <rdfs:subClassOf>
            <owl:Restriction>
                <owl:onProperty rdf:resource="https://w3id.org/italia/social-security/onto/socialSafetyNet/haRegistroDellaPrestazioneLavorativa"/>
                <owl:someValuesFrom rdf:resource="http://www.w3.org/2002/07/owl#Thing"/>
            </owl:Restriction>
        </rdfs:subClassOf>
    </owl:Class>
    <owl:Class>
        <owl:intersectionOf rdf:parseType="Collection">
            <owl:Restriction>
                <owl:onProperty rdf:resource="https://w3id.org/italia/onto/RO/holdsRoleInTime"/>
                <owl:someValuesFrom rdf:resource="https://w3id.org/italia/social-security/onto/socialSafetyNet/DatoreDiLavoro"/>
            </owl:Restriction>
            <owl:Restriction>
                <owl:onProperty rdf:resource="https://w3id.org/italia/onto/RO/holdsRoleInTime"/>
                <owl:someValuesFrom rdf:resource="https://w3id.org/italia/social-security/onto/socialSafetyNet/ImprenditoreAgricolo"/>
            </owl:Restriction>
        </owl:intersectionOf>
        <rdfs:subClassOf rdf:resource="https://w3id.org/italia/social-security/onto/socialSafetyNet/DatoreDiLavoroAgricolo"/>
    </owl:Class>
    <owl:Class>
        <owl:oneOf rdf:parseType="Collection">
            <rdf:Description rdf:about="https://w3id.org/italia/controlled-vocabulary/classifications-for-organizations/ateco-2007/A"/>
        </owl:oneOf>
        <rdfs:subClassOf rdf:resource="https://w3id.org/italia/social-security/onto/socialSafetyNet/AttivitàAgricola"/>
    </owl:Class>
    <owl:Restriction>
        <owl:onProperty rdf:resource="https://w3id.org/italia/onto/RO/holdsRoleInTime"/>
        <owl:someValuesFrom rdf:resource="https://w3id.org/italia/social-security/onto/socialSafetyNet/DatoreDiLavoroAgricolo"/>
        <rdfs:subClassOf>
            <owl:Restriction>
                <owl:onProperty rdf:resource="https://w3id.org/italia/onto/RO/holdsRoleInTime"/>
                <owl:someValuesFrom rdf:resource="https://w3id.org/italia/social-security/onto/socialSafetyNet/DatoreDiLavoro"/>
            </owl:Restriction>
        </rdfs:subClassOf>
    </owl:Restriction>
    <owl:Restriction>
        <owl:onProperty rdf:resource="https://w3id.org/italia/onto/RO/holdsRoleInTime"/>
        <owl:someValuesFrom rdf:resource="https://w3id.org/italia/social-security/onto/socialSafetyNet/DatoreDiLavoroAgricolo"/>
        <rdfs:subClassOf>
            <owl:Restriction>
                <owl:onProperty rdf:resource="https://w3id.org/italia/onto/RO/holdsRoleInTime"/>
                <owl:someValuesFrom rdf:resource="https://w3id.org/italia/social-security/onto/socialSafetyNet/ImprenditoreAgricolo"/>
            </owl:Restriction>
        </rdfs:subClassOf>
    </owl:Restriction>
    <owl:Restriction>
        <owl:onProperty rdf:resource="https://w3id.org/italia/onto/RO/holdsRoleInTime"/>
        <owl:someValuesFrom rdf:resource="https://w3id.org/italia/social-security/onto/socialSafetyNet/ImprenditoreAgricolo"/>
        <rdfs:subClassOf>
            <owl:Restriction>
                <owl:onProperty rdf:resource="https://w3id.org/italia/onto/COV/hasActivityType"/>
                <owl:someValuesFrom rdf:resource="https://w3id.org/italia/social-security/onto/socialSafetyNet/AttivitàAgricola"/>
            </owl:Restriction>
        </rdfs:subClassOf>
    </owl:Restriction>
    <owl:Restriction>
        <owl:onProperty rdf:resource="https://w3id.org/italia/onto/RO/holdsRoleInTime"/>
        <owl:someValuesFrom rdf:resource="https://w3id.org/italia/social-security/onto/socialSafetyNet/LiberoProfessionistaProtetto"/>
        <rdfs:subClassOf>
            <owl:Restriction>
                <owl:onProperty rdf:resource="https://w3id.org/italia/social-security/onto/socialSafetyNet/èIscrittoAlboProfessionale"/>
                <owl:someValuesFrom rdf:resource="http://www.w3.org/2002/07/owl#Thing"/>
            </owl:Restriction>
        </rdfs:subClassOf>
    </owl:Restriction>
    <owl:Restriction>
        <owl:onProperty rdf:resource="https://w3id.org/italia/onto/RO/holdsRoleInTime"/>
        <owl:someValuesFrom>
            <owl:Restriction>
                <owl:onProperty rdf:resource="https://w3id.org/italia/social-security/onto/socialSafetyNet/haDID"/>
                <owl:someValuesFrom rdf:resource="http://www.w3.org/2002/07/owl#Thing"/>
            </owl:Restriction>
        </owl:someValuesFrom>
        <rdfs:subClassOf>
            <owl:Restriction>
                <owl:onProperty rdf:resource="https://w3id.org/italia/social-security/onto/socialSafetyNet/èIscrittoUfficioDelLavoro"/>
                <owl:someValuesFrom rdf:resource="http://www.w3.org/2002/07/owl#Thing"/>
            </owl:Restriction>
        </rdfs:subClassOf>
    </owl:Restriction>
    <owl:Restriction>
        <owl:onProperty rdf:resource="https://w3id.org/italia/social-security/onto/socialSafetyNet/accettaContrattoDiLavoro"/>
        <owl:someValuesFrom rdf:resource="https://w3id.org/italia/social-security/onto/contributions/ContrattoDiLavoroDomestico"/>
        <rdfs:subClassOf rdf:resource="https://w3id.org/italia/social-security/onto/contributions/LavoratoreDomestico"/>
    </owl:Restriction>
    <owl:Restriction>
        <owl:onProperty rdf:resource="https://w3id.org/italia/social-security/onto/socialSafetyNet/accettaContrattoDiLavoro"/>
        <owl:someValuesFrom rdf:resource="https://w3id.org/italia/social-security/onto/socialSafetyNet/CollaborazioneCoordinataEContinuativa"/>
        <rdfs:subClassOf rdf:resource="https://w3id.org/italia/social-security/onto/socialSafetyNet/LavoratoreParasubordinato"/>
    </owl:Restriction>
    <owl:Restriction>
        <owl:onProperty rdf:resource="https://w3id.org/italia/social-security/onto/socialSafetyNet/accettaContrattoDiLavoro"/>
        <owl:someValuesFrom rdf:resource="https://w3id.org/italia/social-security/onto/socialSafetyNet/ContrattoDOpera"/>
        <rdfs:subClassOf>
            <owl:Class>
                <owl:unionOf rdf:parseType="Collection">
                    <rdf:Description rdf:about="https://w3id.org/italia/social-security/onto/socialSafetyNet/LavoratoreAutonomo"/>
                    <rdf:Description rdf:about="https://w3id.org/italia/social-security/onto/socialSafetyNet/LavoratoreAutonomoOccasionale"/>
                </owl:unionOf>
            </owl:Class>
        </rdfs:subClassOf>
    </owl:Restriction>
    <owl:Restriction>
        <owl:onProperty rdf:resource="https://w3id.org/italia/social-security/onto/socialSafetyNet/accettaContrattoDiLavoro"/>
        <owl:someValuesFrom rdf:resource="https://w3id.org/italia/social-security/onto/socialSafetyNet/ContrattoDOperaProfessionale"/>
        <rdfs:subClassOf rdf:resource="https://w3id.org/italia/social-security/onto/socialSafetyNet/LiberoProfessionista"/>
    </owl:Restriction>
    <owl:Restriction>
        <owl:onProperty rdf:resource="https://w3id.org/italia/social-security/onto/socialSafetyNet/accettaContrattoDiLavoro"/>
        <owl:someValuesFrom rdf:resource="https://w3id.org/italia/social-security/onto/socialSafetyNet/ContrattoDiApprendistato"/>
        <rdfs:subClassOf rdf:resource="https://w3id.org/italia/social-security/onto/socialSafetyNet/Apprendista"/>
    </owl:Restriction>
    <owl:Restriction>
        <owl:onProperty rdf:resource="https://w3id.org/italia/social-security/onto/socialSafetyNet/accettaContrattoDiLavoro"/>
        <owl:someValuesFrom rdf:resource="https://w3id.org/italia/social-security/onto/socialSafetyNet/ContrattoDiLavoroSubordinato"/>
        <rdfs:subClassOf rdf:resource="https://w3id.org/italia/social-security/onto/socialSafetyNet/LavoratoreSubordinato"/>
    </owl:Restriction>
    <owl:Restriction>
        <owl:onProperty rdf:resource="https://w3id.org/italia/social-security/onto/socialSafetyNet/accettaContrattoDiLavoro"/>
        <owl:someValuesFrom>
            <owl:Class>
                <owl:intersectionOf rdf:parseType="Collection">
                    <owl:Class>
                        <owl:complementOf>
                            <owl:Class>
                                <owl:unionOf rdf:parseType="Collection">
                                    <rdf:Description rdf:about="https://w3id.org/italia/social-security/onto/contributions/ContrattoDiLavoroDomestico"/>
                                    <rdf:Description rdf:about="https://w3id.org/italia/social-security/onto/socialSafetyNet/ContrattoDOpera"/>
                                </owl:unionOf>
                            </owl:Class>
                        </owl:complementOf>
                    </owl:Class>
                    <owl:Restriction>
                        <owl:onProperty>
                            <rdf:Description>
                                <owl:inverseOf rdf:resource="https://w3id.org/italia/social-security/onto/socialSafetyNet/proponeContrattoDiLavoro"/>
                            </rdf:Description>
                        </owl:onProperty>
                        <owl:someValuesFrom>
                            <owl:Class>
                                <owl:intersectionOf rdf:parseType="Collection">
                                    <rdf:Description rdf:about="https://w3id.org/italia/onto/COV/PrivateOrganization"/>
                                    <owl:Restriction>
                                        <owl:onProperty rdf:resource="https://w3id.org/italia/onto/RO/holdsRoleInTime"/>
                                        <owl:someValuesFrom rdf:resource="https://w3id.org/italia/social-security/onto/socialSafetyNet/DatoreDiLavoro"/>
                                    </owl:Restriction>
                                </owl:intersectionOf>
                            </owl:Class>
                        </owl:someValuesFrom>
                    </owl:Restriction>
                </owl:intersectionOf>
            </owl:Class>
        </owl:someValuesFrom>
        <rdfs:subClassOf rdf:resource="https://w3id.org/italia/social-security/onto/socialSafetyNet/DipendentePrivato"/>
    </owl:Restriction>
    <owl:Restriction>
        <owl:onProperty rdf:resource="https://w3id.org/italia/social-security/onto/socialSafetyNet/accettaContrattoDiLavoro"/>
        <owl:someValuesFrom>
            <owl:Class>
                <owl:intersectionOf rdf:parseType="Collection">
                    <owl:Class>
                        <owl:complementOf>
                            <owl:Class>
                                <owl:unionOf rdf:parseType="Collection">
                                    <rdf:Description rdf:about="https://w3id.org/italia/social-security/onto/contributions/ContrattoDiLavoroDomestico"/>
                                    <rdf:Description rdf:about="https://w3id.org/italia/social-security/onto/socialSafetyNet/ContrattoDOpera"/>
                                </owl:unionOf>
                            </owl:Class>
                        </owl:complementOf>
                    </owl:Class>
                    <owl:Restriction>
                        <owl:onProperty>
                            <rdf:Description>
                                <owl:inverseOf rdf:resource="https://w3id.org/italia/social-security/onto/socialSafetyNet/proponeContrattoDiLavoro"/>
                            </rdf:Description>
                        </owl:onProperty>
                        <owl:someValuesFrom>
                            <owl:Class>
                                <owl:intersectionOf rdf:parseType="Collection">
                                    <rdf:Description rdf:about="https://w3id.org/italia/onto/COV/PublicOrganization"/>
                                    <owl:Restriction>
                                        <owl:onProperty rdf:resource="https://w3id.org/italia/onto/RO/holdsRoleInTime"/>
                                        <owl:someValuesFrom rdf:resource="https://w3id.org/italia/social-security/onto/socialSafetyNet/DatoreDiLavoro"/>
                                    </owl:Restriction>
                                </owl:intersectionOf>
                            </owl:Class>
                        </owl:someValuesFrom>
                    </owl:Restriction>
                </owl:intersectionOf>
            </owl:Class>
        </owl:someValuesFrom>
        <rdfs:subClassOf rdf:resource="https://w3id.org/italia/social-security/onto/socialSafetyNet/DipendentePubblico"/>
    </owl:Restriction>
    <owl:Restriction>
        <owl:onProperty rdf:resource="https://w3id.org/italia/social-security/onto/socialSafetyNet/accettaContrattoDiLavoro"/>
        <owl:someValuesFrom>
            <owl:Restriction>
                <owl:onProperty>
                    <rdf:Description>
                        <owl:inverseOf rdf:resource="https://w3id.org/italia/social-security/onto/socialSafetyNet/proponeContrattoDiLavoro"/>
                    </rdf:Description>
                </owl:onProperty>
                <owl:someValuesFrom rdf:resource="https://w3id.org/italia/social-security/onto/socialSafetyNet/DatoreDiLavoroAgricolo"/>
            </owl:Restriction>
        </owl:someValuesFrom>
        <rdfs:subClassOf rdf:resource="https://w3id.org/italia/social-security/onto/socialSafetyNet/LavoratoreSubordinatoAgricolo"/>
    </owl:Restriction>
    <owl:Restriction>
        <owl:onProperty rdf:resource="https://w3id.org/italia/social-security/onto/socialSafetyNet/generaStatoDiDisoccupazione"/>
        <owl:someValuesFrom rdf:resource="https://w3id.org/italia/social-security/onto/socialSafetyNet/StatoDiDisoccupazioneInvolontaria"/>
        <rdfs:subClassOf>
            <owl:Restriction>
                <owl:onProperty rdf:resource="https://w3id.org/italia/social-security/onto/socialSafetyNet/haMotivoCessazioneRapportoDiLavoro"/>
                <owl:someValuesFrom rdf:resource="https://w3id.org/italia/social-security/onto/socialSafetyNet/MotivoCessazioneInvolontaria"/>
            </owl:Restriction>
        </rdfs:subClassOf>
    </owl:Restriction>
    <owl:Restriction>
        <owl:onProperty rdf:resource="https://w3id.org/italia/social-security/onto/socialSafetyNet/generaStatoDiDisoccupazione"/>
        <owl:someValuesFrom rdf:resource="https://w3id.org/italia/social-security/onto/socialSafetyNet/StatoDiDisoccupazioneVolontaria"/>
        <rdfs:subClassOf>
            <owl:Restriction>
                <owl:onProperty rdf:resource="https://w3id.org/italia/social-security/onto/socialSafetyNet/haMotivoCessazioneRapportoDiLavoro"/>
                <owl:someValuesFrom rdf:resource="https://w3id.org/italia/social-security/onto/socialSafetyNet/MotivoCessazioneVolontaria"/>
            </owl:Restriction>
        </rdfs:subClassOf>
    </owl:Restriction>
    <owl:Restriction>
        <owl:onProperty rdf:resource="https://w3id.org/italia/social-security/onto/socialSafetyNet/haMotivoCessazioneRapportoDiLavoro"/>
        <owl:someValuesFrom rdf:resource="https://w3id.org/italia/social-security/onto/socialSafetyNet/MotivoCessazioneInvolontaria"/>
        <rdfs:subClassOf>
            <owl:Restriction>
                <owl:onProperty rdf:resource="https://w3id.org/italia/social-security/onto/socialSafetyNet/generaStatoDiDisoccupazione"/>
                <owl:someValuesFrom rdf:resource="https://w3id.org/italia/social-security/onto/socialSafetyNet/StatoDiDisoccupazioneInvolontaria"/>
            </owl:Restriction>
        </rdfs:subClassOf>
    </owl:Restriction>
    <owl:Restriction>
        <owl:onProperty rdf:resource="https://w3id.org/italia/social-security/onto/socialSafetyNet/haMotivoCessazioneRapportoDiLavoro"/>
        <owl:someValuesFrom rdf:resource="https://w3id.org/italia/social-security/onto/socialSafetyNet/MotivoCessazioneVolontaria"/>
        <rdfs:subClassOf>
            <owl:Restriction>
                <owl:onProperty rdf:resource="https://w3id.org/italia/social-security/onto/socialSafetyNet/generaStatoDiDisoccupazione"/>
                <owl:someValuesFrom rdf:resource="https://w3id.org/italia/social-security/onto/socialSafetyNet/StatoDiDisoccupazioneVolontaria"/>
            </owl:Restriction>
        </rdfs:subClassOf>
    </owl:Restriction>
    <owl:Restriction>
        <owl:onProperty rdf:resource="https://w3id.org/italia/social-security/onto/socialSafetyNet/haStatoDiDomandaNASpI"/>
        <owl:someValuesFrom rdf:resource="https://w3id.org/italia/social-security/onto/socialSafetyNet/StatoDiAccoltaDiDomandaNASpI"/>
        <rdfs:subClassOf>
            <owl:Restriction>
                <owl:onProperty>
                    <rdf:Description>
                        <owl:inverseOf rdf:resource="https://w3id.org/italia/social-security/onto/socialSafetyNet/haDomandaNASpI"/>
                    </rdf:Description>
                </owl:onProperty>
                <owl:someValuesFrom rdf:resource="http://www.w3.org/2002/07/owl#Thing"/>
            </owl:Restriction>
        </rdfs:subClassOf>
    </owl:Restriction>
    <owl:Restriction>
        <owl:onProperty rdf:resource="https://w3id.org/italia/social-security/onto/socialSafetyNet/haStatoDiLavoro"/>
        <owl:someValuesFrom>
            <owl:Class>
                <owl:unionOf rdf:parseType="Collection">
                    <rdf:Description rdf:about="https://w3id.org/italia/social-security/onto/socialSafetyNet/StatoDiDisoccupazione"/>
                    <rdf:Description rdf:about="https://w3id.org/italia/social-security/onto/socialSafetyNet/StatoDiInoccupazione"/>
                </owl:unionOf>
            </owl:Class>
        </owl:someValuesFrom>
        <rdfs:subClassOf>
            <owl:Restriction>
                <owl:onProperty rdf:resource="https://w3id.org/italia/social-security/onto/socialSafetyNet/haDID"/>
                <owl:someValuesFrom rdf:resource="http://www.w3.org/2002/07/owl#Thing"/>
            </owl:Restriction>
        </rdfs:subClassOf>
    </owl:Restriction>
    <owl:Restriction>
        <owl:onProperty rdf:resource="https://w3id.org/italia/social-security/onto/socialSafetyNet/proponeContrattoDiLavoro"/>
        <owl:someValuesFrom rdf:resource="https://w3id.org/italia/social-security/onto/socialSafetyNet/ContrattoDOpera"/>
        <rdfs:subClassOf rdf:resource="https://w3id.org/italia/social-security/onto/socialSafetyNet/CommittenteDOpera"/>
    </owl:Restriction>
    <owl:Restriction>
        <owl:onProperty rdf:resource="https://w3id.org/italia/social-security/onto/socialSafetyNet/proponeContrattoDiLavoro"/>
        <owl:someValuesFrom>
            <owl:Class>
                <owl:unionOf rdf:parseType="Collection">
                    <rdf:Description rdf:about="https://w3id.org/italia/social-security/onto/socialSafetyNet/CollaborazioneCoordinataEContinuativa"/>
                    <rdf:Description rdf:about="https://w3id.org/italia/social-security/onto/socialSafetyNet/ContrattoDiLavoroSubordinato"/>
                </owl:unionOf>
            </owl:Class>
        </owl:someValuesFrom>
        <rdfs:subClassOf rdf:resource="https://w3id.org/italia/social-security/onto/socialSafetyNet/DatoreDiLavoro"/>
    </owl:Restriction>
    <owl:Restriction>
        <owl:onProperty>
            <rdf:Description>
                <owl:inverseOf rdf:resource="https://w3id.org/italia/onto/CLV/hasCountry"/>
            </rdf:Description>
        </owl:onProperty>
        <owl:someValuesFrom>
            <owl:Restriction>
                <owl:onProperty>
                    <rdf:Description>
                        <owl:inverseOf rdf:resource="https://w3id.org/italia/onto/CPV/residentIn"/>
                    </rdf:Description>
                </owl:onProperty>
                <owl:someValuesFrom>
                    <owl:Class>
                        <owl:intersectionOf rdf:parseType="Collection">
                            <owl:Restriction>
                                <owl:onProperty rdf:resource="https://w3id.org/italia/onto/RO/holdsRoleInTime"/>
                                <owl:someValuesFrom rdf:resource="https://w3id.org/italia/social-security/onto/socialSafetyNet/RichiedenteNASpI"/>
                            </owl:Restriction>
                            <owl:Restriction>
                                <owl:onProperty rdf:resource="https://w3id.org/italia/onto/RO/holdsRoleInTime"/>
                                <owl:someValuesFrom>
                                    <owl:Class>
                                        <owl:unionOf rdf:parseType="Collection">
                                            <rdf:Description rdf:about="https://w3id.org/italia/social-security/onto/socialSafetyNet/LavoratoreDiversoDalFrontaliero"/>
                                            <rdf:Description rdf:about="https://w3id.org/italia/social-security/onto/socialSafetyNet/LavoratoreFrontaliero"/>
                                        </owl:unionOf>
                                    </owl:Class>
                                </owl:someValuesFrom>
                            </owl:Restriction>
                        </owl:intersectionOf>
                    </owl:Class>
                </owl:someValuesFrom>
            </owl:Restriction>
        </owl:someValuesFrom>
        <rdfs:subClassOf>
            <owl:Class>
                <owl:oneOf rdf:parseType="Collection">
                    <rdf:Description rdf:about="http://w3id.org/italia/controlled-vocabulary/territorial-classifications/countries/italy/ITA"/>
                </owl:oneOf>
            </owl:Class>
        </rdfs:subClassOf>
    </owl:Restriction>
    <owl:Restriction>
        <owl:onProperty>
            <rdf:Description>
                <owl:inverseOf rdf:resource="https://w3id.org/italia/onto/l0/hasFirstMember"/>
            </rdf:Description>
        </owl:onProperty>
        <owl:someValuesFrom rdf:resource="https://w3id.org/italia/social-security/onto/socialSafetyNet/FascicoloDiLavoro"/>
        <rdfs:subClassOf>
            <owl:Class>
                <owl:unionOf rdf:parseType="Collection">
                    <rdf:Description rdf:about="https://w3id.org/italia/social-security/onto/socialSafetyNet/StatoDiInoccupazione"/>
                    <rdf:Description rdf:about="https://w3id.org/italia/social-security/onto/socialSafetyNet/StatoDiOccupazione"/>
                </owl:unionOf>
            </owl:Class>
        </rdfs:subClassOf>
    </owl:Restriction>
    <owl:Restriction>
        <owl:onProperty>
            <rdf:Description>
                <owl:inverseOf rdf:resource="https://w3id.org/italia/onto/l0/hasMember"/>
            </rdf:Description>
        </owl:onProperty>
        <owl:someValuesFrom rdf:resource="https://w3id.org/italia/social-security/onto/socialSafetyNet/EstrattoContoContributivo"/>
        <rdfs:subClassOf rdf:resource="https://w3id.org/italia/social-security/onto/socialSafetyNet/ContributoPrevidenziale"/>
    </owl:Restriction>
    <owl:Restriction>
        <owl:onProperty>
            <rdf:Description>
                <owl:inverseOf rdf:resource="https://w3id.org/italia/onto/l0/hasMember"/>
            </rdf:Description>
        </owl:onProperty>
        <owl:someValuesFrom rdf:resource="https://w3id.org/italia/social-security/onto/socialSafetyNet/FascicoloDiLavoro"/>
        <rdfs:subClassOf rdf:resource="https://w3id.org/italia/social-security/onto/socialSafetyNet/StatoDiLavoro"/>
    </owl:Restriction>
    <owl:Restriction>
        <owl:onProperty>
            <rdf:Description>
                <owl:inverseOf rdf:resource="https://w3id.org/italia/social-security/onto/socialSafetyNet/haBeneficiarioPrestazioneDiSostegnoAlReddito"/>
            </rdf:Description>
        </owl:onProperty>
        <owl:someValuesFrom rdf:resource="https://w3id.org/italia/social-security/onto/socialSafetyNet/DetrazioneFiscalePerCarichiFamigliari"/>
        <rdfs:subClassOf rdf:resource="https://w3id.org/italia/social-security/onto/socialSafetyNet/BeneficiarioDetrazioneFiscalePerCarichiFamiliari"/>
    </owl:Restriction>
    <owl:Restriction>
        <owl:onProperty>
            <rdf:Description>
                <owl:inverseOf rdf:resource="https://w3id.org/italia/social-security/onto/socialSafetyNet/haBeneficiarioPrestazioneDiSostegnoAlReddito"/>
            </rdf:Description>
        </owl:onProperty>
        <owl:someValuesFrom rdf:resource="https://w3id.org/italia/social-security/onto/socialSafetyNet/PrestazioneANF"/>
        <rdfs:subClassOf rdf:resource="https://w3id.org/italia/social-security/onto/socialSafetyNet/BeneficiarioPrestazioneANF"/>
    </owl:Restriction>
    <owl:Restriction>
        <owl:onProperty>
            <rdf:Description>
                <owl:inverseOf rdf:resource="https://w3id.org/italia/social-security/onto/socialSafetyNet/haBeneficiarioPrestazioneDiSostegnoAlReddito"/>
            </rdf:Description>
        </owl:onProperty>
        <owl:someValuesFrom rdf:resource="https://w3id.org/italia/social-security/onto/socialSafetyNet/PrestazioneDIS-COLL"/>
        <rdfs:subClassOf rdf:resource="https://w3id.org/italia/social-security/onto/socialSafetyNet/BeneficiarioDIS-COLL"/>
    </owl:Restriction>
    <owl:Restriction>
        <owl:onProperty>
            <rdf:Description>
                <owl:inverseOf rdf:resource="https://w3id.org/italia/social-security/onto/socialSafetyNet/haBeneficiarioPrestazioneDiSostegnoAlReddito"/>
            </rdf:Description>
        </owl:onProperty>
        <owl:someValuesFrom rdf:resource="https://w3id.org/italia/social-security/onto/socialSafetyNet/PrestazioneNASpI"/>
        <rdfs:subClassOf rdf:resource="https://w3id.org/italia/social-security/onto/socialSafetyNet/BeneficiarioNASpI"/>
    </owl:Restriction>
    <owl:Restriction>
        <owl:onProperty>
            <rdf:Description>
                <owl:inverseOf rdf:resource="https://w3id.org/italia/social-security/onto/socialSafetyNet/haContributoObbligatorio"/>
            </rdf:Description>
        </owl:onProperty>
        <owl:someValuesFrom rdf:resource="https://w3id.org/italia/social-security/onto/socialSafetyNet/ContrattoDiLavoroSubordinato"/>
        <rdfs:subClassOf rdf:resource="https://w3id.org/italia/social-security/onto/socialSafetyNet/ContributoAssicurazioneGeneraleObbligatoria"/>
    </owl:Restriction>
    <owl:Restriction>
        <owl:onProperty>
            <rdf:Description>
                <owl:inverseOf rdf:resource="https://w3id.org/italia/social-security/onto/socialSafetyNet/haStatoCompetente"/>
            </rdf:Description>
        </owl:onProperty>
        <owl:someValuesFrom>
            <owl:Restriction>
                <owl:onProperty>
                    <rdf:Description>
                        <owl:inverseOf rdf:resource="https://w3id.org/italia/social-security/onto/socialSafetyNet/haSituazioneLavorativa"/>
                    </rdf:Description>
                </owl:onProperty>
                <owl:someValuesFrom rdf:resource="http://www.w3.org/2002/07/owl#Thing"/>
            </owl:Restriction>
        </owl:someValuesFrom>
        <rdfs:subClassOf>
            <owl:Class>
                <owl:oneOf rdf:parseType="Collection">
                    <rdf:Description rdf:about="http://w3id.org/italia/controlled-vocabulary/territorial-classifications/countries/italy/ITA"/>
                </owl:oneOf>
            </owl:Class>
        </rdfs:subClassOf>
    </owl:Restriction>
    <owl:Restriction>
        <owl:onProperty>
            <rdf:Description>
                <owl:inverseOf rdf:resource="https://w3id.org/italia/social-security/onto/socialSafetyNet/haUfficioDelLavoroDiIscrizione"/>
            </rdf:Description>
        </owl:onProperty>
        <owl:someValuesFrom>
            <owl:Restriction>
                <owl:onProperty>
                    <rdf:Description>
                        <owl:inverseOf rdf:resource="https://w3id.org/italia/social-security/onto/socialSafetyNet/èIscrittoUfficioDelLavoro"/>
                    </rdf:Description>
                </owl:onProperty>
                <owl:someValuesFrom>
                    <owl:Restriction>
                        <owl:onProperty rdf:resource="https://w3id.org/italia/social-security/onto/socialSafetyNet/haDID"/>
                        <owl:someValuesFrom rdf:resource="http://www.w3.org/2002/07/owl#Thing"/>
                    </owl:Restriction>
                </owl:someValuesFrom>
            </owl:Restriction>
        </owl:someValuesFrom>
        <rdfs:subClassOf rdf:resource="https://w3id.org/italia/social-security/onto/socialSafetyNet/CentroPerLImpiego"/>
    </owl:Restriction>
    <rdf:Description>
        <rdf:type rdf:resource="http://www.w3.org/2002/07/owl#AllDisjointClasses"/>
        <owl:members rdf:parseType="Collection">
            <rdf:Description rdf:about="https://w3id.org/italia/social-security/onto/socialSafetyNet/AttoDiCertificazioneDiBeneficiarioNASpI"/>
            <rdf:Description rdf:about="https://w3id.org/italia/social-security/onto/socialSafetyNet/AttoDiCertificazioneLavoroEstero"/>
            <rdf:Description rdf:about="https://w3id.org/italia/social-security/onto/socialSafetyNet/AttoDiCessazioneRapportoDiLavoro"/>
            <rdf:Description rdf:about="https://w3id.org/italia/social-security/onto/socialSafetyNet/AttoDiDecadenzaNASpI"/>
            <rdf:Description rdf:about="https://w3id.org/italia/social-security/onto/socialSafetyNet/AttoDiDecadenzaStatoDiDisoccupazione"/>
            <rdf:Description rdf:about="https://w3id.org/italia/social-security/onto/socialSafetyNet/AttoDiNotificaEventoInEspatrio"/>
            <rdf:Description rdf:about="https://w3id.org/italia/social-security/onto/socialSafetyNet/AttoDiNotificaViolazioneObblighiAttivazione"/>
            <rdf:Description rdf:about="https://w3id.org/italia/social-security/onto/socialSafetyNet/AttoDiRinunciaAllaNASpI"/>
            <rdf:Description rdf:about="https://w3id.org/italia/social-security/onto/socialSafetyNet/DichiarazioneDiImmediataDisponibilità"/>
        </owl:members>
    </rdf:Description>
    <rdf:Description>
        <rdf:type rdf:resource="http://www.w3.org/2002/07/owl#AllDisjointClasses"/>
        <owl:members rdf:parseType="Collection">
            <rdf:Description rdf:about="https://w3id.org/italia/social-security/onto/socialSafetyNet/BeneficiarioDIS-COLL"/>
            <rdf:Description rdf:about="https://w3id.org/italia/social-security/onto/socialSafetyNet/BeneficiarioDetrazioneFiscalePerCarichiFamiliari"/>
            <rdf:Description rdf:about="https://w3id.org/italia/social-security/onto/socialSafetyNet/BeneficiarioNASpI"/>
            <rdf:Description rdf:about="https://w3id.org/italia/social-security/onto/socialSafetyNet/BeneficiarioPrestazioneANF"/>
        </owl:members>
    </rdf:Description>
    <rdf:Description>
        <rdf:type rdf:resource="http://www.w3.org/2002/07/owl#AllDisjointClasses"/>
        <owl:members rdf:parseType="Collection">
            <rdf:Description rdf:about="https://w3id.org/italia/social-security/onto/socialSafetyNet/CollaborazioneCoordinataEContinuativa"/>
            <rdf:Description rdf:about="https://w3id.org/italia/social-security/onto/socialSafetyNet/ContrattoDOpera"/>
            <rdf:Description rdf:about="https://w3id.org/italia/social-security/onto/socialSafetyNet/ContrattoDOperaProfessionale"/>
            <rdf:Description rdf:about="https://w3id.org/italia/social-security/onto/socialSafetyNet/ContrattoDiLavoroSubordinato"/>
        </owl:members>
    </rdf:Description>
    <rdf:Description>
        <rdf:type rdf:resource="http://www.w3.org/2002/07/owl#AllDisjointClasses"/>
        <owl:members rdf:parseType="Collection">
            <rdf:Description rdf:about="https://w3id.org/italia/social-security/onto/socialSafetyNet/ComunicazioneEventoNASpI"/>
            <rdf:Description rdf:about="https://w3id.org/italia/social-security/onto/socialSafetyNet/ComunicazioneVariazioneNASpI"/>
            <rdf:Description rdf:about="https://w3id.org/italia/social-security/onto/socialSafetyNet/StatoDiBozzaComunicazioneNASpI"/>
        </owl:members>
    </rdf:Description>
    <rdf:Description>
        <rdf:type rdf:resource="http://www.w3.org/2002/07/owl#AllDisjointClasses"/>
        <owl:members rdf:parseType="Collection">
            <rdf:Description rdf:about="https://w3id.org/italia/social-security/onto/socialSafetyNet/ComunicazioneNASpI"/>
            <rdf:Description rdf:about="https://w3id.org/italia/social-security/onto/socialSafetyNet/ContrattoDiLavoro"/>
            <rdf:Description rdf:about="https://w3id.org/italia/social-security/onto/socialSafetyNet/ContributoPrevidenziale"/>
            <rdf:Description rdf:about="https://w3id.org/italia/social-security/onto/socialSafetyNet/DomandaDiPensionamento"/>
            <rdf:Description rdf:about="https://w3id.org/italia/social-security/onto/socialSafetyNet/EspatrioInNASpI"/>
            <rdf:Description rdf:about="https://w3id.org/italia/social-security/onto/socialSafetyNet/IndisponibilitàPerNASpI"/>
            <rdf:Description rdf:about="https://w3id.org/italia/social-security/onto/socialSafetyNet/IscrizioneAlboProfessionale"/>
            <rdf:Description rdf:about="https://w3id.org/italia/social-security/onto/socialSafetyNet/IscrizioneUfficioDelLavoro"/>
            <rdf:Description rdf:about="https://w3id.org/italia/social-security/onto/socialSafetyNet/PrestazioneLavorativa"/>
            <rdf:Description rdf:about="https://w3id.org/italia/social-security/onto/socialSafetyNet/StatoDiDomandaNASpI"/>
            <rdf:Description rdf:about="https://w3id.org/italia/social-security/onto/socialSafetyNet/StatoDiLavoro"/>
            <rdf:Description rdf:about="https://w3id.org/italia/social-security/onto/socialSafetyNet/StatoDiPrestazioneNASpI"/>
        </owl:members>
    </rdf:Description>
    <rdf:Description>
        <rdf:type rdf:resource="http://www.w3.org/2002/07/owl#AllDisjointClasses"/>
        <owl:members rdf:parseType="Collection">
            <rdf:Description rdf:about="https://w3id.org/italia/social-security/onto/socialSafetyNet/ContributoAssicurazioneGeneraleObbligatoria"/>
            <rdf:Description rdf:about="https://w3id.org/italia/social-security/onto/socialSafetyNet/ContributoGestioneSeparata"/>
            <rdf:Description rdf:about="https://w3id.org/italia/social-security/onto/socialSafetyNet/ContributoGestioneSpecialeArtigiani"/>
            <rdf:Description rdf:about="https://w3id.org/italia/social-security/onto/socialSafetyNet/ContributoGestioneSpecialeCommercianti"/>
            <rdf:Description rdf:about="https://w3id.org/italia/social-security/onto/socialSafetyNet/ContributoGestioneSpecialeLavoratoriAgricoli"/>
            <rdf:Description rdf:about="https://w3id.org/italia/social-security/onto/socialSafetyNet/ContributoLavoroEstero"/>
        </owl:members>
    </rdf:Description>
    <rdf:Description>
        <rdf:type rdf:resource="http://www.w3.org/2002/07/owl#AllDisjointClasses"/>
        <owl:members rdf:parseType="Collection">
            <rdf:Description rdf:about="https://w3id.org/italia/social-security/onto/socialSafetyNet/ContributoDaRiscatto"/>
            <rdf:Description rdf:about="https://w3id.org/italia/social-security/onto/socialSafetyNet/ContributoFigurativo"/>
            <rdf:Description rdf:about="https://w3id.org/italia/social-security/onto/socialSafetyNet/ContributoObbligatorio"/>
            <rdf:Description rdf:about="https://w3id.org/italia/social-security/onto/socialSafetyNet/ContributoVolontario"/>
        </owl:members>
    </rdf:Description>
    <rdf:Description>
        <rdf:type rdf:resource="http://www.w3.org/2002/07/owl#AllDisjointClasses"/>
        <owl:members rdf:parseType="Collection">
            <rdf:Description rdf:about="https://w3id.org/italia/social-security/onto/socialSafetyNet/DelegatoDomandaNASpI"/>
            <rdf:Description rdf:about="https://w3id.org/italia/social-security/onto/socialSafetyNet/ImprenditoreAgricolo"/>
            <rdf:Description rdf:about="https://w3id.org/italia/social-security/onto/socialSafetyNet/TitolareDelRapportoDiLavoro"/>
        </owl:members>
    </rdf:Description>
    <rdf:Description>
        <rdf:type rdf:resource="http://www.w3.org/2002/07/owl#AllDisjointClasses"/>
        <owl:members rdf:parseType="Collection">
            <rdf:Description rdf:about="https://w3id.org/italia/social-security/onto/socialSafetyNet/DetrazioneFiscalePerCarichiFamigliari"/>
            <rdf:Description rdf:about="https://w3id.org/italia/social-security/onto/socialSafetyNet/PrestazioneANF"/>
            <rdf:Description rdf:about="https://w3id.org/italia/social-security/onto/socialSafetyNet/PrestazioneDIS-COLL"/>
            <rdf:Description rdf:about="https://w3id.org/italia/social-security/onto/socialSafetyNet/PrestazioneNASpI"/>
        </owl:members>
    </rdf:Description>
    <rdf:Description>
        <rdf:type rdf:resource="http://www.w3.org/2002/07/owl#AllDisjointClasses"/>
        <owl:members rdf:parseType="Collection">
            <rdf:Description rdf:about="https://w3id.org/italia/social-security/onto/socialSafetyNet/LavoratoreAutonomo"/>
            <rdf:Description rdf:about="https://w3id.org/italia/social-security/onto/socialSafetyNet/LavoratoreAutonomoOccasionale"/>
            <rdf:Description rdf:about="https://w3id.org/italia/social-security/onto/socialSafetyNet/LavoratoreParasubordinato"/>
            <rdf:Description rdf:about="https://w3id.org/italia/social-security/onto/socialSafetyNet/LavoratoreSubordinato"/>
            <rdf:Description rdf:about="https://w3id.org/italia/social-security/onto/socialSafetyNet/LiberoProfessionista"/>
        </owl:members>
    </rdf:Description>
    <rdf:Description>
        <rdf:type rdf:resource="http://www.w3.org/2002/07/owl#AllDisjointClasses"/>
        <owl:members rdf:parseType="Collection">
            <rdf:Description rdf:about="https://w3id.org/italia/social-security/onto/socialSafetyNet/StatoDiAccoltaDiDomandaNASpI"/>
            <rdf:Description rdf:about="https://w3id.org/italia/social-security/onto/socialSafetyNet/StatoDiBozzaDiDomandaNASpI"/>
            <rdf:Description rdf:about="https://w3id.org/italia/social-security/onto/socialSafetyNet/StatoDiIntegrazioneDiDomandaNASpI"/>
            <rdf:Description rdf:about="https://w3id.org/italia/social-security/onto/socialSafetyNet/StatoDiProtocollataDiDomandaNASpI"/>
            <rdf:Description rdf:about="https://w3id.org/italia/social-security/onto/socialSafetyNet/StatoDiRicorsoDiDomandaNASpI"/>
            <rdf:Description rdf:about="https://w3id.org/italia/social-security/onto/socialSafetyNet/StatoDiRiesameDiDomandaNASpI"/>
            <rdf:Description rdf:about="https://w3id.org/italia/social-security/onto/socialSafetyNet/StatoDiRifiutataDiDomandaNASpI"/>
        </owl:members>
    </rdf:Description>
    <rdf:Description>
        <rdf:type rdf:resource="http://www.w3.org/2002/07/owl#AllDisjointClasses"/>
        <owl:members rdf:parseType="Collection">
            <rdf:Description rdf:about="https://w3id.org/italia/social-security/onto/socialSafetyNet/StatoDiCessatoDiNASpI"/>
            <rdf:Description rdf:about="https://w3id.org/italia/social-security/onto/socialSafetyNet/StatoDiDecadutoDiNASpI"/>
            <rdf:Description rdf:about="https://w3id.org/italia/social-security/onto/socialSafetyNet/StatoDiErogatoDiNASpI"/>
            <rdf:Description rdf:about="https://w3id.org/italia/social-security/onto/socialSafetyNet/StatoDiSospesoDiNASpI"/>
        </owl:members>
    </rdf:Description>
    <rdf:Description>
        <rdf:type rdf:resource="http://www.w3.org/2002/07/owl#AllDisjointClasses"/>
        <owl:members rdf:parseType="Collection">
            <rdf:Description rdf:about="https://w3id.org/italia/social-security/onto/socialSafetyNet/StatoDiDisoccupazione"/>
            <rdf:Description rdf:about="https://w3id.org/italia/social-security/onto/socialSafetyNet/StatoDiInoccupazione"/>
            <rdf:Description rdf:about="https://w3id.org/italia/social-security/onto/socialSafetyNet/StatoDiOccupazione"/>
        </owl:members>
    </rdf:Description>
    <rdf:Description>
        <rdf:type rdf:resource="http://www.w3.org/2002/07/owl#AllDisjointClasses"/>
        <owl:members rdf:parseType="Collection">
            <rdf:Description rdf:about="https://w3id.org/italia/social-security/onto/socialSafetyNet/VariazioneDelegaRiscossioneContributiSindacaliNASpI"/>
            <rdf:Description rdf:about="https://w3id.org/italia/social-security/onto/socialSafetyNet/VariazioneDomicilioNASpI"/>
            <rdf:Description rdf:about="https://w3id.org/italia/social-security/onto/socialSafetyNet/VariazioneModalitàDiPagamentoNASpI"/>
            <rdf:Description rdf:about="https://w3id.org/italia/social-security/onto/socialSafetyNet/VariazioneRecapitoNASpI"/>
        </owl:members>
    </rdf:Description>
    <owl:Class>
        <owl:oneOf rdf:parseType="Collection">
            <rdf:Description rdf:about="http://w3id.org/italia/controlled-vocabulary/territorial-classifications/countries/italy/ITA"/>
        </owl:oneOf>
        <owl:disjointWith>
            <owl:Restriction>
                <owl:onProperty rdf:resource="https://w3id.org/italia/onto/CLV/hasCountry"/>
                <owl:someValuesFrom>
                    <owl:Restriction>
                        <owl:onProperty rdf:resource="https://w3id.org/italia/onto/CLV/withAddress"/>
                        <owl:someValuesFrom>
                            <owl:Restriction>
                                <owl:onProperty rdf:resource="https://w3id.org/italia/onto/CLV/hasAdressinTime"/>
                                <owl:someValuesFrom>
                                    <owl:Restriction>
                                        <owl:onProperty rdf:resource="https://w3id.org/italia/social-security/onto/socialSafetyNet/èRegolatoDaContratto"/>
                                        <owl:someValuesFrom>
                                            <owl:Restriction>
                                                <owl:onProperty rdf:resource="https://w3id.org/italia/social-security/onto/socialSafetyNet/haContributoObbligatorio"/>
                                                <owl:someValuesFrom rdf:resource="https://w3id.org/italia/social-security/onto/socialSafetyNet/ContributoLavoroEstero"/>
                                            </owl:Restriction>
                                        </owl:someValuesFrom>
                                    </owl:Restriction>
                                </owl:someValuesFrom>
                            </owl:Restriction>
                        </owl:someValuesFrom>
                    </owl:Restriction>
                </owl:someValuesFrom>
            </owl:Restriction>
        </owl:disjointWith>
    </owl:Class>
</rdf:RDF>



<!-- Generated by the OWL API (version 4.5.26.2023-07-17T20:34:13Z) https://github.com/owlcs/owlapi -->

