<https://w3id.org/italia/social-security/onto/core/> <http://www.w3.org/1999/02/22-rdf-syntax-ns#type> <http://www.w3.org/2002/07/owl#Ontology> .
<https://w3id.org/italia/social-security/onto/core/> <http://www.w3.org/2002/07/owl#versionIRI> <https://w3id.org/italia/social-security/onto/core/1.0> .
<https://w3id.org/italia/social-security/onto/core/> <http://www.w3.org/2002/07/owl#imports> <https://w3id.org/italia/onto/CLV/> .
<https://w3id.org/italia/social-security/onto/core/> <http://www.w3.org/2002/07/owl#imports> <https://w3id.org/italia/onto/COV/> .
<https://w3id.org/italia/social-security/onto/core/> <http://www.w3.org/2002/07/owl#imports> <https://w3id.org/italia/onto/CPV/> .
<https://w3id.org/italia/social-security/onto/core/> <http://www.w3.org/2002/07/owl#imports> <https://w3id.org/italia/onto/l0/> .
<https://w3id.org/italia/social-security/onto/core/> <http://www.w3.org/2002/07/owl#imports> <https://w3id.org/italia/onto/RO/> .
<https://w3id.org/italia/social-security/onto/core/> <http://purl.org/dc/terms/title> "Ontologia Core di INPS "@it .
<https://w3id.org/italia/social-security/onto/core/> <http://purl.org/dc/terms/title> "Core INPS Ontology"@en .
<https://w3id.org/italia/social-security/onto/core/> <https://w3id.org/italia/onto/ADMS/last> <https://w3id.org/italia/social-security/onto/core/1.0> .
<https://w3id.org/italia/social-security/onto/core/> <http://www.w3.org/ns/dcat#keyword> "Persona"@it .
<https://w3id.org/italia/social-security/onto/core/> <http://www.w3.org/ns/dcat#keyword> "Agente"@it .
<https://w3id.org/italia/social-security/onto/core/> <http://www.w3.org/ns/dcat#keyword> "Sede INPS"@it .
<https://w3id.org/italia/social-security/onto/core/> <http://www.w3.org/ns/dcat#keyword> "Organizzazione"@it .
<https://w3id.org/italia/social-security/onto/core/> <http://www.w3.org/ns/dcat#keyword> "Person"@en .
<https://w3id.org/italia/social-security/onto/core/> <http://www.w3.org/ns/dcat#keyword> "Agent"@en .
<https://w3id.org/italia/social-security/onto/core/> <http://www.w3.org/ns/dcat#keyword> "INPS Office"@en .
<https://w3id.org/italia/social-security/onto/core/> <http://www.w3.org/ns/dcat#keyword> "Organization"@en .
<https://w3id.org/italia/social-security/onto/core/> <http://www.w3.org/2000/01/rdf-schema#comment> "Ontologia INPS relativa alle componenti del dominio funzionale dell'istituto comuni a procedure e servizi svolti dall'ente stesso. Tra di essi troviamo, ad esempio, le dislocazioni territoriali, come le sedi, e le entit\u00E0 astratte, come i ruoli."@it .
<https://w3id.org/italia/social-security/onto/core/> <http://www.w3.org/2000/01/rdf-schema#comment> "This is the ontology of the INPS Organization about components of the institution's functional domain common to procedures and services performed by the institution itself. These include, for example, territorial dislocations, such as locations, and abstract entities, such as roles."@en .
<https://w3id.org/italia/social-security/onto/core/> <https://w3id.org/italia/onto/ADMS/target> "Cittadini"@it .
<https://w3id.org/italia/social-security/onto/core/> <https://w3id.org/italia/onto/ADMS/target> "Imprese"@it .
<https://w3id.org/italia/social-security/onto/core/> <https://w3id.org/italia/onto/ADMS/target> "Pubbliche Amministrazioni"@it .
<https://w3id.org/italia/social-security/onto/core/> <http://www.w3.org/ns/dcat#contactPoint> <https://w3id.org/italia/social-security/data/organization/DirezioneCentraleTII> .
<https://w3id.org/italia/social-security/onto/core/> <http://purl.org/dc/terms/creator> <https://w3id.org/italia/social-security/data/organization/inps> .
<https://w3id.org/italia/social-security/onto/core/> <http://purl.org/dc/terms/issued> "2024-01-16T00:00:00Z"^^<http://www.w3.org/2001/XMLSchema#dateTime> .
<https://w3id.org/italia/social-security/onto/core/> <https://w3id.org/italia/onto/ADMS/type> <https://w3id.org/italia/onto/ADMS/ServiceOnytology> .
<https://w3id.org/italia/social-security/onto/core/> <https://w3id.org/italia/onto/ADMS/hasSemanticAssetDistribution> <https://w3id.org/italia/social-security/data/core/distribution/CORE-RDF-TURTLE> .
<https://w3id.org/italia/social-security/onto/core/> <https://w3id.org/italia/onto/ADMS/hasSemanticAssetDistribution> <https://w3id.org/italia/social-security/data/core/distribution/CORE-RDF-XML> .
<https://w3id.org/italia/social-security/onto/core/> <https://w3id.org/italia/onto/ADMS/hasSemanticAssetDistribution> <https://w3id.org/italia/social-security/data/core/distribution/CORE-N-TRIPLES> .
<https://w3id.org/italia/social-security/onto/core/> <http://www.w3.org/2000/01/rdf-schema#isDefinedBy> <https://w3id.org/italia/social-security/onto/core/> .
<https://w3id.org/italia/social-security/onto/core/> <http://purl.org/dc/terms/modified> "2024-01-17T00:00:00Z"^^<http://www.w3.org/2001/XMLSchema#dateTime> .
<https://w3id.org/italia/social-security/onto/core/> <http://www.w3.org/2000/01/rdf-schema#label> "Ontologia Core di INPS"@it .
<https://w3id.org/italia/social-security/onto/core/> <http://www.w3.org/2000/01/rdf-schema#label> "Core INPS Ontology"@en .
<https://w3id.org/italia/social-security/onto/core/> <https://w3id.org/italia/onto/ADMS/hasKeyClass> <https://w3id.org/italia/social-security/onto/core/SedeINPS> .
<https://w3id.org/italia/social-security/onto/core/> <https://w3id.org/italia/onto/ADMS/hasKeyClass> <https://w3id.org/italia/social-security/onto/core/RuoloDiAgente> .
<https://w3id.org/italia/social-security/onto/core/> <https://w3id.org/italia/onto/ADMS/hasKeyClass> <https://w3id.org/italia/social-security/onto/core/RuoloDiOrganizzazione> .
<https://w3id.org/italia/social-security/onto/core/> <https://w3id.org/italia/onto/ADMS/hasKeyClass> <https://w3id.org/italia/social-security/onto/core/RuoloDiPersona> .
<https://w3id.org/italia/social-security/onto/core/> <https://w3id.org/italia/onto/ADMS/semanticAssetInUse> <https://w3id.org/italia/data/project/NDC> .
<https://w3id.org/italia/social-security/onto/core/> <https://w3id.org/italia/onto/ADMS/hasTask> <https://w3id.org/italia/onto/ADMS/AnnotationTask> .
<https://w3id.org/italia/social-security/onto/core/> <https://w3id.org/italia/onto/ADMS/hasTask> <https://w3id.org/italia/onto/ADMS/QueryFormulationTask> .
<https://w3id.org/italia/social-security/onto/core/> <https://w3id.org/italia/onto/ADMS/hasTask> <https://w3id.org/italia/onto/ADMS/SearchTask> .
<https://w3id.org/italia/social-security/onto/core/> <https://w3id.org/italia/onto/ADMS/status> "catalogued" .
<https://w3id.org/italia/social-security/onto/core/> <https://w3id.org/italia/onto/ADMS/status> "published" .
<https://w3id.org/italia/social-security/onto/core/> <http://purl.org/dc/terms/accrualPeriodicity> <http://publications.europa.eu/resource/authority/frequency/IRREG> .
<https://w3id.org/italia/social-security/onto/core/> <http://purl.org/dc/terms/rightsHolder> <https://w3id.org/italia/social-security/data/organization/DirezioneCentraleTII> .
<https://w3id.org/italia/social-security/onto/core/> <https://w3id.org/italia/onto/ADMS/hasContributor> <https://w3id.org/italia/social-security/data/organization/td> .
<https://w3id.org/italia/social-security/onto/core/> <http://www.w3.org/2002/07/owl#versionInfo> "Versione 1.0 - Modificata il 17 Gennaio 2024"@it .
<https://w3id.org/italia/social-security/onto/core/> <http://www.w3.org/2002/07/owl#versionInfo> "Version 1.0 - Modified on 17 January 2024"@en .
<https://w3id.org/italia/social-security/onto/core/> <https://w3id.org/italia/onto/ADMS/hasOntologyLanguage> <https://w3id.org/italia/onto/ADMS/OWL> .
<https://w3id.org/italia/social-security/onto/core/> <https://w3id.org/italia/onto/ADMS/hasFormalityLevel> <https://w3id.org/italia/onto/ADMS/Formal> .
<https://w3id.org/italia/social-security/onto/core/> <http://www.w3.org/ns/dcat#theme> <http://publications.europa.eu/resource/authority/data-theme/SOCI> .
<https://w3id.org/italia/social-security/onto/core/> <http://purl.org/dc/terms/publisher> <https://w3id.org/italia/social-security/data/organization/DirezioneCentraleTII> .
<https://w3id.org/italia/social-security/onto/core/> <https://w3id.org/italia/onto/ADMS/officialURI> "https://w3id.org/italia/social-security/onto/core"^^<http://www.w3.org/2001/XMLSchema#anyURI> .
<https://w3id.org/italia/social-security/onto/core/> <http://purl.org/dc/terms/language> <http://publications.europa.eu/resource/authority/language/ENG> .
<https://w3id.org/italia/social-security/onto/core/> <http://purl.org/dc/terms/language> <http://publications.europa.eu/resource/authority/language/ITA> .
<https://w3id.org/italia/social-security/onto/core/> <https://w3id.org/italia/onto/ADMS/acronym> "inps" .
<https://w3id.org/italia/social-security/onto/core/> <http://purl.org/dc/terms/description> "Ontologia INPS relativa alle componenti del dominio funzionale dell'istituto comuni a procedure e servizi svolti dall'ente stesso. Tra di essi troviamo, ad esempio, le dislocazioni territoriali, come le sedi, e le entit\u00E0 astratte, come i ruoli."@it .
<https://w3id.org/italia/social-security/onto/core/> <http://purl.org/dc/terms/description> "This is the ontology of the INPS Organization about components of the institution's functional domain common to procedures and services performed by the institution itself. These include, for example, territorial dislocations, such as locations, and abstract entities, such as roles."@en .
<https://w3id.org/italia/social-security/onto/core/> <http://purl.org/dc/terms/identifier> "https://w3id.org/italia/social-security/onto/core" .
<https://w3id.org/italia/social-security/onto/core/> <https://w3id.org/italia/onto/ADMS/prefix> "inpsc" .
<http://www.w3.org/2001/XMLSchema#string> <http://www.w3.org/1999/02/22-rdf-syntax-ns#type> <http://www.w3.org/2000/01/rdf-schema#Datatype> .
<https://w3id.org/italia/onto/CLV/hasAddress> <http://www.w3.org/1999/02/22-rdf-syntax-ns#type> <http://www.w3.org/2002/07/owl#ObjectProperty> .
<https://w3id.org/italia/onto/CLV/hasAddress> <http://www.w3.org/1999/02/22-rdf-syntax-ns#type> <http://www.w3.org/2002/07/owl#FunctionalProperty> .
<https://w3id.org/italia/onto/CLV/hasAddressComponent> <http://www.w3.org/1999/02/22-rdf-syntax-ns#type> <http://www.w3.org/2002/07/owl#ObjectProperty> .
<https://w3id.org/italia/onto/CLV/hasPrimaryAddress> <http://www.w3.org/1999/02/22-rdf-syntax-ns#type> <http://www.w3.org/2002/07/owl#ObjectProperty> .
<https://w3id.org/italia/onto/COV/hasPublicOrganization> <http://www.w3.org/1999/02/22-rdf-syntax-ns#type> <http://www.w3.org/2002/07/owl#ObjectProperty> .
<https://w3id.org/italia/onto/COV/hasPublicOrganization> <http://www.w3.org/1999/02/22-rdf-syntax-ns#type> <http://www.w3.org/2002/07/owl#FunctionalProperty> .
<https://w3id.org/italia/onto/CPV/hasCurrentResidence> <http://www.w3.org/1999/02/22-rdf-syntax-ns#type> <http://www.w3.org/2002/07/owl#ObjectProperty> .
<https://w3id.org/italia/onto/RO/holdsRoleInTime> <http://www.w3.org/1999/02/22-rdf-syntax-ns#type> <http://www.w3.org/2002/07/owl#ObjectProperty> .
<https://w3id.org/italia/social-security/onto/core/haSedeINPS> <http://www.w3.org/1999/02/22-rdf-syntax-ns#type> <http://www.w3.org/2002/07/owl#ObjectProperty> .
<https://w3id.org/italia/social-security/onto/core/haSedeINPS> <http://www.w3.org/1999/02/22-rdf-syntax-ns#type> <http://www.w3.org/2002/07/owl#FunctionalProperty> .
<https://w3id.org/italia/social-security/onto/core/haSedeINPS> <http://www.w3.org/2000/01/rdf-schema#domain> _:genid1 .
<https://w3id.org/italia/social-security/onto/core/haSedeINPS> <http://www.w3.org/2000/01/rdf-schema#range> <https://w3id.org/italia/social-security/onto/core/SedeINPS> .
<https://w3id.org/italia/social-security/onto/core/haSedeINPS> <http://www.w3.org/2000/01/rdf-schema#comment> "Relationship linking a Living Person or an Organization to an INPS Office. Each Living Person or Organization has a single INPS office."@en .
<https://w3id.org/italia/social-security/onto/core/haSedeINPS> <http://www.w3.org/2000/01/rdf-schema#comment> "Relazione che collega una Persona in Vita o un'Organizzazione ad una Sede INPS. Ciascuna Persona in Vita o Organizzazione ha un'unica Sede INPS."@it .
<https://w3id.org/italia/social-security/onto/core/haSedeINPS> <http://www.w3.org/2000/01/rdf-schema#label> "ha sede INPS"@it .
<https://w3id.org/italia/social-security/onto/core/haSedeINPS> <http://www.w3.org/2000/01/rdf-schema#label> "has INPS office"@en .
_:genid1 <http://www.w3.org/1999/02/22-rdf-syntax-ns#type> <http://www.w3.org/2002/07/owl#Class> .
_:genid1 <http://www.w3.org/2002/07/owl#unionOf> _:genid2 .
_:genid2 <http://www.w3.org/1999/02/22-rdf-syntax-ns#first> <https://w3id.org/italia/onto/COV/Organization> .
_:genid2 <http://www.w3.org/1999/02/22-rdf-syntax-ns#rest> _:genid3 .
_:genid3 <http://www.w3.org/1999/02/22-rdf-syntax-ns#first> <https://w3id.org/italia/onto/CPV/Alive> .
_:genid3 <http://www.w3.org/1999/02/22-rdf-syntax-ns#rest> <http://www.w3.org/1999/02/22-rdf-syntax-ns#nil> .
<https://w3id.org/italia/social-security/onto/core/codiceSedeINPS> <http://www.w3.org/1999/02/22-rdf-syntax-ns#type> <http://www.w3.org/2002/07/owl#DatatypeProperty> .
<https://w3id.org/italia/social-security/onto/core/codiceSedeINPS> <http://www.w3.org/1999/02/22-rdf-syntax-ns#type> <http://www.w3.org/2002/07/owl#FunctionalProperty> .
<https://w3id.org/italia/social-security/onto/core/codiceSedeINPS> <http://www.w3.org/2000/01/rdf-schema#domain> <https://w3id.org/italia/social-security/onto/core/SedeINPS> .
<https://w3id.org/italia/social-security/onto/core/codiceSedeINPS> <http://www.w3.org/2000/01/rdf-schema#range> <http://www.w3.org/2001/XMLSchema#string> .
<https://w3id.org/italia/social-security/onto/core/codiceSedeINPS> <http://www.w3.org/2000/01/rdf-schema#comment> "INPS office identification code"@en .
<https://w3id.org/italia/social-security/onto/core/codiceSedeINPS> <http://www.w3.org/2000/01/rdf-schema#comment> "This is the identification code of the INPS office."@en .
<https://w3id.org/italia/social-security/onto/core/codiceSedeINPS> <http://www.w3.org/2000/01/rdf-schema#comment> "\u00C8 il codice relativo alla Sede INPS."@it .
<https://w3id.org/italia/social-security/onto/core/codiceSedeINPS> <http://www.w3.org/2000/01/rdf-schema#label> "codice sede INPS"@it .
<https://w3id.org/italia/onto/COV/HomogeneousOrganizationalArea> <http://www.w3.org/1999/02/22-rdf-syntax-ns#type> <http://www.w3.org/2002/07/owl#Class> .
<https://w3id.org/italia/onto/COV/Organization> <http://www.w3.org/1999/02/22-rdf-syntax-ns#type> <http://www.w3.org/2002/07/owl#Class> .
<https://w3id.org/italia/onto/COV/Organization> <http://www.w3.org/2000/01/rdf-schema#subClassOf> <https://w3id.org/italia/onto/l0/Agent> .
<https://w3id.org/italia/onto/COV/Organization> <http://www.w3.org/2002/07/owl#disjointWith> <https://w3id.org/italia/onto/CPV/Person> .
<https://w3id.org/italia/onto/COV/PublicOrganization> <http://www.w3.org/1999/02/22-rdf-syntax-ns#type> <http://www.w3.org/2002/07/owl#Class> .
<https://w3id.org/italia/onto/CPV/Alive> <http://www.w3.org/1999/02/22-rdf-syntax-ns#type> <http://www.w3.org/2002/07/owl#Class> .
<https://w3id.org/italia/onto/CPV/Alive> <http://www.w3.org/2000/01/rdf-schema#subClassOf> <https://w3id.org/italia/onto/CPV/Person> .
<https://w3id.org/italia/onto/CPV/Alive> <http://www.w3.org/2002/07/owl#disjointWith> <https://w3id.org/italia/onto/CPV/Dead> .
<https://w3id.org/italia/onto/CPV/Dead> <http://www.w3.org/1999/02/22-rdf-syntax-ns#type> <http://www.w3.org/2002/07/owl#Class> .
<https://w3id.org/italia/onto/CPV/Dead> <http://www.w3.org/2000/01/rdf-schema#subClassOf> <https://w3id.org/italia/onto/CPV/Person> .
<https://w3id.org/italia/onto/CPV/Person> <http://www.w3.org/1999/02/22-rdf-syntax-ns#type> <http://www.w3.org/2002/07/owl#Class> .
<https://w3id.org/italia/onto/CPV/Person> <http://www.w3.org/2000/01/rdf-schema#subClassOf> <https://w3id.org/italia/onto/l0/Agent> .
<https://w3id.org/italia/onto/l0/Agent> <http://www.w3.org/1999/02/22-rdf-syntax-ns#type> <http://www.w3.org/2002/07/owl#Class> .
<https://w3id.org/italia/social-security/onto/core/RuoloDiAgente> <http://www.w3.org/1999/02/22-rdf-syntax-ns#type> <http://www.w3.org/2002/07/owl#Class> .
<https://w3id.org/italia/social-security/onto/core/RuoloDiAgente> <http://www.w3.org/2000/01/rdf-schema#subClassOf> _:genid4 .
<https://w3id.org/italia/social-security/onto/core/RuoloDiAgente> <http://www.w3.org/2000/01/rdf-schema#comment> "Insieme di mansioni, compiti, responsabilit\u00E0 e doveri attribuiti in un intervallo di tempo, anche non ancora terminato, a una persona o a una organizzazione considerando queste ultime specializzazioni di agente. "@it .
<https://w3id.org/italia/social-security/onto/core/RuoloDiAgente> <http://www.w3.org/2000/01/rdf-schema#comment> "Set of tasks, duties and responsabilities attributed in a certain time interval, possible not yet determined, to a person or organization, considering these as specializations of an agent. "@en .
<https://w3id.org/italia/social-security/onto/core/RuoloDiAgente> <http://www.w3.org/2000/01/rdf-schema#label> "Agent Role"@en .
<https://w3id.org/italia/social-security/onto/core/RuoloDiAgente> <http://www.w3.org/2000/01/rdf-schema#label> "Ruolo Di Agente"@it .
_:genid4 <http://www.w3.org/1999/02/22-rdf-syntax-ns#type> <http://www.w3.org/2002/07/owl#Restriction> .
_:genid4 <http://www.w3.org/2002/07/owl#onProperty> _:genid5 .
_:genid4 <http://www.w3.org/2002/07/owl#someValuesFrom> _:genid6 .
_:genid5 <http://www.w3.org/2002/07/owl#inverseOf> <https://w3id.org/italia/onto/RO/holdsRoleInTime> .
_:genid6 <http://www.w3.org/1999/02/22-rdf-syntax-ns#type> <http://www.w3.org/2002/07/owl#Class> .
_:genid6 <http://www.w3.org/2002/07/owl#unionOf> _:genid7 .
_:genid7 <http://www.w3.org/1999/02/22-rdf-syntax-ns#first> <https://w3id.org/italia/onto/COV/Organization> .
_:genid7 <http://www.w3.org/1999/02/22-rdf-syntax-ns#rest> _:genid8 .
_:genid8 <http://www.w3.org/1999/02/22-rdf-syntax-ns#first> <https://w3id.org/italia/onto/CPV/Person> .
_:genid8 <http://www.w3.org/1999/02/22-rdf-syntax-ns#rest> <http://www.w3.org/1999/02/22-rdf-syntax-ns#nil> .
<https://w3id.org/italia/social-security/onto/core/RuoloDiOrganizzazione> <http://www.w3.org/1999/02/22-rdf-syntax-ns#type> <http://www.w3.org/2002/07/owl#Class> .
<https://w3id.org/italia/social-security/onto/core/RuoloDiOrganizzazione> <http://www.w3.org/2000/01/rdf-schema#subClassOf> <https://w3id.org/italia/social-security/onto/core/RuoloDiAgente> .
<https://w3id.org/italia/social-security/onto/core/RuoloDiOrganizzazione> <http://www.w3.org/2000/01/rdf-schema#subClassOf> _:genid9 .
<https://w3id.org/italia/social-security/onto/core/RuoloDiOrganizzazione> <http://www.w3.org/2002/07/owl#disjointWith> <https://w3id.org/italia/social-security/onto/core/RuoloDiPersona> .
<https://w3id.org/italia/social-security/onto/core/RuoloDiOrganizzazione> <http://www.w3.org/2000/01/rdf-schema#comment> "Specializzazione della classe Ruolo Di Agente limitata alle sole organizzazioni."@it .
<https://w3id.org/italia/social-security/onto/core/RuoloDiOrganizzazione> <http://www.w3.org/2000/01/rdf-schema#comment> "Subclass of the Agent Role class, limited to organization."@en .
<https://w3id.org/italia/social-security/onto/core/RuoloDiOrganizzazione> <http://www.w3.org/2000/01/rdf-schema#label> "Organization Role"@en .
<https://w3id.org/italia/social-security/onto/core/RuoloDiOrganizzazione> <http://www.w3.org/2000/01/rdf-schema#label> "Ruolo Di Organizzazione"@it .
_:genid9 <http://www.w3.org/1999/02/22-rdf-syntax-ns#type> <http://www.w3.org/2002/07/owl#Restriction> .
_:genid9 <http://www.w3.org/2002/07/owl#onProperty> _:genid10 .
_:genid9 <http://www.w3.org/2002/07/owl#someValuesFrom> <https://w3id.org/italia/onto/COV/Organization> .
_:genid10 <http://www.w3.org/2002/07/owl#inverseOf> <https://w3id.org/italia/onto/RO/holdsRoleInTime> .
<https://w3id.org/italia/social-security/onto/core/RuoloDiPersona> <http://www.w3.org/1999/02/22-rdf-syntax-ns#type> <http://www.w3.org/2002/07/owl#Class> .
<https://w3id.org/italia/social-security/onto/core/RuoloDiPersona> <http://www.w3.org/2000/01/rdf-schema#subClassOf> <https://w3id.org/italia/social-security/onto/core/RuoloDiAgente> .
<https://w3id.org/italia/social-security/onto/core/RuoloDiPersona> <http://www.w3.org/2000/01/rdf-schema#subClassOf> _:genid11 .
<https://w3id.org/italia/social-security/onto/core/RuoloDiPersona> <http://www.w3.org/2000/01/rdf-schema#comment> "Specializzazione della classe Ruolo Di Agente limitata alle sole persone, in vita o decedute."@it .
<https://w3id.org/italia/social-security/onto/core/RuoloDiPersona> <http://www.w3.org/2000/01/rdf-schema#comment> "Subclass of the Agent Role class, limited to people, living or deceased."@en .
<https://w3id.org/italia/social-security/onto/core/RuoloDiPersona> <http://www.w3.org/2000/01/rdf-schema#label> "Person Role"@en .
<https://w3id.org/italia/social-security/onto/core/RuoloDiPersona> <http://www.w3.org/2000/01/rdf-schema#label> "Ruolo Di Persona"@it .
_:genid11 <http://www.w3.org/1999/02/22-rdf-syntax-ns#type> <http://www.w3.org/2002/07/owl#Restriction> .
_:genid11 <http://www.w3.org/2002/07/owl#onProperty> _:genid12 .
_:genid11 <http://www.w3.org/2002/07/owl#someValuesFrom> <https://w3id.org/italia/onto/CPV/Person> .
_:genid12 <http://www.w3.org/2002/07/owl#inverseOf> <https://w3id.org/italia/onto/RO/holdsRoleInTime> .
<https://w3id.org/italia/social-security/onto/core/RuoloDiPersonaDeceduta> <http://www.w3.org/1999/02/22-rdf-syntax-ns#type> <http://www.w3.org/2002/07/owl#Class> .
<https://w3id.org/italia/social-security/onto/core/RuoloDiPersonaDeceduta> <http://www.w3.org/2000/01/rdf-schema#subClassOf> <https://w3id.org/italia/social-security/onto/core/RuoloDiPersona> .
<https://w3id.org/italia/social-security/onto/core/RuoloDiPersonaDeceduta> <http://www.w3.org/2000/01/rdf-schema#subClassOf> _:genid13 .
<https://w3id.org/italia/social-security/onto/core/RuoloDiPersonaDeceduta> <http://www.w3.org/2002/07/owl#disjointWith> <https://w3id.org/italia/social-security/onto/core/RuoloDiPersonaViva> .
<https://w3id.org/italia/social-security/onto/core/RuoloDiPersonaDeceduta> <http://www.w3.org/2000/01/rdf-schema#comment> "Specializzazione della classe Ruolo Di Persona limitata alle sole persone decedute."@it .
<https://w3id.org/italia/social-security/onto/core/RuoloDiPersonaDeceduta> <http://www.w3.org/2000/01/rdf-schema#comment> "Subclass of the Person Role class, limited to only dead persons."@en .
<https://w3id.org/italia/social-security/onto/core/RuoloDiPersonaDeceduta> <http://www.w3.org/2000/01/rdf-schema#label> "Dead Person Role"@en .
<https://w3id.org/italia/social-security/onto/core/RuoloDiPersonaDeceduta> <http://www.w3.org/2000/01/rdf-schema#label> "Ruolo Di Persona Deceduta"@it .
_:genid13 <http://www.w3.org/1999/02/22-rdf-syntax-ns#type> <http://www.w3.org/2002/07/owl#Restriction> .
_:genid13 <http://www.w3.org/2002/07/owl#onProperty> _:genid14 .
_:genid13 <http://www.w3.org/2002/07/owl#someValuesFrom> <https://w3id.org/italia/onto/CPV/Dead> .
_:genid14 <http://www.w3.org/2002/07/owl#inverseOf> <https://w3id.org/italia/onto/RO/holdsRoleInTime> .
<https://w3id.org/italia/social-security/onto/core/RuoloDiPersonaViva> <http://www.w3.org/1999/02/22-rdf-syntax-ns#type> <http://www.w3.org/2002/07/owl#Class> .
<https://w3id.org/italia/social-security/onto/core/RuoloDiPersonaViva> <http://www.w3.org/2000/01/rdf-schema#subClassOf> <https://w3id.org/italia/social-security/onto/core/RuoloDiPersona> .
<https://w3id.org/italia/social-security/onto/core/RuoloDiPersonaViva> <http://www.w3.org/2000/01/rdf-schema#subClassOf> _:genid15 .
<https://w3id.org/italia/social-security/onto/core/RuoloDiPersonaViva> <http://www.w3.org/2000/01/rdf-schema#comment> "Specializzazione della classe Ruolo Di Persona limitata alle sole persone in vita."@it .
<https://w3id.org/italia/social-security/onto/core/RuoloDiPersonaViva> <http://www.w3.org/2000/01/rdf-schema#comment> "Subclass of the Person Role class, limited to only alive persons."@en .
<https://w3id.org/italia/social-security/onto/core/RuoloDiPersonaViva> <http://www.w3.org/2000/01/rdf-schema#label> "Alive Person Role"@en .
<https://w3id.org/italia/social-security/onto/core/RuoloDiPersonaViva> <http://www.w3.org/2000/01/rdf-schema#label> "Ruolo Di Persona Viva"@it .
_:genid15 <http://www.w3.org/1999/02/22-rdf-syntax-ns#type> <http://www.w3.org/2002/07/owl#Restriction> .
_:genid15 <http://www.w3.org/2002/07/owl#onProperty> _:genid16 .
_:genid15 <http://www.w3.org/2002/07/owl#someValuesFrom> <https://w3id.org/italia/onto/CPV/Alive> .
_:genid16 <http://www.w3.org/2002/07/owl#inverseOf> <https://w3id.org/italia/onto/RO/holdsRoleInTime> .
<https://w3id.org/italia/social-security/onto/core/SedeINPS> <http://www.w3.org/1999/02/22-rdf-syntax-ns#type> <http://www.w3.org/2002/07/owl#Class> .
<https://w3id.org/italia/social-security/onto/core/SedeINPS> <http://www.w3.org/2000/01/rdf-schema#subClassOf> <https://w3id.org/italia/onto/COV/HomogeneousOrganizationalArea> .
<https://w3id.org/italia/social-security/onto/core/SedeINPS> <http://www.w3.org/2000/01/rdf-schema#subClassOf> _:genid17 .
<https://w3id.org/italia/social-security/onto/core/SedeINPS> <http://www.w3.org/2000/01/rdf-schema#subClassOf> _:genid20 .
<https://w3id.org/italia/social-security/onto/core/SedeINPS> <http://www.w3.org/2000/01/rdf-schema#comment> "INPS is divided into central, regional and metropolitan structures with guidance, monitoring and coordination tasks, and into territorial offices with operational and user contact functions. In particular, the Institute, throughout the Italian national territory, has set up a \"service network\" organization which, in a \"proximity\" logic, is divided into: metropolitan coordination structures, provincial level structures, regional structures. Each INPS office is similar to a Homogeneous Organizational Area (AOO), each benefiting from a single entry and/or exit document flow (IT Protocol service) for the provision of services and the receipt of requests. In this sense, each INPS office is assigned, in addition to an office code assigned by the Institute, also a unique AOO identification code within the Index of Public Administrations (IPA) which makes it possible to identify the telematic communication channels legally permitted that is, at least one certified mailbox for each AOO. The competent INPS office for a citizen and/or company is established on the basis of the citizen's residence and/or the address of the company headquarters."@en .
<https://w3id.org/italia/social-security/onto/core/SedeINPS> <http://www.w3.org/2000/01/rdf-schema#comment> "L\u2019INPS \u00E8 articolato in strutture centrali, regionali e metropolitane con compiti di indirizzo, monitoraggio e coordinamento, e in sedi territoriali con funzioni operative e di contatto con l\u2019utenza. In particolare, l\u2019Istituto, su tutto il territorio nazionale italiano, si \u00E8 dotato di un\u2019organizzazione \u201Ca reti di servizio\u201D che, in logica di \u201Cprossimit\u00E0\u201D, si suddivide in: strutture di coordinamento metropolitano, strutture a livello provinciale, strutture a livello regionale. Ogni sede INPS \u00E8 assimilabile ad un Area Organizzativa Omogenea (AOO) usufruendo ciascuna per l'erogazione di servizi e il ricevimento delle richieste, di un unico flusso documentale di entrata e/o uscita (servizio di Protocollo Informatico). In tal senso ad ogni Sede INPS \u00E8 assegnato, oltre ad un codice di sede attribuito dall'Istituto, anche un codice identificativo AOO univoco nell'ambito dell'Indice delle Pubbliche Amministrazioni (IPA) che permette di individuare i canali di comunicazione telematica normativamente pervisti e cio\u00E8 almeno una casella di posta elettronica certificata per ciascun AOO. La sede INPS competente per un cittadino e/o un'impresa \u00E8 stabilita in base alla residenza del cittadino e/o all'indirizzo della sede dell'impresa."@it .
<https://w3id.org/italia/social-security/onto/core/SedeINPS> <http://www.w3.org/2000/01/rdf-schema#label> "INPS Office"@en .
<https://w3id.org/italia/social-security/onto/core/SedeINPS> <http://www.w3.org/2000/01/rdf-schema#label> "Sede INPS"@it .
_:genid17 <http://www.w3.org/1999/02/22-rdf-syntax-ns#type> <http://www.w3.org/2002/07/owl#Restriction> .
_:genid17 <http://www.w3.org/2002/07/owl#onProperty> <https://w3id.org/italia/onto/COV/hasPublicOrganization> .
_:genid17 <http://www.w3.org/2002/07/owl#someValuesFrom> _:genid18 .
_:genid18 <http://www.w3.org/1999/02/22-rdf-syntax-ns#type> <http://www.w3.org/2002/07/owl#Class> .
_:genid18 <http://www.w3.org/2002/07/owl#oneOf> _:genid19 .
_:genid19 <http://www.w3.org/1999/02/22-rdf-syntax-ns#first> <https://w3id.org/italia/social-security/onto/core/INPS> .
_:genid19 <http://www.w3.org/1999/02/22-rdf-syntax-ns#rest> <http://www.w3.org/1999/02/22-rdf-syntax-ns#nil> .
_:genid20 <http://www.w3.org/1999/02/22-rdf-syntax-ns#type> <http://www.w3.org/2002/07/owl#Restriction> .
_:genid20 <http://www.w3.org/2002/07/owl#onProperty> <https://w3id.org/italia/social-security/onto/core/codiceSedeINPS> .
_:genid20 <http://www.w3.org/2002/07/owl#someValuesFrom> <http://www.w3.org/2000/01/rdf-schema#Literal> .
<https://w3id.org/italia/social-security/onto/core/INPS> <http://www.w3.org/1999/02/22-rdf-syntax-ns#type> <http://www.w3.org/2002/07/owl#NamedIndividual> .
<https://w3id.org/italia/social-security/onto/core/INPS> <http://www.w3.org/1999/02/22-rdf-syntax-ns#type> <https://w3id.org/italia/onto/COV/PublicOrganization> .
<https://w3id.org/italia/social-security/onto/core/INPS> <http://www.w3.org/2000/01/rdf-schema#comment> "L'Istituto Nazionale della Previdenza Sociale \u00E8 l'Ente Pubblico che gestisce la liquidazione e il pagamento delle pensioni e delle indennit\u00E0 di natura previdenziale e assistenziale. Le pensioni sono prestazioni previdenziali, determinate sulla base di rapporti assicurativi e finanziate con i contributi di lavoratori e aziende pubbliche e private. Invece, le prestazioni assistenziali o \u201Ca sostegno del reddito\u201D tutelano i lavoratori che si trovano in particolari momenti di difficolt\u00E0 della loro vita lavorativa e provvedono al pagamento di somme destinate a coloro che hanno redditi modesti e famiglie numerose. Per alcune di queste prestazioni l\u2019INPS \u00E8 coinvolto solo nella fase di erogazione, mentre per altre svolge tutto il procedimento di assegnazione."@it .
<https://w3id.org/italia/social-security/onto/core/INPS> <http://www.w3.org/2000/01/rdf-schema#comment> "The National Institute for Social Security is the Italian Public Organization that supplies pensions and other services of social security to who has the right. It also does contributory activity collecting the contributions. The services are based on a mandatory insurance relationship and are funded with the contributions of employed workers, elaborated as a percentage of the wage. It also manages welfare services or \"income support\" services that protect workers who find themselves in particular difficult moments in their working life and provide for the payment of sums intended for those with modest incomes and large families."@en .
<https://w3id.org/italia/social-security/onto/core/INPS> <http://www.w3.org/2000/01/rdf-schema#label> "INPS"@en .
<https://w3id.org/italia/social-security/onto/core/INPS> <http://www.w3.org/2000/01/rdf-schema#label> "INPS"@it .
_:genid21 <http://www.w3.org/1999/02/22-rdf-syntax-ns#type> <http://www.w3.org/2002/07/owl#Class> .
_:genid21 <http://www.w3.org/2002/07/owl#oneOf> _:genid22 .
_:genid21 <http://www.w3.org/2000/01/rdf-schema#subClassOf> <https://w3id.org/italia/onto/COV/PublicOrganization> .
_:genid22 <http://www.w3.org/1999/02/22-rdf-syntax-ns#first> <https://w3id.org/italia/social-security/onto/core/INPS> .
_:genid22 <http://www.w3.org/1999/02/22-rdf-syntax-ns#rest> <http://www.w3.org/1999/02/22-rdf-syntax-ns#nil> .
_:genid23 <http://www.w3.org/1999/02/22-rdf-syntax-ns#type> <http://www.w3.org/2002/07/owl#Restriction> .
_:genid23 <http://www.w3.org/2002/07/owl#onProperty> _:genid24 .
_:genid23 <http://www.w3.org/2002/07/owl#someValuesFrom> _:genid25 .
_:genid23 <http://www.w3.org/2000/01/rdf-schema#subClassOf> _:genid27 .
_:genid24 <http://www.w3.org/2002/07/owl#inverseOf> <https://w3id.org/italia/onto/CLV/hasAddressComponent> .
_:genid25 <http://www.w3.org/1999/02/22-rdf-syntax-ns#type> <http://www.w3.org/2002/07/owl#Restriction> .
_:genid25 <http://www.w3.org/2002/07/owl#onProperty> _:genid26 .
_:genid25 <http://www.w3.org/2002/07/owl#someValuesFrom> <https://w3id.org/italia/onto/COV/Organization> .
_:genid26 <http://www.w3.org/2002/07/owl#inverseOf> <https://w3id.org/italia/onto/CLV/hasPrimaryAddress> .
_:genid27 <http://www.w3.org/1999/02/22-rdf-syntax-ns#type> <http://www.w3.org/2002/07/owl#Restriction> .
_:genid27 <http://www.w3.org/2002/07/owl#onProperty> _:genid28 .
_:genid27 <http://www.w3.org/2002/07/owl#someValuesFrom> _:genid29 .
_:genid28 <http://www.w3.org/2002/07/owl#inverseOf> <https://w3id.org/italia/onto/CLV/hasAddressComponent> .
_:genid29 <http://www.w3.org/1999/02/22-rdf-syntax-ns#type> <http://www.w3.org/2002/07/owl#Restriction> .
_:genid29 <http://www.w3.org/2002/07/owl#onProperty> _:genid30 .
_:genid29 <http://www.w3.org/2002/07/owl#someValuesFrom> _:genid31 .
_:genid30 <http://www.w3.org/2002/07/owl#inverseOf> <https://w3id.org/italia/onto/CLV/hasAddress> .
_:genid31 <http://www.w3.org/1999/02/22-rdf-syntax-ns#type> <http://www.w3.org/2002/07/owl#Restriction> .
_:genid31 <http://www.w3.org/2002/07/owl#onProperty> _:genid32 .
_:genid31 <http://www.w3.org/2002/07/owl#someValuesFrom> <http://www.w3.org/2002/07/owl#Thing> .
_:genid32 <http://www.w3.org/2002/07/owl#inverseOf> <https://w3id.org/italia/social-security/onto/core/haSedeINPS> .
_:genid33 <http://www.w3.org/1999/02/22-rdf-syntax-ns#type> <http://www.w3.org/2002/07/owl#Restriction> .
_:genid33 <http://www.w3.org/2002/07/owl#onProperty> _:genid34 .
_:genid33 <http://www.w3.org/2002/07/owl#someValuesFrom> _:genid35 .
_:genid33 <http://www.w3.org/2000/01/rdf-schema#subClassOf> _:genid37 .
_:genid34 <http://www.w3.org/2002/07/owl#inverseOf> <https://w3id.org/italia/onto/CLV/hasAddressComponent> .
_:genid35 <http://www.w3.org/1999/02/22-rdf-syntax-ns#type> <http://www.w3.org/2002/07/owl#Restriction> .
_:genid35 <http://www.w3.org/2002/07/owl#onProperty> _:genid36 .
_:genid35 <http://www.w3.org/2002/07/owl#someValuesFrom> <https://w3id.org/italia/onto/CPV/Alive> .
_:genid36 <http://www.w3.org/2002/07/owl#inverseOf> <https://w3id.org/italia/onto/CPV/hasCurrentResidence> .
_:genid37 <http://www.w3.org/1999/02/22-rdf-syntax-ns#type> <http://www.w3.org/2002/07/owl#Restriction> .
_:genid37 <http://www.w3.org/2002/07/owl#onProperty> _:genid38 .
_:genid37 <http://www.w3.org/2002/07/owl#someValuesFrom> _:genid39 .
_:genid38 <http://www.w3.org/2002/07/owl#inverseOf> <https://w3id.org/italia/onto/CLV/hasAddressComponent> .
_:genid39 <http://www.w3.org/1999/02/22-rdf-syntax-ns#type> <http://www.w3.org/2002/07/owl#Restriction> .
_:genid39 <http://www.w3.org/2002/07/owl#onProperty> _:genid40 .
_:genid39 <http://www.w3.org/2002/07/owl#someValuesFrom> _:genid41 .
_:genid40 <http://www.w3.org/2002/07/owl#inverseOf> <https://w3id.org/italia/onto/CLV/hasAddress> .
_:genid41 <http://www.w3.org/1999/02/22-rdf-syntax-ns#type> <http://www.w3.org/2002/07/owl#Restriction> .
_:genid41 <http://www.w3.org/2002/07/owl#onProperty> _:genid42 .
_:genid41 <http://www.w3.org/2002/07/owl#someValuesFrom> <http://www.w3.org/2002/07/owl#Thing> .
_:genid42 <http://www.w3.org/2002/07/owl#inverseOf> <https://w3id.org/italia/social-security/onto/core/haSedeINPS> .
_:genid43 <http://www.w3.org/1999/02/22-rdf-syntax-ns#type> <http://www.w3.org/2002/07/owl#Restriction> .
_:genid43 <http://www.w3.org/2002/07/owl#onProperty> _:genid44 .
_:genid43 <http://www.w3.org/2002/07/owl#someValuesFrom> <https://w3id.org/italia/onto/COV/Organization> .
_:genid43 <http://www.w3.org/2000/01/rdf-schema#subClassOf> <https://w3id.org/italia/social-security/onto/core/RuoloDiOrganizzazione> .
_:genid44 <http://www.w3.org/2002/07/owl#inverseOf> <https://w3id.org/italia/onto/RO/holdsRoleInTime> .
_:genid45 <http://www.w3.org/1999/02/22-rdf-syntax-ns#type> <http://www.w3.org/2002/07/owl#Restriction> .
_:genid45 <http://www.w3.org/2002/07/owl#onProperty> _:genid46 .
_:genid45 <http://www.w3.org/2002/07/owl#someValuesFrom> <https://w3id.org/italia/onto/CPV/Alive> .
_:genid45 <http://www.w3.org/2000/01/rdf-schema#subClassOf> <https://w3id.org/italia/social-security/onto/core/RuoloDiPersonaViva> .
_:genid46 <http://www.w3.org/2002/07/owl#inverseOf> <https://w3id.org/italia/onto/RO/holdsRoleInTime> .
_:genid47 <http://www.w3.org/1999/02/22-rdf-syntax-ns#type> <http://www.w3.org/2002/07/owl#Restriction> .
_:genid47 <http://www.w3.org/2002/07/owl#onProperty> _:genid48 .
_:genid47 <http://www.w3.org/2002/07/owl#someValuesFrom> <https://w3id.org/italia/onto/CPV/Dead> .
_:genid47 <http://www.w3.org/2000/01/rdf-schema#subClassOf> <https://w3id.org/italia/social-security/onto/core/RuoloDiPersonaDeceduta> .
_:genid48 <http://www.w3.org/2002/07/owl#inverseOf> <https://w3id.org/italia/onto/RO/holdsRoleInTime> .
_:genid49 <http://www.w3.org/1999/02/22-rdf-syntax-ns#type> <http://www.w3.org/2002/07/owl#Restriction> .
_:genid49 <http://www.w3.org/2002/07/owl#onProperty> _:genid50 .
_:genid49 <http://www.w3.org/2002/07/owl#someValuesFrom> <https://w3id.org/italia/onto/CPV/Person> .
_:genid49 <http://www.w3.org/2000/01/rdf-schema#subClassOf> <https://w3id.org/italia/social-security/onto/core/RuoloDiPersona> .
_:genid50 <http://www.w3.org/2002/07/owl#inverseOf> <https://w3id.org/italia/onto/RO/holdsRoleInTime> .
_:genid51 <http://www.w3.org/1999/02/22-rdf-syntax-ns#type> <http://www.w3.org/2002/07/owl#Restriction> .
_:genid51 <http://www.w3.org/2002/07/owl#onProperty> _:genid52 .
_:genid51 <http://www.w3.org/2002/07/owl#someValuesFrom> _:genid53 .
_:genid51 <http://www.w3.org/2000/01/rdf-schema#subClassOf> <https://w3id.org/italia/social-security/onto/core/RuoloDiAgente> .
_:genid52 <http://www.w3.org/2002/07/owl#inverseOf> <https://w3id.org/italia/onto/RO/holdsRoleInTime> .
_:genid53 <http://www.w3.org/1999/02/22-rdf-syntax-ns#type> <http://www.w3.org/2002/07/owl#Class> .
_:genid53 <http://www.w3.org/2002/07/owl#unionOf> _:genid54 .
_:genid54 <http://www.w3.org/1999/02/22-rdf-syntax-ns#first> <https://w3id.org/italia/onto/COV/Organization> .
_:genid54 <http://www.w3.org/1999/02/22-rdf-syntax-ns#rest> _:genid55 .
_:genid55 <http://www.w3.org/1999/02/22-rdf-syntax-ns#first> <https://w3id.org/italia/onto/CPV/Person> .
_:genid55 <http://www.w3.org/1999/02/22-rdf-syntax-ns#rest> <http://www.w3.org/1999/02/22-rdf-syntax-ns#nil> .
<https://w3id.org/italia/social-security/data/core/distribution/CORE-N-TRIPLES> <http://www.w3.org/1999/02/22-rdf-syntax-ns#type> <https://w3id.org/italia/onto/ADMS/SemanticAssetDistribution> .
<https://w3id.org/italia/social-security/data/core/distribution/CORE-N-TRIPLES> <http://www.w3.org/1999/02/22-rdf-syntax-ns#type> <http://www.w3.org/ns/dcat#Distribution> .
<https://w3id.org/italia/social-security/data/core/distribution/CORE-N-TRIPLES> <http://www.w3.org/1999/02/22-rdf-syntax-ns#type> <http://dati.gov.it/onto/dcatapit#Distribution> .
<https://w3id.org/italia/social-security/data/core/distribution/CORE-N-TRIPLES> <http://www.w3.org/1999/02/22-rdf-syntax-ns#type> <http://www.w3.org/2002/07/owl#NamedIndividual> .
<https://w3id.org/italia/social-security/data/core/distribution/CORE-N-TRIPLES> <http://www.w3.org/ns/dcat#accessURL> <https://github.com/INPS-it/NDC/tree/main/assets/ontologies/core/latest> .
<https://w3id.org/italia/social-security/data/core/distribution/CORE-N-TRIPLES> <http://www.w3.org/ns/dcat#downloadURL> <https://raw.githubusercontent.com/INPS-it/NDC/main/assets/ontologies/core/latest/core.n3> .
<https://w3id.org/italia/social-security/data/core/distribution/CORE-N-TRIPLES> <http://purl.org/dc/terms/description> "Questa \u00E8 la distribuzione N-TRIPLES dell'ontologia INPS relativa alle componenti del dominio funzionale dell'istituto comuni a procedure e servizi svolti dall'ente stesso. Tra di essi troviamo, ad esempio, le dislocazioni territoriali, come le sedi, e le entit\u00E0 astratte, come i ruoli."@it .
<https://w3id.org/italia/social-security/data/core/distribution/CORE-N-TRIPLES> <http://purl.org/dc/terms/description> "This is the distribution in N-TRIPLES of the INPS Ontology about components of the institution's functional domain common to procedures and services performed by the institution itself. These include, for example, territorial dislocations, such as locations, and abstract entities, such as roles."@en .
<https://w3id.org/italia/social-security/data/core/distribution/CORE-N-TRIPLES> <http://purl.org/dc/terms/format> <http://publications.europa.eu/resource/authority/file-type/RDF_N_TRIPLES> .
<https://w3id.org/italia/social-security/data/core/distribution/CORE-N-TRIPLES> <http://purl.org/dc/terms/license> <http://creativecommons.org/licenses/by/4.0/> .
<https://w3id.org/italia/social-security/data/core/distribution/CORE-N-TRIPLES> <http://purl.org/dc/terms/title> "Distribuzione N-TRIPLES dell'ontologia INPS - Core"@it .
<https://w3id.org/italia/social-security/data/core/distribution/CORE-N-TRIPLES> <http://purl.org/dc/terms/title> "N-TRIPLES distribution of the INPS ontology - Core"@en .
<https://w3id.org/italia/social-security/data/core/distribution/CORE-RDF-TURTLE> <http://www.w3.org/1999/02/22-rdf-syntax-ns#type> <https://w3id.org/italia/onto/ADMS/SemanticAssetDistribution> .
<https://w3id.org/italia/social-security/data/core/distribution/CORE-RDF-TURTLE> <http://www.w3.org/1999/02/22-rdf-syntax-ns#type> <http://www.w3.org/ns/dcat#Distribution> .
<https://w3id.org/italia/social-security/data/core/distribution/CORE-RDF-TURTLE> <http://www.w3.org/1999/02/22-rdf-syntax-ns#type> <http://dati.gov.it/onto/dcatapit#Distribution> .
<https://w3id.org/italia/social-security/data/core/distribution/CORE-RDF-TURTLE> <http://www.w3.org/1999/02/22-rdf-syntax-ns#type> <http://www.w3.org/2002/07/owl#NamedIndividual> .
<https://w3id.org/italia/social-security/data/core/distribution/CORE-RDF-TURTLE> <http://www.w3.org/ns/dcat#accessURL> <https://github.com/INPS-it/NDC/tree/main/assets/ontologies/core/latest> .
<https://w3id.org/italia/social-security/data/core/distribution/CORE-RDF-TURTLE> <http://www.w3.org/ns/dcat#downloadURL> <https://raw.githubusercontent.com/INPS-it/NDC/main/assets/ontologies/core/latest/core.ttl> .
<https://w3id.org/italia/social-security/data/core/distribution/CORE-RDF-TURTLE> <http://purl.org/dc/terms/description> "Questa \u00E8 la distribuzione RDF/Turtle dell'ontologia INPS relativa alle componenti del dominio funzionale dell'istituto comuni a procedure e servizi svolti dall'ente stesso. Tra di essi troviamo, ad esempio, le dislocazioni territoriali, come le sedi, e le entit\u00E0 astratte, come i ruoli."@it .
<https://w3id.org/italia/social-security/data/core/distribution/CORE-RDF-TURTLE> <http://purl.org/dc/terms/description> "This is the distribution in RDF/Turtle of the INPS Ontology about components of the institution's functional domain common to procedures and services performed by the institution itself. These include, for example, territorial dislocations, such as locations, and abstract entities, such as roles."@en .
<https://w3id.org/italia/social-security/data/core/distribution/CORE-RDF-TURTLE> <http://purl.org/dc/terms/format> <http://publications.europa.eu/resource/authority/file-type/RDF_TURTLE> .
<https://w3id.org/italia/social-security/data/core/distribution/CORE-RDF-TURTLE> <http://purl.org/dc/terms/license> <http://creativecommons.org/licenses/by/4.0/> .
<https://w3id.org/italia/social-security/data/core/distribution/CORE-RDF-TURTLE> <http://purl.org/dc/terms/title> "Distribuzione RDF/Turtle dell'ontologia INPS - Core"@it .
<https://w3id.org/italia/social-security/data/core/distribution/CORE-RDF-TURTLE> <http://purl.org/dc/terms/title> "RDF/Turtle distribution of the INPS ontology - Core"@en .
<https://w3id.org/italia/social-security/data/core/distribution/CORE-RDF-XML> <http://www.w3.org/1999/02/22-rdf-syntax-ns#type> <https://w3id.org/italia/onto/ADMS/SemanticAssetDistribution> .
<https://w3id.org/italia/social-security/data/core/distribution/CORE-RDF-XML> <http://www.w3.org/1999/02/22-rdf-syntax-ns#type> <http://www.w3.org/ns/dcat#Distribution> .
<https://w3id.org/italia/social-security/data/core/distribution/CORE-RDF-XML> <http://www.w3.org/1999/02/22-rdf-syntax-ns#type> <http://dati.gov.it/onto/dcatapit#Distribution> .
<https://w3id.org/italia/social-security/data/core/distribution/CORE-RDF-XML> <http://www.w3.org/1999/02/22-rdf-syntax-ns#type> <http://www.w3.org/2002/07/owl#NamedIndividual> .
<https://w3id.org/italia/social-security/data/core/distribution/CORE-RDF-XML> <http://www.w3.org/ns/dcat#accessURL> <https://github.com/INPS-it/NDC/tree/main/assets/ontologies/core/latest> .
<https://w3id.org/italia/social-security/data/core/distribution/CORE-RDF-XML> <http://www.w3.org/ns/dcat#downloadURL> <https://raw.githubusercontent.com/INPS-it/NDC/main/assets/ontologies/core/latest/core.owl> .
<https://w3id.org/italia/social-security/data/core/distribution/CORE-RDF-XML> <http://purl.org/dc/terms/description> "Questa \u00E8 la distribuzione RDF/XML dell'ontologia INPS relativa alle componenti del dominio funzionale dell'istituto comuni a procedure e servizi svolti dall'ente stesso. Tra di essi troviamo, ad esempio, le dislocazioni territoriali, come le sedi, e le entit\u00E0 astratte, come i ruoli."@it .
<https://w3id.org/italia/social-security/data/core/distribution/CORE-RDF-XML> <http://purl.org/dc/terms/description> "This is the distribution in RDF/XML of the INPS Ontology about components of the institution's functional domain common to procedures and services performed by the institution itself. These include, for example, territorial dislocations, such as locations, and abstract entities, such as roles."@en .
<https://w3id.org/italia/social-security/data/core/distribution/CORE-RDF-XML> <http://purl.org/dc/terms/format> <http://publications.europa.eu/resource/authority/file-type/RDF_XML> .
<https://w3id.org/italia/social-security/data/core/distribution/CORE-RDF-XML> <http://purl.org/dc/terms/license> <http://creativecommons.org/licenses/by/4.0/> .
<https://w3id.org/italia/social-security/data/core/distribution/CORE-RDF-XML> <http://purl.org/dc/terms/title> "Distribuzione RDF/XML dell'ontologia INPS - Core"@it .
<https://w3id.org/italia/social-security/data/core/distribution/CORE-RDF-XML> <http://purl.org/dc/terms/title> "RDF/XML distribution of the INPS ontology - Core"@en .
<https://w3id.org/italia/social-security/data/organization/DirezioneCentraleTII> <http://www.w3.org/1999/02/22-rdf-syntax-ns#type> <http://dati.gov.it/onto/dcatapit#Organization> .
<https://w3id.org/italia/social-security/data/organization/DirezioneCentraleTII> <http://www.w3.org/1999/02/22-rdf-syntax-ns#type> <http://www.w3.org/2002/07/owl#NamedIndividual> .
<https://w3id.org/italia/social-security/data/organization/DirezioneCentraleTII> <http://www.w3.org/1999/02/22-rdf-syntax-ns#type> <http://www.w3.org/2006/vcard/ns#Kind> .
<https://w3id.org/italia/social-security/data/organization/DirezioneCentraleTII> <http://www.w3.org/1999/02/22-rdf-syntax-ns#type> <http://www.w3.org/2006/vcard/ns#Organization> .
<https://w3id.org/italia/social-security/data/organization/DirezioneCentraleTII> <http://purl.org/dc/terms/identifier> "DirezioneCentraleTII" .
<https://w3id.org/italia/social-security/data/organization/DirezioneCentraleTII> <http://xmlns.com/foaf/0.1/name> "Central Management of Information Technology and Innovations"@en .
<https://w3id.org/italia/social-security/data/organization/DirezioneCentraleTII> <http://xmlns.com/foaf/0.1/name> "Direzione Centrale Tecnologia, Informatica e Innovazione"@it .
<https://w3id.org/italia/social-security/data/organization/DirezioneCentraleTII> <http://www.w3.org/2006/vcard/ns#fn> "Direzione Centrale Tecnologia, Informatica e Innovazione" .
<https://w3id.org/italia/social-security/data/organization/DirezioneCentraleTII> <http://www.w3.org/2006/vcard/ns#hasEmail> <mailto:dc.tecnologiainformaticaeinnovazione@postacert.inps.gov.it> .
<https://w3id.org/italia/social-security/data/organization/inps> <http://www.w3.org/1999/02/22-rdf-syntax-ns#type> <https://w3id.org/italia/onto/COV/PublicOrganization> .
<https://w3id.org/italia/social-security/data/organization/inps> <http://www.w3.org/1999/02/22-rdf-syntax-ns#type> <http://dati.gov.it/onto/dcatapit#Agent> .
<https://w3id.org/italia/social-security/data/organization/inps> <http://www.w3.org/1999/02/22-rdf-syntax-ns#type> <http://xmlns.com/foaf/0.1/Agent> .
<https://w3id.org/italia/social-security/data/organization/inps> <http://www.w3.org/1999/02/22-rdf-syntax-ns#type> <http://www.w3.org/2002/07/owl#NamedIndividual> .
<https://w3id.org/italia/social-security/data/organization/inps> <http://purl.org/dc/terms/identifier> "inps" .
<https://w3id.org/italia/social-security/data/organization/inps> <http://xmlns.com/foaf/0.1/name> "Istituto nazionale della previdenza sociale"@it .
<https://w3id.org/italia/social-security/data/organization/inps> <http://xmlns.com/foaf/0.1/name> "National institute for Social Security"@en .
<https://w3id.org/italia/social-security/data/organization/td> <http://www.w3.org/1999/02/22-rdf-syntax-ns#type> <http://dati.gov.it/onto/dcatapit#Agent> .
<https://w3id.org/italia/social-security/data/organization/td> <http://www.w3.org/1999/02/22-rdf-syntax-ns#type> <http://xmlns.com/foaf/0.1/Agent> .
<https://w3id.org/italia/social-security/data/organization/td> <http://www.w3.org/1999/02/22-rdf-syntax-ns#type> <http://www.w3.org/2002/07/owl#NamedIndividual> .
<https://w3id.org/italia/social-security/data/organization/td> <http://purl.org/dc/terms/identifier> "TD" .
<https://w3id.org/italia/social-security/data/organization/td> <http://xmlns.com/foaf/0.1/name> "Digital Transformation Team"@en .
<https://w3id.org/italia/social-security/data/organization/td> <http://xmlns.com/foaf/0.1/name> "Team per la Trasformazione Digitale"@it .