<?xml version="1.0"?>
<rdf:RDF xmlns="https://w3id.org/italia/onto/OP21/"
     xml:base="https://w3id.org/italia/onto/OP21/"
     xmlns:adms="https://w3id.org/italia/onto/ADMS/"
     xmlns:L0="https://w3id.org/italia/onto/l0/"
     xmlns:owl="http://www.w3.org/2002/07/owl#"
     xmlns:swrlb="http://www.w3.org/2003/11/swrlb#"
     xmlns:CPV="https://w3id.org/italia/onto/CPV/"
     xmlns:swrl="http://www.w3.org/2003/11/swrl#"
     xmlns:xsd="http://www.w3.org/2001/XMLSchema#"
     xmlns:skos="http://www.w3.org/2004/02/skos/core#"
     xmlns:rdfs="http://www.w3.org/2000/01/rdf-schema#"
     xmlns:COV="https://w3id.org/italia/onto/COV/"
     xmlns:vcard="http://www.w3.org/2006/vcard/ns#"
     xmlns:CLV="https://w3id.org/italia/onto/CLV/"
	 xmlns:prov="http://www.w3.org/ns/prov#"
     xmlns:op21="https://w3id.org/italia/onto/OP21/"
     xmlns:dct="http://purl.org/dc/terms/"
     xmlns:rdf="http://www.w3.org/1999/02/22-rdf-syntax-ns#"
     xmlns:TI="https://w3id.org/italia/onto/TI/"
     xmlns:xml="http://www.w3.org/XML/1998/namespace"
     xmlns:dcatapit="http://dati.gov.it/onto/dcatapit#"
     xmlns:time="http://www.w3.org/2006/time#"
     xmlns:dcat="http://www.w3.org/ns/dcat#"
     xmlns:RO="https://w3id.org/italia/onto/RO/"
     xmlns:foaf="http://xmlns.com/foaf/0.1/"
     xmlns:dc="http://purl.org/dc/elements/1.1/">
    <owl:Ontology rdf:about="https://w3id.org/italia/onto/OP21/">
        <owl:versionIRI rdf:resource="https://w3id.org/italia/onto/OP21/1.1"/>
        <adms:last rdf:resource="https://w3id.org/italia/onto/OP21/1.1"/>
        <dct:modified rdf:datatype="http://www.w3.org/2001/XMLSchema#dateTime">2023-03-30T00:00:00Z</dct:modified>
        <dcat:keyword xml:lang="it">Ricongiunzione</dcat:keyword>
        <adms:target xml:lang="it">Cittadini</adms:target>
        <dcat:keyword xml:lang="en">Redemption Application</dcat:keyword>
        <owl:versionInfo xml:lang="it">Versione 1.1 - Modificata il 30 Marzo 2023</owl:versionInfo>
        <dcat:keyword xml:lang="en">Domestic Worker</dcat:keyword>
        <dct:description xml:lang="it">Ontologia INPS relativa alle pratiche di Riscatto, Ricongiunzione e Rendita, e al Lavoratore Domestico.</dct:description>
        <rdfs:isDefinedBy rdf:resource="https://w3id.org/italia/onto/OP21"/>
        <adms:hasKeyClass rdf:resource="https://w3id.org/italia/onto/OP21/PraticaDiRiscatto"/>
        <adms:type rdf:resource="https://w3id.org/italia/onto/ADMS/ServiceOntology"/>
        <dcat:keyword xml:lang="it">Lavoratore Domestico</dcat:keyword>
        <rdfs:label xml:lang="en">INPS Ontology about Redemption, Aggregation, Life Annuities and Domestic Worker</rdfs:label>
        <adms:target xml:lang="it">Pubbliche Amministrazioni</adms:target>
        <adms:hasSemanticAssetDistribution rdf:resource="https://w3id.org/italia/data/OP21/distribution/OP21-RDF-TURTLE"/>
		<adms:hasSemanticAssetDistribution rdf:resource="https://w3id.org/italia/data/OP21/distribution/OP21-N-TRIPLES"/>
		<adms:hasSemanticAssetDistribution rdf:resource="https://w3id.org/italia/data/OP21/distribution/OP21-RDF-XML"/>
        <dct:title xml:lang="it">Ontologia INPS relativa a Riscatti, Ricongiunzioni, Rendite e Lavoratore Domestico</dct:title>
        <dcat:contactPoint rdf:resource="https://w3id.org/italia/data/OP21/organization/DirezioneCentraleTII"/>
        <adms:semanticAssetInUse rdf:resource="https://w3id.org/italia/data/project/NDC"/>
        <owl:imports rdf:resource="https://w3id.org/italia/onto/TI/"/>
        <owl:versionInfo xml:lang="en">Version 1.1 - Modified on 30 March 2023</owl:versionInfo>
        <adms:hasTask rdf:resource="https://w3id.org/italia/onto/ADMS/QueryFormulationTask"/>
        <adms:status>catalogued</adms:status>
        <dct:description xml:lang="en">This is the ontology of the INPS Organization about Redemption, Aggregation and Life Annuity Application, and Domestic Worker.</dct:description>
        <owl:imports rdf:resource="https://w3id.org/italia/onto/l0/"/>
        <dcat:keyword xml:lang="en">Aggregation Application</dcat:keyword>
        <dcat:keyword xml:lang="it">Riscatto</dcat:keyword>
        <dct:accrualPeriodicity rdf:resource="http://publications.europa.eu/resource/authority/frequency/IRREG"/>
        <owl:imports rdf:resource="https://w3id.org/italia/onto/CLV/"/>
        <rdfs:comment xml:lang="it">Ontologia INPS relativa alle pratiche di Riscatto, Ricongiunzione e Rendita, e al Lavoratore Domestico.</rdfs:comment>
        <owl:imports rdf:resource="https://w3id.org/italia/onto/CPV/"/>
        <adms:hasOntologyLanguage rdf:resource="https://w3id.org/italia/onto/ADMS/OWL"/>
        <dct:title xml:lang="en">INPS Ontology about Redemption, Aggregation, Life Annuities and Domestic Worker</dct:title>
        <adms:hasFormalityLevel rdf:resource="https://w3id.org/italia/onto/ADMS/Formal"/>
        <dcat:theme rdf:resource="http://publications.europa.eu/resource/authority/data-theme/SOCI"/>
        <dct:rightsHolder rdf:resource="https://w3id.org/italia/data/OP21/organization/inps"/>
        <dcat:keyword xml:lang="it">Rendita</dcat:keyword>
        <adms:hasTask rdf:resource="https://w3id.org/italia/onto/ADMS/AnnotationTask"/>
        <adms:officialURI rdf:datatype="http://www.w3.org/2001/XMLSchema#anyURI">https://w3id.org/italia/onto/OP21/</adms:officialURI>
        <dct:language rdf:resource="http://publications.europa.eu/resource/authority/language/ENG"/>
        <adms:hasTask rdf:resource="https://w3id.org/italia/onto/ADMS/SearchTask"/>
        <rdfs:comment xml:lang="en">This is the ontology of the INPS Organization about Redemption, Aggregation and Life Annuity Application, and Domestic Worker.</rdfs:comment>
        <adms:hasContributor rdf:resource="https://w3id.org/italia/data/OP21/organization/td"/>
        <adms:hasKeyClass rdf:resource="https://w3id.org/italia/onto/OP21/PraticaDiRicongiunzione"/>
        <owl:imports rdf:resource="https://w3id.org/italia/onto/RO/"/>
        <dct:creator rdf:resource="https://w3id.org/italia/data/OP21/organization/inps"/>
        <dct:identifier>https://w3id.org/italia/onto/OP21/</dct:identifier>
        <adms:prefix>inpsproc21</adms:prefix>
		<prov:wasDerivedFrom rdf:resource="https://w3id.org/italia/onto/OP21/1.0"/>
		<adms:prev rdf:resource="https://w3id.org/italia/onto/OP21/1.0"/>
        <dct:language rdf:resource="http://publications.europa.eu/resource/authority/language/ITA"/>
        <adms:acronym>inps</adms:acronym>
        <rdfs:label xml:lang="it">Ontologia INPS relativa a Riscatti, Ricongiunzioni, Rendite e Lavoratore Domestico</rdfs:label>
        <dct:issued rdf:datatype="http://www.w3.org/2001/XMLSchema#dateTime">2023-01-03T00:00:00Z</dct:issued>
        <adms:target xml:lang="it">Imprese</adms:target>
        <dct:publisher rdf:resource="https://w3id.org/italia/data/OP21/organization/inps"/>
        <adms:status>published</adms:status>
        <dcat:keyword xml:lang="en">Life Annuities Application</dcat:keyword>
        <owl:imports rdf:resource="https://w3id.org/italia/onto/COV/"/>
        <adms:hasKeyClass rdf:resource="https://w3id.org/italia/onto/OP21/PraticaDiRendita"/>
        <adms:hasKeyClass rdf:resource="https://w3id.org/italia/onto/OP21/LavoratoreDomestico"/>
    </owl:Ontology>



    <!--
    ///////////////////////////////////////////////////////////////////////////////////////
    //
    // Annotation properties
    //
    ///////////////////////////////////////////////////////////////////////////////////////
     -->




    <!-- http://purl.org/dc/terms/description -->

    <owl:AnnotationProperty rdf:about="http://purl.org/dc/terms/description"/>



    <!-- http://purl.org/dc/terms/format -->

    <owl:AnnotationProperty rdf:about="http://purl.org/dc/terms/format"/>



    <!-- http://purl.org/dc/terms/identifier -->

    <owl:AnnotationProperty rdf:about="http://purl.org/dc/terms/identifier"/>



    <!-- http://purl.org/dc/terms/license -->

    <owl:AnnotationProperty rdf:about="http://purl.org/dc/terms/license"/>



    <!-- http://purl.org/dc/terms/title -->

    <owl:AnnotationProperty rdf:about="http://purl.org/dc/terms/title"/>



    <!-- http://www.w3.org/2006/vcard/ns#fn -->

    <owl:AnnotationProperty rdf:about="http://www.w3.org/2006/vcard/ns#fn"/>



    <!-- http://www.w3.org/2006/vcard/ns#hasEmail -->

    <owl:AnnotationProperty rdf:about="http://www.w3.org/2006/vcard/ns#hasEmail"/>



    <!-- http://www.w3.org/ns/dcat#accessURL -->

    <owl:AnnotationProperty rdf:about="http://www.w3.org/ns/dcat#accessURL"/>



    <!-- http://www.w3.org/ns/dcat#downloadURL -->

    <owl:AnnotationProperty rdf:about="http://www.w3.org/ns/dcat#downloadURL"/>



    <!-- http://xmlns.com/foaf/0.1/name -->

    <owl:AnnotationProperty rdf:about="http://xmlns.com/foaf/0.1/name"/>



    <!--
    ///////////////////////////////////////////////////////////////////////////////////////
    //
    // Datatypes
    //
    ///////////////////////////////////////////////////////////////////////////////////////
     -->




    <!-- http://www.w3.org/2001/XMLSchema#boolean -->

    <rdfs:Datatype rdf:about="http://www.w3.org/2001/XMLSchema#boolean"/>



    <!-- http://www.w3.org/2001/XMLSchema#dateTime -->

    <rdfs:Datatype rdf:about="http://www.w3.org/2001/XMLSchema#dateTime"/>



    <!-- http://www.w3.org/2001/XMLSchema#decimal -->

    <rdfs:Datatype rdf:about="http://www.w3.org/2001/XMLSchema#decimal"/>



    <!-- http://www.w3.org/2001/XMLSchema#integer -->

    <rdfs:Datatype rdf:about="http://www.w3.org/2001/XMLSchema#integer"/>



    <!-- http://www.w3.org/2001/XMLSchema#string -->

    <rdfs:Datatype rdf:about="http://www.w3.org/2001/XMLSchema#string"/>



    <!--
    ///////////////////////////////////////////////////////////////////////////////////////
    //
    // Object Properties
    //
    ///////////////////////////////////////////////////////////////////////////////////////
     -->




    <!-- https://w3id.org/italia/onto/CLV/hasAddress -->

    <owl:ObjectProperty rdf:about="https://w3id.org/italia/onto/CLV/hasAddress"/>



    <!-- https://w3id.org/italia/onto/CLV/hasAddressComponent -->

    <owl:ObjectProperty rdf:about="https://w3id.org/italia/onto/CLV/hasAddressComponent"/>



    <!-- https://w3id.org/italia/onto/CLV/hasPrimaryAddress -->

    <owl:ObjectProperty rdf:about="https://w3id.org/italia/onto/CLV/hasPrimaryAddress"/>



    <!-- https://w3id.org/italia/onto/COV/hasOrganizzation -->

    <owl:ObjectProperty rdf:about="https://w3id.org/italia/onto/COV/hasOrganizzation">
        <rdf:type rdf:resource="http://www.w3.org/2002/07/owl#FunctionalProperty"/>
        <rdfs:domain rdf:resource="https://w3id.org/italia/onto/OP21/SedeINPS"/>
        <rdfs:range rdf:resource="https://w3id.org/italia/onto/COV/PublicOrganization"/>
    </owl:ObjectProperty>



    <!-- https://w3id.org/italia/onto/CPV/hasCurrentResidence -->

    <owl:ObjectProperty rdf:about="https://w3id.org/italia/onto/CPV/hasCurrentResidence"/>



    <!-- https://w3id.org/italia/onto/CPV/hasParentalRelationshipWith -->

    <owl:ObjectProperty rdf:about="https://w3id.org/italia/onto/CPV/hasParentalRelationshipWith"/>



    <!-- https://w3id.org/italia/onto/OP21/accedeServizioDiPagamento -->

    <owl:ObjectProperty rdf:about="https://w3id.org/italia/onto/OP21/accedeServizioDiPagamento">
        <rdf:type rdf:resource="http://www.w3.org/2002/07/owl#InverseFunctionalProperty"/>
        <rdfs:domain rdf:resource="https://w3id.org/italia/onto/OP21/Pagatore"/>
        <rdfs:range rdf:resource="https://w3id.org/italia/onto/OP21/SessionePagamentoElettronico"/>
        <rdfs:comment xml:lang="en">Relationship linking a Debtor to an Electronic Payment Session. Each Session has a single Debtor who accesses the payment service.</rdfs:comment>
        <rdfs:comment xml:lang="it">Relazione che collega un Debitore ad una Sessione di Pagamento Elettronico. Ciascuna Sessione ha un unico Debitore che accede al servizio di pagamento.</rdfs:comment>
        <rdfs:label xml:lang="it">accede servizio di pagamento</rdfs:label>
        <rdfs:label xml:lang="en">access payment service</rdfs:label>
    </owl:ObjectProperty>



    <!-- https://w3id.org/italia/onto/OP21/attivaOrdineDiPagamento -->

    <owl:ObjectProperty rdf:about="https://w3id.org/italia/onto/OP21/attivaOrdineDiPagamento">
        <rdf:type rdf:resource="http://www.w3.org/2002/07/owl#FunctionalProperty"/>
        <rdf:type rdf:resource="http://www.w3.org/2002/07/owl#InverseFunctionalProperty"/>
        <rdfs:domain>
            <owl:Class>
                <owl:unionOf rdf:parseType="Collection">
                    <rdf:Description rdf:about="https://w3id.org/italia/onto/OP21/Pagamento"/>
                    <rdf:Description rdf:about="https://w3id.org/italia/onto/OP21/PrenotazioneDiPagamento"/>
                </owl:unionOf>
            </owl:Class>
        </rdfs:domain>
        <rdfs:range rdf:resource="https://w3id.org/italia/onto/OP21/OrdineDiPagamento"/>
        <rdfs:comment xml:lang="en">Relationship linking a Payment or Payment Reservation to a Payment Order.</rdfs:comment>
        <rdfs:comment xml:lang="it">Relazione che collega un Pagamento o una Prenotazione di Pagamento a un Ordine di Pagamento.</rdfs:comment>
        <rdfs:label xml:lang="en">activates payment order</rdfs:label>
        <rdfs:label xml:lang="it">attiva ordine di pagamento</rdfs:label>
    </owl:ObjectProperty>



    <!-- https://w3id.org/italia/onto/OP21/autorizzaMandato -->

    <owl:ObjectProperty rdf:about="https://w3id.org/italia/onto/OP21/autorizzaMandato">
        <rdf:type rdf:resource="http://www.w3.org/2002/07/owl#FunctionalProperty"/>
        <rdfs:domain rdf:resource="https://w3id.org/italia/onto/OP21/AttoDiAttivazioneMandato"/>
        <rdfs:range rdf:resource="https://w3id.org/italia/onto/OP21/MandatoSDDAttivo"/>
        <rdfs:comment xml:lang="en">Relationship linking a Mandate Activation Deed to the Active SDD Mandate it authorizes. Each Activation Deed authorizes a single SDD Mandate.</rdfs:comment>
        <rdfs:comment xml:lang="it">Relazione che collega un Atto di Attivazione Mandato al Mandato SDD Attivo che autorizza. Ciascun Atto di Attivazione autorizza un unico Mandato SDD.</rdfs:comment>
        <rdfs:label xml:lang="en">authorizes mandate</rdfs:label>
        <rdfs:label xml:lang="it">autorizza mandato</rdfs:label>
    </owl:ObjectProperty>



    <!-- https://w3id.org/italia/onto/OP21/avvisoHaEnteCreditore -->

    <owl:ObjectProperty rdf:about="https://w3id.org/italia/onto/OP21/avvisoHaEnteCreditore">
        <rdf:type rdf:resource="http://www.w3.org/2002/07/owl#FunctionalProperty"/>
        <rdfs:domain rdf:resource="https://w3id.org/italia/onto/OP21/AvvisoDiPagamento"/>
        <rdfs:range rdf:resource="https://w3id.org/italia/onto/OP21/EnteCreditore"/>
        <rdfs:comment xml:lang="en">Functional link between the Payment Notice and the Creditor Institution demanding the payment.</rdfs:comment>
        <rdfs:comment xml:lang="it">Legame funzionale tra l&apos;Avviso Di Pagamento e l&apos;Ente Creditore che esige il pagamento.</rdfs:comment>
        <rdfs:label xml:lang="it">avviso ha ente creditore</rdfs:label>
        <rdfs:label xml:lang="en">notice has creditor institution</rdfs:label>
    </owl:ObjectProperty>



    <!-- https://w3id.org/italia/onto/OP21/depositoAvvioRapporto -->

    <owl:ObjectProperty rdf:about="https://w3id.org/italia/onto/OP21/depositoAvvioRapporto">
        <rdf:type rdf:resource="http://www.w3.org/2002/07/owl#FunctionalProperty"/>
        <rdfs:domain rdf:resource="https://w3id.org/italia/onto/OP21/RapportoDiLavoroDomesticoAttivo"/>
        <rdfs:range rdf:resource="https://w3id.org/italia/onto/COV/PublicOrganization"/>
        <rdfs:comment xml:lang="en">Relationship linking an Active Domestic Work Relationship to a Public Organization. Each Active Domestic Work Relationship is linked to a single Public Organization.</rdfs:comment>
        <rdfs:comment xml:lang="it">Relazione che collega un Rapporto di Lavoro Domestico Attivo ad un&apos;Organizzazione Pubblica. Ciascun Rapporto di Lavoro Domestico Attivo è collegato ad un&apos;unica Organizzazione Pubblica.</rdfs:comment>
        <rdfs:label xml:lang="it">deposito avvio rapporto</rdfs:label>
        <rdfs:label xml:lang="en">work relationship activation deposit</rdfs:label>
    </owl:ObjectProperty>



    <!-- https://w3id.org/italia/onto/OP21/depositoCessazioneRapporto -->

    <owl:ObjectProperty rdf:about="https://w3id.org/italia/onto/OP21/depositoCessazioneRapporto">
        <rdf:type rdf:resource="http://www.w3.org/2002/07/owl#FunctionalProperty"/>
        <rdfs:domain rdf:resource="https://w3id.org/italia/onto/OP21/RapportoDiLavoroDomesticoCessato"/>
        <rdfs:range rdf:resource="https://w3id.org/italia/onto/COV/PublicOrganization"/>
        <rdfs:comment xml:lang="en">Relationship linking a Terminated  Domestic Work Relationship to a Public Organization. Each Terminated Relationship is linked to a single Public Organization.</rdfs:comment>
        <rdfs:comment xml:lang="it">Relazione che collega un Rapporto di Lavoro Domestico Cessato ad un&apos;Organizzazione Pubblica. Ciascun Rapporto di Lavoro Domestico Cessato è collegato ad un&apos;unica Organizzazione Pubblica.</rdfs:comment>
        <rdfs:label xml:lang="it">deposito cessazione rapporto</rdfs:label>
        <rdfs:label xml:lang="en">work relationship termination deposit</rdfs:label>
    </owl:ObjectProperty>



    <!-- https://w3id.org/italia/onto/OP21/emetteAtto -->

    <owl:ObjectProperty rdf:about="https://w3id.org/italia/onto/OP21/emetteAtto">
        <rdf:type rdf:resource="http://www.w3.org/2002/07/owl#InverseFunctionalProperty"/>
        <rdfs:domain rdf:resource="https://w3id.org/italia/onto/OP21/SedeINPS"/>
        <rdfs:range rdf:resource="https://w3id.org/italia/onto/OP21/AttoAdeguamentoContributivo"/>
        <rdfs:comment xml:lang="it">Relazione che collega una Sede INPS ad un Atto di Adeguamento Contributivo emesso da questa. Ciascun Atto è emesso da un&apos;unica Sede INPS.</rdfs:comment>
        <rdfs:comment xml:lang="en">Report linking an INPS office to a Tax Adjustment Deed issued by it. Each deed is issued by a single INPS office.</rdfs:comment>
        <rdfs:label xml:lang="it">emette atto</rdfs:label>
        <rdfs:label xml:lang="en">issues deed</rdfs:label>
    </owl:ObjectProperty>



    <!-- https://w3id.org/italia/onto/OP21/emetteEsitoPagamento -->

    <owl:ObjectProperty rdf:about="https://w3id.org/italia/onto/OP21/emetteEsitoPagamento">
        <rdf:type rdf:resource="http://www.w3.org/2002/07/owl#InverseFunctionalProperty"/>
        <rdfs:domain rdf:resource="https://w3id.org/italia/onto/OP21/EnteCreditore"/>
        <rdfs:range rdf:resource="https://w3id.org/italia/onto/OP21/EsitoPagamento"/>
        <rdfs:comment xml:lang="en">Relationship linking a Creditor Authority to a Payment Outcome issued by it. Each outcome is issued by a single authority.</rdfs:comment>
        <rdfs:comment xml:lang="it">Relazione che collega un Ente Creditore ad un Esito Pagamento emesso da questo. Ciascun Esito è emesso da un unico Ente.</rdfs:comment>
        <rdfs:label xml:lang="it">emette esito pagamento</rdfs:label>
        <rdfs:label xml:lang="en">issues payment outcome</rdfs:label>
    </owl:ObjectProperty>



    <!-- https://w3id.org/italia/onto/OP21/esegueAccredito -->

    <owl:ObjectProperty rdf:about="https://w3id.org/italia/onto/OP21/esegueAccredito">
        <rdf:type rdf:resource="http://www.w3.org/2002/07/owl#FunctionalProperty"/>
        <rdf:type rdf:resource="http://www.w3.org/2002/07/owl#InverseFunctionalProperty"/>
        <rdfs:domain rdf:resource="https://w3id.org/italia/onto/OP21/OrdineDiPagamento"/>
        <rdfs:range rdf:resource="https://w3id.org/italia/onto/OP21/MovimentoDiDenaro"/>
        <rdfs:comment xml:lang="en">Relationship linking a Payment Order to a Money Movement.</rdfs:comment>
        <rdfs:comment xml:lang="it">Relazione che collega un Ordine di Pagamento ad un Movimento Di Denaro.</rdfs:comment>
        <rdfs:label xml:lang="it">esegue accredito</rdfs:label>
        <rdfs:label xml:lang="en">performs credit</rdfs:label>
    </owl:ObjectProperty>



    <!-- https://w3id.org/italia/onto/OP21/esegueAddebito -->

    <owl:ObjectProperty rdf:about="https://w3id.org/italia/onto/OP21/esegueAddebito">
        <rdf:type rdf:resource="http://www.w3.org/2002/07/owl#FunctionalProperty"/>
        <rdf:type rdf:resource="http://www.w3.org/2002/07/owl#InverseFunctionalProperty"/>
        <rdfs:domain rdf:resource="https://w3id.org/italia/onto/OP21/OrdineDiPagamento"/>
        <rdfs:range rdf:resource="https://w3id.org/italia/onto/OP21/MovimentoDiDenaro"/>
        <rdfs:comment xml:lang="en">Relationship linking a Payment Order to a Money Movement.</rdfs:comment>
        <rdfs:comment xml:lang="it">Relazione che collega un Ordine di Pagamento ad un Movimento Di Denaro.</rdfs:comment>
        <rdfs:label xml:lang="it">esegue addebito</rdfs:label>
        <rdfs:label xml:lang="en">performs charge</rdfs:label>
    </owl:ObjectProperty>



    <!-- https://w3id.org/italia/onto/OP21/eseguePagamento -->

    <owl:ObjectProperty rdf:about="https://w3id.org/italia/onto/OP21/eseguePagamento">
        <rdf:type rdf:resource="http://www.w3.org/2002/07/owl#InverseFunctionalProperty"/>
        <rdfs:domain rdf:resource="https://w3id.org/italia/onto/OP21/Pagatore"/>
        <rdfs:range rdf:resource="https://w3id.org/italia/onto/OP21/Pagamento"/>
        <rdfs:comment xml:lang="en">Relationship linking a Debtor to a Payment. Each Payment is made by a single Debtor.</rdfs:comment>
        <rdfs:comment xml:lang="it">Relazione che collega un Debitore ad un Pagamento. Ciascun Pagamento è eseguito da un unico Debitore.</rdfs:comment>
        <rdfs:label xml:lang="it">esegue pagamento</rdfs:label>
        <rdfs:label xml:lang="en">performs payment</rdfs:label>
    </owl:ObjectProperty>



    <!-- https://w3id.org/italia/onto/OP21/haAttoAdeguamentoContributivo -->

    <owl:ObjectProperty rdf:about="https://w3id.org/italia/onto/OP21/haAttoAdeguamentoContributivo">
        <rdf:type rdf:resource="http://www.w3.org/2002/07/owl#FunctionalProperty"/>
        <rdf:type rdf:resource="http://www.w3.org/2002/07/owl#InverseFunctionalProperty"/>
        <rdfs:domain rdf:resource="https://w3id.org/italia/onto/OP21/PraticaAdeguamentoContributivo"/>
        <rdfs:range rdf:resource="https://w3id.org/italia/onto/OP21/AttoAdeguamentoContributivo"/>
        <rdfs:comment xml:lang="en">Relationship linking a Tax Adjustment Applcation to a Tax Adjustment Deed.</rdfs:comment>
        <rdfs:comment xml:lang="it">Relazione che collega una Pratica di Adeguamento Contributivo ad un Atto di Adeguamento Contributivo.</rdfs:comment>
        <rdfs:label xml:lang="it">ha atto adeguamento contributivo</rdfs:label>
        <rdfs:label xml:lang="en">has tax adjustment deed</rdfs:label>
    </owl:ObjectProperty>



    <!-- https://w3id.org/italia/onto/OP21/haContoCorrente -->

    <owl:ObjectProperty rdf:about="https://w3id.org/italia/onto/OP21/haContoCorrente">
        <rdf:type rdf:resource="http://www.w3.org/2002/07/owl#FunctionalProperty"/>
        <rdf:type rdf:resource="http://www.w3.org/2002/07/owl#InverseFunctionalProperty"/>
        <rdfs:domain rdf:resource="https://w3id.org/italia/onto/OP21/Correntista"/>
        <rdfs:range rdf:resource="https://w3id.org/italia/onto/OP21/ContoCorrente"/>
        <rdfs:comment xml:lang="en">Relationship linking a Bank Account Holder to a Bank Account. Each Bank Account belongs to a single Bank Account Holder.</rdfs:comment>
        <rdfs:comment xml:lang="it">Relazione che collega un Correntista ad un Conto Corrente. Ciascun Conto Corrente appartiene ad un unico Correntista.</rdfs:comment>
        <rdfs:label xml:lang="it">ha conto corrente</rdfs:label>
        <rdfs:label xml:lang="en">has bank account</rdfs:label>
    </owl:ObjectProperty>



    <!-- https://w3id.org/italia/onto/OP21/haContributoTrimestraleFinale -->

    <owl:ObjectProperty rdf:about="https://w3id.org/italia/onto/OP21/haContributoTrimestraleFinale">
        <rdf:type rdf:resource="http://www.w3.org/2002/07/owl#InverseFunctionalProperty"/>
        <rdfs:domain rdf:resource="https://w3id.org/italia/onto/OP21/RapportoDiLavoroDomesticoCessato"/>
        <rdfs:range rdf:resource="https://w3id.org/italia/onto/OP21/ContributoTrimestraleFinale"/>
        <rdfs:comment xml:lang="it">Relazione che collega un Rapporto di Lavoro Domestico Cessato ad un Contributo Trimestrale Finale. Ciascun Contributo Trimestrale Finale è collegato ad un unico Rapporto di Lavoro.</rdfs:comment>
        <rdfs:comment xml:lang="en">Report linking a Ceased Domestic Work Relationship to a Final Quarterly Contribution. Each Final Quarterly Contribution is linked to a single Work Relationship.</rdfs:comment>
        <rdfs:label xml:lang="it">ha contributo trimestrale finale</rdfs:label>
        <rdfs:label xml:lang="en">has final quarterly contribution</rdfs:label>
    </owl:ObjectProperty>



    <!-- https://w3id.org/italia/onto/OP21/haContributoTrimestraleOrdinario -->

    <owl:ObjectProperty rdf:about="https://w3id.org/italia/onto/OP21/haContributoTrimestraleOrdinario">
        <rdf:type rdf:resource="http://www.w3.org/2002/07/owl#InverseFunctionalProperty"/>
        <rdfs:domain rdf:resource="https://w3id.org/italia/onto/OP21/RapportoDiLavoroDomesticoAttivo"/>
        <rdfs:range rdf:resource="https://w3id.org/italia/onto/OP21/ContributoTrimestraleOrdinario"/>
        <rdfs:comment xml:lang="en">Relationship linking an Active Domestic Work Relationship to an Ordinary Quarterly Contribution. Each Ordinary Quarterly Contribution is linked to a single Work Relationship.</rdfs:comment>
        <rdfs:comment xml:lang="it">Relazione che collega un Rapporto di Lavoro Domestico Attivo ad un Contributo Trimestrale Ordinario. Ciascun Contributo Trimestrale Ordinario è collegato ad un unico Rapporto di Lavoro.</rdfs:comment>
        <rdfs:label xml:lang="it">ha contributo trimestrale ordinario</rdfs:label>
        <rdfs:label xml:lang="en">has an ordinary quarterly contribution</rdfs:label>
    </owl:ObjectProperty>



    <!-- https://w3id.org/italia/onto/OP21/haCreditoreMandato -->

    <owl:ObjectProperty rdf:about="https://w3id.org/italia/onto/OP21/haCreditoreMandato">
        <rdf:type rdf:resource="http://www.w3.org/2002/07/owl#FunctionalProperty"/>
        <rdfs:domain rdf:resource="https://w3id.org/italia/onto/OP21/MandatoSDD"/>
        <rdfs:range rdf:resource="https://w3id.org/italia/onto/OP21/CreditoreMandato"/>
        <rdfs:comment xml:lang="en">Relationship linking an SDD Mandate to the Mandate Creditor.</rdfs:comment>
        <rdfs:comment xml:lang="it">Relazione che collega un Mandato SDD al Creditore del Mandato.</rdfs:comment>
        <rdfs:label xml:lang="it">ha creditore mandato</rdfs:label>
        <rdfs:label xml:lang="en">has mandate creditor</rdfs:label>
    </owl:ObjectProperty>



    <!-- https://w3id.org/italia/onto/OP21/haDatoreDiLavoro -->

    <owl:ObjectProperty rdf:about="https://w3id.org/italia/onto/OP21/haDatoreDiLavoro">
        <rdf:type rdf:resource="http://www.w3.org/2002/07/owl#FunctionalProperty"/>
        <rdfs:domain rdf:resource="https://w3id.org/italia/onto/OP21/RapportoDiLavoroDomestico"/>
        <rdfs:range rdf:resource="https://w3id.org/italia/onto/OP21/DatoreDiLavoroDomestico"/>
        <rdfs:comment xml:lang="en">Relationship linking a Domestic Work Relationship to a Domestic Work Employer. Each Employment Relationship has a single Employer.</rdfs:comment>
        <rdfs:comment xml:lang="it">Relazione che collega un Rapporto di Lavoro Domestico ad un Datore di Lavoro Domestico. Ciascun Rapporto di Lavoro ha un unico Datore di Lavoro.</rdfs:comment>
        <rdfs:label xml:lang="it">ha datore di lavoro</rdfs:label>
        <rdfs:label xml:lang="en">has employer</rdfs:label>
    </owl:ObjectProperty>



    <!-- https://w3id.org/italia/onto/OP21/haDebitoreMandato -->

    <owl:ObjectProperty rdf:about="https://w3id.org/italia/onto/OP21/haDebitoreMandato">
        <rdf:type rdf:resource="http://www.w3.org/2002/07/owl#FunctionalProperty"/>
        <rdfs:domain rdf:resource="https://w3id.org/italia/onto/OP21/MandatoSDD"/>
        <rdfs:range rdf:resource="https://w3id.org/italia/onto/OP21/DebitoreMandato"/>
        <rdfs:comment xml:lang="en">Relationship linking an SDD Mandate to the Mandate Debtor. Each Mandate has a single Debtor.</rdfs:comment>
        <rdfs:comment xml:lang="it">Relazione che collega un Mandato SDD al Debitore del Mandato. Ciascun Mandato ha un unico Debitore.</rdfs:comment>
        <rdfs:label xml:lang="it">ha debitore mandato</rdfs:label>
        <rdfs:label xml:lang="en">has mandate debtor</rdfs:label>
    </owl:ObjectProperty>



    <!-- https://w3id.org/italia/onto/OP21/haDomandaAdeguamentoContributivo -->

    <owl:ObjectProperty rdf:about="https://w3id.org/italia/onto/OP21/haDomandaAdeguamentoContributivo">
        <rdf:type rdf:resource="http://www.w3.org/2002/07/owl#InverseFunctionalProperty"/>
        <rdfs:domain rdf:resource="https://w3id.org/italia/onto/OP21/PraticaAdeguamentoContributivo"/>
        <rdfs:range rdf:resource="https://w3id.org/italia/onto/OP21/DomandaAdeguamentoContributivo"/>
        <rdfs:comment xml:lang="en">Relationship linking a Tax Adjustment Application to a Tax Adjustment Request. Each Request is linked to a single Application.</rdfs:comment>
        <rdfs:comment xml:lang="it">Relazione che collega una Pratica di Adeguamento Contributivo ad una Domanda di Adeguamento Contributivo. Ciascuna Domanda è collegata ad un&apos;unica Pratica.</rdfs:comment>
        <rdfs:label xml:lang="it">ha domanda adeguamento contributivo</rdfs:label>
        <rdfs:label xml:lang="en">has tax adjustment application</rdfs:label>
    </owl:ObjectProperty>



    <!-- https://w3id.org/italia/onto/OP21/haEsitoPagamento -->

    <owl:ObjectProperty rdf:about="https://w3id.org/italia/onto/OP21/haEsitoPagamento">
        <owl:inverseOf rdf:resource="https://w3id.org/italia/onto/OP21/riferiscePagamento"/>
        <rdf:type rdf:resource="http://www.w3.org/2002/07/owl#InverseFunctionalProperty"/>
        <rdfs:domain rdf:resource="https://w3id.org/italia/onto/OP21/Pagamento"/>
        <rdfs:range rdf:resource="https://w3id.org/italia/onto/OP21/EsitoPagamento"/>
        <rdfs:comment xml:lang="en">Relationship linking a Payment to a Payment Outcome. Each Payment Outcome relates to a single Payment.</rdfs:comment>
        <rdfs:comment xml:lang="it">Relazione che collega un Pagamento a un Esito Pagamento. Ciascun Esito Pagamento è relativo ad un unico Pagamento.</rdfs:comment>
        <rdfs:label xml:lang="it">ha esito pagamento</rdfs:label>
        <rdfs:label xml:lang="en">has payment outcome</rdfs:label>
    </owl:ObjectProperty>



    <!-- https://w3id.org/italia/onto/OP21/haFinalità -->

    <owl:ObjectProperty rdf:about="https://w3id.org/italia/onto/OP21/haFinalità">
        <rdf:type rdf:resource="http://www.w3.org/2002/07/owl#FunctionalProperty"/>
        <rdfs:domain rdf:resource="https://w3id.org/italia/onto/OP21/BollettinoDiPagamento"/>
        <rdfs:range rdf:resource="https://w3id.org/italia/onto/OP21/Finalità"/>
        <rdfs:comment xml:lang="en">Relationship linking each Payment Slip to a Purpose. Each Slipt has a single Purpose.</rdfs:comment>
        <rdfs:comment xml:lang="it">Relazione che collega ciascun Bolletino di Pagamento a una Finalità. Ciascun Bollettino ha un&apos;unica Finalità.</rdfs:comment>
        <rdfs:label xml:lang="it">ha finalità</rdfs:label>
        <rdfs:label xml:lang="en">has purpose</rdfs:label>
    </owl:ObjectProperty>



    <!-- https://w3id.org/italia/onto/OP21/haIntervalloDiRendicontazione -->

    <owl:ObjectProperty rdf:about="https://w3id.org/italia/onto/OP21/haIntervalloDiRendicontazione">
        <rdfs:domain rdf:resource="https://w3id.org/italia/onto/OP21/FlussoDiRendicontazione"/>
        <rdfs:range rdf:resource="https://w3id.org/italia/onto/TI/TimeInterval"/>
        <rdfs:comment xml:lang="en">Relationship linking a Reporting Flow to a Time Interval</rdfs:comment>
        <rdfs:comment xml:lang="it">Relazione che collega un Flusso di Rendicontazione a un Intervallo di Tempo.</rdfs:comment>
        <rdfs:label xml:lang="it">ha intervallo di rendicontazione</rdfs:label>
        <rdfs:label xml:lang="en">has reporting interval</rdfs:label>
    </owl:ObjectProperty>



    <!-- https://w3id.org/italia/onto/OP21/haIstitutoDiCredito -->

    <owl:ObjectProperty rdf:about="https://w3id.org/italia/onto/OP21/haIstitutoDiCredito">
        <rdf:type rdf:resource="http://www.w3.org/2002/07/owl#FunctionalProperty"/>
        <rdfs:domain rdf:resource="https://w3id.org/italia/onto/OP21/ContoCorrente"/>
        <rdfs:range rdf:resource="https://w3id.org/italia/onto/OP21/IstitutoDiCredito"/>
        <rdfs:comment xml:lang="en">Relationship linking a Bank Account to a Credit Institution. Each Bank Account belongs to a single Credit Institution.</rdfs:comment>
        <rdfs:comment xml:lang="it">Relazione che collega un Conto Corrente ad un Istituto di Credito. Ciascun Conto Corrente appartiene ad un unico Istituto di Credito.</rdfs:comment>
        <rdfs:label xml:lang="it">ha istituto di credito</rdfs:label>
        <rdfs:label xml:lang="en">has credit institution</rdfs:label>
    </owl:ObjectProperty>



    <!-- https://w3id.org/italia/onto/OP21/haLavoratoreDomestico -->

    <owl:ObjectProperty rdf:about="https://w3id.org/italia/onto/OP21/haLavoratoreDomestico">
        <rdf:type rdf:resource="http://www.w3.org/2002/07/owl#FunctionalProperty"/>
        <rdfs:domain rdf:resource="https://w3id.org/italia/onto/OP21/RapportoDiLavoroDomestico"/>
        <rdfs:range rdf:resource="https://w3id.org/italia/onto/OP21/LavoratoreDomestico"/>
        <rdfs:comment xml:lang="en">Relationship linking a Domestic Work Relationship to a Domestic Worker. Each Domestic Work Relationship involves a single Domestic Worker.</rdfs:comment>
        <rdfs:comment xml:lang="it">Relazione che collega un Rapporto di Lavoro Domestico a un Lavoratore Domestico. Ciascun Rapporto di Lavoro Domestico coinvolge un unico Lavoratore Domestico.</rdfs:comment>
        <rdfs:label xml:lang="it">ha lavoratore domestico</rdfs:label>
        <rdfs:label xml:lang="en">has domestic worker</rdfs:label>
    </owl:ObjectProperty>



    <!-- https://w3id.org/italia/onto/OP21/haModalitàDiPagamento -->

    <owl:ObjectProperty rdf:about="https://w3id.org/italia/onto/OP21/haModalitàDiPagamento">
        <rdf:type rdf:resource="http://www.w3.org/2002/07/owl#FunctionalProperty"/>
        <rdfs:domain rdf:resource="https://w3id.org/italia/onto/OP21/BollettinoDiPagamento"/>
        <rdfs:range rdf:resource="https://w3id.org/italia/onto/OP21/ModalitàDiPagamento"/>
        <rdfs:comment xml:lang="en">Relationship linking a Payment Slip to a Payment Method. Each Bulletin has a single Payment Method.</rdfs:comment>
        <rdfs:comment xml:lang="it">Relazione che collega un Bollettino di Pagamento ad una Modalità di Pagamento. Ciascun Bollettino ha un&apos;unica Modalità di Pagamento.</rdfs:comment>
        <rdfs:label xml:lang="it">ha modalità di pagamento</rdfs:label>
        <rdfs:label xml:lang="en">has payment mode</rdfs:label>
    </owl:ObjectProperty>



    <!-- https://w3id.org/italia/onto/OP21/haNotaDiMovimento -->

    <owl:ObjectProperty rdf:about="https://w3id.org/italia/onto/OP21/haNotaDiMovimento">
        <rdfs:subPropertyOf rdf:resource="https://w3id.org/italia/onto/l0/hasMember"/>
        <rdfs:domain rdf:resource="https://w3id.org/italia/onto/OP21/FlussoDiRendicontazione"/>
        <rdfs:range rdf:resource="https://w3id.org/italia/onto/OP21/RicevutaDiMovimento"/>
        <rdfs:comment xml:lang="en">Relationship linking a Reporting Flow to a Movement Receipt.</rdfs:comment>
        <rdfs:comment xml:lang="it">Relazione che collega un Flusso di Rendicontazione ad una Ricevuta Di Movimento.</rdfs:comment>
        <rdfs:label xml:lang="it">ha nota di movimento</rdfs:label>
        <rdfs:label xml:lang="en">has movement receipt</rdfs:label>
    </owl:ObjectProperty>



    <!-- https://w3id.org/italia/onto/OP21/haNotificaDiPagamento -->

    <owl:ObjectProperty rdf:about="https://w3id.org/italia/onto/OP21/haNotificaDiPagamento">
        <rdf:type rdf:resource="http://www.w3.org/2002/07/owl#FunctionalProperty"/>
        <rdfs:domain>
            <owl:Class>
                <owl:unionOf rdf:parseType="Collection">
                    <rdf:Description rdf:about="https://w3id.org/italia/onto/OP21/Pagamento"/>
                    <rdf:Description rdf:about="https://w3id.org/italia/onto/OP21/PrenotazioneDiPagamento"/>
                </owl:unionOf>
            </owl:Class>
        </rdfs:domain>
        <rdfs:range>
            <owl:Class>
                <owl:unionOf rdf:parseType="Collection">
                    <rdf:Description rdf:about="https://w3id.org/italia/onto/OP21/AvvisoDiPagamento"/>
                    <rdf:Description rdf:about="https://w3id.org/italia/onto/OP21/BollettinoMAV"/>
                </owl:unionOf>
            </owl:Class>
        </rdfs:range>
        <rdfs:comment xml:lang="en">Relationship linking a Payment or Payment Reservation to a MAV Bulletin or Payment Notice. Each Payment or Payment Reservation is linked to a single MAV Bulletin or Payment Notice.</rdfs:comment>
        <rdfs:comment xml:lang="it">Relazione che collega un Pagamento o una Prenotazione di Pagamento a un Bollettino MAV o ad un Avviso di Pagamento. Ciascun Pagamento o Prenotazione di Pagamento è collegato ad un unico Bollettino MAV o Avviso di Pagamento.</rdfs:comment>
        <rdfs:label xml:lang="it">ha notifica di pagamento</rdfs:label>
        <rdfs:label xml:lang="en">has payment notice</rdfs:label>
    </owl:ObjectProperty>



    <!-- https://w3id.org/italia/onto/OP21/haOnereContributivo -->

    <owl:ObjectProperty rdf:about="https://w3id.org/italia/onto/OP21/haOnereContributivo">
        <rdf:type rdf:resource="http://www.w3.org/2002/07/owl#FunctionalProperty"/>
        <rdf:type rdf:resource="http://www.w3.org/2002/07/owl#InverseFunctionalProperty"/>
        <rdfs:domain rdf:resource="https://w3id.org/italia/onto/OP21/StatoDiNotificatoImportoDiPratica"/>
        <rdfs:range rdf:resource="https://w3id.org/italia/onto/OP21/OnereContributivo"/>
        <rdfs:comment xml:lang="en">Relationship linking an Application State of Notified Amount to a Contribution Charge.</rdfs:comment>
        <rdfs:comment xml:lang="it">Relazione che collega uno Stato di Notificato Importo di Pratica ad un Onere Contributivo.</rdfs:comment>
        <rdfs:label xml:lang="it">ha onere contributivo</rdfs:label>
        <rdfs:label xml:lang="en">has a contribution charge</rdfs:label>
    </owl:ObjectProperty>



    <!-- https://w3id.org/italia/onto/OP21/haOrganizzazioneDiAssistenza -->

    <owl:ObjectProperty rdf:about="https://w3id.org/italia/onto/OP21/haOrganizzazioneDiAssistenza">
        <rdfs:domain rdf:resource="https://w3id.org/italia/onto/OP21/ContrattoDiLavoro"/>
        <rdfs:range rdf:resource="https://w3id.org/italia/onto/OP21/OrganizzazioneDiAssistenza"/>
        <rdfs:comment xml:lang="en">Relationship linking an Employment Agreement to a Support Organisation.</rdfs:comment>
        <rdfs:comment xml:lang="it">Relazione che collega un Contratto di Lavoro ad un&apos;Organizzazione di Assistenza.</rdfs:comment>
        <rdfs:label xml:lang="it">ha organizzazione di assistenza</rdfs:label>
        <rdfs:label xml:lang="en">has support organization</rdfs:label>
    </owl:ObjectProperty>



    <!-- https://w3id.org/italia/onto/OP21/haPagamento -->

    <owl:ObjectProperty rdf:about="https://w3id.org/italia/onto/OP21/haPagamento">
        <rdf:type rdf:resource="http://www.w3.org/2002/07/owl#InverseFunctionalProperty"/>
        <rdfs:domain rdf:resource="https://w3id.org/italia/onto/OP21/BollettinoDiPagamento"/>
        <rdfs:range rdf:resource="https://w3id.org/italia/onto/OP21/Pagamento"/>
        <rdfs:comment xml:lang="en">Object Property which connects a Payment Slip with the Payment.</rdfs:comment>
        <rdfs:comment xml:lang="it">Relazione che collega un Bollettino di pagamento con il Pagamento.</rdfs:comment>
        <rdfs:label xml:lang="it">ha pagamento</rdfs:label>
        <rdfs:label xml:lang="en">has payment</rdfs:label>
    </owl:ObjectProperty>



    <!-- https://w3id.org/italia/onto/OP21/haPagatoreOnere -->

    <owl:ObjectProperty rdf:about="https://w3id.org/italia/onto/OP21/haPagatoreOnere">
        <rdf:type rdf:resource="http://www.w3.org/2002/07/owl#FunctionalProperty"/>
        <rdfs:domain rdf:resource="https://w3id.org/italia/onto/OP21/PraticaAdeguamentoContributivo"/>
        <rdfs:range rdf:resource="https://w3id.org/italia/onto/OP21/Superstite"/>
        <rdfs:comment xml:lang="it">Relazione che collega una Pratica di Adeguamento Contributivo a un Superstite. Ciascuna Pratica ha un unico pagatore.</rdfs:comment>
        <rdfs:comment xml:lang="en">Report linking a Tax Adjustment Applcation to a Survivor. Each Application has a single payer.</rdfs:comment>
        <rdfs:label xml:lang="it">ha pagatore onere</rdfs:label>
        <rdfs:label xml:lang="en">has payer</rdfs:label>
    </owl:ObjectProperty>



    <!-- https://w3id.org/italia/onto/OP21/haPianoDiAmmortamento -->

    <owl:ObjectProperty rdf:about="https://w3id.org/italia/onto/OP21/haPianoDiAmmortamento">
        <rdf:type rdf:resource="http://www.w3.org/2002/07/owl#FunctionalProperty"/>
        <rdf:type rdf:resource="http://www.w3.org/2002/07/owl#InverseFunctionalProperty"/>
        <rdfs:domain rdf:resource="https://w3id.org/italia/onto/OP21/StatoDiNotificatoImportoDiPratica"/>
        <rdfs:range rdf:resource="https://w3id.org/italia/onto/OP21/PianoDiAmmortamento"/>
        <rdfs:comment xml:lang="en">Relationship linking an Application Status of Notified Amount to an Amortization Plan.</rdfs:comment>
        <rdfs:comment xml:lang="it">Relazione che collega uno Stato di Notificato Importo di Pratica ad un Piano di Ammortamento.</rdfs:comment>
        <rdfs:label xml:lang="it">ha piano di ammortamento</rdfs:label>
        <rdfs:label xml:lang="en">has amortization plan</rdfs:label>
    </owl:ObjectProperty>



    <!-- https://w3id.org/italia/onto/OP21/haPraticaPerMandato -->

    <owl:ObjectProperty rdf:about="https://w3id.org/italia/onto/OP21/haPraticaPerMandato">
        <rdf:type rdf:resource="http://www.w3.org/2002/07/owl#FunctionalProperty"/>
        <rdfs:domain rdf:resource="https://w3id.org/italia/onto/OP21/MandatoSDD"/>
        <rdfs:range rdf:resource="https://w3id.org/italia/onto/OP21/PraticaDiAdeguamentoRateizzata"/>
        <rdfs:comment xml:lang="it">Relazione che collega un Mandato SDD ad una Pratica di Adeguamento Rateizzato. Ciascun Mandato ha un&apos;unica Pratica.</rdfs:comment>
        <rdfs:comment xml:lang="en">Report linking an SDD Mandate to an Contribution Adjustment Application by Installments. Each Mandate has a single Application.</rdfs:comment>
        <rdfs:label xml:lang="it">ha pratica per mandato</rdfs:label>
        <rdfs:label xml:lang="en">has application for mandate</rdfs:label>
    </owl:ObjectProperty>



    <!-- https://w3id.org/italia/onto/OP21/haRata -->

    <owl:ObjectProperty rdf:about="https://w3id.org/italia/onto/OP21/haRata">
        <rdfs:subPropertyOf rdf:resource="https://w3id.org/italia/onto/l0/hasMember"/>
        <rdf:type rdf:resource="http://www.w3.org/2002/07/owl#FunctionalProperty"/>
        <rdf:type rdf:resource="http://www.w3.org/2002/07/owl#InverseFunctionalProperty"/>
        <rdfs:domain rdf:resource="https://w3id.org/italia/onto/OP21/PianoDiAmmortamento"/>
        <rdfs:range rdf:resource="https://w3id.org/italia/onto/OP21/RataDiOnereContributivo"/>
        <rdfs:comment xml:lang="it">Relazione che collega un Piano di Ammortamento ad una Rata di Onere Contributivo.</rdfs:comment>
        <rdfs:comment xml:lang="en">Report linking an Amortization Plan to a Contribution Charge Installment.</rdfs:comment>
        <rdfs:label xml:lang="it">ha rata</rdfs:label>
        <rdfs:label xml:lang="en">has installment</rdfs:label>
    </owl:ObjectProperty>



    <!-- https://w3id.org/italia/onto/OP21/haRataSuccessiva -->

    <owl:ObjectProperty rdf:about="https://w3id.org/italia/onto/OP21/haRataSuccessiva">
        <rdfs:subPropertyOf rdf:resource="https://w3id.org/italia/onto/l0/follows"/>
        <rdfs:domain rdf:resource="https://w3id.org/italia/onto/OP21/RataDiOnereContributivo"/>
        <rdfs:range rdf:resource="https://w3id.org/italia/onto/OP21/RataDiOnereContributivo"/>
        <rdfs:comment xml:lang="en">Relationship linking a Contribution Fee Installment to the next Installment.</rdfs:comment>
        <rdfs:comment xml:lang="it">Relazione che collega una Rata di Onere Contributivo alla Rata successiva.</rdfs:comment>
        <rdfs:label xml:lang="it">ha rata successiva</rdfs:label>
        <rdfs:label xml:lang="en">has next installment</rdfs:label>
    </owl:ObjectProperty>



    <!-- https://w3id.org/italia/onto/OP21/haSedeINPS -->

    <owl:ObjectProperty rdf:about="https://w3id.org/italia/onto/OP21/haSedeINPS">
        <rdf:type rdf:resource="http://www.w3.org/2002/07/owl#FunctionalProperty"/>
        <rdfs:domain>
            <owl:Class>
                <owl:unionOf rdf:parseType="Collection">
                    <rdf:Description rdf:about="https://w3id.org/italia/onto/COV/Organization"/>
                    <rdf:Description rdf:about="https://w3id.org/italia/onto/CPV/Alive"/>
                </owl:unionOf>
            </owl:Class>
        </rdfs:domain>
        <rdfs:range rdf:resource="https://w3id.org/italia/onto/OP21/SedeINPS"/>
        <rdfs:comment xml:lang="en">Relationship linking a Living Person or an Organization to an INPS Office. Each Living Person or Organization has a single INPS office.</rdfs:comment>
        <rdfs:comment xml:lang="it">Relazione che collega una Persona in Vita o un&apos;Organizzazione ad una Sede INPS. Ciascuna Persona in Vita o Organizzazione ha un&apos;unica Sede INPS.</rdfs:comment>
        <rdfs:label xml:lang="it">ha sede INPS</rdfs:label>
        <rdfs:label xml:lang="en">has INPS office</rdfs:label>
    </owl:ObjectProperty>



    <!-- https://w3id.org/italia/onto/OP21/haServizioDiPagamento -->

    <owl:ObjectProperty rdf:about="https://w3id.org/italia/onto/OP21/haServizioDiPagamento">
        <rdf:type rdf:resource="http://www.w3.org/2002/07/owl#InverseFunctionalProperty"/>
        <rdfs:domain rdf:resource="https://w3id.org/italia/onto/OP21/PrestatoreDiServiziDiPagamento"/>
        <rdfs:range rdf:resource="https://w3id.org/italia/onto/OP21/ServizioDiPagamento"/>
        <rdfs:comment xml:lang="en">Relationship linking a Payment Service Provider to a Payment Service. Each Payment Service is provided by a single Provider.</rdfs:comment>
        <rdfs:comment xml:lang="it">Relazione che collega un Prestatore di Servizi di Pagamento ad un Servizio di Pagamento. Ciascun Servizio di Pagamento è erogato da un unico Prestatore.</rdfs:comment>
        <rdfs:label xml:lang="it">ha servizio di pagamento</rdfs:label>
        <rdfs:label xml:lang="en">has payment service</rdfs:label>
    </owl:ObjectProperty>



    <!-- https://w3id.org/italia/onto/OP21/haSettimanaDelTrimestre -->

    <owl:ObjectProperty rdf:about="https://w3id.org/italia/onto/OP21/haSettimanaDelTrimestre">
        <rdfs:domain rdf:resource="https://w3id.org/italia/onto/OP21/ContributoTrimestraleModificato"/>
        <rdfs:range rdf:resource="https://w3id.org/italia/onto/OP21/SettimanaDelMese"/>
        <rdfs:comment xml:lang="en">Relationship which connects a Modified Quarterly Contribution with the Week of the quarter in which it takes place.</rdfs:comment>
        <rdfs:comment xml:lang="it">Relazione che collega un Contributo Trimestrale Modificato alla Settimana del trimestre.</rdfs:comment>
        <rdfs:label xml:lang="it">ha settimana del trimestre</rdfs:label>
        <rdfs:label xml:lang="en">has week of quarter</rdfs:label>
    </owl:ObjectProperty>



    <!-- https://w3id.org/italia/onto/OP21/haSistemaDiPagamentoElettronico -->

    <owl:ObjectProperty rdf:about="https://w3id.org/italia/onto/OP21/haSistemaDiPagamentoElettronico">
        <rdf:type rdf:resource="http://www.w3.org/2002/07/owl#FunctionalProperty"/>
        <rdfs:domain rdf:resource="https://w3id.org/italia/onto/OP21/SessionePagamentoElettronico"/>
        <rdfs:range rdf:resource="https://w3id.org/italia/onto/OP21/SistemaDiPagamentoElettronico"/>
        <rdfs:comment xml:lang="it">Lega in modo univoco una Sessione (di) Pagamento Elettronico con il Sistema Di Pagamento Elettrronico su cui è stata avviata tale sessione</rdfs:comment>
        <rdfs:comment xml:lang="en">Uniquely links an Electronic Payment Session with the Electronic Payment System on which this session was started</rdfs:comment>
        <rdfs:label xml:lang="it">ha sistema di pagamento elettronico</rdfs:label>
        <rdfs:label xml:lang="en">has electronic payment system</rdfs:label>
    </owl:ObjectProperty>



    <!-- https://w3id.org/italia/onto/OP21/haTitolarePratica -->

    <owl:ObjectProperty rdf:about="https://w3id.org/italia/onto/OP21/haTitolarePratica">
        <rdf:type rdf:resource="http://www.w3.org/2002/07/owl#FunctionalProperty"/>
        <rdfs:domain rdf:resource="https://w3id.org/italia/onto/OP21/PraticaAdeguamentoContributivo"/>
        <rdfs:range rdf:resource="https://w3id.org/italia/onto/OP21/TitolarePratica"/>
        <rdfs:comment xml:lang="en">Relationship linking a Tax Adjustment Application to an Application Holder. Each Application has a single Holder.</rdfs:comment>
        <rdfs:comment xml:lang="it">Relazione che collega una Pratica di Adeguamento Contributivo ad un Titolare Pratica. Ciascuna Pratica ha un unico Titolare.</rdfs:comment>
        <rdfs:label xml:lang="it">ha titolare pratica</rdfs:label>
        <rdfs:label xml:lang="en">has application holder</rdfs:label>
    </owl:ObjectProperty>



    <!-- https://w3id.org/italia/onto/OP21/haTrimestreDiAnno -->

    <owl:ObjectProperty rdf:about="https://w3id.org/italia/onto/OP21/haTrimestreDiAnno">
        <rdf:type rdf:resource="http://www.w3.org/2002/07/owl#FunctionalProperty"/>
        <rdfs:domain rdf:resource="https://w3id.org/italia/onto/OP21/ContributoTrimestraleOrdinario"/>
        <rdfs:range rdf:resource="https://w3id.org/italia/onto/OP21/TrimestreDiAnno"/>
        <rdfs:comment xml:lang="en">Relationship that connects an Ordinary Quarterly Contribution with the Quarter in which it takes place. Each Contribution can take place in only one quarter (1st, 2nd, 3rd, or 4th).</rdfs:comment>
        <rdfs:comment xml:lang="it">Relazione che collega un Contributo Trimestrale Ordinario con Trimestre dell&apos;anno in cui avviene. Ciascun Contributo può avvenire in un solo trimestre (I, II, III, o IV).</rdfs:comment>
        <rdfs:label xml:lang="it">ha trimestre di anno</rdfs:label>
        <rdfs:label xml:lang="en">has quarterly</rdfs:label>
    </owl:ObjectProperty>



    <!-- https://w3id.org/italia/onto/OP21/haVersamentoOrganizzazione -->

    <owl:ObjectProperty rdf:about="https://w3id.org/italia/onto/OP21/haVersamentoOrganizzazione">
        <rdf:type rdf:resource="http://www.w3.org/2002/07/owl#FunctionalProperty"/>
        <rdfs:domain rdf:resource="https://w3id.org/italia/onto/OP21/ContributoTrimestraleModificato"/>
        <rdfs:range rdf:resource="https://w3id.org/italia/onto/OP21/OrganizzazioneDiAssistenza"/>
        <rdfs:comment xml:lang="en">Relationship linking an Amended Quarterly Contribution to a Support Organization. Each Contribution can be paid by a single Organization.</rdfs:comment>
        <rdfs:comment xml:lang="it">Relazione che collega un Contributo Trimestrale Modificato ad un&apos;Organizzazione di Assistenza. Ciascun Contibuto può essere versato da un&apos;unica Organizzazione.</rdfs:comment>
        <rdfs:label xml:lang="it">ha versamento organizzazione</rdfs:label>
        <rdfs:label xml:lang="en">has payment organization</rdfs:label>
    </owl:ObjectProperty>



    <!-- https://w3id.org/italia/onto/OP21/inviaFlussoDiRendicontazione -->

    <owl:ObjectProperty rdf:about="https://w3id.org/italia/onto/OP21/inviaFlussoDiRendicontazione">
        <rdf:type rdf:resource="http://www.w3.org/2002/07/owl#InverseFunctionalProperty"/>
        <rdfs:domain rdf:resource="https://w3id.org/italia/onto/OP21/PrestatoreDiServiziDiPagamento"/>
        <rdfs:range rdf:resource="https://w3id.org/italia/onto/OP21/FlussoDiRendicontazione"/>
        <rdfs:comment xml:lang="en">Relationship linking a Payment Service Provider to a Reporting Flow. Each Reporting Flow is sent by a single Provider.</rdfs:comment>
        <rdfs:comment xml:lang="it">Relazione che collega un Prestatore di Servizi di Pagamento a un Flusso di Rendicontazione. Ciascun Flusso di Rendicontazione è inviato da un unico Prestatore.</rdfs:comment>
        <rdfs:label xml:lang="it">invia flusso di rendicontazione</rdfs:label>
        <rdfs:label xml:lang="en">send reporting flow</rdfs:label>
    </owl:ObjectProperty>



    <!-- https://w3id.org/italia/onto/OP21/inviaRicevutaDiMovimento -->

    <owl:ObjectProperty rdf:about="https://w3id.org/italia/onto/OP21/inviaRicevutaDiMovimento">
        <rdf:type rdf:resource="http://www.w3.org/2002/07/owl#FunctionalProperty"/>
        <rdf:type rdf:resource="http://www.w3.org/2002/07/owl#InverseFunctionalProperty"/>
        <rdfs:domain rdf:resource="https://w3id.org/italia/onto/OP21/MovimentoDiDenaro"/>
        <rdfs:range rdf:resource="https://w3id.org/italia/onto/OP21/RicevutaDiMovimento"/>
        <rdfs:comment xml:lang="en">Relationship linking a Money Movement to a Movement Receipt.</rdfs:comment>
        <rdfs:comment xml:lang="it">Relazione che collega un Movimento Di Denaro ad una Ricevuta di Movimento.</rdfs:comment>
        <rdfs:label xml:lang="it">invia ricevuta di movimento</rdfs:label>
        <rdfs:label xml:lang="en">sends movement receipt</rdfs:label>
    </owl:ObjectProperty>



    <!-- https://w3id.org/italia/onto/OP21/istruiscePratica -->

    <owl:ObjectProperty rdf:about="https://w3id.org/italia/onto/OP21/istruiscePratica">
        <rdfs:domain rdf:resource="https://w3id.org/italia/onto/OP21/SedeINPS"/>
        <rdfs:range rdf:resource="https://w3id.org/italia/onto/OP21/PraticaAdeguamentoContributivo"/>
        <rdfs:comment xml:lang="en">Relationship linking an INPS Office with one or more Tax Adjustment Applications which the office instructs.</rdfs:comment>
        <rdfs:comment xml:lang="it">Relazione che collega una Sede INPS con la Pratica di Adeguamento Contributivo istruita dalla sede.</rdfs:comment>
        <rdfs:label xml:lang="en">instructs application</rdfs:label>
        <rdfs:label xml:lang="it">istruisce pratica</rdfs:label>
    </owl:ObjectProperty>



    <!-- https://w3id.org/italia/onto/OP21/movimentoAgisceSu -->

    <owl:ObjectProperty rdf:about="https://w3id.org/italia/onto/OP21/movimentoAgisceSu">
        <rdf:type rdf:resource="http://www.w3.org/2002/07/owl#FunctionalProperty"/>
        <rdfs:domain rdf:resource="https://w3id.org/italia/onto/OP21/MovimentoDiDenaro"/>
        <rdfs:range rdf:resource="https://w3id.org/italia/onto/OP21/ContoCorrente"/>
        <rdfs:comment xml:lang="en">Functional link between a Money Movement and the Current Account on which this movement takes place.</rdfs:comment>
        <rdfs:comment xml:lang="it">Legame funzionale tra un Movimento Di Denaro e il Conto Corrente su cui avviene tale movimento.</rdfs:comment>
        <rdfs:label xml:lang="en">movement acts on</rdfs:label>
        <rdfs:label xml:lang="it">movimento agisce su</rdfs:label>
    </owl:ObjectProperty>



    <!-- https://w3id.org/italia/onto/OP21/prenotaPagamento -->

    <owl:ObjectProperty rdf:about="https://w3id.org/italia/onto/OP21/prenotaPagamento">
        <rdf:type rdf:resource="http://www.w3.org/2002/07/owl#InverseFunctionalProperty"/>
        <rdfs:domain>
            <owl:Class>
                <owl:unionOf rdf:parseType="Collection">
                    <rdf:Description rdf:about="https://w3id.org/italia/onto/OP21/MandatoSDDAttivo"/>
                    <rdf:Description rdf:about="https://w3id.org/italia/onto/OP21/SessionePagamentoElettronico"/>
                </owl:unionOf>
            </owl:Class>
        </rdfs:domain>
        <rdfs:range rdf:resource="https://w3id.org/italia/onto/OP21/PrenotazioneDiPagamento"/>
        <rdfs:comment xml:lang="en">Relationship linking a Payment Service Host or an Active SDD Mandate with a Payment Reservation. Each Active SDD Mandate reserves at least one payment.</rdfs:comment>
        <rdfs:comment xml:lang="it">Relazione che collega un Gestore di Servizi di Pagamento o un Mandato SDD Attivo con una Prenotazione di Pagamento. Ciascun Mandato SDD Attivo prenota un almeno pagamento.</rdfs:comment>
        <rdfs:label xml:lang="it">prenota pagamento</rdfs:label>
        <rdfs:label xml:lang="en">reserves payment</rdfs:label>
    </owl:ObjectProperty>



    <!-- https://w3id.org/italia/onto/OP21/presentaDomandaAdeguamentoContributivo -->

    <owl:ObjectProperty rdf:about="https://w3id.org/italia/onto/OP21/presentaDomandaAdeguamentoContributivo">
        <rdf:type rdf:resource="http://www.w3.org/2002/07/owl#InverseFunctionalProperty"/>
        <rdfs:domain rdf:resource="https://w3id.org/italia/onto/OP21/RichiedenteAdeguamentoContributivo"/>
        <rdfs:range rdf:resource="https://w3id.org/italia/onto/OP21/DomandaAdeguamentoContributivo"/>
        <rdfs:comment xml:lang="en">Relationship linking each Tax Adjustment Applicant to the Tax Adjustment Application he or she has submitted.</rdfs:comment>
        <rdfs:comment xml:lang="it">Relazione che collega ciascun Richiedente Adeguamento Contributivo con la Domanda di Adeguamento Contributivo presentata.</rdfs:comment>
        <rdfs:label xml:lang="it">presenta domanda adeguamento contributivo</rdfs:label>
        <rdfs:label xml:lang="en">submits tax adjustment application</rdfs:label>
    </owl:ObjectProperty>



    <!-- https://w3id.org/italia/onto/OP21/revocaMandato -->

    <owl:ObjectProperty rdf:about="https://w3id.org/italia/onto/OP21/revocaMandato">
        <rdf:type rdf:resource="http://www.w3.org/2002/07/owl#FunctionalProperty"/>
        <rdfs:domain rdf:resource="https://w3id.org/italia/onto/OP21/AttoDiRevocaMandato"/>
        <rdfs:range rdf:resource="https://w3id.org/italia/onto/OP21/MandatoSDDRevocato"/>
        <rdfs:comment xml:lang="en">Relationship linking each SDD Mandate Withdrawl Deed with the Revoked SDD Mandate. Each Withdrawl Deed revokes a single SDD Mandate.</rdfs:comment>
        <rdfs:comment xml:lang="it">Relazione che collega ciascun Atto di Revoca Mandato con il Mandato SDD Revocato. Ciascun Atto revoca un unico Mandato SDD.</rdfs:comment>
        <rdfs:label xml:lang="it">revoca mandato</rdfs:label>
        <rdfs:label xml:lang="en">revokes mandate</rdfs:label>
    </owl:ObjectProperty>



    <!-- https://w3id.org/italia/onto/OP21/riceveDomanda -->

    <owl:ObjectProperty rdf:about="https://w3id.org/italia/onto/OP21/riceveDomanda">
        <rdf:type rdf:resource="http://www.w3.org/2002/07/owl#InverseFunctionalProperty"/>
        <rdfs:domain rdf:resource="https://w3id.org/italia/onto/OP21/SedeINPS"/>
        <rdfs:range rdf:resource="https://w3id.org/italia/onto/OP21/DomandaAdeguamentoContributivo"/>
        <rdfs:comment xml:lang="en">Relationship linking an INPS Office with one or more Tax Adjustment Applications. Each Tax Adjustment Application is received by exactly one INPS Office.</rdfs:comment>
        <rdfs:comment xml:lang="it">Relazione che collega una Sede INPS con una o più Domande di Adeguamento Contributivo. Ciascuna Domanda di Adeguamento Contributivo è ricevuta da esattamente una Sede INPS.</rdfs:comment>
        <rdfs:label xml:lang="en">receives request</rdfs:label>
        <rdfs:label xml:lang="it">riceve domanda</rdfs:label>
    </owl:ObjectProperty>



    <!-- https://w3id.org/italia/onto/OP21/riceveFlussoDiRendicontazione -->

    <owl:ObjectProperty rdf:about="https://w3id.org/italia/onto/OP21/riceveFlussoDiRendicontazione">
        <rdf:type rdf:resource="http://www.w3.org/2002/07/owl#InverseFunctionalProperty"/>
        <rdfs:domain rdf:resource="https://w3id.org/italia/onto/OP21/EnteCreditore"/>
        <rdfs:range rdf:resource="https://w3id.org/italia/onto/OP21/FlussoDiRendicontazione"/>
        <rdfs:comment xml:lang="en">Relationship linking a Creditor Institution with one or more Reporting Flows. Each Reporting Flow is received by exactly one Creditor Institution.</rdfs:comment>
        <rdfs:comment xml:lang="it">Relazione che collega un Ente Creditore con uno o più Flussi di Rendicontazione. Un Flusso di Rendicontazione è ricevuto da esattamente un Ente Creditore.</rdfs:comment>
        <rdfs:label xml:lang="en">receives reporting flow</rdfs:label>
        <rdfs:label xml:lang="it">riceve flusso di rendicontazione</rdfs:label>
    </owl:ObjectProperty>



    <!-- https://w3id.org/italia/onto/OP21/riceveRicevutaDiAccredito -->

    <owl:ObjectProperty rdf:about="https://w3id.org/italia/onto/OP21/riceveRicevutaDiAccredito">
        <rdf:type rdf:resource="http://www.w3.org/2002/07/owl#InverseFunctionalProperty"/>
        <rdfs:domain rdf:resource="https://w3id.org/italia/onto/OP21/EnteCreditore"/>
        <rdfs:range rdf:resource="https://w3id.org/italia/onto/OP21/RicevutaDiMovimento"/>
        <rdfs:comment xml:lang="en">Relationship linking a Creditor Institution with one or more Credit Receipts. Each Credit Receipt is received by exactly one Creditor Institution.</rdfs:comment>
        <rdfs:comment xml:lang="it">Relazione che collega un Ente Creditore con una o più Ricevute di Accredito. Una Ricevuta di Accredito è ricevuta esattamente da un Ente Creditore.</rdfs:comment>
        <rdfs:label xml:lang="en">receives credit receipt</rdfs:label>
        <rdfs:label xml:lang="it">riceve ricevuta di accredito</rdfs:label>
    </owl:ObjectProperty>



    <!-- https://w3id.org/italia/onto/OP21/riferiscePagamento -->

    <owl:ObjectProperty rdf:about="https://w3id.org/italia/onto/OP21/riferiscePagamento">
        <rdf:type rdf:resource="http://www.w3.org/2002/07/owl#FunctionalProperty"/>
        <rdfs:comment xml:lang="en">Relationship inverse of has payment outcome, which links a Payment Outcome with a Payment to which it refers. A Payment Outcome refers to one and only one Payment.</rdfs:comment>
        <rdfs:comment xml:lang="it">Relazione inversa della relazione ha esito pagamento, che lega un Esito Pagamento al Pagamento a cui si riferisce. Un Esito Pagamento si riferisce sempre e solo ad un Pagamento.</rdfs:comment>
        <rdfs:label xml:lang="en">refers payment</rdfs:label>
        <rdfs:label xml:lang="it">riferisce pagamento</rdfs:label>
    </owl:ObjectProperty>



    <!-- https://w3id.org/italia/onto/OP21/stabilisceFlussoDiAddebito -->

    <owl:ObjectProperty rdf:about="https://w3id.org/italia/onto/OP21/stabilisceFlussoDiAddebito">
        <rdfs:domain rdf:resource="https://w3id.org/italia/onto/OP21/AttoDiAttivazioneMandato"/>
        <rdfs:range rdf:resource="https://w3id.org/italia/onto/OP21/ContoCorrente"/>
        <rdfs:comment xml:lang="en">Relationship linking an SDD Mandate Activation Deed with the two Bank Accounts that are involved in a payment, the Mandate Creditor and the Mandate Debtor.</rdfs:comment>
        <rdfs:comment xml:lang="it">Relazione che collega un Atto di Attivazione Mandato con i due Conti Correnti interessati dal pagamento, quello del Creditore Mandato e quello del Debitore Mandato.</rdfs:comment>
        <rdfs:label xml:lang="en">establishes charge flow</rdfs:label>
        <rdfs:label xml:lang="it">stabilisce flusso di addebito</rdfs:label>
    </owl:ObjectProperty>



    <!-- https://w3id.org/italia/onto/OP21/utilizzaServizioDiPagamento -->

    <owl:ObjectProperty rdf:about="https://w3id.org/italia/onto/OP21/utilizzaServizioDiPagamento">
        <rdf:type rdf:resource="http://www.w3.org/2002/07/owl#FunctionalProperty"/>
        <rdfs:domain rdf:resource="https://w3id.org/italia/onto/OP21/OrdineDiPagamento"/>
        <rdfs:range rdf:resource="https://w3id.org/italia/onto/OP21/ServizioDiPagamento"/>
        <rdfs:comment xml:lang="en">Relationship linking a Payment Order  to at most one payment service by the PSP, which the Debtor uses to make the payment he is due.</rdfs:comment>
        <rdfs:comment xml:lang="it">Relazione che collega un Ordine di Pagamento con al più uno dei servizi di pagamento offerti dal PSP, attraverso il quale il debitore esegue il pagamento dovuto.</rdfs:comment>
        <rdfs:label xml:lang="en">uses payment service</rdfs:label>
        <rdfs:label xml:lang="it">utilizza servizio di pagamento</rdfs:label>
    </owl:ObjectProperty>



    <!-- https://w3id.org/italia/onto/OP21/èMeseDelTrimestre -->

    <owl:ObjectProperty rdf:about="https://w3id.org/italia/onto/OP21/èMeseDelTrimestre">
        <rdf:type rdf:resource="http://www.w3.org/2002/07/owl#FunctionalProperty"/>
        <rdfs:domain rdf:resource="https://w3id.org/italia/onto/OP21/MeseDiTrimestre"/>
        <rdfs:range rdf:resource="https://w3id.org/italia/onto/OP21/TrimestreDiAnno"/>
        <rdfs:comment xml:lang="en">Relationship linking a Month of a Quarter to the Quarter of a Year to which it belongs. Each Month belongs to a single Quarter.</rdfs:comment>
        <rdfs:comment xml:lang="it">Relazione che collega un Mese di Trimestre al Trimestre di Anno a cui appartiene. Ciascun Mese appartiene ad un unico Trimestre.</rdfs:comment>
        <rdfs:label xml:lang="en">is month of trimester</rdfs:label>
        <rdfs:label xml:lang="it">è mese del trimestre</rdfs:label>
    </owl:ObjectProperty>



    <!-- https://w3id.org/italia/onto/OP21/èOriginatoDa -->

    <owl:ObjectProperty rdf:about="https://w3id.org/italia/onto/OP21/èOriginatoDa">
        <rdf:type rdf:resource="http://www.w3.org/2002/07/owl#FunctionalProperty"/>
        <rdf:type rdf:resource="http://www.w3.org/2002/07/owl#InverseFunctionalProperty"/>
        <rdfs:domain rdf:resource="https://w3id.org/italia/onto/OP21/RapportoDiLavoroDomestico"/>
        <rdfs:range rdf:resource="https://w3id.org/italia/onto/OP21/ContrattoDiLavoro"/>
        <rdfs:comment xml:lang="en">Relationship linking a Domestic Work Relationship to the Employment Contract from which it is derived.</rdfs:comment>
        <rdfs:comment xml:lang="it">Relazione che collega un Rapporto di Lavoro Domestico al Contratto di Lavoro da cui è generato.</rdfs:comment>
        <rdfs:label xml:lang="en">is derived by</rdfs:label>
        <rdfs:label xml:lang="it">è originato da</rdfs:label>
    </owl:ObjectProperty>



    <!-- https://w3id.org/italia/onto/OP21/èSettimanaDelMese -->

    <owl:ObjectProperty rdf:about="https://w3id.org/italia/onto/OP21/èSettimanaDelMese">
        <rdf:type rdf:resource="http://www.w3.org/2002/07/owl#FunctionalProperty"/>
        <rdfs:domain rdf:resource="https://w3id.org/italia/onto/OP21/SettimanaDelMese"/>
        <rdfs:range rdf:resource="https://w3id.org/italia/onto/OP21/MeseDiTrimestre"/>
        <rdfs:comment xml:lang="en">Relationship linking a Week of the Month to the Month of Quarter to which it belongs. Each Week belongs to a single Month.</rdfs:comment>
        <rdfs:comment xml:lang="it">Relazione che collega una Settimana del Mese al Mese di Trimestre a cui appartiene. Ciascuna Settimana appartiene ad un unico Mese.</rdfs:comment>
        <rdfs:label xml:lang="en">is week of the month</rdfs:label>
        <rdfs:label xml:lang="it">è settimana del mese</rdfs:label>
    </owl:ObjectProperty>



    <!-- https://w3id.org/italia/onto/OP21/èSuperstite -->

    <owl:ObjectProperty rdf:about="https://w3id.org/italia/onto/OP21/èSuperstite">
        <rdfs:subPropertyOf rdf:resource="https://w3id.org/italia/onto/CPV/hasParentalRelationshipWith"/>
        <rdfs:domain rdf:resource="https://w3id.org/italia/onto/OP21/Superstite"/>
        <rdfs:range>
            <owl:Class>
                <owl:intersectionOf rdf:parseType="Collection">
                    <rdf:Description rdf:about="https://w3id.org/italia/onto/CPV/Dead"/>
                    <rdf:Description rdf:about="https://w3id.org/italia/onto/OP21/TitolarePratica"/>
                </owl:intersectionOf>
            </owl:Class>
        </rdfs:range>
        <rdfs:comment xml:lang="en">Relationship linking a Survivor to a Dead Application Holder.</rdfs:comment>
        <rdfs:comment xml:lang="it">Relazione che collega un Supersite con una Persona Non in Vita e Titolare Pratica.</rdfs:comment>
        <rdfs:label xml:lang="en">is survivor</rdfs:label>
        <rdfs:label xml:lang="it">è superstite</rdfs:label>
    </owl:ObjectProperty>



    <!-- https://w3id.org/italia/onto/RO/holdsRoleInTime -->

    <owl:ObjectProperty rdf:about="https://w3id.org/italia/onto/RO/holdsRoleInTime">
        <rdfs:range rdf:resource="https://w3id.org/italia/onto/RO/TimeIndexedRole"/>
    </owl:ObjectProperty>



    <!-- https://w3id.org/italia/onto/TI/atTime -->

    <owl:ObjectProperty rdf:about="https://w3id.org/italia/onto/TI/atTime"/>



    <!-- https://w3id.org/italia/onto/TI/hasTemporalEntity -->

    <owl:ObjectProperty rdf:about="https://w3id.org/italia/onto/TI/hasTemporalEntity"/>



    <!-- https://w3id.org/italia/onto/l0/follows -->

    <owl:ObjectProperty rdf:about="https://w3id.org/italia/onto/l0/follows"/>



    <!-- https://w3id.org/italia/onto/l0/hasMember -->

    <owl:ObjectProperty rdf:about="https://w3id.org/italia/onto/l0/hasMember"/>



    <!--
    ///////////////////////////////////////////////////////////////////////////////////////
    //
    // Data properties
    //
    ///////////////////////////////////////////////////////////////////////////////////////
     -->




    <!-- https://w3id.org/italia/onto/COV/AOOIdentifier -->

    <owl:DatatypeProperty rdf:about="https://w3id.org/italia/onto/COV/AOOIdentifier">
        <rdf:type rdf:resource="http://www.w3.org/2002/07/owl#FunctionalProperty"/>
    </owl:DatatypeProperty>



    <!-- https://w3id.org/italia/onto/COV/IPACode -->

    <owl:DatatypeProperty rdf:about="https://w3id.org/italia/onto/COV/IPACode">
        <rdf:type rdf:resource="http://www.w3.org/2002/07/owl#FunctionalProperty"/>
        <rdfs:domain rdf:resource="https://w3id.org/italia/onto/COV/PublicOrganization"/>
    </owl:DatatypeProperty>



    <!-- https://w3id.org/italia/onto/COV/LegalName -->

    <owl:DatatypeProperty rdf:about="https://w3id.org/italia/onto/COV/LegalName">
        <rdfs:domain rdf:resource="https://w3id.org/italia/onto/COV/Organization"/>
    </owl:DatatypeProperty>



    <!-- https://w3id.org/italia/onto/COV/taxCode -->

    <owl:DatatypeProperty rdf:about="https://w3id.org/italia/onto/COV/taxCode">
        <rdf:type rdf:resource="http://www.w3.org/2002/07/owl#FunctionalProperty"/>
        <rdfs:domain rdf:resource="https://w3id.org/italia/onto/COV/Organization"/>
    </owl:DatatypeProperty>



    <!-- https://w3id.org/italia/onto/CPV/familyName -->

    <owl:DatatypeProperty rdf:about="https://w3id.org/italia/onto/CPV/familyName">
        <rdfs:domain rdf:resource="https://w3id.org/italia/onto/CPV/Person"/>
    </owl:DatatypeProperty>



    <!-- https://w3id.org/italia/onto/CPV/givenName -->

    <owl:DatatypeProperty rdf:about="https://w3id.org/italia/onto/CPV/givenName">
        <rdfs:domain rdf:resource="https://w3id.org/italia/onto/CPV/Person"/>
    </owl:DatatypeProperty>



    <!-- https://w3id.org/italia/onto/CPV/taxCode -->

    <owl:DatatypeProperty rdf:about="https://w3id.org/italia/onto/CPV/taxCode">
        <rdf:type rdf:resource="http://www.w3.org/2002/07/owl#FunctionalProperty"/>
        <rdfs:domain rdf:resource="https://w3id.org/italia/onto/CPV/Person"/>
    </owl:DatatypeProperty>



    <!-- https://w3id.org/italia/onto/OP21/IBAN -->

    <owl:DatatypeProperty rdf:about="https://w3id.org/italia/onto/OP21/IBAN">
        <rdf:type rdf:resource="http://www.w3.org/2002/07/owl#FunctionalProperty"/>
        <rdfs:domain rdf:resource="https://w3id.org/italia/onto/OP21/ContoCorrente"/>
        <rdfs:range rdf:resource="http://www.w3.org/2001/XMLSchema#string"/>
        <rdfs:comment xml:lang="it">Codice delle coordinate bancarie, conforme allo standard internazionale, che individua in modo univoco un conto bancario</rdfs:comment>
        <rdfs:comment xml:lang="en">International Bank Account Number</rdfs:comment>
        <rdfs:label xml:lang="en">IBAN</rdfs:label>
        <rdfs:label xml:lang="it">IBAN</rdfs:label>
    </owl:DatatypeProperty>



    <!-- https://w3id.org/italia/onto/OP21/IUV -->

    <owl:DatatypeProperty rdf:about="https://w3id.org/italia/onto/OP21/IUV">
        <rdf:type rdf:resource="http://www.w3.org/2002/07/owl#FunctionalProperty"/>
        <rdfs:domain rdf:resource="https://w3id.org/italia/onto/OP21/AvvisoDiPagamento"/>
        <rdfs:range rdf:resource="http://www.w3.org/2001/XMLSchema#string"/>
        <rdfs:comment xml:lang="it">Identificativo Univoco Versamento</rdfs:comment>
        <rdfs:comment xml:lang="en">Unique Payment Identification</rdfs:comment>
        <rdfs:label xml:lang="en">IUV</rdfs:label>
        <rdfs:label xml:lang="it">IUV</rdfs:label>
    </owl:DatatypeProperty>



    <!-- https://w3id.org/italia/onto/OP21/addebitoRicorrente -->

    <owl:DatatypeProperty rdf:about="https://w3id.org/italia/onto/OP21/addebitoRicorrente">
        <rdf:type rdf:resource="http://www.w3.org/2002/07/owl#FunctionalProperty"/>
        <rdfs:domain rdf:resource="https://w3id.org/italia/onto/OP21/MandatoSDD"/>
        <rdfs:range rdf:resource="http://www.w3.org/2001/XMLSchema#boolean"/>
        <rdfs:comment xml:lang="it">Assume il valore &quot;true&quot; se il Mandato SDD ha un addebito ricorrente, altrimenti assume il valore &quot;false&quot;.</rdfs:comment>
        <rdfs:comment xml:lang="en">It assumes the value &quot;true&quot; if the SDD Mandate has a recurring charge, otherwise it assumes the value &quot;false&quot;.</rdfs:comment>
        <rdfs:label xml:lang="it">addebito ricorrente</rdfs:label>
        <rdfs:label xml:lang="en">recurring credit</rdfs:label>
    </owl:DatatypeProperty>



    <!-- https://w3id.org/italia/onto/OP21/annoContributoTrimestrale -->

    <owl:DatatypeProperty rdf:about="https://w3id.org/italia/onto/OP21/annoContributoTrimestrale">
        <rdf:type rdf:resource="http://www.w3.org/2002/07/owl#FunctionalProperty"/>
        <rdfs:domain rdf:resource="https://w3id.org/italia/onto/OP21/ContributoTrimestraleOrdinario"/>
        <rdfs:range rdf:resource="http://www.w3.org/2001/XMLSchema#integer"/>
        <rdfs:comment xml:lang="en">It is the year in which the ordinary quarterly contribution is paid.</rdfs:comment>
        <rdfs:comment xml:lang="it">È l&apos;anno in cui viene versato il contributo trimestrale ordinario.</rdfs:comment>
        <rdfs:label xml:lang="it">anno contributo trimestrale</rdfs:label>
        <rdfs:label xml:lang="en">quarterly contribution year</rdfs:label>
    </owl:DatatypeProperty>



    <!-- https://w3id.org/italia/onto/OP21/causaleMovimento -->

    <owl:DatatypeProperty rdf:about="https://w3id.org/italia/onto/OP21/causaleMovimento">
        <rdf:type rdf:resource="http://www.w3.org/2002/07/owl#FunctionalProperty"/>
        <rdfs:domain rdf:resource="https://w3id.org/italia/onto/OP21/MovimentoDiDenaro"/>
        <rdfs:range rdf:resource="http://www.w3.org/2001/XMLSchema#string"/>
        <rdfs:comment xml:lang="en">Motivation of the movement, necessary to identify the motive of the movement of momey on a bank account.</rdfs:comment>
        <rdfs:comment xml:lang="it">Motivazione del movimento, serve a identificare il motivo dello movimento di denaro su un conto corrente.</rdfs:comment>
        <rdfs:label xml:lang="it">causale movimento</rdfs:label>
        <rdfs:label xml:lang="en">movement motive</rdfs:label>
    </owl:DatatypeProperty>



    <!-- https://w3id.org/italia/onto/OP21/codiceAvviso -->

    <owl:DatatypeProperty rdf:about="https://w3id.org/italia/onto/OP21/codiceAvviso">
        <rdf:type rdf:resource="http://www.w3.org/2002/07/owl#FunctionalProperty"/>
        <rdfs:domain rdf:resource="https://w3id.org/italia/onto/OP21/AvvisoDiPagamento"/>
        <rdfs:range rdf:resource="http://www.w3.org/2001/XMLSchema#string"/>
        <rdfs:comment xml:lang="en">Identification code of the Payment Notice.</rdfs:comment>
        <rdfs:comment xml:lang="it">È il codice relativo all&apos;Avviso Di Pagamento.</rdfs:comment>
        <rdfs:label xml:lang="it">codice avviso</rdfs:label>
        <rdfs:label xml:lang="en">notice code</rdfs:label>
    </owl:DatatypeProperty>



    <!-- https://w3id.org/italia/onto/OP21/codiceCBILL -->

    <owl:DatatypeProperty rdf:about="https://w3id.org/italia/onto/OP21/codiceCBILL">
        <rdf:type rdf:resource="http://www.w3.org/2002/07/owl#FunctionalProperty"/>
        <rdfs:domain rdf:resource="https://w3id.org/italia/onto/OP21/EnteCreditore"/>
        <rdfs:range rdf:resource="http://www.w3.org/2001/XMLSchema#string"/>
        <rdfs:comment xml:lang="it">Codice identificativo di Enti e Aziende che aderiscono al circuito CBILL/pagoPA</rdfs:comment>
        <rdfs:comment xml:lang="en">Identification code of Organizations and Companies that adhere to the CBILL/pagoPA circuit.</rdfs:comment>
        <rdfs:label xml:lang="en">CBILL code</rdfs:label>
        <rdfs:label xml:lang="it">codice CBILL</rdfs:label>
    </owl:DatatypeProperty>



    <!-- https://w3id.org/italia/onto/OP21/codiceContrattoDiLavoro -->

    <owl:DatatypeProperty rdf:about="https://w3id.org/italia/onto/OP21/codiceContrattoDiLavoro">
        <owl:equivalentProperty rdf:resource="https://w3id.org/italia/onto/OP21/codiceRapportoDiLavoro"/>
        <rdf:type rdf:resource="http://www.w3.org/2002/07/owl#FunctionalProperty"/>
        <rdfs:domain rdf:resource="https://w3id.org/italia/onto/OP21/ContrattoDiLavoro"/>
        <rdfs:range rdf:resource="http://www.w3.org/2001/XMLSchema#string"/>
        <rdfs:comment xml:lang="en">It is the Domestic Work Contract code equivalent to the Domestic Work Relationship code it originated.</rdfs:comment>
        <rdfs:comment xml:lang="it">È il codice del Contratto Di Lavoro Domestico equivalente al codice del Rapporto Di Lavoro Domestico a cui ha dato origine.</rdfs:comment>
        <rdfs:label xml:lang="it">codice contratto di lavoro</rdfs:label>
        <rdfs:label xml:lang="en">employment contract code</rdfs:label>
    </owl:DatatypeProperty>



    <!-- https://w3id.org/italia/onto/OP21/codiceINPS -->

    <owl:DatatypeProperty rdf:about="https://w3id.org/italia/onto/OP21/codiceINPS">
        <rdf:type rdf:resource="http://www.w3.org/2002/07/owl#FunctionalProperty"/>
        <rdfs:domain>
            <owl:Class>
                <owl:unionOf rdf:parseType="Collection">
                    <rdf:Description rdf:about="https://w3id.org/italia/onto/OP21/BollettinoDiPagamentoRata"/>
                    <rdf:Description rdf:about="https://w3id.org/italia/onto/OP21/BollettinoDiPagamentoUnico"/>
                </owl:unionOf>
            </owl:Class>
        </rdfs:domain>
        <rdfs:range rdf:resource="http://www.w3.org/2001/XMLSchema#string"/>
        <rdfs:comment xml:lang="en">It is the code that INPS assigns to the Payment Slip in cases of single or installment payment. It is made up of the application number and the code of the INPS office.</rdfs:comment>
        <rdfs:comment xml:lang="it">È il codice che l&apos;INPS assegna al Bollettino Di Pagamento nei casi di pagamento unico o di rata. È composto dal numero pratica e dl codice della sede INPS.</rdfs:comment>
        <rdfs:label xml:lang="en">INPS code</rdfs:label>
        <rdfs:label xml:lang="it">codice INPS</rdfs:label>
    </owl:DatatypeProperty>



    <!-- https://w3id.org/italia/onto/OP21/codiceMAV -->

    <owl:DatatypeProperty rdf:about="https://w3id.org/italia/onto/OP21/codiceMAV">
        <rdf:type rdf:resource="http://www.w3.org/2002/07/owl#FunctionalProperty"/>
        <rdfs:domain rdf:resource="https://w3id.org/italia/onto/OP21/BollettinoMAV"/>
        <rdfs:range rdf:resource="http://www.w3.org/2001/XMLSchema#string"/>
        <rdfs:comment xml:lang="it">Codice identificativo di un bollettino MAV.</rdfs:comment>
        <rdfs:comment xml:lang="en">Identification code of a MAV slip.</rdfs:comment>
        <rdfs:label xml:lang="en">MAV code</rdfs:label>
        <rdfs:label xml:lang="it">codice MAV</rdfs:label>
    </owl:DatatypeProperty>



    <!-- https://w3id.org/italia/onto/OP21/codiceMandato -->

    <owl:DatatypeProperty rdf:about="https://w3id.org/italia/onto/OP21/codiceMandato">
        <rdf:type rdf:resource="http://www.w3.org/2002/07/owl#FunctionalProperty"/>
        <rdfs:domain rdf:resource="https://w3id.org/italia/onto/OP21/MandatoSDD"/>
        <rdfs:range rdf:resource="http://www.w3.org/2001/XMLSchema#string"/>
        <rdfs:comment xml:lang="en">Identification code of the SDD Mandate.</rdfs:comment>
        <rdfs:comment xml:lang="it">È il codice relativo al Mandato SDD.</rdfs:comment>
        <rdfs:label xml:lang="it">codice mandato</rdfs:label>
        <rdfs:label xml:lang="en">mandate code</rdfs:label>
    </owl:DatatypeProperty>



    <!-- https://w3id.org/italia/onto/OP21/codiceOrganizzazione -->

    <owl:DatatypeProperty rdf:about="https://w3id.org/italia/onto/OP21/codiceOrganizzazione">
        <rdf:type rdf:resource="http://www.w3.org/2002/07/owl#FunctionalProperty"/>
        <rdfs:domain rdf:resource="https://w3id.org/italia/onto/OP21/OrganizzazioneDiAssistenza"/>
        <rdfs:range rdf:resource="http://www.w3.org/2001/XMLSchema#string"/>
        <rdfs:comment xml:lang="en">Identification code of the Support Organization.</rdfs:comment>
        <rdfs:comment xml:lang="it">È il codice relativo all&apos;Organizzazione Di Assistenza.</rdfs:comment>
        <rdfs:label xml:lang="it">codice organizzazione</rdfs:label>
        <rdfs:label xml:lang="en">organization code</rdfs:label>
    </owl:DatatypeProperty>



    <!-- https://w3id.org/italia/onto/OP21/codiceRID -->

    <owl:DatatypeProperty rdf:about="https://w3id.org/italia/onto/OP21/codiceRID">
        <rdf:type rdf:resource="http://www.w3.org/2002/07/owl#FunctionalProperty"/>
        <rdfs:domain rdf:resource="https://w3id.org/italia/onto/OP21/RID"/>
        <rdfs:range rdf:resource="http://www.w3.org/2001/XMLSchema#string"/>
        <rdfs:comment xml:lang="en">The RID identification code.</rdfs:comment>
        <rdfs:comment xml:lang="it">È il codice relativo al RID.</rdfs:comment>
        <rdfs:label xml:lang="en">RID code</rdfs:label>
        <rdfs:label xml:lang="it">codice RID</rdfs:label>
    </owl:DatatypeProperty>



    <!-- https://w3id.org/italia/onto/OP21/codiceRapportoDiLavoro -->

    <owl:DatatypeProperty rdf:about="https://w3id.org/italia/onto/OP21/codiceRapportoDiLavoro">
        <rdf:type rdf:resource="http://www.w3.org/2002/07/owl#FunctionalProperty"/>
        <rdfs:domain rdf:resource="https://w3id.org/italia/onto/OP21/RapportoDiLavoroDomestico"/>
        <rdfs:range rdf:resource="http://www.w3.org/2001/XMLSchema#string"/>
        <rdfs:comment xml:lang="en">The Domestic Work Relationship code assigned by INPS when registering the relevant contract.</rdfs:comment>
        <rdfs:comment xml:lang="it">È il codice relativo al  Rapporto Di Lavoro Domestico assegnato da INPS al momento della registrazione del relativo contratto.</rdfs:comment>
        <rdfs:label xml:lang="it">codice rapporto di lavoro</rdfs:label>
        <rdfs:label xml:lang="en">employment relationship code</rdfs:label>
    </owl:DatatypeProperty>



    <!-- https://w3id.org/italia/onto/OP21/codiceRiscossione -->

    <owl:DatatypeProperty rdf:about="https://w3id.org/italia/onto/OP21/codiceRiscossione">
        <rdf:type rdf:resource="http://www.w3.org/2002/07/owl#FunctionalProperty"/>
        <rdfs:domain rdf:resource="https://w3id.org/italia/onto/OP21/EsitoPagamentoDefinitivo"/>
        <rdfs:range rdf:resource="http://www.w3.org/2001/XMLSchema#string"/>
        <rdfs:comment xml:lang="it">Identifica e certifica l&apos;avvenuto incasso di un pagamento.</rdfs:comment>
        <rdfs:comment xml:lang="en">Identifies and certifies that a payment has been collected.</rdfs:comment>
        <rdfs:label xml:lang="it">codice riscossione</rdfs:label>
        <rdfs:label xml:lang="en">collection code</rdfs:label>
    </owl:DatatypeProperty>



    <!-- https://w3id.org/italia/onto/OP21/codiceSedeINPS -->

    <owl:DatatypeProperty rdf:about="https://w3id.org/italia/onto/OP21/codiceSedeINPS">
        <rdf:type rdf:resource="http://www.w3.org/2002/07/owl#FunctionalProperty"/>
        <rdfs:domain rdf:resource="https://w3id.org/italia/onto/OP21/SedeINPS"/>
        <rdfs:range rdf:resource="http://www.w3.org/2001/XMLSchema#string"/>
        <rdfs:comment xml:lang="en">This is the identification code of the INPS office.</rdfs:comment>
        <rdfs:comment xml:lang="it">È il codice relativo alla Sede INPS.</rdfs:comment>
        <rdfs:label xml:lang="en">INPS office identification code</rdfs:label>
        <rdfs:label xml:lang="it">codice sede INPS</rdfs:label>
    </owl:DatatypeProperty>



    <!-- https://w3id.org/italia/onto/OP21/codiceServizioDiPagamento -->

    <owl:DatatypeProperty rdf:about="https://w3id.org/italia/onto/OP21/codiceServizioDiPagamento">
        <rdf:type rdf:resource="http://www.w3.org/2002/07/owl#FunctionalProperty"/>
        <rdfs:domain rdf:resource="https://w3id.org/italia/onto/OP21/ServizioDiPagamento"/>
        <rdfs:range rdf:resource="http://www.w3.org/2001/XMLSchema#string"/>
        <rdfs:comment xml:lang="en">Identification code of the Payment Service</rdfs:comment>
        <rdfs:comment xml:lang="it">È il codice relativo al Servizio Di Pagamento.</rdfs:comment>
        <rdfs:label xml:lang="it">codice servizio di pagamento</rdfs:label>
        <rdfs:label xml:lang="en">payment service code</rdfs:label>
    </owl:DatatypeProperty>



    <!-- https://w3id.org/italia/onto/OP21/codiceSistemaDiPagamento -->

    <owl:DatatypeProperty rdf:about="https://w3id.org/italia/onto/OP21/codiceSistemaDiPagamento">
        <rdf:type rdf:resource="http://www.w3.org/2002/07/owl#FunctionalProperty"/>
        <rdfs:domain rdf:resource="https://w3id.org/italia/onto/OP21/SistemaDiPagamentoElettronico"/>
        <rdfs:range rdf:resource="http://www.w3.org/2001/XMLSchema#string"/>
        <rdfs:comment xml:lang="en">Identification code of the Electronic Payment System.</rdfs:comment>
        <rdfs:comment xml:lang="it">È il codice relativo al Sistema Di Pagamento Elettronico.</rdfs:comment>
        <rdfs:label xml:lang="it">codice sistema di pagamento</rdfs:label>
        <rdfs:label xml:lang="en">payment system code</rdfs:label>
    </owl:DatatypeProperty>



    <!-- https://w3id.org/italia/onto/OP21/dataAtto -->

    <owl:DatatypeProperty rdf:about="https://w3id.org/italia/onto/OP21/dataAtto">
        <rdf:type rdf:resource="http://www.w3.org/2002/07/owl#FunctionalProperty"/>
        <rdfs:domain rdf:resource="https://w3id.org/italia/onto/OP21/AttoAdeguamentoContributivo"/>
        <rdfs:range rdf:resource="http://www.w3.org/2001/XMLSchema#dateTime"/>
        <rdfs:comment xml:lang="en">It is the date of the Tax Contribution Adjustment Deed.</rdfs:comment>
        <rdfs:comment xml:lang="it">È la data dell&apos;Atto Adeguamento Contributivo.</rdfs:comment>
        <rdfs:label xml:lang="it">data atto</rdfs:label>
        <rdfs:label xml:lang="en">deed date</rdfs:label>
    </owl:DatatypeProperty>



    <!-- https://w3id.org/italia/onto/OP21/dataDepositoContratto -->

    <owl:DatatypeProperty rdf:about="https://w3id.org/italia/onto/OP21/dataDepositoContratto">
        <rdf:type rdf:resource="http://www.w3.org/2002/07/owl#FunctionalProperty"/>
        <rdfs:domain rdf:resource="https://w3id.org/italia/onto/OP21/RapportoDiLavoroDomestico"/>
        <rdfs:range rdf:resource="http://www.w3.org/2001/XMLSchema#dateTime"/>
        <rdfs:comment xml:lang="en">It is the filing date of the Employment Contract</rdfs:comment>
        <rdfs:comment xml:lang="it">È la data di deposito del Contratto Di Lavoro</rdfs:comment>
        <rdfs:label xml:lang="en">contract filing date</rdfs:label>
        <rdfs:label xml:lang="it">data deposito contratto</rdfs:label>
    </owl:DatatypeProperty>



    <!-- https://w3id.org/italia/onto/OP21/dataDiPrenotazione -->

    <owl:DatatypeProperty rdf:about="https://w3id.org/italia/onto/OP21/dataDiPrenotazione">
        <rdf:type rdf:resource="http://www.w3.org/2002/07/owl#FunctionalProperty"/>
        <rdfs:domain rdf:resource="https://w3id.org/italia/onto/OP21/PrenotazioneDiPagamento"/>
        <rdfs:range rdf:resource="http://www.w3.org/2001/XMLSchema#dateTime"/>
        <rdfs:comment xml:lang="en">It is the date in which the Payment is reserved.</rdfs:comment>
        <rdfs:comment xml:lang="it">È la data relativa alla Prenotazione Di Pagamento.</rdfs:comment>
        <rdfs:label xml:lang="en">booking date</rdfs:label>
        <rdfs:label xml:lang="it">data di prenotazione</rdfs:label>
    </owl:DatatypeProperty>



    <!-- https://w3id.org/italia/onto/OP21/dataDomanda -->

    <owl:DatatypeProperty rdf:about="https://w3id.org/italia/onto/OP21/dataDomanda">
        <rdf:type rdf:resource="http://www.w3.org/2002/07/owl#FunctionalProperty"/>
        <rdfs:domain rdf:resource="https://w3id.org/italia/onto/OP21/DomandaAdeguamentoContributivo"/>
        <rdfs:range rdf:resource="http://www.w3.org/2001/XMLSchema#dateTime"/>
        <rdfs:comment xml:lang="en">This is the date of the Tax Adjustment Application.</rdfs:comment>
        <rdfs:comment xml:lang="it">È la data relativa alla Domanda Adeguamento Contributivo.</rdfs:comment>
        <rdfs:label xml:lang="it">data domanda</rdfs:label>
        <rdfs:label xml:lang="en">request date</rdfs:label>
    </owl:DatatypeProperty>



    <!-- https://w3id.org/italia/onto/OP21/dataFineRapporto -->

    <owl:DatatypeProperty rdf:about="https://w3id.org/italia/onto/OP21/dataFineRapporto">
        <rdf:type rdf:resource="http://www.w3.org/2002/07/owl#FunctionalProperty"/>
        <rdfs:domain rdf:resource="https://w3id.org/italia/onto/OP21/RapportoDiLavoroDomesticoCessato"/>
        <rdfs:range rdf:resource="http://www.w3.org/2001/XMLSchema#dateTime"/>
        <rdfs:comment xml:lang="en">It is the date of termination of a Domestic Work Relationship.</rdfs:comment>
        <rdfs:comment xml:lang="it">È la data di cessazione di un Rapporto Di Lavoro Domestico.</rdfs:comment>
        <rdfs:label xml:lang="it">data fine rapporto</rdfs:label>
        <rdfs:label xml:lang="en">relationship end date</rdfs:label>
    </owl:DatatypeProperty>



    <!-- https://w3id.org/italia/onto/OP21/dataInizioRapporto -->

    <owl:DatatypeProperty rdf:about="https://w3id.org/italia/onto/OP21/dataInizioRapporto">
        <rdf:type rdf:resource="http://www.w3.org/2002/07/owl#FunctionalProperty"/>
        <rdfs:domain rdf:resource="https://w3id.org/italia/onto/OP21/RapportoDiLavoroDomesticoAttivo"/>
        <rdfs:range rdf:resource="http://www.w3.org/2001/XMLSchema#dateTime"/>
        <rdfs:comment xml:lang="en">It is the start date of a Domestic Work Relationship</rdfs:comment>
        <rdfs:comment xml:lang="it">È la data di inizio di un Rapporto Di Lavoro Domestico</rdfs:comment>
        <rdfs:label xml:lang="it">data inizio rapporto</rdfs:label>
        <rdfs:label xml:lang="en">relationship start date</rdfs:label>
    </owl:DatatypeProperty>



    <!-- https://w3id.org/italia/onto/OP21/dataMovimento -->

    <owl:DatatypeProperty rdf:about="https://w3id.org/italia/onto/OP21/dataMovimento">
        <rdf:type rdf:resource="http://www.w3.org/2002/07/owl#FunctionalProperty"/>
        <rdfs:domain rdf:resource="https://w3id.org/italia/onto/OP21/MovimentoDiDenaro"/>
        <rdfs:range rdf:resource="http://www.w3.org/2001/XMLSchema#dateTime"/>
        <rdfs:comment xml:lang="en">Date of the Money Movement.</rdfs:comment>
        <rdfs:comment xml:lang="it">È la data relativa al Movimento Di Denaro.</rdfs:comment>
        <rdfs:label xml:lang="it">data movimento</rdfs:label>
        <rdfs:label xml:lang="en">movement date</rdfs:label>
    </owl:DatatypeProperty>



    <!-- https://w3id.org/italia/onto/OP21/dataOrdinePagamento -->

    <owl:DatatypeProperty rdf:about="https://w3id.org/italia/onto/OP21/dataOrdinePagamento">
        <rdf:type rdf:resource="http://www.w3.org/2002/07/owl#FunctionalProperty"/>
        <rdfs:domain rdf:resource="https://w3id.org/italia/onto/OP21/OrdineDiPagamento"/>
        <rdfs:range rdf:resource="http://www.w3.org/2001/XMLSchema#dateTime"/>
        <rdfs:comment xml:lang="en">It is the date of the Payment Order.</rdfs:comment>
        <rdfs:comment xml:lang="it">È la data relativa all&apos;Ordine Di Pagamento.</rdfs:comment>
        <rdfs:label xml:lang="it">data ordine pagamento</rdfs:label>
        <rdfs:label xml:lang="en">payment order date</rdfs:label>
    </owl:DatatypeProperty>



    <!-- https://w3id.org/italia/onto/OP21/dataPagamento -->

    <owl:DatatypeProperty rdf:about="https://w3id.org/italia/onto/OP21/dataPagamento">
        <rdf:type rdf:resource="http://www.w3.org/2002/07/owl#FunctionalProperty"/>
        <rdfs:domain rdf:resource="https://w3id.org/italia/onto/OP21/Pagamento"/>
        <rdfs:range rdf:resource="http://www.w3.org/2001/XMLSchema#dateTime"/>
        <rdfs:comment xml:lang="en">It is the date in which the Payment is performed.</rdfs:comment>
        <rdfs:comment xml:lang="it">È la data relativa al Pagamento.</rdfs:comment>
        <rdfs:label xml:lang="it">data pagamento</rdfs:label>
        <rdfs:label xml:lang="en">payment date</rdfs:label>
    </owl:DatatypeProperty>



    <!-- https://w3id.org/italia/onto/OP21/dataRicevuta -->

    <owl:DatatypeProperty rdf:about="https://w3id.org/italia/onto/OP21/dataRicevuta">
        <rdf:type rdf:resource="http://www.w3.org/2002/07/owl#FunctionalProperty"/>
        <rdfs:domain rdf:resource="https://w3id.org/italia/onto/OP21/RicevutaDiMovimento"/>
        <rdfs:range rdf:resource="http://www.w3.org/2001/XMLSchema#dateTime"/>
        <rdfs:comment xml:lang="en">It is the date of the Movement Receipt.</rdfs:comment>
        <rdfs:comment xml:lang="it">È la data relativa alla Ricevuta Di Movimento.</rdfs:comment>
        <rdfs:label xml:lang="it">data ricevuta</rdfs:label>
        <rdfs:label xml:lang="en">receipt date</rdfs:label>
    </owl:DatatypeProperty>



    <!-- https://w3id.org/italia/onto/OP21/dataScadenzaContributoTrimestrale -->

    <owl:DatatypeProperty rdf:about="https://w3id.org/italia/onto/OP21/dataScadenzaContributoTrimestrale">
        <rdf:type rdf:resource="http://www.w3.org/2002/07/owl#FunctionalProperty"/>
        <rdfs:domain rdf:resource="https://w3id.org/italia/onto/OP21/ContributoTrimestraleOrdinario"/>
        <rdfs:range rdf:resource="http://www.w3.org/2001/XMLSchema#dateTime"/>
        <rdfs:comment xml:lang="en">It is the due date for the payment of quarterly contributions by a domestic worker.</rdfs:comment>
        <rdfs:comment xml:lang="it">È la data di scadenza per il versamento dei contributi trimestrali di un lavoratore domestico.</rdfs:comment>
        <rdfs:label xml:lang="it">data scadenza contributo trimestrale</rdfs:label>
        <rdfs:label xml:lang="en">quarterly contribution due date</rdfs:label>
    </owl:DatatypeProperty>



    <!-- https://w3id.org/italia/onto/OP21/dataScadenzaOnereContributivo -->

    <owl:DatatypeProperty rdf:about="https://w3id.org/italia/onto/OP21/dataScadenzaOnereContributivo">
        <rdf:type rdf:resource="http://www.w3.org/2002/07/owl#FunctionalProperty"/>
        <rdfs:domain rdf:resource="https://w3id.org/italia/onto/OP21/OnereContributivo"/>
        <rdfs:range rdf:resource="http://www.w3.org/2001/XMLSchema#dateTime"/>
        <rdfs:comment xml:lang="en">It is the expiry date relating to the Contribution Fee.</rdfs:comment>
        <rdfs:comment xml:lang="it">È la data di scadenza relativa all&apos;Onere Contributivo.</rdfs:comment>
        <rdfs:label xml:lang="en">contribution due date</rdfs:label>
        <rdfs:label xml:lang="it">data scadenza onere contributivo</rdfs:label>
    </owl:DatatypeProperty>



    <!-- https://w3id.org/italia/onto/OP21/dataScadenzaPagamento -->

    <owl:DatatypeProperty rdf:about="https://w3id.org/italia/onto/OP21/dataScadenzaPagamento">
        <rdf:type rdf:resource="http://www.w3.org/2002/07/owl#FunctionalProperty"/>
        <rdfs:domain rdf:resource="https://w3id.org/italia/onto/OP21/AvvisoDiPagamento"/>
        <rdfs:range rdf:resource="http://www.w3.org/2001/XMLSchema#dateTime"/>
        <rdfs:comment xml:lang="en">It is the expiry date relating to the Payment Notice.</rdfs:comment>
        <rdfs:comment xml:lang="it">È la data di scadenza relativa all&apos;Avviso Di Pagamento.</rdfs:comment>
        <rdfs:label xml:lang="it">data scadenza pagamento</rdfs:label>
        <rdfs:label xml:lang="en">payment due date</rdfs:label>
    </owl:DatatypeProperty>



    <!-- https://w3id.org/italia/onto/OP21/dataScadenzaRata -->

    <owl:DatatypeProperty rdf:about="https://w3id.org/italia/onto/OP21/dataScadenzaRata">
        <rdf:type rdf:resource="http://www.w3.org/2002/07/owl#FunctionalProperty"/>
        <rdfs:domain rdf:resource="https://w3id.org/italia/onto/OP21/RataDiOnereContributivo"/>
        <rdfs:range rdf:resource="http://www.w3.org/2001/XMLSchema#dateTime"/>
        <rdfs:comment xml:lang="en">It is the expiry date relating to the Contribution Charge Installment.</rdfs:comment>
        <rdfs:comment xml:lang="it">È la data di scadenza relativa alla Rata Dell&apos;Onere Contributivo.</rdfs:comment>
        <rdfs:label xml:lang="it">data scadenza rata</rdfs:label>
        <rdfs:label xml:lang="en">installment deadline date</rdfs:label>
    </owl:DatatypeProperty>



    <!-- https://w3id.org/italia/onto/OP21/descrizioneEsitoPagamento -->

    <owl:DatatypeProperty rdf:about="https://w3id.org/italia/onto/OP21/descrizioneEsitoPagamento">
        <rdfs:domain rdf:resource="https://w3id.org/italia/onto/OP21/EsitoPagamento"/>
        <rdfs:range rdf:resource="http://www.w3.org/2001/XMLSchema#string"/>
        <rdfs:comment xml:lang="en">A description of the payment outcome. In case the outcome is &quot;deferred&quot;, the outcome of the payment is not yet known.</rdfs:comment>
        <rdfs:comment xml:lang="it">È una descrizione associata all&apos;Esito Pagamento. Nel caso in cui l&apos;esito risulta &quot;DIFFERITO&quot; non si conosce ancora l’esito del pagamento.</rdfs:comment>
        <rdfs:label xml:lang="it">descrizione esito pagamento</rdfs:label>
        <rdfs:label xml:lang="en">payment outcome description</rdfs:label>
    </owl:DatatypeProperty>



    <!-- https://w3id.org/italia/onto/OP21/descrizioneFinalità -->

    <owl:DatatypeProperty rdf:about="https://w3id.org/italia/onto/OP21/descrizioneFinalità">
        <rdf:type rdf:resource="http://www.w3.org/2002/07/owl#FunctionalProperty"/>
        <rdfs:domain rdf:resource="https://w3id.org/italia/onto/OP21/Finalità"/>
        <rdfs:range rdf:resource="http://www.w3.org/2001/XMLSchema#string"/>
        <rdfs:comment xml:lang="en">Description of the Purpose of the Payment.</rdfs:comment>
        <rdfs:comment xml:lang="it">È la descrizione relativa alla Finalità.</rdfs:comment>
        <rdfs:label xml:lang="it">descrizione finalità</rdfs:label>
        <rdfs:label xml:lang="en">purpose description</rdfs:label>
    </owl:DatatypeProperty>



    <!-- https://w3id.org/italia/onto/OP21/descrizionePratica -->

    <owl:DatatypeProperty rdf:about="https://w3id.org/italia/onto/OP21/descrizionePratica">
        <rdf:type rdf:resource="http://www.w3.org/2002/07/owl#FunctionalProperty"/>
        <rdfs:domain rdf:resource="https://w3id.org/italia/onto/OP21/PraticaAdeguamentoContributivo"/>
        <rdfs:range rdf:resource="http://www.w3.org/2001/XMLSchema#string"/>
        <rdfs:comment xml:lang="en">Description of the Tax Adjustment Application.</rdfs:comment>
        <rdfs:comment xml:lang="it">È la descrizione relativa alla Pratica.</rdfs:comment>
        <rdfs:label xml:lang="en">application description</rdfs:label>
        <rdfs:label xml:lang="it">descrizione pratica</rdfs:label>
    </owl:DatatypeProperty>



    <!-- https://w3id.org/italia/onto/OP21/identificatoreCorrentista -->

    <owl:DatatypeProperty rdf:about="https://w3id.org/italia/onto/OP21/identificatoreCorrentista">
        <rdfs:subPropertyOf rdf:resource="https://w3id.org/italia/onto/l0/identifier"/>
        <rdf:type rdf:resource="http://www.w3.org/2002/07/owl#FunctionalProperty"/>
        <rdfs:domain rdf:resource="https://w3id.org/italia/onto/OP21/Correntista"/>
        <rdfs:range rdf:resource="http://www.w3.org/2001/XMLSchema#string"/>
        <rdfs:comment xml:lang="it">Identifica il Correntista.</rdfs:comment>
        <rdfs:comment xml:lang="en">Identifies the Account Holder</rdfs:comment>
        <rdfs:label xml:lang="en">account holder identifier</rdfs:label>
        <rdfs:label xml:lang="it">identificatore correntista</rdfs:label>
    </owl:DatatypeProperty>



    <!-- https://w3id.org/italia/onto/OP21/identificatoreDatoreDiLavoroDomestico -->

    <owl:DatatypeProperty rdf:about="https://w3id.org/italia/onto/OP21/identificatoreDatoreDiLavoroDomestico">
        <rdfs:subPropertyOf rdf:resource="https://w3id.org/italia/onto/l0/identifier"/>
        <rdf:type rdf:resource="http://www.w3.org/2002/07/owl#FunctionalProperty"/>
        <rdfs:domain rdf:resource="https://w3id.org/italia/onto/OP21/DatoreDiLavoroDomestico"/>
        <rdfs:range rdf:resource="http://www.w3.org/2001/XMLSchema#string"/>
        <rdfs:comment xml:lang="it">Identifica il Datore Di Lavoro Domestico.</rdfs:comment>
        <rdfs:comment xml:lang="en">Identifies the Domestic Employer</rdfs:comment>
        <rdfs:label xml:lang="en">domestic employer identifier</rdfs:label>
        <rdfs:label xml:lang="it">identificatore datore di lavoro domestico</rdfs:label>
    </owl:DatatypeProperty>



    <!-- https://w3id.org/italia/onto/OP21/identificatoreEsitoPagamento -->

    <owl:DatatypeProperty rdf:about="https://w3id.org/italia/onto/OP21/identificatoreEsitoPagamento">
        <rdfs:subPropertyOf rdf:resource="https://w3id.org/italia/onto/l0/identifier"/>
        <rdf:type rdf:resource="http://www.w3.org/2002/07/owl#FunctionalProperty"/>
        <rdfs:domain rdf:resource="https://w3id.org/italia/onto/OP21/EsitoPagamento"/>
        <rdfs:range rdf:resource="http://www.w3.org/2001/XMLSchema#string"/>
        <rdfs:comment xml:lang="en">Identification code of the Payment Outcome.</rdfs:comment>
        <rdfs:comment xml:lang="it">È l&apos;identificativo di un Esito Pagamento.</rdfs:comment>
        <rdfs:label xml:lang="it">identificatore esito pagamento</rdfs:label>
        <rdfs:label xml:lang="en">payment outcome identifier</rdfs:label>
    </owl:DatatypeProperty>



    <!-- https://w3id.org/italia/onto/OP21/identificatoreLavoratoreDomestico -->

    <owl:DatatypeProperty rdf:about="https://w3id.org/italia/onto/OP21/identificatoreLavoratoreDomestico">
        <rdfs:subPropertyOf rdf:resource="https://w3id.org/italia/onto/l0/identifier"/>
        <rdf:type rdf:resource="http://www.w3.org/2002/07/owl#FunctionalProperty"/>
        <rdfs:domain rdf:resource="https://w3id.org/italia/onto/OP21/LavoratoreDomestico"/>
        <rdfs:range rdf:resource="http://www.w3.org/2001/XMLSchema#string"/>
        <rdfs:comment xml:lang="it">Identifica il Lavoratore Domestico.</rdfs:comment>
        <rdfs:comment xml:lang="en">Identifies the Domestic Worker</rdfs:comment>
        <rdfs:label xml:lang="en">domestic worker identifier</rdfs:label>
        <rdfs:label xml:lang="it">identificatore lavoratore domestico</rdfs:label>
    </owl:DatatypeProperty>



    <!-- https://w3id.org/italia/onto/OP21/identificatoreMovimento -->

    <owl:DatatypeProperty rdf:about="https://w3id.org/italia/onto/OP21/identificatoreMovimento">
        <owl:equivalentProperty rdf:resource="https://w3id.org/italia/onto/OP21/identificatoreRicevuta"/>
        <rdf:type rdf:resource="http://www.w3.org/2002/07/owl#FunctionalProperty"/>
        <rdfs:domain rdf:resource="https://w3id.org/italia/onto/OP21/MovimentoDiDenaro"/>
        <rdfs:range rdf:resource="http://www.w3.org/2001/XMLSchema#string"/>
        <rdfs:comment xml:lang="it">Identifica un Movimento Di Denaro.</rdfs:comment>
        <rdfs:comment xml:lang="en">Identifies a Money Movement.</rdfs:comment>
        <rdfs:label xml:lang="it">identificatore movimento</rdfs:label>
        <rdfs:label xml:lang="en">movement identifier</rdfs:label>
    </owl:DatatypeProperty>



    <!-- https://w3id.org/italia/onto/OP21/identificatoreOrdinePagamento -->

    <owl:DatatypeProperty rdf:about="https://w3id.org/italia/onto/OP21/identificatoreOrdinePagamento">
        <rdf:type rdf:resource="http://www.w3.org/2002/07/owl#FunctionalProperty"/>
        <rdfs:domain rdf:resource="https://w3id.org/italia/onto/OP21/OrdineDiPagamento"/>
        <rdfs:range rdf:resource="http://www.w3.org/2001/XMLSchema#string"/>
        <rdfs:comment xml:lang="it">Identifica l&apos;Ordine Di Pagamento.</rdfs:comment>
        <rdfs:comment xml:lang="en">Identifies the Payment Order.</rdfs:comment>
        <rdfs:label xml:lang="it">identificatore ordine pagamento</rdfs:label>
        <rdfs:label xml:lang="en">payment order identifier</rdfs:label>
    </owl:DatatypeProperty>



    <!-- https://w3id.org/italia/onto/OP21/identificatorePrenotazionePagamento -->

    <owl:DatatypeProperty rdf:about="https://w3id.org/italia/onto/OP21/identificatorePrenotazionePagamento">
        <rdfs:subPropertyOf rdf:resource="https://w3id.org/italia/onto/l0/identifier"/>
        <rdf:type rdf:resource="http://www.w3.org/2002/07/owl#FunctionalProperty"/>
        <rdfs:domain rdf:resource="https://w3id.org/italia/onto/OP21/PrenotazioneDiPagamento"/>
        <rdfs:range rdf:resource="http://www.w3.org/2001/XMLSchema#string"/>
        <rdfs:comment xml:lang="it">Identificatore della prenotazione di pagamento.</rdfs:comment>
        <rdfs:comment xml:lang="en">Identifies the payment reservation.</rdfs:comment>
        <rdfs:label xml:lang="it">identificatore prenotazione pagamento</rdfs:label>
        <rdfs:label xml:lang="en">payment reservation identifier</rdfs:label>
    </owl:DatatypeProperty>



    <!-- https://w3id.org/italia/onto/OP21/identificatoreRicevuta -->

    <owl:DatatypeProperty rdf:about="https://w3id.org/italia/onto/OP21/identificatoreRicevuta">
        <rdf:type rdf:resource="http://www.w3.org/2002/07/owl#FunctionalProperty"/>
        <rdfs:domain rdf:resource="https://w3id.org/italia/onto/OP21/RicevutaDiMovimento"/>
        <rdfs:range rdf:resource="http://www.w3.org/2001/XMLSchema#string"/>
        <rdfs:comment xml:lang="it">Identifica una Ricevuta Di Movimento. È equivalente all&apos;identificativo di un Movimento Di Denaro.</rdfs:comment>
        <rdfs:comment xml:lang="en">Identifies a Movement Receipt. It is equivalent to a movement identifier.</rdfs:comment>
        <rdfs:label xml:lang="it">identificatore ricevuta</rdfs:label>
        <rdfs:label xml:lang="en">receipt identifier</rdfs:label>
    </owl:DatatypeProperty>



    <!-- https://w3id.org/italia/onto/OP21/identificatoreRichiedenteAdeguamentoContributivo -->

    <owl:DatatypeProperty rdf:about="https://w3id.org/italia/onto/OP21/identificatoreRichiedenteAdeguamentoContributivo">
        <rdfs:subPropertyOf rdf:resource="https://w3id.org/italia/onto/l0/identifier"/>
        <rdf:type rdf:resource="http://www.w3.org/2002/07/owl#FunctionalProperty"/>
        <rdfs:domain rdf:resource="https://w3id.org/italia/onto/OP21/RichiedenteAdeguamentoContributivo"/>
        <rdfs:range rdf:resource="http://www.w3.org/2001/XMLSchema#string"/>
        <rdfs:comment xml:lang="it">Identifica il Richiedente Adeguamento Contributivo.</rdfs:comment>
        <rdfs:comment xml:lang="en">Identifies the Contribution Adjustment Applicant.</rdfs:comment>
        <rdfs:label xml:lang="en">contribution adjustment applicant identifier</rdfs:label>
        <rdfs:label xml:lang="it">identificatore richiedente adeguamento contributivo</rdfs:label>
    </owl:DatatypeProperty>



    <!-- https://w3id.org/italia/onto/OP21/identificatoreSessionePagamento -->

    <owl:DatatypeProperty rdf:about="https://w3id.org/italia/onto/OP21/identificatoreSessionePagamento">
        <rdf:type rdf:resource="http://www.w3.org/2002/07/owl#FunctionalProperty"/>
        <rdfs:domain rdf:resource="https://w3id.org/italia/onto/OP21/SessionePagamentoElettronico"/>
        <rdfs:range rdf:resource="http://www.w3.org/2001/XMLSchema#string"/>
        <rdfs:comment xml:lang="it">Identifica la Sessione Di Pagamento.</rdfs:comment>
        <rdfs:comment xml:lang="en">Identifies the Payment Session.</rdfs:comment>
        <rdfs:label xml:lang="it">identificatore sessione pagamento</rdfs:label>
        <rdfs:label xml:lang="en">payment session identifier</rdfs:label>
    </owl:DatatypeProperty>



    <!-- https://w3id.org/italia/onto/OP21/importoCommissioneMovimento -->

    <owl:DatatypeProperty rdf:about="https://w3id.org/italia/onto/OP21/importoCommissioneMovimento">
        <rdf:type rdf:resource="http://www.w3.org/2002/07/owl#FunctionalProperty"/>
        <rdfs:domain rdf:resource="https://w3id.org/italia/onto/OP21/MovimentoDiDenaro"/>
        <rdfs:range rdf:resource="http://www.w3.org/2001/XMLSchema#decimal"/>
        <rdfs:comment xml:lang="en">It is the cost of a Money Movement operation, if any.</rdfs:comment>
        <rdfs:comment xml:lang="it">È il costo di una operazione di Movimento Di Denaro, se presente.</rdfs:comment>
        <rdfs:label xml:lang="it">importo commissione movimento</rdfs:label>
        <rdfs:label xml:lang="en">movement commission amount</rdfs:label>
    </owl:DatatypeProperty>



    <!-- https://w3id.org/italia/onto/OP21/importoContributoTrimestrale -->

    <owl:DatatypeProperty rdf:about="https://w3id.org/italia/onto/OP21/importoContributoTrimestrale">
        <rdf:type rdf:resource="http://www.w3.org/2002/07/owl#FunctionalProperty"/>
        <rdfs:domain rdf:resource="https://w3id.org/italia/onto/OP21/ContributoTrimestraleOrdinario"/>
        <rdfs:range rdf:resource="http://www.w3.org/2001/XMLSchema#decimal"/>
        <rdfs:comment xml:lang="en">It is the cash amount relating to the Ordinary Quarterly Contribution.</rdfs:comment>
        <rdfs:comment xml:lang="it">È l&apos;importo in denaro relativo al Contributo Trimestrale Ordinario.</rdfs:comment>
        <rdfs:label xml:lang="it">importo contributo trimestrale</rdfs:label>
        <rdfs:label xml:lang="en">quarterly contribution amount</rdfs:label>
    </owl:DatatypeProperty>



    <!-- https://w3id.org/italia/onto/OP21/importoMovimento -->

    <owl:DatatypeProperty rdf:about="https://w3id.org/italia/onto/OP21/importoMovimento">
        <rdf:type rdf:resource="http://www.w3.org/2002/07/owl#FunctionalProperty"/>
        <rdfs:domain rdf:resource="https://w3id.org/italia/onto/OP21/MovimentoDiDenaro"/>
        <rdfs:range rdf:resource="http://www.w3.org/2001/XMLSchema#decimal"/>
        <rdfs:comment xml:lang="it">Importo di un movimento di denaro.</rdfs:comment>
        <rdfs:comment xml:lang="en">It is the money amount of a movement.</rdfs:comment>
        <rdfs:label xml:lang="it">importo movimento</rdfs:label>
        <rdfs:label xml:lang="en">movement amount</rdfs:label>
    </owl:DatatypeProperty>



    <!-- https://w3id.org/italia/onto/OP21/importoOnereContributivo -->

    <owl:DatatypeProperty rdf:about="https://w3id.org/italia/onto/OP21/importoOnereContributivo">
        <rdf:type rdf:resource="http://www.w3.org/2002/07/owl#FunctionalProperty"/>
        <rdfs:domain rdf:resource="https://w3id.org/italia/onto/OP21/OnereContributivo"/>
        <rdfs:range rdf:resource="http://www.w3.org/2001/XMLSchema#decimal"/>
        <rdfs:comment xml:lang="en">It is the cash amount relating to the Contribution Charge.</rdfs:comment>
        <rdfs:comment xml:lang="it">È l&apos;importo in denaro relativo all&apos;Onere Contributivo.</rdfs:comment>
        <rdfs:label xml:lang="en">contribution charge amount</rdfs:label>
        <rdfs:label xml:lang="it">importo onere contributivo</rdfs:label>
    </owl:DatatypeProperty>



    <!-- https://w3id.org/italia/onto/OP21/importoPagamento -->

    <owl:DatatypeProperty rdf:about="https://w3id.org/italia/onto/OP21/importoPagamento">
        <rdf:type rdf:resource="http://www.w3.org/2002/07/owl#FunctionalProperty"/>
        <rdfs:domain rdf:resource="https://w3id.org/italia/onto/OP21/Pagamento"/>
        <rdfs:range rdf:resource="http://www.w3.org/2001/XMLSchema#decimal"/>
        <rdfs:comment xml:lang="en">It is the cash amount related to the Payment.</rdfs:comment>
        <rdfs:comment xml:lang="it">È l&apos;importo in denaro relativo al Pagamento.</rdfs:comment>
        <rdfs:label xml:lang="en">amount paid</rdfs:label>
        <rdfs:label xml:lang="it">importo pagamento</rdfs:label>
    </owl:DatatypeProperty>



    <!-- https://w3id.org/italia/onto/OP21/importoPrenotato -->

    <owl:DatatypeProperty rdf:about="https://w3id.org/italia/onto/OP21/importoPrenotato">
        <rdf:type rdf:resource="http://www.w3.org/2002/07/owl#FunctionalProperty"/>
        <rdfs:domain rdf:resource="https://w3id.org/italia/onto/OP21/PrenotazioneDiPagamento"/>
        <rdfs:range rdf:resource="http://www.w3.org/2001/XMLSchema#decimal"/>
        <rdfs:comment xml:lang="en">It is the cash amount relating to the Payment Reservation.</rdfs:comment>
        <rdfs:comment xml:lang="it">È l&apos;importo in denaro relativo alla Prenotazione Di Pagamento.</rdfs:comment>
        <rdfs:label xml:lang="en">booked amount</rdfs:label>
        <rdfs:label xml:lang="it">importo prenotato</rdfs:label>
    </owl:DatatypeProperty>



    <!-- https://w3id.org/italia/onto/OP21/importoRata -->

    <owl:DatatypeProperty rdf:about="https://w3id.org/italia/onto/OP21/importoRata">
        <rdf:type rdf:resource="http://www.w3.org/2002/07/owl#FunctionalProperty"/>
        <rdfs:domain rdf:resource="https://w3id.org/italia/onto/OP21/PianoDiAmmortamento"/>
        <rdfs:range rdf:resource="http://www.w3.org/2001/XMLSchema#decimal"/>
        <rdfs:comment xml:lang="en">It is the cash amount of the installment in the Amortization Plan of an SDD Mandate.</rdfs:comment>
        <rdfs:comment xml:lang="it">È l&apos;importo in denaro della rata nel Piano Di Ammortamento di un Mandato SDD.</rdfs:comment>
        <rdfs:label xml:lang="it">importo rata</rdfs:label>
        <rdfs:label xml:lang="en">installment amount</rdfs:label>
    </owl:DatatypeProperty>



    <!-- https://w3id.org/italia/onto/OP21/importoVersamentoOrganizzazione -->

    <owl:DatatypeProperty rdf:about="https://w3id.org/italia/onto/OP21/importoVersamentoOrganizzazione">
        <rdf:type rdf:resource="http://www.w3.org/2002/07/owl#FunctionalProperty"/>
        <rdfs:domain rdf:resource="https://w3id.org/italia/onto/OP21/ContributoTrimestraleModificato"/>
        <rdfs:range rdf:resource="http://www.w3.org/2001/XMLSchema#decimal"/>
        <rdfs:comment xml:lang="en">It is the organization&apos;s cash amount in an Amended Quarterly Contribution.</rdfs:comment>
        <rdfs:comment xml:lang="it">È l&apos;importo in denaro dell&apos;organizzazione in un Contributo Trimestrale Modificato.</rdfs:comment>
        <rdfs:label xml:lang="it">importo versamento organizzazione</rdfs:label>
        <rdfs:label xml:lang="en">organization payment amount</rdfs:label>
    </owl:DatatypeProperty>



    <!-- https://w3id.org/italia/onto/OP21/indiceMese -->

    <owl:DatatypeProperty rdf:about="https://w3id.org/italia/onto/OP21/indiceMese">
        <rdf:type rdf:resource="http://www.w3.org/2002/07/owl#FunctionalProperty"/>
        <rdfs:domain rdf:resource="https://w3id.org/italia/onto/OP21/MeseDiTrimestre"/>
        <rdfs:range rdf:resource="http://www.w3.org/2001/XMLSchema#integer"/>
        <rdfs:comment xml:lang="en">It is the Month Of Quarter index (1, 2 or 3).</rdfs:comment>
        <rdfs:comment xml:lang="it">È l&apos;indice del Mese Di Trimestre (1, 2 o 3).</rdfs:comment>
        <rdfs:label xml:lang="it">indice mese</rdfs:label>
        <rdfs:label xml:lang="en">monthly index</rdfs:label>
    </owl:DatatypeProperty>



    <!-- https://w3id.org/italia/onto/OP21/indiceSettimana -->

    <owl:DatatypeProperty rdf:about="https://w3id.org/italia/onto/OP21/indiceSettimana">
        <rdf:type rdf:resource="http://www.w3.org/2002/07/owl#FunctionalProperty"/>
        <rdfs:domain rdf:resource="https://w3id.org/italia/onto/OP21/SettimanaDelMese"/>
        <rdfs:range rdf:resource="http://www.w3.org/2001/XMLSchema#integer"/>
        <rdfs:comment xml:lang="en">It is the Week Of The Month index (1, 2, 3, 4 or 5).</rdfs:comment>
        <rdfs:comment xml:lang="it">È l&apos;indice della Settimana Del Mese (1, 2, 3, 4 o 5).</rdfs:comment>
        <rdfs:label xml:lang="it">indice settimana</rdfs:label>
        <rdfs:label xml:lang="en">weekly index</rdfs:label>
    </owl:DatatypeProperty>



    <!-- https://w3id.org/italia/onto/OP21/indiceTrimestre -->

    <owl:DatatypeProperty rdf:about="https://w3id.org/italia/onto/OP21/indiceTrimestre">
        <rdf:type rdf:resource="http://www.w3.org/2002/07/owl#FunctionalProperty"/>
        <rdfs:domain rdf:resource="https://w3id.org/italia/onto/OP21/TrimestreDiAnno"/>
        <rdfs:range rdf:resource="http://www.w3.org/2001/XMLSchema#integer"/>
        <rdfs:comment xml:lang="en">It is the Quarterly index (1, 2, 3 or 4).</rdfs:comment>
        <rdfs:comment xml:lang="it">È l&apos;indice del Trimestre Di Anno (1, 2, 3 o 4).</rdfs:comment>
        <rdfs:label xml:lang="it">indice trimestre</rdfs:label>
        <rdfs:label xml:lang="en">quarterly index</rdfs:label>
    </owl:DatatypeProperty>



    <!-- https://w3id.org/italia/onto/OP21/modalitàPOSVirtuale -->

    <owl:DatatypeProperty rdf:about="https://w3id.org/italia/onto/OP21/modalitàPOSVirtuale">
        <rdf:type rdf:resource="http://www.w3.org/2002/07/owl#FunctionalProperty"/>
        <rdfs:domain rdf:resource="https://w3id.org/italia/onto/OP21/POSVirtuale"/>
        <rdfs:range rdf:resource="http://www.w3.org/2001/XMLSchema#string"/>
        <rdfs:comment xml:lang="it">Nome assegnato al Sistema di Pagamento Elettronico, in questo caso POS virtuale.</rdfs:comment>
        <rdfs:comment xml:lang="en">virtual POS mode</rdfs:comment>
        <rdfs:label xml:lang="it">modalità POS virtuale</rdfs:label>
        <rdfs:label xml:lang="en">virtual POS mode</rdfs:label>
    </owl:DatatypeProperty>



    <!-- https://w3id.org/italia/onto/OP21/modalitàRetiAmiche -->

    <owl:DatatypeProperty rdf:about="https://w3id.org/italia/onto/OP21/modalitàRetiAmiche">
        <rdf:type rdf:resource="http://www.w3.org/2002/07/owl#FunctionalProperty"/>
        <rdfs:domain rdf:resource="https://w3id.org/italia/onto/OP21/RetiAmiche"/>
        <rdfs:range rdf:resource="http://www.w3.org/2001/XMLSchema#string"/>
        <rdfs:comment xml:lang="it">Nome assegnato al Sistema di Pagamento Elettronico, in questo caso Reti Amiche.</rdfs:comment>
        <rdfs:comment xml:lang="en">Reti Amiche mode</rdfs:comment>
        <rdfs:label xml:lang="en">Reti Amiche mode</rdfs:label>
        <rdfs:label xml:lang="it">modalità Reti Amiche</rdfs:label>
    </owl:DatatypeProperty>



    <!-- https://w3id.org/italia/onto/OP21/numeroAtto -->

    <owl:DatatypeProperty rdf:about="https://w3id.org/italia/onto/OP21/numeroAtto">
        <rdf:type rdf:resource="http://www.w3.org/2002/07/owl#FunctionalProperty"/>
        <rdfs:domain rdf:resource="https://w3id.org/italia/onto/OP21/AttoAdeguamentoContributivo"/>
        <rdfs:range rdf:resource="http://www.w3.org/2001/XMLSchema#integer"/>
        <rdfs:comment xml:lang="en">It is the identification  code number of to the Tax Adjustment Act.</rdfs:comment>
        <rdfs:comment xml:lang="it">È il numero relativo all&apos;Atto Adeguamento Contributivo.</rdfs:comment>
        <rdfs:label xml:lang="en">deed identification code number</rdfs:label>
        <rdfs:label xml:lang="it">numero atto</rdfs:label>
    </owl:DatatypeProperty>



    <!-- https://w3id.org/italia/onto/OP21/numeroContoDiAddebito -->

    <owl:DatatypeProperty rdf:about="https://w3id.org/italia/onto/OP21/numeroContoDiAddebito">
        <rdf:type rdf:resource="http://www.w3.org/2002/07/owl#FunctionalProperty"/>
        <rdfs:domain rdf:resource="https://w3id.org/italia/onto/OP21/MandatoSDDRichiesto"/>
        <rdfs:range rdf:resource="http://www.w3.org/2001/XMLSchema#string"/>
        <rdfs:comment xml:lang="en">This is the current account number (IBAN) indicated by the debtor when requesting activation of the SDD mandate in his name and which must be subjected to adequacy and ownership checks.</rdfs:comment>
        <rdfs:comment xml:lang="it">È il numero di conto corrente (IBAN) indicato dal debitore in fase di richiesta di attivazione del mandato SDD a lui intestato e che deve essere sottoposto alle verifiche di congruità e titolarità.</rdfs:comment>
        <rdfs:label xml:lang="en">debit account number</rdfs:label>
        <rdfs:label xml:lang="it">numero conto di addebito</rdfs:label>
    </owl:DatatypeProperty>



    <!-- https://w3id.org/italia/onto/OP21/numeroDomanda -->

    <owl:DatatypeProperty rdf:about="https://w3id.org/italia/onto/OP21/numeroDomanda">
        <rdf:type rdf:resource="http://www.w3.org/2002/07/owl#FunctionalProperty"/>
        <rdfs:domain rdf:resource="https://w3id.org/italia/onto/OP21/DomandaAdeguamentoContributivo"/>
        <rdfs:range rdf:resource="http://www.w3.org/2001/XMLSchema#integer"/>
        <rdfs:comment xml:lang="en">This is the identification code number of the Contribution Adjustment Application.</rdfs:comment>
        <rdfs:comment xml:lang="it">È il numero relativo alla Domanda Adeguamento Contributivo.</rdfs:comment>
        <rdfs:label xml:lang="en">application identification code number</rdfs:label>
        <rdfs:label xml:lang="it">numero domanda</rdfs:label>
    </owl:DatatypeProperty>



    <!-- https://w3id.org/italia/onto/OP21/numeroOreRetribuiteContrattuali -->

    <owl:DatatypeProperty rdf:about="https://w3id.org/italia/onto/OP21/numeroOreRetribuiteContrattuali">
        <rdf:type rdf:resource="http://www.w3.org/2002/07/owl#FunctionalProperty"/>
        <rdfs:domain rdf:resource="https://w3id.org/italia/onto/OP21/ContributoTrimestralePrecompilato"/>
        <rdfs:range rdf:resource="http://www.w3.org/2001/XMLSchema#integer"/>
        <rdfs:comment xml:lang="en">It is the number of paid contractual hours relating to the Pre-compiled Quarterly Contribution.</rdfs:comment>
        <rdfs:comment xml:lang="it">È il numero delle ore retribuite previste dal Contratto Di Lavoro per il trimestre nel relativo Contributo Trimestrale Precompilato.</rdfs:comment>
        <rdfs:label xml:lang="en">number of contractual paid hours</rdfs:label>
        <rdfs:label xml:lang="it">numero ore retribuite contrattuali</rdfs:label>
    </owl:DatatypeProperty>



    <!-- https://w3id.org/italia/onto/OP21/numeroOreRetribuiteInserito -->

    <owl:DatatypeProperty rdf:about="https://w3id.org/italia/onto/OP21/numeroOreRetribuiteInserito">
        <rdf:type rdf:resource="http://www.w3.org/2002/07/owl#FunctionalProperty"/>
        <rdfs:domain rdf:resource="https://w3id.org/italia/onto/OP21/ContributoTrimestraleModificato"/>
        <rdfs:range rdf:resource="http://www.w3.org/2001/XMLSchema#integer"/>
        <rdfs:comment xml:lang="en">It is the number of hours entered relating to the Modified Quarterly Contribution.</rdfs:comment>
        <rdfs:comment xml:lang="it">È il numero delle ore inserito relative al Contributo Trimestrale Modificato.</rdfs:comment>
        <rdfs:label xml:lang="en">number of hours paid inserted</rdfs:label>
        <rdfs:label xml:lang="it">numero ore retribuite inserito</rdfs:label>
    </owl:DatatypeProperty>



    <!-- https://w3id.org/italia/onto/OP21/numeroOreSettimanali -->

    <owl:DatatypeProperty rdf:about="https://w3id.org/italia/onto/OP21/numeroOreSettimanali">
        <rdf:type rdf:resource="http://www.w3.org/2002/07/owl#FunctionalProperty"/>
        <rdfs:domain rdf:resource="https://w3id.org/italia/onto/OP21/ContrattoDiLavoro"/>
        <rdfs:range rdf:resource="http://www.w3.org/2001/XMLSchema#integer"/>
        <rdfs:comment xml:lang="en">It is the number of weekly hours indicated in the Employment Contract.</rdfs:comment>
        <rdfs:comment xml:lang="it">È il numero delle ore settimanali indicate nel Contratto Di Lavoro.</rdfs:comment>
        <rdfs:label xml:lang="en">number of weekly hours</rdfs:label>
        <rdfs:label xml:lang="it">numero ore settimanali</rdfs:label>
    </owl:DatatypeProperty>



    <!-- https://w3id.org/italia/onto/OP21/numeroPratica -->

    <owl:DatatypeProperty rdf:about="https://w3id.org/italia/onto/OP21/numeroPratica">
        <rdf:type rdf:resource="http://www.w3.org/2002/07/owl#FunctionalProperty"/>
        <rdfs:domain rdf:resource="https://w3id.org/italia/onto/OP21/PraticaAdeguamentoContributivo"/>
        <rdfs:range rdf:resource="http://www.w3.org/2001/XMLSchema#integer"/>
        <rdfs:comment xml:lang="en">It is the identification code number of the Contribution Adjustment Practice.</rdfs:comment>
        <rdfs:comment xml:lang="it">È il numero della Pratica Adeguamento Contributivo.</rdfs:comment>
        <rdfs:label xml:lang="en">application identification code number</rdfs:label>
        <rdfs:label xml:lang="it">numero pratica</rdfs:label>
    </owl:DatatypeProperty>



    <!-- https://w3id.org/italia/onto/OP21/numeroRata -->

    <owl:DatatypeProperty rdf:about="https://w3id.org/italia/onto/OP21/numeroRata">
        <rdf:type rdf:resource="http://www.w3.org/2002/07/owl#FunctionalProperty"/>
        <rdfs:domain rdf:resource="https://w3id.org/italia/onto/OP21/RataDiOnereContributivo"/>
        <rdfs:range rdf:resource="http://www.w3.org/2001/XMLSchema#integer"/>
        <rdfs:comment xml:lang="en">It is the progressive number of the Contribution Charge Installment.</rdfs:comment>
        <rdfs:comment xml:lang="it">È il numero progressivo della Rata Di Onere Contributivo.</rdfs:comment>
        <rdfs:label xml:lang="en">installment number</rdfs:label>
        <rdfs:label xml:lang="it">numero rata</rdfs:label>
    </owl:DatatypeProperty>



    <!-- https://w3id.org/italia/onto/OP21/numeroRate -->

    <owl:DatatypeProperty rdf:about="https://w3id.org/italia/onto/OP21/numeroRate">
        <rdf:type rdf:resource="http://www.w3.org/2002/07/owl#FunctionalProperty"/>
        <rdfs:domain rdf:resource="https://w3id.org/italia/onto/OP21/PianoDiAmmortamento"/>
        <rdfs:range rdf:resource="http://www.w3.org/2001/XMLSchema#integer"/>
        <rdfs:comment xml:lang="en">It is the number of installments envisaged in the Amortization Plan.</rdfs:comment>
        <rdfs:comment xml:lang="it">È il numero di rate previsto nel Piano Di Ammortamento.</rdfs:comment>
        <rdfs:label xml:lang="en">number of installments</rdfs:label>
        <rdfs:label xml:lang="it">numero rate</rdfs:label>
    </owl:DatatypeProperty>



    <!-- https://w3id.org/italia/onto/OP21/numeroSettimaneMancatoPreavviso -->

    <owl:DatatypeProperty rdf:about="https://w3id.org/italia/onto/OP21/numeroSettimaneMancatoPreavviso">
        <rdf:type rdf:resource="http://www.w3.org/2002/07/owl#FunctionalProperty"/>
        <rdfs:domain rdf:resource="https://w3id.org/italia/onto/OP21/ContributoTrimestraleFinale"/>
        <rdfs:range rdf:resource="http://www.w3.org/2001/XMLSchema#integer"/>
        <rdfs:comment xml:lang="en">It is the number of weeks of no notice or untaken holidays with which the Domestic Work Employer has terminated the Domestic Work Relationship. They are paid in the Final Quarterly Contribution.</rdfs:comment>
        <rdfs:comment xml:lang="it">È il numero di settimane di mancato preavviso o ferie non godute con cui il Datore Di Lavoro Domestico ha cessato il Rapporto Di Lavoro Domestico. Sono corrisposte nel Contributo Trimestrale Finale.</rdfs:comment>
        <rdfs:label xml:lang="en">number of weeks for lack of notice</rdfs:label>
        <rdfs:label xml:lang="it">numero settimane mancato preavviso</rdfs:label>
    </owl:DatatypeProperty>



    <!-- https://w3id.org/italia/onto/OP21/numeroSettimanePreavviso -->

    <owl:DatatypeProperty rdf:about="https://w3id.org/italia/onto/OP21/numeroSettimanePreavviso">
        <rdf:type rdf:resource="http://www.w3.org/2002/07/owl#FunctionalProperty"/>
        <rdfs:domain rdf:resource="https://w3id.org/italia/onto/OP21/ContrattoDiLavoro"/>
        <rdfs:range rdf:resource="http://www.w3.org/2001/XMLSchema#integer"/>
        <rdfs:comment xml:lang="en">It is the number of weeks notice with which the Domestic Work Employer can terminate the Domestic Work Relationship.</rdfs:comment>
        <rdfs:comment xml:lang="it">È il numero di settimane di preavviso con il quale il Datore Di Lavoro Domestico può cessare il Rapporto Di Lavoro Domestico.</rdfs:comment>
        <rdfs:label xml:lang="en">number of weeks notice</rdfs:label>
        <rdfs:label xml:lang="it">numero settimane preavviso</rdfs:label>
    </owl:DatatypeProperty>



    <!-- https://w3id.org/italia/onto/OP21/retribuzioneOrariaEffettiva -->

    <owl:DatatypeProperty rdf:about="https://w3id.org/italia/onto/OP21/retribuzioneOrariaEffettiva">
        <rdf:type rdf:resource="http://www.w3.org/2002/07/owl#FunctionalProperty"/>
        <rdfs:domain rdf:resource="https://w3id.org/italia/onto/OP21/ContrattoDiLavoro"/>
        <rdfs:range rdf:resource="http://www.w3.org/2001/XMLSchema#decimal"/>
        <rdfs:comment xml:lang="en">It is the hourly wage stipulated in the Employment Contract. The minimum hourly wage allowed must not be lower than that established by the regulations of the current year.</rdfs:comment>
        <rdfs:comment xml:lang="it">È la retribuzione oraria stipulata nel Contratto Di Lavoro. La retribuzione oraria minima consentita non deve essere inferiore a quanto stabilito dalla normativa dell’anno in corso.</rdfs:comment>
        <rdfs:label xml:lang="en">actual hourly wage</rdfs:label>
        <rdfs:label xml:lang="it">retribuzione oraria effettiva</rdfs:label>
    </owl:DatatypeProperty>



    <!-- https://w3id.org/italia/onto/OP21/retribuzioneOrariaEffettivaInserita -->

    <owl:DatatypeProperty rdf:about="https://w3id.org/italia/onto/OP21/retribuzioneOrariaEffettivaInserita">
        <rdf:type rdf:resource="http://www.w3.org/2002/07/owl#FunctionalProperty"/>
        <rdfs:domain rdf:resource="https://w3id.org/italia/onto/OP21/ContributoTrimestraleModificato"/>
        <rdfs:range rdf:resource="http://www.w3.org/2001/XMLSchema#decimal"/>
        <rdfs:comment xml:lang="en">It is the hourly wage paid in the Modified Quarterly Contribution. The minimum hourly wage allowed must not be lower than that established by the regulations of the current year.</rdfs:comment>
        <rdfs:comment xml:lang="it">È la retribuzione oraria corrispostra nel Contributo Trimestrale Modificato. La retribuzione oraria minima consentita non deve essere inferiore a quanto stabilito dalla normativa dell’anno in corso.</rdfs:comment>
        <rdfs:label xml:lang="en">effective hourly wage entered</rdfs:label>
        <rdfs:label xml:lang="it">retribuzione oraria effettiva inserita</rdfs:label>
    </owl:DatatypeProperty>



    <!-- https://w3id.org/italia/onto/OP21/tempoRichiestaAttivazione -->

    <owl:DatatypeProperty rdf:about="https://w3id.org/italia/onto/OP21/tempoRichiestaAttivazione">
        <rdf:type rdf:resource="http://www.w3.org/2002/07/owl#FunctionalProperty"/>
        <rdfs:domain rdf:resource="https://w3id.org/italia/onto/OP21/AttoDiAttivazioneMandato"/>
        <rdfs:range rdf:resource="http://www.w3.org/2001/XMLSchema#dateTime"/>
        <rdfs:comment xml:lang="it">Indica quando è stato richiesto l&apos;Atto Di Attivazione Mandato.</rdfs:comment>
        <rdfs:comment xml:lang="en">Indicates when the Mandate Activation Deed was requested.</rdfs:comment>
        <rdfs:label xml:lang="en">activation request time</rdfs:label>
        <rdfs:label xml:lang="it">tempo richiesta attivazione</rdfs:label>
    </owl:DatatypeProperty>



    <!-- https://w3id.org/italia/onto/OP21/tempoRichiestaRevoca -->

    <owl:DatatypeProperty rdf:about="https://w3id.org/italia/onto/OP21/tempoRichiestaRevoca">
        <rdf:type rdf:resource="http://www.w3.org/2002/07/owl#FunctionalProperty"/>
        <rdfs:domain rdf:resource="https://w3id.org/italia/onto/OP21/AttoDiRevocaMandato"/>
        <rdfs:range rdf:resource="http://www.w3.org/2001/XMLSchema#dateTime"/>
        <rdfs:comment xml:lang="it">Indica quando è stato richiesto l&apos;Atto Di Revoca Mandato.</rdfs:comment>
        <rdfs:comment xml:lang="en">Indicates when the Mandate Deactivation Deed was requested.</rdfs:comment>
        <rdfs:label xml:lang="en">revocation request time</rdfs:label>
        <rdfs:label xml:lang="it">tempo richiesta revoca</rdfs:label>
    </owl:DatatypeProperty>



    <!-- https://w3id.org/italia/onto/TI/endTime -->

    <owl:DatatypeProperty rdf:about="https://w3id.org/italia/onto/TI/endTime">
        <rdfs:domain rdf:resource="https://w3id.org/italia/onto/TI/TimeInterval"/>
    </owl:DatatypeProperty>



    <!-- https://w3id.org/italia/onto/TI/startTime -->

    <owl:DatatypeProperty rdf:about="https://w3id.org/italia/onto/TI/startTime">
        <rdfs:domain rdf:resource="https://w3id.org/italia/onto/TI/TimeInterval"/>
    </owl:DatatypeProperty>



    <!-- https://w3id.org/italia/onto/l0/identifier -->

    <owl:DatatypeProperty rdf:about="https://w3id.org/italia/onto/l0/identifier"/>



    <!--
    ///////////////////////////////////////////////////////////////////////////////////////
    //
    // Classes
    //
    ///////////////////////////////////////////////////////////////////////////////////////
     -->




    <!-- https://w3id.org/italia/onto/COV/HomogeneousOrganizationalArea -->

    <owl:Class rdf:about="https://w3id.org/italia/onto/COV/HomogeneousOrganizationalArea">
        <rdfs:subClassOf>
            <owl:Restriction>
                <owl:onProperty rdf:resource="https://w3id.org/italia/onto/COV/AOOIdentifier"/>
                <owl:someValuesFrom rdf:resource="http://www.w3.org/2000/01/rdf-schema#Literal"/>
            </owl:Restriction>
        </rdfs:subClassOf>
    </owl:Class>



    <!-- https://w3id.org/italia/onto/COV/Organization -->

    <owl:Class rdf:about="https://w3id.org/italia/onto/COV/Organization">
        <owl:equivalentClass>
            <owl:Restriction>
                <owl:onProperty rdf:resource="https://w3id.org/italia/onto/COV/LegalName"/>
                <owl:someValuesFrom rdf:resource="http://www.w3.org/2000/01/rdf-schema#Literal"/>
            </owl:Restriction>
        </owl:equivalentClass>
        <owl:equivalentClass>
            <owl:Restriction>
                <owl:onProperty rdf:resource="https://w3id.org/italia/onto/COV/taxCode"/>
                <owl:someValuesFrom rdf:resource="http://www.w3.org/2000/01/rdf-schema#Literal"/>
            </owl:Restriction>
        </owl:equivalentClass>
        <rdfs:subClassOf>
            <owl:Restriction>
                <owl:onProperty rdf:resource="https://w3id.org/italia/onto/OP21/haSedeINPS"/>
                <owl:someValuesFrom rdf:resource="http://www.w3.org/2002/07/owl#Thing"/>
            </owl:Restriction>
        </rdfs:subClassOf>
        <owl:disjointWith rdf:resource="https://w3id.org/italia/onto/CPV/Person"/>
    </owl:Class>



    <!-- https://w3id.org/italia/onto/COV/PublicOrganization -->

    <owl:Class rdf:about="https://w3id.org/italia/onto/COV/PublicOrganization">
        <owl:equivalentClass>
            <owl:Restriction>
                <owl:onProperty>
                    <rdf:Description>
                        <owl:inverseOf rdf:resource="https://w3id.org/italia/onto/COV/hasOrganizzation"/>
                    </rdf:Description>
                </owl:onProperty>
                <owl:someValuesFrom rdf:resource="http://www.w3.org/2002/07/owl#Thing"/>
            </owl:Restriction>
        </owl:equivalentClass>
        <rdfs:subClassOf rdf:resource="https://w3id.org/italia/onto/COV/Organization"/>
    </owl:Class>



    <!-- https://w3id.org/italia/onto/CPV/Alive -->

    <owl:Class rdf:about="https://w3id.org/italia/onto/CPV/Alive">
        <rdfs:subClassOf rdf:resource="https://w3id.org/italia/onto/CPV/Person"/>
        <rdfs:subClassOf>
            <owl:Restriction>
                <owl:onProperty rdf:resource="https://w3id.org/italia/onto/OP21/haSedeINPS"/>
                <owl:someValuesFrom rdf:resource="http://www.w3.org/2002/07/owl#Thing"/>
            </owl:Restriction>
        </rdfs:subClassOf>
    </owl:Class>



    <!-- https://w3id.org/italia/onto/CPV/Dead -->

    <owl:Class rdf:about="https://w3id.org/italia/onto/CPV/Dead"/>



    <!-- https://w3id.org/italia/onto/CPV/Person -->

    <owl:Class rdf:about="https://w3id.org/italia/onto/CPV/Person">
        <owl:equivalentClass>
            <owl:Restriction>
                <owl:onProperty rdf:resource="https://w3id.org/italia/onto/CPV/familyName"/>
                <owl:someValuesFrom rdf:resource="http://www.w3.org/2000/01/rdf-schema#Literal"/>
            </owl:Restriction>
        </owl:equivalentClass>
        <owl:equivalentClass>
            <owl:Restriction>
                <owl:onProperty rdf:resource="https://w3id.org/italia/onto/CPV/givenName"/>
                <owl:someValuesFrom rdf:resource="http://www.w3.org/2000/01/rdf-schema#Literal"/>
            </owl:Restriction>
        </owl:equivalentClass>
        <owl:equivalentClass>
            <owl:Restriction>
                <owl:onProperty rdf:resource="https://w3id.org/italia/onto/CPV/taxCode"/>
                <owl:someValuesFrom rdf:resource="http://www.w3.org/2000/01/rdf-schema#Literal"/>
            </owl:Restriction>
        </owl:equivalentClass>
    </owl:Class>



    <!-- https://w3id.org/italia/onto/OP21/AttoAdeguamentoContributivo -->

    <owl:Class rdf:about="https://w3id.org/italia/onto/OP21/AttoAdeguamentoContributivo">
        <owl:equivalentClass>
            <owl:Restriction>
                <owl:onProperty>
                    <rdf:Description>
                        <owl:inverseOf rdf:resource="https://w3id.org/italia/onto/OP21/emetteAtto"/>
                    </rdf:Description>
                </owl:onProperty>
                <owl:someValuesFrom rdf:resource="http://www.w3.org/2002/07/owl#Thing"/>
            </owl:Restriction>
        </owl:equivalentClass>
        <owl:equivalentClass>
            <owl:Restriction>
                <owl:onProperty>
                    <rdf:Description>
                        <owl:inverseOf rdf:resource="https://w3id.org/italia/onto/OP21/haAttoAdeguamentoContributivo"/>
                    </rdf:Description>
                </owl:onProperty>
                <owl:someValuesFrom rdf:resource="http://www.w3.org/2002/07/owl#Thing"/>
            </owl:Restriction>
        </owl:equivalentClass>
        <owl:equivalentClass>
            <owl:Restriction>
                <owl:onProperty rdf:resource="https://w3id.org/italia/onto/OP21/dataAtto"/>
                <owl:someValuesFrom rdf:resource="http://www.w3.org/2000/01/rdf-schema#Literal"/>
            </owl:Restriction>
        </owl:equivalentClass>
        <owl:equivalentClass>
            <owl:Restriction>
                <owl:onProperty rdf:resource="https://w3id.org/italia/onto/OP21/numeroAtto"/>
                <owl:someValuesFrom rdf:resource="http://www.w3.org/2000/01/rdf-schema#Literal"/>
            </owl:Restriction>
        </owl:equivalentClass>
        <rdfs:comment xml:lang="en">Explicit manifestation by the INPS of the decision taken regarding a Contribution Adjustment Application. This decision, if positive, establishes the amount of the Contribution Charge to be paid and the terms of the payment. The deed is characterized by a number and a date. The deed is issued by the competent INPS office for the Applicant who submitted the application. The deed is linked to one and only one Contribution Adjustment Practice (of) Contribution Adjustment and, in particular, this practice belongs to the class Status of Notified Amount of Practice</rdfs:comment>
        <rdfs:comment xml:lang="it">Manifestazione esplicita da parte dell&apos;INPS della decisione assunta in merito ad una Domanda (di) Adeguamento Contributivo. Tale decisione, se positiva, stabilisce l&apos;importo dell&apos;Onere Contributivo da versare e i termini del versamento. L&apos;atto è caratterizzato da un numero e da una data. L&apos;emissione dell&apos;atto è a cura della Sede INPS competente per il Richiedente che ha presentato la domanda. L&apos;atto è legato ad una e una sola Pratica (di) Adeguamento Contributivo e, in particolare, tale pratica appartiene alla classe Stato Di Notificato Importo Di Pratica</rdfs:comment>
        <rdfs:label xml:lang="it">Atto Adeguamento Contributivo</rdfs:label>
        <rdfs:label xml:lang="en">Contribution Adjustment Deed</rdfs:label>
    </owl:Class>



    <!-- https://w3id.org/italia/onto/OP21/AttoDiAttivazioneMandato -->

    <owl:Class rdf:about="https://w3id.org/italia/onto/OP21/AttoDiAttivazioneMandato">
        <owl:equivalentClass>
            <owl:Restriction>
                <owl:onProperty rdf:resource="https://w3id.org/italia/onto/OP21/autorizzaMandato"/>
                <owl:someValuesFrom rdf:resource="http://www.w3.org/2002/07/owl#Thing"/>
            </owl:Restriction>
        </owl:equivalentClass>
        <owl:equivalentClass>
            <owl:Restriction>
                <owl:onProperty rdf:resource="https://w3id.org/italia/onto/OP21/stabilisceFlussoDiAddebito"/>
                <owl:someValuesFrom rdf:resource="http://www.w3.org/2002/07/owl#Thing"/>
            </owl:Restriction>
        </owl:equivalentClass>
        <owl:equivalentClass>
            <owl:Restriction>
                <owl:onProperty rdf:resource="https://w3id.org/italia/onto/OP21/tempoRichiestaAttivazione"/>
                <owl:someValuesFrom rdf:resource="http://www.w3.org/2000/01/rdf-schema#Literal"/>
            </owl:Restriction>
        </owl:equivalentClass>
        <rdfs:subClassOf>
            <owl:Class>
                <owl:intersectionOf rdf:parseType="Collection">
                    <owl:Restriction>
                        <owl:onProperty rdf:resource="https://w3id.org/italia/onto/OP21/stabilisceFlussoDiAddebito"/>
                        <owl:minCardinality rdf:datatype="http://www.w3.org/2001/XMLSchema#nonNegativeInteger">2</owl:minCardinality>
                    </owl:Restriction>
                    <owl:Restriction>
                        <owl:onProperty rdf:resource="https://w3id.org/italia/onto/OP21/stabilisceFlussoDiAddebito"/>
                        <owl:maxCardinality rdf:datatype="http://www.w3.org/2001/XMLSchema#nonNegativeInteger">2</owl:maxCardinality>
                    </owl:Restriction>
                </owl:intersectionOf>
            </owl:Class>
        </rdfs:subClassOf>
        <rdfs:comment xml:lang="en">It is the formal authorization issued by the Mandate Debtor to the Mandate Creditor so that the latter can request the Bank depositary of the debtor&apos;s account to debit this account with the amount indicated in the deed itself, according to the recurrence also indicated , starting from the month following the time (date and time) in which the deed was issued. The deed is valid until revoked or until the debt is extinguished. The deed is necessarily and obligatorily linked to two current accounts respectively in the name of the Mandate Creditor and the Mandate Debtor.</rdfs:comment>
        <rdfs:comment xml:lang="it">È l&apos;autorizzazione formale rilasciata dal Debitore Mandato al Creditore Mandato affinchè quest&apos;ultimo possa richiedere all&apos;Istituto di Credito depositario del conto del debitore, di addebitare su tale conto l&apos;importo indicato nell&apos;atto stesso, secondo la ricorrenza anch&apos;essa indicata, a partire dal mese successivo rispetto al tempo (data e ora) in cui l&apos;atto è stato emesso. L&apos;atto è valido fino a revoca ovvero all&apos;estinzione del debito. L&apos;atto è legato necessariamente e obbligatoriamente a due conti correnti intestati rispettivamente al Creditore Mandato e al Debitore Mandato.</rdfs:comment>
        <rdfs:label xml:lang="it">Atto Di Attivazione Mandato</rdfs:label>
        <rdfs:label xml:lang="en">SDD Mandate Activation Deed</rdfs:label>
    </owl:Class>



    <!-- https://w3id.org/italia/onto/OP21/AttoDiRevocaMandato -->

    <owl:Class rdf:about="https://w3id.org/italia/onto/OP21/AttoDiRevocaMandato">
        <owl:equivalentClass>
            <owl:Restriction>
                <owl:onProperty rdf:resource="https://w3id.org/italia/onto/OP21/revocaMandato"/>
                <owl:someValuesFrom rdf:resource="http://www.w3.org/2002/07/owl#Thing"/>
            </owl:Restriction>
        </owl:equivalentClass>
        <owl:equivalentClass>
            <owl:Restriction>
                <owl:onProperty rdf:resource="https://w3id.org/italia/onto/OP21/tempoRichiestaRevoca"/>
                <owl:someValuesFrom rdf:resource="http://www.w3.org/2000/01/rdf-schema#Literal"/>
            </owl:Restriction>
        </owl:equivalentClass>
        <rdfs:comment xml:lang="en">It is the revocation communication of an active SDD mandate. The automatic debit will be suspended starting from the month following the time (date and time) of the presentation of the revocation.</rdfs:comment>
        <rdfs:comment xml:lang="it">È la comunicazione di revoca di un mandato SDD attivo. L’addebito automatico sarà sospeso a partire dal mese successivo al tempo (data e ora) della presentazione della revoca.</rdfs:comment>
        <rdfs:label xml:lang="it">Atto Di Revoca Mandato</rdfs:label>
        <rdfs:label xml:lang="en">SDD Mandate Withdrawl Deed</rdfs:label>
    </owl:Class>



    <!-- https://w3id.org/italia/onto/OP21/AvvisoDiPagamento -->

    <owl:Class rdf:about="https://w3id.org/italia/onto/OP21/AvvisoDiPagamento">
        <owl:equivalentClass>
            <owl:Restriction>
                <owl:onProperty rdf:resource="https://w3id.org/italia/onto/OP21/avvisoHaEnteCreditore"/>
                <owl:someValuesFrom rdf:resource="http://www.w3.org/2002/07/owl#Thing"/>
            </owl:Restriction>
        </owl:equivalentClass>
        <owl:equivalentClass>
            <owl:Restriction>
                <owl:onProperty rdf:resource="https://w3id.org/italia/onto/OP21/IUV"/>
                <owl:someValuesFrom rdf:resource="http://www.w3.org/2000/01/rdf-schema#Literal"/>
            </owl:Restriction>
        </owl:equivalentClass>
        <owl:equivalentClass>
            <owl:Restriction>
                <owl:onProperty rdf:resource="https://w3id.org/italia/onto/OP21/codiceAvviso"/>
                <owl:someValuesFrom rdf:resource="http://www.w3.org/2000/01/rdf-schema#Literal"/>
            </owl:Restriction>
        </owl:equivalentClass>
        <owl:equivalentClass>
            <owl:Restriction>
                <owl:onProperty rdf:resource="https://w3id.org/italia/onto/OP21/dataScadenzaPagamento"/>
                <owl:someValuesFrom rdf:resource="http://www.w3.org/2000/01/rdf-schema#Literal"/>
            </owl:Restriction>
        </owl:equivalentClass>
        <owl:disjointWith rdf:resource="https://w3id.org/italia/onto/OP21/BollettinoMAV"/>
        <owl:disjointWith rdf:resource="https://w3id.org/italia/onto/OP21/SessionePagamentoElettronico"/>
        <rdfs:comment xml:lang="en">Document that contains the minimum information necessary to make a payment on the pagoPA platform. The payment advice fields are defined by AgID as follows:
- Creditor body: contains all the details of the Public Administration to which the payment is intended (Istitution Name, Tax Code, CBILL Code);
- Account holder: reports the data of the citizen/company making the payment;
- Payment information: contains the notice code made up of the three fields that indicate the beneficiary institution and the IUV (Unique Payment Identification);
- The amount;
- The deadline (which may not coincide with the due date) ;
- Details of amounts: the reason for the payment and the amount; in the particular case of the payment of contributions, the details that generated the amount of the contribution to be paid are reported in two copies;
- Service availability and payment methods; where the postal current account number to be used is referred to the address of the payment portal to make the payment online or for payment via Poste using the new white PA slip “TD123”.
- Barcode: for data acquisition through optical reading;
- QR code: for data acquisition through optical reading;
The elements contained in the notice allow payment to be made through the widest network of financial intermediaries and methods.</rdfs:comment>
        <rdfs:comment xml:lang="it">È la notifica che contiene le informazioni minime necessarie ad effettuare un pagamento sulla piattaforma pagoPA. Gli attributi dell’Avviso Di Pagamento sono stabiliti da AgID come segue:
- Ente creditore: riporta tutti gli estremi della Pubblica Amministrazione a cui è destinato il pagamento (Ragione Sociale, Codice Fiscale, Codice CBILL);
- Intestatario: riporta i dati del cittadino/impresa che effettua il pagamento;
- Informazioni di pagamento: contiene il Codice Avviso formato dai tre campi che indicano l’Ente beneficiario e dallo IUV (Identificativo Unico di Pagamento);
- Importo;
- Scadenza dell’avviso (che può non coincidere con la scadenza del dovuto);
- Causale del versamento; nel caso particolare del pagamento di contributi sono riportate, in doppia copia, i dettagli che hanno generato l&apos;importo contributivo da versare;
- Disponibilità del servizio e modalità di pagamento; dove si rinvia all’indirizzo del portale dei pagamenti per effettuare il pagamento on line oppure per il pagamento tramite Poste attraverso l’utilizzo del nuovo bollettino PA bianco “TD123” il numero di conto corrente postale da utilizzare.
- Codice a barre (per l’acquisizione dei dati attraverso lettura ottica);
- Codice QR (per l’acquisizione dei dati attraverso lettura ottica);
Gli elementi contenuti nell’avviso consentono di effettuare il pagamento attraverso la più ampia rete di modalità e intermediari finanziari.</rdfs:comment>
        <rdfs:label xml:lang="it">Avviso Di Pagamento</rdfs:label>
        <rdfs:label xml:lang="en">Payment Notice</rdfs:label>
    </owl:Class>



    <!-- https://w3id.org/italia/onto/OP21/BollettinoDiPagamento -->

    <owl:Class rdf:about="https://w3id.org/italia/onto/OP21/BollettinoDiPagamento">
        <owl:equivalentClass>
            <owl:Restriction>
                <owl:onProperty rdf:resource="https://w3id.org/italia/onto/OP21/haFinalità"/>
                <owl:someValuesFrom rdf:resource="http://www.w3.org/2002/07/owl#Thing"/>
            </owl:Restriction>
        </owl:equivalentClass>
        <owl:equivalentClass>
            <owl:Restriction>
                <owl:onProperty rdf:resource="https://w3id.org/italia/onto/OP21/haModalitàDiPagamento"/>
                <owl:someValuesFrom rdf:resource="http://www.w3.org/2002/07/owl#Thing"/>
            </owl:Restriction>
        </owl:equivalentClass>
        <rdfs:comment xml:lang="en">It is the notification of payment referring to a debt position towards an institution or a company. Depending on the Purpose to which the slip is necessarily associated, the latter indicates the reason for the payment, the amount, the expiry date and the possible payment methods. In recent times, the payment slip is increasingly embodied by the payment notice pagoPA which performs the same function as a postal payment slip or MAV but which makes payment possible using other channels besides the Italian post office.</rdfs:comment>
        <rdfs:comment xml:lang="it">È la notifica di pagamento riferita a una posizione debitoria nei confronti di un Ente o un’Azienda. In funzione della Finalità a cui il bollettino è necessariamente associato quest&apos;ultimo indica la causale del pagamento, l&apos;importo, la data di scadenza e le possibili modalità di pagamento. In tempi recenti il bollettino viene sempre più spesso incarnato dall’Avviso di Pagamento pagoPA che svolge la stessa funzione di un bollettino postale o di un MAV ma che rende possibile il pagamento utilizzando anche altri canali oltre alle Poste Italiane.</rdfs:comment>
        <rdfs:label xml:lang="it">Bollettino Di Pagamento</rdfs:label>
        <rdfs:label xml:lang="en">Payment Slip</rdfs:label>
    </owl:Class>



    <!-- https://w3id.org/italia/onto/OP21/BollettinoDiPagamentoContributo -->

    <owl:Class rdf:about="https://w3id.org/italia/onto/OP21/BollettinoDiPagamentoContributo">
        <owl:equivalentClass>
            <owl:Restriction>
                <owl:onProperty rdf:resource="https://w3id.org/italia/onto/OP21/haFinalità"/>
                <owl:someValuesFrom rdf:resource="https://w3id.org/italia/onto/OP21/ContributoTrimestraleOrdinario"/>
            </owl:Restriction>
        </owl:equivalentClass>
        <rdfs:comment xml:lang="it">Sottoclasse di Bollettino di Pagamento riferito al pagamento di un Contributo Trimestrale Ordinario derivante da un Rapporto Di Lavoro in essere o testé cessato. È caratterizzato dall&apos;anno e trimestre a cui il contributo si riferisce, il numero di ore retribuite e la retribuzione oraria effettiva applicata, tutti derivati dalla associata occorrenza di Contributo Trimestrale Ordinario nel suo ruolo di Finalità.</rdfs:comment>
        <rdfs:comment xml:lang="en">Sub-class of Payment slip referring to the payment of an Ordinary Quarterly Contribution deriving from an existing or recently terminated Employment Relationship. It is characterized by the year and quarter to which the contribution refers, the number of hours paid and the effective hourly wage applied, all derived from the associated occurrence of the Ordinary Quarterly Contribution in its role of Purpose.</rdfs:comment>
        <rdfs:label xml:lang="it">Bollettino Di Pagamento Contributo</rdfs:label>
        <rdfs:label xml:lang="en">Tax Payment Slipt</rdfs:label>
    </owl:Class>



    <!-- https://w3id.org/italia/onto/OP21/BollettinoDiPagamentoRata -->

    <owl:Class rdf:about="https://w3id.org/italia/onto/OP21/BollettinoDiPagamentoRata">
        <owl:equivalentClass>
            <owl:Restriction>
                <owl:onProperty rdf:resource="https://w3id.org/italia/onto/OP21/haFinalità"/>
                <owl:someValuesFrom rdf:resource="https://w3id.org/italia/onto/OP21/RataDiOnereContributivo"/>
            </owl:Restriction>
        </owl:equivalentClass>
        <rdfs:subClassOf>
            <owl:Restriction>
                <owl:onProperty rdf:resource="https://w3id.org/italia/onto/OP21/codiceINPS"/>
                <owl:someValuesFrom rdf:resource="http://www.w3.org/2000/01/rdf-schema#Literal"/>
            </owl:Restriction>
        </rdfs:subClassOf>
        <owl:disjointWith rdf:resource="https://w3id.org/italia/onto/OP21/BollettinoDiPagamentoUnico"/>
        <rdfs:comment xml:lang="it">Sottoclasse di Bollettino di Pagamento riferito al pagamento di una Rata di Onere Contributivo facente parte di un Piano di Ammortamento derivante da una pratica di riscatto, ricongiunzione, rendita. È caratterizzato dalla presenza del codice INPS che codifica il numero di pratica e la sede INPS che la gestisce e dall&apos;indice della rata a cui il bollettino si riferisce, derivata dalla associata occorrenza di Rata Di Onere Contributivo nel suo ruolo di Finalità.</rdfs:comment>
        <rdfs:comment xml:lang="en">Sub-class of Payment Slip referring to the payment of a Tax Contribution Installment forming part of an Amortization Plan deriving from a redemption, reunion, or income procedure. It is characterized by the presence of the INPS code which encodes the application number and the INPS office which manages it and by the index of the installment to which the bulletin refers, derived from the associated occurrence of the Contribution Charge Installment in its role of Purpose.</rdfs:comment>
        <rdfs:label xml:lang="it">Bollettino Di Pagamento Rata</rdfs:label>
        <rdfs:label xml:lang="en">Installment Payment Slip</rdfs:label>
    </owl:Class>



    <!-- https://w3id.org/italia/onto/OP21/BollettinoDiPagamentoUnico -->

    <owl:Class rdf:about="https://w3id.org/italia/onto/OP21/BollettinoDiPagamentoUnico">
        <owl:equivalentClass>
            <owl:Restriction>
                <owl:onProperty rdf:resource="https://w3id.org/italia/onto/OP21/haFinalità"/>
                <owl:someValuesFrom rdf:resource="https://w3id.org/italia/onto/OP21/OnereContributivo"/>
            </owl:Restriction>
        </owl:equivalentClass>
        <rdfs:subClassOf>
            <owl:Restriction>
                <owl:onProperty rdf:resource="https://w3id.org/italia/onto/OP21/codiceINPS"/>
                <owl:someValuesFrom rdf:resource="http://www.w3.org/2000/01/rdf-schema#Literal"/>
            </owl:Restriction>
        </rdfs:subClassOf>
        <rdfs:comment xml:lang="it">Sottoclasse di Bollettino di Pagamento riferito al pagamento di un Onere Contributivo, derivante da una pratica di riscatto, ricongiunzione, rendita, in un&apos;unica soluzione (pagamento a saldo). È caratterizzato dalla presenza del codice INPS che codifica il numero di pratica e la sede INPS che la gestisce.</rdfs:comment>
        <rdfs:comment xml:lang="en">Sub-class of Payment Slip referring to the payment of a Contribution Charge, deriving from a practice of redemption, reunion, or income, in a single solution (payment of the balance). It is characterized by the presence of the INPS code which encodes the case number and the INPS office which manages it.</rdfs:comment>
        <rdfs:label xml:lang="it">Bollettino Di Pagamento Unico</rdfs:label>
        <rdfs:label xml:lang="en">Single Payment Slip</rdfs:label>
    </owl:Class>



    <!-- https://w3id.org/italia/onto/OP21/BollettinoMAV -->

    <owl:Class rdf:about="https://w3id.org/italia/onto/OP21/BollettinoMAV">
        <owl:equivalentClass>
            <owl:Restriction>
                <owl:onProperty rdf:resource="https://w3id.org/italia/onto/OP21/codiceMAV"/>
                <owl:someValuesFrom rdf:resource="http://www.w3.org/2000/01/rdf-schema#Literal"/>
            </owl:Restriction>
        </owl:equivalentClass>
        <rdfs:comment xml:lang="it">Il bollettino MAV (Pagamento Mediante Avviso) è un bollettino il cui pagamento segue una procedura interbancaria standard e che contiene le informazioni necessarie alla banca del creditore e al creditore stesso per la riconciliazione del pagamento.</rdfs:comment>
        <rdfs:comment xml:lang="en">The MAV slip (Payment by Notice) is a slip whose payment follows a standard interbank procedure and which contains the information necessary for the creditor&apos;s bank and the creditor himself to reconcile the payment.</rdfs:comment>
        <rdfs:label xml:lang="it">Bollettino MAV</rdfs:label>
        <rdfs:label xml:lang="en">MAV Payment Slip</rdfs:label>
    </owl:Class>



    <!-- https://w3id.org/italia/onto/OP21/ContoCorrente -->

    <owl:Class rdf:about="https://w3id.org/italia/onto/OP21/ContoCorrente">
        <owl:equivalentClass>
            <owl:Restriction>
                <owl:onProperty rdf:resource="https://w3id.org/italia/onto/OP21/haIstitutoDiCredito"/>
                <owl:someValuesFrom rdf:resource="http://www.w3.org/2002/07/owl#Thing"/>
            </owl:Restriction>
        </owl:equivalentClass>
        <owl:equivalentClass>
            <owl:Restriction>
                <owl:onProperty>
                    <rdf:Description>
                        <owl:inverseOf rdf:resource="https://w3id.org/italia/onto/OP21/haContoCorrente"/>
                    </rdf:Description>
                </owl:onProperty>
                <owl:someValuesFrom rdf:resource="http://www.w3.org/2002/07/owl#Thing"/>
            </owl:Restriction>
        </owl:equivalentClass>
        <owl:equivalentClass>
            <owl:Restriction>
                <owl:onProperty rdf:resource="https://w3id.org/italia/onto/OP21/IBAN"/>
                <owl:someValuesFrom rdf:resource="http://www.w3.org/2000/01/rdf-schema#Literal"/>
            </owl:Restriction>
        </owl:equivalentClass>
        <rdfs:comment xml:lang="en">A Bank Account is a financial account maintained by a bank or other financial institution in which the financial transactions between the bank and a customer, the Account Holder, are recorded. Each financial institution sets the terms and conditions for each type of account it offers, which are classified in commonly understood types, such as deposit accounts, credit card accounts, current accounts, loan accounts or many other types of account. An Account Holder may have more than one account. Once an account is opened, funds entrusted by the Account Holder to the financial institution on deposit are recorded in the account designated by the customer. Funds can be withdrawn from loan loaders.</rdfs:comment>
        <rdfs:comment xml:lang="it">Un conto corrente è un conto finanziario gestito da una banca o altro istituto finanziario in cui sono registrate le transazioni finanziarie tra la banca e un cliente, il titolare del conto. Ogni istituto finanziario stabilisce i termini e le condizioni per ogni tipo di conto che offre, che sono classificati in tipologie comunemente intese, come conti di deposito, conti di carte di credito, conti correnti, conti di prestito o altri tipi di conto. Un titolare di conto può avere più di un conto. Una volta aperto un conto, i fondi affidati in deposito dal titolare del conto all&apos;istituto finanziario vengono registrati sul conto designato dal cliente.</rdfs:comment>
        <rdfs:label xml:lang="en">Bank Account</rdfs:label>
        <rdfs:label xml:lang="it">Conto Corrente</rdfs:label>
    </owl:Class>



    <!-- https://w3id.org/italia/onto/OP21/ContrattoDiLavoro -->

    <owl:Class rdf:about="https://w3id.org/italia/onto/OP21/ContrattoDiLavoro">
        <owl:equivalentClass>
            <owl:Restriction>
                <owl:onProperty>
                    <rdf:Description>
                        <owl:inverseOf rdf:resource="https://w3id.org/italia/onto/OP21/èOriginatoDa"/>
                    </rdf:Description>
                </owl:onProperty>
                <owl:someValuesFrom rdf:resource="http://www.w3.org/2002/07/owl#Thing"/>
            </owl:Restriction>
        </owl:equivalentClass>
        <owl:equivalentClass>
            <owl:Restriction>
                <owl:onProperty rdf:resource="https://w3id.org/italia/onto/OP21/codiceContrattoDiLavoro"/>
                <owl:someValuesFrom rdf:resource="http://www.w3.org/2000/01/rdf-schema#Literal"/>
            </owl:Restriction>
        </owl:equivalentClass>
        <owl:equivalentClass>
            <owl:Restriction>
                <owl:onProperty rdf:resource="https://w3id.org/italia/onto/OP21/numeroOreSettimanali"/>
                <owl:someValuesFrom rdf:resource="http://www.w3.org/2000/01/rdf-schema#Literal"/>
            </owl:Restriction>
        </owl:equivalentClass>
        <owl:equivalentClass>
            <owl:Restriction>
                <owl:onProperty rdf:resource="https://w3id.org/italia/onto/OP21/retribuzioneOrariaEffettiva"/>
                <owl:someValuesFrom rdf:resource="http://www.w3.org/2000/01/rdf-schema#Literal"/>
            </owl:Restriction>
        </owl:equivalentClass>
        <rdfs:comment xml:lang="en">An employment contract is an agreement that covers the working relationship between a company and an employee. It allows both parties to clearly understand their obligations and the terms of employment. More specifically, an employment contract can include salary or wages, schedule, duration of employment, general responsibilities, confidentiality, communications, benefits, and future competition.</rdfs:comment>
        <rdfs:comment xml:lang="it">Un contratto di lavoro, o lettera di assunzione, è un accordo che da origine ad un rapporto di lavoro tra un datore di lavoro e un lavoratore. Consente a entrambe le parti di comprendere chiaramente i propri obblighi e le condizioni di lavoro. Nel contesto del dominio, definisce i termini del rapporto stesso indicando: la quantità e distribuzione delle ore settimanali lavorate, la loro retribuzione effettiva, le ferie, il TFR, i termini di preavviso e quanto altro risulta necessario per la definizione del rapporto stesso e nel rispetto del Contratto Collettivo, se esistente, del settore di riferimento.</rdfs:comment>
        <rdfs:label xml:lang="it">Contratto Di Lavoro</rdfs:label>
        <rdfs:label xml:lang="en">Work Contract</rdfs:label>
    </owl:Class>



    <!-- https://w3id.org/italia/onto/OP21/ContributoTrimestraleFinale -->

    <owl:Class rdf:about="https://w3id.org/italia/onto/OP21/ContributoTrimestraleFinale">
        <owl:equivalentClass>
            <owl:Restriction>
                <owl:onProperty>
                    <rdf:Description>
                        <owl:inverseOf rdf:resource="https://w3id.org/italia/onto/OP21/haContributoTrimestraleFinale"/>
                    </rdf:Description>
                </owl:onProperty>
                <owl:someValuesFrom rdf:resource="http://www.w3.org/2002/07/owl#Thing"/>
            </owl:Restriction>
        </owl:equivalentClass>
        <rdfs:subClassOf rdf:resource="https://w3id.org/italia/onto/OP21/ContributoTrimestraleOrdinario"/>
        <rdfs:comment xml:lang="it">Sottoclasse di Contributo Trimestrale Ordinario legato ad un Rapporto Di Lavoro Domestico Cessato che indica la competenza per l&apos;ultimo trimestre di lavoro. In questo caso i contributi devono riguardare anche le eventuali ore relative alle settimane di mancato preavviso o ferie non godute che verranno attribuite a settimane successive alla data di cessazione con possibile esubero nel trimestre successivo. A tal fine è indicato il numero di settimane di preavviso.</rdfs:comment>
        <rdfs:comment xml:lang="en">Sub-class of Ordinary Quarterly Contribution linked to a Ceased Domestic Work Report indicating the competence for the last quarter of work. In this case the contributions must also relate to any hours relating to weeks of missed notice or untaken holidays which will be attributed to weeks following the date of termination with possible redundancy in the following quarter. For this purpose, the number of weeks notice is indicated.</rdfs:comment>
        <rdfs:label xml:lang="it">Contributo Trimestrale Finale</rdfs:label>
        <rdfs:label xml:lang="en">Final Quarterly Contribution</rdfs:label>
    </owl:Class>



    <!-- https://w3id.org/italia/onto/OP21/ContributoTrimestraleModificato -->

    <owl:Class rdf:about="https://w3id.org/italia/onto/OP21/ContributoTrimestraleModificato">
        <owl:equivalentClass>
            <owl:Restriction>
                <owl:onProperty rdf:resource="https://w3id.org/italia/onto/OP21/haSettimanaDelTrimestre"/>
                <owl:someValuesFrom rdf:resource="http://www.w3.org/2002/07/owl#Thing"/>
            </owl:Restriction>
        </owl:equivalentClass>
        <owl:equivalentClass>
            <owl:Restriction>
                <owl:onProperty rdf:resource="https://w3id.org/italia/onto/OP21/numeroOreRetribuiteInserito"/>
                <owl:someValuesFrom rdf:resource="http://www.w3.org/2000/01/rdf-schema#Literal"/>
            </owl:Restriction>
        </owl:equivalentClass>
        <owl:equivalentClass>
            <owl:Restriction>
                <owl:onProperty rdf:resource="https://w3id.org/italia/onto/OP21/retribuzioneOrariaEffettivaInserita"/>
                <owl:someValuesFrom rdf:resource="http://www.w3.org/2000/01/rdf-schema#Literal"/>
            </owl:Restriction>
        </owl:equivalentClass>
        <owl:disjointWith rdf:resource="https://w3id.org/italia/onto/OP21/ContributoTrimestralePrecompilato"/>
        <rdfs:comment xml:lang="it">Sottoclasse di Contributo Trimestrale Ordinario che indica gli elementi utili al calcolo dell&apos;importo dei contributi personalizzati per lo specifico trimestre dell&apos;anno. In particolare, specifica il numero di ore retribuite del trimestre, la retribuzione oraria del trimestre, le settimane di presenza per ciascun mese del trimestre, mediante il legame con la Settimana Del Mese, importo e destinatario del contributo versato ad una Organizzazione Di Assistenza. </rdfs:comment>
        <rdfs:comment xml:lang="en">Sub-class of Ordinary Quarterly Contribution which indicates the elements useful for calculating the amount of personalized contributions for the specific quarter of the year. In particular, it specifies the number of hours paid for the quarter, the hourly salary for the quarter, the weeks of presence for each month of the quarter, by linking it with the Week Of The Month, amount and recipient of the contribution paid to a Support Organization.</rdfs:comment>
        <rdfs:label xml:lang="it">Contributo Trimestrale Modificato</rdfs:label>
        <rdfs:label xml:lang="en">Modified Quarterly Contribution</rdfs:label>
    </owl:Class>



    <!-- https://w3id.org/italia/onto/OP21/ContributoTrimestraleOrdinario -->

    <owl:Class rdf:about="https://w3id.org/italia/onto/OP21/ContributoTrimestraleOrdinario">
        <owl:equivalentClass>
            <owl:Class>
                <owl:unionOf rdf:parseType="Collection">
                    <rdf:Description rdf:about="https://w3id.org/italia/onto/OP21/ContributoTrimestraleModificato"/>
                    <rdf:Description rdf:about="https://w3id.org/italia/onto/OP21/ContributoTrimestralePrecompilato"/>
                </owl:unionOf>
            </owl:Class>
        </owl:equivalentClass>
        <owl:equivalentClass>
            <owl:Restriction>
                <owl:onProperty rdf:resource="https://w3id.org/italia/onto/OP21/haTrimestreDiAnno"/>
                <owl:someValuesFrom rdf:resource="http://www.w3.org/2002/07/owl#Thing"/>
            </owl:Restriction>
        </owl:equivalentClass>
        <owl:equivalentClass>
            <owl:Restriction>
                <owl:onProperty>
                    <rdf:Description>
                        <owl:inverseOf rdf:resource="https://w3id.org/italia/onto/OP21/haContributoTrimestraleOrdinario"/>
                    </rdf:Description>
                </owl:onProperty>
                <owl:someValuesFrom rdf:resource="http://www.w3.org/2002/07/owl#Thing"/>
            </owl:Restriction>
        </owl:equivalentClass>
        <owl:equivalentClass>
            <owl:Restriction>
                <owl:onProperty rdf:resource="https://w3id.org/italia/onto/OP21/annoContributoTrimestrale"/>
                <owl:someValuesFrom rdf:resource="http://www.w3.org/2000/01/rdf-schema#Literal"/>
            </owl:Restriction>
        </owl:equivalentClass>
        <owl:equivalentClass>
            <owl:Restriction>
                <owl:onProperty rdf:resource="https://w3id.org/italia/onto/OP21/dataScadenzaContributoTrimestrale"/>
                <owl:someValuesFrom rdf:resource="http://www.w3.org/2000/01/rdf-schema#Literal"/>
            </owl:Restriction>
        </owl:equivalentClass>
        <owl:equivalentClass>
            <owl:Restriction>
                <owl:onProperty rdf:resource="https://w3id.org/italia/onto/OP21/importoContributoTrimestrale"/>
                <owl:someValuesFrom rdf:resource="http://www.w3.org/2000/01/rdf-schema#Literal"/>
            </owl:Restriction>
        </owl:equivalentClass>
        <rdfs:comment xml:lang="it">Classifica le competenze trimestrali dei contributi che il datore di lavoro deve versare in base alle ore lavorate nel trimestre e della retribuzione oraria effettiva. È caratterizzato dall&apos;anno e dal trimestre a cui la competenza si riferisce, dall&apos;importo e dalla data di scadenza del versamento.</rdfs:comment>
        <rdfs:comment xml:lang="en">Classifies the quarterly fees of the contributions that the employer must pay based on the hours worked in the quarter and the actual hourly wage. It is characterized by the year and quarter to which the accrual refers, by the amount and due date of the payment.</rdfs:comment>
        <rdfs:label xml:lang="it">Contributo Trimestrale Ordinario</rdfs:label>
        <rdfs:label xml:lang="en">Regular Quarterly Contribution</rdfs:label>
    </owl:Class>



    <!-- https://w3id.org/italia/onto/OP21/ContributoTrimestralePrecompilato -->

    <owl:Class rdf:about="https://w3id.org/italia/onto/OP21/ContributoTrimestralePrecompilato">
        <owl:equivalentClass>
            <owl:Restriction>
                <owl:onProperty rdf:resource="https://w3id.org/italia/onto/OP21/numeroOreRetribuiteContrattuali"/>
                <owl:someValuesFrom rdf:resource="http://www.w3.org/2000/01/rdf-schema#Literal"/>
            </owl:Restriction>
        </owl:equivalentClass>
        <rdfs:comment xml:lang="it">Sottoclasse di Contributo Trimestrale Ordinario che indica gli elementi utili al calcolo dell&apos;importo dei contributi per uno specifico trimestre dell&apos;anno derivati dal Contratto Di Lavoro depositato. In particolare, specifica il numero di ore retribuite contrattuali effettive di competenza del trimestre che possono variare da trimestre a trimestre.</rdfs:comment>
        <rdfs:comment xml:lang="en">Sub-class of Ordinary Quarterly Contribution which indicates the elements useful for calculating the amount of contributions for a specific quarter of the year deriving from the Employment Contract filed. In particular, it specifies the number of actual contractual paid hours pertaining to the quarter which may vary from quarter to quarter.</rdfs:comment>
        <rdfs:label xml:lang="it">Contributo Trimestrale Precompilato</rdfs:label>
        <rdfs:label xml:lang="en">Pre-compiled Quarterly Contribution</rdfs:label>
    </owl:Class>



    <!-- https://w3id.org/italia/onto/OP21/Correntista -->

    <owl:Class rdf:about="https://w3id.org/italia/onto/OP21/Correntista">
        <owl:equivalentClass>
            <owl:Restriction>
                <owl:onProperty rdf:resource="https://w3id.org/italia/onto/OP21/haContoCorrente"/>
                <owl:someValuesFrom rdf:resource="http://www.w3.org/2002/07/owl#Thing"/>
            </owl:Restriction>
        </owl:equivalentClass>
        <owl:equivalentClass>
            <owl:Restriction>
                <owl:onProperty rdf:resource="https://w3id.org/italia/onto/OP21/identificatoreCorrentista"/>
                <owl:someValuesFrom rdf:resource="http://www.w3.org/2000/01/rdf-schema#Literal"/>
            </owl:Restriction>
        </owl:equivalentClass>
        <owl:disjointWith rdf:resource="https://w3id.org/italia/onto/OP21/DatoreDiLavoroDomestico"/>
        <rdfs:comment xml:lang="en">An Account Holder is the person listed or identified as the holder of a Bank Account. A person, other than a Financial Institution, holding a Bank Account for the benefit of another person as an agent, a custodian, a nominee, a signatory, an investment advisor, an intermediary, or as a legal guardian, is not treated as the Account Holder. In these circumstances that other person is the Account Holder. For example in the case of a parent/child relationship where the parent is acting as a legal guardian, the child is regarded as the Account Holder. With respect to a jointly held account, each joint holder is treated as an Account Holder.</rdfs:comment>
        <rdfs:comment xml:lang="it">Sottoclasse di Ruolo di Agente che classifica i titolari di un conto bancario. Una persona, diversa da un istituto finanziario, titolare di un conto bancario a beneficio di un&apos;altra persona in qualità di agente, custode, intestatario, firmatario, consulente per gli investimenti, intermediario o tutore legale, non è trattata come titolare del conto. In queste circostanze, l&apos;altra persona è titolare del conto. Ad esempio, nel caso di un rapporto genitore/figlio in cui il genitore agisce in qualità di tutore legale, il figlio è considerato il titolare del conto. Per quanto riguarda un conto cointestato, ogni cointestatario è trattato come un titolare del conto, rappresentando ciascuno una istanza della classe. Ciascuna istanza possiede un identificatore.</rdfs:comment>
        <rdfs:label xml:lang="en">Account Holder</rdfs:label>
        <rdfs:label xml:lang="it">Correntista</rdfs:label>
    </owl:Class>



    <!-- https://w3id.org/italia/onto/OP21/CreditoreMandato -->

    <owl:Class rdf:about="https://w3id.org/italia/onto/OP21/CreditoreMandato">
        <rdfs:comment xml:lang="it">Sottoclasse di Correntista associata a Mandato SDD con il ruolo di creditore.</rdfs:comment>
        <rdfs:comment xml:lang="en">Sub-class of bank account holder associated with SDD Mandate with the role of creditor.</rdfs:comment>
        <rdfs:label xml:lang="it">Creditore Mandato</rdfs:label>
        <rdfs:label xml:lang="en">Mandate Creditor</rdfs:label>
    </owl:Class>



    <!-- https://w3id.org/italia/onto/OP21/DatoreDiLavoroDomestico -->

    <owl:Class rdf:about="https://w3id.org/italia/onto/OP21/DatoreDiLavoroDomestico">
        <owl:equivalentClass>
            <owl:Restriction>
                <owl:onProperty>
                    <rdf:Description>
                        <owl:inverseOf rdf:resource="https://w3id.org/italia/onto/OP21/haDatoreDiLavoro"/>
                    </rdf:Description>
                </owl:onProperty>
                <owl:someValuesFrom rdf:resource="http://www.w3.org/2002/07/owl#Thing"/>
            </owl:Restriction>
        </owl:equivalentClass>
        <owl:equivalentClass>
            <owl:Restriction>
                <owl:onProperty rdf:resource="https://w3id.org/italia/onto/OP21/identificatoreDatoreDiLavoroDomestico"/>
                <owl:someValuesFrom rdf:resource="http://www.w3.org/2000/01/rdf-schema#Literal"/>
            </owl:Restriction>
        </owl:equivalentClass>
        <owl:disjointWith rdf:resource="https://w3id.org/italia/onto/OP21/RichiedenteAdeguamentoContributivo"/>
        <rdfs:comment xml:lang="en">An employer of a domestic worker is a person who employs someone who is considered a domestic worker.</rdfs:comment>
        <rdfs:comment xml:lang="it">Sottoclasse di Ruolo di Agente che rappresenta il titolare di un rapporto di lavoro con un lavoratore domestico. È solitamente una persona fisica ma, in alcuni particolari casi, può essere una organizzazione qual ora quest&apos;ultima si configuri come una “comunità stabile” o una “convivenze familiarmente strutturata” senza fini di lucro presso cui il lavoratore svolge servizi domestici tipici della vita familiare. Ciascuna istanza possiede un identificatore.</rdfs:comment>
        <rdfs:label xml:lang="it">Datore Di Lavoro Domestico</rdfs:label>
        <rdfs:label xml:lang="en">Domestic Employer</rdfs:label>
    </owl:Class>



    <!-- https://w3id.org/italia/onto/OP21/DebitoreMandato -->

    <owl:Class rdf:about="https://w3id.org/italia/onto/OP21/DebitoreMandato">
        <owl:equivalentClass>
            <owl:Restriction>
                <owl:onProperty>
                    <rdf:Description>
                        <owl:inverseOf rdf:resource="https://w3id.org/italia/onto/OP21/haDebitoreMandato"/>
                    </rdf:Description>
                </owl:onProperty>
                <owl:someValuesFrom rdf:resource="http://www.w3.org/2002/07/owl#Thing"/>
            </owl:Restriction>
        </owl:equivalentClass>
        <rdfs:comment xml:lang="it">Sottoclasse di Correntista associata a Mandato SDD con il ruolo di debitore.</rdfs:comment>
        <rdfs:comment xml:lang="en">Sub-class of bank account holder associated with SDD Mandate with the role of debtor.</rdfs:comment>
        <rdfs:label xml:lang="it">Debitore Mandato</rdfs:label>
        <rdfs:label xml:lang="en">Mandate Debtor</rdfs:label>
    </owl:Class>



    <!-- https://w3id.org/italia/onto/OP21/DomandaAdeguamentoContributivo -->

    <owl:Class rdf:about="https://w3id.org/italia/onto/OP21/DomandaAdeguamentoContributivo">
        <owl:equivalentClass>
            <owl:Restriction>
                <owl:onProperty>
                    <rdf:Description>
                        <owl:inverseOf rdf:resource="https://w3id.org/italia/onto/OP21/presentaDomandaAdeguamentoContributivo"/>
                    </rdf:Description>
                </owl:onProperty>
                <owl:someValuesFrom rdf:resource="http://www.w3.org/2002/07/owl#Thing"/>
            </owl:Restriction>
        </owl:equivalentClass>
        <owl:equivalentClass>
            <owl:Restriction>
                <owl:onProperty>
                    <rdf:Description>
                        <owl:inverseOf rdf:resource="https://w3id.org/italia/onto/OP21/riceveDomanda"/>
                    </rdf:Description>
                </owl:onProperty>
                <owl:someValuesFrom rdf:resource="http://www.w3.org/2002/07/owl#Thing"/>
            </owl:Restriction>
        </owl:equivalentClass>
        <owl:equivalentClass>
            <owl:Restriction>
                <owl:onProperty rdf:resource="https://w3id.org/italia/onto/OP21/dataDomanda"/>
                <owl:someValuesFrom rdf:resource="http://www.w3.org/2000/01/rdf-schema#Literal"/>
            </owl:Restriction>
        </owl:equivalentClass>
        <owl:equivalentClass>
            <owl:Restriction>
                <owl:onProperty rdf:resource="https://w3id.org/italia/onto/OP21/numeroDomanda"/>
                <owl:someValuesFrom rdf:resource="http://www.w3.org/2000/01/rdf-schema#Literal"/>
            </owl:Restriction>
        </owl:equivalentClass>
        <rdfs:comment xml:lang="it">L’esercizio della facoltà di riscatto, ricongiunzione, rendita presuppone la presentazione di apposita domanda da parte dell’interessato Richiedente secondo le modalità specifiche previste da ciascuna facoltà che possono differire sia in termini delle informazioni e documentazioni richieste sia in termini di destinatari della domanda (INPS più eventuali altri Fondi interessati). La presentazione della domanda avviene telematicamente usufruendo del servizio predisposto da INPS eventualmente per l tramite di un intermediario (Patronato, CAF, etc.). La domanda è caratterizzata da una data e un numero assegnato alla stessa dalla Sede INPS competente territorialmente all&apos;atto della presentazione. Quest&apos;ultima istruirà la relativa pratica per gestire la domanda ricevuta.</rdfs:comment>
        <rdfs:comment xml:lang="en">The exercise of the right of redemption, reunion, annuity presupposes the presentation of a specific request by the interested Applicant according to the specific methods provided for by each faculty which may differ both in terms of the information and documentation requested and in terms of recipients of the request (INPS plus any other Funds involved). The application is submitted electronically using the service provided by INPS, possibly through an intermediary (Patronage, CAF, etc.). The application is characterized by a date and a number assigned to it by the territorially competent INPS office at the time of presentation. The latter will instruct the relative practice to manage the received request.</rdfs:comment>
        <rdfs:label xml:lang="en">Contribution Adjustment Claim</rdfs:label>
        <rdfs:label xml:lang="it">Domanda Adeguamento Contributivo</rdfs:label>
    </owl:Class>



    <!-- https://w3id.org/italia/onto/OP21/EnteCreditore -->

    <owl:Class rdf:about="https://w3id.org/italia/onto/OP21/EnteCreditore">
        <rdfs:subClassOf rdf:resource="https://w3id.org/italia/onto/COV/PublicOrganization"/>
        <rdfs:comment xml:lang="it">Sottoclasse di COV:PublicOrganization abilitata a riscuotere le somme dovute all&apos;ente stesso.</rdfs:comment>
        <rdfs:comment xml:lang="en">Subclass of COV:PublicOrganization authorized to collect the sums due to the entity itself.</rdfs:comment>
        <rdfs:label xml:lang="en">Creditor Institution</rdfs:label>
        <rdfs:label xml:lang="it">Ente Creditore</rdfs:label>
    </owl:Class>



    <!-- https://w3id.org/italia/onto/OP21/EsitoPagamento -->

    <owl:Class rdf:about="https://w3id.org/italia/onto/OP21/EsitoPagamento">
        <owl:equivalentClass>
            <owl:Class>
                <owl:unionOf rdf:parseType="Collection">
                    <rdf:Description rdf:about="https://w3id.org/italia/onto/OP21/EsitoPagamentoDefinitivo"/>
                    <rdf:Description rdf:about="https://w3id.org/italia/onto/OP21/EsitoPagamentoProvvisorio"/>
                </owl:unionOf>
            </owl:Class>
        </owl:equivalentClass>
        <owl:equivalentClass>
            <owl:Restriction>
                <owl:onProperty>
                    <rdf:Description>
                        <owl:inverseOf rdf:resource="https://w3id.org/italia/onto/OP21/emetteEsitoPagamento"/>
                    </rdf:Description>
                </owl:onProperty>
                <owl:someValuesFrom rdf:resource="http://www.w3.org/2002/07/owl#Thing"/>
            </owl:Restriction>
        </owl:equivalentClass>
        <owl:equivalentClass>
            <owl:Restriction>
                <owl:onProperty>
                    <rdf:Description>
                        <owl:inverseOf rdf:resource="https://w3id.org/italia/onto/OP21/haEsitoPagamento"/>
                    </rdf:Description>
                </owl:onProperty>
                <owl:someValuesFrom rdf:resource="http://www.w3.org/2002/07/owl#Thing"/>
            </owl:Restriction>
        </owl:equivalentClass>
        <owl:equivalentClass>
            <owl:Restriction>
                <owl:onProperty rdf:resource="https://w3id.org/italia/onto/OP21/descrizioneEsitoPagamento"/>
                <owl:someValuesFrom rdf:resource="http://www.w3.org/2000/01/rdf-schema#Literal"/>
            </owl:Restriction>
        </owl:equivalentClass>
        <owl:equivalentClass>
            <owl:Restriction>
                <owl:onProperty rdf:resource="https://w3id.org/italia/onto/OP21/identificatoreEsitoPagamento"/>
                <owl:someValuesFrom rdf:resource="http://www.w3.org/2000/01/rdf-schema#Literal"/>
            </owl:Restriction>
        </owl:equivalentClass>
        <rdfs:comment xml:lang="it">Esprime l&apos;esito dell&apos;unico pagamento a cui è associato. È caratterizzato da un identificativo e da una o più descrizioni. L&apos;esito di un pagamento può non essere immediatamente noto poichè l&apos;esecuzione del pagamento può coinvolgere diversi intermediari che potrebbero non comunicare in tempo reale l&apos;effettivo buon fine dell&apos;operazione a loro carico. Quindi a meno di un insuccesso immediato l&apos;esito positivo è confermato salvo buon fine ovvero in attesa di conferma da parte dei PSP coinvolti. In questo senso la classe si configura come un evento associato ad un intervallo temporale di validità (sottoclasse TI:TimeIndexedEvent) potendo evolvere nel tempo.</rdfs:comment>
        <rdfs:comment xml:lang="en">Expresses the outcome of the single payment to which it is associated. It is characterized by an identifier and one or more descriptions. The outcome of a payment may not be immediately known as the execution of the payment may involve various intermediaries who may not communicate in real time the effective completion of the operation. Therefore, unless there is an immediate failure, the positive outcome is confirmed subject to successful completion or awaiting confirmation from the PSPs involved. In this sense, the class is configured as an event associated with a valid time interval (subclass TI:TimeIndexedEvent) being able to evolve over time.</rdfs:comment>
        <rdfs:label xml:lang="it">Esito Pagamento</rdfs:label>
        <rdfs:label xml:lang="en">Payment Outcome</rdfs:label>
    </owl:Class>



    <!-- https://w3id.org/italia/onto/OP21/EsitoPagamentoDefinitivo -->

    <owl:Class rdf:about="https://w3id.org/italia/onto/OP21/EsitoPagamentoDefinitivo">
        <owl:equivalentClass>
            <owl:Restriction>
                <owl:onProperty rdf:resource="https://w3id.org/italia/onto/OP21/codiceRiscossione"/>
                <owl:someValuesFrom rdf:resource="http://www.w3.org/2000/01/rdf-schema#Literal"/>
            </owl:Restriction>
        </owl:equivalentClass>
        <owl:disjointWith rdf:resource="https://w3id.org/italia/onto/OP21/EsitoPagamentoProvvisorio"/>
        <rdfs:comment xml:lang="it">Sottoclasse di Esito Pagamento che esprime il buon esito del pagamento associato disponendo anche del codice riscossione che certifica l&apos;avvenuto incasso della somma pagata. Dei pagamenti associati a esiti di questa classe è possibile ottenere la relativa ricevuta di pagamento.</rdfs:comment>
        <rdfs:comment xml:lang="en">Subclass of Payment Outcome which expresses the successful outcome of the associated payment also having the collection code which certifies that the amount paid has been collected. For payments associated with outcomes of this class, it is possible to obtain the relative payment receipt.</rdfs:comment>
        <rdfs:label xml:lang="en">Definitive Payment Outcome</rdfs:label>
        <rdfs:label xml:lang="it">Esito Pagamento Definitivo</rdfs:label>
    </owl:Class>



    <!-- https://w3id.org/italia/onto/OP21/EsitoPagamentoProvvisorio -->

    <owl:Class rdf:about="https://w3id.org/italia/onto/OP21/EsitoPagamentoProvvisorio">
        <rdfs:comment xml:lang="it">Sottoclasse di Esito Pagamento che aggrega esiti di pagamenti non ancora confermati.</rdfs:comment>
        <rdfs:comment xml:lang="en">Sub-class of Payment Outcome that aggregates payment outcomes that have not yet been confirmed.</rdfs:comment>
        <rdfs:label xml:lang="it">Esito Pagamento Provvisorio</rdfs:label>
        <rdfs:label xml:lang="en">Temporary Payment Outcome</rdfs:label>
    </owl:Class>



    <!-- https://w3id.org/italia/onto/OP21/Finalità -->

    <owl:Class rdf:about="https://w3id.org/italia/onto/OP21/Finalità">
        <owl:equivalentClass>
            <owl:Restriction>
                <owl:onProperty rdf:resource="https://w3id.org/italia/onto/OP21/descrizioneFinalità"/>
                <owl:someValuesFrom rdf:resource="http://www.w3.org/2000/01/rdf-schema#Literal"/>
            </owl:Restriction>
        </owl:equivalentClass>
        <rdfs:comment xml:lang="it">Esprime la causale del Bollettino Di Pagamento associato.</rdfs:comment>
        <rdfs:comment xml:lang="en">Expresses the reason for the associated Payment Slip.</rdfs:comment>
        <rdfs:label xml:lang="it">Finalità</rdfs:label>
        <rdfs:label xml:lang="en">Purpose</rdfs:label>
    </owl:Class>



    <!-- https://w3id.org/italia/onto/OP21/FlussoDiRendicontazione -->

    <owl:Class rdf:about="https://w3id.org/italia/onto/OP21/FlussoDiRendicontazione">
        <owl:equivalentClass>
            <owl:Restriction>
                <owl:onProperty rdf:resource="https://w3id.org/italia/onto/OP21/haIntervalloDiRendicontazione"/>
                <owl:someValuesFrom rdf:resource="http://www.w3.org/2002/07/owl#Thing"/>
            </owl:Restriction>
        </owl:equivalentClass>
        <owl:equivalentClass>
            <owl:Restriction>
                <owl:onProperty rdf:resource="https://w3id.org/italia/onto/OP21/haNotaDiMovimento"/>
                <owl:someValuesFrom rdf:resource="http://www.w3.org/2002/07/owl#Thing"/>
            </owl:Restriction>
        </owl:equivalentClass>
        <owl:equivalentClass>
            <owl:Restriction>
                <owl:onProperty>
                    <rdf:Description>
                        <owl:inverseOf rdf:resource="https://w3id.org/italia/onto/OP21/inviaFlussoDiRendicontazione"/>
                    </rdf:Description>
                </owl:onProperty>
                <owl:someValuesFrom rdf:resource="http://www.w3.org/2002/07/owl#Thing"/>
            </owl:Restriction>
        </owl:equivalentClass>
        <owl:equivalentClass>
            <owl:Restriction>
                <owl:onProperty>
                    <rdf:Description>
                        <owl:inverseOf rdf:resource="https://w3id.org/italia/onto/OP21/riceveFlussoDiRendicontazione"/>
                    </rdf:Description>
                </owl:onProperty>
                <owl:someValuesFrom rdf:resource="http://www.w3.org/2002/07/owl#Thing"/>
            </owl:Restriction>
        </owl:equivalentClass>
        <rdfs:subClassOf rdf:resource="https://w3id.org/italia/onto/l0/Collection"/>
        <rdfs:comment xml:lang="it">Sottoclasse di L0:Collection che aggrega le ricevute di movimento emesse da un PSP nei confronti di un Ente, riferite ad un intervallo di tempo.</rdfs:comment>
        <rdfs:comment xml:lang="en">Subclass of L0:Collection that aggregate the movement receipts issued by a PSP to an Organization, referring to a time interval.</rdfs:comment>
        <rdfs:label xml:lang="it">Flusso Di Rendicontazione</rdfs:label>
        <rdfs:label xml:lang="en">Reporting Flow</rdfs:label>
    </owl:Class>



    <!-- https://w3id.org/italia/onto/OP21/IstitutoDiCredito -->

    <owl:Class rdf:about="https://w3id.org/italia/onto/OP21/IstitutoDiCredito">
        <rdfs:subClassOf rdf:resource="https://w3id.org/italia/onto/OP21/PrestatoreDiServiziDiPagamento"/>
        <rdfs:comment xml:lang="en">An undertaking whose business is to receive deposits or other repayable funds from the public and to grant credit for its own account.</rdfs:comment>
        <rdfs:comment xml:lang="it">Un&apos;impresa la cui attività è ricevere depositi o altri fondi rimborsabili dal pubblico e concedere credito per proprio conto.</rdfs:comment>
        <rdfs:label xml:lang="en">Credit Institution</rdfs:label>
        <rdfs:label xml:lang="it">Istituto Di Credito</rdfs:label>
    </owl:Class>



    <!-- https://w3id.org/italia/onto/OP21/LavoratoreDomestico -->

    <owl:Class rdf:about="https://w3id.org/italia/onto/OP21/LavoratoreDomestico">
        <owl:equivalentClass>
            <owl:Restriction>
                <owl:onProperty rdf:resource="https://w3id.org/italia/onto/OP21/identificatoreLavoratoreDomestico"/>
                <owl:someValuesFrom rdf:resource="http://www.w3.org/2000/01/rdf-schema#Literal"/>
            </owl:Restriction>
        </owl:equivalentClass>
        <owl:disjointWith rdf:resource="https://w3id.org/italia/onto/OP21/RichiedenteAdeguamentoContributivo"/>
        <rdfs:comment xml:lang="en">A Domestic Worker is a person who works within the scope of a residence. Domestic workers perform a variety of household services for an individual, from providing cleaning and household maintenance, or cooking, laundry and ironing, or care for children and elderly dependents, and other household errands.</rdfs:comment>
        <rdfs:comment xml:lang="it">Sottoclasse di Ruolo Di Persona Viva che svolge mansioni e prestazioni di servizi domestici diretti al funzionamento della vita familiare nell&apos;ambito di una residenza. I lavoratori domestici svolgono quindi una varietà di servizi rivolti ad un individuo e/o ad una comunità, dalla pulizia e manutenzione della casa, alla cucina, al bucato e alla stiratura, alla cura dei bambini e degli anziani a carico e ad altre commissioni domestiche. Ciascuna istanza possiede un identificatore.</rdfs:comment>
        <rdfs:label xml:lang="en">Domestic Worker</rdfs:label>
        <rdfs:label xml:lang="it">Lavoratore Domestico</rdfs:label>
    </owl:Class>



    <!-- https://w3id.org/italia/onto/OP21/MandatoSDD -->

    <owl:Class rdf:about="https://w3id.org/italia/onto/OP21/MandatoSDD">
        <owl:equivalentClass>
            <owl:Class>
                <owl:unionOf rdf:parseType="Collection">
                    <rdf:Description rdf:about="https://w3id.org/italia/onto/OP21/MandatoSDDAttivo"/>
                    <rdf:Description rdf:about="https://w3id.org/italia/onto/OP21/MandatoSDDNonAttivabile"/>
                    <rdf:Description rdf:about="https://w3id.org/italia/onto/OP21/MandatoSDDRevocato"/>
                    <rdf:Description rdf:about="https://w3id.org/italia/onto/OP21/MandatoSDDRichiedibile"/>
                    <rdf:Description rdf:about="https://w3id.org/italia/onto/OP21/MandatoSDDRichiesto"/>
                </owl:unionOf>
            </owl:Class>
        </owl:equivalentClass>
        <owl:equivalentClass>
            <owl:Restriction>
                <owl:onProperty rdf:resource="https://w3id.org/italia/onto/OP21/haCreditoreMandato"/>
                <owl:someValuesFrom rdf:resource="http://www.w3.org/2002/07/owl#Thing"/>
            </owl:Restriction>
        </owl:equivalentClass>
        <owl:equivalentClass>
            <owl:Restriction>
                <owl:onProperty rdf:resource="https://w3id.org/italia/onto/OP21/haPraticaPerMandato"/>
                <owl:someValuesFrom rdf:resource="http://www.w3.org/2002/07/owl#Thing"/>
            </owl:Restriction>
        </owl:equivalentClass>
        <owl:equivalentClass>
            <owl:Restriction>
                <owl:onProperty rdf:resource="https://w3id.org/italia/onto/OP21/addebitoRicorrente"/>
                <owl:someValuesFrom rdf:resource="http://www.w3.org/2000/01/rdf-schema#Literal"/>
            </owl:Restriction>
        </owl:equivalentClass>
        <owl:equivalentClass>
            <owl:Restriction>
                <owl:onProperty rdf:resource="https://w3id.org/italia/onto/OP21/codiceMandato"/>
                <owl:someValuesFrom rdf:resource="http://www.w3.org/2000/01/rdf-schema#Literal"/>
            </owl:Restriction>
        </owl:equivalentClass>
        <rdfs:comment xml:lang="it">Il Mandato SDD (Sepa Direct Debit) è uno strumento d&apos;incasso preautorizzato utilizzato all&apos;interno di paesi dell&apos;area SEPA con scadenze e importi predeterminati. È caratterizzato da un codice identificativo e dalla possibilità di indicare se trattasi di un pagamento ricorrente o unico. Al mandato sono necessariamente legati il soggetto creditore e il soggetto debitore mediante l&apos;indicazione dei rispettivi IBAN. Le istanze di questa classe possono evolvere nel tempo, assumendo di volta in volta un diverso stato le cui caratteristiche sono legate ad un intervallo temporale di validità. Per questo la classe è sottoclasse della classe TI:TimeIndexedEvent (da OntoPiA - Ontologia del Tempo). Ciascuno stato è rappresentato da una sottoclasse disgiunta da tutte le altre.</rdfs:comment>
        <rdfs:comment xml:lang="en">SEPA Direct Debit (SDD) is a specific payment scheme within SEPA that is used for regular payments such as for subscriptions and bills. Like all SEPA payments, these transactions must be in euros, and payments are bank to bank.</rdfs:comment>
        <rdfs:label xml:lang="it">Mandato SDD</rdfs:label>
        <rdfs:label xml:lang="en">SDD Mandate</rdfs:label>
    </owl:Class>



    <!-- https://w3id.org/italia/onto/OP21/MandatoSDDAttivo -->

    <owl:Class rdf:about="https://w3id.org/italia/onto/OP21/MandatoSDDAttivo">
        <owl:equivalentClass>
            <owl:Restriction>
                <owl:onProperty>
                    <rdf:Description>
                        <owl:inverseOf rdf:resource="https://w3id.org/italia/onto/OP21/autorizzaMandato"/>
                    </rdf:Description>
                </owl:onProperty>
                <owl:someValuesFrom rdf:resource="http://www.w3.org/2002/07/owl#Thing"/>
            </owl:Restriction>
        </owl:equivalentClass>
        <owl:disjointWith rdf:resource="https://w3id.org/italia/onto/OP21/RID"/>
        <owl:disjointWith rdf:resource="https://w3id.org/italia/onto/OP21/SessionePagamentoElettronico"/>
        <rdfs:comment xml:lang="en">SDD Mandate sub-class which aggregates the required mandates that have satisfied the adequacy and ownership checks and which have therefore given rise to a Mandate Activation Deed, unequivocally and obligatorily linked to the single mandate instance.</rdfs:comment>
        <rdfs:comment xml:lang="it">Sottoclasse di Mandato SDD che aggrega i mandati richiesti che hanno soddisfatto i controlli di congruità e titolarità e che hanno dato quindi luogo ad un Atto di Attivazione Mandato, legato univocamente e obbligatoriamente alla singola istanza di mandato.</rdfs:comment>
        <rdfs:label xml:lang="en">Active SDD Mandate</rdfs:label>
        <rdfs:label xml:lang="it">Mandato SDD Attivo</rdfs:label>
    </owl:Class>



    <!-- https://w3id.org/italia/onto/OP21/MandatoSDDNonAttivabile -->

    <owl:Class rdf:about="https://w3id.org/italia/onto/OP21/MandatoSDDNonAttivabile">
        <rdfs:comment xml:lang="en">SDD Mandate sub-class that aggregates requested mandates that have not satisfied the adequacy and entitlement checks.</rdfs:comment>
        <rdfs:comment xml:lang="it">Sottoclasse di Mandato SDD che aggrega i mandati richiesti che non hanno soddisfatto i controlli di congruità e titolarità.</rdfs:comment>
        <rdfs:label xml:lang="it">Mandato SDD Non Attivabile</rdfs:label>
        <rdfs:label xml:lang="en">SDD Mandate which cannot be activated</rdfs:label>
    </owl:Class>



    <!-- https://w3id.org/italia/onto/OP21/MandatoSDDRevocato -->

    <owl:Class rdf:about="https://w3id.org/italia/onto/OP21/MandatoSDDRevocato">
        <owl:equivalentClass>
            <owl:Restriction>
                <owl:onProperty>
                    <rdf:Description>
                        <owl:inverseOf rdf:resource="https://w3id.org/italia/onto/OP21/revocaMandato"/>
                    </rdf:Description>
                </owl:onProperty>
                <owl:someValuesFrom rdf:resource="http://www.w3.org/2002/07/owl#Thing"/>
            </owl:Restriction>
        </owl:equivalentClass>
        <rdfs:comment xml:lang="en">SDD Mandate sub-class which aggregates the active mandates that have been revoked with a specific Mandate Revocation Deed, univocally and obligatorily linked to the single mandate instance.</rdfs:comment>
        <rdfs:comment xml:lang="it">Sottoclasse di Mandato SDD che aggrega i mandati attivi che sono stati revocati con apposito Atto di Revoca Mandato, legato univocamente e obbligatoriamente alla singola istanza di mandato.</rdfs:comment>
        <rdfs:label xml:lang="it">Mandato SDD Revocato</rdfs:label>
        <rdfs:label xml:lang="en">Revoked SDD Mandate</rdfs:label>
    </owl:Class>



    <!-- https://w3id.org/italia/onto/OP21/MandatoSDDRichiedibile -->

    <owl:Class rdf:about="https://w3id.org/italia/onto/OP21/MandatoSDDRichiedibile">
        <owl:equivalentClass>
            <owl:Class>
                <owl:intersectionOf rdf:parseType="Collection">
                    <rdf:Description rdf:about="https://w3id.org/italia/onto/OP21/MandatoSDD"/>
                    <owl:Class>
                        <owl:complementOf>
                            <owl:Restriction>
                                <owl:onProperty rdf:resource="https://w3id.org/italia/onto/OP21/haDebitoreMandato"/>
                                <owl:someValuesFrom rdf:resource="http://www.w3.org/2002/07/owl#Thing"/>
                            </owl:Restriction>
                        </owl:complementOf>
                    </owl:Class>
                </owl:intersectionOf>
            </owl:Class>
        </owl:equivalentClass>
        <rdfs:comment xml:lang="en">SDD Mandate sub-class which aggregates the mandates pre-compiled by the Creditor Institution and in which the creditor&apos;s data are present but those of the debtor absent. These pre-compiled mandates are available for all installments and constitute the initial state of an SDD Mandate.</rdfs:comment>
        <rdfs:comment xml:lang="it">Sottoclasse di Mandato SDD che aggrega i mandati precompilati a cura dell&apos;Ente Creditore e in cui sono presenti i dati del creditore ma assenti quelli del debitore. Questi mandati precompilati sono disponibili per tutte le pratiche rateizzate e costituiscono lo stato iniziale di un Mandato SDD.</rdfs:comment>
        <rdfs:label xml:lang="it">Mandato SDD Richiedibile</rdfs:label>
        <rdfs:label xml:lang="en">Requestable SDD Mandate</rdfs:label>
    </owl:Class>



    <!-- https://w3id.org/italia/onto/OP21/MandatoSDDRichiesto -->

    <owl:Class rdf:about="https://w3id.org/italia/onto/OP21/MandatoSDDRichiesto">
        <owl:equivalentClass>
            <owl:Restriction>
                <owl:onProperty rdf:resource="https://w3id.org/italia/onto/OP21/numeroContoDiAddebito"/>
                <owl:someValuesFrom rdf:resource="http://www.w3.org/2000/01/rdf-schema#Literal"/>
            </owl:Restriction>
        </owl:equivalentClass>
        <rdfs:comment xml:lang="it">Sottoclasse di Mandato SDD che aggrega quei mandati per cui è stata richiesta l&apos;attivazione indicando il numero di conto del debitore (IBAN). In questo stato l&apos;Ente Creditore svolge le verifiche del caso sul numero indicato in primo luogo per accertare, anche con il coinvolgimento dell&apos;Istituto di Credito depositario del conto, se l&apos;intestatario del conto corrisponde all&apos;intestatario debitore del mandato ovvero il pagatore della pratica di adeguamento contributivo che può essere il titolare della pratica stessa, se in vita, o, in caso contrario, un suo superstite. Queste verifiche possono essere contestuali alla richiesta ovvero richiedere un tempo di sospensione della richiesta in attesa di verifica.</rdfs:comment>
        <rdfs:comment xml:lang="en">Sub-class of SDD Mandate which aggregates those mandates for which activation has been requested by indicating the debtor&apos;s bank account number (IBAN). In this status, the Creditor Institution carries out the necessary checks on the number indicated firstly to ascertain, along with the involvement of the Account Depositary Credit Institution, whether the account holder corresponds to the debtor holder of the mandate or the payer of the tax contribution adjustment application, who may be the holder of the file itself, if alive, or, if not, one of his survivors. These checks can be contextual to the request or require a period of suspension of the request pending verification.</rdfs:comment>
        <rdfs:label xml:lang="it">Mandato SDD Richiesto</rdfs:label>
        <rdfs:label xml:lang="en">Requested SDD Mandate</rdfs:label>
    </owl:Class>



    <!-- https://w3id.org/italia/onto/OP21/MeseDiTrimestre -->

    <owl:Class rdf:about="https://w3id.org/italia/onto/OP21/MeseDiTrimestre">
        <owl:equivalentClass>
            <owl:Restriction>
                <owl:onProperty rdf:resource="https://w3id.org/italia/onto/OP21/èMeseDelTrimestre"/>
                <owl:someValuesFrom rdf:resource="http://www.w3.org/2002/07/owl#Thing"/>
            </owl:Restriction>
        </owl:equivalentClass>
        <owl:equivalentClass>
            <owl:Restriction>
                <owl:onProperty>
                    <rdf:Description>
                        <owl:inverseOf rdf:resource="https://w3id.org/italia/onto/OP21/èSettimanaDelMese"/>
                    </rdf:Description>
                </owl:onProperty>
                <owl:someValuesFrom rdf:resource="http://www.w3.org/2002/07/owl#Thing"/>
            </owl:Restriction>
        </owl:equivalentClass>
        <owl:equivalentClass>
            <owl:Restriction>
                <owl:onProperty rdf:resource="https://w3id.org/italia/onto/OP21/indiceMese"/>
                <owl:someValuesFrom rdf:resource="http://www.w3.org/2000/01/rdf-schema#Literal"/>
            </owl:Restriction>
        </owl:equivalentClass>
        <rdfs:comment xml:lang="en">Index of the months present in a calendar quarter. Basically first, second and third (subclass of TI:TemporalEntity).</rdfs:comment>
        <rdfs:comment xml:lang="it">Indice dei mesi presenti in un trimestre solare. In pratica primo, secondo e terzo (sottoclasse di TI:TemporalEntity).</rdfs:comment>
        <rdfs:label xml:lang="it">Mese Di Trimestre</rdfs:label>
        <rdfs:label xml:lang="en">Month of Trimester</rdfs:label>
    </owl:Class>



    <!-- https://w3id.org/italia/onto/OP21/ModalitàDiPagamento -->

    <owl:Class rdf:about="https://w3id.org/italia/onto/OP21/ModalitàDiPagamento">
        <owl:equivalentClass>
            <owl:Class>
                <owl:unionOf rdf:parseType="Collection">
                    <rdf:Description rdf:about="https://w3id.org/italia/onto/OP21/AvvisoDiPagamento"/>
                    <rdf:Description rdf:about="https://w3id.org/italia/onto/OP21/SessionePagamentoElettronico"/>
                </owl:unionOf>
            </owl:Class>
        </owl:equivalentClass>
        <owl:equivalentClass>
            <owl:Restriction>
                <owl:onProperty>
                    <rdf:Description>
                        <owl:inverseOf rdf:resource="https://w3id.org/italia/onto/OP21/haModalitàDiPagamento"/>
                    </rdf:Description>
                </owl:onProperty>
                <owl:someValuesFrom rdf:resource="http://www.w3.org/2002/07/owl#Thing"/>
            </owl:Restriction>
        </owl:equivalentClass>
        <rdfs:comment xml:lang="it">Esprime la modalità con cui viene pagato un Bollettino Di Pagamento. </rdfs:comment>
        <rdfs:comment xml:lang="en">Expresses the method by which a payment slip is paid.</rdfs:comment>
        <rdfs:label xml:lang="it">Modalità Di Pagamento</rdfs:label>
        <rdfs:label xml:lang="en">Payment Mode</rdfs:label>
    </owl:Class>



    <!-- https://w3id.org/italia/onto/OP21/MovimentoDiDenaro -->

    <owl:Class rdf:about="https://w3id.org/italia/onto/OP21/MovimentoDiDenaro">
        <owl:equivalentClass>
            <owl:Restriction>
                <owl:onProperty rdf:resource="https://w3id.org/italia/onto/OP21/inviaRicevutaDiMovimento"/>
                <owl:someValuesFrom rdf:resource="http://www.w3.org/2002/07/owl#Thing"/>
            </owl:Restriction>
        </owl:equivalentClass>
        <owl:equivalentClass>
            <owl:Restriction>
                <owl:onProperty rdf:resource="https://w3id.org/italia/onto/OP21/movimentoAgisceSu"/>
                <owl:someValuesFrom rdf:resource="http://www.w3.org/2002/07/owl#Thing"/>
            </owl:Restriction>
        </owl:equivalentClass>
        <owl:equivalentClass>
            <owl:Restriction>
                <owl:onProperty>
                    <rdf:Description>
                        <owl:inverseOf rdf:resource="https://w3id.org/italia/onto/OP21/esegueAccredito"/>
                    </rdf:Description>
                </owl:onProperty>
                <owl:someValuesFrom rdf:resource="http://www.w3.org/2002/07/owl#Thing"/>
            </owl:Restriction>
        </owl:equivalentClass>
        <owl:equivalentClass>
            <owl:Restriction>
                <owl:onProperty>
                    <rdf:Description>
                        <owl:inverseOf rdf:resource="https://w3id.org/italia/onto/OP21/esegueAddebito"/>
                    </rdf:Description>
                </owl:onProperty>
                <owl:someValuesFrom rdf:resource="http://www.w3.org/2002/07/owl#Thing"/>
            </owl:Restriction>
        </owl:equivalentClass>
        <owl:equivalentClass>
            <owl:Restriction>
                <owl:onProperty rdf:resource="https://w3id.org/italia/onto/OP21/causaleMovimento"/>
                <owl:someValuesFrom rdf:resource="http://www.w3.org/2000/01/rdf-schema#Literal"/>
            </owl:Restriction>
        </owl:equivalentClass>
        <owl:equivalentClass>
            <owl:Restriction>
                <owl:onProperty rdf:resource="https://w3id.org/italia/onto/OP21/dataMovimento"/>
                <owl:someValuesFrom rdf:resource="http://www.w3.org/2000/01/rdf-schema#Literal"/>
            </owl:Restriction>
        </owl:equivalentClass>
        <owl:equivalentClass>
            <owl:Restriction>
                <owl:onProperty rdf:resource="https://w3id.org/italia/onto/OP21/identificatoreMovimento"/>
                <owl:someValuesFrom rdf:resource="http://www.w3.org/2000/01/rdf-schema#Literal"/>
            </owl:Restriction>
        </owl:equivalentClass>
        <owl:equivalentClass>
            <owl:Restriction>
                <owl:onProperty rdf:resource="https://w3id.org/italia/onto/OP21/importoMovimento"/>
                <owl:someValuesFrom rdf:resource="http://www.w3.org/2000/01/rdf-schema#Literal"/>
            </owl:Restriction>
        </owl:equivalentClass>
        <rdfs:comment xml:lang="en">Movement of a sum of money induced by a Payment Order on a Current Account. This movement increases (credit) or decreases (debit) the availability of money in the Current Account. A commission may be charged for executing the movement, usually in the debit transaction. It is characterized by an identifier, an amount and a date.</rdfs:comment>
        <rdfs:comment xml:lang="it">Movimento di una somma di denaro indotto da un Ordine Di Pagamento su un Conto Corrente. Tale movimento aumenta (accredito) o diminuisce (addebito) la disponibilità di denaro del Conto Corrente. Può essere addebita una commissione per l&apos;esecuzione del movimento, solitamente nell&apos;operazione di addebito. È caratterizzata da un identificatore, un importo e una data.</rdfs:comment>
        <rdfs:label xml:lang="en">Money Movement</rdfs:label>
        <rdfs:label xml:lang="it">Movimento Di Denaro</rdfs:label>
    </owl:Class>



    <!-- https://w3id.org/italia/onto/OP21/OnereContributivo -->

    <owl:Class rdf:about="https://w3id.org/italia/onto/OP21/OnereContributivo">
        <owl:equivalentClass>
            <owl:Restriction>
                <owl:onProperty>
                    <rdf:Description>
                        <owl:inverseOf rdf:resource="https://w3id.org/italia/onto/OP21/haOnereContributivo"/>
                    </rdf:Description>
                </owl:onProperty>
                <owl:someValuesFrom rdf:resource="http://www.w3.org/2002/07/owl#Thing"/>
            </owl:Restriction>
        </owl:equivalentClass>
        <owl:equivalentClass>
            <owl:Restriction>
                <owl:onProperty rdf:resource="https://w3id.org/italia/onto/OP21/dataScadenzaOnereContributivo"/>
                <owl:someValuesFrom rdf:resource="http://www.w3.org/2000/01/rdf-schema#Literal"/>
            </owl:Restriction>
        </owl:equivalentClass>
        <owl:equivalentClass>
            <owl:Restriction>
                <owl:onProperty rdf:resource="https://w3id.org/italia/onto/OP21/importoOnereContributivo"/>
                <owl:someValuesFrom rdf:resource="http://www.w3.org/2000/01/rdf-schema#Literal"/>
            </owl:Restriction>
        </owl:equivalentClass>
        <rdfs:comment xml:lang="en">Amount of money that the Holder of n Application, or one of his survivors, are requested to pay in order to satisfy the acceptance of the presented application. The amount of this sum is established by INPS with a specific document and communicated to the Applicant together with the date by which said sum must be paid, under penalty of forfeiture of the application. Each instance of the class is necessarily linked to one and only one case in Notified Amount status. It is a subclass of Purpose, thus resulting linked to the Payment Slip class to which it provides the data for its compilation.</rdfs:comment>
        <rdfs:comment xml:lang="it">Somma di denaro che il Titolare di una Pratica, o un suo Superstite, sono chiamati a versare per soddisfare l&apos;accettazione della domanda presentata. L&apos;importo di detta somma è stabilito dall&apos;INPS con apposito Atto e comunicato al Richiedente unitamente alla data entro cui detta somma deve essere versata pena la decadenza della domanda. Ogni istanza della classe è necessariamente legata ad una ed una sola pratica in stato di Notificato Importo. È sottoclasse di Finalità risultando in tal modo legata alla classe Bollettino Di Pagamento a cui fornisce i dati per la compilazione dello stesso.</rdfs:comment>
        <rdfs:label xml:lang="en">Contributory Charge</rdfs:label>
        <rdfs:label xml:lang="it">Onere Contributivo</rdfs:label>
    </owl:Class>



    <!-- https://w3id.org/italia/onto/OP21/OrdineDiPagamento -->

    <owl:Class rdf:about="https://w3id.org/italia/onto/OP21/OrdineDiPagamento">
        <owl:equivalentClass>
            <owl:Restriction>
                <owl:onProperty rdf:resource="https://w3id.org/italia/onto/OP21/esegueAccredito"/>
                <owl:someValuesFrom rdf:resource="http://www.w3.org/2002/07/owl#Thing"/>
            </owl:Restriction>
        </owl:equivalentClass>
        <owl:equivalentClass>
            <owl:Restriction>
                <owl:onProperty rdf:resource="https://w3id.org/italia/onto/OP21/esegueAddebito"/>
                <owl:someValuesFrom rdf:resource="http://www.w3.org/2002/07/owl#Thing"/>
            </owl:Restriction>
        </owl:equivalentClass>
        <owl:equivalentClass>
            <owl:Restriction>
                <owl:onProperty rdf:resource="https://w3id.org/italia/onto/OP21/utilizzaServizioDiPagamento"/>
                <owl:someValuesFrom rdf:resource="http://www.w3.org/2002/07/owl#Thing"/>
            </owl:Restriction>
        </owl:equivalentClass>
        <owl:equivalentClass>
            <owl:Restriction>
                <owl:onProperty>
                    <rdf:Description>
                        <owl:inverseOf rdf:resource="https://w3id.org/italia/onto/OP21/attivaOrdineDiPagamento"/>
                    </rdf:Description>
                </owl:onProperty>
                <owl:someValuesFrom rdf:resource="http://www.w3.org/2002/07/owl#Thing"/>
            </owl:Restriction>
        </owl:equivalentClass>
        <owl:equivalentClass>
            <owl:Restriction>
                <owl:onProperty rdf:resource="https://w3id.org/italia/onto/OP21/dataOrdinePagamento"/>
                <owl:someValuesFrom rdf:resource="http://www.w3.org/2000/01/rdf-schema#Literal"/>
            </owl:Restriction>
        </owl:equivalentClass>
        <owl:equivalentClass>
            <owl:Restriction>
                <owl:onProperty rdf:resource="https://w3id.org/italia/onto/OP21/identificatoreOrdinePagamento"/>
                <owl:someValuesFrom rdf:resource="http://www.w3.org/2000/01/rdf-schema#Literal"/>
            </owl:Restriction>
        </owl:equivalentClass>
        <rdfs:comment xml:lang="en">It is the materialization of a Payment made through a Payment Service provided by a PSP. It is characterized by an identifier and a date and is uniquely linked to the money transactions that debit and credit the amount of money transferred via the payment order.</rdfs:comment>
        <rdfs:comment xml:lang="it">È la materializzazione di un Pagamento eseguito tramite un Servizio Di Pagamento erogato da un PSP. È caratterizzato da un identificatore e da una data ed è legato univocamente alle transazioni di denaro che addebitano e accreditano la somma di denaro trasferita tramite l&apos;ordine di pagamento.</rdfs:comment>
        <rdfs:label xml:lang="it">Ordine Di Pagamento</rdfs:label>
        <rdfs:label xml:lang="en">Payment Order</rdfs:label>
    </owl:Class>



    <!-- https://w3id.org/italia/onto/OP21/OrganizzazioneDiAssistenza -->

    <owl:Class rdf:about="https://w3id.org/italia/onto/OP21/OrganizzazioneDiAssistenza">
        <owl:equivalentClass>
            <owl:Restriction>
                <owl:onProperty>
                    <rdf:Description>
                        <owl:inverseOf rdf:resource="https://w3id.org/italia/onto/OP21/haOrganizzazioneDiAssistenza"/>
                    </rdf:Description>
                </owl:onProperty>
                <owl:someValuesFrom rdf:resource="http://www.w3.org/2002/07/owl#Thing"/>
            </owl:Restriction>
        </owl:equivalentClass>
        <owl:equivalentClass>
            <owl:Restriction>
                <owl:onProperty>
                    <rdf:Description>
                        <owl:inverseOf rdf:resource="https://w3id.org/italia/onto/OP21/haVersamentoOrganizzazione"/>
                    </rdf:Description>
                </owl:onProperty>
                <owl:someValuesFrom rdf:resource="http://www.w3.org/2002/07/owl#Thing"/>
            </owl:Restriction>
        </owl:equivalentClass>
        <owl:equivalentClass>
            <owl:Restriction>
                <owl:onProperty rdf:resource="https://w3id.org/italia/onto/OP21/codiceOrganizzazione"/>
                <owl:someValuesFrom rdf:resource="http://www.w3.org/2000/01/rdf-schema#Literal"/>
            </owl:Restriction>
        </owl:equivalentClass>
        <rdfs:comment xml:lang="en">Body that has the purpose of providing benefits and services in favor of workers and employers, including health care and insurance treatments, supplementary and additional to public services.</rdfs:comment>
        <rdfs:comment xml:lang="it">Organismo che ha lo scopo di fornire prestazioni e servizi a favore dei lavoratori e datori di lavoro, comprensivi di trattamenti assistenziali sanitari e assicurativi, integrativi e aggiuntivi delle prestazioni pubbliche.</rdfs:comment>
        <rdfs:label xml:lang="en">Assistance Organization</rdfs:label>
        <rdfs:label xml:lang="it">Organizzazione Di Assistenza</rdfs:label>
    </owl:Class>



    <!-- https://w3id.org/italia/onto/OP21/POSVirtuale -->

    <owl:Class rdf:about="https://w3id.org/italia/onto/OP21/POSVirtuale">
        <owl:disjointWith rdf:resource="https://w3id.org/italia/onto/OP21/RetiAmiche"/>
        <rdfs:comment xml:lang="en">A Virtual POS (Point of Sale) is typically a web or windows application that can be used by card-accepting merchants to manually authorize card transactions. Most Payment Services Providers offer this type of functionality.</rdfs:comment>
        <rdfs:comment xml:lang="it">Sistema di pagamento costituito da un software capace di eseguire le transazioni di pagamento direttamente online.</rdfs:comment>
        <rdfs:label xml:lang="it">POS Virtuale</rdfs:label>
        <rdfs:label xml:lang="en">Virtual POS</rdfs:label>
    </owl:Class>



    <!-- https://w3id.org/italia/onto/OP21/Pagamento -->

    <owl:Class rdf:about="https://w3id.org/italia/onto/OP21/Pagamento">
        <owl:equivalentClass>
            <owl:Restriction>
                <owl:onProperty rdf:resource="https://w3id.org/italia/onto/OP21/haEsitoPagamento"/>
                <owl:someValuesFrom rdf:resource="http://www.w3.org/2002/07/owl#Thing"/>
            </owl:Restriction>
        </owl:equivalentClass>
        <owl:equivalentClass>
            <owl:Restriction>
                <owl:onProperty>
                    <rdf:Description>
                        <owl:inverseOf rdf:resource="https://w3id.org/italia/onto/OP21/eseguePagamento"/>
                    </rdf:Description>
                </owl:onProperty>
                <owl:someValuesFrom rdf:resource="http://www.w3.org/2002/07/owl#Thing"/>
            </owl:Restriction>
        </owl:equivalentClass>
        <owl:equivalentClass>
            <owl:Restriction>
                <owl:onProperty rdf:resource="https://w3id.org/italia/onto/OP21/dataPagamento"/>
                <owl:someValuesFrom rdf:resource="http://www.w3.org/2000/01/rdf-schema#Literal"/>
            </owl:Restriction>
        </owl:equivalentClass>
        <owl:equivalentClass>
            <owl:Restriction>
                <owl:onProperty rdf:resource="https://w3id.org/italia/onto/OP21/importoPagamento"/>
                <owl:someValuesFrom rdf:resource="http://www.w3.org/2000/01/rdf-schema#Literal"/>
            </owl:Restriction>
        </owl:equivalentClass>
        <owl:disjointWith rdf:resource="https://w3id.org/italia/onto/OP21/PrenotazioneDiPagamento"/>
        <rdfs:comment xml:lang="en">Transfer of a sum of money as consideration for a service or as a means of extinguishing an obligation. If it takes place through traced methods, therefore not in cash, it materializes in a Payment Order entrusted to a PSP which is responsible for actually carrying out the transfer. It features a date and amount.</rdfs:comment>
        <rdfs:comment xml:lang="it">Trasferimento di una somma di denaro come corrispettivo di una prestazione o come mezzo di estinzione di un&apos;obbligazione. Nel caso avvenga tramite modalità tracciate, quindi non in contanti, si materializza in un Ordine Di Pagamento affidato ad un PSP che si fa carico di eseguire effettivamente il trasferimento. È caratterizzato da una data e un importo.</rdfs:comment>
        <rdfs:label xml:lang="it">Pagamento</rdfs:label>
        <rdfs:label xml:lang="en">Payment</rdfs:label>
    </owl:Class>



    <!-- https://w3id.org/italia/onto/OP21/Pagatore -->

    <owl:Class rdf:about="https://w3id.org/italia/onto/OP21/Pagatore">
        <rdfs:comment xml:lang="en">Abstract superclass that aggregates agent roles called to make payments, using methods common to all payers, to satisfy obligations contracted by themselves or by another subject formally related to them.</rdfs:comment>
        <rdfs:comment xml:lang="it">Superclasse astratta che aggrega ruoli di agente chiamati ad eseguire pagamenti, mediante modalità comuni a tutti pagatori, per soddisfare obbligazioni contratte da essi stessi o da altro soggetto ad essi formalmente legato.</rdfs:comment>
        <rdfs:label xml:lang="it">Pagatore</rdfs:label>
        <rdfs:label xml:lang="en">Payer</rdfs:label>
    </owl:Class>



    <!-- https://w3id.org/italia/onto/OP21/PianoDiAmmortamento -->

    <owl:Class rdf:about="https://w3id.org/italia/onto/OP21/PianoDiAmmortamento">
        <owl:equivalentClass>
            <owl:Restriction>
                <owl:onProperty rdf:resource="https://w3id.org/italia/onto/OP21/haRata"/>
                <owl:someValuesFrom rdf:resource="http://www.w3.org/2002/07/owl#Thing"/>
            </owl:Restriction>
        </owl:equivalentClass>
        <owl:equivalentClass>
            <owl:Restriction>
                <owl:onProperty>
                    <rdf:Description>
                        <owl:inverseOf rdf:resource="https://w3id.org/italia/onto/OP21/haPianoDiAmmortamento"/>
                    </rdf:Description>
                </owl:onProperty>
                <owl:someValuesFrom rdf:resource="http://www.w3.org/2002/07/owl#Thing"/>
            </owl:Restriction>
        </owl:equivalentClass>
        <owl:equivalentClass>
            <owl:Restriction>
                <owl:onProperty rdf:resource="https://w3id.org/italia/onto/OP21/importoRata"/>
                <owl:someValuesFrom rdf:resource="http://www.w3.org/2000/01/rdf-schema#Literal"/>
            </owl:Restriction>
        </owl:equivalentClass>
        <owl:equivalentClass>
            <owl:Restriction>
                <owl:onProperty rdf:resource="https://w3id.org/italia/onto/OP21/numeroRate"/>
                <owl:someValuesFrom rdf:resource="http://www.w3.org/2000/01/rdf-schema#Literal"/>
            </owl:Restriction>
        </owl:equivalentClass>
        <rdfs:subClassOf rdf:resource="https://w3id.org/italia/onto/l0/Sequence"/>
        <rdfs:comment xml:lang="it">Il piano di ammortamento è il programma di restituzione rateale di un debito, che solitamente scompone le rate in quote capitale e quote interessi, e specifica il capitale residuo dovuto dopo ciascun pagamento. È caratterizzato da un numero di rate e dall&apos;importo di ciascuna rata, solitamente costante. Nel contesto di questo dominio rappresenta la rateizzazione dell&apos;Onere Contributivo e viene proposto al Richiedente come modalità alternativa rispetto al versamento unico. Il Richiedente può aderire a tale piano o chiedere una sua modifica, ad esempio per ridurre il numero di rate proposte. Ogni istanza della classe è necessariamente legata ad una ed una sola pratica in stato di Notificato Importo. La classe si comporta come una Sequenze per cui ad ogni istanza della classe sono legate le istanze della classe Rata Di Onere Contributivo corrispondenti ciascuna ad una rata del piano.</rdfs:comment>
        <rdfs:comment xml:lang="en">The amortization schedule is the schedule for repaying a debt by installments, which usually breaks down the installments into principal and interest portions, and specifies the residual principal due after each payment.</rdfs:comment>
        <rdfs:label xml:lang="en">Amortization Schedule</rdfs:label>
        <rdfs:label xml:lang="it">Piano Di Ammortamento</rdfs:label>
    </owl:Class>



    <!-- https://w3id.org/italia/onto/OP21/PraticaAdeguamentoContributivo -->

    <owl:Class rdf:about="https://w3id.org/italia/onto/OP21/PraticaAdeguamentoContributivo">
        <owl:equivalentClass>
            <owl:Restriction>
                <owl:onProperty rdf:resource="https://w3id.org/italia/onto/OP21/haDomandaAdeguamentoContributivo"/>
                <owl:someValuesFrom rdf:resource="http://www.w3.org/2002/07/owl#Thing"/>
            </owl:Restriction>
        </owl:equivalentClass>
        <owl:equivalentClass>
            <owl:Restriction>
                <owl:onProperty rdf:resource="https://w3id.org/italia/onto/OP21/haTitolarePratica"/>
                <owl:someValuesFrom rdf:resource="http://www.w3.org/2002/07/owl#Thing"/>
            </owl:Restriction>
        </owl:equivalentClass>
        <owl:equivalentClass>
            <owl:Restriction>
                <owl:onProperty>
                    <rdf:Description>
                        <owl:inverseOf rdf:resource="https://w3id.org/italia/onto/OP21/istruiscePratica"/>
                    </rdf:Description>
                </owl:onProperty>
                <owl:someValuesFrom rdf:resource="http://www.w3.org/2002/07/owl#Thing"/>
            </owl:Restriction>
        </owl:equivalentClass>
        <owl:equivalentClass>
            <owl:Restriction>
                <owl:onProperty rdf:resource="https://w3id.org/italia/onto/OP21/descrizionePratica"/>
                <owl:someValuesFrom rdf:resource="http://www.w3.org/2000/01/rdf-schema#Literal"/>
            </owl:Restriction>
        </owl:equivalentClass>
        <owl:equivalentClass>
            <owl:Restriction>
                <owl:onProperty rdf:resource="https://w3id.org/italia/onto/OP21/numeroPratica"/>
                <owl:someValuesFrom rdf:resource="http://www.w3.org/2000/01/rdf-schema#Literal"/>
            </owl:Restriction>
        </owl:equivalentClass>
        <rdfs:comment xml:lang="en">Abstract class that aggregates the different types of practices initiated by the INPS, in particular the practices of redemption and/or reunification of contributions, including annuities. Each file has a unique identifier and a description and is obligatorily linked to one and only one Application (for) Contribution Adjustment, against which the file itself was instructed by the INPS office competent for the Applicant who presented the application. Once the file has been assessed by INPS, it is linked to one and only one Contribution Adjustment Act (of) Contribution Adjustment with which the aforementioned INPS office informs the Applicant of the outcome of the application. Instances of this class can evolve over time, each time assuming a different state whose characteristics are linked to a time interval of validity. This is why the class is a subclass of the TI:TimeIndexedEvent class (from OntoPiA - Time Ontology). The possible states of instances are classified by its disjoint subclasses denoted by names with the prefix Status.</rdfs:comment>
        <rdfs:comment xml:lang="it">Classe astratta che aggrega le diverse tipologie di pratiche istruite dall&apos;INPS, in particolare le pratiche di riscatto e/o ricongiunzione di contributi, ivi comprese le rendite. Ciascuna pratica ha un identificativo e una descrizione ed è legata obbligatoriamente ad una e una sola Domanda (di) Adeguamento Contributivo, a fronte della quale la pratica stessa è stata istruita a cura della Sede INPS competente per il Richiedente che ha presentato la domanda. Una volta che la pratica è stata valutata dall&apos;INPS, viene legata ad uno ed un solo Atto (di) Adeguamento Contributivo con cui la suddetta Sede INPS comunica al Richiedente l&apos;esito della domanda. Le istanze di questa classe possono evolvere nel tempo, assumendo di volta in volta un diverso stato le cui caratteristiche sono legate ad un intervallo temporale di validità. Per questo la classe è sottoclasse della classe TI:TimeIndexedEvent (da OntoPiA - Ontologia del Tempo). I possibili stati delle istanze sono classificati da sue sottoclassi disgiunte denotate da nomi aventi il prefisso Stato. Ad una Pratica è legato obbligatoriamente uno ed un solo titolare della Pratica che corrisponde alla persona che possiede i requisiti per attivare la facoltà e, solo se il titolare è deceduto, uno ed un solo superstite pagatore.</rdfs:comment>
        <rdfs:label xml:lang="en">Contribution Adjustment Application</rdfs:label>
        <rdfs:label xml:lang="it">Pratica Adeguamento Contributivo</rdfs:label>
    </owl:Class>



    <!-- https://w3id.org/italia/onto/OP21/PraticaDiAdeguamentoRateizzata -->

    <owl:Class rdf:about="https://w3id.org/italia/onto/OP21/PraticaDiAdeguamentoRateizzata">
        <owl:equivalentClass>
            <owl:Restriction>
                <owl:onProperty rdf:resource="https://w3id.org/italia/onto/OP21/haPianoDiAmmortamento"/>
                <owl:someValuesFrom rdf:resource="https://w3id.org/italia/onto/OP21/PianoDiAmmortamento"/>
            </owl:Restriction>
        </owl:equivalentClass>
        <owl:equivalentClass>
            <owl:Restriction>
                <owl:onProperty>
                    <rdf:Description>
                        <owl:inverseOf rdf:resource="https://w3id.org/italia/onto/OP21/haPraticaPerMandato"/>
                    </rdf:Description>
                </owl:onProperty>
                <owl:someValuesFrom rdf:resource="http://www.w3.org/2002/07/owl#Thing"/>
            </owl:Restriction>
        </owl:equivalentClass>
        <rdfs:comment xml:lang="it">Classifica le pratiche di adeguamento contributivo in stato di Notificato Importo che sono legate ad un piano di ammortamento e come tali prevedono la possibilità di attivare un mandato SDD per il pagamento delle rate.</rdfs:comment>
        <rdfs:comment xml:lang="en">Classifies the tax adjustment applications in Notified Amount status which are linked to an amortization plan and as such provide for the possibility of activating an SDD mandate for the payment of installments.</rdfs:comment>
        <rdfs:label xml:lang="en">Contribution Adjustment Application by Installments</rdfs:label>
        <rdfs:label xml:lang="it">Pratica Di Adeguamento Rateizzata</rdfs:label>
    </owl:Class>



    <!-- https://w3id.org/italia/onto/OP21/PraticaDiRendita -->

    <owl:Class rdf:about="https://w3id.org/italia/onto/OP21/PraticaDiRendita">
        <rdfs:comment xml:lang="it">Particolare forma di riscatto che consente, previa esibizione di prove rigorose, di versare un onere a copertura dei periodi di lavoro la cui contribuzione sia stata omessa e che non sia più recuperabile. Presuppone quindi l’inadempimento dell’obbligo assicurativo per l’IVS che non deve essere più suscettibile di recupero da parte dell’INPS per maturata prescrizione. In tale contesto, l’INPS riconosce la rendita vitalizia solo nei casi di esistenza certa del rapporto di lavoro e di sussistenza dei requisiti prescritti dalla legge inerenti all’obbligo di versamento dei contributi nei periodi oggetto di riscatto. La domanda può in questo caso essere presentata: dal datore di lavoro che ha omesso il versamento dei contributi o dal lavoratore stesso, anche se già pensionato, o dai suoi superstiti. A fronte della presentazione della domanda, l&apos;INPS istruisce la relativa Pratica di Rendita per la valutazione dell&apos;accoglimento della richiesta e la determinazione degli oneri a carico del Richiedente.</rdfs:comment>
        <rdfs:comment xml:lang="en">The constitution of life annuities serves to rectify missing contributions for invalidity, old-age and survivors&apos; insurance that are time-barred and is therefore on the premise that the entity required to pay the contributions has failed to comply with a contribution obligation. The constitution of annuities or redeeming periods through buyback contributions may be claimed: by an employer that has failed to pay the contributions and in this way intends to pay said contributions by rectifying the damage caused to the employee; by the employee themselves, in lieu of the employer, either if they still working or if they have already been granted the pension; by survivors of the worker. On approval of the claim, the decision is sent to claimants by registered post and also specifies the payment methods and terms.</rdfs:comment>
        <rdfs:label xml:lang="en">Life Annuities Application</rdfs:label>
        <rdfs:label xml:lang="it">Pratica Di Rendita</rdfs:label>
    </owl:Class>



    <!-- https://w3id.org/italia/onto/OP21/PraticaDiRicongiunzione -->

    <owl:Class rdf:about="https://w3id.org/italia/onto/OP21/PraticaDiRicongiunzione">
        <rdfs:comment xml:lang="it">Istituto che consente, a chi ha posizioni assicurative in gestioni previdenziali diverse, di riunire, mediante trasferimento, tutti i periodi contributivi presso un’unica gestione, allo scopo di ottenere una sola pensione. Tale ricongiunzione avviene a domanda dell’assicurato o dei suoi superstiti e deve riguardare tutti i periodi di contribuzione che il lavoratore ha maturato in almeno due diverse forme previdenziali fino al momento della richiesta e che non siano già stati utilizzati per liquidare una pensione. I periodi così ricongiunti sono utilizzabili come se fossero stati versati nel fondo di destinazione e danno diritto ad un trattamento pensionistico basato sui requisiti di quest’ultimo fondo. A fronte della presentazione della domanda, l&apos;INPS istruisce la relativa Pratica di Ricongiunzione per la valutazione dell&apos;accoglimento della richiesta e la determinazione di eventuali oneri a carico del Richiedente.</rdfs:comment>
        <rdfs:comment xml:lang="en">The aggregation of insurance periods allows the transfer of existing contributions from at multiple institutes to a single institute in order to obtain a unified pension. The aggregation of insurance periods can be carried out free of charge or for payment.</rdfs:comment>
        <rdfs:label xml:lang="en">Aggregation Application</rdfs:label>
        <rdfs:label xml:lang="it">Pratica Di Ricongiunzione</rdfs:label>
    </owl:Class>



    <!-- https://w3id.org/italia/onto/OP21/PraticaDiRiscatto -->

    <owl:Class rdf:about="https://w3id.org/italia/onto/OP21/PraticaDiRiscatto">
        <rdfs:comment xml:lang="it">Istituto che consente al lavoratore, anche già pensionato, di conseguire, a proprie spese, il riconoscimento contributivo per specifici periodi altrimenti privi di contribuzione. Trattasi tipicamente di periodi in cui o non era previsto l’obbligo contributivo (ad esempio, gli anni di studio per il conseguimento della laurea o titolo di studio equiparato) o l’attività lavorativa si è svolta all’estero o vi è stata omissione rispetto all’obbligo di pagamento dei contributi spettanti. Il riscatto resta una facoltà a discrezione del lavoratore/pensionato (o dei superstiti in caso di decesso), che deve quindi farne espressa domanda all’INPS. Temporalmente, i contributi riscattati si collocheranno nello stesso periodo nel quale avrebbero dovuto essere versati. A fronte della presentazione della domanda, l&apos;INPS istruisce la relativa Pratica di Riscatto per la valutazione dell&apos;accoglimento della richiesta e la determinazione degli oneri a carico del Richiedente.</rdfs:comment>
        <rdfs:comment xml:lang="en">Redemption applications for pension purposes can be carried out in order to consider for pension purposes periods such as graduation years, years of employment abroad, periods non covered by contributions, periods of missing and time-barred contributions, and some periods expressly envisaged by the law and not covered by contribution </rdfs:comment>
        <rdfs:label xml:lang="it">Pratica Di Riscatto</rdfs:label>
        <rdfs:label xml:lang="en">Redemption Application</rdfs:label>
    </owl:Class>



    <!-- https://w3id.org/italia/onto/OP21/PrenotazioneDiPagamento -->

    <owl:Class rdf:about="https://w3id.org/italia/onto/OP21/PrenotazioneDiPagamento">
        <owl:equivalentClass>
            <owl:Restriction>
                <owl:onProperty>
                    <rdf:Description>
                        <owl:inverseOf rdf:resource="https://w3id.org/italia/onto/OP21/prenotaPagamento"/>
                    </rdf:Description>
                </owl:onProperty>
                <owl:someValuesFrom rdf:resource="http://www.w3.org/2002/07/owl#Thing"/>
            </owl:Restriction>
        </owl:equivalentClass>
        <owl:equivalentClass>
            <owl:Restriction>
                <owl:onProperty rdf:resource="https://w3id.org/italia/onto/OP21/dataDiPrenotazione"/>
                <owl:someValuesFrom rdf:resource="http://www.w3.org/2000/01/rdf-schema#Literal"/>
            </owl:Restriction>
        </owl:equivalentClass>
        <owl:equivalentClass>
            <owl:Restriction>
                <owl:onProperty rdf:resource="https://w3id.org/italia/onto/OP21/identificatorePrenotazionePagamento"/>
                <owl:someValuesFrom rdf:resource="http://www.w3.org/2000/01/rdf-schema#Literal"/>
            </owl:Restriction>
        </owl:equivalentClass>
        <owl:equivalentClass>
            <owl:Restriction>
                <owl:onProperty rdf:resource="https://w3id.org/italia/onto/OP21/importoPrenotato"/>
                <owl:someValuesFrom rdf:resource="http://www.w3.org/2000/01/rdf-schema#Literal"/>
            </owl:Restriction>
        </owl:equivalentClass>
        <rdfs:comment xml:lang="it">Esprime l&apos;impegno ad eseguire un Ordine Di Pagamento. Tale impegno può essere espresso da un Sistema di Pagamento Elettronico nell&apos;ambito di una Sessione di Pagamento, certificando così l&apos;avvenuta presa in carico del pagamento da parte del PSP scelto dal Pagatore, salvo buon fine, oppure da parte di un Istituto Di Credito che ha ricevuto un Mandato SDD o, nel passato, un RID. È caratterizzato da un identificativo, una data di prenotazione e dall&apos;importo del pagamento prenotato.</rdfs:comment>
        <rdfs:comment xml:lang="en">Expresses the commitment to execute a Payment Order. This commitment can be expressed by an Electronic Payment System within a Payment Session, thus certifying that the payment has been taken over by the PSP chosen by the Payer, subject to collection, or by a Credit Institution who has received an SDD Mandate or, in the past, a RID. It is characterized by an identifier, a reservation date and the reserved payment amount.</rdfs:comment>
        <rdfs:label xml:lang="en">Payment Reservation</rdfs:label>
        <rdfs:label xml:lang="it">Prenotazione Di Pagamento</rdfs:label>
    </owl:Class>



    <!-- https://w3id.org/italia/onto/OP21/PrestatoreDiServiziDiPagamento -->

    <owl:Class rdf:about="https://w3id.org/italia/onto/OP21/PrestatoreDiServiziDiPagamento">
        <rdfs:comment xml:lang="en">A Payment Service Provider offer online services to organizations and operators to accept electronic payments through different payment modes, such as credit cart, direct bank or postal account charge, or deferred or real time wire transfer.</rdfs:comment>
        <rdfs:comment xml:lang="it">Un Prestatore di Servizi di Pagamento (PSP) offre servizi di pagamento online ad Enti ed esercenti per accettare pagamenti elettronici con diversi metodi di pagamento, tra cui carta di credito, addebito diretto su conto corrente bancario o postale, trasferimento bancario differito o in tempo reale. L’opportunità di utilizzare un PSP permette di offrire ai propri clienti/utenti diversi canali di pagamento senza l’onere di dover stipulare contratti ad-hoc con i singoli sistemi di pagamento potendo inoltre contare su costi più bassi perché legati a maggiori volumi complessivi. Sono PSP, tra gli altri: banche, Poste Italiane, istituti di moneta elettronica e istituti di pagamento.</rdfs:comment>
        <rdfs:label xml:lang="en">Payment Service Provider</rdfs:label>
        <rdfs:label xml:lang="it">Prestatore Di Servizi Di Pagamento</rdfs:label>
    </owl:Class>



    <!-- https://w3id.org/italia/onto/OP21/RID -->

    <owl:Class rdf:about="https://w3id.org/italia/onto/OP21/RID">
        <owl:equivalentClass>
            <owl:Restriction>
                <owl:onProperty rdf:resource="https://w3id.org/italia/onto/OP21/codiceRID"/>
                <owl:someValuesFrom rdf:resource="http://www.w3.org/2000/01/rdf-schema#Literal"/>
            </owl:Restriction>
        </owl:equivalentClass>
        <rdfs:comment xml:lang="en">An arrangement made with a bank that allows a third party to transfer money from a person&apos;s account on agreed dates, typically in order to pay bills.</rdfs:comment>
        <rdfs:comment xml:lang="it">Il RID, Rapporto Interbancario Diretto, è un servizio di incasso crediti che prevede che il titolare di un conto corrente conferisca alla propria banca un’autorizzazione continuativa ad accettare gli ordini di addebito provenienti da un determinato creditore. Dal 1 febbraio 2014, per effetto del regolamento UE 260/2012, il RID è stato integralmente sostituito dall’analogo servizio Sepa Direct Debit (SDD).</rdfs:comment>
        <rdfs:label xml:lang="it">RID</rdfs:label>
        <rdfs:label xml:lang="en">RID (direct banking)</rdfs:label>
    </owl:Class>



    <!-- https://w3id.org/italia/onto/OP21/RapportoDiLavoroDomestico -->

    <owl:Class rdf:about="https://w3id.org/italia/onto/OP21/RapportoDiLavoroDomestico">
        <owl:equivalentClass>
            <owl:Class>
                <owl:unionOf rdf:parseType="Collection">
                    <rdf:Description rdf:about="https://w3id.org/italia/onto/OP21/RapportoDiLavoroDomesticoAttivo"/>
                    <rdf:Description rdf:about="https://w3id.org/italia/onto/OP21/RapportoDiLavoroDomesticoCessato"/>
                </owl:unionOf>
            </owl:Class>
        </owl:equivalentClass>
        <owl:equivalentClass>
            <owl:Restriction>
                <owl:onProperty rdf:resource="https://w3id.org/italia/onto/OP21/haDatoreDiLavoro"/>
                <owl:someValuesFrom rdf:resource="http://www.w3.org/2002/07/owl#Thing"/>
            </owl:Restriction>
        </owl:equivalentClass>
        <owl:equivalentClass>
            <owl:Restriction>
                <owl:onProperty rdf:resource="https://w3id.org/italia/onto/OP21/haLavoratoreDomestico"/>
                <owl:someValuesFrom rdf:resource="http://www.w3.org/2002/07/owl#Thing"/>
            </owl:Restriction>
        </owl:equivalentClass>
        <owl:equivalentClass>
            <owl:Restriction>
                <owl:onProperty rdf:resource="https://w3id.org/italia/onto/OP21/èOriginatoDa"/>
                <owl:someValuesFrom rdf:resource="http://www.w3.org/2002/07/owl#Thing"/>
            </owl:Restriction>
        </owl:equivalentClass>
        <owl:equivalentClass>
            <owl:Restriction>
                <owl:onProperty rdf:resource="https://w3id.org/italia/onto/OP21/codiceRapportoDiLavoro"/>
                <owl:someValuesFrom rdf:resource="http://www.w3.org/2000/01/rdf-schema#Literal"/>
            </owl:Restriction>
        </owl:equivalentClass>
        <owl:equivalentClass>
            <owl:Restriction>
                <owl:onProperty rdf:resource="https://w3id.org/italia/onto/OP21/dataDepositoContratto"/>
                <owl:someValuesFrom rdf:resource="http://www.w3.org/2000/01/rdf-schema#Literal"/>
            </owl:Restriction>
        </owl:equivalentClass>
        <rdfs:comment xml:lang="en">Employment relationship between an employer and a subordinate worker who provides services of a domestic nature aimed at the functioning of family life. The employer is obliged to notify INPS of the establishment of this employment relationship, before the date of employment, as well as any change to the terms of the relationship itself or its termination. By virtue of this communication, the employment relationship is assigned by INPS an identification code useful for any subsequent fulfillment relating to the relationship itself. The contract can change over time, therefore each instance is associated with a validity interval (subclass of TI:TimeIndexedEvent).</rdfs:comment>
        <rdfs:comment xml:lang="it">Rapporto di lavoro tra un datore di lavoro e un lavoratore subordinato che presta servizi di carattere domestico diretti al funzionamento della vita familiare. È fatto obbligo al datore di lavoro di comunicare all’INPS l’istaurarsi di tale rapporto di lavoro, prima della data di assunzione, così come qualsiasi modifica dei termini del rapporto stesso ovvero la sua cessazione. In virtù di tale comunicazione, al rapporto di lavoro viene assegnato da INPS un codice identificativo utile per qualsiasi successivo adempimento inerente al rapporto stesso. Il contratto può modificarsi nel tempo quindi a ciascuna istanza è associato un intervallo di validità (sottoclasse di TI:TimeIndexedEvent).</rdfs:comment>
        <rdfs:label xml:lang="en">Domestic Employment Relationship</rdfs:label>
        <rdfs:label xml:lang="it">Rapporto Di Lavoro Domestico</rdfs:label>
    </owl:Class>



    <!-- https://w3id.org/italia/onto/OP21/RapportoDiLavoroDomesticoAttivo -->

    <owl:Class rdf:about="https://w3id.org/italia/onto/OP21/RapportoDiLavoroDomesticoAttivo">
        <owl:equivalentClass>
            <owl:Restriction>
                <owl:onProperty rdf:resource="https://w3id.org/italia/onto/OP21/depositoAvvioRapporto"/>
                <owl:someValuesFrom rdf:resource="http://www.w3.org/2002/07/owl#Thing"/>
            </owl:Restriction>
        </owl:equivalentClass>
        <owl:equivalentClass>
            <owl:Restriction>
                <owl:onProperty rdf:resource="https://w3id.org/italia/onto/OP21/dataInizioRapporto"/>
                <owl:someValuesFrom rdf:resource="http://www.w3.org/2000/01/rdf-schema#Literal"/>
            </owl:Restriction>
        </owl:equivalentClass>
        <owl:disjointWith rdf:resource="https://w3id.org/italia/onto/OP21/RapportoDiLavoroDomesticoCessato"/>
        <rdfs:comment xml:lang="it">Sottoclasse di Rapporto di Lavoro Domestico che classifica i rapporti attualmente attivi. È caratterizzato dalla data di inizio del rapporto.</rdfs:comment>
        <rdfs:comment xml:lang="en">Subclass of Domestic Employment Relationship that classifies currently active relationships. It has a relationship start date.</rdfs:comment>
        <rdfs:label xml:lang="en">Active Domestic Employment Relationship</rdfs:label>
        <rdfs:label xml:lang="it">Rapporto Di Lavoro Domestico Attivo</rdfs:label>
    </owl:Class>



    <!-- https://w3id.org/italia/onto/OP21/RapportoDiLavoroDomesticoCessato -->

    <owl:Class rdf:about="https://w3id.org/italia/onto/OP21/RapportoDiLavoroDomesticoCessato">
        <owl:equivalentClass>
            <owl:Restriction>
                <owl:onProperty rdf:resource="https://w3id.org/italia/onto/OP21/depositoCessazioneRapporto"/>
                <owl:someValuesFrom rdf:resource="http://www.w3.org/2002/07/owl#Thing"/>
            </owl:Restriction>
        </owl:equivalentClass>
        <owl:equivalentClass>
            <owl:Restriction>
                <owl:onProperty rdf:resource="https://w3id.org/italia/onto/OP21/dataFineRapporto"/>
                <owl:someValuesFrom rdf:resource="http://www.w3.org/2000/01/rdf-schema#Literal"/>
            </owl:Restriction>
        </owl:equivalentClass>
        <rdfs:comment xml:lang="it">Sottoclasse di Rapporto di Lavoro Domestico che classifica i rapporti non più attivi. È caratterizzato dalla data di fine del rapporto.</rdfs:comment>
        <rdfs:comment xml:lang="en">Subclass of Domestic Employment Relationship that classifies currently inactive relationships. It has a relationship end date.</rdfs:comment>
        <rdfs:label xml:lang="it">Rapporto Di Lavoro Domestico Cessato</rdfs:label>
        <rdfs:label xml:lang="en">Terminated Domestic Employment Relationship</rdfs:label>
    </owl:Class>



    <!-- https://w3id.org/italia/onto/OP21/RataDiOnereContributivo -->

    <owl:Class rdf:about="https://w3id.org/italia/onto/OP21/RataDiOnereContributivo">
        <owl:equivalentClass>
            <owl:Restriction>
                <owl:onProperty>
                    <rdf:Description>
                        <owl:inverseOf rdf:resource="https://w3id.org/italia/onto/OP21/haRata"/>
                    </rdf:Description>
                </owl:onProperty>
                <owl:someValuesFrom rdf:resource="http://www.w3.org/2002/07/owl#Thing"/>
            </owl:Restriction>
        </owl:equivalentClass>
        <owl:equivalentClass>
            <owl:Restriction>
                <owl:onProperty rdf:resource="https://w3id.org/italia/onto/OP21/dataScadenzaRata"/>
                <owl:someValuesFrom rdf:resource="http://www.w3.org/2000/01/rdf-schema#Literal"/>
            </owl:Restriction>
        </owl:equivalentClass>
        <owl:equivalentClass>
            <owl:Restriction>
                <owl:onProperty rdf:resource="https://w3id.org/italia/onto/OP21/numeroRata"/>
                <owl:someValuesFrom rdf:resource="http://www.w3.org/2000/01/rdf-schema#Literal"/>
            </owl:Restriction>
        </owl:equivalentClass>
        <rdfs:comment xml:lang="it">Classifica le rate di un piano di ammortamento, ciascuna legata al rispettivo piano e alla rata successiva dello stesso piano. Ciascuna istanza è caratterizzata dall&apos;indice della rata, relativamente al piano di cui fa parte, e dalla sua data di scadenza. È sottoclasse di Finalità risultando in tal modo legata alla classe Bollettino Di Pagamento a cui fornisce i dati per la compilazione dello stesso.</rdfs:comment>
        <rdfs:comment xml:lang="en">Classifies the installments of an amortization plan, each linked to the respective plan and to the next installment of the same plan. Each application is characterized by the index of the installment, relative to the plan to which it belongs, and by its expiry date. It is a subclass of Purpose, thus resulting linked to the Payment Slip class to which it provides the data for its compilation.</rdfs:comment>
        <rdfs:label xml:lang="en">Contributory Charge Installment</rdfs:label>
        <rdfs:label xml:lang="it">Rata Di Onere Contributivo</rdfs:label>
    </owl:Class>



    <!-- https://w3id.org/italia/onto/OP21/RetiAmiche -->

    <owl:Class rdf:about="https://w3id.org/italia/onto/OP21/RetiAmiche">
        <rdfs:comment xml:lang="it">Il servizio Reti Amiche, istituito nel 2009, permette ai cittadini di ritirare la pensione, prelevare cifre, anche di modesta entità, versare contributi INPS per colf e badanti, o pagare bollette di terzi cui sono affidati incarichi di lavoro, presso tabaccherie italiane. Il sistema di pagamento online tramite la convenzione Reti Amiche è stato disattivato dal 13/02/2021 per Lottomatica, e per Unicredit, Poste Italiane e SisalPAY dal 28/02/2021. Reti Amiche è stato sostituito dal sistema PagoPA.</rdfs:comment>
        <rdfs:comment xml:lang="en">The Reti Amiche service, established in 2009, allows citizens to withdraw their pension, withdraw even modest amounts, pay INPS contributions for domestic workers and carers, or pay bills for third parties entrusted with work assignments, at Italian tobacconists. The online payment system through the Reti Amiche convention was deactivated from 02/13/2021 for Lottomatica, and for Unicredit, Poste Italiane and SisalPAY from 02/28/2021. Reti Amiche has been replaced by the PagoPA system.</rdfs:comment>
        <rdfs:label xml:lang="en">Reti Amiche</rdfs:label>
        <rdfs:label xml:lang="it">Reti Amiche</rdfs:label>
    </owl:Class>



    <!-- https://w3id.org/italia/onto/OP21/RicevutaDiMovimento -->

    <owl:Class rdf:about="https://w3id.org/italia/onto/OP21/RicevutaDiMovimento">
        <owl:equivalentClass>
            <owl:Restriction>
                <owl:onProperty>
                    <rdf:Description>
                        <owl:inverseOf rdf:resource="https://w3id.org/italia/onto/OP21/inviaRicevutaDiMovimento"/>
                    </rdf:Description>
                </owl:onProperty>
                <owl:someValuesFrom rdf:resource="http://www.w3.org/2002/07/owl#Thing"/>
            </owl:Restriction>
        </owl:equivalentClass>
        <owl:equivalentClass>
            <owl:Restriction>
                <owl:onProperty rdf:resource="https://w3id.org/italia/onto/OP21/dataRicevuta"/>
                <owl:someValuesFrom rdf:resource="http://www.w3.org/2000/01/rdf-schema#Literal"/>
            </owl:Restriction>
        </owl:equivalentClass>
        <owl:equivalentClass>
            <owl:Restriction>
                <owl:onProperty rdf:resource="https://w3id.org/italia/onto/OP21/identificatoreRicevuta"/>
                <owl:someValuesFrom rdf:resource="http://www.w3.org/2000/01/rdf-schema#Literal"/>
            </owl:Restriction>
        </owl:equivalentClass>
        <rdfs:comment xml:lang="en">Attestation addressed to the Creditor Institution of the crediting of a sum of money determined by a Money Movement induced by a Payment Order. It is characterized by an identifier equivalent to the movement of which it is received and a date.</rdfs:comment>
        <rdfs:comment xml:lang="it">Attestazione rivolta all&apos;Ente Creditore dell&apos;avvenuto movimento di accredito di una somma di denaro determinata da un Movimento Di Denaro indotto da un Ordine Di Pagamento. È caratterizzata da un identificativo equivalente a quello del movimento di cui è ricevuta e una data.</rdfs:comment>
        <rdfs:label xml:lang="en">Movement Receipt</rdfs:label>
        <rdfs:label xml:lang="it">Ricevuta Di Movimento</rdfs:label>
    </owl:Class>



    <!-- https://w3id.org/italia/onto/OP21/RichiedenteAdeguamentoContributivo -->

    <owl:Class rdf:about="https://w3id.org/italia/onto/OP21/RichiedenteAdeguamentoContributivo">
        <owl:equivalentClass>
            <owl:Restriction>
                <owl:onProperty rdf:resource="https://w3id.org/italia/onto/OP21/presentaDomandaAdeguamentoContributivo"/>
                <owl:someValuesFrom rdf:resource="http://www.w3.org/2002/07/owl#Thing"/>
            </owl:Restriction>
        </owl:equivalentClass>
        <owl:equivalentClass>
            <owl:Restriction>
                <owl:onProperty rdf:resource="https://w3id.org/italia/onto/OP21/identificatoreRichiedenteAdeguamentoContributivo"/>
                <owl:someValuesFrom rdf:resource="http://www.w3.org/2000/01/rdf-schema#Literal"/>
            </owl:Restriction>
        </owl:equivalentClass>
        <rdfs:comment xml:lang="it">Sottoclasse di Ruolo Di Persona Viva che classifica le persone in vita che presentano una domanda di adeguamento contributivo (per riscatto, ricongiunzione o rendita) per se stessi o per una persona deceduta essendone un superstite, parente o affine. In questo secondo caso, il Richiedente presenta la domanda per conto e in vece dell&apos;avente diritto, assumendosi il compito di versare gli eventuali oneri derivanti. La platea di persone fisiche che possono ricoprire il ruolo di Richiedente è piuttosto ampia comprendendo i lavoratori, dipendenti e autonomi, così come i lavoratori già pensionati. Ciascuna istanza del ruolo è caratterizzata da un identificativo.</rdfs:comment>
        <rdfs:comment xml:lang="en">Subclass of Role of Living Person which classifies living people who submit an application for tax contribution adjustment (for redemption, reunion or income) for themselves or for a deceased person of which they are a survivor, relative or similar. In this second case, the Applicant submits the application on behalf of and in place of the person, taking responsability for the task of paying any resulting charges. The variety of natural persons who can fill the role of Applicant is quite broad, including workers, employees and self-employed, as well as workers who have already retired. Each instance of such roles is characterized by an identifier.</rdfs:comment>
        <rdfs:label xml:lang="it">Richiedente Adeguamento Contributivo</rdfs:label>
        <rdfs:label xml:lang="en">Tax Adjustment Applicant</rdfs:label>
    </owl:Class>



    <!-- https://w3id.org/italia/onto/OP21/RuoloDiAgente -->

    <owl:Class rdf:about="https://w3id.org/italia/onto/OP21/RuoloDiAgente">
        <owl:equivalentClass>
            <owl:Restriction>
                <owl:onProperty>
                    <rdf:Description>
                        <owl:inverseOf rdf:resource="https://w3id.org/italia/onto/RO/holdsRoleInTime"/>
                    </rdf:Description>
                </owl:onProperty>
                <owl:someValuesFrom>
                    <owl:Class>
                        <owl:unionOf rdf:parseType="Collection">
                            <rdf:Description rdf:about="https://w3id.org/italia/onto/COV/Organization"/>
                            <rdf:Description rdf:about="https://w3id.org/italia/onto/CPV/Person"/>
                        </owl:unionOf>
                    </owl:Class>
                </owl:someValuesFrom>
            </owl:Restriction>
        </owl:equivalentClass>
        <rdfs:comment xml:lang="it">Insieme di mansioni, compiti, responsabilità e doveri attribuiti in un intervallo di tempo, anche non ancora terminato, a una persona o a una organizzazione considerando queste ultime specializzazioni di agente. </rdfs:comment>
        <rdfs:comment xml:lang="en">Set of tasks, duties and responsabilities attributed in a certain time interval, possible not yet determined, to a person or organization, considering these as specializations of an agent. </rdfs:comment>
        <rdfs:label xml:lang="en">Agent Role</rdfs:label>
        <rdfs:label xml:lang="it">Ruolo Di Agente</rdfs:label>
    </owl:Class>



    <!-- https://w3id.org/italia/onto/OP21/RuoloDiPersona -->

    <owl:Class rdf:about="https://w3id.org/italia/onto/OP21/RuoloDiPersona">
        <owl:equivalentClass>
            <owl:Restriction>
                <owl:onProperty>
                    <rdf:Description>
                        <owl:inverseOf rdf:resource="https://w3id.org/italia/onto/RO/holdsRoleInTime"/>
                    </rdf:Description>
                </owl:onProperty>
                <owl:someValuesFrom rdf:resource="https://w3id.org/italia/onto/CPV/Person"/>
            </owl:Restriction>
        </owl:equivalentClass>
        <rdfs:subClassOf rdf:resource="https://w3id.org/italia/onto/OP21/RuoloDiAgente"/>
        <rdfs:comment xml:lang="it">Specializzazione della classe Ruolo Di Agente limitata alle sole persone, in vita o decedute.</rdfs:comment>
        <rdfs:comment xml:lang="en">Subclass of the Agent Role class, limited to people, living or deceased.</rdfs:comment>
        <rdfs:label xml:lang="en">Person Role</rdfs:label>
        <rdfs:label xml:lang="it">Ruolo Di Persona</rdfs:label>
    </owl:Class>



    <!-- https://w3id.org/italia/onto/OP21/RuoloDiPersonaViva -->

    <owl:Class rdf:about="https://w3id.org/italia/onto/OP21/RuoloDiPersonaViva">
        <owl:equivalentClass>
            <owl:Restriction>
                <owl:onProperty>
                    <rdf:Description>
                        <owl:inverseOf rdf:resource="https://w3id.org/italia/onto/RO/holdsRoleInTime"/>
                    </rdf:Description>
                </owl:onProperty>
                <owl:someValuesFrom rdf:resource="https://w3id.org/italia/onto/CPV/Alive"/>
            </owl:Restriction>
        </owl:equivalentClass>
        <rdfs:subClassOf rdf:resource="https://w3id.org/italia/onto/OP21/RuoloDiPersona"/>
        <rdfs:comment xml:lang="it">Specializzazione della classe Ruolo Di Persona limitata alle sole persone in vita.</rdfs:comment>
        <rdfs:comment xml:lang="en">Subclass of the Person Role class, limited to only alive persons.</rdfs:comment>
        <rdfs:label xml:lang="en">Alive Person Role</rdfs:label>
        <rdfs:label xml:lang="it">Ruolo Di Persona Viva</rdfs:label>
    </owl:Class>



    <!-- https://w3id.org/italia/onto/OP21/SedeINPS -->

    <owl:Class rdf:about="https://w3id.org/italia/onto/OP21/SedeINPS">
        <owl:equivalentClass>
            <owl:Restriction>
                <owl:onProperty rdf:resource="https://w3id.org/italia/onto/COV/hasOrganizzation"/>
                <owl:someValuesFrom rdf:resource="http://www.w3.org/2002/07/owl#Thing"/>
            </owl:Restriction>
        </owl:equivalentClass>
        <owl:equivalentClass>
            <owl:Restriction>
                <owl:onProperty rdf:resource="https://w3id.org/italia/onto/OP21/codiceSedeINPS"/>
                <owl:someValuesFrom rdf:resource="http://www.w3.org/2000/01/rdf-schema#Literal"/>
            </owl:Restriction>
        </owl:equivalentClass>
        <rdfs:subClassOf rdf:resource="https://w3id.org/italia/onto/COV/HomogeneousOrganizationalArea"/>
        <rdfs:comment xml:lang="en">INPS is divided into central, regional and metropolitan structures with guidance, monitoring and coordination tasks, and into territorial offices with operational and user contact functions. In particular, the Institute, throughout the Italian national territory, has set up a &quot;service network&quot; organization which, in a &quot;proximity&quot; logic, is divided into: metropolitan coordination structures, provincial level structures, regional structures. Each INPS office is similar to a Homogeneous Organizational Area (AOO), each benefiting from a single entry and/or exit document flow (IT Protocol service) for the provision of services and the receipt of requests. In this sense, each INPS office is assigned, in addition to an office code assigned by the Institute, also a unique AOO identification code within the Index of Public Administrations (IPA) which makes it possible to identify the telematic communication channels legally permitted that is, at least one certified mailbox for each AOO. The competent INPS office for a citizen and/or company is established on the basis of the citizen&apos;s residence and/or the address of the company headquarters.</rdfs:comment>
        <rdfs:comment xml:lang="it">L’INPS è articolato in strutture centrali, regionali e metropolitane con compiti di indirizzo, monitoraggio e coordinamento, e in sedi territoriali con funzioni operative e di contatto con l’utenza. In particolare, l’Istituto, su tutto il territorio nazionale italiano, si è dotato di un’organizzazione “a reti di servizio” che, in logica di “prossimità”, si suddivide in: strutture di coordinamento metropolitano, strutture a livello provinciale, strutture a livello regionale. Ogni sede INPS è assimilabile ad un Area Organizzativa Omogenea (AOO) usufruendo ciascuna per l&apos;erogazione di servizi e il ricevimento delle richieste, di un unico flusso documentale di entrata e/o uscita (servizio di Protocollo Informatico). In tal senso ad ogni Sede INPS è assegnato, oltre ad un codice di sede attribuito dall&apos;Istituto, anche un codice identificativo AOO univoco nell&apos;ambito dell&apos;Indice delle Pubbliche Amministrazioni (IPA) che permette di individuare i canali di comunicazione telematica normativamente pervisti e cioè almeno una casella di posta elettronica certificata per ciascun AOO. La sede INPS competente per un cittadino e/o un&apos;impresa è stabilita in base alla residenza del cittadino e/o all&apos;indirizzo della sede dell&apos;impresa.</rdfs:comment>
        <rdfs:label xml:lang="en">INPS Office</rdfs:label>
        <rdfs:label xml:lang="it">Sede INPS</rdfs:label>
    </owl:Class>



    <!-- https://w3id.org/italia/onto/OP21/ServizioDiPagamento -->

    <owl:Class rdf:about="https://w3id.org/italia/onto/OP21/ServizioDiPagamento">
        <owl:equivalentClass>
            <owl:Restriction>
                <owl:onProperty>
                    <rdf:Description>
                        <owl:inverseOf rdf:resource="https://w3id.org/italia/onto/OP21/haServizioDiPagamento"/>
                    </rdf:Description>
                </owl:onProperty>
                <owl:someValuesFrom rdf:resource="http://www.w3.org/2002/07/owl#Thing"/>
            </owl:Restriction>
        </owl:equivalentClass>
        <owl:equivalentClass>
            <owl:Restriction>
                <owl:onProperty rdf:resource="https://w3id.org/italia/onto/OP21/codiceServizioDiPagamento"/>
                <owl:someValuesFrom rdf:resource="http://www.w3.org/2000/01/rdf-schema#Literal"/>
            </owl:Restriction>
        </owl:equivalentClass>
        <rdfs:comment xml:lang="en">Payment service offered by a Payment Service Provider. Each service is identified by a code.</rdfs:comment>
        <rdfs:comment xml:lang="it">Servizio di pagamento offerto da un Prestatore Di Servizi Di Pagamento. Ciascun servizio è identificato da un codice.</rdfs:comment>
        <rdfs:label xml:lang="en">Payment Service</rdfs:label>
        <rdfs:label xml:lang="it">Servizio Di Pagamento</rdfs:label>
    </owl:Class>



    <!-- https://w3id.org/italia/onto/OP21/SessionePagamentoElettronico -->

    <owl:Class rdf:about="https://w3id.org/italia/onto/OP21/SessionePagamentoElettronico">
        <owl:equivalentClass>
            <owl:Restriction>
                <owl:onProperty rdf:resource="https://w3id.org/italia/onto/OP21/haSistemaDiPagamentoElettronico"/>
                <owl:someValuesFrom rdf:resource="http://www.w3.org/2002/07/owl#Thing"/>
            </owl:Restriction>
        </owl:equivalentClass>
        <owl:equivalentClass>
            <owl:Restriction>
                <owl:onProperty>
                    <rdf:Description>
                        <owl:inverseOf rdf:resource="https://w3id.org/italia/onto/OP21/accedeServizioDiPagamento"/>
                    </rdf:Description>
                </owl:onProperty>
                <owl:someValuesFrom rdf:resource="http://www.w3.org/2002/07/owl#Thing"/>
            </owl:Restriction>
        </owl:equivalentClass>
        <owl:equivalentClass>
            <owl:Restriction>
                <owl:onProperty rdf:resource="https://w3id.org/italia/onto/OP21/identificatoreSessionePagamento"/>
                <owl:someValuesFrom rdf:resource="http://www.w3.org/2000/01/rdf-schema#Literal"/>
            </owl:Restriction>
        </owl:equivalentClass>
        <rdfs:comment xml:lang="it">Classifica l&apos;intervallo di tempo entro cui sono svolte le attività utili all&apos;esecuzione di un pagamento da parte di un Pagatore nell&apos;ambito di un Sistema Di Pagamento Elettronico, includendo l&apos;attività di autenticazione e connessione al sistema stesso. È sottoclasse di TI:TimeIndexedEvent e ciascuna istanza ha un identificatore. L&apos;accesso al Sistema Di Pagamento Elettronico può essere instradato da un ulteriore ambiente di interazione che propone il suddetto sistema come Modalità Di Pagamento.</rdfs:comment>
        <rdfs:comment xml:lang="en">Classifies the time interval within which the activities useful for the execution of a payment by a Payer within an Electronic Payment System are carried out, including authentication and connection to the system itself. It is subclass of TI:TimeIndexedEvent and each instance has an identifier. Access to the Electronic Payment System can be routed from a further interaction environment that offers the aforementioned system as a Payment Method.</rdfs:comment>
        <rdfs:label xml:lang="en">Electronic Payment Session</rdfs:label>
        <rdfs:label xml:lang="it">Sessione Pagamento Elettronico</rdfs:label>
    </owl:Class>



    <!-- https://w3id.org/italia/onto/OP21/SettimanaDelMese -->

    <owl:Class rdf:about="https://w3id.org/italia/onto/OP21/SettimanaDelMese">
        <owl:equivalentClass>
            <owl:Restriction>
                <owl:onProperty rdf:resource="https://w3id.org/italia/onto/OP21/èSettimanaDelMese"/>
                <owl:someValuesFrom rdf:resource="http://www.w3.org/2002/07/owl#Thing"/>
            </owl:Restriction>
        </owl:equivalentClass>
        <owl:equivalentClass>
            <owl:Restriction>
                <owl:onProperty rdf:resource="https://w3id.org/italia/onto/OP21/indiceSettimana"/>
                <owl:someValuesFrom rdf:resource="http://www.w3.org/2000/01/rdf-schema#Literal"/>
            </owl:Restriction>
        </owl:equivalentClass>
        <rdfs:comment xml:lang="en">Index of the week in a calendar month. Practically, it assumes instances 1 to 5 (subclass of TI:TemporalEntity).</rdfs:comment>
        <rdfs:comment xml:lang="it">Indice della settimana in un mese solare. In pratica assume istanze da 1 a 5 (sottoclasse di TI:TemporalEntity).</rdfs:comment>
        <rdfs:label xml:lang="it">Settimana Del Mese</rdfs:label>
        <rdfs:label xml:lang="en">Week Of The Month</rdfs:label>
    </owl:Class>



    <!-- https://w3id.org/italia/onto/OP21/SistemaDiPagamentoElettronico -->

    <owl:Class rdf:about="https://w3id.org/italia/onto/OP21/SistemaDiPagamentoElettronico">
        <owl:equivalentClass>
            <owl:Class>
                <owl:unionOf rdf:parseType="Collection">
                    <rdf:Description rdf:about="https://w3id.org/italia/onto/OP21/SistemaDiPagamentoElettronicoAttivo"/>
                    <rdf:Description rdf:about="https://w3id.org/italia/onto/OP21/SistemaDiPagamentoElettronicoDisattivo"/>
                </owl:unionOf>
            </owl:Class>
        </owl:equivalentClass>
        <owl:equivalentClass>
            <owl:Restriction>
                <owl:onProperty rdf:resource="https://w3id.org/italia/onto/OP21/codiceSistemaDiPagamento"/>
                <owl:someValuesFrom rdf:resource="http://www.w3.org/2000/01/rdf-schema#Literal"/>
            </owl:Restriction>
        </owl:equivalentClass>
        <rdfs:comment xml:lang="en">An electronic payment system is a collection of specific tools and procedures that allow the virtual transfer of money without the physical passage of cash. The most widely used means of electronic payment is the payment card, which consists of a physical or digital medium, which contains the data of the holder and of the card itself, such as name and surname, the card number, the circuit to which the card adheres , the financial intermediary (bank, financial company or company operating in financial services) that issued it, the expiry date, etc. During the payment procedure, these data are read by the devices supplied by the person receiving the payment or, if the payment is made via the web, communicated by the payer through a specific page of the website dedicated to the payment and, if no anomalies are found, enable the transfer of the money, by the financial intermediary or the issuing company, from the cardholder to the creditor. The system then registers the amount, the date, the card details and the payment recipient. Among the other methods of electronic payment there is the electronic transfer which allows the transfer of money from your current account to that of the creditor through the home banking service. These systems include online payment platforms that act as telematic intermediaries between creditors and debtors, allowing the exchange of money between different Payment Service Providers (PSPs), each belonging to one of the parties to the transaction. Each system is identified by a specific identification code.</rdfs:comment>
        <rdfs:comment xml:lang="it">Un sistema di pagamento elettronico è una collezione di specifici strumenti e procedure che permettono il trasferimento virtuale di denaro senza che vi sia il passaggio fisico di contante. Il mezzo di pagamento elettronico maggiormente utilizzato è la carta di pagamento, che consiste in un supporto fisico o digitale, che riporta i dati del titolare e della carta stessa, quali nome e cognome, il numero della carta, il circuito al quale la carta aderisce, l’intermediario finanziario (banca, società finanziaria o società che opera nei servizi finanziari) che l’ha emessa, la data di scadenza, etc. Durante la procedura di pagamento, tali dati vengono letti dai dispositivi in dotazione presso chi riceve il pagamento o, se il pagamento è effettuato via web, comunicati dal pagatore tramite una specifica pagina del sito dedicato al pagamento e, qualora non si rilevino anomalie, abilitano il trasferimento del denaro, a cura dell’intermediario finanziario o della società emittente, dal titolare della carta al soggetto creditore. Il sistema provvede, poi, a registrare l’importo, la data, i dati della carta e del destinatario del pagamento. Tra le altre modalità di pagamento elettronico vi è Il bonifico elettronico che permette il trasferimento di denaro dal proprio conto corrente a quello del creditore attraverso il servizio di home banking. Rientrano tra questi sistemi le piattaforme di pagamento on-line che fungono da intermediari telematici tra creditori e debitori, permettendo lo scambio di denaro tra diversi Prestatori di Servizi di Pagamento (PSP) ciascuno facente capo ad una delle parti della transazione. Ciascun sistema è identificato da uno specifico codice identificativo.</rdfs:comment>
        <rdfs:label xml:lang="en">Electronic Payment System</rdfs:label>
        <rdfs:label xml:lang="it">Sistema Di Pagamento Elettronico</rdfs:label>
    </owl:Class>



    <!-- https://w3id.org/italia/onto/OP21/SistemaDiPagamentoElettronicoAttivo -->

    <owl:Class rdf:about="https://w3id.org/italia/onto/OP21/SistemaDiPagamentoElettronicoAttivo">
        <owl:disjointWith rdf:resource="https://w3id.org/italia/onto/OP21/SistemaDiPagamentoElettronicoDisattivo"/>
        <rdfs:comment xml:lang="en">An Active Electronic Payment System is an Electronic Payment System which is currently in use, meaning it can be adopted by citizens or organizations to make electronic payments.</rdfs:comment>
        <rdfs:comment xml:lang="it">Un Sistema di Pagamento Elettronico Attivo è un Sistema di Pagamento Elettronico attualmente in funzione, e quindi usufruibile per effettuare dei pagamenti.</rdfs:comment>
        <rdfs:label xml:lang="en">Active Electronic Payment System</rdfs:label>
        <rdfs:label xml:lang="it">Sistema Di Pagamento Elettronico Attivo</rdfs:label>
    </owl:Class>



    <!-- https://w3id.org/italia/onto/OP21/SistemaDiPagamentoElettronicoDisattivo -->

    <owl:Class rdf:about="https://w3id.org/italia/onto/OP21/SistemaDiPagamentoElettronicoDisattivo">
        <owl:equivalentClass>
            <owl:Class>
                <owl:unionOf rdf:parseType="Collection">
                    <rdf:Description rdf:about="https://w3id.org/italia/onto/OP21/POSVirtuale"/>
                    <rdf:Description rdf:about="https://w3id.org/italia/onto/OP21/RetiAmiche"/>
                </owl:unionOf>
            </owl:Class>
        </owl:equivalentClass>
        <rdfs:comment xml:lang="en">A Deactivated Electronic Payment System is an Electronic Payment System whose functionality is discontinued, and is therefore no longer usable by citizens or organizations to make electronic payments. The identity of such a system is maintained after its deactivation to characterize the payments made with this system in the past.</rdfs:comment>
        <rdfs:comment xml:lang="it">Un Sistema Di Pagamento Elettronico Disattivo è un Sistema Di Pagamento Elettronico la cui funzionalità è stata disattivata, ed è quindi non più usufruibile da cittadini o organizzazioni per effettuare pagamenti elettronici. L&apos;identità di un tale sistema viene mantenuta dopo la sua disattivazione per caratterizzare i pagamenti effettuati con tale sistema nel passato.</rdfs:comment>
        <rdfs:label xml:lang="en">Deactivated Electronic Payment System</rdfs:label>
        <rdfs:label xml:lang="it">Sistema Di Pagamento Elettronico Disattivo</rdfs:label>
    </owl:Class>



    <!-- https://w3id.org/italia/onto/OP21/StatoDiAccreditoParzialeDiPratica -->

    <owl:Class rdf:about="https://w3id.org/italia/onto/OP21/StatoDiAccreditoParzialeDiPratica">
        <rdfs:comment xml:lang="it">Sottoclasse di Pratica Adeguamento Contributivo che classifica le pratiche i cui oneri necessari per il loro perfezionamento economico sono stati versati in modo parziale.</rdfs:comment>
        <rdfs:comment xml:lang="en">Subclass of Tax Adjustment Application which classifies the applications whose costs necessary for their economic closure have been paid in part.</rdfs:comment>
        <rdfs:label xml:lang="en">Partial Credit of the Application Status</rdfs:label>
        <rdfs:label xml:lang="it">Stato Di Accredito Parziale Di Pratica</rdfs:label>
    </owl:Class>



    <!-- https://w3id.org/italia/onto/OP21/StatoDiNotificatoImportoDiPratica -->

    <owl:Class rdf:about="https://w3id.org/italia/onto/OP21/StatoDiNotificatoImportoDiPratica">
        <owl:equivalentClass>
            <owl:Restriction>
                <owl:onProperty rdf:resource="https://w3id.org/italia/onto/OP21/haAttoAdeguamentoContributivo"/>
                <owl:someValuesFrom rdf:resource="https://w3id.org/italia/onto/OP21/AttoAdeguamentoContributivo"/>
            </owl:Restriction>
        </owl:equivalentClass>
        <owl:equivalentClass>
            <owl:Restriction>
                <owl:onProperty rdf:resource="https://w3id.org/italia/onto/OP21/haOnereContributivo"/>
                <owl:someValuesFrom rdf:resource="http://www.w3.org/2002/07/owl#Thing"/>
            </owl:Restriction>
        </owl:equivalentClass>
        <rdfs:comment xml:lang="it">Sottoclasse di Pratica Adeguamento Contributivo che aggrega le pratiche per cui è stata emesso l&apos;Atto (di) Adeguamento Contributivo. È stato quindi comunicato l&apos;importo dell&apos;onere contributivo che il Richiedente dovrà versare all&apos;Istituto nonchè le modalità, ad esempio proponendo un piano di ammortamento, e i tempi di tale versamento. Le pratiche appartenenti a questa classe sono esigibili cioè possono essere soggette a pagamento da parte del Debitore. L&apos;esecuzione di almeno un pagamento implica l&apos;accettazione da parte del Richiedente dei termini indicati nell&apos;atto.</rdfs:comment>
        <rdfs:comment xml:lang="en">Subclass of Tax Adjustment Application which aggregates the applications for which the Tax Adjustment Deed was issued. The amount of the contribution fee that the Applicant will have to pay to the Institute was then communicated, as well as the methods and times for this payment. The applications belonging to this class are payable, i.e. they can be subject to payment by the Debtor. The execution of at least one payment implies acceptance by the Applicant of the terms indicated in the deed.</rdfs:comment>
        <rdfs:label xml:lang="en">Notified Amount of the Application Status</rdfs:label>
        <rdfs:label xml:lang="it">Stato Di Notificato Importo Di Pratica</rdfs:label>
    </owl:Class>



    <!-- https://w3id.org/italia/onto/OP21/StatoDiPagamentoRatealeInCorso -->

    <owl:Class rdf:about="https://w3id.org/italia/onto/OP21/StatoDiPagamentoRatealeInCorso">
        <rdfs:comment xml:lang="it">Sottoclasse di Pratica Adeguamento Contributivo che classifica le pratiche per cui è stato concordato un piano di ammortamento e i cui pagamenti sono regolari.</rdfs:comment>
        <rdfs:comment xml:lang="en">Subclass of Tax Adjustment Application which classifies the applications for which an amortization plan has been agreed upon and whose installments are regularly paid.</rdfs:comment>
        <rdfs:label xml:lang="en">Ongoing Installment Payment Status</rdfs:label>
        <rdfs:label xml:lang="it">Stato Di Pagamento Rateale In Corso</rdfs:label>
    </owl:Class>



    <!-- https://w3id.org/italia/onto/OP21/StatoDiPraticaDefinita -->

    <owl:Class rdf:about="https://w3id.org/italia/onto/OP21/StatoDiPraticaDefinita">
        <rdfs:comment xml:lang="it">Sottoclasse di Pratica Adeguamento Contributivo che classifica le pratiche di cui è stato saldato l&apos;onere dovuto. Rappresenta lo stato finale di una pratica.</rdfs:comment>
        <rdfs:comment xml:lang="en">Subclass of Tax Adjustment Application which classifies the applications whose costs have been paid in full. It is the final state of an application.</rdfs:comment>
        <rdfs:label xml:lang="en">Defined Application Status</rdfs:label>
        <rdfs:label xml:lang="it">Stato Di Pratica Definita</rdfs:label>
    </owl:Class>



    <!-- https://w3id.org/italia/onto/OP21/StatoInizialeDiPratica -->

    <owl:Class rdf:about="https://w3id.org/italia/onto/OP21/StatoInizialeDiPratica">
        <rdfs:comment xml:lang="it">Sottoclasse di Pratica Adeguamento Contributivo che classifica le pratiche istruite a fronte del ricevimento di una Domanda (di) Adeguamento Contributivo ma non ancora elaborate da parte delle Sede INPS. Rappresenta lo stato iniziale di una pratica.</rdfs:comment>
        <rdfs:comment xml:lang="en">Subclass of Tax Adjustment Application which classifies the applications for which a Tax Adjustment Application has been received but not yet handled by INPS office. It is the initial state of an application.</rdfs:comment>
        <rdfs:label xml:lang="en">Initial Application Status</rdfs:label>
        <rdfs:label xml:lang="it">Stato Iniziale Di Pratica</rdfs:label>
    </owl:Class>



    <!-- https://w3id.org/italia/onto/OP21/Superstite -->

    <owl:Class rdf:about="https://w3id.org/italia/onto/OP21/Superstite">
        <owl:equivalentClass>
            <owl:Restriction>
                <owl:onProperty rdf:resource="https://w3id.org/italia/onto/OP21/èSuperstite"/>
                <owl:someValuesFrom rdf:resource="http://www.w3.org/2002/07/owl#Thing"/>
            </owl:Restriction>
        </owl:equivalentClass>
        <owl:equivalentClass>
            <owl:Restriction>
                <owl:onProperty>
                    <rdf:Description>
                        <owl:inverseOf rdf:resource="https://w3id.org/italia/onto/OP21/haPagatoreOnere"/>
                    </rdf:Description>
                </owl:onProperty>
                <owl:someValuesFrom rdf:resource="http://www.w3.org/2002/07/owl#Thing"/>
            </owl:Restriction>
        </owl:equivalentClass>
        <rdfs:subClassOf rdf:resource="https://w3id.org/italia/onto/CPV/Alive"/>
        <owl:disjointWith>
            <owl:Class>
                <owl:intersectionOf rdf:parseType="Collection">
                    <rdf:Description rdf:about="https://w3id.org/italia/onto/CPV/Alive"/>
                    <rdf:Description rdf:about="https://w3id.org/italia/onto/OP21/TitolarePratica"/>
                </owl:intersectionOf>
            </owl:Class>
        </owl:disjointWith>
        <rdfs:comment xml:lang="it">Sottoclasse di Persona in Vita che, avendo un legame parentale con un Titolare Pratica deceduto, ha presentato domanda di riscatto, ricongiunzione o rendita per conto e in vece di detto Titolare; quindi, in questo caso, corrisponde al Richiedente. Per ciò, tale superstite si fa carico del pagamento degli eventuali oneri derivanti dall&apos;accoglimento della domanda e risulta legato alla Pratica derivante dalla domanda stessa in qualità di pagatore, ruolo quest&apos;ultimo che è assorbito da quello di Titolare qual ora quest&apos;ultimo sia in vita.</rdfs:comment>
        <rdfs:comment xml:lang="en">Subclass of Living Person who, having a parental relationship with a deceased Application Holder, has presented a redemption, reunion or income request on behalf of and in place of said Holder; therefore, in this case, it corresponds to the Applicant. For this reason, this survivor takes care of the payment of any charges deriving from the acceptance of the request and is linked to the Application deriving from the request itself as payer, the latter role being absorbed by that of Holder in case he is alive.</rdfs:comment>
        <rdfs:label xml:lang="it">Superstite</rdfs:label>
        <rdfs:label xml:lang="en">Survivor</rdfs:label>
    </owl:Class>



    <!-- https://w3id.org/italia/onto/OP21/TitolarePratica -->

    <owl:Class rdf:about="https://w3id.org/italia/onto/OP21/TitolarePratica">
        <owl:equivalentClass>
            <owl:Restriction>
                <owl:onProperty>
                    <rdf:Description>
                        <owl:inverseOf rdf:resource="https://w3id.org/italia/onto/OP21/haTitolarePratica"/>
                    </rdf:Description>
                </owl:onProperty>
                <owl:someValuesFrom rdf:resource="http://www.w3.org/2002/07/owl#Thing"/>
            </owl:Restriction>
        </owl:equivalentClass>
        <rdfs:subClassOf rdf:resource="https://w3id.org/italia/onto/CPV/Person"/>
        <rdfs:comment xml:lang="it">Sottoclasse di Persona (Fisica) che classifica le persone a cui, facendo seguito alla presentazione di idonea domanda, sono riconosciuti i requisiti per accedere alla facoltà di riscatto, ricongiunzione o rendita. Tali requisiti possono essere riconosciuti al Titolare anche se non più in vita. Il Titolare è obbligatoriamente legato ad almeno una Pratica. Nel caso il Titolare sia in vita, corrisponde al Richiedente.</rdfs:comment>
        <rdfs:comment xml:lang="en">Sub-class of Person (Physical) which classifies the people who, following the presentation of a suitable application, are recognized as having the requisites for accessing the option of redemption, reunion or income. These requirements can be recognized to the Holder even if no longer alive. The Holder is compulsorily linked to at least one Application. If the Owner is alive, it corresponds to the Applicant.</rdfs:comment>
        <rdfs:label xml:lang="en">Application Holder</rdfs:label>
        <rdfs:label xml:lang="it">Titolare Pratica</rdfs:label>
    </owl:Class>



    <!-- https://w3id.org/italia/onto/OP21/TrimestreDiAnno -->

    <owl:Class rdf:about="https://w3id.org/italia/onto/OP21/TrimestreDiAnno">
        <owl:equivalentClass>
            <owl:Restriction>
                <owl:onProperty>
                    <rdf:Description>
                        <owl:inverseOf rdf:resource="https://w3id.org/italia/onto/OP21/èMeseDelTrimestre"/>
                    </rdf:Description>
                </owl:onProperty>
                <owl:someValuesFrom rdf:resource="http://www.w3.org/2002/07/owl#Thing"/>
            </owl:Restriction>
        </owl:equivalentClass>
        <owl:equivalentClass>
            <owl:Restriction>
                <owl:onProperty rdf:resource="https://w3id.org/italia/onto/OP21/indiceTrimestre"/>
                <owl:someValuesFrom rdf:resource="http://www.w3.org/2000/01/rdf-schema#Literal"/>
            </owl:Restriction>
        </owl:equivalentClass>
        <rdfs:comment xml:lang="en">A quarter refers to one-fourth of a year (three months) and is typically expressed as Q1 for the first quarter, Q2 for the second quarter, and so forth (subclass of TI:TemporalEntity)</rdfs:comment>
        <rdfs:comment xml:lang="it">Periodo di tre mesi in cui è suddiviso un anno solare, tipicamente indicati con primo trimestre, secondo trimestre, e così via (sottoclasse di TI:TemporalEntity)</rdfs:comment>
        <rdfs:label xml:lang="en">Quarter</rdfs:label>
        <rdfs:label xml:lang="it">Trimestre Di Anno</rdfs:label>
    </owl:Class>



    <!-- https://w3id.org/italia/onto/RO/TimeIndexedRole -->

    <owl:Class rdf:about="https://w3id.org/italia/onto/RO/TimeIndexedRole">
        <owl:equivalentClass>
            <owl:Restriction>
                <owl:onProperty>
                    <rdf:Description>
                        <owl:inverseOf rdf:resource="https://w3id.org/italia/onto/RO/holdsRoleInTime"/>
                    </rdf:Description>
                </owl:onProperty>
                <owl:someValuesFrom rdf:resource="http://www.w3.org/2002/07/owl#Thing"/>
            </owl:Restriction>
        </owl:equivalentClass>
    </owl:Class>



    <!-- https://w3id.org/italia/onto/TI/TemporalEntity -->

    <owl:Class rdf:about="https://w3id.org/italia/onto/TI/TemporalEntity"/>



    <!-- https://w3id.org/italia/onto/TI/TimeIndexedEvent -->

    <owl:Class rdf:about="https://w3id.org/italia/onto/TI/TimeIndexedEvent">
        <rdfs:subClassOf>
            <owl:Restriction>
                <owl:onProperty rdf:resource="https://w3id.org/italia/onto/TI/atTime"/>
                <owl:someValuesFrom rdf:resource="https://w3id.org/italia/onto/TI/TimeInterval"/>
            </owl:Restriction>
        </rdfs:subClassOf>
    </owl:Class>



    <!-- https://w3id.org/italia/onto/TI/TimeInterval -->

    <owl:Class rdf:about="https://w3id.org/italia/onto/TI/TimeInterval">
        <rdfs:subClassOf>
            <owl:Restriction>
                <owl:onProperty>
                    <rdf:Description>
                        <owl:inverseOf rdf:resource="https://w3id.org/italia/onto/TI/hasTemporalEntity"/>
                    </rdf:Description>
                </owl:onProperty>
                <owl:someValuesFrom rdf:resource="https://w3id.org/italia/onto/RO/TimeIndexedRole"/>
            </owl:Restriction>
        </rdfs:subClassOf>
        <rdfs:subClassOf>
            <owl:Restriction>
                <owl:onProperty rdf:resource="https://w3id.org/italia/onto/TI/endTime"/>
                <owl:maxCardinality rdf:datatype="http://www.w3.org/2001/XMLSchema#nonNegativeInteger">1</owl:maxCardinality>
            </owl:Restriction>
        </rdfs:subClassOf>
        <rdfs:subClassOf>
            <owl:Restriction>
                <owl:onProperty rdf:resource="https://w3id.org/italia/onto/TI/startTime"/>
                <owl:maxCardinality rdf:datatype="http://www.w3.org/2001/XMLSchema#nonNegativeInteger">1</owl:maxCardinality>
            </owl:Restriction>
        </rdfs:subClassOf>
    </owl:Class>



    <!-- https://w3id.org/italia/onto/l0/Agent -->

    <owl:Class rdf:about="https://w3id.org/italia/onto/l0/Agent"/>



    <!-- https://w3id.org/italia/onto/l0/Collection -->

    <owl:Class rdf:about="https://w3id.org/italia/onto/l0/Collection"/>



    <!-- https://w3id.org/italia/onto/l0/Sequence -->

    <owl:Class rdf:about="https://w3id.org/italia/onto/l0/Sequence"/>



    <!--
    ///////////////////////////////////////////////////////////////////////////////////////
    //
    // Individuals
    //
    ///////////////////////////////////////////////////////////////////////////////////////
     -->




    <!-- https://w3id.org/italia/data/OP21/distribution/OP21-RDF-TURTLE -->

    <owl:NamedIndividual rdf:about="https://w3id.org/italia/data/OP21/distribution/OP21-RDF-TURTLE">
	    <rdf:type rdf:resource="http://dati.gov.it/onto/dcatapit/Distribution"/>
		<rdf:type rdf:resource="http://www.w3.org/ns/dcat#Distribution"/>
        <dct:description xml:lang="it">Questa è la distribuzione RDF/Turtle dell'ontologia INPS relativa a Riscatti, Ricongiunzioni, Rendite e Lavoratore Domestico</dct:description>
        <dct:description xml:lang="en">This is the distribution in RDF/Turtle of the INPS Ontology about Redemption, Aggregation, Life Annuities and Domestic Worker</dct:description>
        <dct:format rdf:resource="http://publications.europa.eu/resource/authority/file-type/RDF"/>
        <dct:license rdf:resource="http://creativecommons.org/licenses/by/4.0/"/>
        <dct:title xml:lang="it">Distribuzione RDF/Turtle dell'ontologia INPS - Procedura 21</dct:title>
        <dct:title xml:lang="en">RDF/Turtle distribution of the INPS ontology - 21 Procedure</dct:title>
        <dcat:accessURL rdf:resource="https://github.com/INPS-it/NDC/tree/main/assets/ontologies/OP21/latest"/>
        <dcat:downloadURL rdf:resource="https://raw.githubusercontent.com/INPS-it/NDC/main/assets/ontologies/OP21/latest/OP21.ttl"/>
    </owl:NamedIndividual>

<!-- https://w3id.org/italia/data/OP21/distribution/OP21-N-TRIPLES -->

    <owl:NamedIndividual rdf:about="https://w3id.org/italia/data/OP21/distribution/OP21-N-TRIPLES">
	    <rdf:type rdf:resource="http://dati.gov.it/onto/dcatapit/Distribution"/>
		<rdf:type rdf:resource="http://www.w3.org/ns/dcat#Distribution"/>
        <dct:description xml:lang="it">Questa è la distribuzione N-TRIPLES dell'ontologia INPS relativa a Riscatti, Ricongiunzioni, Rendite e Lavoratore Domestico</dct:description>
        <dct:description xml:lang="en">This is the distribution in N-TRIPLES of the INPS Ontology about Redemption, Aggregation, Life Annuities and Domestic Worker</dct:description>
        <dct:format rdf:resource="http://publications.europa.eu/resource/authority/file-type/RDF"/>
        <dct:license rdf:resource="http://creativecommons.org/licenses/by/4.0/"/>
        <dct:title xml:lang="it">Distribuzione N-TRIPLES dell'ontologia INPS - Procedura 21</dct:title>
        <dct:title xml:lang="en">N-TRIPLES distribution of the INPS ontology - 21 Procedure</dct:title>
        <dcat:accessURL rdf:resource="https://github.com/INPS-it/NDC/tree/main/assets/ontologies/OP21/latest"/>
        <dcat:downloadURL rdf:resource="https://raw.githubusercontent.com/INPS-it/NDC/main/assets/ontologies/OP21/latest/OP21.n3"/>
    </owl:NamedIndividual>

<!-- https://w3id.org/italia/data/OP21/distribution/OP21-RDF-XML -->

    <owl:NamedIndividual rdf:about="https://w3id.org/italia/data/OP21/distribution/OP21-RDF-XML">
	    <rdf:type rdf:resource="http://dati.gov.it/onto/dcatapit/Distribution"/>
		<rdf:type rdf:resource="http://www.w3.org/ns/dcat#Distribution"/>
        <dct:description xml:lang="it">Questa è la distribuzione RDF/XML dell'ontologia INPS relativa a Riscatti, Ricongiunzioni, Rendite e Lavoratore Domestico</dct:description>
        <dct:description xml:lang="en">This is the distribution in RDF/XML of the INPS Ontology about Redemption, Aggregation, Life Annuities and Domestic Worker</dct:description>
        <dct:format rdf:resource="http://publications.europa.eu/resource/authority/file-type/RDF"/>
        <dct:license rdf:resource="http://creativecommons.org/licenses/by/4.0/"/>
        <dct:title xml:lang="it">Distribuzione RDF/XML dell'ontologia INPS - Procedura 21</dct:title>
        <dct:title xml:lang="en">RDF/XML distribution of the INPS ontology - 21 Procedure</dct:title>
        <dcat:accessURL rdf:resource="https://github.com/INPS-it/NDC/tree/main/assets/ontologies/OP21/latest"/>
        <dcat:downloadURL rdf:resource="https://raw.githubusercontent.com/INPS-it/NDC/main/assets/ontologies/OP21/latest/OP21.owl"/>
    </owl:NamedIndividual>



    <!-- https://w3id.org/italia/data/OP21/organization/DirezioneCentraleTII -->

    <owl:NamedIndividual rdf:about="https://w3id.org/italia/data/OP21/organization/DirezioneCentraleTII">
		<rdf:type rdf:resource="http://dati.gov.it/onto/dcatapit#Organization"/>
		<rdf:type rdf:resource="http://www.w3.org/2006/vcard/ns#Organization"/>
		<rdf:type rdf:resource="http://www.w3.org/2006/vcard/ns#Kind"/>
        <vcard:fn>Direzione Centrale Tecnologia, Informatica e Innovazione</vcard:fn>
        <vcard:hasEmail rdf:resource="mailto:dc.tecnologiainformaticaeinnovazione@postacert.inps.gov.it"/>
    </owl:NamedIndividual>



    <!-- https://w3id.org/italia/data/OP21/organization/td -->

    <owl:NamedIndividual rdf:about="https://w3id.org/italia/data/OP21/organization/td">
        <rdf:type rdf:resource="http://dati.gov.it/onto/dcatapit#Agent"/>
        <rdf:type rdf:resource="http://xmlns.com/foaf/0.1/Agent"/>
		<dct:identifier>TD</dct:identifier>
        <foaf:name xml:lang="en">Digital Transformation Team</foaf:name>
        <foaf:name xml:lang="it">Team per la Trasformazione Digitale</foaf:name>
    </owl:NamedIndividual>

    <!-- https://w3id.org/italia/data/OP21/organization/inps -->

<owl:NamedIndividual rdf:about="https://w3id.org/italia/data/OP21/organization/inps">
        <rdf:type rdf:resource="http://dati.gov.it/onto/dcatapit#Agent"/>
        <rdf:type rdf:resource="http://xmlns.com/foaf/0.1/Agent"/>
		<dct:identifier>inps</dct:identifier>
        <foaf:name xml:lang="it">Istituto nazionale della previdenza sociale</foaf:name>
        <foaf:name xml:lang="en">National institute for Social Security</foaf:name>
    </owl:NamedIndividual>

	<!-- https://w3id.org/italia/data/OP21/organization/pagoPA -->

<owl:NamedIndividual rdf:about="https://w3id.org/italia/data/OP21/organization/pagoPA">
        <rdf:type rdf:resource="https://w3id.org/italia/data/OP21/SistemaDiPagamentoElettronicoAttivo"/>
        <rdf:type rdf:resource="http://dati.gov.it/onto/dcatapit#Agent"/>
        <rdf:type rdf:resource="http://xmlns.com/foaf/0.1/Agent"/>
		<dct:identifier>pagoPA</dct:identifier>
        <foaf:name xml:lang="it">Pago PA</foaf:name>
		<foaf:name xml:lang="en">Pago PA</foaf:name>
        <rdfs:comment xml:lang="en">PagoPA is an electronic payments system created to make any payment to the Public Administration easier, safer and more transparent. The platform enables citizens and businesses to make payments to public bodies in a standardized way, both online and offline, through participating Payment Service Providers (PSPs). PagoPA provides citizens with a reliable, efficient and personalized payment experience by allowing them to choose from multiple payment channels and instruments according to their habits, having complete visibility of the cost of the service in total transparency. In addition, pagoPA automatically updates the amount due and ensures with immediacy that the entity has correctly received the payment. PagoPA enables public administrations to collect money centrally and efficiently, offering automatic reporting and reconciliation systems with significant savings in resources, time and costs and ensuring better service to citizens.</rdfs:comment>
        <rdfs:comment xml:lang="it">PagoPA è il Sistema Di Pagamento Elettronico italiano per i pagamenti a favore della Pubblica Amministrazione, grazie al quale tutti i pagamenti effettuati da cittadini e imprese verso qualsiasi tipologia di Ente Pubblico avvengono in conformità a standard e regole definiti da AgID, semplificando e aumentando la qualità e la quantità dei servizi di pagamento offerti. Offre una modalità standardizzata di pagamento che si può utilizzare attraverso molti e diversificati strumenti e canali di pagamento, accessibili sia tramite il sito dell’Ente Creditore verso il quale occorre effettuare un pagamento, sia tramite gli sportelli fisici e virtuali messi a disposizione da numerosi PSP sia tramite il sito pagoPA. L’aspetto innovativo di questo approccio è rendere indipendente l’Ente Creditore dal PSP poiché l’intermediazione tra questi due soggetti è svolta da pagoPA senza la necessità di alcuna convenzione tra i primi due. Allo stesso tempo, offrendo pagoPA numerosi modalità e canali di pagamento consente all’utente di optare per quello di maggior convenienza, economica e/o logistica. È infatti l’utente debitore a scegliere il proprio PSP eventualmente corrispondendo a quest’ultimo una commissione per il servizio prestato. In breve, lo schema di pagamento tramite piattaforma pagoPA prevede la partecipazione: - della Pubblica Amministrazione o Gestore di Servizio Pubblico, in qualità di beneficiario del pagamento disposto dal cittadino/impresa; - del PSP del debitore, in qualità di soggetto che esegue l’addebito sul conto di quest’ultimo e che ordina l’accredito sul conto del PSP della Pubblica Amministrazione o del Gestore di Servizio Pubblico, già contrattualizzato con il contratto di tesoreria di quest’ultimo; In tale operatività, non sussistendo alcuna attività di incasso da parte di terzi e riversamento dal terzo al beneficiario, nessun soggetto si configura come agente contabile (fonte: AgID).</rdfs:comment>
    </owl:NamedIndividual>



    <!--
    ///////////////////////////////////////////////////////////////////////////////////////
    //
    // General axioms
    //
    ///////////////////////////////////////////////////////////////////////////////////////
     -->

    <owl:Class>
        <owl:intersectionOf rdf:parseType="Collection">
            <rdf:Description rdf:about="https://w3id.org/italia/onto/CPV/Dead"/>
            <rdf:Description rdf:about="https://w3id.org/italia/onto/OP21/TitolarePratica"/>
        </owl:intersectionOf>
        <owl:equivalentClass>
            <owl:Restriction>
                <owl:onProperty>
                    <rdf:Description>
                        <owl:inverseOf rdf:resource="https://w3id.org/italia/onto/OP21/èSuperstite"/>
                    </rdf:Description>
                </owl:onProperty>
                <owl:someValuesFrom rdf:resource="http://www.w3.org/2002/07/owl#Thing"/>
            </owl:Restriction>
        </owl:equivalentClass>
    </owl:Class>
    <owl:Class>
        <owl:unionOf rdf:parseType="Collection">
            <rdf:Description rdf:about="https://w3id.org/italia/onto/OP21/Superstite"/>
            <owl:Class>
                <owl:intersectionOf rdf:parseType="Collection">
                    <rdf:Description rdf:about="https://w3id.org/italia/onto/CPV/Alive"/>
                    <rdf:Description rdf:about="https://w3id.org/italia/onto/OP21/TitolarePratica"/>
                </owl:intersectionOf>
            </owl:Class>
        </owl:unionOf>
        <owl:equivalentClass>
            <owl:Restriction>
                <owl:onProperty rdf:resource="https://w3id.org/italia/onto/RO/holdsRoleInTime"/>
                <owl:someValuesFrom rdf:resource="https://w3id.org/italia/onto/OP21/RichiedenteAdeguamentoContributivo"/>
            </owl:Restriction>
        </owl:equivalentClass>
    </owl:Class>
    <owl:Class>
        <owl:unionOf rdf:parseType="Collection">
            <rdf:Description rdf:about="https://w3id.org/italia/onto/COV/Organization"/>
            <rdf:Description rdf:about="https://w3id.org/italia/onto/CPV/Person"/>
        </owl:unionOf>
        <rdfs:subClassOf rdf:resource="https://w3id.org/italia/onto/l0/Agent"/>
    </owl:Class>
    <owl:Class>
        <owl:unionOf rdf:parseType="Collection">
            <rdf:Description rdf:about="https://w3id.org/italia/onto/OP21/BollettinoDiPagamentoContributo"/>
            <rdf:Description rdf:about="https://w3id.org/italia/onto/OP21/BollettinoDiPagamentoRata"/>
            <rdf:Description rdf:about="https://w3id.org/italia/onto/OP21/BollettinoDiPagamentoUnico"/>
        </owl:unionOf>
        <rdfs:subClassOf rdf:resource="https://w3id.org/italia/onto/OP21/BollettinoDiPagamento"/>
    </owl:Class>
    <owl:Class>
        <owl:unionOf rdf:parseType="Collection">
            <rdf:Description rdf:about="https://w3id.org/italia/onto/OP21/ContributoTrimestraleOrdinario"/>
            <rdf:Description rdf:about="https://w3id.org/italia/onto/OP21/OnereContributivo"/>
            <rdf:Description rdf:about="https://w3id.org/italia/onto/OP21/RataDiOnereContributivo"/>
        </owl:unionOf>
        <rdfs:subClassOf rdf:resource="https://w3id.org/italia/onto/OP21/Finalità"/>
    </owl:Class>
    <owl:Class>
        <owl:unionOf rdf:parseType="Collection">
            <rdf:Description rdf:about="https://w3id.org/italia/onto/OP21/Correntista"/>
            <rdf:Description rdf:about="https://w3id.org/italia/onto/OP21/DatoreDiLavoroDomestico"/>
        </owl:unionOf>
        <rdfs:subClassOf rdf:resource="https://w3id.org/italia/onto/OP21/RuoloDiAgente"/>
    </owl:Class>
    <owl:Class>
        <owl:unionOf rdf:parseType="Collection">
            <rdf:Description rdf:about="https://w3id.org/italia/onto/OP21/CreditoreMandato"/>
            <rdf:Description rdf:about="https://w3id.org/italia/onto/OP21/DebitoreMandato"/>
        </owl:unionOf>
        <rdfs:subClassOf rdf:resource="https://w3id.org/italia/onto/OP21/Correntista"/>
    </owl:Class>
    <owl:Class>
        <owl:unionOf rdf:parseType="Collection">
            <rdf:Description rdf:about="https://w3id.org/italia/onto/OP21/DatoreDiLavoroDomestico"/>
            <rdf:Description rdf:about="https://w3id.org/italia/onto/OP21/RichiedenteAdeguamentoContributivo"/>
        </owl:unionOf>
        <rdfs:subClassOf rdf:resource="https://w3id.org/italia/onto/OP21/Pagatore"/>
    </owl:Class>
    <owl:Class>
        <owl:unionOf rdf:parseType="Collection">
            <rdf:Description rdf:about="https://w3id.org/italia/onto/OP21/EsitoPagamento"/>
            <rdf:Description rdf:about="https://w3id.org/italia/onto/OP21/MandatoSDD"/>
            <rdf:Description rdf:about="https://w3id.org/italia/onto/OP21/MovimentoDiDenaro"/>
            <rdf:Description rdf:about="https://w3id.org/italia/onto/OP21/PraticaAdeguamentoContributivo"/>
            <rdf:Description rdf:about="https://w3id.org/italia/onto/OP21/RapportoDiLavoroDomestico"/>
            <rdf:Description rdf:about="https://w3id.org/italia/onto/OP21/SessionePagamentoElettronico"/>
        </owl:unionOf>
        <rdfs:subClassOf rdf:resource="https://w3id.org/italia/onto/TI/TimeIndexedEvent"/>
    </owl:Class>
    <owl:Class>
        <owl:unionOf rdf:parseType="Collection">
            <rdf:Description rdf:about="https://w3id.org/italia/onto/OP21/LavoratoreDomestico"/>
            <rdf:Description rdf:about="https://w3id.org/italia/onto/OP21/RichiedenteAdeguamentoContributivo"/>
        </owl:unionOf>
        <rdfs:subClassOf rdf:resource="https://w3id.org/italia/onto/OP21/RuoloDiPersonaViva"/>
    </owl:Class>
    <owl:Class>
        <owl:unionOf rdf:parseType="Collection">
            <rdf:Description rdf:about="https://w3id.org/italia/onto/OP21/MandatoSDDAttivo"/>
            <rdf:Description rdf:about="https://w3id.org/italia/onto/OP21/RID"/>
        </owl:unionOf>
        <rdfs:subClassOf>
            <owl:Restriction>
                <owl:onProperty rdf:resource="https://w3id.org/italia/onto/OP21/prenotaPagamento"/>
                <owl:someValuesFrom rdf:resource="http://www.w3.org/2002/07/owl#Thing"/>
            </owl:Restriction>
        </rdfs:subClassOf>
    </owl:Class>
    <owl:Class>
        <owl:unionOf rdf:parseType="Collection">
            <rdf:Description rdf:about="https://w3id.org/italia/onto/OP21/MeseDiTrimestre"/>
            <rdf:Description rdf:about="https://w3id.org/italia/onto/OP21/SettimanaDelMese"/>
            <rdf:Description rdf:about="https://w3id.org/italia/onto/OP21/TrimestreDiAnno"/>
        </owl:unionOf>
        <rdfs:subClassOf rdf:resource="https://w3id.org/italia/onto/TI/TemporalEntity"/>
    </owl:Class>
    <owl:Class>
        <owl:unionOf rdf:parseType="Collection">
            <rdf:Description rdf:about="https://w3id.org/italia/onto/OP21/OrganizzazioneDiAssistenza"/>
            <rdf:Description rdf:about="https://w3id.org/italia/onto/OP21/PrestatoreDiServiziDiPagamento"/>
        </owl:unionOf>
        <rdfs:subClassOf rdf:resource="https://w3id.org/italia/onto/COV/Organization"/>
    </owl:Class>
    <owl:Class>
        <owl:unionOf rdf:parseType="Collection">
            <rdf:Description rdf:about="https://w3id.org/italia/onto/OP21/PraticaDiRendita"/>
            <rdf:Description rdf:about="https://w3id.org/italia/onto/OP21/PraticaDiRicongiunzione"/>
            <rdf:Description rdf:about="https://w3id.org/italia/onto/OP21/PraticaDiRiscatto"/>
        </owl:unionOf>
        <rdfs:subClassOf rdf:resource="https://w3id.org/italia/onto/OP21/PraticaAdeguamentoContributivo"/>
    </owl:Class>
    <owl:Class>
        <owl:unionOf rdf:parseType="Collection">
            <rdf:Description rdf:about="https://w3id.org/italia/onto/OP21/StatoDiAccreditoParzialeDiPratica"/>
            <rdf:Description rdf:about="https://w3id.org/italia/onto/OP21/StatoDiNotificatoImportoDiPratica"/>
            <rdf:Description rdf:about="https://w3id.org/italia/onto/OP21/StatoDiPagamentoRatealeInCorso"/>
            <rdf:Description rdf:about="https://w3id.org/italia/onto/OP21/StatoDiPraticaDefinita"/>
            <rdf:Description rdf:about="https://w3id.org/italia/onto/OP21/StatoInizialeDiPratica"/>
        </owl:unionOf>
        <rdfs:subClassOf rdf:resource="https://w3id.org/italia/onto/OP21/PraticaAdeguamentoContributivo"/>
    </owl:Class>
    <owl:Restriction>
        <owl:onProperty>
            <rdf:Description>
                <owl:inverseOf rdf:resource="https://w3id.org/italia/onto/CLV/hasAddressComponent"/>
            </rdf:Description>
        </owl:onProperty>
        <owl:someValuesFrom>
            <owl:Restriction>
                <owl:onProperty>
                    <rdf:Description>
                        <owl:inverseOf rdf:resource="https://w3id.org/italia/onto/CLV/hasPrimaryAddress"/>
                    </rdf:Description>
                </owl:onProperty>
                <owl:someValuesFrom rdf:resource="https://w3id.org/italia/onto/COV/Organization"/>
            </owl:Restriction>
        </owl:someValuesFrom>
        <rdfs:subClassOf>
            <owl:Restriction>
                <owl:onProperty>
                    <rdf:Description>
                        <owl:inverseOf rdf:resource="https://w3id.org/italia/onto/CLV/hasAddressComponent"/>
                    </rdf:Description>
                </owl:onProperty>
                <owl:someValuesFrom>
                    <owl:Restriction>
                        <owl:onProperty>
                            <rdf:Description>
                                <owl:inverseOf rdf:resource="https://w3id.org/italia/onto/CLV/hasAddress"/>
                            </rdf:Description>
                        </owl:onProperty>
                        <owl:someValuesFrom>
                            <owl:Restriction>
                                <owl:onProperty>
                                    <rdf:Description>
                                        <owl:inverseOf rdf:resource="https://w3id.org/italia/onto/OP21/haSedeINPS"/>
                                    </rdf:Description>
                                </owl:onProperty>
                                <owl:someValuesFrom rdf:resource="http://www.w3.org/2002/07/owl#Thing"/>
                            </owl:Restriction>
                        </owl:someValuesFrom>
                    </owl:Restriction>
                </owl:someValuesFrom>
            </owl:Restriction>
        </rdfs:subClassOf>
    </owl:Restriction>
    <owl:Restriction>
        <owl:onProperty>
            <rdf:Description>
                <owl:inverseOf rdf:resource="https://w3id.org/italia/onto/CLV/hasAddressComponent"/>
            </rdf:Description>
        </owl:onProperty>
        <owl:someValuesFrom>
            <owl:Restriction>
                <owl:onProperty>
                    <rdf:Description>
                        <owl:inverseOf rdf:resource="https://w3id.org/italia/onto/CPV/hasCurrentResidence"/>
                    </rdf:Description>
                </owl:onProperty>
                <owl:someValuesFrom rdf:resource="https://w3id.org/italia/onto/CPV/Alive"/>
            </owl:Restriction>
        </owl:someValuesFrom>
        <rdfs:subClassOf>
            <owl:Restriction>
                <owl:onProperty>
                    <rdf:Description>
                        <owl:inverseOf rdf:resource="https://w3id.org/italia/onto/CLV/hasAddressComponent"/>
                    </rdf:Description>
                </owl:onProperty>
                <owl:someValuesFrom>
                    <owl:Restriction>
                        <owl:onProperty>
                            <rdf:Description>
                                <owl:inverseOf rdf:resource="https://w3id.org/italia/onto/CLV/hasAddress"/>
                            </rdf:Description>
                        </owl:onProperty>
                        <owl:someValuesFrom>
                            <owl:Restriction>
                                <owl:onProperty>
                                    <rdf:Description>
                                        <owl:inverseOf rdf:resource="https://w3id.org/italia/onto/OP21/haSedeINPS"/>
                                    </rdf:Description>
                                </owl:onProperty>
                                <owl:someValuesFrom rdf:resource="http://www.w3.org/2002/07/owl#Thing"/>
                            </owl:Restriction>
                        </owl:someValuesFrom>
                    </owl:Restriction>
                </owl:someValuesFrom>
            </owl:Restriction>
        </rdfs:subClassOf>
    </owl:Restriction>
    <rdf:Description>
        <rdf:type rdf:resource="http://www.w3.org/2002/07/owl#AllDisjointClasses"/>
        <owl:members rdf:parseType="Collection">
            <rdf:Description rdf:about="https://w3id.org/italia/onto/OP21/BollettinoDiPagamentoContributo"/>
            <rdf:Description rdf:about="https://w3id.org/italia/onto/OP21/BollettinoDiPagamentoRata"/>
            <rdf:Description rdf:about="https://w3id.org/italia/onto/OP21/BollettinoDiPagamentoUnico"/>
        </owl:members>
    </rdf:Description>
    <rdf:Description>
        <rdf:type rdf:resource="http://www.w3.org/2002/07/owl#AllDisjointClasses"/>
        <owl:members rdf:parseType="Collection">
            <rdf:Description rdf:about="https://w3id.org/italia/onto/OP21/ContributoTrimestraleOrdinario"/>
            <rdf:Description rdf:about="https://w3id.org/italia/onto/OP21/OnereContributivo"/>
            <rdf:Description rdf:about="https://w3id.org/italia/onto/OP21/RataDiOnereContributivo"/>
        </owl:members>
    </rdf:Description>
    <rdf:Description>
        <rdf:type rdf:resource="http://www.w3.org/2002/07/owl#AllDisjointClasses"/>
        <owl:members rdf:parseType="Collection">
            <rdf:Description rdf:about="https://w3id.org/italia/onto/OP21/EsitoPagamento"/>
            <rdf:Description rdf:about="https://w3id.org/italia/onto/OP21/MandatoSDD"/>
            <rdf:Description rdf:about="https://w3id.org/italia/onto/OP21/MovimentoDiDenaro"/>
            <rdf:Description rdf:about="https://w3id.org/italia/onto/OP21/PraticaAdeguamentoContributivo"/>
            <rdf:Description rdf:about="https://w3id.org/italia/onto/OP21/RapportoDiLavoroDomestico"/>
            <rdf:Description rdf:about="https://w3id.org/italia/onto/OP21/SessionePagamentoElettronico"/>
        </owl:members>
    </rdf:Description>
    <rdf:Description>
        <rdf:type rdf:resource="http://www.w3.org/2002/07/owl#AllDisjointClasses"/>
        <owl:members rdf:parseType="Collection">
            <rdf:Description rdf:about="https://w3id.org/italia/onto/OP21/MandatoSDDAttivo"/>
            <rdf:Description rdf:about="https://w3id.org/italia/onto/OP21/MandatoSDDNonAttivabile"/>
            <rdf:Description rdf:about="https://w3id.org/italia/onto/OP21/MandatoSDDRevocato"/>
            <rdf:Description rdf:about="https://w3id.org/italia/onto/OP21/MandatoSDDRichiedibile"/>
            <rdf:Description rdf:about="https://w3id.org/italia/onto/OP21/MandatoSDDRichiesto"/>
        </owl:members>
    </rdf:Description>
    <rdf:Description>
        <rdf:type rdf:resource="http://www.w3.org/2002/07/owl#AllDisjointClasses"/>
        <owl:members rdf:parseType="Collection">
            <rdf:Description rdf:about="https://w3id.org/italia/onto/OP21/MeseDiTrimestre"/>
            <rdf:Description rdf:about="https://w3id.org/italia/onto/OP21/SettimanaDelMese"/>
            <rdf:Description rdf:about="https://w3id.org/italia/onto/OP21/TrimestreDiAnno"/>
        </owl:members>
    </rdf:Description>
    <rdf:Description>
        <rdf:type rdf:resource="http://www.w3.org/2002/07/owl#AllDisjointClasses"/>
        <owl:members rdf:parseType="Collection">
            <rdf:Description rdf:about="https://w3id.org/italia/onto/OP21/PraticaDiRendita"/>
            <rdf:Description rdf:about="https://w3id.org/italia/onto/OP21/PraticaDiRicongiunzione"/>
            <rdf:Description rdf:about="https://w3id.org/italia/onto/OP21/PraticaDiRiscatto"/>
        </owl:members>
    </rdf:Description>
    <rdf:Description>
        <rdf:type rdf:resource="http://www.w3.org/2002/07/owl#AllDisjointClasses"/>
        <owl:members rdf:parseType="Collection">
            <rdf:Description rdf:about="https://w3id.org/italia/onto/OP21/StatoDiAccreditoParzialeDiPratica"/>
            <rdf:Description rdf:about="https://w3id.org/italia/onto/OP21/StatoDiNotificatoImportoDiPratica"/>
            <rdf:Description rdf:about="https://w3id.org/italia/onto/OP21/StatoDiPagamentoRatealeInCorso"/>
            <rdf:Description rdf:about="https://w3id.org/italia/onto/OP21/StatoDiPraticaDefinita"/>
            <rdf:Description rdf:about="https://w3id.org/italia/onto/OP21/StatoInizialeDiPratica"/>
        </owl:members>
    </rdf:Description>
</rdf:RDF>



<!-- Generated by the OWL API (version 2.4) https://github.com/owlcs/owlapi -->

